<?xml version="1.0" encoding="utf-8" ?>
<rdf:RDF xmlns:rdf="http://www.w3.org/1999/02/22-rdf-syntax-ns#"
  xmlns:skos="http://www.w3.org/2004/02/skos/core#">

  <skos:Concept rdf:about="http://data.europeana.eu/concept/music/genre/Music">
    <skos:prefLabel xml:lang="en">Music</skos:prefLabel>
    <skos:closeMatch rdf:resource="http://rdf.freebase.com/m.04rlf"/>
    <skos:definition xml:lang="en">Music is an art form whose medium is sound and silence. Its
      common elements are pitch, rhythm, dynamics, and the sonic qualities of timbre and texture.
      The word derives from Greek μουσική. The creation, performance, significance, and even the
      definition of music vary according to culture and social context. Music ranges from strictly
      organized compositions, through improvisational music to aleatoric forms. Music can be divided
      into genres and subgenres, although the dividing lines and relationships between music genres
      are often subtle, sometimes open to personal interpretation, and occasionally controversial.
      Within the arts, music may be classified as a performing art, a fine art, and auditory art. It
      may also be divided among art music and folk music. There is also a strong connection between
      music and mathematics. Music may be played and heard live, may be part of a dramatic work or
      film, or may be recorded. To many people in many cultures, music is an important part of their
      way of life. Ancient Greek and Indian philosophers defined music as tones ordered horizontally
      as melodies and vertically as harmonies.</skos:definition>
    <skos:inScheme rdf:resource="http://data.europeana.eu/concept/music/genre/Music_Genre_Scheme"/>
  </skos:Concept>

  <skos:ConceptScheme rdf:about="http://data.europeana.eu/concept/music/genre/Music_Genre_Scheme">
    <skos:prefLabel xml:lang="en">Music Genre Scheme</skos:prefLabel>
  </skos:ConceptScheme>

  <skos:Concept
    rdf:about="http://data.europeana.eu/concept/music/genre/African_popular_music_fusions">
    <skos:prefLabel xml:lang="en">Afropop fusions</skos:prefLabel>
    <skos:closeMatch rdf:resource="http://rdf.freebase.com/ns/m.02p4l6s"/>
    <skos:broader rdf:resource="http://data.europeana.eu/concept/music/genre/Folk_music_fusions"/>
    <skos:definition xml:lang="en">Fusion genres based on African popular music</skos:definition>
    <skos:broadMatch rdf:resource="http://dbpedia.org/resource/African_popular_music"/>
    <skos:inScheme rdf:resource="http://data.europeana.eu/concept/music/genre/Music_Genre_Scheme"/>
  </skos:Concept>

  <skos:Concept rdf:about="http://data.europeana.eu/concept/music/genre/Asian_music_pop">
    <skos:prefLabel xml:lang="en">Asian pop</skos:prefLabel>
    <skos:closeMatch rdf:resource="http://rdf.freebase.com/ns/m.028sqc"/>
    <skos:broader rdf:resource="http://data.europeana.eu/concept/music/genre/Popular_music"/>
    <skos:definition xml:lang="en">Popular music Asia including all asian regions</skos:definition>
    <skos:broadMatch rdf:resource="http://dbpedia.org/resource/Asian_music#pop"/>
    <skos:inScheme rdf:resource="http://data.europeana.eu/concept/music/genre/Music_Genre_Scheme"/>
  </skos:Concept>

  <skos:Concept rdf:about="http://data.europeana.eu/concept/music/genre/Alternative_rock_fusions">
    <skos:prefLabel xml:lang="en">Alternative rock fusions</skos:prefLabel>
    <skos:broader rdf:resource="http://data.europeana.eu/concept/music/genre/Rock_music_fusions"/>
    <skos:definition xml:lang="en">Fusion genres based on alternative rock music</skos:definition>
    <skos:broadMatch rdf:resource="http://dbpedia.org/resource/Alternative_rock"/>
    <skos:inScheme rdf:resource="http://data.europeana.eu/concept/music/genre/Music_Genre_Scheme"/>
  </skos:Concept>

  <skos:Concept rdf:about="http://data.europeana.eu/concept/music/genre/Blues_fusions">
    <skos:prefLabel xml:lang="en">Blues fusions</skos:prefLabel>
    <skos:broader rdf:resource="http://data.europeana.eu/concept/music/genre/Fusion_(music)_fusions"/>
    <skos:definition xml:lang="en">Fusion genres based on Blues</skos:definition>
    <skos:broadMatch rdf:resource="http://dbpedia.org/resource/Blues"/>
    <skos:inScheme rdf:resource="http://data.europeana.eu/concept/music/genre/Music_Genre_Scheme"/>
  </skos:Concept>

  <skos:Concept rdf:about="http://data.europeana.eu/concept/music/genre/Country_music_fusions">
    <skos:prefLabel xml:lang="en">Country music fusions</skos:prefLabel>
    <skos:broader rdf:resource="http://data.europeana.eu/concept/music/genre/Fusion_(music)_fusions"/>
    <skos:definition xml:lang="en">Fusion genres based on country music</skos:definition>
    <skos:broadMatch rdf:resource="http://dbpedia.org/resource/Country_music"/>
    <skos:inScheme rdf:resource="http://data.europeana.eu/concept/music/genre/Music_Genre_Scheme"/>
  </skos:Concept>

  <skos:Concept rdf:about="http://data.europeana.eu/concept/music/genre/Electronic_music_fusions">
    <skos:prefLabel xml:lang="en">Electronic music fusions</skos:prefLabel>
    <skos:broader rdf:resource="http://data.europeana.eu/concept/music/genre/Fusion_(music)_fusions"/>
    <skos:definition xml:lang="en">Fusion genres based on electronic music</skos:definition>
    <skos:broadMatch
      rdf:resource="http://data.europeana.eu/concept/music/genre/http%3A%2F%2Fdbpedia.org%2Fresource%2FElectronic+music"/>
    <skos:inScheme rdf:resource="http://data.europeana.eu/concept/music/genre/Music_Genre_Scheme"/>
  </skos:Concept>

  <skos:Concept rdf:about="http://data.europeana.eu/concept/music/genre/Electronic_rock_fusions">
    <skos:prefLabel xml:lang="en">Electronic rock fusions</skos:prefLabel>
    <skos:broader rdf:resource="http://data.europeana.eu/concept/music/genre/Rock_music_fusions"/>
    <skos:definition xml:lang="en">Fusion genres based on electronic rock music</skos:definition>
    <skos:broadMatch rdf:resource="http://dbpedia.org/resource/Electronic_rock"/>
    <skos:inScheme rdf:resource="http://data.europeana.eu/concept/music/genre/Music_Genre_Scheme"/>
  </skos:Concept>

  <skos:Concept rdf:about="http://data.europeana.eu/concept/music/genre/Folk_music_fusions">
    <skos:prefLabel xml:lang="en">Folk music fusions</skos:prefLabel>
    <skos:broader rdf:resource="http://data.europeana.eu/concept/music/genre/Fusion_(music)_fusions"/>
    <skos:definition xml:lang="en">Fusion genres based on folk music</skos:definition>
    <skos:broadMatch rdf:resource="http://dbpedia.org/resource/Folk_music"/>
    <skos:inScheme rdf:resource="http://data.europeana.eu/concept/music/genre/Music_Genre_Scheme"/>
  </skos:Concept>

  <skos:Concept rdf:about="http://data.europeana.eu/concept/music/genre/Heavy_metal_music_fusions">
    <skos:prefLabel xml:lang="en">Heavy metal fusions</skos:prefLabel>
    <skos:broader rdf:resource="http://data.europeana.eu/concept/music/genre/Rock_music_fusions"/>
    <skos:definition xml:lang="en">Fusion genres based on heavy metal music</skos:definition>
    <skos:broadMatch rdf:resource="http://dbpedia.org/resource/Heavy_metal_music"/>
    <skos:inScheme rdf:resource="http://data.europeana.eu/concept/music/genre/Music_Genre_Scheme"/>
  </skos:Concept>

  <skos:Concept rdf:about="http://data.europeana.eu/concept/music/genre/Hip_hop_music_fusions">
    <skos:prefLabel xml:lang="en">Hip hop fusions</skos:prefLabel>
    <skos:broader
      rdf:resource="http://data.europeana.eu/concept/music/genre/Electronic_music_fusions"/>
    <skos:definition xml:lang="en">Fusion genres based on hip hop music</skos:definition>
    <skos:broadMatch rdf:resource="http://dbpedia.org/resource/Hip_hop_music"/>
    <skos:inScheme rdf:resource="http://data.europeana.eu/concept/music/genre/Music_Genre_Scheme"/>
  </skos:Concept>

  <skos:Concept rdf:about="http://data.europeana.eu/concept/music/genre/House_music_fusions">
    <skos:prefLabel xml:lang="en">House fusions</skos:prefLabel>
    <skos:broader
      rdf:resource="http://data.europeana.eu/concept/music/genre/Electronic_music_fusions"/>
    <skos:definition xml:lang="en">Fusion genres based on house music</skos:definition>
    <skos:broadMatch rdf:resource="http://dbpedia.org/resource/House_music"/>
    <skos:inScheme rdf:resource="http://data.europeana.eu/concept/music/genre/Music_Genre_Scheme"/>
  </skos:Concept>

  <skos:Concept rdf:about="http://data.europeana.eu/concept/music/genre/Jazz_fusions">
    <skos:prefLabel xml:lang="en">Jazz music fusions</skos:prefLabel>
    <skos:broader rdf:resource="http://data.europeana.eu/concept/music/genre/Fusion_(music)_fusions"/>
    <skos:definition xml:lang="en">Fusion genres based on jazz music</skos:definition>
    <skos:broadMatch rdf:resource="http://dbpedia.org/resource/Jazz"/>
    <skos:inScheme rdf:resource="http://data.europeana.eu/concept/music/genre/Music_Genre_Scheme"/>
  </skos:Concept>

  <skos:Concept rdf:about="http://data.europeana.eu/concept/music/genre/Pop_music_fusions">
    <skos:prefLabel xml:lang="en">Pop fusions</skos:prefLabel>
    <skos:broader rdf:resource="http://data.europeana.eu/concept/music/genre/Fusion_(music)_fusions"/>
    <skos:definition xml:lang="en">Fusion genres based on pop music</skos:definition>
    <skos:broadMatch rdf:resource="http://dbpedia.org/resource/Pop_music"/>
    <skos:inScheme rdf:resource="http://data.europeana.eu/concept/music/genre/Music_Genre_Scheme"/>
  </skos:Concept>

  <skos:Concept rdf:about="http://data.europeana.eu/concept/music/genre/Punk_rock_fusions">
    <skos:prefLabel xml:lang="en">Punk fusions</skos:prefLabel>
    <skos:broader rdf:resource="http://data.europeana.eu/concept/music/genre/Rock_music_fusions"/>
    <skos:definition xml:lang="en">Fusion genres based on punk rock music</skos:definition>
    <skos:broadMatch rdf:resource="http://dbpedia.org/resource/Punk_rock"/>
    <skos:inScheme rdf:resource="http://data.europeana.eu/concept/music/genre/Music_Genre_Scheme"/>
  </skos:Concept>

  <skos:Concept rdf:about="http://data.europeana.eu/concept/music/genre/Rock_music_fusions">
    <skos:prefLabel xml:lang="en">Rock fusions</skos:prefLabel>
    <skos:broader rdf:resource="http://data.europeana.eu/concept/music/genre/Fusion_(music)_fusions"/>
    <skos:definition xml:lang="en">Fusion genres based on rock music</skos:definition>
    <skos:broadMatch rdf:resource="http://dbpedia.org/resource/Rock_music"/>
    <skos:inScheme rdf:resource="http://data.europeana.eu/concept/music/genre/Music_Genre_Scheme"/>
  </skos:Concept>

  <skos:Concept rdf:about="http://data.europeana.eu/concept/music/genre/Techno_fusions">
    <skos:prefLabel xml:lang="en">Techno fusions</skos:prefLabel>
    <skos:broader
      rdf:resource="http://data.europeana.eu/concept/music/genre/Electronic_music_fusions"/>
    <skos:definition xml:lang="en">Fusion genres based on techno music</skos:definition>
    <skos:broadMatch rdf:resource="http://dbpedia.org/resource/Techno"/>
    <skos:inScheme rdf:resource="http://data.europeana.eu/concept/music/genre/Music_Genre_Scheme"/>
  </skos:Concept>

  <skos:Concept rdf:about="http://data.europeana.eu/concept/music/genre/Martial_music">
    <skos:prefLabel xml:lang="en">Military music</skos:prefLabel>
    <skos:prefLabel xml:lang="fi">Sotilasmusiikki</skos:prefLabel>
    <skos:prefLabel xml:lang="de">Martial Industrial</skos:prefLabel>
    <skos:prefLabel xml:lang="ru">Военная музыка</skos:prefLabel>
    <skos:prefLabel xml:lang="sr">Војна музика</skos:prefLabel>
    <skos:prefLabel xml:lang="sv">Martial Industrial</skos:prefLabel>
    <skos:closeMatch rdf:resource="http://rdf.freebase.com/ns/m.075bdw"/>
    <skos:broader rdf:resource="http://data.europeana.eu/concept/music/genre/Music"/>
    <skos:definition xml:lang="en">Martial music or military music is a specific genre of music
      intended for use in military settings. Much of the military music has been composed to
      announce military events as with bugle calls and fanfares, or accompany marching formations
      with drum cadences, or mark special occasions as by military bands. However, music has been
      employed in battle for centuries, sometimes to intimidate the enemy and other times to
      encourage combatants, or to assist in organization and timing of actions in warfare. Depending
      on the culture, a variety of percussion and musical instruments have been used, such as drums,
      fifes, bugles, trumpets or other horns, bagpipes, triangles, cymbals, as well as larger
      military bands or full orchestras. Although some martial music has been composed in written
      form, other music has been developed or taught by ear, such as bugle calls or drum cadences,
      relying on group memory to coordinate the sounds.</skos:definition>
    <skos:exactMatch xml:lang="en">http://dbpedia.org/resource/Martial_music</skos:exactMatch>
    <skos:inScheme rdf:resource="http://data.europeana.eu/concept/music/genre/Music_Genre_Scheme"/>
    <skos:altLabel xml:lang="en">Martial music</skos:altLabel>
  </skos:Concept>

  <skos:Concept rdf:about="http://data.europeana.eu/concept/music/genre/Childrens_music">
    <skos:prefLabel xml:lang="en">Children's music</skos:prefLabel>
    <skos:prefLabel xml:lang="bg">Детска песен</skos:prefLabel>
    <skos:prefLabel xml:lang="da">Børnemusik</skos:prefLabel>
    <skos:prefLabel xml:lang="fr">Musique pour enfants</skos:prefLabel>
    <skos:prefLabel xml:lang="it">Musica per bambini</skos:prefLabel>
    <skos:prefLabel xml:lang="pt">Música para crianças</skos:prefLabel>
    <skos:prefLabel xml:lang="ru">Детские пластинки</skos:prefLabel>
    <skos:prefLabel xml:lang="vi">Nhạc thiếu nhi</skos:prefLabel>
    <skos:closeMatch rdf:resource="http://rdf.freebase.com/ns/m.05fw6t"/>
    <skos:broader rdf:resource="http://data.europeana.eu/concept/music/genre/Music"/>
    <skos:definition xml:lang="en">Children's music is music composed and performed for children by
      adults. In European-influenced contexts this means music, usually songs, written specifically
      for a juvenile audience. The composers are usually adults. Children's music has historically
      held both entertainment and educational functions. Children's music is often designed to
      provide an entertaining means of teaching children about their culture, other cultures, good
      behavior, facts and skills. Many are folk songs, but there is a whole genre of educational
      music that has become increasingly popular.</skos:definition>
    <skos:exactMatch xml:lang="en">http://dbpedia.org/resource/Children's_music</skos:exactMatch>
    <skos:inScheme rdf:resource="http://data.europeana.eu/concept/music/genre/Music_Genre_Scheme"/>
    <skos:altLabel xml:lang="en">Children's music</skos:altLabel>
  </skos:Concept>

  <skos:Concept rdf:about="http://data.europeana.eu/concept/music/genre/Art_music">
    <skos:prefLabel xml:lang="en">Art music</skos:prefLabel>
    <skos:prefLabel xml:lang="ca">Música culta</skos:prefLabel>
    <skos:prefLabel xml:lang="da">Kunstmusik</skos:prefLabel>
    <skos:prefLabel xml:lang="nl">Kunstmuziek</skos:prefLabel>
    <skos:prefLabel xml:lang="et">Süvamuusika</skos:prefLabel>
    <skos:prefLabel xml:lang="fr">Musique savante</skos:prefLabel>
    <skos:prefLabel xml:lang="de">Kunstmusik</skos:prefLabel>
    <skos:prefLabel xml:lang="it">Musica colta</skos:prefLabel>
    <skos:prefLabel xml:lang="ru">Академическая музыка</skos:prefLabel>
    <skos:prefLabel xml:lang="es">Música culta</skos:prefLabel>
    <skos:prefLabel xml:lang="uk">Академічна музика</skos:prefLabel>
    <skos:prefLabel xml:lang="en">Art</skos:prefLabel>
    <skos:closeMatch rdf:resource="http://rdf.freebase.com/ns/m.02p19y6"/>
    <skos:broader rdf:resource="http://data.europeana.eu/concept/music/genre/Music"/>
    <skos:definition xml:lang="en">Art music—also known as formal music, serious music, erudite
      music, or legitimate music —is an umbrella term used to refer to musical traditions implying
      advanced structural and theoretical considerations and a written musical tradition. The notion
      of art music is a frequent and well-defined musicological distinction, e.g., referred to by
      musicologist Philip Tagg as one of an &quot;axiomatic triangle consisting of 'folk', 'art' and
      'popular' musics.&quot; He explains that each of these three is distinguishable from the
      others according to certain criteria. The main tradition in the Western world is usually
      called classical music. In this regard, it is frequently used as a contrasting term to popular
      music and traditional or folk music. The term also covers non-Western classical traditions
      such as Chinese classical music and Traditional Japanese music.</skos:definition>
    <skos:exactMatch xml:lang="en">http://dbpedia.org/resource/Art_music</skos:exactMatch>
    <skos:inScheme rdf:resource="http://data.europeana.eu/concept/music/genre/Music_Genre_Scheme"/>
    <skos:altLabel xml:lang="en">Art music</skos:altLabel>
  </skos:Concept>

  <skos:Concept rdf:about="http://data.europeana.eu/concept/music/genre/World_music">
    <skos:prefLabel xml:lang="en">Traditional (world) music</skos:prefLabel>
    <skos:prefLabel xml:lang="ar">موسيقى العالم</skos:prefLabel>
    <skos:prefLabel xml:lang="ca">World music</skos:prefLabel>
    <skos:prefLabel xml:lang="cs">World music</skos:prefLabel>
    <skos:prefLabel xml:lang="da">Verdensmusik</skos:prefLabel>
    <skos:prefLabel xml:lang="nl">Wereldmuziek</skos:prefLabel>
    <skos:prefLabel xml:lang="et">Maailmamuusika</skos:prefLabel>
    <skos:prefLabel xml:lang="fi">Maailmanmusiikki</skos:prefLabel>
    <skos:prefLabel xml:lang="fr">Musiques du monde</skos:prefLabel>
    <skos:prefLabel xml:lang="de">Weltmusik</skos:prefLabel>
    <skos:prefLabel xml:lang="hu">Világzene</skos:prefLabel>
    <skos:prefLabel xml:lang="id">Musik dunia</skos:prefLabel>
    <skos:prefLabel xml:lang="it">World music</skos:prefLabel>
    <skos:prefLabel xml:lang="ja">ワールドミュージック</skos:prefLabel>
    <skos:prefLabel xml:lang="ko">월드 뮤직</skos:prefLabel>
    <skos:prefLabel xml:lang="lt">Pasaulio etninė muzika</skos:prefLabel>
    <skos:prefLabel xml:lang="no">Verdensmusikk</skos:prefLabel>
    <skos:prefLabel xml:lang="fa">موسیقی جهان</skos:prefLabel>
    <skos:prefLabel xml:lang="pl">World music</skos:prefLabel>
    <skos:prefLabel xml:lang="pt">Música do mundo</skos:prefLabel>
    <skos:prefLabel xml:lang="ro">World music</skos:prefLabel>
    <skos:prefLabel xml:lang="ru">Этническая музыка</skos:prefLabel>
    <skos:prefLabel xml:lang="sr">Етно музика</skos:prefLabel>
    <skos:prefLabel xml:lang="es">World music</skos:prefLabel>
    <skos:prefLabel xml:lang="sv">Världsmusik</skos:prefLabel>
    <skos:prefLabel xml:lang="th">เวิลด์มิวสิก</skos:prefLabel>
    <skos:prefLabel xml:lang="uk">Етнічна музика</skos:prefLabel>
    <skos:prefLabel xml:lang="vi">World music</skos:prefLabel>
    <skos:closeMatch rdf:resource="http://rdf.freebase.com/ns/m.0827d"/>
    <skos:broader rdf:resource="http://data.europeana.eu/concept/music/genre/Music"/>
    <skos:definition xml:lang="en">World music is a musical category encompassing many different
      styles of music from around the world, including traditional music, neotraditional music, and
      music where more than one cultural tradition intermingle. World music's inclusive nature and
      elasticity as a musical category pose obstacles to a universal definition, but its ethic of
      interest in the culturally exotic is encapsulated in fRoots magazine's description of the
      genre as &quot;local music from out there&quot;. The term originated in the late 20th century
      as a marketing category and academic classification for non-Western traditional music.
      Globalization has facilitated the expansion of world music's audiences and scope. It has grown
      to include hybrid sub-genres such as world fusion, global fusion, ethnic fusion and
      worldbeat.</skos:definition>
    <skos:broadMatch rdf:resource="http://dbpedia.org/resource/World_music"/>
    <skos:inScheme rdf:resource="http://data.europeana.eu/concept/music/genre/Music_Genre_Scheme"/>
    <skos:altLabel xml:lang="en">World music</skos:altLabel>
  </skos:Concept>

  <skos:Concept rdf:about="http://data.europeana.eu/concept/music/genre/Popular_music">
    <skos:prefLabel xml:lang="en">Popular music</skos:prefLabel>
    <skos:prefLabel xml:lang="ar">موسيقى شائعة</skos:prefLabel>
    <skos:prefLabel xml:lang="ca">Música popular</skos:prefLabel>
    <skos:prefLabel xml:lang="cs">Populární hudba</skos:prefLabel>
    <skos:prefLabel xml:lang="nl">Lichte muziek</skos:prefLabel>
    <skos:prefLabel xml:lang="fi">Populaarimusiikki</skos:prefLabel>
    <skos:prefLabel xml:lang="fr">Musique populaire</skos:prefLabel>
    <skos:prefLabel xml:lang="hu">Könnyűzene</skos:prefLabel>
    <skos:prefLabel xml:lang="id">Musik populer</skos:prefLabel>
    <skos:prefLabel xml:lang="it">Popular music</skos:prefLabel>
    <skos:prefLabel xml:lang="ja">ポピュラー音楽</skos:prefLabel>
    <skos:prefLabel xml:lang="ko">대중음악</skos:prefLabel>
    <skos:prefLabel xml:lang="fa">موسیقی عامه‌پسند</skos:prefLabel>
    <skos:prefLabel xml:lang="pl">Muzyka rozrywkowa</skos:prefLabel>
    <skos:prefLabel xml:lang="pt">Música popular</skos:prefLabel>
    <skos:prefLabel xml:lang="ro">Muzică de consum</skos:prefLabel>
    <skos:prefLabel xml:lang="ru">Популярная музыка</skos:prefLabel>
    <skos:prefLabel xml:lang="sr">Забавна музика</skos:prefLabel>
    <skos:prefLabel xml:lang="sk">Populárna hudba</skos:prefLabel>
    <skos:prefLabel xml:lang="sl">Popularna glasba</skos:prefLabel>
    <skos:prefLabel xml:lang="es">Música popular</skos:prefLabel>
    <skos:prefLabel xml:lang="sv">Populärmusik</skos:prefLabel>
    <skos:prefLabel xml:lang="th">เพลงสมัยนิยม</skos:prefLabel>
    <skos:prefLabel xml:lang="vi">Nhạc đại chúng</skos:prefLabel>
    <skos:prefLabel xml:lang="en">Popular</skos:prefLabel>
    <skos:closeMatch rdf:resource="http://rdf.freebase.com/ns/m.05r9t"/>
    <skos:broader rdf:resource="http://data.europeana.eu/concept/music/genre/Music"/>
    <skos:definition xml:lang="en">Popular music belongs to any of a number of musical genres
      &quot;having wide appeal&quot; and is typically distributed to large audiences through the
      music industry. It stands in contrast to both art music and traditional music, which are
      typically disseminated academically or orally to smaller, local audiences. The original
      application of the term is to music of the 1880s Tin Pan Alley period in the United States.
      Although popular music sometimes is known as &quot;pop music,&quot; the two terms are not
      interchangeable. Popular music is a generic term for music of all ages that appeals to popular
      tastes, whereas pop music usually refers to a specific musical genre.</skos:definition>
    <skos:exactMatch xml:lang="en">http://dbpedia.org/resource/Popular_music</skos:exactMatch>
    <skos:inScheme rdf:resource="http://data.europeana.eu/concept/music/genre/Music_Genre_Scheme"/>
    <skos:altLabel xml:lang="en">pop music</skos:altLabel>
    <skos:altLabel xml:lang="en">Popular music</skos:altLabel>
  </skos:Concept>

  <skos:Concept rdf:about="http://data.europeana.eu/concept/music/genre/Religious_music">
    <skos:prefLabel xml:lang="en">Religious music</skos:prefLabel>
    <skos:prefLabel xml:lang="ca">Música religiosa</skos:prefLabel>
    <skos:prefLabel xml:lang="hr">Vjerska glazba</skos:prefLabel>
    <skos:prefLabel xml:lang="cs">Duchovní hudba</skos:prefLabel>
    <skos:prefLabel xml:lang="nl">Kerkmuziek</skos:prefLabel>
    <skos:prefLabel xml:lang="et">Vaimulik muusika</skos:prefLabel>
    <skos:prefLabel xml:lang="fi">Hengellinen musiikki</skos:prefLabel>
    <skos:prefLabel xml:lang="fr">Musique sacrée</skos:prefLabel>
    <skos:prefLabel xml:lang="de">Geistliche Musik</skos:prefLabel>
    <skos:prefLabel xml:lang="el">Χριστιανική μουσική</skos:prefLabel>
    <skos:prefLabel xml:lang="id">Musik Gereja</skos:prefLabel>
    <skos:prefLabel xml:lang="it">Musica sacra</skos:prefLabel>
    <skos:prefLabel xml:lang="ja">キリスト教音楽</skos:prefLabel>
    <skos:prefLabel xml:lang="ko">종교 음악</skos:prefLabel>
    <skos:prefLabel xml:lang="pt">Música religiosa</skos:prefLabel>
    <skos:prefLabel xml:lang="ru">Духовная музыка</skos:prefLabel>
    <skos:prefLabel xml:lang="sr">Хришћанска музика</skos:prefLabel>
    <skos:prefLabel xml:lang="sk">Náboženská hudba</skos:prefLabel>
    <skos:prefLabel xml:lang="es">Música sacra</skos:prefLabel>
    <skos:prefLabel xml:lang="sv">Andlig musik</skos:prefLabel>
    <skos:closeMatch rdf:resource="http://rdf.freebase.com/ns/m.0138g2"/>
    <skos:broader rdf:resource="http://data.europeana.eu/concept/music/genre/Music"/>
    <skos:definition xml:lang="en">Religious music is music performed or composed for religious use
      or through religious influence.</skos:definition>
    <skos:exactMatch xml:lang="en">http://dbpedia.org/resource/Religious_music</skos:exactMatch>
    <skos:inScheme rdf:resource="http://data.europeana.eu/concept/music/genre/Music_Genre_Scheme"/>
    <skos:altLabel xml:lang="en">Sacred music</skos:altLabel>
  </skos:Concept>

  <skos:Concept rdf:about="http://data.europeana.eu/concept/music/genre/Fusion_(music)_fusions">
    <skos:prefLabel xml:lang="en">Fusion music</skos:prefLabel>
    <skos:prefLabel xml:lang="ar">راب كور</skos:prefLabel>
    <skos:prefLabel xml:lang="ca">Jazz rock</skos:prefLabel>
    <skos:prefLabel xml:lang="cs">Fusion</skos:prefLabel>
    <skos:prefLabel xml:lang="da">Fusion</skos:prefLabel>
    <skos:prefLabel xml:lang="nl">Jazzrock</skos:prefLabel>
    <skos:prefLabel xml:lang="fr">Fusion de genres musicaux</skos:prefLabel>
    <skos:prefLabel xml:lang="hi">फ्यूजन संगीत</skos:prefLabel>
    <skos:prefLabel xml:lang="hu">Fúziós zene</skos:prefLabel>
    <skos:prefLabel xml:lang="ko">믹스처 록</skos:prefLabel>
    <skos:prefLabel xml:lang="fa">موسیقی تلفیقی</skos:prefLabel>
    <skos:prefLabel xml:lang="ro">Fusion</skos:prefLabel>
    <skos:prefLabel xml:lang="ru">Фьюжн</skos:prefLabel>
    <skos:prefLabel xml:lang="sr">Фузија</skos:prefLabel>
    <skos:prefLabel xml:lang="sv">Fusion</skos:prefLabel>
    <skos:prefLabel xml:lang="uk">Ф'южн</skos:prefLabel>
    <skos:closeMatch rdf:resource="http://rdf.freebase.com/ns/m.05rwlj"/>
    <skos:broader rdf:resource="http://data.europeana.eu/concept/music/genre/Music"/>
    <skos:definition xml:lang="en">Fusion est un terme général qui fut utilisé dans le rock
      essentiellement dans les années 1990 pour désigner divers styles de fusion de genres musicaux
      comme le funk-rock ou le rap-rock. Ce courant ne doit pas être confondu avec la fusion
      jazz-rock, qui est un courant dérivé du jazz et incorporant des éléments du
      rock.</skos:definition>
    <skos:exactMatch xml:lang="en">http://dbpedia.org/resource/Fusion_(music)</skos:exactMatch>
    <skos:inScheme rdf:resource="http://data.europeana.eu/concept/music/genre/Music_Genre_Scheme"/>
    <skos:altLabel xml:lang="en">Fusion</skos:altLabel>
    <skos:altLabel xml:lang="en">Fusion genre</skos:altLabel>
  </skos:Concept>

  <skos:Concept rdf:about="http://data.europeana.eu/concept/music/genre/Acid_jazz">
    <skos:prefLabel xml:lang="en">Acid jazz</skos:prefLabel>
    <skos:prefLabel xml:lang="ca">Acid Jazz</skos:prefLabel>
    <skos:prefLabel xml:lang="hr">Acid jazz</skos:prefLabel>
    <skos:prefLabel xml:lang="cs">Acid jazz</skos:prefLabel>
    <skos:prefLabel xml:lang="da">Acid jazz</skos:prefLabel>
    <skos:prefLabel xml:lang="nl">Acid jazz</skos:prefLabel>
    <skos:prefLabel xml:lang="fi">Acid jazz</skos:prefLabel>
    <skos:prefLabel xml:lang="fr">Acid jazz</skos:prefLabel>
    <skos:prefLabel xml:lang="de">Acid Jazz</skos:prefLabel>
    <skos:prefLabel xml:lang="hu">Acid jazz</skos:prefLabel>
    <skos:prefLabel xml:lang="id">Acid jazz</skos:prefLabel>
    <skos:prefLabel xml:lang="it">Acid jazz</skos:prefLabel>
    <skos:prefLabel xml:lang="ja">アシッドジャズ</skos:prefLabel>
    <skos:prefLabel xml:lang="ko">애시드 재즈</skos:prefLabel>
    <skos:prefLabel xml:lang="no">Acid jazz</skos:prefLabel>
    <skos:prefLabel xml:lang="fa">اسید جاز</skos:prefLabel>
    <skos:prefLabel xml:lang="pl">Acid jazz</skos:prefLabel>
    <skos:prefLabel xml:lang="pt">Acid jazz</skos:prefLabel>
    <skos:prefLabel xml:lang="ro">Acid jazz</skos:prefLabel>
    <skos:prefLabel xml:lang="ru">Эйсид-джаз</skos:prefLabel>
    <skos:prefLabel xml:lang="es">Acid jazz</skos:prefLabel>
    <skos:prefLabel xml:lang="sv">Acid jazz</skos:prefLabel>
    <skos:prefLabel xml:lang="th">เอซิดแจ๊ส</skos:prefLabel>
    <skos:prefLabel xml:lang="uk">Ейсид-джаз</skos:prefLabel>
    <skos:closeMatch rdf:resource="http://rdf.freebase.com/ns/m.01n4bh"/>
    <skos:broader rdf:resource="http://data.europeana.eu/concept/music/genre/Jazz_fusions"/>
    <skos:definition xml:lang="en">Acid jazz, also known as club jazz, is a musical genre that
      combines elements of jazz, soul, funk, disco and hip-hop. Acid jazz originated in the London
      club scene of the mid-1980s in the rare groove movement and spread to the US, Japan, Eastern
      Europe and Brazil. Major acts included Brand New Heavies, Incognito, Us3 and Jamiroquai from
      the UK and A Tribe Called Quest, Buckshot LeFonque and Digable Planets from the US. The rise
      of electronic club music in the mid to late 1990s led to a decline in interest, and in the
      twenty-first century, the movement became indistinct as a genre. Many acts that might have
      been defined as acid jazz are now seen as jazz funk, neo soul or jazz rap.</skos:definition>
    <skos:exactMatch xml:lang="en">http://dbpedia.org/resource/Acid_jazz</skos:exactMatch>
    <skos:inScheme rdf:resource="http://data.europeana.eu/concept/music/genre/Music_Genre_Scheme"/>
    <skos:altLabel xml:lang="en">Acid jazz</skos:altLabel>
  </skos:Concept>

  <skos:Concept rdf:about="http://data.europeana.eu/concept/music/genre/Bambuco">
    <skos:prefLabel xml:lang="en">Bambuco</skos:prefLabel>
    <skos:prefLabel xml:lang="ca">Bambuco</skos:prefLabel>
    <skos:prefLabel xml:lang="nl">Bambuco</skos:prefLabel>
    <skos:prefLabel xml:lang="fr">Bambuco</skos:prefLabel>
    <skos:prefLabel xml:lang="de">Bambuco</skos:prefLabel>
    <skos:prefLabel xml:lang="it">Bambuco</skos:prefLabel>
    <skos:prefLabel xml:lang="pt">Bambuco</skos:prefLabel>
    <skos:prefLabel xml:lang="ru">Бамбуко</skos:prefLabel>
    <skos:prefLabel xml:lang="es">Bambuco</skos:prefLabel>
    <skos:closeMatch rdf:resource="http://rdf.freebase.com/ns/m.025j27"/>
    <skos:broader
      rdf:resource="http://data.europeana.eu/concept/music/genre/Latin_American_music_traditional"/>
    <skos:definition xml:lang="en">Bambuco is a traditional music genre originated from Colombia. It
      has a beat structure similar to the European waltz or polska. Typically a bambuco piece is a
      folk music song accompanied by a stylized group dance in either a 6/8 or 3/4 meter. &lt;p&gt;
      Bambuco took a cultural foothold in the Andean region of Colombia and has spread in popularity
      throughout Latin America. The Festival Folclórico y Reinado Nacional del Bambuco in Neiva is a
      festival celebrating bambuco music.</skos:definition>
    <skos:exactMatch xml:lang="en">http://dbpedia.org/resource/Bambuco</skos:exactMatch>
    <skos:inScheme rdf:resource="http://data.europeana.eu/concept/music/genre/Music_Genre_Scheme"/>
    <skos:altLabel xml:lang="en">Bambuco</skos:altLabel>
  </skos:Concept>

  <skos:Concept rdf:about="http://data.europeana.eu/concept/music/genre/Bolero">
    <skos:prefLabel xml:lang="en">Bolero</skos:prefLabel>
    <skos:prefLabel xml:lang="ar">بوليرو</skos:prefLabel>
    <skos:prefLabel xml:lang="ca">Bolero</skos:prefLabel>
    <skos:prefLabel xml:lang="hr">Bolero</skos:prefLabel>
    <skos:prefLabel xml:lang="nl">Bolero</skos:prefLabel>
    <skos:prefLabel xml:lang="et">Boolero</skos:prefLabel>
    <skos:prefLabel xml:lang="fi">Bolero</skos:prefLabel>
    <skos:prefLabel xml:lang="fr">Boléro</skos:prefLabel>
    <skos:prefLabel xml:lang="de">Bolero</skos:prefLabel>
    <skos:prefLabel xml:lang="it">Bolero</skos:prefLabel>
    <skos:prefLabel xml:lang="ja">ボレロ</skos:prefLabel>
    <skos:prefLabel xml:lang="ko">볼레로</skos:prefLabel>
    <skos:prefLabel xml:lang="no">Bolero</skos:prefLabel>
    <skos:prefLabel xml:lang="pl">Bolero</skos:prefLabel>
    <skos:prefLabel xml:lang="pt">Bolero</skos:prefLabel>
    <skos:prefLabel xml:lang="ro">Bolero</skos:prefLabel>
    <skos:prefLabel xml:lang="ru">Болеро</skos:prefLabel>
    <skos:prefLabel xml:lang="sl">Bolero</skos:prefLabel>
    <skos:prefLabel xml:lang="es">Bolero</skos:prefLabel>
    <skos:prefLabel xml:lang="sv">Bolero</skos:prefLabel>
    <skos:prefLabel xml:lang="uk">Болеро</skos:prefLabel>
    <skos:prefLabel xml:lang="vi">Bolero</skos:prefLabel>
    <skos:closeMatch rdf:resource="http://rdf.freebase.com/ns/m.01v9sc"/>
    <skos:broader
      rdf:resource="http://data.europeana.eu/concept/music/genre/Latin_American_music_popular"/>
    <skos:definition xml:lang="en">Bolero is a genre of slow-tempo Latin music and its associated
      dance. There are Spanish and Cuban forms which are both significant and which have separate
      origins. &lt;p&gt; The term is also used for some art music. In all its forms, the bolero has
      been popular for over a century.</skos:definition>
    <skos:exactMatch xml:lang="en">http://dbpedia.org/resource/Bolero</skos:exactMatch>
    <skos:inScheme rdf:resource="http://data.europeana.eu/concept/music/genre/Music_Genre_Scheme"/>
    <skos:altLabel xml:lang="en">Bolero</skos:altLabel>
  </skos:Concept>

  <skos:Concept rdf:about="http://data.europeana.eu/concept/music/genre/Bebop">
    <skos:prefLabel xml:lang="en">Bebop</skos:prefLabel>
    <skos:prefLabel xml:lang="bg">Бибоп</skos:prefLabel>
    <skos:prefLabel xml:lang="ca">Bebop</skos:prefLabel>
    <skos:prefLabel xml:lang="hr">Bebop</skos:prefLabel>
    <skos:prefLabel xml:lang="cs">Bebop</skos:prefLabel>
    <skos:prefLabel xml:lang="da">Bebop</skos:prefLabel>
    <skos:prefLabel xml:lang="nl">Bop</skos:prefLabel>
    <skos:prefLabel xml:lang="et">Bebop</skos:prefLabel>
    <skos:prefLabel xml:lang="fi">Bebop</skos:prefLabel>
    <skos:prefLabel xml:lang="fr">Bebop</skos:prefLabel>
    <skos:prefLabel xml:lang="de">Bebop</skos:prefLabel>
    <skos:prefLabel xml:lang="el">Μπίμποπ</skos:prefLabel>
    <skos:prefLabel xml:lang="hu">Bebop</skos:prefLabel>
    <skos:prefLabel xml:lang="id">Bebop</skos:prefLabel>
    <skos:prefLabel xml:lang="it">Bebop</skos:prefLabel>
    <skos:prefLabel xml:lang="ja">ビバップ</skos:prefLabel>
    <skos:prefLabel xml:lang="ko">비밥</skos:prefLabel>
    <skos:prefLabel xml:lang="lt">Bibopas</skos:prefLabel>
    <skos:prefLabel xml:lang="no">Bebop</skos:prefLabel>
    <skos:prefLabel xml:lang="fa">بیباپ</skos:prefLabel>
    <skos:prefLabel xml:lang="pl">Bebop</skos:prefLabel>
    <skos:prefLabel xml:lang="pt">Bebop</skos:prefLabel>
    <skos:prefLabel xml:lang="ru">Бибоп</skos:prefLabel>
    <skos:prefLabel xml:lang="sr">Би-бап</skos:prefLabel>
    <skos:prefLabel xml:lang="sk">Bebop</skos:prefLabel>
    <skos:prefLabel xml:lang="es">Bebop</skos:prefLabel>
    <skos:prefLabel xml:lang="sv">Bebop</skos:prefLabel>
    <skos:prefLabel xml:lang="tr">Bebop</skos:prefLabel>
    <skos:prefLabel xml:lang="uk">Бібоп</skos:prefLabel>
    <skos:closeMatch rdf:resource="http://rdf.freebase.com/ns/m.0cx6f"/>
    <skos:broader rdf:resource="http://data.europeana.eu/concept/music/genre/Jazz"/>
    <skos:definition xml:lang="en">Bebop or bop is a style of jazz characterized by a fast tempo,
      instrumental virtuosity, and improvisation based on the combination of harmonic structure and
      melody. It was developed in the early and mid-1940s. It first surfaced in musicians' argot
      some time during the first two years of American involvement in the Second World War. This
      style of jazz ultimately became synonymous with modern jazz, as either category reached a
      certain final maturity in the 1960s.</skos:definition>
    <skos:exactMatch xml:lang="en">http://dbpedia.org/resource/Bebop</skos:exactMatch>
    <skos:inScheme rdf:resource="http://data.europeana.eu/concept/music/genre/Music_Genre_Scheme"/>
    <skos:altLabel xml:lang="en">Bebop</skos:altLabel>
  </skos:Concept>

  <skos:Concept rdf:about="http://data.europeana.eu/concept/music/genre/Blues">
    <skos:prefLabel xml:lang="en">Blues</skos:prefLabel>
    <skos:prefLabel xml:lang="ar">بلوز</skos:prefLabel>
    <skos:prefLabel xml:lang="bg">Блус</skos:prefLabel>
    <skos:prefLabel xml:lang="ca">Blues</skos:prefLabel>
    <skos:prefLabel xml:lang="hr">Blues</skos:prefLabel>
    <skos:prefLabel xml:lang="cs">Blues</skos:prefLabel>
    <skos:prefLabel xml:lang="da">Blues</skos:prefLabel>
    <skos:prefLabel xml:lang="nl">Blues</skos:prefLabel>
    <skos:prefLabel xml:lang="et">Bluus</skos:prefLabel>
    <skos:prefLabel xml:lang="fi">Blues</skos:prefLabel>
    <skos:prefLabel xml:lang="fr">Blues</skos:prefLabel>
    <skos:prefLabel xml:lang="de">Blues</skos:prefLabel>
    <skos:prefLabel xml:lang="el">Μπλουζ</skos:prefLabel>
    <skos:prefLabel xml:lang="hi">ब्लूज़</skos:prefLabel>
    <skos:prefLabel xml:lang="hu">Blues</skos:prefLabel>
    <skos:prefLabel xml:lang="id">Blues</skos:prefLabel>
    <skos:prefLabel xml:lang="it">Blues</skos:prefLabel>
    <skos:prefLabel xml:lang="ja">ブルース</skos:prefLabel>
    <skos:prefLabel xml:lang="ko">블루스</skos:prefLabel>
    <skos:prefLabel xml:lang="lv">Blūzs</skos:prefLabel>
    <skos:prefLabel xml:lang="lt">Bliuzas</skos:prefLabel>
    <skos:prefLabel xml:lang="ms">Blues</skos:prefLabel>
    <skos:prefLabel xml:lang="no">Blues</skos:prefLabel>
    <skos:prefLabel xml:lang="fa">موسیقی بلوز</skos:prefLabel>
    <skos:prefLabel xml:lang="pl">Blues</skos:prefLabel>
    <skos:prefLabel xml:lang="pt">Blues</skos:prefLabel>
    <skos:prefLabel xml:lang="ro">Blues</skos:prefLabel>
    <skos:prefLabel xml:lang="ru">Блюз</skos:prefLabel>
    <skos:prefLabel xml:lang="sr">Bluz</skos:prefLabel>
    <skos:prefLabel xml:lang="sk">Blues</skos:prefLabel>
    <skos:prefLabel xml:lang="sl">Blues</skos:prefLabel>
    <skos:prefLabel xml:lang="es">Blues</skos:prefLabel>
    <skos:prefLabel xml:lang="sv">Blues</skos:prefLabel>
    <skos:prefLabel xml:lang="th">บลูส์</skos:prefLabel>
    <skos:prefLabel xml:lang="tr">Blues</skos:prefLabel>
    <skos:prefLabel xml:lang="uk">Блюз</skos:prefLabel>
    <skos:prefLabel xml:lang="vi">Blues</skos:prefLabel>
    <skos:closeMatch rdf:resource="http://rdf.freebase.com/ns/m.0155w"/>
    <skos:broader rdf:resource="http://data.europeana.eu/concept/music/genre/Popular_music"/>
    <skos:definition xml:lang="en">Blues is a musical form and genre that originated in
      African-American communities in the &quot;Deep South&quot; of the United States around the end
      of the 19th century from spirituals, work songs, field hollers, shouts and chants, and rhymed
      simple narrative ballads. The blues form, ubiquitous in jazz, rhythm and blues and rock and
      roll, is characterized by specific chord progressions, of which the twelve-bar blues is the
      most common. The blue notes that, for expressive purposes are sung or played flattened or
      gradually bent in relation to the pitch of the major scale, are also an important part of the
      sound. &lt;p&gt; Blues as a genre is based on the blues form but possesses other
      characteristics such as lyrics, bass lines, and instruments. Blues sub-genres include country
      blues, such as Delta, Piedmont and Texas blues, and urban blues styles such as Chicago and
      West Coast blues. World War II marked the transition from acoustic to electric blues and the
      progressive opening of blues music to a wider audience, especially white listeners. In the
      1960s and 1970s, a hybrid form called blues-rock evolved.</skos:definition>
    <skos:exactMatch xml:lang="en">http://dbpedia.org/resource/Blues</skos:exactMatch>
    <skos:inScheme rdf:resource="http://data.europeana.eu/concept/music/genre/Music_Genre_Scheme"/>
    <skos:altLabel xml:lang="en">Blues music</skos:altLabel>
    <skos:altLabel xml:lang="en">Blues</skos:altLabel>
  </skos:Concept>

  <skos:Concept rdf:about="http://data.europeana.eu/concept/music/genre/Boogie-woogie">
    <skos:prefLabel xml:lang="en">Boogie-woogie</skos:prefLabel>
    <skos:prefLabel xml:lang="bg">Буги-вуги</skos:prefLabel>
    <skos:prefLabel xml:lang="ca">Bugui-bugui</skos:prefLabel>
    <skos:prefLabel xml:lang="hr">Boogie-woogie</skos:prefLabel>
    <skos:prefLabel xml:lang="cs">Boogie-woogie</skos:prefLabel>
    <skos:prefLabel xml:lang="da">Boogie-woogie</skos:prefLabel>
    <skos:prefLabel xml:lang="nl">Boogiewoogie</skos:prefLabel>
    <skos:prefLabel xml:lang="et">Bugi-vugi</skos:prefLabel>
    <skos:prefLabel xml:lang="fi">Boogie woogie</skos:prefLabel>
    <skos:prefLabel xml:lang="fr">Boogie-woogie</skos:prefLabel>
    <skos:prefLabel xml:lang="de">Boogie-Woogie</skos:prefLabel>
    <skos:prefLabel xml:lang="el">Μπούγκι</skos:prefLabel>
    <skos:prefLabel xml:lang="hu">Boogie-woogie</skos:prefLabel>
    <skos:prefLabel xml:lang="id">Boogie-Woogie</skos:prefLabel>
    <skos:prefLabel xml:lang="it">Boogie-woogie</skos:prefLabel>
    <skos:prefLabel xml:lang="ko">부기우기</skos:prefLabel>
    <skos:prefLabel xml:lang="no">Boogie-woogie</skos:prefLabel>
    <skos:prefLabel xml:lang="pl">Boogie-woogie</skos:prefLabel>
    <skos:prefLabel xml:lang="pt">Boogie-woogie</skos:prefLabel>
    <skos:prefLabel xml:lang="ru">Буги-вуги</skos:prefLabel>
    <skos:prefLabel xml:lang="es">Boogie-woogie</skos:prefLabel>
    <skos:prefLabel xml:lang="sv">Boogie woogie</skos:prefLabel>
    <skos:prefLabel xml:lang="uk">Буґі-вуґі</skos:prefLabel>
    <skos:closeMatch rdf:resource="http://rdf.freebase.com/ns/m.016vzr"/>
    <skos:broader rdf:resource="http://data.europeana.eu/concept/music/genre/Jazz_fusions"/>
    <skos:definition xml:lang="en">Boogie-woogie is an African American style of piano-based blues
      that became popular after 1928, but originated much earlier in the century, and was extended
      from piano, to three pianos at once, guitar, big band, and country and western music, and even
      gospel. While the blues traditionally expresses a variety of emotions, boogie-woogie is mainly
      associated with dancing. The lyrics of one of the earliest hits, &quot;Pinetop's Boogie
      Woogie&quot;, consist entirely of instructions to dancers: &lt;p&gt; Now, when I tell you to
      hold yourself, don't you move a peg. &lt;p&gt; And when I tell you to get it, I want you to
      Boogie Woogie! &lt;p&gt; It is characterized by a regular bass figure, in the left hand. The
      bass figure is transposed according to the chord changes. &lt;p&gt; It is not strictly a solo
      piano style, but is also used to accompany singers and as a solo part in bands and small
      combos. It is sometimes called &quot;eight to the bar&quot;, as much of it is written in
      common time time using eighth notes. The chord progressions are typically based on I - IV - V
      - I.</skos:definition>
    <skos:exactMatch xml:lang="en">http://dbpedia.org/resource/Boogie-woogie</skos:exactMatch>
    <skos:inScheme rdf:resource="http://data.europeana.eu/concept/music/genre/Music_Genre_Scheme"/>
    <skos:altLabel xml:lang="en">Boogie-woogie</skos:altLabel>
  </skos:Concept>

  <skos:Concept rdf:about="http://data.europeana.eu/concept/music/genre/Bossa_nova">
    <skos:prefLabel xml:lang="en">Bossa nova</skos:prefLabel>
    <skos:prefLabel xml:lang="ar">بوسا نوفا</skos:prefLabel>
    <skos:prefLabel xml:lang="bg">Боса нова</skos:prefLabel>
    <skos:prefLabel xml:lang="ca">Bossa nova</skos:prefLabel>
    <skos:prefLabel xml:lang="hr">Bossa nova</skos:prefLabel>
    <skos:prefLabel xml:lang="cs">Bossa nova</skos:prefLabel>
    <skos:prefLabel xml:lang="da">Bossanova</skos:prefLabel>
    <skos:prefLabel xml:lang="nl">Bossanova</skos:prefLabel>
    <skos:prefLabel xml:lang="fil">Bossa nova</skos:prefLabel>
    <skos:prefLabel xml:lang="fi">Bossa nova</skos:prefLabel>
    <skos:prefLabel xml:lang="fr">Bossa nova</skos:prefLabel>
    <skos:prefLabel xml:lang="de">Bossa Nova</skos:prefLabel>
    <skos:prefLabel xml:lang="el">Μπόσα νόβα</skos:prefLabel>
    <skos:prefLabel xml:lang="hu">Bossa nova</skos:prefLabel>
    <skos:prefLabel xml:lang="id">Bossa nova</skos:prefLabel>
    <skos:prefLabel xml:lang="it">Bossa nova</skos:prefLabel>
    <skos:prefLabel xml:lang="ja">ボサノヴァ</skos:prefLabel>
    <skos:prefLabel xml:lang="ko">보사노바</skos:prefLabel>
    <skos:prefLabel xml:lang="es-419">Bossa nova</skos:prefLabel>
    <skos:prefLabel xml:lang="ms">Bossa nova</skos:prefLabel>
    <skos:prefLabel xml:lang="no">Bossa nova</skos:prefLabel>
    <skos:prefLabel xml:lang="fa">بوسا نوا</skos:prefLabel>
    <skos:prefLabel xml:lang="pl">Bossa nova</skos:prefLabel>
    <skos:prefLabel xml:lang="pt">Bossa Nova</skos:prefLabel>
    <skos:prefLabel xml:lang="ro">Bossa-nova</skos:prefLabel>
    <skos:prefLabel xml:lang="ru">Босанова</skos:prefLabel>
    <skos:prefLabel xml:lang="sr">Боса нова</skos:prefLabel>
    <skos:prefLabel xml:lang="sk">Bossa Nova</skos:prefLabel>
    <skos:prefLabel xml:lang="es">Bossa nova</skos:prefLabel>
    <skos:prefLabel xml:lang="sv">Bossa nova</skos:prefLabel>
    <skos:prefLabel xml:lang="th">บอสซาโนวา</skos:prefLabel>
    <skos:prefLabel xml:lang="tr">Bossa nova</skos:prefLabel>
    <skos:prefLabel xml:lang="uk">Босанова</skos:prefLabel>
    <skos:closeMatch rdf:resource="http://rdf.freebase.com/ns/m.01kcty"/>
    <skos:broader
      rdf:resource="http://data.europeana.eu/concept/music/genre/Latin_American_music_popular"/>
    <skos:definition xml:lang="en">Bossa nova is a genre of Brazilian music, which developed and was
      popularized in the 1950s and 1960s and is today one of the best-known Brazilian music genres
      abroad. The phrase bossa nova means literally &quot;new trend&quot;. A lyrical fusion of samba
      and jazz, bossa nova acquired a large following in the 1960s initially among young musicians
      and college students. Since its inception, it has remained a vital part of the standard jazz
      repertoire.</skos:definition>
    <skos:exactMatch xml:lang="en">http://dbpedia.org/resource/Bossa_nova</skos:exactMatch>
    <skos:inScheme rdf:resource="http://data.europeana.eu/concept/music/genre/Music_Genre_Scheme"/>
    <skos:altLabel xml:lang="en">Bossa nova</skos:altLabel>
  </skos:Concept>

  <skos:Concept rdf:about="http://data.europeana.eu/concept/music/genre/Bullerengue">
    <skos:prefLabel xml:lang="en">Bullerengue</skos:prefLabel>
    <skos:prefLabel xml:lang="es">Bullerengue</skos:prefLabel>
    <skos:closeMatch rdf:resource="http://rdf.freebase.com/ns/m.0gh6sdn"/>
    <skos:broader
      rdf:resource="http://data.europeana.eu/concept/music/genre/Latin_American_music_popular"/>
    <skos:definition xml:lang="en">Bullerengue is a musical style and dance from the Caribbean
      Region of Colombia and the Darién Province in Panama. It is a cumbia-based style traditionally
      sung exclusively by women. Some famous bullerengue singers are Irene Martinez, Antún Castro,
      Estefanía Caycedo, Alé Kumá, Benigna Solís, Martina camargo and Etelvina Maldonado. In recent
      decades, Petrona Martínez and Totó la Momposina have increased Bullerengue's international
      popularity and success, having been nominees for the Latin Grammy Award for Best Folk
      Album.</skos:definition>
    <skos:exactMatch xml:lang="en">http://dbpedia.org/resource/Bullerengue</skos:exactMatch>
    <skos:inScheme rdf:resource="http://data.europeana.eu/concept/music/genre/Music_Genre_Scheme"/>
    <skos:altLabel xml:lang="en">Bullerengue</skos:altLabel>
  </skos:Concept>

  <skos:Concept rdf:about="http://data.europeana.eu/concept/music/genre/Cabaret">
    <skos:prefLabel xml:lang="en">Cabaret</skos:prefLabel>
    <skos:prefLabel xml:lang="ar">كباريه</skos:prefLabel>
    <skos:prefLabel xml:lang="bg">Кабаре</skos:prefLabel>
    <skos:prefLabel xml:lang="ca">Cabaret</skos:prefLabel>
    <skos:prefLabel xml:lang="hr">Kabaret</skos:prefLabel>
    <skos:prefLabel xml:lang="cs">Kabaret</skos:prefLabel>
    <skos:prefLabel xml:lang="da">Kabaret</skos:prefLabel>
    <skos:prefLabel xml:lang="nl">Cabaret</skos:prefLabel>
    <skos:prefLabel xml:lang="et">Kabaree</skos:prefLabel>
    <skos:prefLabel xml:lang="fi">Kabaree</skos:prefLabel>
    <skos:prefLabel xml:lang="fr">Cabaret</skos:prefLabel>
    <skos:prefLabel xml:lang="de">Kabarett</skos:prefLabel>
    <skos:prefLabel xml:lang="hu">Kabaré</skos:prefLabel>
    <skos:prefLabel xml:lang="id">Kabaret</skos:prefLabel>
    <skos:prefLabel xml:lang="it">Cabaret</skos:prefLabel>
    <skos:prefLabel xml:lang="ja">キャバレー</skos:prefLabel>
    <skos:prefLabel xml:lang="ko">카바레</skos:prefLabel>
    <skos:prefLabel xml:lang="lv">Kabarē</skos:prefLabel>
    <skos:prefLabel xml:lang="no">Kabaret</skos:prefLabel>
    <skos:prefLabel xml:lang="fa">کاباره</skos:prefLabel>
    <skos:prefLabel xml:lang="pl">Kabaret</skos:prefLabel>
    <skos:prefLabel xml:lang="pt">Cabaré</skos:prefLabel>
    <skos:prefLabel xml:lang="ro">Cabaret</skos:prefLabel>
    <skos:prefLabel xml:lang="ru">Кабаре</skos:prefLabel>
    <skos:prefLabel xml:lang="sr">Кабаре</skos:prefLabel>
    <skos:prefLabel xml:lang="sk">Kabaret</skos:prefLabel>
    <skos:prefLabel xml:lang="sl">Kabaret</skos:prefLabel>
    <skos:prefLabel xml:lang="es">Cabaré</skos:prefLabel>
    <skos:prefLabel xml:lang="sv">Kabaré</skos:prefLabel>
    <skos:prefLabel xml:lang="th">คาบาเรต์</skos:prefLabel>
    <skos:prefLabel xml:lang="tr">Kabare</skos:prefLabel>
    <skos:prefLabel xml:lang="uk">Кабаре</skos:prefLabel>
    <skos:prefLabel xml:lang="vi">Cabaret</skos:prefLabel>
    <skos:closeMatch rdf:resource="http://rdf.freebase.com/ns/m.0g64p"/>
    <skos:broader rdf:resource="http://data.europeana.eu/concept/music/genre/Fusion_(music)_fusions"/>
    <skos:definition xml:lang="en">Cabaret is a form of entertainment featuring music, song, dance,
      recitation or drama. It is mainly distinguished by the performance venue, such as in a
      restaurant, pub or nightclub with a stage for performances. The audience, often dining or
      drinking, does not typically dance but usually sits at tables. Performances are usually
      introduced by a master of ceremonies or MC. The entertainment is often oriented towards adult
      audiences. &lt;p&gt; Cabaret also sometimes refers to a Mediterranean-style brothel – a bar
      with tables and women who mingle with and entertain the clientele. Traditionally these
      establishments can also feature some form of stage entertainment, often singers and dancers or
      burlesque entertainers.</skos:definition>
    <skos:exactMatch xml:lang="en">http://dbpedia.org/resource/Cabaret</skos:exactMatch>
    <skos:inScheme rdf:resource="http://data.europeana.eu/concept/music/genre/Music_Genre_Scheme"/>
    <skos:altLabel xml:lang="en">Cabaret</skos:altLabel>
  </skos:Concept>

  <skos:Concept rdf:about="http://data.europeana.eu/concept/music/genre/Chacarera">
    <skos:prefLabel xml:lang="en">Chacarera</skos:prefLabel>
    <skos:prefLabel xml:lang="ca">Chacarera</skos:prefLabel>
    <skos:prefLabel xml:lang="fr">Chacarera</skos:prefLabel>
    <skos:prefLabel xml:lang="de">Chacarera</skos:prefLabel>
    <skos:prefLabel xml:lang="it">Chacarera</skos:prefLabel>
    <skos:prefLabel xml:lang="ja">チャカレーラ</skos:prefLabel>
    <skos:prefLabel xml:lang="pl">Chacarera</skos:prefLabel>
    <skos:prefLabel xml:lang="pt">Chacarera</skos:prefLabel>
    <skos:prefLabel xml:lang="es">Chacarera</skos:prefLabel>
    <skos:closeMatch rdf:resource="http://rdf.freebase.com/ns/m.05lzyf"/>
    <skos:broader
      rdf:resource="http://data.europeana.eu/concept/music/genre/Latin_American_music_traditional"/>
    <skos:definition xml:lang="en">The Chacarera is a dance and music originating in Argentina. It
      is a genre of folk music that, for many Argentines, serves as a rural counterpart to the
      cosmopolitan imagery of the Tango. A dance form played by contemporary musicians as soloists
      or in small ensembles of voice, guitar, violin and bombo drum, the Chacarera is often
      legitimized by its “origin” in the remote province of Santiago del Estero. It is also the
      product of a romanticized construction of national identity projected by urban cultural
      institutions and disseminated through the mass media.</skos:definition>
    <skos:exactMatch xml:lang="en">http://dbpedia.org/resource/Chacarera</skos:exactMatch>
    <skos:inScheme rdf:resource="http://data.europeana.eu/concept/music/genre/Music_Genre_Scheme"/>
    <skos:altLabel xml:lang="en">Chacarera</skos:altLabel>
  </skos:Concept>

  <skos:Concept rdf:about="http://data.europeana.eu/concept/music/genre/Chanson">
    <skos:prefLabel xml:lang="en">Chanson</skos:prefLabel>
    <skos:prefLabel xml:lang="ar">شانسون</skos:prefLabel>
    <skos:prefLabel xml:lang="bg">Шансон</skos:prefLabel>
    <skos:prefLabel xml:lang="hr">Šansona</skos:prefLabel>
    <skos:prefLabel xml:lang="cs">Šanson</skos:prefLabel>
    <skos:prefLabel xml:lang="da">Chanson française</skos:prefLabel>
    <skos:prefLabel xml:lang="nl">Chanson</skos:prefLabel>
    <skos:prefLabel xml:lang="et">Šansoon</skos:prefLabel>
    <skos:prefLabel xml:lang="fi">Chanson</skos:prefLabel>
    <skos:prefLabel xml:lang="fr">Chanson française</skos:prefLabel>
    <skos:prefLabel xml:lang="de">Chanson</skos:prefLabel>
    <skos:prefLabel xml:lang="el">Σανσόν</skos:prefLabel>
    <skos:prefLabel xml:lang="hu">Sanzon</skos:prefLabel>
    <skos:prefLabel xml:lang="it">Chanson</skos:prefLabel>
    <skos:prefLabel xml:lang="ja">シャンソン</skos:prefLabel>
    <skos:prefLabel xml:lang="ko">샹송</skos:prefLabel>
    <skos:prefLabel xml:lang="no">Chanson</skos:prefLabel>
    <skos:prefLabel xml:lang="pl">Chanson</skos:prefLabel>
    <skos:prefLabel xml:lang="pt">Chanson</skos:prefLabel>
    <skos:prefLabel xml:lang="ru">Шансон</skos:prefLabel>
    <skos:prefLabel xml:lang="sr">Шансона</skos:prefLabel>
    <skos:prefLabel xml:lang="sk">Šansón</skos:prefLabel>
    <skos:prefLabel xml:lang="sl">Šanson</skos:prefLabel>
    <skos:prefLabel xml:lang="es">Chanson</skos:prefLabel>
    <skos:prefLabel xml:lang="sv">Chanson</skos:prefLabel>
    <skos:prefLabel xml:lang="tr">Chanson</skos:prefLabel>
    <skos:prefLabel xml:lang="uk">Шансон</skos:prefLabel>
    <skos:prefLabel xml:lang="vi">Chanson</skos:prefLabel>
    <skos:closeMatch rdf:resource="http://rdf.freebase.com/ns/m.024sbq"/>
    <skos:broader rdf:resource="http://data.europeana.eu/concept/music/genre/Art_music"/>
    <skos:definition xml:lang="en">A chanson is in general any lyric-driven French song, usually
      polyphonic and secular. A singer specializing in chansons is known as a &quot;chanteur&quot;
      or &quot;chanteuse&quot;, a collection of chansons, especially from the late Middle Ages and
      Renaissance, is also known as a chansonnier.</skos:definition>
    <skos:exactMatch xml:lang="en">http://dbpedia.org/resource/Chanson</skos:exactMatch>
    <skos:inScheme rdf:resource="http://data.europeana.eu/concept/music/genre/Music_Genre_Scheme"/>
    <skos:altLabel xml:lang="en">Chanson</skos:altLabel>
  </skos:Concept>

  <skos:Concept rdf:about="http://data.europeana.eu/concept/music/genre/Chicago_blues">
    <skos:prefLabel xml:lang="en">Chicago blues</skos:prefLabel>
    <skos:prefLabel xml:lang="bg">Чикагски блус</skos:prefLabel>
    <skos:prefLabel xml:lang="ca">Chicago blues</skos:prefLabel>
    <skos:prefLabel xml:lang="cs">Chicago blues</skos:prefLabel>
    <skos:prefLabel xml:lang="nl">Chicago blues</skos:prefLabel>
    <skos:prefLabel xml:lang="fr">Chicago blues</skos:prefLabel>
    <skos:prefLabel xml:lang="de">Chicago Blues</skos:prefLabel>
    <skos:prefLabel xml:lang="it">Chicago blues</skos:prefLabel>
    <skos:prefLabel xml:lang="ja">シカゴ・ブルース</skos:prefLabel>
    <skos:prefLabel xml:lang="no">Chicago-blues</skos:prefLabel>
    <skos:prefLabel xml:lang="pl">Blues chicagowski</skos:prefLabel>
    <skos:prefLabel xml:lang="pt">Chicago blues</skos:prefLabel>
    <skos:prefLabel xml:lang="ru">Чикагский блюз</skos:prefLabel>
    <skos:prefLabel xml:lang="es">Chicago blues</skos:prefLabel>
    <skos:closeMatch rdf:resource="http://rdf.freebase.com/ns/m.01730d"/>
    <skos:broader rdf:resource="http://data.europeana.eu/concept/music/genre/Blues"/>
    <skos:definition xml:lang="en">The Chicago blues is a form of blues music indigenous to Chicago,
      Illinois. Chicago blues is a type of urban blues. Urban blues evolved from classic blues as a
      result of the great depression and developed in the first half of the twentieth century during
      the Great Migration, when Black workers moved from the Southern United States into the
      industrial cities of the Northern United States such as Chicago. &lt;p&gt; Urban blues started
      in Chicago and St. Louis, as music created by part-time musicians playing as street musicians,
      at rent parties, and other events within the black community. For example, bottleneck
      guitarist Kokomo Arnold was a steelworker and had a moonshine business that was far more
      profitable than his music. &lt;p&gt; One of the most important early incubators for Chicago
      blues was the open air market on Maxwell street. The Maxwell street market was one of the
      largest open air markets in the nation. Residents of the black community would frequent it to
      buy and sell just about anything. It was a natural location for blues musicians to perform.
      The standard path for blues musicians was to start out as street musicians and at house
      parties and to eventually make their way to blues clubs.</skos:definition>
    <skos:exactMatch xml:lang="en">http://dbpedia.org/resource/Chicago_blues</skos:exactMatch>
    <skos:inScheme rdf:resource="http://data.europeana.eu/concept/music/genre/Music_Genre_Scheme"/>
    <skos:altLabel xml:lang="en">Chicago blues</skos:altLabel>
  </skos:Concept>

  <skos:Concept rdf:about="http://data.europeana.eu/concept/music/genre/Cool_jazz">
    <skos:prefLabel xml:lang="en">Cool jazz</skos:prefLabel>
    <skos:prefLabel xml:lang="ca">Cool</skos:prefLabel>
    <skos:prefLabel xml:lang="hr">Cool jazz</skos:prefLabel>
    <skos:prefLabel xml:lang="cs">Cool jazz</skos:prefLabel>
    <skos:prefLabel xml:lang="da">Cool jazz</skos:prefLabel>
    <skos:prefLabel xml:lang="nl">Cooljazz</skos:prefLabel>
    <skos:prefLabel xml:lang="et">Cool jazz</skos:prefLabel>
    <skos:prefLabel xml:lang="fi">Cool jazz</skos:prefLabel>
    <skos:prefLabel xml:lang="fr">Cool jazz</skos:prefLabel>
    <skos:prefLabel xml:lang="de">Cool Jazz</skos:prefLabel>
    <skos:prefLabel xml:lang="el">Κουλ τζαζ</skos:prefLabel>
    <skos:prefLabel xml:lang="hu">Cool jazz</skos:prefLabel>
    <skos:prefLabel xml:lang="it">Cool jazz</skos:prefLabel>
    <skos:prefLabel xml:lang="ja">クール・ジャズ</skos:prefLabel>
    <skos:prefLabel xml:lang="ko">쿨 재즈</skos:prefLabel>
    <skos:prefLabel xml:lang="no">Cool jazz</skos:prefLabel>
    <skos:prefLabel xml:lang="fa">کول جز</skos:prefLabel>
    <skos:prefLabel xml:lang="pl">Cool jazz</skos:prefLabel>
    <skos:prefLabel xml:lang="pt">Cool jazz</skos:prefLabel>
    <skos:prefLabel xml:lang="ru">Кул-джаз</skos:prefLabel>
    <skos:prefLabel xml:lang="sr">Кул</skos:prefLabel>
    <skos:prefLabel xml:lang="es">Cool</skos:prefLabel>
    <skos:prefLabel xml:lang="sv">Cool jazz</skos:prefLabel>
    <skos:prefLabel xml:lang="uk">Кул-джаз</skos:prefLabel>
    <skos:closeMatch rdf:resource="http://rdf.freebase.com/ns/m.01ppfv"/>
    <skos:broader rdf:resource="http://data.europeana.eu/concept/music/genre/Jazz"/>
    <skos:definition xml:lang="en">Cool jazz is a style of modern jazz music that arose following
      the Second World War. It is characterized by its relaxed tempos and lighter tone, in contrast
      to the bebop style. Cool jazz often employs formal arrangements and incorporates elements of
      classical music.</skos:definition>
    <skos:exactMatch xml:lang="en">http://dbpedia.org/resource/Cool_jazz</skos:exactMatch>
    <skos:inScheme rdf:resource="http://data.europeana.eu/concept/music/genre/Music_Genre_Scheme"/>
    <skos:altLabel xml:lang="en">Cool jazz</skos:altLabel>
  </skos:Concept>

  <skos:Concept rdf:about="http://data.europeana.eu/concept/music/genre/Corrido">
    <skos:prefLabel xml:lang="en">Corrido</skos:prefLabel>
    <skos:prefLabel xml:lang="nl">Corrido</skos:prefLabel>
    <skos:prefLabel xml:lang="fil">Korido</skos:prefLabel>
    <skos:prefLabel xml:lang="fr">Corrido</skos:prefLabel>
    <skos:prefLabel xml:lang="de">Corrido</skos:prefLabel>
    <skos:prefLabel xml:lang="hu">Corrido</skos:prefLabel>
    <skos:prefLabel xml:lang="it">Corrido</skos:prefLabel>
    <skos:prefLabel xml:lang="ja">コッリド</skos:prefLabel>
    <skos:prefLabel xml:lang="ru">Корридо</skos:prefLabel>
    <skos:prefLabel xml:lang="es">Corrido</skos:prefLabel>
    <skos:closeMatch rdf:resource="http://rdf.freebase.com/ns/m.04qrwg"/>
    <skos:broader
      rdf:resource="http://data.europeana.eu/concept/music/genre/Latin_American_music_popular"/>
    <skos:definition xml:lang="en">The corrido is a popular narrative song and poetry form, a
      ballad. The songs are often about oppression, history, daily life for peasants, and other
      socially relevant topics. It is still a popular form today in Mexico and was widely popular
      during the Nicaraguan Revolutions of the 20th century. The corrido derives largely from the
      romance, and in its most known form consists of a salutation from the singer and prologue to
      the story, the story itself, and a moral and farewell from the singer.</skos:definition>
    <skos:exactMatch xml:lang="en">http://dbpedia.org/resource/Corrido</skos:exactMatch>
    <skos:inScheme rdf:resource="http://data.europeana.eu/concept/music/genre/Music_Genre_Scheme"/>
    <skos:altLabel xml:lang="en">Corrido</skos:altLabel>
  </skos:Concept>

  <skos:Concept rdf:about="http://data.europeana.eu/concept/music/genre/Country">
    <skos:prefLabel xml:lang="en">Country</skos:prefLabel>
    <skos:prefLabel xml:lang="ar">موسيقى الريف</skos:prefLabel>
    <skos:prefLabel xml:lang="bg">Кънтри</skos:prefLabel>
    <skos:prefLabel xml:lang="ca">Country</skos:prefLabel>
    <skos:prefLabel xml:lang="hr">Country</skos:prefLabel>
    <skos:prefLabel xml:lang="cs">Country</skos:prefLabel>
    <skos:prefLabel xml:lang="da">Country</skos:prefLabel>
    <skos:prefLabel xml:lang="nl">Countrymuziek</skos:prefLabel>
    <skos:prefLabel xml:lang="et">Kantrimuusika</skos:prefLabel>
    <skos:prefLabel xml:lang="fil">Country</skos:prefLabel>
    <skos:prefLabel xml:lang="fi">Country</skos:prefLabel>
    <skos:prefLabel xml:lang="fr">Musique country</skos:prefLabel>
    <skos:prefLabel xml:lang="de">Country-Musik</skos:prefLabel>
    <skos:prefLabel xml:lang="el">Κάντρι</skos:prefLabel>
    <skos:prefLabel xml:lang="hi">देशी संगीत</skos:prefLabel>
    <skos:prefLabel xml:lang="hu">Country</skos:prefLabel>
    <skos:prefLabel xml:lang="id">Musik country</skos:prefLabel>
    <skos:prefLabel xml:lang="it">Country</skos:prefLabel>
    <skos:prefLabel xml:lang="ja">カントリー・ミュージック</skos:prefLabel>
    <skos:prefLabel xml:lang="ko">컨트리 음악</skos:prefLabel>
    <skos:prefLabel xml:lang="lv">Kantrī mūzika</skos:prefLabel>
    <skos:prefLabel xml:lang="lt">Country muzika</skos:prefLabel>
    <skos:prefLabel xml:lang="no">Country</skos:prefLabel>
    <skos:prefLabel xml:lang="fa">موسیقی کانتری</skos:prefLabel>
    <skos:prefLabel xml:lang="pl">Muzyka country</skos:prefLabel>
    <skos:prefLabel xml:lang="pt">Música country</skos:prefLabel>
    <skos:prefLabel xml:lang="ro">Country</skos:prefLabel>
    <skos:prefLabel xml:lang="ru">Кантри</skos:prefLabel>
    <skos:prefLabel xml:lang="sr">Кантри музика</skos:prefLabel>
    <skos:prefLabel xml:lang="sk">Country</skos:prefLabel>
    <skos:prefLabel xml:lang="sl">Country</skos:prefLabel>
    <skos:prefLabel xml:lang="es">Country</skos:prefLabel>
    <skos:prefLabel xml:lang="sv">Countrymusik</skos:prefLabel>
    <skos:prefLabel xml:lang="th">คันทรี</skos:prefLabel>
    <skos:prefLabel xml:lang="tr">Country</skos:prefLabel>
    <skos:prefLabel xml:lang="uk">Кантрі</skos:prefLabel>
    <skos:prefLabel xml:lang="vi">Nhạc đồng quê</skos:prefLabel>
    <skos:closeMatch rdf:resource="http://rdf.freebase.com/ns/m.01lyv"/>
    <skos:broader rdf:resource="http://data.europeana.eu/concept/music/genre/Popular_music"/>
    <skos:definition xml:lang="en">Country music is a genre of American popular music that
      originated in Southern United States in the 1920s. It takes its roots from the southeastern
      genre of American folk music and Western music. Blues modes have been used extensively
      throughout its recorded history. Country music often consists of ballads and dance tunes with
      generally simple forms and harmonies accompanied by mostly string instruments such as banjos,
      electric and acoustic guitars, fiddles, and harmonicas. &lt;p&gt; The term country music
      gained popularity in the 1940s in preference to the earlier term hillbilly music, it came to
      encompass Western music, which evolved parallel to hillbilly music from similar roots, in the
      mid-20th century. The term country music is used today to describe many styles and sub genres.
      The origins of country music are the folk music of mostly white, working-class Americans, who
      blended popular songs, Irish and Celtic fiddle tunes, traditional ballads, and cowboy songs,
      along with African American blues and various musical traditions from European immigrant
      communities.</skos:definition>
    <skos:exactMatch xml:lang="en">http://dbpedia.org/resource/Country</skos:exactMatch>
    <skos:inScheme rdf:resource="http://data.europeana.eu/concept/music/genre/Music_Genre_Scheme"/>
    <skos:altLabel xml:lang="en">Country music</skos:altLabel>
    <skos:altLabel xml:lang="en">Country &amp; Western</skos:altLabel>
    <skos:altLabel xml:lang="en">Country and Western</skos:altLabel>
    <skos:altLabel xml:lang="en">Country</skos:altLabel>
  </skos:Concept>

  <skos:Concept rdf:about="http://data.europeana.eu/concept/music/genre/Country_rock">
    <skos:prefLabel xml:lang="en">Country rock</skos:prefLabel>
    <skos:prefLabel xml:lang="cs">Country rock</skos:prefLabel>
    <skos:prefLabel xml:lang="da">Country rock</skos:prefLabel>
    <skos:prefLabel xml:lang="nl">Countryrock</skos:prefLabel>
    <skos:prefLabel xml:lang="fi">Country rock</skos:prefLabel>
    <skos:prefLabel xml:lang="fr">Country rock</skos:prefLabel>
    <skos:prefLabel xml:lang="de">Country-Rock</skos:prefLabel>
    <skos:prefLabel xml:lang="hu">Country rock</skos:prefLabel>
    <skos:prefLabel xml:lang="it">Country rock</skos:prefLabel>
    <skos:prefLabel xml:lang="ja">カントリーロック</skos:prefLabel>
    <skos:prefLabel xml:lang="ko">컨트리 록</skos:prefLabel>
    <skos:prefLabel xml:lang="no">Countryrock</skos:prefLabel>
    <skos:prefLabel xml:lang="pl">Country rock</skos:prefLabel>
    <skos:prefLabel xml:lang="pt">Country rock</skos:prefLabel>
    <skos:prefLabel xml:lang="ro">Country rock</skos:prefLabel>
    <skos:prefLabel xml:lang="ru">Кантри-рок</skos:prefLabel>
    <skos:prefLabel xml:lang="sk">Country rock</skos:prefLabel>
    <skos:prefLabel xml:lang="sl">Country rock</skos:prefLabel>
    <skos:prefLabel xml:lang="es">Country rock</skos:prefLabel>
    <skos:prefLabel xml:lang="sv">Countryrock</skos:prefLabel>
    <skos:prefLabel xml:lang="th">คันทรี ร็อก</skos:prefLabel>
    <skos:prefLabel xml:lang="uk">Кантрі-рок</skos:prefLabel>
    <skos:closeMatch rdf:resource="http://rdf.freebase.com/ns/m.0mhfr"/>
    <skos:broader rdf:resource="http://data.europeana.eu/concept/music/genre/Country_music_fusions"/>
    <skos:definition xml:lang="en">Country rock is a subgenre of country music, formed from the
      fusion of rock with country. The term is generally used to refer to the wave of rock musicians
      who began to record country-flavored records in the late 1960s and early 1970s, beginning with
      Bob Dylan and The Byrds and reaching its greatest popularity in the 1970s with artists like
      Linda Ronstadt and the Eagles.</skos:definition>
    <skos:exactMatch xml:lang="en">http://dbpedia.org/resource/Country_rock</skos:exactMatch>
    <skos:inScheme rdf:resource="http://data.europeana.eu/concept/music/genre/Music_Genre_Scheme"/>
    <skos:altLabel xml:lang="en">Country rock</skos:altLabel>
  </skos:Concept>

  <skos:Concept rdf:about="http://data.europeana.eu/concept/music/genre/Cueca">
    <skos:prefLabel xml:lang="en">Cueca</skos:prefLabel>
    <skos:prefLabel xml:lang="ca">Cueca</skos:prefLabel>
    <skos:prefLabel xml:lang="fr">Cueca</skos:prefLabel>
    <skos:prefLabel xml:lang="de">Cueca</skos:prefLabel>
    <skos:prefLabel xml:lang="it">Cueca</skos:prefLabel>
    <skos:prefLabel xml:lang="ja">クエッカ</skos:prefLabel>
    <skos:prefLabel xml:lang="pt">Cueca</skos:prefLabel>
    <skos:prefLabel xml:lang="es">Cueca</skos:prefLabel>
    <skos:prefLabel xml:lang="sv">Cueca</skos:prefLabel>
    <skos:closeMatch rdf:resource="http://rdf.freebase.com/ns/m.04nm_x"/>
    <skos:broader
      rdf:resource="http://data.europeana.eu/concept/music/genre/Latin_American_music_traditional"/>
    <skos:definition xml:lang="en">Cueca is a family of musical styles and associated dances from
      Argentina, Chile and Bolivia. In Chile, the cueca holds the status of national dance, where it
      was officially selected on September 18, 1979.</skos:definition>
    <skos:exactMatch xml:lang="en">http://dbpedia.org/resource/Cueca</skos:exactMatch>
    <skos:inScheme rdf:resource="http://data.europeana.eu/concept/music/genre/Music_Genre_Scheme"/>
    <skos:altLabel xml:lang="en">Cueca</skos:altLabel>
  </skos:Concept>

  <skos:Concept rdf:about="http://data.europeana.eu/concept/music/genre/Cumbia">
    <skos:prefLabel xml:lang="en">Cumbia</skos:prefLabel>
    <skos:prefLabel xml:lang="ca">Cúmbia</skos:prefLabel>
    <skos:prefLabel xml:lang="da">Cumbia</skos:prefLabel>
    <skos:prefLabel xml:lang="nl">Cumbia</skos:prefLabel>
    <skos:prefLabel xml:lang="fi">Cumbia</skos:prefLabel>
    <skos:prefLabel xml:lang="fr">Cumbia</skos:prefLabel>
    <skos:prefLabel xml:lang="de">Cumbia</skos:prefLabel>
    <skos:prefLabel xml:lang="hu">Cumbia</skos:prefLabel>
    <skos:prefLabel xml:lang="it">Cumbia</skos:prefLabel>
    <skos:prefLabel xml:lang="ja">クンビア</skos:prefLabel>
    <skos:prefLabel xml:lang="ko">꿈비아</skos:prefLabel>
    <skos:prefLabel xml:lang="lt">Kumbija</skos:prefLabel>
    <skos:prefLabel xml:lang="no">Cumbia</skos:prefLabel>
    <skos:prefLabel xml:lang="pl">Cumbia</skos:prefLabel>
    <skos:prefLabel xml:lang="pt">Cúmbia</skos:prefLabel>
    <skos:prefLabel xml:lang="ro">Cumbia</skos:prefLabel>
    <skos:prefLabel xml:lang="ru">Кумбия</skos:prefLabel>
    <skos:prefLabel xml:lang="es">Cumbia</skos:prefLabel>
    <skos:prefLabel xml:lang="sv">Cumbia</skos:prefLabel>
    <skos:prefLabel xml:lang="tr">Kumbiya</skos:prefLabel>
    <skos:closeMatch rdf:resource="http://rdf.freebase.com/ns/m.02ccj9"/>
    <skos:broader
      rdf:resource="http://data.europeana.eu/concept/music/genre/Latin_American_music_traditional"/>
    <skos:definition xml:lang="en">Cumbia is a music genre popular throughout Latin America. The
      Cumbia originated in Colombia's Caribbean coastal region and Panama, from the musical and
      cultural fusion of Native Colombians and Panamanians, slaves brought from Africa, and the
      Spanish during colonial times in the old country of Pocabuy, which is located in Colombia's
      Momposina Depression and in the northeast of Panama, in the ancient palenques of the Congo
      nation. &lt;p&gt; Cumbia began as a courtship dance practiced among the African population,
      which was later mixed with Amerindian steps and European and African instruments and musical
      characteristics. Cumbia is very popular in the Andean region and the Southern Cone, and is for
      example more popular than the salsa in many parts of these regions.</skos:definition>
    <skos:exactMatch xml:lang="en">http://dbpedia.org/resource/Cumbia</skos:exactMatch>
    <skos:inScheme rdf:resource="http://data.europeana.eu/concept/music/genre/Music_Genre_Scheme"/>
    <skos:altLabel xml:lang="en">Cumbia</skos:altLabel>
  </skos:Concept>

  <skos:Concept rdf:about="http://data.europeana.eu/concept/music/genre/Cumbia_villera">
    <skos:prefLabel xml:lang="en">Cumbia villera</skos:prefLabel>
    <skos:prefLabel xml:lang="de">Cumbia Villera</skos:prefLabel>
    <skos:prefLabel xml:lang="pt">Cumbia villera</skos:prefLabel>
    <skos:prefLabel xml:lang="es">Cumbia villera</skos:prefLabel>
    <skos:prefLabel xml:lang="sv">Cumbia villera</skos:prefLabel>
    <skos:closeMatch rdf:resource="http://rdf.freebase.com/ns/m.06wdnn"/>
    <skos:broader
      rdf:resource="http://data.europeana.eu/concept/music/genre/Latin_American_music_traditional"/>
    <skos:definition xml:lang="en">Cumbia villera is a typically Argentine form of cumbia music born
      in the villas miseria around Buenos Aires and then popularized in other large urban
      settlements.</skos:definition>
    <skos:exactMatch xml:lang="en">http://dbpedia.org/resource/Cumbia_villera</skos:exactMatch>
    <skos:inScheme rdf:resource="http://data.europeana.eu/concept/music/genre/Music_Genre_Scheme"/>
    <skos:altLabel xml:lang="en">Cumbia villera</skos:altLabel>
  </skos:Concept>

  <skos:Concept rdf:about="http://data.europeana.eu/concept/music/genre/Dance">
    <skos:prefLabel xml:lang="en">Dance</skos:prefLabel>
    <skos:prefLabel xml:lang="ca">Dance</skos:prefLabel>
    <skos:prefLabel xml:lang="hr">Dance</skos:prefLabel>
    <skos:prefLabel xml:lang="cs">Taneční hudba</skos:prefLabel>
    <skos:prefLabel xml:lang="nl">Dance music</skos:prefLabel>
    <skos:prefLabel xml:lang="et">Tantsumuusika</skos:prefLabel>
    <skos:prefLabel xml:lang="fr">Musique de danse</skos:prefLabel>
    <skos:prefLabel xml:lang="de">Tanzmusik</skos:prefLabel>
    <skos:prefLabel xml:lang="hu">Dance</skos:prefLabel>
    <skos:prefLabel xml:lang="id">Musik dansa</skos:prefLabel>
    <skos:prefLabel xml:lang="it">Musica dance</skos:prefLabel>
    <skos:prefLabel xml:lang="ja">ダンス ミュージック</skos:prefLabel>
    <skos:prefLabel xml:lang="ko">댄스 음악</skos:prefLabel>
    <skos:prefLabel xml:lang="lv">Deju mūzika</skos:prefLabel>
    <skos:prefLabel xml:lang="lt">Šokių muzika</skos:prefLabel>
    <skos:prefLabel xml:lang="fa">موسیقی رقص</skos:prefLabel>
    <skos:prefLabel xml:lang="pl">Dance</skos:prefLabel>
    <skos:prefLabel xml:lang="pt">Dance music</skos:prefLabel>
    <skos:prefLabel xml:lang="ro">Muzică dance</skos:prefLabel>
    <skos:prefLabel xml:lang="ru">Танцевальная музыка</skos:prefLabel>
    <skos:prefLabel xml:lang="sr">Денс музика</skos:prefLabel>
    <skos:prefLabel xml:lang="sk">Tanečná hudba</skos:prefLabel>
    <skos:prefLabel xml:lang="sl">Dance music</skos:prefLabel>
    <skos:prefLabel xml:lang="es">Dance</skos:prefLabel>
    <skos:prefLabel xml:lang="sv">Dansmusik</skos:prefLabel>
    <skos:prefLabel xml:lang="th">เพลงแดนซ์</skos:prefLabel>
    <skos:prefLabel xml:lang="tr">Dans müziği</skos:prefLabel>
    <skos:prefLabel xml:lang="uk">Танцювальна музика</skos:prefLabel>
    <skos:prefLabel xml:lang="vi">Nhạc dance</skos:prefLabel>
    <skos:closeMatch rdf:resource="http://rdf.freebase.com/ns/m.0ggx5q"/>
    <skos:broader rdf:resource="http://data.europeana.eu/concept/music/genre/Electronic_music"/>
    <skos:definition xml:lang="en">Dance music is music composed specifically to facilitate or
      accompany dancing. It can be either a whole musical piece or part of a larger musical
      arrangement. In terms of performance, the major categories are live dance music and recorded
      dance music.</skos:definition>
    <skos:exactMatch xml:lang="en">http://dbpedia.org/resource/Dance</skos:exactMatch>
    <skos:inScheme rdf:resource="http://data.europeana.eu/concept/music/genre/Music_Genre_Scheme"/>
    <skos:altLabel xml:lang="en">Dance music</skos:altLabel>
  </skos:Concept>

  <skos:Concept rdf:about="http://data.europeana.eu/concept/music/genre/Disco">
    <skos:prefLabel xml:lang="en">Disco</skos:prefLabel>
    <skos:prefLabel xml:lang="ar">ديسكو</skos:prefLabel>
    <skos:prefLabel xml:lang="bg">Диско</skos:prefLabel>
    <skos:prefLabel xml:lang="ca">Música disco</skos:prefLabel>
    <skos:prefLabel xml:lang="hr">Disco</skos:prefLabel>
    <skos:prefLabel xml:lang="cs">Disco</skos:prefLabel>
    <skos:prefLabel xml:lang="da">Disco</skos:prefLabel>
    <skos:prefLabel xml:lang="nl">Disco</skos:prefLabel>
    <skos:prefLabel xml:lang="et">Diskomuusika</skos:prefLabel>
    <skos:prefLabel xml:lang="fi">Disko</skos:prefLabel>
    <skos:prefLabel xml:lang="fr">Disco</skos:prefLabel>
    <skos:prefLabel xml:lang="de">Disco</skos:prefLabel>
    <skos:prefLabel xml:lang="hu">Diszkó</skos:prefLabel>
    <skos:prefLabel xml:lang="id">Disko</skos:prefLabel>
    <skos:prefLabel xml:lang="it">Disco music</skos:prefLabel>
    <skos:prefLabel xml:lang="ja">ディスコ</skos:prefLabel>
    <skos:prefLabel xml:lang="ko">디스코</skos:prefLabel>
    <skos:prefLabel xml:lang="lv">Disko mūzika</skos:prefLabel>
    <skos:prefLabel xml:lang="lt">Disko</skos:prefLabel>
    <skos:prefLabel xml:lang="no">Disco</skos:prefLabel>
    <skos:prefLabel xml:lang="fa">دیسکو</skos:prefLabel>
    <skos:prefLabel xml:lang="pl">Disco</skos:prefLabel>
    <skos:prefLabel xml:lang="pt">Música disco</skos:prefLabel>
    <skos:prefLabel xml:lang="ro">Muzică disco</skos:prefLabel>
    <skos:prefLabel xml:lang="ru">Диско</skos:prefLabel>
    <skos:prefLabel xml:lang="sr">Диско музика</skos:prefLabel>
    <skos:prefLabel xml:lang="sk">Disko</skos:prefLabel>
    <skos:prefLabel xml:lang="es">Música disco</skos:prefLabel>
    <skos:prefLabel xml:lang="sv">Disco</skos:prefLabel>
    <skos:prefLabel xml:lang="th">ดิสโก้</skos:prefLabel>
    <skos:prefLabel xml:lang="tr">Disko</skos:prefLabel>
    <skos:prefLabel xml:lang="uk">Диско</skos:prefLabel>
    <skos:closeMatch rdf:resource="http://rdf.freebase.com/ns/m.026z9"/>
    <skos:broader
      rdf:resource="http://data.europeana.eu/concept/music/genre/Electronic_music_fusions"/>
    <skos:definition xml:lang="en">Disco is a genre of music that was popular in the 1970s, though
      it has since enjoyed brief resurgences including the present day. The term is derived from
      discothèque. Its initial audiences were club-goers from the African American, GLBTQ, Italian
      American, Latino, and psychedelic communities in New York City and Philadelphia during the
      late 1960s and early 1970s. Disco also was a reaction against both the domination of rock
      music and the stigmatization of dance music by the counterculture during this period. Women
      embraced disco as well, and the music eventually expanded to several other popular groups of
      the time. &lt;p&gt; In what is considered a forerunner to disco-style clubs, New York City DJ
      David Mancuso opened The Loft, a members-only private dance club set in his own home, in
      February 1970. AllMusic claims some have argued that Isaac Hayes and Barry White were playing
      what would be called disco music as early as 1971. According to the music guide, there is
      disagreement as to what the first disco song was.</skos:definition>
    <skos:exactMatch xml:lang="en">http://dbpedia.org/resource/Disco</skos:exactMatch>
    <skos:inScheme rdf:resource="http://data.europeana.eu/concept/music/genre/Music_Genre_Scheme"/>
    <skos:altLabel xml:lang="en">Disco music</skos:altLabel>
    <skos:altLabel xml:lang="en">Disco</skos:altLabel>
  </skos:Concept>

  <skos:Concept rdf:about="http://data.europeana.eu/concept/music/genre/Dixieland">
    <skos:prefLabel xml:lang="en">Dixieland</skos:prefLabel>
    <skos:prefLabel xml:lang="ca">Dixieland</skos:prefLabel>
    <skos:prefLabel xml:lang="hr">Dixieland</skos:prefLabel>
    <skos:prefLabel xml:lang="nl">Dixieland</skos:prefLabel>
    <skos:prefLabel xml:lang="et">Diksiländ</skos:prefLabel>
    <skos:prefLabel xml:lang="fi">Dixieland</skos:prefLabel>
    <skos:prefLabel xml:lang="fr">Dixieland</skos:prefLabel>
    <skos:prefLabel xml:lang="de">Dixieland</skos:prefLabel>
    <skos:prefLabel xml:lang="el">Ντίξιλαντ</skos:prefLabel>
    <skos:prefLabel xml:lang="hu">Dixieland</skos:prefLabel>
    <skos:prefLabel xml:lang="id">Dixieland</skos:prefLabel>
    <skos:prefLabel xml:lang="it">Dixieland</skos:prefLabel>
    <skos:prefLabel xml:lang="ja">ディキシーランド・ジャズ</skos:prefLabel>
    <skos:prefLabel xml:lang="ko">딕실랜드</skos:prefLabel>
    <skos:prefLabel xml:lang="lv">Diksilends</skos:prefLabel>
    <skos:prefLabel xml:lang="no">New Orleans jazz</skos:prefLabel>
    <skos:prefLabel xml:lang="fa">دیکسی‌لند</skos:prefLabel>
    <skos:prefLabel xml:lang="pt">Dixieland</skos:prefLabel>
    <skos:prefLabel xml:lang="ro">Dixieland</skos:prefLabel>
    <skos:prefLabel xml:lang="ru">Диксиленд</skos:prefLabel>
    <skos:prefLabel xml:lang="sl">Dixieland</skos:prefLabel>
    <skos:prefLabel xml:lang="es">Dixieland</skos:prefLabel>
    <skos:prefLabel xml:lang="sv">Dixieland</skos:prefLabel>
    <skos:prefLabel xml:lang="uk">Диксиленд</skos:prefLabel>
    <skos:closeMatch rdf:resource="http://rdf.freebase.com/ns/m.09xw2"/>
    <skos:broader rdf:resource="http://data.europeana.eu/concept/music/genre/Jazz"/>
    <skos:definition xml:lang="en">Dixieland music or New Orleans Jazz, sometimes referred to as Hot
      jazz or Early Jazz, is a style of jazz music which developed in New Orleans at the start of
      the 20th century, and was spread to Chicago and New York City by New Orleans bands in the
      1910s. &lt;p&gt; Well-known jazz standard songs from the Dixieland era, such as &quot;Basin
      Street Blues&quot; and &quot;When the Saints Go Marching In&quot;, are known even to non-jazz
      fans. With its beginnings in Dixieland and Riverboat jazz, and progression to Chicago-style
      jazz or hot jazz as developed by Louis Armstrong and others, Chicago-style jazz or hot jazz
      was also a transition and combination of 2-beat to 4-beat, introducing Swing in its earliest
      form. &lt;p&gt; Hot jazz or Chicago-style jazz was also the current original music that began
      the Lindy Hop dance craze as it developed in Harlem.</skos:definition>
    <skos:exactMatch xml:lang="en">http://dbpedia.org/resource/Dixieland</skos:exactMatch>
    <skos:inScheme rdf:resource="http://data.europeana.eu/concept/music/genre/Music_Genre_Scheme"/>
    <skos:altLabel xml:lang="en">Dixieland jazz</skos:altLabel>
    <skos:altLabel xml:lang="en">New Orleans Jazz</skos:altLabel>
    <skos:altLabel xml:lang="en">Hot Jazz</skos:altLabel>
    <skos:altLabel xml:lang="en">Early Jazz</skos:altLabel>
    <skos:altLabel xml:lang="en">Dixieland</skos:altLabel>
  </skos:Concept>

  <skos:Concept rdf:about="http://data.europeana.eu/concept/music/genre/Doo-wop">
    <skos:prefLabel xml:lang="en">Doo-wop</skos:prefLabel>
    <skos:prefLabel xml:lang="bg">Ду-уап</skos:prefLabel>
    <skos:prefLabel xml:lang="ca">Doo-wop</skos:prefLabel>
    <skos:prefLabel xml:lang="hr">Doo wop</skos:prefLabel>
    <skos:prefLabel xml:lang="cs">Doo-wop</skos:prefLabel>
    <skos:prefLabel xml:lang="nl">Doo-wop</skos:prefLabel>
    <skos:prefLabel xml:lang="fi">Doo-wop</skos:prefLabel>
    <skos:prefLabel xml:lang="fr">Doo-wop</skos:prefLabel>
    <skos:prefLabel xml:lang="de">Doo Wop</skos:prefLabel>
    <skos:prefLabel xml:lang="hu">Doo-wop</skos:prefLabel>
    <skos:prefLabel xml:lang="it">Doo-wop</skos:prefLabel>
    <skos:prefLabel xml:lang="ja">ドゥーワップ</skos:prefLabel>
    <skos:prefLabel xml:lang="ko">두왑</skos:prefLabel>
    <skos:prefLabel xml:lang="no">Doo-wop</skos:prefLabel>
    <skos:prefLabel xml:lang="pl">Doo wop</skos:prefLabel>
    <skos:prefLabel xml:lang="pt">Doo-wop</skos:prefLabel>
    <skos:prefLabel xml:lang="ro">Doo-wop</skos:prefLabel>
    <skos:prefLabel xml:lang="ru">Ду-воп</skos:prefLabel>
    <skos:prefLabel xml:lang="sk">Doo-wop</skos:prefLabel>
    <skos:prefLabel xml:lang="es">Doo wop</skos:prefLabel>
    <skos:prefLabel xml:lang="sv">Doo wop</skos:prefLabel>
    <skos:prefLabel xml:lang="th">ดูวอป</skos:prefLabel>
    <skos:closeMatch rdf:resource="http://rdf.freebase.com/ns/m.0nk3g"/>
    <skos:broader rdf:resource="http://data.europeana.eu/concept/music/genre/Rhythm_and_blues"/>
    <skos:definition xml:lang="en">Doo-wop is a style of rhythm and blues which emerged in African
      American communities in New York, Philadelphia, Chicago, Baltimore, Newark, Pittsburgh,
      Cincinnati, Detroit, Washington D.C and Los Angeles in the 1940s, achieving mainstream
      popularity in the 1950s and early 1960s. Built upon vocal harmony, doo-wop was one of the most
      mainstream, pop-oriented R&amp;B styles of the time. Singer Bill Kenny is often called the
      &quot;Godfather of Doo-wop&quot; for his &quot;top and bottom&quot; format featuring a high
      tenor lead and &quot;talking bass&quot; in the middle of the song. &lt;p&gt; Doo-wop features
      vocal group harmony, nonsense syllables, a simple beat, sometimes little or no
      instrumentation, and simple music and lyrics.</skos:definition>
    <skos:exactMatch xml:lang="en">http://dbpedia.org/resource/Doo-wop</skos:exactMatch>
    <skos:inScheme rdf:resource="http://data.europeana.eu/concept/music/genre/Music_Genre_Scheme"/>
    <skos:altLabel xml:lang="en">Doo-wop</skos:altLabel>
  </skos:Concept>

  <skos:Concept rdf:about="http://data.europeana.eu/concept/music/genre/Drum_and_bass">
    <skos:prefLabel xml:lang="en">Drum and bass</skos:prefLabel>
    <skos:prefLabel xml:lang="bg">Дръм енд бейс</skos:prefLabel>
    <skos:prefLabel xml:lang="ca">Drum and bass</skos:prefLabel>
    <skos:prefLabel xml:lang="hr">Drum and bass</skos:prefLabel>
    <skos:prefLabel xml:lang="cs">Drum and Bass</skos:prefLabel>
    <skos:prefLabel xml:lang="da">Drum and bass</skos:prefLabel>
    <skos:prefLabel xml:lang="nl">Drum and bass</skos:prefLabel>
    <skos:prefLabel xml:lang="et">Drum and bass</skos:prefLabel>
    <skos:prefLabel xml:lang="fi">Drum’n’bass</skos:prefLabel>
    <skos:prefLabel xml:lang="fr">Drum and bass</skos:prefLabel>
    <skos:prefLabel xml:lang="de">Drum and Bass</skos:prefLabel>
    <skos:prefLabel xml:lang="hu">Drum and bass</skos:prefLabel>
    <skos:prefLabel xml:lang="it">Drum and bass</skos:prefLabel>
    <skos:prefLabel xml:lang="ja">ドラムンベース</skos:prefLabel>
    <skos:prefLabel xml:lang="ko">드럼 앤 베이스</skos:prefLabel>
    <skos:prefLabel xml:lang="lv">Drum and bass</skos:prefLabel>
    <skos:prefLabel xml:lang="lt">Drum and bass</skos:prefLabel>
    <skos:prefLabel xml:lang="no">Drum and Bass</skos:prefLabel>
    <skos:prefLabel xml:lang="fa">درام اند بیس</skos:prefLabel>
    <skos:prefLabel xml:lang="pl">Drum and bass</skos:prefLabel>
    <skos:prefLabel xml:lang="pt">Drum and bass</skos:prefLabel>
    <skos:prefLabel xml:lang="ro">Drum and bass</skos:prefLabel>
    <skos:prefLabel xml:lang="ru">Драм-н-бэйс</skos:prefLabel>
    <skos:prefLabel xml:lang="sr">Drum and bass</skos:prefLabel>
    <skos:prefLabel xml:lang="sk">Drum and bass</skos:prefLabel>
    <skos:prefLabel xml:lang="es">Drum and bass</skos:prefLabel>
    <skos:prefLabel xml:lang="sv">Drum and bass</skos:prefLabel>
    <skos:prefLabel xml:lang="th">ดรัมแอนด์เบส</skos:prefLabel>
    <skos:prefLabel xml:lang="uk">Драм-енд-бейс</skos:prefLabel>
    <skos:closeMatch rdf:resource="http://rdf.freebase.com/ns/m.0283d"/>
    <skos:broader rdf:resource="http://data.europeana.eu/concept/music/genre/Electronic_music"/>
    <skos:definition xml:lang="en">Drum and bass is a type of electronic music which emerged in
      England in the early 1990s. The genre is characterized by fast breakbeats with heavy bass and
      sub-bass lines.</skos:definition>
    <skos:exactMatch xml:lang="en">http://dbpedia.org/resource/Drum_and_bass</skos:exactMatch>
    <skos:inScheme rdf:resource="http://data.europeana.eu/concept/music/genre/Music_Genre_Scheme"/>
    <skos:altLabel xml:lang="en">dnb</skos:altLabel>
    <skos:altLabel xml:lang="en">drum n bass</skos:altLabel>
    <skos:altLabel xml:lang="en">drum ’n’ bass</skos:altLabel>
    <skos:altLabel xml:lang="en">d'n'b</skos:altLabel>
    <skos:altLabel xml:lang="en">drum &amp; bass</skos:altLabel>
    <skos:altLabel xml:lang="en">d&amp;b</skos:altLabel>
    <skos:altLabel xml:lang="en">Drum and bass</skos:altLabel>
  </skos:Concept>

  <skos:Concept rdf:about="http://data.europeana.eu/concept/music/genre/Electronic_music">
    <skos:prefLabel xml:lang="en">Electronic music</skos:prefLabel>
    <skos:closeMatch rdf:resource="http://rdf.freebase.com/ns/m.02lkt"/>
    <skos:broader rdf:resource="http://data.europeana.eu/concept/music/genre/Popular_music"/>
    <skos:exactMatch xml:lang="en">http://dbpedia.org/resource/Electronic_music</skos:exactMatch>
    <skos:inScheme rdf:resource="http://data.europeana.eu/concept/music/genre/Music_Genre_Scheme"/>
    <skos:altLabel xml:lang="en">Electronic music</skos:altLabel>
  </skos:Concept>

  <skos:Concept rdf:about="http://data.europeana.eu/concept/music/genre/Emo">
    <skos:prefLabel xml:lang="en">Emo</skos:prefLabel>
    <skos:prefLabel xml:lang="ar">إيمو</skos:prefLabel>
    <skos:prefLabel xml:lang="bg">Емо</skos:prefLabel>
    <skos:prefLabel xml:lang="ca">Emocore</skos:prefLabel>
    <skos:prefLabel xml:lang="hr">Emo</skos:prefLabel>
    <skos:prefLabel xml:lang="cs">Emo</skos:prefLabel>
    <skos:prefLabel xml:lang="da">Emo</skos:prefLabel>
    <skos:prefLabel xml:lang="nl">Emocore</skos:prefLabel>
    <skos:prefLabel xml:lang="et">Emo</skos:prefLabel>
    <skos:prefLabel xml:lang="fi">Emo</skos:prefLabel>
    <skos:prefLabel xml:lang="fr">Emo</skos:prefLabel>
    <skos:prefLabel xml:lang="de">Emo</skos:prefLabel>
    <skos:prefLabel xml:lang="el">Emo</skos:prefLabel>
    <skos:prefLabel xml:lang="hu">Emo</skos:prefLabel>
    <skos:prefLabel xml:lang="id">Emo</skos:prefLabel>
    <skos:prefLabel xml:lang="it">Emo</skos:prefLabel>
    <skos:prefLabel xml:lang="ja">エモ</skos:prefLabel>
    <skos:prefLabel xml:lang="ko">이모</skos:prefLabel>
    <skos:prefLabel xml:lang="lv">Emo</skos:prefLabel>
    <skos:prefLabel xml:lang="lt">Emo</skos:prefLabel>
    <skos:prefLabel xml:lang="ms">Emo</skos:prefLabel>
    <skos:prefLabel xml:lang="no">Emo</skos:prefLabel>
    <skos:prefLabel xml:lang="fa">ایمو</skos:prefLabel>
    <skos:prefLabel xml:lang="pl">Emo</skos:prefLabel>
    <skos:prefLabel xml:lang="pt">Emo</skos:prefLabel>
    <skos:prefLabel xml:lang="ro">Emo</skos:prefLabel>
    <skos:prefLabel xml:lang="ru">Эмо</skos:prefLabel>
    <skos:prefLabel xml:lang="sr">Емо</skos:prefLabel>
    <skos:prefLabel xml:lang="sk">Emo</skos:prefLabel>
    <skos:prefLabel xml:lang="sl">Emo</skos:prefLabel>
    <skos:prefLabel xml:lang="es">Emo</skos:prefLabel>
    <skos:prefLabel xml:lang="sv">Emo</skos:prefLabel>
    <skos:prefLabel xml:lang="th">อีโม</skos:prefLabel>
    <skos:prefLabel xml:lang="tr">Emocore</skos:prefLabel>
    <skos:prefLabel xml:lang="uk">Емо</skos:prefLabel>
    <skos:closeMatch rdf:resource="http://rdf.freebase.com/ns/m.0pm85"/>
    <skos:broader rdf:resource="http://data.europeana.eu/concept/music/genre/Rock_music"/>
    <skos:definition xml:lang="en">Emo is a style of rock music characterized by melodic
      musicianship and expressive, often confessional, lyrics. It originated in the mid-1980s
      hardcore punk movement of Washington, D.C., where it was known as &quot;emotional
      hardcore&quot; or &quot;emocore&quot; and pioneered by bands such as Rites of Spring and
      Embrace. &lt;p&gt; As the style was echoed by contemporary American punk rock bands, its sound
      and meaning shifted and changed, blending with pop punk and indie rock and encapsulated in the
      early 1990s by groups such as Jawbreaker and Sunny Day Real Estate. By the mid-1990s numerous
      emo acts emerged from the Midwestern and Central United States, and several independent record
      labels began to specialize in the style. &lt;p&gt; Emo broke into mainstream culture in the
      early 2000s with the platinum-selling success of Jimmy Eat World and Dashboard Confessional
      and the emergence of the subgenre &quot;screamo&quot;. In recent years the term
      &quot;emo&quot; has been applied by critics and journalists to a variety of artists, including
      multiplatinum acts and groups with disparate styles and sounds.</skos:definition>
    <skos:exactMatch xml:lang="en">http://dbpedia.org/resource/Emo</skos:exactMatch>
    <skos:inScheme rdf:resource="http://data.europeana.eu/concept/music/genre/Music_Genre_Scheme"/>
    <skos:altLabel xml:lang="en">emotional hardcore</skos:altLabel>
    <skos:altLabel xml:lang="en">Emo</skos:altLabel>
  </skos:Concept>

  <skos:Concept rdf:about="http://data.europeana.eu/concept/music/genre/Enka">
    <skos:prefLabel xml:lang="en">Enka</skos:prefLabel>
    <skos:prefLabel xml:lang="ca">Enka</skos:prefLabel>
    <skos:prefLabel xml:lang="nl">Enka</skos:prefLabel>
    <skos:prefLabel xml:lang="fi">Enka</skos:prefLabel>
    <skos:prefLabel xml:lang="fr">Enka</skos:prefLabel>
    <skos:prefLabel xml:lang="de">Enka</skos:prefLabel>
    <skos:prefLabel xml:lang="id">Enka</skos:prefLabel>
    <skos:prefLabel xml:lang="it">Enka</skos:prefLabel>
    <skos:prefLabel xml:lang="ja">演歌</skos:prefLabel>
    <skos:prefLabel xml:lang="ko">엔카</skos:prefLabel>
    <skos:prefLabel xml:lang="pl">Enka</skos:prefLabel>
    <skos:prefLabel xml:lang="pt">Enka</skos:prefLabel>
    <skos:prefLabel xml:lang="ru">Энка</skos:prefLabel>
    <skos:prefLabel xml:lang="es">Enka</skos:prefLabel>
    <skos:prefLabel xml:lang="sv">Enka</skos:prefLabel>
    <skos:prefLabel xml:lang="th">เอ็งกะ</skos:prefLabel>
    <skos:prefLabel xml:lang="vi">Enka</skos:prefLabel>
    <skos:closeMatch rdf:resource="http://rdf.freebase.com/ns/m.015tgr"/>
    <skos:broader rdf:resource="http://data.europeana.eu/concept/music/genre/Asian_music_pop"/>
    <skos:definition xml:lang="en">Enka is a popular Japanese music genre considered to resemble
      traditional Japanese music stylistically. Modern enka, however, is a relatively recent musical
      form which arose in the context of such postwar expressions of modern Japanese nonmaterial
      nationalism as nihonjinron, while adopting a more traditional musical style in its vocalism
      than ry?k?ka music, popular during the prewar years. &lt;p&gt; Modern enka, as developed in
      the postwar era, is a form of sentimental ballad music. Some of the first modern enka singers
      were Hachiro Kasuga, Michiya Mihashi, and Hideo Murata. The revival of enka in its modern form
      is said to date from 1969, when Keiko Fuji made her debut. Male singer is famous as Kiyoshi
      Hikawa.</skos:definition>
    <skos:exactMatch xml:lang="en">http://dbpedia.org/resource/Enka</skos:exactMatch>
    <skos:inScheme rdf:resource="http://data.europeana.eu/concept/music/genre/Music_Genre_Scheme"/>
    <skos:altLabel xml:lang="en">Enka</skos:altLabel>
  </skos:Concept>

  <skos:Concept rdf:about="http://data.europeana.eu/concept/music/genre/Fado">
    <skos:prefLabel xml:lang="en">Fado</skos:prefLabel>
    <skos:prefLabel xml:lang="ar">فادو</skos:prefLabel>
    <skos:prefLabel xml:lang="bg">Фадо</skos:prefLabel>
    <skos:prefLabel xml:lang="ca">Fado</skos:prefLabel>
    <skos:prefLabel xml:lang="hr">Fado</skos:prefLabel>
    <skos:prefLabel xml:lang="cs">Fado</skos:prefLabel>
    <skos:prefLabel xml:lang="da">Fado</skos:prefLabel>
    <skos:prefLabel xml:lang="nl">Fado</skos:prefLabel>
    <skos:prefLabel xml:lang="et">Fado</skos:prefLabel>
    <skos:prefLabel xml:lang="fi">Fado</skos:prefLabel>
    <skos:prefLabel xml:lang="fr">Fado</skos:prefLabel>
    <skos:prefLabel xml:lang="de">Fado</skos:prefLabel>
    <skos:prefLabel xml:lang="el">Φάντο</skos:prefLabel>
    <skos:prefLabel xml:lang="hu">Fado</skos:prefLabel>
    <skos:prefLabel xml:lang="id">Fado</skos:prefLabel>
    <skos:prefLabel xml:lang="it">Fado</skos:prefLabel>
    <skos:prefLabel xml:lang="ja">ファド</skos:prefLabel>
    <skos:prefLabel xml:lang="ko">파두</skos:prefLabel>
    <skos:prefLabel xml:lang="es-419">Fado</skos:prefLabel>
    <skos:prefLabel xml:lang="lt">Fado</skos:prefLabel>
    <skos:prefLabel xml:lang="no">Fado</skos:prefLabel>
    <skos:prefLabel xml:lang="fa">فادو</skos:prefLabel>
    <skos:prefLabel xml:lang="pl">Fado</skos:prefLabel>
    <skos:prefLabel xml:lang="pt">Fado</skos:prefLabel>
    <skos:prefLabel xml:lang="ro">Fado</skos:prefLabel>
    <skos:prefLabel xml:lang="ru">Фаду</skos:prefLabel>
    <skos:prefLabel xml:lang="sr">Фадо</skos:prefLabel>
    <skos:prefLabel xml:lang="sk">Fado</skos:prefLabel>
    <skos:prefLabel xml:lang="es">Fado</skos:prefLabel>
    <skos:prefLabel xml:lang="sv">Fado</skos:prefLabel>
    <skos:prefLabel xml:lang="tr">Fado</skos:prefLabel>
    <skos:prefLabel xml:lang="uk">Фаду</skos:prefLabel>
    <skos:closeMatch rdf:resource="http://rdf.freebase.com/ns/m.0178qc"/>
    <skos:broader rdf:resource="http://data.europeana.eu/concept/music/genre/Art_music"/>
    <skos:definition xml:lang="en">Fado is a music genre which can be traced to the 1820s in
      Portugal, but probably with much earlier origins. Fado historian and scholar Rui Vieira Nery
      states that &quot;the only reliable information on the history of Fado was orally transmitted
      and goes back to the 1820s and 1830s at best. But even that information was frequently
      modified within the generational transmission process that made it reach us today.&quot; In
      popular belief, fado is a form of music characterized by mournful tunes and lyrics, often
      about the sea or the life of the poor, and infused with a characteristic sentiment of
      resignation, fatefulness and melancholia. However, although the origins are difficult to
      trace, today fado is regarded, by many, as simply a form of song which can be about anything,
      but must follow a certain structure. The music is usually linked to the Portuguese word
      saudade which symbolizes the feeling of loss. Famous singers of fado include Amália Rodrigues,
      Dulce Pontes, Carlos do Carmo, Mariza, Mafalda Arnauth, António Zambujo, Ana Moura, Camané,
      Helder Moutinho, Aldina Duarte, Joanna Amandoeira, Ricardo Robeiro, Argentina Santos,
      Carminho, Mísia, and Cristina Branco.</skos:definition>
    <skos:exactMatch xml:lang="en">http://dbpedia.org/resource/Fado</skos:exactMatch>
    <skos:inScheme rdf:resource="http://data.europeana.eu/concept/music/genre/Music_Genre_Scheme"/>
    <skos:altLabel xml:lang="en">Fado</skos:altLabel>
  </skos:Concept>

  <skos:Concept rdf:about="http://data.europeana.eu/concept/music/genre/Flamenco">
    <skos:prefLabel xml:lang="en">Flamenco</skos:prefLabel>
    <skos:prefLabel xml:lang="ar">فلامنكو</skos:prefLabel>
    <skos:prefLabel xml:lang="bg">Фламенко</skos:prefLabel>
    <skos:prefLabel xml:lang="ca">Música flamenca</skos:prefLabel>
    <skos:prefLabel xml:lang="hr">Flamenco</skos:prefLabel>
    <skos:prefLabel xml:lang="cs">Flamenco</skos:prefLabel>
    <skos:prefLabel xml:lang="da">Flamenco</skos:prefLabel>
    <skos:prefLabel xml:lang="nl">Flamenco</skos:prefLabel>
    <skos:prefLabel xml:lang="et">Flamenko</skos:prefLabel>
    <skos:prefLabel xml:lang="fi">Flamenco</skos:prefLabel>
    <skos:prefLabel xml:lang="fr">Flamenco</skos:prefLabel>
    <skos:prefLabel xml:lang="de">Flamenco</skos:prefLabel>
    <skos:prefLabel xml:lang="el">Φλαμένκο</skos:prefLabel>
    <skos:prefLabel xml:lang="hu">Flamenco</skos:prefLabel>
    <skos:prefLabel xml:lang="id">Flamenco</skos:prefLabel>
    <skos:prefLabel xml:lang="it">Flamenco</skos:prefLabel>
    <skos:prefLabel xml:lang="ja">フラメンコ</skos:prefLabel>
    <skos:prefLabel xml:lang="ko">플라멩코</skos:prefLabel>
    <skos:prefLabel xml:lang="lv">Flamenko</skos:prefLabel>
    <skos:prefLabel xml:lang="lt">Flamenko</skos:prefLabel>
    <skos:prefLabel xml:lang="no">Flamenco</skos:prefLabel>
    <skos:prefLabel xml:lang="fa">فلامنکو</skos:prefLabel>
    <skos:prefLabel xml:lang="pl">Flamenco</skos:prefLabel>
    <skos:prefLabel xml:lang="pt">Flamenco</skos:prefLabel>
    <skos:prefLabel xml:lang="ro">Flamenco</skos:prefLabel>
    <skos:prefLabel xml:lang="ru">Фламенко</skos:prefLabel>
    <skos:prefLabel xml:lang="sr">Фламенко</skos:prefLabel>
    <skos:prefLabel xml:lang="sk">Flamenco</skos:prefLabel>
    <skos:prefLabel xml:lang="sl">Flamenko</skos:prefLabel>
    <skos:prefLabel xml:lang="es">Flamenco</skos:prefLabel>
    <skos:prefLabel xml:lang="sv">Flamenco</skos:prefLabel>
    <skos:prefLabel xml:lang="th">ฟลาเมงโก</skos:prefLabel>
    <skos:prefLabel xml:lang="tr">Flamenko</skos:prefLabel>
    <skos:prefLabel xml:lang="uk">Фламенко</skos:prefLabel>
    <skos:prefLabel xml:lang="vi">Flamenco</skos:prefLabel>
    <skos:closeMatch rdf:resource="http://rdf.freebase.com/ns/m.0326g"/>
    <skos:broader
      rdf:resource="http://data.europeana.eu/concept/music/genre/Latin_American_music_traditional"/>
    <skos:definition xml:lang="en">Flamenco is a form of Spanish folk music and dance from the
      region of Andalusia in southern Spain. It includes cante, toque, baile and palmas. First
      mentioned in literature in 1774, the genre grew out of Andalusian and Romani music and dance
      styles. Flamenco is often associated with the Romani people of Spain and a number of famous
      flamenco artists are of this ethnicity. Flamenco was first recorded in the late 18th century
      but the genre underwent a dramatic development in the late 19th century. &lt;p&gt; In recent
      years flamenco has become popular all over the world and is taught in many countries: in Japan
      there are more academies than there are in Spain. On November 16, 2010 UNESCO declared
      flamenco one of the Masterpieces of the Oral and Intangible Heritage of
      Humanity.</skos:definition>
    <skos:exactMatch xml:lang="en">http://dbpedia.org/resource/Flamenco</skos:exactMatch>
    <skos:inScheme rdf:resource="http://data.europeana.eu/concept/music/genre/Music_Genre_Scheme"/>
    <skos:altLabel xml:lang="en">Flamenco</skos:altLabel>
  </skos:Concept>

  <skos:Concept rdf:about="http://data.europeana.eu/concept/music/genre/Folk">
    <skos:prefLabel xml:lang="en">Folk</skos:prefLabel>
    <skos:prefLabel xml:lang="ca">Poble</skos:prefLabel>
    <skos:prefLabel xml:lang="nl">Volk</skos:prefLabel>
    <skos:prefLabel xml:lang="de">Volk</skos:prefLabel>
    <skos:prefLabel xml:lang="it">Popolo</skos:prefLabel>
    <skos:prefLabel xml:lang="pt">Povo</skos:prefLabel>
    <skos:prefLabel xml:lang="ru">Народ</skos:prefLabel>
    <skos:prefLabel xml:lang="es">Pueblo (sociedad)</skos:prefLabel>
    <skos:prefLabel xml:lang="uk">Народність</skos:prefLabel>
    <skos:closeMatch rdf:resource="http://rdf.freebase.com/ns/m.0fdp85"/>
    <skos:broader rdf:resource="http://data.europeana.eu/concept/music/genre/Popular_music"/>
    <skos:definition xml:lang="en">The English word Folk is derived from a Germanic noun, *fulka
      meaning &quot;people&quot; or &quot;army&quot;. The English word folk has cognates in most of
      the other Germanic languages. Folk may be a Germanic root that is unique to the Germanic
      languages, although Latin vulgus, &quot;the common people&quot;, has been suggested as a
      possible cognate.</skos:definition>
    <skos:exactMatch xml:lang="en">http://dbpedia.org/resource/Folk</skos:exactMatch>
    <skos:inScheme rdf:resource="http://data.europeana.eu/concept/music/genre/Music_Genre_Scheme"/>
    <skos:altLabel xml:lang="en">folk music</skos:altLabel>
    <skos:altLabel xml:lang="en">Folk</skos:altLabel>
  </skos:Concept>

  <skos:Concept rdf:about="http://data.europeana.eu/concept/music/genre/Folk_music">
    <skos:prefLabel xml:lang="en">Folk Music</skos:prefLabel>
    <skos:prefLabel xml:lang="ar">موسيقى فلكلورية</skos:prefLabel>
    <skos:prefLabel xml:lang="ca">Folk</skos:prefLabel>
    <skos:prefLabel xml:lang="hr">Narodna glazba</skos:prefLabel>
    <skos:prefLabel xml:lang="cs">Folk</skos:prefLabel>
    <skos:prefLabel xml:lang="da">Folkemusik</skos:prefLabel>
    <skos:prefLabel xml:lang="nl">Folk</skos:prefLabel>
    <skos:prefLabel xml:lang="et">Rahvamuusika</skos:prefLabel>
    <skos:prefLabel xml:lang="fil">Awiting-bayan</skos:prefLabel>
    <skos:prefLabel xml:lang="fi">Folkmusiikki</skos:prefLabel>
    <skos:prefLabel xml:lang="fr">Musique folk</skos:prefLabel>
    <skos:prefLabel xml:lang="de">Folk</skos:prefLabel>
    <skos:prefLabel xml:lang="el">Φολκ</skos:prefLabel>
    <skos:prefLabel xml:lang="hi">लोक संगीत</skos:prefLabel>
    <skos:prefLabel xml:lang="hu">Népzene</skos:prefLabel>
    <skos:prefLabel xml:lang="id">Lagu daerah</skos:prefLabel>
    <skos:prefLabel xml:lang="it">Musica folk</skos:prefLabel>
    <skos:prefLabel xml:lang="ja">フォークソング</skos:prefLabel>
    <skos:prefLabel xml:lang="ko">포크송</skos:prefLabel>
    <skos:prefLabel xml:lang="lv">Folkmūzika</skos:prefLabel>
    <skos:prefLabel xml:lang="lt">Liaudies muzika</skos:prefLabel>
    <skos:prefLabel xml:lang="ms">Lagu Kedaerahan</skos:prefLabel>
    <skos:prefLabel xml:lang="no">Folkemusikk</skos:prefLabel>
    <skos:prefLabel xml:lang="fa">موسیقی بومی</skos:prefLabel>
    <skos:prefLabel xml:lang="pl">Muzyka folkowa</skos:prefLabel>
    <skos:prefLabel xml:lang="pt">Música folclórica</skos:prefLabel>
    <skos:prefLabel xml:lang="ro">Muzică folk</skos:prefLabel>
    <skos:prefLabel xml:lang="ru">Фолк-музыка</skos:prefLabel>
    <skos:prefLabel xml:lang="sr">Folk muzika</skos:prefLabel>
    <skos:prefLabel xml:lang="sk">Folk</skos:prefLabel>
    <skos:prefLabel xml:lang="sl">Ljudska glasba</skos:prefLabel>
    <skos:prefLabel xml:lang="es">Música folk</skos:prefLabel>
    <skos:prefLabel xml:lang="sv">Folkmusik</skos:prefLabel>
    <skos:prefLabel xml:lang="th">ดนตรีโฟล์ก</skos:prefLabel>
    <skos:prefLabel xml:lang="tr">Halk müziği</skos:prefLabel>
    <skos:prefLabel xml:lang="uk">Фолк-музика</skos:prefLabel>
    <skos:prefLabel xml:lang="vi">Dân ca</skos:prefLabel>
    <skos:prefLabel xml:lang="en">Traditional European Folk</skos:prefLabel>
    <skos:closeMatch rdf:resource="http://rdf.freebase.com/ns/m.02w4v"/>
    <skos:broader rdf:resource="http://data.europeana.eu/concept/music/genre/Popular_music"/>
    <skos:definition xml:lang="en">Folk music includes both traditional music and the genre that
      evolved from it during the 20th century folk revival. The term originated in the 19th century
      but is often applied to music that is older than that. Some types of folk music are also
      called world music. &lt;p&gt; Traditional folk music has been defined in several ways: as
      music transmitted by mouth, as music of the lower classes, and as music with unknown
      composers. It has been contrasted with commercial and classical styles. One meaning often
      given is that of old songs, with no known composers, another is music that has been
      transmitted and evolved by a process of oral transmission or performed by custom over a long
      period of time. &lt;p&gt; Starting in the mid-20th century a new form of popular folk music
      evolved from traditional folk music. This process and period is called the folk revival and
      reached a zenith in the 1960s. This form of music is sometimes called contemporary folk music
      or folk revival music to distinguish it from earlier folk forms. Smaller similar revivals have
      occurred elsewhere in the world at other times, but the term folk music has typically not been
      applied to the new music created during those revivals.</skos:definition>
    <skos:exactMatch xml:lang="en">http://dbpedia.org/resource/Folk_music</skos:exactMatch>
    <skos:inScheme rdf:resource="http://data.europeana.eu/concept/music/genre/Music_Genre_Scheme"/>
    <skos:altLabel xml:lang="en">folk</skos:altLabel>
    <skos:altLabel xml:lang="en">Folk music</skos:altLabel>
  </skos:Concept>

  <skos:Concept rdf:about="http://data.europeana.eu/concept/music/genre/Folk_rock">
    <skos:prefLabel xml:lang="en">Folk Rock</skos:prefLabel>
    <skos:prefLabel xml:lang="bg">Фолк рок</skos:prefLabel>
    <skos:prefLabel xml:lang="ca">Folk rock</skos:prefLabel>
    <skos:prefLabel xml:lang="hr">Folk rock</skos:prefLabel>
    <skos:prefLabel xml:lang="cs">Folk rock</skos:prefLabel>
    <skos:prefLabel xml:lang="da">Folkrock</skos:prefLabel>
    <skos:prefLabel xml:lang="nl">Folkrock</skos:prefLabel>
    <skos:prefLabel xml:lang="et">Folkrokk</skos:prefLabel>
    <skos:prefLabel xml:lang="fi">Folk rock</skos:prefLabel>
    <skos:prefLabel xml:lang="fr">Folk rock</skos:prefLabel>
    <skos:prefLabel xml:lang="de">Folk-Rock</skos:prefLabel>
    <skos:prefLabel xml:lang="hu">Folk-rock</skos:prefLabel>
    <skos:prefLabel xml:lang="id">Folk rock</skos:prefLabel>
    <skos:prefLabel xml:lang="it">Folk rock</skos:prefLabel>
    <skos:prefLabel xml:lang="ja">フォークロック</skos:prefLabel>
    <skos:prefLabel xml:lang="ko">포크 록</skos:prefLabel>
    <skos:prefLabel xml:lang="lv">Folkroks</skos:prefLabel>
    <skos:prefLabel xml:lang="lt">Folkrokas</skos:prefLabel>
    <skos:prefLabel xml:lang="no">Folkrock</skos:prefLabel>
    <skos:prefLabel xml:lang="fa">فولک راک</skos:prefLabel>
    <skos:prefLabel xml:lang="pl">Folk rock</skos:prefLabel>
    <skos:prefLabel xml:lang="pt">Folk rock</skos:prefLabel>
    <skos:prefLabel xml:lang="ru">Фолк-рок</skos:prefLabel>
    <skos:prefLabel xml:lang="sk">Folk rock</skos:prefLabel>
    <skos:prefLabel xml:lang="sl">Folk rock</skos:prefLabel>
    <skos:prefLabel xml:lang="es">Folk rock</skos:prefLabel>
    <skos:prefLabel xml:lang="sv">Folkrock</skos:prefLabel>
    <skos:prefLabel xml:lang="th">โฟล์กร็อก</skos:prefLabel>
    <skos:prefLabel xml:lang="tr">Folk rock</skos:prefLabel>
    <skos:prefLabel xml:lang="uk">Фольк-рок</skos:prefLabel>
    <skos:closeMatch rdf:resource="http://rdf.freebase.com/ns/m.016jny"/>
    <skos:broader rdf:resource="http://data.europeana.eu/concept/music/genre/Rock_music_fusions"/>
    <skos:definition xml:lang="en">Folk rock is a musical genre combining elements of folk music and
      rock music. In its earliest and narrowest sense, the term referred to a genre that arose in
      the United States and the UK around the mid-1960s. The genre was pioneered by the Los Angeles
      band The Byrds, who began playing traditional folk music and Bob Dylan-penned material with
      rock instrumentation, in a style heavily influenced by The Beatles and other British bands.
      The term &quot;folk rock&quot; was itself first coined by the U.S. music press to describe The
      Byrds' music in June 1965, the same month that the band's debut album was issued. The release
      of The Byrds' cover version of Dylan's &quot;Mr. Tambourine Man&quot; and its subsequent
      commercial success initiated the folk rock explosion of the mid-1960s. Dylan himself was also
      influential on the genre, particularly his recordings with an electric rock band on the
      Bringing It All Back Home, Highway 61 Revisited, and Blonde on Blonde albums. Dylan's July 25,
      1965 appearance at the Newport Folk Festival with an electric backing band is also considered
      a pivotal moment in the development of folk rock.</skos:definition>
    <skos:exactMatch xml:lang="en">http://dbpedia.org/resource/Folk_rock</skos:exactMatch>
    <skos:inScheme rdf:resource="http://data.europeana.eu/concept/music/genre/Music_Genre_Scheme"/>
    <skos:altLabel xml:lang="en">Folk rock</skos:altLabel>
  </skos:Concept>

  <skos:Concept rdf:about="http://data.europeana.eu/concept/music/genre/Foxtrot">
    <skos:prefLabel xml:lang="en">Foxtrot</skos:prefLabel>
    <skos:prefLabel xml:lang="ar">فوكستروت</skos:prefLabel>
    <skos:prefLabel xml:lang="ca">Fox lent</skos:prefLabel>
    <skos:prefLabel xml:lang="hr">Foxtrot</skos:prefLabel>
    <skos:prefLabel xml:lang="cs">Foxtrot</skos:prefLabel>
    <skos:prefLabel xml:lang="da">Foxtrot</skos:prefLabel>
    <skos:prefLabel xml:lang="nl">Foxtrot</skos:prefLabel>
    <skos:prefLabel xml:lang="et">Fokstrott</skos:prefLabel>
    <skos:prefLabel xml:lang="fi">Foxtrot</skos:prefLabel>
    <skos:prefLabel xml:lang="fr">Slow fox</skos:prefLabel>
    <skos:prefLabel xml:lang="de">Foxtrott</skos:prefLabel>
    <skos:prefLabel xml:lang="hu">Foxtrott</skos:prefLabel>
    <skos:prefLabel xml:lang="it">Foxtrot</skos:prefLabel>
    <skos:prefLabel xml:lang="ja">フォックストロット</skos:prefLabel>
    <skos:prefLabel xml:lang="no">Foxtrot</skos:prefLabel>
    <skos:prefLabel xml:lang="pl">Fokstrot</skos:prefLabel>
    <skos:prefLabel xml:lang="pt">Foxtrote</skos:prefLabel>
    <skos:prefLabel xml:lang="ro">Foxtrot</skos:prefLabel>
    <skos:prefLabel xml:lang="ru">Фокстрот</skos:prefLabel>
    <skos:prefLabel xml:lang="sr">Фокстрот</skos:prefLabel>
    <skos:prefLabel xml:lang="es">Foxtrot</skos:prefLabel>
    <skos:prefLabel xml:lang="sv">Foxtrot</skos:prefLabel>
    <skos:prefLabel xml:lang="uk">Фокстрот</skos:prefLabel>
    <skos:prefLabel xml:lang="vi">Foxtrot</skos:prefLabel>
    <skos:closeMatch rdf:resource="http://rdf.freebase.com/ns/m.01dyt1"/>
    <skos:broader rdf:resource="http://data.europeana.eu/concept/music/genre/Art_music"/>
    <skos:definition xml:lang="en">The foxtrot is a smooth, progressive dance characterized by long,
      continuous flowing movements across the dance floor. It is danced to big band music. The dance
      is similar in its look to waltz, although the rhythm is in a 4 &lt;p&gt; 4 time signature
      instead of 3 &lt;p&gt; 4. Developed in the 1910s, the foxtrot reached its height of popularity
      in the 1930s, and remains practiced today.</skos:definition>
    <skos:exactMatch xml:lang="en">http://dbpedia.org/resource/Foxtrot</skos:exactMatch>
    <skos:inScheme rdf:resource="http://data.europeana.eu/concept/music/genre/Music_Genre_Scheme"/>
    <skos:altLabel xml:lang="en">Fox trot</skos:altLabel>
    <skos:altLabel xml:lang="en">Foxtrot</skos:altLabel>
  </skos:Concept>

  <skos:Concept rdf:about="http://data.europeana.eu/concept/music/genre/Free_jazz">
    <skos:prefLabel xml:lang="en">Free jazz</skos:prefLabel>
    <skos:prefLabel xml:lang="ca">Free-jazz</skos:prefLabel>
    <skos:prefLabel xml:lang="hr">Free jazz</skos:prefLabel>
    <skos:prefLabel xml:lang="cs">Free jazz</skos:prefLabel>
    <skos:prefLabel xml:lang="da">Free jazz</skos:prefLabel>
    <skos:prefLabel xml:lang="nl">Free jazz</skos:prefLabel>
    <skos:prefLabel xml:lang="et">Free jazz</skos:prefLabel>
    <skos:prefLabel xml:lang="fi">Free jazz</skos:prefLabel>
    <skos:prefLabel xml:lang="fr">Free jazz</skos:prefLabel>
    <skos:prefLabel xml:lang="de">Free Jazz</skos:prefLabel>
    <skos:prefLabel xml:lang="hu">Free jazz</skos:prefLabel>
    <skos:prefLabel xml:lang="it">Free jazz</skos:prefLabel>
    <skos:prefLabel xml:lang="ja">フリー・ジャズ</skos:prefLabel>
    <skos:prefLabel xml:lang="ko">프리 재즈</skos:prefLabel>
    <skos:prefLabel xml:lang="lv">Brīvais džezs</skos:prefLabel>
    <skos:prefLabel xml:lang="lt">Laisvasis džiazas</skos:prefLabel>
    <skos:prefLabel xml:lang="no">Frijazz</skos:prefLabel>
    <skos:prefLabel xml:lang="fa">جاز آزاد</skos:prefLabel>
    <skos:prefLabel xml:lang="pl">Free jazz</skos:prefLabel>
    <skos:prefLabel xml:lang="pt">Free jazz</skos:prefLabel>
    <skos:prefLabel xml:lang="ru">Фри-джаз</skos:prefLabel>
    <skos:prefLabel xml:lang="es">Free jazz</skos:prefLabel>
    <skos:prefLabel xml:lang="sv">Frijazz</skos:prefLabel>
    <skos:prefLabel xml:lang="uk">Фрі-джаз</skos:prefLabel>
    <skos:closeMatch rdf:resource="http://rdf.freebase.com/ns/m.0p9xd"/>
    <skos:broader rdf:resource="http://data.europeana.eu/concept/music/genre/Jazz_fusions"/>
    <skos:definition xml:lang="en">Free jazz is an approach to jazz music that was first developed
      in the 1950s and 1960s. Though the music produced by free jazz composers varied widely, the
      common feature was a dissatisfaction with the limitations of bebop, hard bop, and modal jazz,
      which had developed in the 1940s and 1950s. Each in their own way, free jazz musicians
      attempted to alter, extend, or break down the conventions of jazz, often by discarding
      hitherto invariable features of jazz, such as fixed chord changes or tempos. While usually
      considered experimental and avant-garde, free jazz has also oppositely been conceived as an
      attempt to return jazz to its &quot;primitive&quot;, often religious roots, and emphasis on
      collective improvisation. &lt;p&gt; Free jazz is strongly associated with the 1950s
      innovations of Ornette Coleman and Cecil Taylor and the later works of saxophonist John
      Coltrane. Other important pioneers include Charles Mingus, Eric Dolphy, Albert Ayler, Archie
      Shepp, Joe Maneri and Sun Ra. Although today &quot;free jazz&quot; is the generally used term,
      many other terms were used to describe the loosely defined movement, including
      &quot;avant-garde&quot;, &quot;energy music&quot; and &quot;The New
      Thing&quot;.</skos:definition>
    <skos:exactMatch xml:lang="en">http://dbpedia.org/resource/Free_jazz</skos:exactMatch>
    <skos:inScheme rdf:resource="http://data.europeana.eu/concept/music/genre/Music_Genre_Scheme"/>
    <skos:altLabel xml:lang="en">Free jazz</skos:altLabel>
  </skos:Concept>

  <skos:Concept rdf:about="http://data.europeana.eu/concept/music/genre/Funk">
    <skos:prefLabel xml:lang="en">Funk</skos:prefLabel>
    <skos:prefLabel xml:lang="ar">فانك</skos:prefLabel>
    <skos:prefLabel xml:lang="bg">Фънк</skos:prefLabel>
    <skos:prefLabel xml:lang="ca">Funk</skos:prefLabel>
    <skos:prefLabel xml:lang="hr">Funk</skos:prefLabel>
    <skos:prefLabel xml:lang="cs">Funk</skos:prefLabel>
    <skos:prefLabel xml:lang="da">Funk</skos:prefLabel>
    <skos:prefLabel xml:lang="nl">Funk</skos:prefLabel>
    <skos:prefLabel xml:lang="et">Funk</skos:prefLabel>
    <skos:prefLabel xml:lang="fi">Funk</skos:prefLabel>
    <skos:prefLabel xml:lang="fr">Funk</skos:prefLabel>
    <skos:prefLabel xml:lang="de">Funk</skos:prefLabel>
    <skos:prefLabel xml:lang="el">Φανκ</skos:prefLabel>
    <skos:prefLabel xml:lang="hu">Funk</skos:prefLabel>
    <skos:prefLabel xml:lang="id">Funk</skos:prefLabel>
    <skos:prefLabel xml:lang="it">Funk</skos:prefLabel>
    <skos:prefLabel xml:lang="ja">ファンク</skos:prefLabel>
    <skos:prefLabel xml:lang="ko">펑크</skos:prefLabel>
    <skos:prefLabel xml:lang="lv">Fankmūzika</skos:prefLabel>
    <skos:prefLabel xml:lang="lt">Fank</skos:prefLabel>
    <skos:prefLabel xml:lang="no">Funk</skos:prefLabel>
    <skos:prefLabel xml:lang="fa">فانک</skos:prefLabel>
    <skos:prefLabel xml:lang="pl">Funk</skos:prefLabel>
    <skos:prefLabel xml:lang="pt">Funk</skos:prefLabel>
    <skos:prefLabel xml:lang="ro">Muzică funk</skos:prefLabel>
    <skos:prefLabel xml:lang="ru">Фанк</skos:prefLabel>
    <skos:prefLabel xml:lang="sr">Фанк</skos:prefLabel>
    <skos:prefLabel xml:lang="sk">Funk</skos:prefLabel>
    <skos:prefLabel xml:lang="sl">Funk</skos:prefLabel>
    <skos:prefLabel xml:lang="es">Funk</skos:prefLabel>
    <skos:prefLabel xml:lang="sv">Funk</skos:prefLabel>
    <skos:prefLabel xml:lang="th">ฟังก์</skos:prefLabel>
    <skos:prefLabel xml:lang="tr">Funk</skos:prefLabel>
    <skos:prefLabel xml:lang="uk">Фанк</skos:prefLabel>
    <skos:closeMatch rdf:resource="http://rdf.freebase.com/ns/m.02x8m"/>
    <skos:broader rdf:resource="http://data.europeana.eu/concept/music/genre/Rhythm_and_blues"/>
    <skos:definition xml:lang="en">Funk is a music genre that originated in the mid to late 1960s
      when African-American musicians created a rhythmic, danceable new form of music through a
      mixture of soul music, jazz, and R&amp;B. Funk de-emphasizes melody and harmony and brings a
      strong rhythmic groove of electric bass and drums to the foreground. Funk songs are often
      based on an extended vamp on a single chord, distinguishing it from R&amp;B and soul songs,
      which are built on chord progressions. &lt;p&gt; Like much African-inspired music, funk
      typically consists of a complex groove with rhythm instruments such as electric guitar,
      electric bass, Hammond organ, and drums playing interlocking rhythms. Funk bands sometimes
      have a horn section of several saxophones, trumpets, and in some cases, a trombone, which
      plays rhythmic &quot;hits&quot;. &lt;p&gt; Many of the most famous bands in the genre also
      played disco and soul extensively. Funk samples have been used extensively in genres including
      hip hop, house music, and drum and bass. It is also the main influence of go-go, a subgenre
      associated with funk.</skos:definition>
    <skos:exactMatch xml:lang="en">http://dbpedia.org/resource/Funk</skos:exactMatch>
    <skos:inScheme rdf:resource="http://data.europeana.eu/concept/music/genre/Music_Genre_Scheme"/>
    <skos:altLabel xml:lang="en">Funk music</skos:altLabel>
    <skos:altLabel xml:lang="en">Funk</skos:altLabel>
  </skos:Concept>

  <skos:Concept rdf:about="http://data.europeana.eu/concept/music/genre/Funk_carioca">
    <skos:prefLabel xml:lang="en">Funk carioca</skos:prefLabel>
    <skos:prefLabel xml:lang="nl">Funk carioca</skos:prefLabel>
    <skos:prefLabel xml:lang="fi">Baile funk</skos:prefLabel>
    <skos:prefLabel xml:lang="fr">Baile funk</skos:prefLabel>
    <skos:prefLabel xml:lang="de">Rio Funk</skos:prefLabel>
    <skos:prefLabel xml:lang="pl">Rio funk</skos:prefLabel>
    <skos:prefLabel xml:lang="pt">Funk carioca</skos:prefLabel>
    <skos:prefLabel xml:lang="es">Funk carioca</skos:prefLabel>
    <skos:prefLabel xml:lang="sv">Baile Funk</skos:prefLabel>
    <skos:closeMatch rdf:resource="http://rdf.freebase.com/ns/m.05q7ms"/>
    <skos:broader
      rdf:resource="http://data.europeana.eu/concept/music/genre/Latin_American_music_popular"/>
    <skos:definition xml:lang="en">Funk carioca, favela funk and, elsewhere in the world, baile
      funk, is a type of dance music from Rio de Janeiro, derived from Miami bass. &lt;p&gt;
      &quot;Baile funk&quot;, in Brazil, refers not to the music, but to the actual parties or
      discothèques in which the music is played. Although originated in Rio, funk carioca has become
      increasingly popular amongst working classes in other parts of Brazil. In the whole country,
      funk carioca is most often simply known as funk, although it is very different musically from
      what funk means in most other places.</skos:definition>
    <skos:exactMatch xml:lang="en">http://dbpedia.org/resource/Funk_carioca</skos:exactMatch>
    <skos:inScheme rdf:resource="http://data.europeana.eu/concept/music/genre/Music_Genre_Scheme"/>
    <skos:altLabel xml:lang="en">Funk carioca</skos:altLabel>
  </skos:Concept>

  <skos:Concept rdf:about="http://data.europeana.eu/concept/music/genre/Gagaku">
    <skos:prefLabel xml:lang="en">Gagaku</skos:prefLabel>
    <skos:prefLabel xml:lang="hr">Gagaku</skos:prefLabel>
    <skos:prefLabel xml:lang="nl">Gagaku</skos:prefLabel>
    <skos:prefLabel xml:lang="fi">Gagaku</skos:prefLabel>
    <skos:prefLabel xml:lang="fr">Gagaku</skos:prefLabel>
    <skos:prefLabel xml:lang="de">Gagaku</skos:prefLabel>
    <skos:prefLabel xml:lang="id">Gagaku</skos:prefLabel>
    <skos:prefLabel xml:lang="it">Gagaku</skos:prefLabel>
    <skos:prefLabel xml:lang="ja">雅楽</skos:prefLabel>
    <skos:prefLabel xml:lang="fa">گاگاکو</skos:prefLabel>
    <skos:prefLabel xml:lang="pl">Gagaku</skos:prefLabel>
    <skos:prefLabel xml:lang="ro">Gagaku</skos:prefLabel>
    <skos:prefLabel xml:lang="ru">Гагаку</skos:prefLabel>
    <skos:prefLabel xml:lang="es">Gagaku</skos:prefLabel>
    <skos:closeMatch rdf:resource="http://rdf.freebase.com/ns/m.029v_q"/>
    <skos:broader rdf:resource="http://data.europeana.eu/concept/music/genre/Art_music"/>
    <skos:definition xml:lang="en">Gagaku is a type of Japanese classical music that has been
      performed at the Imperial Court in Kyoto for several centuries. It consists of three primary
      repertoires: &lt;p&gt; Native Shinto religious music and folk songs and dance, called kuniburi
      no utamai &lt;p&gt; A Goguryeo and Manchurian form, called komagaku &lt;p&gt; A Chinese and
      South Asia form, called t?gaku. &lt;p&gt; Gagaku, like sh?my?, employs the yo scale, a
      pentatonic scale with ascending intervals of two, three, two, two, and three semitones between
      the five scale tones.</skos:definition>
    <skos:exactMatch xml:lang="en">http://dbpedia.org/resource/Gagaku</skos:exactMatch>
    <skos:inScheme rdf:resource="http://data.europeana.eu/concept/music/genre/Music_Genre_Scheme"/>
    <skos:altLabel xml:lang="en">Gagaku</skos:altLabel>
  </skos:Concept>

  <skos:Concept rdf:about="http://data.europeana.eu/concept/music/genre/Gamelan">
    <skos:prefLabel xml:lang="en">Gamelan</skos:prefLabel>
    <skos:prefLabel xml:lang="ar">غاميلان</skos:prefLabel>
    <skos:prefLabel xml:lang="bg">Гамелан</skos:prefLabel>
    <skos:prefLabel xml:lang="ca">Gamelan</skos:prefLabel>
    <skos:prefLabel xml:lang="cs">Gamelan</skos:prefLabel>
    <skos:prefLabel xml:lang="nl">Gamelan</skos:prefLabel>
    <skos:prefLabel xml:lang="et">Gamelan</skos:prefLabel>
    <skos:prefLabel xml:lang="fi">Gamelan</skos:prefLabel>
    <skos:prefLabel xml:lang="fr">Gamelan</skos:prefLabel>
    <skos:prefLabel xml:lang="de">Gamelan</skos:prefLabel>
    <skos:prefLabel xml:lang="hi">गमेलन</skos:prefLabel>
    <skos:prefLabel xml:lang="hu">Gamelán</skos:prefLabel>
    <skos:prefLabel xml:lang="id">Gamelan</skos:prefLabel>
    <skos:prefLabel xml:lang="it">Gamelan</skos:prefLabel>
    <skos:prefLabel xml:lang="ja">ガムラン</skos:prefLabel>
    <skos:prefLabel xml:lang="ko">가믈란</skos:prefLabel>
    <skos:prefLabel xml:lang="lt">Gamelanas</skos:prefLabel>
    <skos:prefLabel xml:lang="ms">Gamelan</skos:prefLabel>
    <skos:prefLabel xml:lang="no">Gamelan</skos:prefLabel>
    <skos:prefLabel xml:lang="pl">Gamelan</skos:prefLabel>
    <skos:prefLabel xml:lang="pt">Gamelão</skos:prefLabel>
    <skos:prefLabel xml:lang="ru">Гамелан</skos:prefLabel>
    <skos:prefLabel xml:lang="sk">Gamelan</skos:prefLabel>
    <skos:prefLabel xml:lang="es">Gamelán</skos:prefLabel>
    <skos:prefLabel xml:lang="sv">Gamelan</skos:prefLabel>
    <skos:prefLabel xml:lang="tr">Gamelan</skos:prefLabel>
    <skos:prefLabel xml:lang="uk">Гамелан</skos:prefLabel>
    <skos:closeMatch rdf:resource="http://rdf.freebase.com/ns/m.0ptwc"/>
    <skos:broader
      rdf:resource="http://data.europeana.eu/concept/music/genre/Music_of_Asia_traditional"/>
    <skos:definition xml:lang="en">A gamelan is a traditional musical ensemble from
      Indonesia.</skos:definition>
    <skos:exactMatch xml:lang="en">http://dbpedia.org/resource/Gamelan</skos:exactMatch>
    <skos:inScheme rdf:resource="http://data.europeana.eu/concept/music/genre/Music_Genre_Scheme"/>
    <skos:altLabel xml:lang="en">Gamelan</skos:altLabel>
  </skos:Concept>

  <skos:Concept rdf:about="http://data.europeana.eu/concept/music/genre/Garage_punk">
    <skos:prefLabel xml:lang="en">Garage punk</skos:prefLabel>
    <skos:prefLabel xml:lang="da">Garagepunk</skos:prefLabel>
    <skos:prefLabel xml:lang="et">Garage punk</skos:prefLabel>
    <skos:prefLabel xml:lang="fi">Garage punk</skos:prefLabel>
    <skos:prefLabel xml:lang="fr">Garage punk</skos:prefLabel>
    <skos:prefLabel xml:lang="it">Garage punk</skos:prefLabel>
    <skos:prefLabel xml:lang="pt">Punk de garagem</skos:prefLabel>
    <skos:prefLabel xml:lang="ru">Гаражный панк</skos:prefLabel>
    <skos:prefLabel xml:lang="sk">Garage punk</skos:prefLabel>
    <skos:prefLabel xml:lang="es">Garage punk</skos:prefLabel>
    <skos:closeMatch rdf:resource="http://rdf.freebase.com/ns/m.0621cs"/>
    <skos:broader>
      <skos:Concept rdf:about="http://data.europeana.eu/concept/music/genre/Punk_rock">
        <skos:prefLabel xml:lang="en">Punk</skos:prefLabel>
        <skos:prefLabel xml:lang="ar">بانك</skos:prefLabel>
        <skos:prefLabel xml:lang="bg">Пънк</skos:prefLabel>
        <skos:prefLabel xml:lang="ca">Punk rock</skos:prefLabel>
        <skos:prefLabel xml:lang="hr">Punk rock</skos:prefLabel>
        <skos:prefLabel xml:lang="cs">Punk</skos:prefLabel>
        <skos:prefLabel xml:lang="da">Punk</skos:prefLabel>
        <skos:prefLabel xml:lang="nl">Punkrock</skos:prefLabel>
        <skos:prefLabel xml:lang="et">Punk rock</skos:prefLabel>
        <skos:prefLabel xml:lang="fi">Punk</skos:prefLabel>
        <skos:prefLabel xml:lang="fr">Punk rock</skos:prefLabel>
        <skos:prefLabel xml:lang="de">Punkmusik</skos:prefLabel>
        <skos:prefLabel xml:lang="el">Πανκ</skos:prefLabel>
        <skos:prefLabel xml:lang="hu">Punk</skos:prefLabel>
        <skos:prefLabel xml:lang="id">Punk rock</skos:prefLabel>
        <skos:prefLabel xml:lang="it">Punk rock</skos:prefLabel>
        <skos:prefLabel xml:lang="ja">パンク・ロック</skos:prefLabel>
        <skos:prefLabel xml:lang="ko">펑크 록</skos:prefLabel>
        <skos:prefLabel xml:lang="lv">Pankroks</skos:prefLabel>
        <skos:prefLabel xml:lang="lt">Pankrokas</skos:prefLabel>
        <skos:prefLabel xml:lang="ms">Rock punk</skos:prefLabel>
        <skos:prefLabel xml:lang="no">Punk</skos:prefLabel>
        <skos:prefLabel xml:lang="fa">پانک راک</skos:prefLabel>
        <skos:prefLabel xml:lang="pl">Punk</skos:prefLabel>
        <skos:prefLabel xml:lang="pt">Punk rock</skos:prefLabel>
        <skos:prefLabel xml:lang="ro">Punk rock</skos:prefLabel>
        <skos:prefLabel xml:lang="ru">Панк-рок</skos:prefLabel>
        <skos:prefLabel xml:lang="sr">Панк рок</skos:prefLabel>
        <skos:prefLabel xml:lang="sk">Punk rock</skos:prefLabel>
        <skos:prefLabel xml:lang="sl">Punk rock</skos:prefLabel>
        <skos:prefLabel xml:lang="es">Punk</skos:prefLabel>
        <skos:prefLabel xml:lang="sv">Punk</skos:prefLabel>
        <skos:prefLabel xml:lang="th">พังก์ร็อก</skos:prefLabel>
        <skos:prefLabel xml:lang="tr">Punk Rock</skos:prefLabel>
        <skos:prefLabel xml:lang="uk">Панк-рок</skos:prefLabel>
        <skos:prefLabel xml:lang="vi">Punk rock</skos:prefLabel>
        <skos:closeMatch rdf:resource="http://rdf.freebase.com/ns/m.05r6t"/>
        <skos:broader rdf:resource="http://data.europeana.eu/concept/music/genre/Rock_music"/>
        <skos:definition xml:lang="en">Punk rock is a rock music genre that developed between 1974
          and 1976 in the United States, United Kingdom, and Australia. Rooted in garage rock and
          other forms of what is now known as protopunk music, punk rock bands eschewed perceived
          excesses of mainstream 1970s rock. Punk bands created fast, hard-edged music, typically
          with short songs, stripped-down instrumentation, and often political, anti-establishment
          lyrics. Punk embraces a DIY ethic, many bands self-produced recordings and distributed
          them through informal channels. &lt;p&gt; The term &quot;punk&quot; was first used in
          relation to rock music by some American critics in the early 1970s, to describe garage
          bands and their devotees. By late 1976, bands such as the Sex Pistols, The Clash and The
          Damned in London, and Television, and the Ramones in New York City were recognized as the
          vanguard of a new musical movement. The following year saw punk rock spreading around the
          world, and it became a major cultural phenomenon in the United Kingdom. For the most part,
          punk took root in local scenes that tended to reject association with the
          mainstream.</skos:definition>
        <skos:exactMatch xml:lang="en">http://dbpedia.org/resource/Punk_rock</skos:exactMatch>
        <skos:inScheme
          rdf:resource="http://data.europeana.eu/concept/music/genre/Music_Genre_Scheme"/>
        <skos:altLabel xml:lang="en">Punk rock</skos:altLabel>
      </skos:Concept>
    </skos:broader>

    <skos:definition xml:lang="en">Garage punk is a fusion of garage rock and modern punk rock. It
      is music characterized by a dirty, choppy guitar sound— lyrics dealing with bad taste and
      rebelliousness, usually played by bands who are on independent record labels or who are
      unsigned. Garage punk bands often distance themselves from hardcore and political punk
      bands.</skos:definition>
    <skos:exactMatch xml:lang="en">http://dbpedia.org/resource/Garage_punk</skos:exactMatch>
    <skos:inScheme rdf:resource="http://data.europeana.eu/concept/music/genre/Music_Genre_Scheme"/>
    <skos:altLabel xml:lang="en">Garage punk</skos:altLabel>
  </skos:Concept>

  <skos:Concept rdf:about="http://data.europeana.eu/concept/music/genre/Garage_rock">
    <skos:prefLabel xml:lang="en">Garage rock</skos:prefLabel>
    <skos:prefLabel xml:lang="ca">Garage rock</skos:prefLabel>
    <skos:prefLabel xml:lang="cs">Garage rock</skos:prefLabel>
    <skos:prefLabel xml:lang="nl">Garagerock</skos:prefLabel>
    <skos:prefLabel xml:lang="fi">Garage rock</skos:prefLabel>
    <skos:prefLabel xml:lang="fr">Garage</skos:prefLabel>
    <skos:prefLabel xml:lang="de">Garage Rock</skos:prefLabel>
    <skos:prefLabel xml:lang="el">Γκαράζ ροκ</skos:prefLabel>
    <skos:prefLabel xml:lang="it">Garage rock</skos:prefLabel>
    <skos:prefLabel xml:lang="ja">ガレージロック</skos:prefLabel>
    <skos:prefLabel xml:lang="ko">개러지 록</skos:prefLabel>
    <skos:prefLabel xml:lang="lv">Garāžroks</skos:prefLabel>
    <skos:prefLabel xml:lang="lt">Garage Rock</skos:prefLabel>
    <skos:prefLabel xml:lang="ms">Garage rock</skos:prefLabel>
    <skos:prefLabel xml:lang="no">Garage rock</skos:prefLabel>
    <skos:prefLabel xml:lang="fa">گاراژ راک</skos:prefLabel>
    <skos:prefLabel xml:lang="pl">Garage rock</skos:prefLabel>
    <skos:prefLabel xml:lang="pt">Rock de garagem</skos:prefLabel>
    <skos:prefLabel xml:lang="ru">Гаражный рок</skos:prefLabel>
    <skos:prefLabel xml:lang="sk">Garage rock</skos:prefLabel>
    <skos:prefLabel xml:lang="es">Garage rock</skos:prefLabel>
    <skos:prefLabel xml:lang="sv">Garagerock</skos:prefLabel>
    <skos:prefLabel xml:lang="th">การาจร็อก</skos:prefLabel>
    <skos:prefLabel xml:lang="uk">Гаражний рок</skos:prefLabel>
    <skos:closeMatch rdf:resource="http://rdf.freebase.com/ns/m.0133_p"/>
    <skos:broader rdf:resource="http://data.europeana.eu/concept/music/genre/Rock_music"/>
    <skos:definition xml:lang="en">Garage rock is a raw form of rock and roll that was first popular
      in the United States and Canada from about 1963 to 1967. Its name derives from the perception
      that many often rehearsed in a family garage. &lt;p&gt; The style was characterised by lyrics
      and delivery that were more aggressive and unsophisticated than in commercial pop music at the
      time, often, for instance, using guitars distorted through a fuzzbox. It began to evolve from
      regional scenes as early as 1958, heavily influenced by surf rock. The &quot;British
      Invasion&quot; of 1964-66 greatly influenced garage bands, providing them with a national
      audience. Thousands of garage bands were extant in the USA and Canada during the era, hundreds
      produced regional hits, and a handful had national chart hits. By 1968 the style largely
      disappeared from the national charts. It was also disappearing at the local level as amateur
      musicians faced college, work or the draft. During the 1960s, it was not recognized as a
      separate music genre and had no specific name.</skos:definition>
    <skos:exactMatch xml:lang="en">http://dbpedia.org/resource/Garage_rock</skos:exactMatch>
    <skos:inScheme rdf:resource="http://data.europeana.eu/concept/music/genre/Music_Genre_Scheme"/>
    <skos:altLabel xml:lang="en">Garage rock</skos:altLabel>
  </skos:Concept>

  <skos:Concept rdf:about="http://data.europeana.eu/concept/music/genre/Gospel">
    <skos:prefLabel xml:lang="en">Gospel</skos:prefLabel>
    <skos:prefLabel xml:lang="ar">غوسبل</skos:prefLabel>
    <skos:prefLabel xml:lang="bg">Госпъл</skos:prefLabel>
    <skos:prefLabel xml:lang="ca">Gospel</skos:prefLabel>
    <skos:prefLabel xml:lang="hr">Gospel</skos:prefLabel>
    <skos:prefLabel xml:lang="cs">Gospel</skos:prefLabel>
    <skos:prefLabel xml:lang="da">Gospel</skos:prefLabel>
    <skos:prefLabel xml:lang="nl">Gospelmuziek</skos:prefLabel>
    <skos:prefLabel xml:lang="et">Gospel</skos:prefLabel>
    <skos:prefLabel xml:lang="fi">Gospel</skos:prefLabel>
    <skos:prefLabel xml:lang="fr">Gospel</skos:prefLabel>
    <skos:prefLabel xml:lang="de">Gospelmusik</skos:prefLabel>
    <skos:prefLabel xml:lang="el">Γκόσπελ</skos:prefLabel>
    <skos:prefLabel xml:lang="hu">Gospel</skos:prefLabel>
    <skos:prefLabel xml:lang="id">Musik gospel</skos:prefLabel>
    <skos:prefLabel xml:lang="it">Gospel</skos:prefLabel>
    <skos:prefLabel xml:lang="ja">ゴスペル</skos:prefLabel>
    <skos:prefLabel xml:lang="ko">복음성가</skos:prefLabel>
    <skos:prefLabel xml:lang="lv">Gospelis</skos:prefLabel>
    <skos:prefLabel xml:lang="lt">Gospelo muzika</skos:prefLabel>
    <skos:prefLabel xml:lang="no">Gospelmusikk</skos:prefLabel>
    <skos:prefLabel xml:lang="fa">موسیقی گاسپل</skos:prefLabel>
    <skos:prefLabel xml:lang="pl">Gospel</skos:prefLabel>
    <skos:prefLabel xml:lang="pt">Música gospel</skos:prefLabel>
    <skos:prefLabel xml:lang="ro">Muzică gospel</skos:prefLabel>
    <skos:prefLabel xml:lang="ru">Госпел</skos:prefLabel>
    <skos:prefLabel xml:lang="sr">Госпел</skos:prefLabel>
    <skos:prefLabel xml:lang="sk">Gospel</skos:prefLabel>
    <skos:prefLabel xml:lang="es">Góspel</skos:prefLabel>
    <skos:prefLabel xml:lang="sv">Gospel</skos:prefLabel>
    <skos:prefLabel xml:lang="th">กอสเปล</skos:prefLabel>
    <skos:prefLabel xml:lang="tr">Gospel müziği</skos:prefLabel>
    <skos:prefLabel xml:lang="uk">Госпел</skos:prefLabel>
    <skos:prefLabel xml:lang="vi">Nhạc Phúc âm</skos:prefLabel>
    <skos:closeMatch rdf:resource="http://rdf.freebase.com/ns/m.016cjb"/>
    <skos:broader rdf:resource="http://data.europeana.eu/concept/music/genre/Religious_music"/>
    <skos:definition xml:lang="en">Gospel music is a music genre in Christian music. The creation,
      performance, significance, and even the definition of gospel music varies according to culture
      and social context. Gospel music is composed and performed for many purposes, including
      aesthetic pleasure, religious or ceremonial purposes, and as an entertainment product for the
      marketplace.</skos:definition>
    <skos:exactMatch xml:lang="en">http://dbpedia.org/resource/Gospel</skos:exactMatch>
    <skos:inScheme rdf:resource="http://data.europeana.eu/concept/music/genre/Music_Genre_Scheme"/>
    <skos:altLabel xml:lang="en">Gospel music</skos:altLabel>
  </skos:Concept>

  <skos:Concept rdf:about="http://data.europeana.eu/concept/music/genre/Grunge">
    <skos:prefLabel xml:lang="en">Grunge</skos:prefLabel>
    <skos:prefLabel xml:lang="bg">Гръндж</skos:prefLabel>
    <skos:prefLabel xml:lang="ca">Grunge</skos:prefLabel>
    <skos:prefLabel xml:lang="hr">Grunge</skos:prefLabel>
    <skos:prefLabel xml:lang="cs">Grunge</skos:prefLabel>
    <skos:prefLabel xml:lang="da">Grunge</skos:prefLabel>
    <skos:prefLabel xml:lang="nl">Grunge</skos:prefLabel>
    <skos:prefLabel xml:lang="et">Grunge</skos:prefLabel>
    <skos:prefLabel xml:lang="fi">Grunge</skos:prefLabel>
    <skos:prefLabel xml:lang="fr">Grunge</skos:prefLabel>
    <skos:prefLabel xml:lang="de">Grunge</skos:prefLabel>
    <skos:prefLabel xml:lang="el">Grunge</skos:prefLabel>
    <skos:prefLabel xml:lang="hu">Grunge</skos:prefLabel>
    <skos:prefLabel xml:lang="id">Grunge</skos:prefLabel>
    <skos:prefLabel xml:lang="it">Grunge</skos:prefLabel>
    <skos:prefLabel xml:lang="ja">グランジ</skos:prefLabel>
    <skos:prefLabel xml:lang="ko">그런지</skos:prefLabel>
    <skos:prefLabel xml:lang="lv">Grandžmūzika</skos:prefLabel>
    <skos:prefLabel xml:lang="lt">Grunge</skos:prefLabel>
    <skos:prefLabel xml:lang="ms">Grunge</skos:prefLabel>
    <skos:prefLabel xml:lang="no">Grunge</skos:prefLabel>
    <skos:prefLabel xml:lang="fa">گرانج</skos:prefLabel>
    <skos:prefLabel xml:lang="pl">Grunge</skos:prefLabel>
    <skos:prefLabel xml:lang="pt">Grunge</skos:prefLabel>
    <skos:prefLabel xml:lang="ro">Grunge</skos:prefLabel>
    <skos:prefLabel xml:lang="ru">Гранж</skos:prefLabel>
    <skos:prefLabel xml:lang="sr">Гранџ</skos:prefLabel>
    <skos:prefLabel xml:lang="sk">Grunge</skos:prefLabel>
    <skos:prefLabel xml:lang="sl">Grunge</skos:prefLabel>
    <skos:prefLabel xml:lang="es">Grunge</skos:prefLabel>
    <skos:prefLabel xml:lang="sv">Grunge</skos:prefLabel>
    <skos:prefLabel xml:lang="th">กรันจ์</skos:prefLabel>
    <skos:prefLabel xml:lang="tr">Grunge</skos:prefLabel>
    <skos:prefLabel xml:lang="uk">Грандж</skos:prefLabel>
    <skos:closeMatch rdf:resource="http://rdf.freebase.com/ns/m.0dls3"/>
    <skos:broader
      rdf:resource="http://data.europeana.eu/concept/music/genre/Alternative_rock_fusions"/>
    <skos:definition xml:lang="en">Grunge is a subgenre of alternative rock that emerged during the
      mid-1980s in the American state of Washington, particularly in the Seattle area. The early
      Grunge movement revolved around Seattle's independent record label Sub Pop, but by the early
      1990s its popularity had spread, with Grunge acts in California and other parts of the U.S.
      building strong followings and signing major record deals. &lt;p&gt; Inspired by hardcore punk
      and heavy metal, grunge is generally characterized by heavily distorted electric guitars,
      contrasting song dynamics, &quot;growling&quot; vocals and apathetic or angst-filled lyrics.
      The grunge aesthetic is stripped-down compared with other forms of rock music, and many grunge
      musicians were noted for their unkempt appearances and rejection of theatrics. &lt;p&gt;
      Grunge became commercially successful in the first half of the 1990s, due mainly to the
      release of Nirvana's Nevermind, Pearl Jam's Ten, Soundgarden's Badmotorfinger, Alice in
      Chains' Dirt, and Stone Temple Pilots' Core. The success of these bands boosted the popularity
      of alternative rock and made grunge the most popular form of hard rock music at the
      time.</skos:definition>
    <skos:exactMatch xml:lang="en">http://dbpedia.org/resource/Grunge</skos:exactMatch>
    <skos:inScheme rdf:resource="http://data.europeana.eu/concept/music/genre/Music_Genre_Scheme"/>
    <skos:altLabel xml:lang="en">Grunge</skos:altLabel>
  </skos:Concept>

  <skos:Concept rdf:about="http://data.europeana.eu/concept/music/genre/Hard_rock">
    <skos:prefLabel xml:lang="en">Hard rock</skos:prefLabel>
    <skos:prefLabel xml:lang="ar">هارد روك</skos:prefLabel>
    <skos:prefLabel xml:lang="bg">Хард рок</skos:prefLabel>
    <skos:prefLabel xml:lang="ca">Rock dur</skos:prefLabel>
    <skos:prefLabel xml:lang="hr">Hard rock</skos:prefLabel>
    <skos:prefLabel xml:lang="cs">Hard rock</skos:prefLabel>
    <skos:prefLabel xml:lang="da">Hård rock</skos:prefLabel>
    <skos:prefLabel xml:lang="nl">Hardrock</skos:prefLabel>
    <skos:prefLabel xml:lang="et">Hard rock</skos:prefLabel>
    <skos:prefLabel xml:lang="fi">Hard rock</skos:prefLabel>
    <skos:prefLabel xml:lang="fr">Hard rock</skos:prefLabel>
    <skos:prefLabel xml:lang="de">Hard Rock</skos:prefLabel>
    <skos:prefLabel xml:lang="el">Χαρντ Ροκ</skos:prefLabel>
    <skos:prefLabel xml:lang="hu">Hard rock</skos:prefLabel>
    <skos:prefLabel xml:lang="id">Hard rock</skos:prefLabel>
    <skos:prefLabel xml:lang="it">Hard rock</skos:prefLabel>
    <skos:prefLabel xml:lang="ja">ハードロック</skos:prefLabel>
    <skos:prefLabel xml:lang="ko">하드 록</skos:prefLabel>
    <skos:prefLabel xml:lang="lv">Smagais roks</skos:prefLabel>
    <skos:prefLabel xml:lang="lt">Sunkusis rokas</skos:prefLabel>
    <skos:prefLabel xml:lang="ms">Hard rock</skos:prefLabel>
    <skos:prefLabel xml:lang="no">Hardrock</skos:prefLabel>
    <skos:prefLabel xml:lang="fa">هارد راک</skos:prefLabel>
    <skos:prefLabel xml:lang="pl">Hard rock</skos:prefLabel>
    <skos:prefLabel xml:lang="pt">Hard rock</skos:prefLabel>
    <skos:prefLabel xml:lang="ro">Hard rock</skos:prefLabel>
    <skos:prefLabel xml:lang="ru">Хард-рок</skos:prefLabel>
    <skos:prefLabel xml:lang="sr">Хард рок</skos:prefLabel>
    <skos:prefLabel xml:lang="sk">Hard rock</skos:prefLabel>
    <skos:prefLabel xml:lang="sl">Hard rock</skos:prefLabel>
    <skos:prefLabel xml:lang="es">Hard rock</skos:prefLabel>
    <skos:prefLabel xml:lang="sv">Hårdrock</skos:prefLabel>
    <skos:prefLabel xml:lang="th">ฮาร์ดร็อก</skos:prefLabel>
    <skos:prefLabel xml:lang="tr">Hard rock</skos:prefLabel>
    <skos:prefLabel xml:lang="uk">Хард-рок</skos:prefLabel>
    <skos:prefLabel xml:lang="vi">Hard rock</skos:prefLabel>
    <skos:closeMatch rdf:resource="http://rdf.freebase.com/ns/m.0xhtw"/>
    <skos:broader rdf:resource="http://data.europeana.eu/concept/music/genre/Rock_music"/>
    <skos:definition xml:lang="en">Hard rock is a loosely defined subgenre of rock music which has
      its earliest roots in mid-1960s garage rock, blues rock and psychedelic rock. It is typified
      by a heavy use of aggressive vocals, distorted electric guitars, bass guitar, drums, and often
      accompanied with pianos and keyboards. &lt;p&gt; Hard rock developed into a major form of
      popular music in the 1970s, with bands such as Led Zeppelin, The Who, Deep Purple, Aerosmith
      and AC/DC. It reached a commercial peak in the 1980s, with glam metal bands like Van Halen,
      Bon Jovi and Def Leppard and the rawer sounds of Guns N' Roses, which followed up with great
      success in the later part of that decade, before losing popularity with the commercial success
      of grunge and later Britpop in the 1990s. Despite this, many post-grunge bands adopted a hard
      rock sound and in the 2000s there came a renewed interest in established bands, attempts at a
      revival, and new hard rock bands that emerged from the garage rock and post-punk revival
      scenes.</skos:definition>
    <skos:exactMatch xml:lang="en">http://dbpedia.org/resource/Hard_rock</skos:exactMatch>
    <skos:inScheme rdf:resource="http://data.europeana.eu/concept/music/genre/Music_Genre_Scheme"/>
    <skos:altLabel xml:lang="en">Hard rock</skos:altLabel>
  </skos:Concept>

  <skos:Concept rdf:about="http://data.europeana.eu/concept/music/genre/Jazz">
    <skos:prefLabel xml:lang="en">Jazz</skos:prefLabel>
    <skos:prefLabel xml:lang="ar">جاز</skos:prefLabel>
    <skos:prefLabel xml:lang="bg">Джаз</skos:prefLabel>
    <skos:prefLabel xml:lang="ca">Jazz</skos:prefLabel>
    <skos:prefLabel xml:lang="hr">Džez</skos:prefLabel>
    <skos:prefLabel xml:lang="cs">Jazz</skos:prefLabel>
    <skos:prefLabel xml:lang="da">Jazz</skos:prefLabel>
    <skos:prefLabel xml:lang="nl">Jazz</skos:prefLabel>
    <skos:prefLabel xml:lang="et">Džäss</skos:prefLabel>
    <skos:prefLabel xml:lang="fil">Jazz</skos:prefLabel>
    <skos:prefLabel xml:lang="fi">Jazz</skos:prefLabel>
    <skos:prefLabel xml:lang="fr">Jazz</skos:prefLabel>
    <skos:prefLabel xml:lang="de">Jazz</skos:prefLabel>
    <skos:prefLabel xml:lang="el">Τζαζ</skos:prefLabel>
    <skos:prefLabel xml:lang="hi">जैज़ संगीत</skos:prefLabel>
    <skos:prefLabel xml:lang="hu">Dzsessz</skos:prefLabel>
    <skos:prefLabel xml:lang="id">Jazz</skos:prefLabel>
    <skos:prefLabel xml:lang="it">Jazz</skos:prefLabel>
    <skos:prefLabel xml:lang="ja">ジャズ</skos:prefLabel>
    <skos:prefLabel xml:lang="ko">재즈</skos:prefLabel>
    <skos:prefLabel xml:lang="lv">Džezs</skos:prefLabel>
    <skos:prefLabel xml:lang="lt">Džiazas</skos:prefLabel>
    <skos:prefLabel xml:lang="ms">Jaz</skos:prefLabel>
    <skos:prefLabel xml:lang="no">Jazz</skos:prefLabel>
    <skos:prefLabel xml:lang="fa">جاز</skos:prefLabel>
    <skos:prefLabel xml:lang="pl">Jazz</skos:prefLabel>
    <skos:prefLabel xml:lang="pt">Jazz</skos:prefLabel>
    <skos:prefLabel xml:lang="ro">Jazz</skos:prefLabel>
    <skos:prefLabel xml:lang="ru">Джаз</skos:prefLabel>
    <skos:prefLabel xml:lang="sr">Џез</skos:prefLabel>
    <skos:prefLabel xml:lang="sk">Džez</skos:prefLabel>
    <skos:prefLabel xml:lang="sl">Jazz</skos:prefLabel>
    <skos:prefLabel xml:lang="es">Jazz</skos:prefLabel>
    <skos:prefLabel xml:lang="sv">Jazz</skos:prefLabel>
    <skos:prefLabel xml:lang="th">แจ๊ส</skos:prefLabel>
    <skos:prefLabel xml:lang="tr">Caz</skos:prefLabel>
    <skos:prefLabel xml:lang="uk">Джаз</skos:prefLabel>
    <skos:prefLabel xml:lang="vi">Jazz</skos:prefLabel>
    <skos:closeMatch rdf:resource="http://rdf.freebase.com/ns/m.03_d0"/>
    <skos:broader rdf:resource="http://data.europeana.eu/concept/music/genre/Popular_music"/>
    <skos:definition xml:lang="en">Jazz is a genre of music that originated in the late nineteenth
      and early twentieth century in the Southern United States. Jazz makes heavy use of
      improvisation, polyrhythms, syncopation, and the swung note, as well as aspects of European
      harmony, American popular music, and African musical elements such as blue notes. A musical
      group that plays jazz is called a jazz band. &lt;p&gt; As jazz spread around the world, it
      drew on different national, regional, and local musical cultures, giving rise to many
      distinctive styles: New Orleans jazz dating from the early 1910s, big band swing, Kansas City
      jazz and Gypsy jazz from the 1930s and 1940s, bebop from the mid-1940s, Afro-Cuban jazz, West
      Coast jazz, ska jazz, cool jazz, Indo jazz, avant-garde jazz, soul jazz, modal jazz, chamber
      jazz, free jazz, Latin jazz, smooth jazz, jazz fusion and jazz rock, jazz funk, loft jazz,
      punk jazz, acid jazz, ethno jazz, jazz rap, M-Base and nu jazz. &lt;p&gt; Louis Armstrong, one
      of the most famous musicians in jazz, said to Bing Crosby on the latter's radio show,
      &quot;Ah, swing, well, we used to call it syncopation, then they called it ragtime, then
      blues, then jazz. Now, it's swing.&quot; &lt;p&gt; In a 1988 interview, jazz musician
      J.</skos:definition>
    <skos:exactMatch xml:lang="en">http://dbpedia.org/resource/Jazz</skos:exactMatch>
    <skos:inScheme rdf:resource="http://data.europeana.eu/concept/music/genre/Music_Genre_Scheme"/>
    <skos:altLabel xml:lang="en">Jazz</skos:altLabel>
  </skos:Concept>

  <skos:Concept rdf:about="http://data.europeana.eu/concept/music/genre/Joropo">
    <skos:prefLabel xml:lang="en">Joropo</skos:prefLabel>
    <skos:prefLabel xml:lang="ca">Joropo</skos:prefLabel>
    <skos:prefLabel xml:lang="fi">Joropo</skos:prefLabel>
    <skos:prefLabel xml:lang="fr">Joropo</skos:prefLabel>
    <skos:prefLabel xml:lang="de">Joropo</skos:prefLabel>
    <skos:prefLabel xml:lang="it">Joropo</skos:prefLabel>
    <skos:prefLabel xml:lang="ja">ホローポ</skos:prefLabel>
    <skos:prefLabel xml:lang="ko">호로포</skos:prefLabel>
    <skos:prefLabel xml:lang="pt">Joropo</skos:prefLabel>
    <skos:prefLabel xml:lang="es">Joropo</skos:prefLabel>
    <skos:closeMatch rdf:resource="http://rdf.freebase.com/ns/m.01y1n5"/>
    <skos:broader
      rdf:resource="http://data.europeana.eu/concept/music/genre/Latin_American_music_traditional"/>
    <skos:definition xml:lang="en">The Joropo is a musical style resembling the waltz, and an
      accompanying dance, having African and European influences originated in Venezuela It's a
      fundamental genre belonging to its typical music or música criolla. It is also the most
      popular &quot;folk rhythm&quot;: the well-known song &quot;Alma Llanera&quot; is a joropo,
      considered the unofficial national anthem of Venezuela. &lt;p&gt; In 1882 it became
      Venezuela's national dance. Formerly, the Spanish word joropo meant &quot;a party&quot;, but
      now it has come to mean a type of music and dance that identifies Venezuelans, ]. In the 18th
      century the llaneros started using the word “joropo” instead of the word &quot;fandango&quot;,
      which was the word used at the time for party and dance.</skos:definition>
    <skos:exactMatch xml:lang="en">http://dbpedia.org/resource/Joropo</skos:exactMatch>
    <skos:inScheme rdf:resource="http://data.europeana.eu/concept/music/genre/Music_Genre_Scheme"/>
    <skos:altLabel xml:lang="en">Joropo</skos:altLabel>
  </skos:Concept>

  <skos:Concept rdf:about="http://data.europeana.eu/concept/music/genre/Jungle">
    <skos:prefLabel xml:lang="en">Jungle</skos:prefLabel>
    <skos:prefLabel xml:lang="ca">Oldschool jungle</skos:prefLabel>
    <skos:prefLabel xml:lang="cs">Jungle</skos:prefLabel>
    <skos:prefLabel xml:lang="nl">Jungle</skos:prefLabel>
    <skos:prefLabel xml:lang="de">Jungle</skos:prefLabel>
    <skos:prefLabel xml:lang="hu">Jungle</skos:prefLabel>
    <skos:prefLabel xml:lang="it">Jungle</skos:prefLabel>
    <skos:prefLabel xml:lang="ja">ジャングル</skos:prefLabel>
    <skos:prefLabel xml:lang="pl">Jungle</skos:prefLabel>
    <skos:prefLabel xml:lang="ru">Джангл</skos:prefLabel>
    <skos:prefLabel xml:lang="sr">Олдскул џангл</skos:prefLabel>
    <skos:prefLabel xml:lang="sk">Oldschool jungle</skos:prefLabel>
    <skos:prefLabel xml:lang="es">Jungle</skos:prefLabel>
    <skos:prefLabel xml:lang="sv">Jungle</skos:prefLabel>
    <skos:prefLabel xml:lang="th">โอลด์สคูลจังเกิล</skos:prefLabel>
    <skos:prefLabel xml:lang="uk">Джангл</skos:prefLabel>
    <skos:prefLabel xml:lang="en">Oldschool jungle</skos:prefLabel>
    <skos:closeMatch rdf:resource="http://rdf.freebase.com/ns/m.01f9gb"/>
    <skos:broader rdf:resource="http://data.europeana.eu/concept/music/genre/Electronic_music"/>
    <skos:definition xml:lang="en">Oldskool jungle, or simply jungle, is a genre of electronic music
      that incorporates influences from other genres, including breakbeat hardcore and
      reggae/dub/dancehall. It is one of several types of music often simply referred to as
      &quot;jungle music&quot;. The fast tempos, breakbeats and other heavily syncopated percussive
      loops, samples and synthesized effects make up the easily recognizable form of jungle. Long
      pitch-shifted snare rolls are common in oldskool jungle. &lt;p&gt; The terms
      &quot;jungle&quot; and &quot;drum and bass&quot; are often used interchangeably, although
      whether the two genres are actually distinct is an ongoing topic of debate. For those
      individuals who consider the two genres as separate entities, drum and bass is usually
      considered to have departed from jungle in the mid to late-1990s. &lt;p&gt; Producers create
      the drum patterns, which are sometimes completely off-beat, by cutting apart breakbeats.
      Jungle producers incorporated classic Jamaican/Caribbean sound-system culture
      production-methods. The slow, deep basslines and simple melodies accentuated the overall
      production, giving jungle its &quot;rolling&quot; quality.</skos:definition>
    <skos:exactMatch xml:lang="en">http://dbpedia.org/resource/Jungle</skos:exactMatch>
    <skos:inScheme rdf:resource="http://data.europeana.eu/concept/music/genre/Music_Genre_Scheme"/>
    <skos:altLabel xml:lang="en">Oldschool jungle</skos:altLabel>
    <skos:altLabel xml:lang="en">drum and bass</skos:altLabel>
    <skos:altLabel xml:lang="en">Jungle</skos:altLabel>
  </skos:Concept>

  <skos:Concept rdf:about="http://data.europeana.eu/concept/music/genre/Klezmer">
    <skos:prefLabel xml:lang="en">Klezmer</skos:prefLabel>
    <skos:prefLabel xml:lang="ca">Klezmer</skos:prefLabel>
    <skos:prefLabel xml:lang="hr">Klezmer</skos:prefLabel>
    <skos:prefLabel xml:lang="cs">Klezmer</skos:prefLabel>
    <skos:prefLabel xml:lang="da">Klezmer</skos:prefLabel>
    <skos:prefLabel xml:lang="nl">Klezmer</skos:prefLabel>
    <skos:prefLabel xml:lang="fi">Klezmer</skos:prefLabel>
    <skos:prefLabel xml:lang="fr">Klezmer</skos:prefLabel>
    <skos:prefLabel xml:lang="de">Klezmer</skos:prefLabel>
    <skos:prefLabel xml:lang="hu">Klezmer</skos:prefLabel>
    <skos:prefLabel xml:lang="it">Klezmer</skos:prefLabel>
    <skos:prefLabel xml:lang="ja">クレズマー</skos:prefLabel>
    <skos:prefLabel xml:lang="no">Klezmer</skos:prefLabel>
    <skos:prefLabel xml:lang="pl">Muzyka klezmerska</skos:prefLabel>
    <skos:prefLabel xml:lang="pt">Klezmer</skos:prefLabel>
    <skos:prefLabel xml:lang="ru">Клезмер</skos:prefLabel>
    <skos:prefLabel xml:lang="sk">Klezmer</skos:prefLabel>
    <skos:prefLabel xml:lang="es">Klezmer</skos:prefLabel>
    <skos:prefLabel xml:lang="sv">Klezmer</skos:prefLabel>
    <skos:prefLabel xml:lang="tr">Klezmer</skos:prefLabel>
    <skos:closeMatch rdf:resource="http://rdf.freebase.com/ns/m.0178n1"/>
    <skos:broader rdf:resource="http://data.europeana.eu/concept/music/genre/Folk_music_traditional"/>
    <skos:definition xml:lang="en">Klezmer is a musical tradition of the Ashkenazi Jews of Eastern
      Europe. Played by professional musicians called klezmorim, the genre originally consisted
      largely of dance tunes and instrumental display pieces for weddings and other celebrations. In
      the United States the genre evolved considerably as Yiddish-speaking Jewish immigrants from
      Eastern Europe, who arrived between 1880 and 1924, met and assimilated American jazz. During
      the initial years after the klezmer revival of the 1970s, this was what most people knew as
      klezmer, although in the current century musicians have begun paying more attention to the
      &quot;original&quot; pre-jazz traditions as revivalists including Josh Horowitz, Yale Strom,
      and Bob Cohen have spent years doing field research in Eastern/Central Europe. Additionally,
      late immigrants from the Soviet Union such as German Goldenshtayn brought their surviving
      repertoires to the United States and Israel in the 1980s. &lt;p&gt; Compared to most other
      European folk music styles, little is known about the history of klezmer music, and much of
      what is said about it must be seen as conjecture.</skos:definition>
    <skos:exactMatch xml:lang="en">http://dbpedia.org/resource/Klezmer</skos:exactMatch>
    <skos:inScheme rdf:resource="http://data.europeana.eu/concept/music/genre/Music_Genre_Scheme"/>
    <skos:altLabel xml:lang="en">Klezmer</skos:altLabel>
  </skos:Concept>

  <skos:Concept rdf:about="http://data.europeana.eu/concept/music/genre/Krautrock">
    <skos:prefLabel xml:lang="en">Krautrock</skos:prefLabel>
    <skos:prefLabel xml:lang="bg">Краутрок</skos:prefLabel>
    <skos:prefLabel xml:lang="ca">Krautrock</skos:prefLabel>
    <skos:prefLabel xml:lang="cs">Krautrock</skos:prefLabel>
    <skos:prefLabel xml:lang="nl">Krautrock</skos:prefLabel>
    <skos:prefLabel xml:lang="fi">Krautrock</skos:prefLabel>
    <skos:prefLabel xml:lang="fr">Krautrock</skos:prefLabel>
    <skos:prefLabel xml:lang="de">Krautrock</skos:prefLabel>
    <skos:prefLabel xml:lang="el">Krautrock</skos:prefLabel>
    <skos:prefLabel xml:lang="it">Krautrock</skos:prefLabel>
    <skos:prefLabel xml:lang="ja">クラウトロック</skos:prefLabel>
    <skos:prefLabel xml:lang="ko">크라우트록</skos:prefLabel>
    <skos:prefLabel xml:lang="lv">Krautroks</skos:prefLabel>
    <skos:prefLabel xml:lang="no">Krautrock</skos:prefLabel>
    <skos:prefLabel xml:lang="fa">کراوت‌راک</skos:prefLabel>
    <skos:prefLabel xml:lang="pl">Krautrock</skos:prefLabel>
    <skos:prefLabel xml:lang="pt">Krautrock</skos:prefLabel>
    <skos:prefLabel xml:lang="ro">Krautrock</skos:prefLabel>
    <skos:prefLabel xml:lang="ru">Краут-рок</skos:prefLabel>
    <skos:prefLabel xml:lang="sk">Krautrock</skos:prefLabel>
    <skos:prefLabel xml:lang="sl">Krautrock</skos:prefLabel>
    <skos:prefLabel xml:lang="es">Krautrock</skos:prefLabel>
    <skos:prefLabel xml:lang="sv">Krautrock</skos:prefLabel>
    <skos:prefLabel xml:lang="th">เคราต์ร็อก</skos:prefLabel>
    <skos:prefLabel xml:lang="tr">Krautrock</skos:prefLabel>
    <skos:prefLabel xml:lang="uk">Краут-рок</skos:prefLabel>
    <skos:closeMatch rdf:resource="http://rdf.freebase.com/ns/m.01pfpt"/>
    <skos:broader>
      <skos:Concept rdf:about="http://data.europeana.eu/concept/music/genre/Progressive_rock">
        <skos:prefLabel xml:lang="en">Progressive rock</skos:prefLabel>
        <skos:prefLabel xml:lang="ar">بروغريسيف روك</skos:prefLabel>
        <skos:prefLabel xml:lang="bg">Прогресив рок</skos:prefLabel>
        <skos:prefLabel xml:lang="ca">Rock progressiu</skos:prefLabel>
        <skos:prefLabel xml:lang="hr">Progresivni rock</skos:prefLabel>
        <skos:prefLabel xml:lang="cs">Progresivní rock</skos:prefLabel>
        <skos:prefLabel xml:lang="da">Progressiv rock</skos:prefLabel>
        <skos:prefLabel xml:lang="nl">Progressieve rock</skos:prefLabel>
        <skos:prefLabel xml:lang="et">Progressiivne rock</skos:prefLabel>
        <skos:prefLabel xml:lang="fi">Progressiivinen rock</skos:prefLabel>
        <skos:prefLabel xml:lang="fr">Rock progressif</skos:prefLabel>
        <skos:prefLabel xml:lang="de">Progressive Rock</skos:prefLabel>
        <skos:prefLabel xml:lang="hu">Progresszív rock</skos:prefLabel>
        <skos:prefLabel xml:lang="id">Progressive rock</skos:prefLabel>
        <skos:prefLabel xml:lang="it">Rock progressivo</skos:prefLabel>
        <skos:prefLabel xml:lang="ja">プログレッシブ・ロック</skos:prefLabel>
        <skos:prefLabel xml:lang="ko">프로그레시브 록</skos:prefLabel>
        <skos:prefLabel xml:lang="lv">Progresīvais roks</skos:prefLabel>
        <skos:prefLabel xml:lang="lt">Progresyvusis rokas</skos:prefLabel>
        <skos:prefLabel xml:lang="no">Progressiv rock</skos:prefLabel>
        <skos:prefLabel xml:lang="fa">پراگرسیو راک</skos:prefLabel>
        <skos:prefLabel xml:lang="pl">Rock progresywny</skos:prefLabel>
        <skos:prefLabel xml:lang="pt">Rock progressivo</skos:prefLabel>
        <skos:prefLabel xml:lang="ro">Rock progresiv</skos:prefLabel>
        <skos:prefLabel xml:lang="ru">Прогрессивный рок</skos:prefLabel>
        <skos:prefLabel xml:lang="sr">Progresivni rok</skos:prefLabel>
        <skos:prefLabel xml:lang="sk">Progresívny rock</skos:prefLabel>
        <skos:prefLabel xml:lang="sl">Progresivni rock</skos:prefLabel>
        <skos:prefLabel xml:lang="es">Rock progresivo</skos:prefLabel>
        <skos:prefLabel xml:lang="sv">Progressiv rock</skos:prefLabel>
        <skos:prefLabel xml:lang="th">โพรเกรสซีฟร็อก</skos:prefLabel>
        <skos:prefLabel xml:lang="tr">Progresif rock</skos:prefLabel>
        <skos:prefLabel xml:lang="uk">Прогресивний рок</skos:prefLabel>
        <skos:closeMatch rdf:resource="http://rdf.freebase.com/ns/m.0dl5d"/>
        <skos:broader rdf:resource="http://data.europeana.eu/concept/music/genre/Rock_music_fusions"/>
        <skos:definition xml:lang="en">Progressive rock, also known as prog rock or prog, is a rock
          music subgenre that originated in the United Kingdom, with further developments in
          Germany, Italy, and France, throughout the mid-to-late 1960s and 1970s. It developed from
          psychedelic rock, and originated, similarly to art rock, as an attempt to give greater
          artistic weight and credibility to rock music. Bands abandoned the short pop single in
          favor of instrumentation and compositional techniques more frequently associated with jazz
          or classical music in an effort to give rock music the same level of musical
          sophistication and critical respect. &lt;p&gt; Songs were replaced by musical suites that
          often stretched to 20 or 40 minutes in length and contained symphonic influences, extended
          musical themes, philosophical lyrics and complex orchestrations. The genre was not without
          criticism, however, as some reviewers found the concepts &quot;pretentious&quot; and the
          sounds &quot;pompous&quot; and &quot;overblown&quot;. &lt;p&gt; Progressive rock saw a
          high level of popularity throughout the 1970s, especially in the middle of the
          decade.</skos:definition>
        <skos:exactMatch xml:lang="en"
          >http://dbpedia.org/resource/Progressive_rock</skos:exactMatch>
        <skos:inScheme
          rdf:resource="http://data.europeana.eu/concept/music/genre/Music_Genre_Scheme"/>
        <skos:altLabel xml:lang="en">Progressive rock</skos:altLabel>
      </skos:Concept>
    </skos:broader>

    <skos:definition xml:lang="en">Krautrock is rock and electronic music that originated in Germany
      in the late 1960s. The term was popularized in the English-speaking press. Later, German media
      started to use it as a term for all German rock bands from the late 1960s and 1970s, while
      abroad the term specifically referred to more experimental artists who often but not always
      used synthesizers and other electronic instruments. &lt;p&gt; The term is a result of the
      English-speaking world's reception of the music at the time and not a reference to any one
      particular scene, style, or movement, as many krautrock artists were not familiar with one
      another. BBC DJ John Peel in particular is largely credited with spreading the reputation of
      krautrock outside of the German-speaking world. &lt;p&gt; Largely divorced from the
      traditional blues and rock &amp; roll influences of British and American rock music up to that
      time, the period contributed to the evolution of electronic music and ambient music as well as
      the birth of post-punk, alternative rock and New Age music. Key artists associated with the
      tag include Can, Amon Düül II, Ash Ra Tempel, Faust, Popol Vuh, Cluster, Tangerine Dream,
      Klaus Schulze, Neu!, and Kraftwerk.</skos:definition>
    <skos:exactMatch xml:lang="en">http://dbpedia.org/resource/Krautrock</skos:exactMatch>
    <skos:inScheme rdf:resource="http://data.europeana.eu/concept/music/genre/Music_Genre_Scheme"/>
    <skos:altLabel xml:lang="en">Krautrock</skos:altLabel>
  </skos:Concept>

  <skos:Concept rdf:about="http://data.europeana.eu/concept/music/genre/Lied">
    <skos:prefLabel xml:lang="en">Lied</skos:prefLabel>
    <skos:prefLabel xml:lang="ca">Lied</skos:prefLabel>
    <skos:prefLabel xml:lang="da">Lied</skos:prefLabel>
    <skos:prefLabel xml:lang="et">Lied</skos:prefLabel>
    <skos:prefLabel xml:lang="fi">Lied</skos:prefLabel>
    <skos:prefLabel xml:lang="fr">Lied</skos:prefLabel>
    <skos:prefLabel xml:lang="de">Kunstlied</skos:prefLabel>
    <skos:prefLabel xml:lang="el">Ληντ</skos:prefLabel>
    <skos:prefLabel xml:lang="it">Lied</skos:prefLabel>
    <skos:prefLabel xml:lang="ja">歌曲</skos:prefLabel>
    <skos:prefLabel xml:lang="ko">가곡</skos:prefLabel>
    <skos:prefLabel xml:lang="ms">Lied</skos:prefLabel>
    <skos:prefLabel xml:lang="no">Lied</skos:prefLabel>
    <skos:prefLabel xml:lang="pt">Lied</skos:prefLabel>
    <skos:prefLabel xml:lang="ro">Lied</skos:prefLabel>
    <skos:prefLabel xml:lang="sl">Samospev</skos:prefLabel>
    <skos:prefLabel xml:lang="es">Lied</skos:prefLabel>
    <skos:prefLabel xml:lang="sv">Romans</skos:prefLabel>
    <skos:prefLabel xml:lang="tr">Lied</skos:prefLabel>
    <skos:prefLabel xml:lang="vi">Lied</skos:prefLabel>
    <skos:closeMatch rdf:resource="http://rdf.freebase.com/ns/m.0kv42"/>
    <skos:broader rdf:resource="http://data.europeana.eu/concept/music/genre/Classical_music"/>
    <skos:definition xml:lang="en">Lied is a German and Dutch word literally meaning
      &quot;song&quot;. It usually describes the setting of romantic German poems to music,
      especially during the nineteenth century, beginning with Carl Loewe, Heinrich Marschner, and
      Franz Schubert. Among English speakers, &quot;Lied&quot; is often used interchangeably with
      &quot;art song&quot; to encompass works that the tradition has inspired in other languages.
      The poetry forming the basis for Lieder often centers upon pastoral themes, or themes of
      romantic love. &lt;p&gt; Typically, Lieder are arranged for a single singer and piano, the
      Lied with orchestral accompaniment being a later development. Some of the most famous examples
      of Lieder are Schubert's &quot;Der Tod und das Mädchen&quot; and &quot;Gretchen am
      Spinnrade&quot;. Sometimes Lieder are gathered in a Liederkreis or &quot;song cycle&quot;—a
      series of songs tied by a single narrative or theme, such as Schubert's Die schöne Müllerin
      and Winterreise, or Robert Schumann's Frauenliebe und -leben and Dichterliebe. Schubert,
      Schumann and Johannes Brahms are most closely associated with this genre, mainly developed in
      the Romantic era.</skos:definition>
    <skos:exactMatch xml:lang="en">http://dbpedia.org/resource/Lied</skos:exactMatch>
    <skos:inScheme rdf:resource="http://data.europeana.eu/concept/music/genre/Music_Genre_Scheme"/>
    <skos:altLabel xml:lang="en">Lied</skos:altLabel>
  </skos:Concept>

  <skos:Concept rdf:about="http://data.europeana.eu/concept/music/genre/Mbalax">
    <skos:prefLabel xml:lang="en">Mbalax</skos:prefLabel>
    <skos:prefLabel xml:lang="ca">Mbalakh</skos:prefLabel>
    <skos:prefLabel xml:lang="fi">Mbalax</skos:prefLabel>
    <skos:prefLabel xml:lang="fr">Mbalax</skos:prefLabel>
    <skos:prefLabel xml:lang="de">Mbalax</skos:prefLabel>
    <skos:prefLabel xml:lang="it">Mbalax</skos:prefLabel>
    <skos:prefLabel xml:lang="ja">ンバラ</skos:prefLabel>
    <skos:prefLabel xml:lang="es">Mbalax</skos:prefLabel>
    <skos:prefLabel xml:lang="sv">Mbalax</skos:prefLabel>
    <skos:closeMatch rdf:resource="http://rdf.freebase.com/ns/m.098tks"/>
    <skos:broader
      rdf:resource="http://data.europeana.eu/concept/music/genre/African_popular_music_fusions"/>
    <skos:definition xml:lang="en">Mbalax is the national popular dance music of Senegal and the
      Gambia. Mbalax is a fusion of popular Western music and dance such as jazz, soul, Latin, and
      rock blended with sabar, the traditional drumming and dance music of Senegal. The genre's name
      derived from the heavy use of accompanying rhythms used in sabar called
      mbalax.</skos:definition>
    <skos:exactMatch xml:lang="en">http://dbpedia.org/resource/Mbalax</skos:exactMatch>
    <skos:inScheme rdf:resource="http://data.europeana.eu/concept/music/genre/Music_Genre_Scheme"/>
    <skos:altLabel xml:lang="en">Mbalax</skos:altLabel>
  </skos:Concept>

  <skos:Concept rdf:about="http://data.europeana.eu/concept/music/genre/Morenada">
    <skos:prefLabel xml:lang="en">Morenada</skos:prefLabel>
    <skos:prefLabel xml:lang="it">Morenada</skos:prefLabel>
    <skos:prefLabel xml:lang="es">Morenada</skos:prefLabel>
    <skos:closeMatch rdf:resource="http://rdf.freebase.com/ns/m.03ntnpr"/>
    <skos:broader
      rdf:resource="http://data.europeana.eu/concept/music/genre/Latin_American_music_traditional"/>
    <skos:definition xml:lang="en">The Morenada is a dance from the Peruvian and Bolivian Andes. The
      dance represents the black slaves brought to Peru and Bolivia.</skos:definition>
    <skos:exactMatch xml:lang="en">http://dbpedia.org/resource/Morenada</skos:exactMatch>
    <skos:inScheme rdf:resource="http://data.europeana.eu/concept/music/genre/Music_Genre_Scheme"/>
    <skos:altLabel xml:lang="en">Morenada</skos:altLabel>
  </skos:Concept>

  <skos:Concept rdf:about="http://data.europeana.eu/concept/music/genre/Narcocorrido">
    <skos:prefLabel xml:lang="en">Narcocorrido</skos:prefLabel>
    <skos:prefLabel xml:lang="nl">Narcocorrido</skos:prefLabel>
    <skos:prefLabel xml:lang="de">Narcocorrido</skos:prefLabel>
    <skos:prefLabel xml:lang="hu">Narcocorrido</skos:prefLabel>
    <skos:prefLabel xml:lang="es">Narcocorrido</skos:prefLabel>
    <skos:prefLabel xml:lang="sv">Narcocorrido</skos:prefLabel>
    <skos:closeMatch rdf:resource="http://rdf.freebase.com/ns/m.04zc4t"/>
    <skos:broader
      rdf:resource="http://data.europeana.eu/concept/music/genre/Latin_American_music_traditional"/>
    <skos:definition xml:lang="en">A narco-corrido is a sub-genere of the Mexican norteño-corrido
      music genre, a traditional folk music from northern Mexico, from which other several genres
      have evolved. This type of music is heard on both sides of the US–Mexican border. It uses a
      danceable, accordion-based polka as a rhythmic base. The first corridos that focus on drug
      smugglers—the narco comes from &quot;narcotics&quot;—have been dated by Juan Ramírez-Pimienta
      to the 1930s. Early corridos go back as far to the Mexican Revolution of 1910, telling the
      stories of revolutionary fighters. Music critics have also compared narcocorrido music to
      gangster rap. &lt;p&gt; Narcocorrido lyrics refer to particular events and include real dates
      and places. The lyrics tend to speak approvingly of illegal activities such as murder,
      torture, racketeering, extortion, drug smuggling, illegal immigration, and sometimes political
      protest due to government corruption.</skos:definition>
    <skos:exactMatch xml:lang="en">http://dbpedia.org/resource/Narcocorrido</skos:exactMatch>
    <skos:inScheme rdf:resource="http://data.europeana.eu/concept/music/genre/Music_Genre_Scheme"/>
    <skos:altLabel xml:lang="en">Narcocorrido</skos:altLabel>
  </skos:Concept>

  <skos:Concept rdf:about="http://data.europeana.eu/concept/music/genre/New_Age">
    <skos:prefLabel xml:lang="en">New Age</skos:prefLabel>
    <skos:prefLabel xml:lang="ar">العصر الجديد</skos:prefLabel>
    <skos:prefLabel xml:lang="bg">Нова епоха</skos:prefLabel>
    <skos:prefLabel xml:lang="ca">New Age</skos:prefLabel>
    <skos:prefLabel xml:lang="hr">New Age</skos:prefLabel>
    <skos:prefLabel xml:lang="cs">New Age</skos:prefLabel>
    <skos:prefLabel xml:lang="da">New age</skos:prefLabel>
    <skos:prefLabel xml:lang="nl">New age</skos:prefLabel>
    <skos:prefLabel xml:lang="et">New Age</skos:prefLabel>
    <skos:prefLabel xml:lang="fi">New Age</skos:prefLabel>
    <skos:prefLabel xml:lang="fr">New Age</skos:prefLabel>
    <skos:prefLabel xml:lang="de">New Age</skos:prefLabel>
    <skos:prefLabel xml:lang="hu">New Age</skos:prefLabel>
    <skos:prefLabel xml:lang="id">Zaman Baru</skos:prefLabel>
    <skos:prefLabel xml:lang="it">New Age</skos:prefLabel>
    <skos:prefLabel xml:lang="ja">ニューエイジ</skos:prefLabel>
    <skos:prefLabel xml:lang="ko">뉴에이지</skos:prefLabel>
    <skos:prefLabel xml:lang="lt">Naujasis Amžius</skos:prefLabel>
    <skos:prefLabel xml:lang="ms">Zaman Baru</skos:prefLabel>
    <skos:prefLabel xml:lang="no">New age</skos:prefLabel>
    <skos:prefLabel xml:lang="pl">New Age</skos:prefLabel>
    <skos:prefLabel xml:lang="pt">Nova Era</skos:prefLabel>
    <skos:prefLabel xml:lang="ro">New Age</skos:prefLabel>
    <skos:prefLabel xml:lang="ru">Нью Эйдж</skos:prefLabel>
    <skos:prefLabel xml:lang="sr">Nju ejdž</skos:prefLabel>
    <skos:prefLabel xml:lang="sk">New Age</skos:prefLabel>
    <skos:prefLabel xml:lang="es">Nueva era</skos:prefLabel>
    <skos:prefLabel xml:lang="sv">New Age</skos:prefLabel>
    <skos:prefLabel xml:lang="tr">New Age</skos:prefLabel>
    <skos:prefLabel xml:lang="uk">Нью-ейдж</skos:prefLabel>
    <skos:closeMatch rdf:resource="http://rdf.freebase.com/ns/m.05g9_"/>
    <skos:broader rdf:resource="http://data.europeana.eu/concept/music/genre/Electronic_music"/>
    <skos:definition xml:lang="en">The New Age movement is a Western spiritual movement that
      developed in the second half of the 20th century. Its central precepts have been described as
      &quot;drawing on both Eastern and Western spiritual and metaphysical traditions and infusing
      them with influences from self-help and motivational psychology&quot;. The term New Age refers
      to the coming astrological Age of Aquarius. &lt;p&gt; The movement aims to create &quot;a
      spirituality without borders or confining dogmas&quot; that is inclusive and pluralistic. It
      holds to &quot;a holistic worldview&quot;, emphasising that the Mind, Body, and Spirit are
      interrelated and that there is a form of monism and unity throughout the universe. It attempts
      to create &quot;a worldview that includes both science and spirituality&quot; and embraces a
      number of forms of mainstream science as well as other forms of science that are considered
      fringe. &lt;p&gt; The origins of the movement can be found in Medieval astrology and alchemy,
      such as the writings of Paracelsus, in Renaissance interests in Hermeticism, in 18th-century
      mysticism, such as that of Emanuel Swedenborg, and in beliefs in animal magnetism espoused by
      Franz Mesmer.</skos:definition>
    <skos:exactMatch xml:lang="en">http://dbpedia.org/resource/New_Age</skos:exactMatch>
    <skos:inScheme rdf:resource="http://data.europeana.eu/concept/music/genre/Music_Genre_Scheme"/>
    <skos:altLabel xml:lang="en">New Age</skos:altLabel>
  </skos:Concept>

  <skos:Concept rdf:about="http://data.europeana.eu/concept/music/genre/Opera">
    <skos:prefLabel xml:lang="en">Opera</skos:prefLabel>
    <skos:prefLabel xml:lang="ar">أوبرا</skos:prefLabel>
    <skos:prefLabel xml:lang="bg">Опера</skos:prefLabel>
    <skos:prefLabel xml:lang="ca">Òpera</skos:prefLabel>
    <skos:prefLabel xml:lang="hr">Opera</skos:prefLabel>
    <skos:prefLabel xml:lang="cs">Opera</skos:prefLabel>
    <skos:prefLabel xml:lang="da">Opera</skos:prefLabel>
    <skos:prefLabel xml:lang="nl">Opera</skos:prefLabel>
    <skos:prefLabel xml:lang="et">Ooper</skos:prefLabel>
    <skos:prefLabel xml:lang="fil">Opera</skos:prefLabel>
    <skos:prefLabel xml:lang="fi">Ooppera</skos:prefLabel>
    <skos:prefLabel xml:lang="fr">Opéra</skos:prefLabel>
    <skos:prefLabel xml:lang="de">Oper</skos:prefLabel>
    <skos:prefLabel xml:lang="el">Όπερα</skos:prefLabel>
    <skos:prefLabel xml:lang="hi">ओपेरा</skos:prefLabel>
    <skos:prefLabel xml:lang="hu">Opera</skos:prefLabel>
    <skos:prefLabel xml:lang="id">Opera</skos:prefLabel>
    <skos:prefLabel xml:lang="it">Opera</skos:prefLabel>
    <skos:prefLabel xml:lang="ja">オペラ</skos:prefLabel>
    <skos:prefLabel xml:lang="ko">오페라</skos:prefLabel>
    <skos:prefLabel xml:lang="lv">Opera</skos:prefLabel>
    <skos:prefLabel xml:lang="lt">Opera</skos:prefLabel>
    <skos:prefLabel xml:lang="ms">Opera</skos:prefLabel>
    <skos:prefLabel xml:lang="no">Opera</skos:prefLabel>
    <skos:prefLabel xml:lang="fa">اپرا</skos:prefLabel>
    <skos:prefLabel xml:lang="pl">Opera</skos:prefLabel>
    <skos:prefLabel xml:lang="pt">Ópera</skos:prefLabel>
    <skos:prefLabel xml:lang="ro">Operă</skos:prefLabel>
    <skos:prefLabel xml:lang="ru">Опера</skos:prefLabel>
    <skos:prefLabel xml:lang="sr">Опера</skos:prefLabel>
    <skos:prefLabel xml:lang="sk">Opera</skos:prefLabel>
    <skos:prefLabel xml:lang="sl">Opera</skos:prefLabel>
    <skos:prefLabel xml:lang="es">Ópera</skos:prefLabel>
    <skos:prefLabel xml:lang="sv">Opera</skos:prefLabel>
    <skos:prefLabel xml:lang="th">โอเปร่า</skos:prefLabel>
    <skos:prefLabel xml:lang="tr">Opera</skos:prefLabel>
    <skos:prefLabel xml:lang="uk">Опера</skos:prefLabel>
    <skos:prefLabel xml:lang="vi">Opera</skos:prefLabel>
    <skos:closeMatch rdf:resource="http://rdf.freebase.com/ns/m.05lls"/>
    <skos:broader rdf:resource="http://data.europeana.eu/concept/music/genre/Classical_music"/>
    <skos:definition xml:lang="en">Opera is an art form in which singers and musicians perform a
      dramatic work combining text and musical score, usually in a theatrical setting. Opera
      incorporates many of the elements of spoken theatre, such as acting, scenery, and costumes and
      sometimes includes dance. The performance is typically given in an opera house, accompanied by
      an orchestra or smaller musical ensemble. &lt;p&gt; Opera is part of the Western classical
      music tradition. It started in Italy at the end of the 16th century and soon spread through
      the rest of Europe: Schütz in Germany, Lully in France, and Purcell in England all helped to
      establish their national traditions in the 17th century. In the 18th century, Italian opera
      continued to dominate most of Europe, except France, attracting foreign composers such as
      Handel. Opera seria was the most prestigious form of Italian opera, until Gluck reacted
      against its artificiality with his &quot;reform&quot; operas in the 1760s.</skos:definition>
    <skos:exactMatch xml:lang="en">http://dbpedia.org/resource/Opera</skos:exactMatch>
    <skos:inScheme rdf:resource="http://data.europeana.eu/concept/music/genre/Music_Genre_Scheme"/>
    <skos:altLabel xml:lang="en">Opera</skos:altLabel>
  </skos:Concept>

  <skos:Concept rdf:about="http://data.europeana.eu/concept/music/genre/Operetta">
    <skos:prefLabel xml:lang="en">Operetta</skos:prefLabel>
    <skos:prefLabel xml:lang="ar">أوبريت</skos:prefLabel>
    <skos:prefLabel xml:lang="bg">Оперета</skos:prefLabel>
    <skos:prefLabel xml:lang="ca">Opereta</skos:prefLabel>
    <skos:prefLabel xml:lang="hr">Opereta</skos:prefLabel>
    <skos:prefLabel xml:lang="cs">Opereta</skos:prefLabel>
    <skos:prefLabel xml:lang="da">Operette</skos:prefLabel>
    <skos:prefLabel xml:lang="nl">Operette</skos:prefLabel>
    <skos:prefLabel xml:lang="et">Operett</skos:prefLabel>
    <skos:prefLabel xml:lang="fi">Operetti</skos:prefLabel>
    <skos:prefLabel xml:lang="fr">Opérette</skos:prefLabel>
    <skos:prefLabel xml:lang="de">Operette</skos:prefLabel>
    <skos:prefLabel xml:lang="el">Οπερέτα</skos:prefLabel>
    <skos:prefLabel xml:lang="hu">Operett</skos:prefLabel>
    <skos:prefLabel xml:lang="id">Operet</skos:prefLabel>
    <skos:prefLabel xml:lang="it">Operetta</skos:prefLabel>
    <skos:prefLabel xml:lang="ja">オペレッタ</skos:prefLabel>
    <skos:prefLabel xml:lang="ko">오페레타</skos:prefLabel>
    <skos:prefLabel xml:lang="lv">Operete</skos:prefLabel>
    <skos:prefLabel xml:lang="lt">Operetė</skos:prefLabel>
    <skos:prefLabel xml:lang="ms">Opereta</skos:prefLabel>
    <skos:prefLabel xml:lang="no">Operette</skos:prefLabel>
    <skos:prefLabel xml:lang="fa">اپرت</skos:prefLabel>
    <skos:prefLabel xml:lang="pl">Operetka</skos:prefLabel>
    <skos:prefLabel xml:lang="pt">Opereta</skos:prefLabel>
    <skos:prefLabel xml:lang="ro">Operetă</skos:prefLabel>
    <skos:prefLabel xml:lang="ru">Оперетта</skos:prefLabel>
    <skos:prefLabel xml:lang="sr">Оперета</skos:prefLabel>
    <skos:prefLabel xml:lang="sk">Opereta</skos:prefLabel>
    <skos:prefLabel xml:lang="sl">Opereta</skos:prefLabel>
    <skos:prefLabel xml:lang="es">Opereta</skos:prefLabel>
    <skos:prefLabel xml:lang="sv">Operett</skos:prefLabel>
    <skos:prefLabel xml:lang="tr">Operet</skos:prefLabel>
    <skos:prefLabel xml:lang="uk">Оперета</skos:prefLabel>
    <skos:prefLabel xml:lang="vi">Operetta</skos:prefLabel>
    <skos:closeMatch rdf:resource="http://rdf.freebase.com/ns/m.09swn"/>
    <skos:broader rdf:resource="http://data.europeana.eu/concept/music/genre/Classical_music"/>
    <skos:definition xml:lang="en">Operetta is a genre of light opera, light in terms both of music
      and subject matter. It is also closely related, in English-language works, to forms of musical
      theatre.</skos:definition>
    <skos:exactMatch xml:lang="en">http://dbpedia.org/resource/Operetta</skos:exactMatch>
    <skos:inScheme rdf:resource="http://data.europeana.eu/concept/music/genre/Music_Genre_Scheme"/>
    <skos:altLabel xml:lang="en">Operetta</skos:altLabel>
  </skos:Concept>

  <skos:Concept rdf:about="http://data.europeana.eu/concept/music/genre/Oratorio">
    <skos:prefLabel xml:lang="en">Oratorio</skos:prefLabel>
    <skos:prefLabel xml:lang="ar">أوراتوريو</skos:prefLabel>
    <skos:prefLabel xml:lang="bg">Оратория</skos:prefLabel>
    <skos:prefLabel xml:lang="ca">Oratori</skos:prefLabel>
    <skos:prefLabel xml:lang="hr">Oratorij</skos:prefLabel>
    <skos:prefLabel xml:lang="cs">Oratorium</skos:prefLabel>
    <skos:prefLabel xml:lang="da">Oratorium</skos:prefLabel>
    <skos:prefLabel xml:lang="nl">Oratorium</skos:prefLabel>
    <skos:prefLabel xml:lang="et">Oratoorium</skos:prefLabel>
    <skos:prefLabel xml:lang="fi">Oratorio</skos:prefLabel>
    <skos:prefLabel xml:lang="fr">Oratorio</skos:prefLabel>
    <skos:prefLabel xml:lang="de">Oratorium</skos:prefLabel>
    <skos:prefLabel xml:lang="el">Ορατόριο</skos:prefLabel>
    <skos:prefLabel xml:lang="hu">Oratórium</skos:prefLabel>
    <skos:prefLabel xml:lang="id">Oratorio</skos:prefLabel>
    <skos:prefLabel xml:lang="it">Oratorio</skos:prefLabel>
    <skos:prefLabel xml:lang="ja">オラトリオ</skos:prefLabel>
    <skos:prefLabel xml:lang="ko">오라토리오</skos:prefLabel>
    <skos:prefLabel xml:lang="lv">Oratorija</skos:prefLabel>
    <skos:prefLabel xml:lang="ms">Oratorio</skos:prefLabel>
    <skos:prefLabel xml:lang="no">Oratorium</skos:prefLabel>
    <skos:prefLabel xml:lang="fa">ارتوریو</skos:prefLabel>
    <skos:prefLabel xml:lang="pl">Oratorium</skos:prefLabel>
    <skos:prefLabel xml:lang="pt">Oratório</skos:prefLabel>
    <skos:prefLabel xml:lang="ro">Oratoriu</skos:prefLabel>
    <skos:prefLabel xml:lang="ru">Оратория</skos:prefLabel>
    <skos:prefLabel xml:lang="sr">Ораторијум</skos:prefLabel>
    <skos:prefLabel xml:lang="sk">Oratórium</skos:prefLabel>
    <skos:prefLabel xml:lang="sl">Oratorij</skos:prefLabel>
    <skos:prefLabel xml:lang="es">Oratorio</skos:prefLabel>
    <skos:prefLabel xml:lang="sv">Oratorium</skos:prefLabel>
    <skos:prefLabel xml:lang="th">ออราทอริโอ</skos:prefLabel>
    <skos:prefLabel xml:lang="tr">Oratoryo</skos:prefLabel>
    <skos:prefLabel xml:lang="uk">Ораторія</skos:prefLabel>
    <skos:closeMatch rdf:resource="http://rdf.freebase.com/ns/m.0knl9"/>
    <skos:broader rdf:resource="http://data.europeana.eu/concept/music/genre/Religious_music"/>
    <skos:definition xml:lang="en">An oratorio is a large musical composition for orchestra, choir,
      and soloists. Like an opera, an oratorio includes the use of a choir, soloists, an ensemble,
      various distinguishable characters, and arias. However, opera is musical theatre, while
      oratorio is strictly a concert piece—though oratorios are sometimes staged as operas, and
      operas are sometimes presented in concert form. In an oratorio there is generally little or no
      interaction between the characters, and no props or elaborate costumes. A particularly
      important difference is in the typical subject matter of the text. Opera tends to deal with
      history and mythology, including age-old devices of romance, deception, and murder, whereas
      the plot of an oratorio often deals with sacred topics, making it appropriate for performance
      in the church. Protestant composers took their stories from the Bible, while Catholic
      composers looked to the lives of saints, as well as to Biblical topics. Oratorios became
      extremely popular in early 17th-century Italy partly because of the success of opera and the
      Catholic Church's prohibition of spectacles during Lent.</skos:definition>
    <skos:exactMatch xml:lang="en">http://dbpedia.org/resource/Oratorio</skos:exactMatch>
    <skos:inScheme rdf:resource="http://data.europeana.eu/concept/music/genre/Music_Genre_Scheme"/>
    <skos:altLabel xml:lang="en">Oratorio</skos:altLabel>
  </skos:Concept>

  <skos:Concept rdf:about="http://data.europeana.eu/concept/music/genre/Pagode">
    <skos:prefLabel xml:lang="en">Pagode</skos:prefLabel>
    <skos:prefLabel xml:lang="fr">Pagode</skos:prefLabel>
    <skos:prefLabel xml:lang="pl">Pagode</skos:prefLabel>
    <skos:prefLabel xml:lang="pt">Pagode</skos:prefLabel>
    <skos:closeMatch rdf:resource="http://rdf.freebase.com/ns/m.03z2yd"/>
    <skos:broader
      rdf:resource="http://data.europeana.eu/concept/music/genre/Latin_American_music_popular"/>
    <skos:definition xml:lang="en">Pagode is a Brazilian style of music which originated in Rio de
      Janeiro, Brazil, as a subgenre of Samba. Pagode originally meant a celebration with lots of
      food, music, dance and party. In 1978, singer Beth Carvalho was introduced to this music,
      liked it from the beginning and recorded tracks by Zeca Pagodinho and others. Apparently, as
      time has gone by, the term &quot;Pagode&quot; has been degraded by many commercial groups who
      have played a version of the music full of clichés, and there is now a sense in which the term
      Pagode means very commercial pop, a negative term. &lt;p&gt; Original Pagode developed in the
      start of the 1980s, with the advent of the band Fundo de Quintal and the introduction of new
      instruments in the classical samba formation. Pagode lyricism also represented a kind of
      evolution towards the tradition of malicious and ironic samba lyrics, with a much heavier use
      of slang and underground terms. &lt;p&gt; The 4-string banjo, whose introduction is mostly
      credited to Almir Guineto, has a different and louder sound than the cavaco, that loudness was
      an advantage in acoustic environments, where there are lots of percussion instruments and
      people singing along. The 4-string banjo is one of the most characteristic instruments of the
      pagode sound.</skos:definition>
    <skos:exactMatch xml:lang="en">http://dbpedia.org/resource/Pagode</skos:exactMatch>
    <skos:inScheme rdf:resource="http://data.europeana.eu/concept/music/genre/Music_Genre_Scheme"/>
    <skos:altLabel xml:lang="en">Pagode</skos:altLabel>
  </skos:Concept>

  <skos:Concept rdf:about="http://data.europeana.eu/concept/music/genre/Pasillo">
    <skos:prefLabel xml:lang="en">Pasillo</skos:prefLabel>
    <skos:prefLabel xml:lang="es">Pasillo</skos:prefLabel>
    <skos:closeMatch rdf:resource="http://rdf.freebase.com/ns/m.0274r_b"/>
    <skos:broader rdf:resource="http://data.europeana.eu/concept/music/genre/Art_music"/>
    <skos:definition xml:lang="en">Pasillo is a South American genre of music extremely popular in
      the territories that composed the 19th century Viceroyalty of New Granada and Gran Colombia:
      Borns in the Capital of Gran Colombia, Bogotá Colombia, spread in the territory, especially
      Ecuador, and to a lesser extent in the mountainous regions of Venezuela and Panama.
      Venezuelans refer to this style of music as &quot;vals&quot;. &lt;p&gt; Today, it has
      incorporated more European features of classical dance, such as Viennese waltz in Colombia and
      features of sanjuanito and yaraví in Ecuador. As it spread during the Gran Colombia period,
      pasillo also absorbed the individual characteristics of isolated villages. This gives it an
      eclectic feel, however, the style, tone, and tempo of the music differ in each village and
      indeed between each country. &lt;p&gt; In its waltz, pasillo alters the classically European
      dance form to accompany guitar, mandolin, and other string instruments.</skos:definition>
    <skos:exactMatch xml:lang="en">http://dbpedia.org/resource/Pasillo</skos:exactMatch>
    <skos:inScheme rdf:resource="http://data.europeana.eu/concept/music/genre/Music_Genre_Scheme"/>
    <skos:altLabel xml:lang="en">Pasillo</skos:altLabel>
  </skos:Concept>

  <skos:Concept rdf:about="http://data.europeana.eu/concept/music/genre/Polka">
    <skos:prefLabel xml:lang="en">Polka</skos:prefLabel>
    <skos:prefLabel xml:lang="ar">بولكا</skos:prefLabel>
    <skos:prefLabel xml:lang="ca">Polca</skos:prefLabel>
    <skos:prefLabel xml:lang="hr">Polka</skos:prefLabel>
    <skos:prefLabel xml:lang="cs">Polka</skos:prefLabel>
    <skos:prefLabel xml:lang="da">Polka</skos:prefLabel>
    <skos:prefLabel xml:lang="nl">Polka</skos:prefLabel>
    <skos:prefLabel xml:lang="et">Polka</skos:prefLabel>
    <skos:prefLabel xml:lang="fil">Polka</skos:prefLabel>
    <skos:prefLabel xml:lang="fi">Polkka</skos:prefLabel>
    <skos:prefLabel xml:lang="fr">Polka</skos:prefLabel>
    <skos:prefLabel xml:lang="de">Polka</skos:prefLabel>
    <skos:prefLabel xml:lang="el">Πόλκα</skos:prefLabel>
    <skos:prefLabel xml:lang="id">Polka</skos:prefLabel>
    <skos:prefLabel xml:lang="it">Polka</skos:prefLabel>
    <skos:prefLabel xml:lang="ja">ポルカ</skos:prefLabel>
    <skos:prefLabel xml:lang="ko">폴카</skos:prefLabel>
    <skos:prefLabel xml:lang="lt">Polka</skos:prefLabel>
    <skos:prefLabel xml:lang="no">Polka</skos:prefLabel>
    <skos:prefLabel xml:lang="pl">Polka</skos:prefLabel>
    <skos:prefLabel xml:lang="pt">Polca</skos:prefLabel>
    <skos:prefLabel xml:lang="ru">Полька</skos:prefLabel>
    <skos:prefLabel xml:lang="sr">Полка</skos:prefLabel>
    <skos:prefLabel xml:lang="sl">Polka</skos:prefLabel>
    <skos:prefLabel xml:lang="es">Polca</skos:prefLabel>
    <skos:prefLabel xml:lang="sv">Polka</skos:prefLabel>
    <skos:prefLabel xml:lang="th">โพลกา</skos:prefLabel>
    <skos:prefLabel xml:lang="tr">polka</skos:prefLabel>
    <skos:prefLabel xml:lang="uk">Полька</skos:prefLabel>
    <skos:prefLabel xml:lang="en">Polca</skos:prefLabel>
    <skos:closeMatch rdf:resource="http://rdf.freebase.com/ns/m.0bwqb"/>
    <skos:broader rdf:resource="http://data.europeana.eu/concept/music/genre/Folk_music_traditional"/>
    <skos:definition xml:lang="en">The polka is a Central European dance and also a genre of dance
      music familiar throughout Europe and the Americas. It originated in the middle of the 19th
      century in Bohemia. Polka is still a popular genre of folk music in many European countries
      and is performed by folk artists in Poland, Latvia, Lithuania, Czech Republic, Netherlands,
      Croatia, Slovenia, Germany, Hungary, Austria, Switzerland, Italy, Ukraine, Belarus, Russia and
      Slovakia. Local varieties of this dance are also found in the Nordic countries, United
      Kingdom, France, Ireland, Latin America and in the United States.</skos:definition>
    <skos:exactMatch xml:lang="en">http://dbpedia.org/resource/Polka</skos:exactMatch>
    <skos:inScheme rdf:resource="http://data.europeana.eu/concept/music/genre/Music_Genre_Scheme"/>
    <skos:altLabel xml:lang="en">Polka</skos:altLabel>
  </skos:Concept>

  <skos:Concept rdf:about="http://data.europeana.eu/concept/music/genre/Porro">
    <skos:prefLabel xml:lang="en">Porro</skos:prefLabel>
    <skos:prefLabel xml:lang="nl">Porro</skos:prefLabel>
    <skos:prefLabel xml:lang="es">Porro</skos:prefLabel>
    <skos:closeMatch rdf:resource="http://rdf.freebase.com/ns/m.0c527_"/>
    <skos:broader
      rdf:resource="http://data.europeana.eu/concept/music/genre/Latin_American_music_traditional"/>
    <skos:definition xml:lang="en">The porro is a musical style and dance from the Caribbean region
      of Colombia. It is a Colombian cumbia rhythm that developed into its own sub-genre. It was
      originally a folkloric expression from the Sinú River area that evolved into a ballroom dance.
      It is played mostly by brass bands or orchestras and danced in couples. &lt;p&gt; The two
      types of folkloric porro are porro palitiao and porro tapao. The term &quot;palitiao&quot; is
      derived from the way the bombo drum is struck along its rim to produce the sound of a cowbell.
      This type of porro is associated with the Sinú River and its surrounding cities and towns.
      Most would agree on San Pelayo, Colombia, Córdoba as its place of birth. This is the reason
      why it can also take the name of porro pelayero. In orchestrated variants, porro palitiao or
      pelayero is known as gaita. See La Sonora Cordobesa and Pacho Galán for sample music of porro
      palitiao and gaita. &lt;p&gt; The porro tapao is associated with the savannas around
      Cartagena, Colombia. Its birthplace is believed to be the town of El Carmen de Bolívar,
      Colombia. In orchestrated forms, this type of porro gets the name of porro
      sabanero.</skos:definition>
    <skos:exactMatch xml:lang="en">http://dbpedia.org/resource/Porro</skos:exactMatch>
    <skos:inScheme rdf:resource="http://data.europeana.eu/concept/music/genre/Music_Genre_Scheme"/>
    <skos:altLabel xml:lang="en">Porro</skos:altLabel>
  </skos:Concept>

  <skos:Concept rdf:about="http://data.europeana.eu/concept/music/genre/Progressive_metal">
    <skos:prefLabel xml:lang="en">Progressive metal</skos:prefLabel>
    <skos:prefLabel xml:lang="ar">بروجريسف ميتال</skos:prefLabel>
    <skos:prefLabel xml:lang="bg">Прогресив метъл</skos:prefLabel>
    <skos:prefLabel xml:lang="ca">Metal progressiu</skos:prefLabel>
    <skos:prefLabel xml:lang="hr">Progresivni metal</skos:prefLabel>
    <skos:prefLabel xml:lang="cs">Progresivní metal</skos:prefLabel>
    <skos:prefLabel xml:lang="da">Progressiv metal</skos:prefLabel>
    <skos:prefLabel xml:lang="nl">Progressieve metal</skos:prefLabel>
    <skos:prefLabel xml:lang="fi">Progressiivinen metalli</skos:prefLabel>
    <skos:prefLabel xml:lang="fr">Metal progressif</skos:prefLabel>
    <skos:prefLabel xml:lang="de">Progressive Metal</skos:prefLabel>
    <skos:prefLabel xml:lang="el">Progressive Metal</skos:prefLabel>
    <skos:prefLabel xml:lang="hu">Progresszív metal</skos:prefLabel>
    <skos:prefLabel xml:lang="id">Progressive metal</skos:prefLabel>
    <skos:prefLabel xml:lang="it">Progressive metal</skos:prefLabel>
    <skos:prefLabel xml:lang="ja">プログレッシブ・メタル</skos:prefLabel>
    <skos:prefLabel xml:lang="ko">프로그레시브 메탈</skos:prefLabel>
    <skos:prefLabel xml:lang="lv">Progresīvais metāls</skos:prefLabel>
    <skos:prefLabel xml:lang="lt">Progresyvusis metalas</skos:prefLabel>
    <skos:prefLabel xml:lang="no">Progressiv metal</skos:prefLabel>
    <skos:prefLabel xml:lang="fa">پراگرسیو متال</skos:prefLabel>
    <skos:prefLabel xml:lang="pl">Metal progresywny</skos:prefLabel>
    <skos:prefLabel xml:lang="pt">Metal progressivo</skos:prefLabel>
    <skos:prefLabel xml:lang="ro">Metal progresiv</skos:prefLabel>
    <skos:prefLabel xml:lang="ru">Прогрессивный метал</skos:prefLabel>
    <skos:prefLabel xml:lang="sr">Прогресивни метал</skos:prefLabel>
    <skos:prefLabel xml:lang="sk">Progresívny metal</skos:prefLabel>
    <skos:prefLabel xml:lang="es">Metal progresivo</skos:prefLabel>
    <skos:prefLabel xml:lang="sv">Progressiv metal</skos:prefLabel>
    <skos:prefLabel xml:lang="th">โปรเกรสซีฟเมทัล</skos:prefLabel>
    <skos:prefLabel xml:lang="tr">Progresif metal</skos:prefLabel>
    <skos:prefLabel xml:lang="uk">Прогресивний метал</skos:prefLabel>
    <skos:closeMatch rdf:resource="http://rdf.freebase.com/ns/m.0hdf8"/>
    <skos:broader
      rdf:resource="http://data.europeana.eu/concept/music/genre/Heavy_metal_music_fusions"/>
    <skos:definition xml:lang="en">Progressive metal is a subgenre of both progressive rock and
      heavy metal, originating in the United Kingdom and the United States In the 1970s. Progressive
      metal blended elements of heavy metal and progressive rock music, taking the loud
      &quot;aggression&quot; and amplified electric guitar-driven sound of the former, with the more
      experimental, complex and &quot;pseudo-classical&quot; compositions of the latter. Progressive
      metal often utilises the conceptual themes associated with progressive rock. Throughout the
      years, progressive metal has borrowed influences from several other genres, including
      classical and jazz fusion music. &lt;p&gt; Whilst the genre emerged towards the late-1980s, it
      was not until the 1990s that progressive metal achieved commercial success. Dream Theater,
      Queensrÿche, Tool and Fates Warning are a few examples of progressive metal bands who achieved
      commercial success, additionally, heavy metal bands such as Metallica incorporated elements of
      progressive music in their work. Progressive metal's popularity started to decline towards the
      end of the 1990s, but it remains a largely underground genre with a committed fan
      base.</skos:definition>
    <skos:exactMatch xml:lang="en">http://dbpedia.org/resource/Progressive_metal</skos:exactMatch>
    <skos:inScheme rdf:resource="http://data.europeana.eu/concept/music/genre/Music_Genre_Scheme"/>
    <skos:altLabel xml:lang="en">Progressive metal</skos:altLabel>
  </skos:Concept>

  <skos:Concept rdf:about="http://data.europeana.eu/concept/music/genre/Psychedelic_rock">
    <skos:prefLabel xml:lang="en">Psychedelic rock</skos:prefLabel>
    <skos:prefLabel xml:lang="ar">سايكيديلك روك</skos:prefLabel>
    <skos:prefLabel xml:lang="bg">Психеделичен рок</skos:prefLabel>
    <skos:prefLabel xml:lang="ca">Rock psicodèlic</skos:prefLabel>
    <skos:prefLabel xml:lang="hr">Psihodelični rock</skos:prefLabel>
    <skos:prefLabel xml:lang="cs">Psychedelický rock</skos:prefLabel>
    <skos:prefLabel xml:lang="da">Psykedelisk rock</skos:prefLabel>
    <skos:prefLabel xml:lang="nl">Psychedelische rock</skos:prefLabel>
    <skos:prefLabel xml:lang="fi">Psykedeelinen rock</skos:prefLabel>
    <skos:prefLabel xml:lang="fr">Rock psychédélique</skos:prefLabel>
    <skos:prefLabel xml:lang="de">Psychedelic Rock</skos:prefLabel>
    <skos:prefLabel xml:lang="hu">Pszichedelikus rock</skos:prefLabel>
    <skos:prefLabel xml:lang="id">Psychedelic rock</skos:prefLabel>
    <skos:prefLabel xml:lang="it">Rock psichedelico</skos:prefLabel>
    <skos:prefLabel xml:lang="ja">サイケデリック・ロック</skos:prefLabel>
    <skos:prefLabel xml:lang="ko">사이키델릭 록</skos:prefLabel>
    <skos:prefLabel xml:lang="lv">Psihodēliskais roks</skos:prefLabel>
    <skos:prefLabel xml:lang="lt">Psichodelinis rokas</skos:prefLabel>
    <skos:prefLabel xml:lang="fa">سایکدلیک راک</skos:prefLabel>
    <skos:prefLabel xml:lang="pl">Rock psychodeliczny</skos:prefLabel>
    <skos:prefLabel xml:lang="pt">Música psicodélica</skos:prefLabel>
    <skos:prefLabel xml:lang="ro">Rock psihedelic</skos:prefLabel>
    <skos:prefLabel xml:lang="ru">Психоделический рок</skos:prefLabel>
    <skos:prefLabel xml:lang="sr">Психоделични рок</skos:prefLabel>
    <skos:prefLabel xml:lang="sk">Psychedelický rock</skos:prefLabel>
    <skos:prefLabel xml:lang="sl">Psihedelični rock</skos:prefLabel>
    <skos:prefLabel xml:lang="es">Rock psicodélico</skos:prefLabel>
    <skos:prefLabel xml:lang="sv">Psykedelisk musik</skos:prefLabel>
    <skos:prefLabel xml:lang="th">ไซเคเดลิกร็อก</skos:prefLabel>
    <skos:prefLabel xml:lang="tr">Psychedelic rock</skos:prefLabel>
    <skos:prefLabel xml:lang="uk">Психоделічний рок</skos:prefLabel>
    <skos:closeMatch rdf:resource="http://rdf.freebase.com/ns/m.05w3f"/>
    <skos:broader rdf:resource="http://data.europeana.eu/concept/music/genre/Rock_music_fusions"/>
    <skos:definition xml:lang="en">Psychedelic rock is a style of rock music that is inspired or
      influenced by psychedelic culture and attempts to replicate and enhance the mind-altering
      experiences of psychedelic drugs. It often uses new recording techniques and effects and draws
      on non-Western sources such as the ragas and drones of Indian music. &lt;p&gt; It was
      pioneered by musicians including the Beatles, the Byrds, and the Yardbirds, emerging as a
      genre during the mid-1960s among folk rock and blues rock bands in the United Kingdom and
      United States, such as Grateful Dead, Jefferson Airplane, the Jimi Hendrix Experience, Cream,
      the Doors and Pink Floyd. It reached a peak in between 1967 and 1969 with the Summer of Love
      and Woodstock Rock Festival, respectively, becoming an international musical movement and
      associated with a widespread counterculture, before beginning a decline as changing attitudes,
      the loss of some key individuals and a back-to-basics movement, led surviving performers to
      move into new musical areas. &lt;p&gt; Psychedelic rock influenced the creation of psychedelic
      pop and psychedelic soul.</skos:definition>
    <skos:exactMatch xml:lang="en">http://dbpedia.org/resource/Psychedelic_rock</skos:exactMatch>
    <skos:inScheme rdf:resource="http://data.europeana.eu/concept/music/genre/Music_Genre_Scheme"/>
    <skos:altLabel xml:lang="en">Psychedelic rock</skos:altLabel>
  </skos:Concept>

  <skos:Concept rdf:about="http://data.europeana.eu/concept/music/genre/Psychobilly">
    <skos:prefLabel xml:lang="en">Psychobilly</skos:prefLabel>
    <skos:prefLabel xml:lang="bg">Психобили</skos:prefLabel>
    <skos:prefLabel xml:lang="cs">Psychobilly</skos:prefLabel>
    <skos:prefLabel xml:lang="da">Psychobilly</skos:prefLabel>
    <skos:prefLabel xml:lang="nl">Psychobilly</skos:prefLabel>
    <skos:prefLabel xml:lang="fi">Psychobilly</skos:prefLabel>
    <skos:prefLabel xml:lang="fr">Psychobilly</skos:prefLabel>
    <skos:prefLabel xml:lang="de">Psychobilly</skos:prefLabel>
    <skos:prefLabel xml:lang="hu">Psychobilly</skos:prefLabel>
    <skos:prefLabel xml:lang="it">Psychobilly</skos:prefLabel>
    <skos:prefLabel xml:lang="ja">サイコビリー</skos:prefLabel>
    <skos:prefLabel xml:lang="ko">사이코빌리</skos:prefLabel>
    <skos:prefLabel xml:lang="lt">Psychobilly</skos:prefLabel>
    <skos:prefLabel xml:lang="pl">Psychobilly</skos:prefLabel>
    <skos:prefLabel xml:lang="pt">Psychobilly</skos:prefLabel>
    <skos:prefLabel xml:lang="ru">Сайкобилли</skos:prefLabel>
    <skos:prefLabel xml:lang="es">Psychobilly</skos:prefLabel>
    <skos:prefLabel xml:lang="sv">Psychobilly</skos:prefLabel>
    <skos:closeMatch rdf:resource="http://rdf.freebase.com/ns/m.018ysx"/>
    <skos:broader rdf:resource="http://data.europeana.eu/concept/music/genre/Punk_rock_fusions"/>
    <skos:definition xml:lang="en">Psychobilly is a fusion genre of rock music that mixes elements
      of punk rock, rockabilly, and other genres. It is one of several subgenres of rockabilly which
      also include thrashabilly, trashabilly, punkabilly, surfabilly and gothabilly. Merriam-Webster
      defines it as &quot;music that blends punk rock and rockabilly&quot;, another dictionary
      defines it as &quot;loud frantic rockabilly music.&quot; About.com defines psychobilly as
      &quot;tak[ing] the traditional countrified rock style known as rockabilly, ramp[ing] up its
      speed to a sweaty pace, and combin[ing] it with punk rock and imagery lifted from horror films
      and late-night sci-fi schlock,...[creating a] gritty honky tonk punk rock.&quot; Psychobilly,
      &quot;while rooted in the twang of rockabilly, owes just as much to the sound of straight up
      three-chord punk, often with a dose of thrash metal.&quot; &lt;p&gt; Psychobilly is often
      characterized by lyrical references to science fiction, horror and exploitation films,
      violence, lurid sexuality, and other topics generally considered taboo, though often presented
      in a comedic or tongue-in-cheek fashion.</skos:definition>
    <skos:exactMatch xml:lang="en">http://dbpedia.org/resource/Psychobilly</skos:exactMatch>
    <skos:inScheme rdf:resource="http://data.europeana.eu/concept/music/genre/Music_Genre_Scheme"/>
    <skos:altLabel xml:lang="en">Psychobilly</skos:altLabel>
  </skos:Concept>

  <skos:Concept rdf:about="http://data.europeana.eu/concept/music/genre/Punta">
    <skos:prefLabel xml:lang="en">Punta</skos:prefLabel>
    <skos:prefLabel xml:lang="fi">Punta</skos:prefLabel>
    <skos:prefLabel xml:lang="de">Punta</skos:prefLabel>
    <skos:prefLabel xml:lang="es">Punta</skos:prefLabel>
    <skos:prefLabel xml:lang="sv">Punta</skos:prefLabel>
    <skos:closeMatch rdf:resource="http://rdf.freebase.com/ns/m.04xl6b"/>
    <skos:broader
      rdf:resource="http://data.europeana.eu/concept/music/genre/Latin_American_music_traditional"/>
    <skos:definition xml:lang="en">Punta is a Garifuna music and dance style performed at
      celebrations and festive occasions. Contemporary punta arose in the last thirty years of the
      twentieth century in Belize, while the earliest notions of the punta dance precede the coming
      together of the West African tribes and the Amerindian tribes of the Caribbean in the 17th
      century The diaspora of Garinagu people, commonly called the &quot;Garifuna Nation&quot;,
      dates back to their origins of the amalgamation of West African slaves and the Arawak and
      Carib Amerindians. Punta is used to reaffirm and express the struggle felt by those of the
      indigenous population's common heritage through cultural art forms, such as dance and music
      and to highlight their strong sense of endurance. Besides Belize, punta also has a following
      in Honduras, Guatemala, Nicaragua, El Salvador, Southern Mexico and the United States. Lyrics
      may be in Garifuna, Kriol, English or Spanish. However, most songs are performed in the
      indigenous Awarak and Carib-based languages of the Garinagu and are often simply contemporary
      adaptations of traditional Garifuna songs. Being the most popular dance in Garifuna culture,
      punta can be performed at wakes, holidays, parties, ancestral celebrations, and other social
      events. Punta is iconic of Garifuna ethnicity and modernity, and can be seen as a poetic folk
      art that connects older cultures and rhythms with new sound. Chumba and hunguhungu, circular
      dances in triple rhythm, are often combined with punta.</skos:definition>
    <skos:exactMatch xml:lang="en">http://dbpedia.org/resource/Punta</skos:exactMatch>
    <skos:inScheme rdf:resource="http://data.europeana.eu/concept/music/genre/Music_Genre_Scheme"/>
    <skos:altLabel xml:lang="en">Punta</skos:altLabel>
  </skos:Concept>

  <skos:Concept rdf:about="http://data.europeana.eu/concept/music/genre/Ragtime">
    <skos:prefLabel xml:lang="en">Ragtime</skos:prefLabel>
    <skos:prefLabel xml:lang="ar">راجتايم</skos:prefLabel>
    <skos:prefLabel xml:lang="bg">Рагтайм</skos:prefLabel>
    <skos:prefLabel xml:lang="ca">Ragtime</skos:prefLabel>
    <skos:prefLabel xml:lang="cs">Ragtime</skos:prefLabel>
    <skos:prefLabel xml:lang="da">Ragtime</skos:prefLabel>
    <skos:prefLabel xml:lang="nl">Ragtime</skos:prefLabel>
    <skos:prefLabel xml:lang="et">Ragtime</skos:prefLabel>
    <skos:prefLabel xml:lang="fi">Ragtime</skos:prefLabel>
    <skos:prefLabel xml:lang="fr">Ragtime</skos:prefLabel>
    <skos:prefLabel xml:lang="de">Ragtime</skos:prefLabel>
    <skos:prefLabel xml:lang="el">Ράγκταϊμ</skos:prefLabel>
    <skos:prefLabel xml:lang="hu">Ragtime</skos:prefLabel>
    <skos:prefLabel xml:lang="it">Ragtime</skos:prefLabel>
    <skos:prefLabel xml:lang="ja">ラグタイム</skos:prefLabel>
    <skos:prefLabel xml:lang="lv">Regtaims</skos:prefLabel>
    <skos:prefLabel xml:lang="lt">Regtaimas</skos:prefLabel>
    <skos:prefLabel xml:lang="no">Ragtime</skos:prefLabel>
    <skos:prefLabel xml:lang="fa">رگتایم</skos:prefLabel>
    <skos:prefLabel xml:lang="pl">Ragtime</skos:prefLabel>
    <skos:prefLabel xml:lang="pt">Ragtime</skos:prefLabel>
    <skos:prefLabel xml:lang="ru">Регтайм</skos:prefLabel>
    <skos:prefLabel xml:lang="sk">Ragtime</skos:prefLabel>
    <skos:prefLabel xml:lang="sl">Ragtime</skos:prefLabel>
    <skos:prefLabel xml:lang="es">Ragtime</skos:prefLabel>
    <skos:prefLabel xml:lang="sv">Ragtime</skos:prefLabel>
    <skos:prefLabel xml:lang="uk">Реґтайм</skos:prefLabel>
    <skos:closeMatch rdf:resource="http://rdf.freebase.com/ns/m.06m6j"/>
    <skos:broader rdf:resource="http://data.europeana.eu/concept/music/genre/Jazz"/>
    <skos:definition xml:lang="en">Ragtime is a musical genre that enjoyed its peak popularity
      between 1895 and 1918. Its main characteristic trait is its syncopated, or &quot;ragged,&quot;
      rhythm. It began as dance music in the red-light districts of African American communities in
      St. Louis and New Orleans years before being published as popular sheet music for piano.
      Ernest Hogan was an innovator and key pioneer who helped develop the musical genre, and is
      credited with coining the term ragtime. Ragtime was also a modification of the march made
      popular by John Philip Sousa, with additional polyrhythms coming from African music. The
      ragtime composer Scott Joplin became famous through the publication in 1899 of the &quot;Maple
      Leaf Rag&quot; and a string of ragtime hits such as &quot;The Entertainer&quot; that followed,
      although he was later forgotten by all but a small, dedicated community of ragtime aficionados
      until the major ragtime revival in the early 1970s. For at least 12 years after its
      publication, the &quot;Maple Leaf Rag&quot; heavily influenced subsequent ragtime composers
      with its melody lines, harmonic progressions or metric patterns.</skos:definition>
    <skos:exactMatch xml:lang="en">http://dbpedia.org/resource/Ragtime</skos:exactMatch>
    <skos:inScheme rdf:resource="http://data.europeana.eu/concept/music/genre/Music_Genre_Scheme"/>
    <skos:altLabel xml:lang="en">Ragtime</skos:altLabel>
  </skos:Concept>

  <skos:Concept rdf:about="http://data.europeana.eu/concept/music/genre/Rebetiko">
    <skos:prefLabel xml:lang="en">Rebetiko</skos:prefLabel>
    <skos:prefLabel xml:lang="bg">Ребетико</skos:prefLabel>
    <skos:prefLabel xml:lang="ca">Rebétiko</skos:prefLabel>
    <skos:prefLabel xml:lang="cs">Rembetiko</skos:prefLabel>
    <skos:prefLabel xml:lang="da">Rembetika</skos:prefLabel>
    <skos:prefLabel xml:lang="nl">Rebetika</skos:prefLabel>
    <skos:prefLabel xml:lang="fi">Rebetiko</skos:prefLabel>
    <skos:prefLabel xml:lang="fr">Rebetiko</skos:prefLabel>
    <skos:prefLabel xml:lang="de">Rembetiko</skos:prefLabel>
    <skos:prefLabel xml:lang="el">Ρεμπέτικα</skos:prefLabel>
    <skos:prefLabel xml:lang="hu">Rembétiko</skos:prefLabel>
    <skos:prefLabel xml:lang="it">Rebetiko</skos:prefLabel>
    <skos:prefLabel xml:lang="pl">Rebetiko</skos:prefLabel>
    <skos:prefLabel xml:lang="pt">Rebético</skos:prefLabel>
    <skos:prefLabel xml:lang="ro">Rembetiko</skos:prefLabel>
    <skos:prefLabel xml:lang="ru">Ребетика</skos:prefLabel>
    <skos:prefLabel xml:lang="sr">Rebetiko</skos:prefLabel>
    <skos:prefLabel xml:lang="es">Rebético</skos:prefLabel>
    <skos:prefLabel xml:lang="sv">Rebetiko</skos:prefLabel>
    <skos:prefLabel xml:lang="tr">Rebetiko</skos:prefLabel>
    <skos:prefLabel xml:lang="uk">Ребетіко</skos:prefLabel>
    <skos:closeMatch rdf:resource="http://rdf.freebase.com/ns/m.04pvlc"/>
    <skos:broader rdf:resource="http://data.europeana.eu/concept/music/genre/Folk_music_traditional"/>
    <skos:definition xml:lang="en">Rebetiko, plural rebetika, occasionally transliterated as
      Rembetiko, is a term used today to designate originally disparate kinds of urban Greek folk
      music which have come to be grouped together since the so-called rebetika revival, which
      started in the 1960s and developed further from the early 1970s onwards.</skos:definition>
    <skos:exactMatch xml:lang="en">http://dbpedia.org/resource/Rebetiko</skos:exactMatch>
    <skos:inScheme rdf:resource="http://data.europeana.eu/concept/music/genre/Music_Genre_Scheme"/>
    <skos:altLabel xml:lang="en">Rebetiko</skos:altLabel>
  </skos:Concept>

  <skos:Concept rdf:about="http://data.europeana.eu/concept/music/genre/Reggae">
    <skos:prefLabel xml:lang="en">Reggae</skos:prefLabel>
    <skos:prefLabel xml:lang="ar">ريغي</skos:prefLabel>
    <skos:prefLabel xml:lang="bg">Реге</skos:prefLabel>
    <skos:prefLabel xml:lang="ca">Reggae</skos:prefLabel>
    <skos:prefLabel xml:lang="hr">Reggae</skos:prefLabel>
    <skos:prefLabel xml:lang="cs">Reggae</skos:prefLabel>
    <skos:prefLabel xml:lang="da">Reggae</skos:prefLabel>
    <skos:prefLabel xml:lang="nl">Reggae</skos:prefLabel>
    <skos:prefLabel xml:lang="et">Reggae</skos:prefLabel>
    <skos:prefLabel xml:lang="fi">Reggae</skos:prefLabel>
    <skos:prefLabel xml:lang="fr">Reggae</skos:prefLabel>
    <skos:prefLabel xml:lang="de">Reggae</skos:prefLabel>
    <skos:prefLabel xml:lang="el">Ρέγκε</skos:prefLabel>
    <skos:prefLabel xml:lang="hi">रेगे</skos:prefLabel>
    <skos:prefLabel xml:lang="hu">Reggae</skos:prefLabel>
    <skos:prefLabel xml:lang="id">Reggae</skos:prefLabel>
    <skos:prefLabel xml:lang="it">Reggae</skos:prefLabel>
    <skos:prefLabel xml:lang="ja">レゲエ</skos:prefLabel>
    <skos:prefLabel xml:lang="ko">레게</skos:prefLabel>
    <skos:prefLabel xml:lang="lv">Regejs</skos:prefLabel>
    <skos:prefLabel xml:lang="lt">Regis</skos:prefLabel>
    <skos:prefLabel xml:lang="ms">Rege</skos:prefLabel>
    <skos:prefLabel xml:lang="no">Reggae</skos:prefLabel>
    <skos:prefLabel xml:lang="fa">رگی</skos:prefLabel>
    <skos:prefLabel xml:lang="pl">Reggae</skos:prefLabel>
    <skos:prefLabel xml:lang="pt">Reggae</skos:prefLabel>
    <skos:prefLabel xml:lang="ro">Muzică reggae</skos:prefLabel>
    <skos:prefLabel xml:lang="ru">Регги</skos:prefLabel>
    <skos:prefLabel xml:lang="sr">Реге</skos:prefLabel>
    <skos:prefLabel xml:lang="sk">Reggae</skos:prefLabel>
    <skos:prefLabel xml:lang="sl">Reggae</skos:prefLabel>
    <skos:prefLabel xml:lang="es">Reggae</skos:prefLabel>
    <skos:prefLabel xml:lang="sv">Reggae</skos:prefLabel>
    <skos:prefLabel xml:lang="th">เร้กเก้</skos:prefLabel>
    <skos:prefLabel xml:lang="tr">Reggae</skos:prefLabel>
    <skos:prefLabel xml:lang="uk">Реґі</skos:prefLabel>
    <skos:prefLabel xml:lang="vi">Reggae</skos:prefLabel>
    <skos:closeMatch rdf:resource="http://rdf.freebase.com/ns/m.06cqb"/>
    <skos:broader
      rdf:resource="http://data.europeana.eu/concept/music/genre/Latin_American_music_popular"/>
    <skos:definition xml:lang="en">Reggae is a music genre first developed in Jamaica in the late
      1960s. While sometimes used in a broad sense to refer to most types of popular Jamaican dance
      music, the term reggae more properly denotes a particular music style that evolved out of the
      earlier genres ska and rocksteady.</skos:definition>
    <skos:exactMatch xml:lang="en">http://dbpedia.org/resource/Reggae</skos:exactMatch>
    <skos:inScheme rdf:resource="http://data.europeana.eu/concept/music/genre/Music_Genre_Scheme"/>
    <skos:altLabel xml:lang="en">Reggae</skos:altLabel>
  </skos:Concept>

  <skos:Concept rdf:about="http://data.europeana.eu/concept/music/genre/Reggaeton">
    <skos:prefLabel xml:lang="en">Reggaeton</skos:prefLabel>
    <skos:prefLabel xml:lang="ar">ريغيه تون</skos:prefLabel>
    <skos:prefLabel xml:lang="ca">Reggaeton</skos:prefLabel>
    <skos:prefLabel xml:lang="cs">Reggaeton</skos:prefLabel>
    <skos:prefLabel xml:lang="da">Reggaeton</skos:prefLabel>
    <skos:prefLabel xml:lang="nl">Reggaetón</skos:prefLabel>
    <skos:prefLabel xml:lang="et">Reggaeton</skos:prefLabel>
    <skos:prefLabel xml:lang="fi">Reggaeton</skos:prefLabel>
    <skos:prefLabel xml:lang="fr">Reggaetón</skos:prefLabel>
    <skos:prefLabel xml:lang="de">Reggaeton</skos:prefLabel>
    <skos:prefLabel xml:lang="el">Ρεγκετόν</skos:prefLabel>
    <skos:prefLabel xml:lang="hu">Reggaetón</skos:prefLabel>
    <skos:prefLabel xml:lang="it">Reggaeton</skos:prefLabel>
    <skos:prefLabel xml:lang="ja">レゲトン</skos:prefLabel>
    <skos:prefLabel xml:lang="ko">레게톤</skos:prefLabel>
    <skos:prefLabel xml:lang="no">Reggaeton</skos:prefLabel>
    <skos:prefLabel xml:lang="pl">Reggaeton</skos:prefLabel>
    <skos:prefLabel xml:lang="pt">Reggaeton</skos:prefLabel>
    <skos:prefLabel xml:lang="ro">Reggaeton</skos:prefLabel>
    <skos:prefLabel xml:lang="ru">Реггетон</skos:prefLabel>
    <skos:prefLabel xml:lang="sr">Регетон</skos:prefLabel>
    <skos:prefLabel xml:lang="sk">Reggaeton</skos:prefLabel>
    <skos:prefLabel xml:lang="es">Reguetón</skos:prefLabel>
    <skos:prefLabel xml:lang="sv">Reggaeton</skos:prefLabel>
    <skos:prefLabel xml:lang="th">เรกเกตัน</skos:prefLabel>
    <skos:prefLabel xml:lang="tr">Reggaeton</skos:prefLabel>
    <skos:prefLabel xml:lang="uk">Реггетон</skos:prefLabel>
    <skos:closeMatch rdf:resource="http://rdf.freebase.com/ns/m.0233qs"/>
    <skos:broader rdf:resource="http://data.europeana.eu/concept/music/genre/Hip_hop_music_fusions"/>
    <skos:definition xml:lang="en">Reggaeton is a music genre which has its roots in Latin and
      Caribbean music. Its sound derives from the Reggae en Español from Panama. The genre was
      invented, shaped and made known in Puerto Rico where it got its name, most of its current
      artists are also from Puerto Rico. After its mainstream exposure in 2004, it spread to North
      American, European, Asian and African audiences. &lt;p&gt; Reggaeton blends musical influences
      of Jamaican dancehall and Trinidadian soca with those of Latin America, such as salsa, bomba,
      Latin American hip hop, and electronica. Vocals include rapping and singing, typically in
      Spanish. Lyrics tend to be derived from hip hop. &lt;p&gt; While it takes influences from hip
      hop and Jamaican dancehall, reggaeton is not precisely the Hispanic or Latin American version
      of either of these genres, reggaeton has its own specific beat and rhythm, whereas Latin hip
      hop is simply hip hop recorded by artists of Latino descent. The specific &quot;riddim&quot;
      that characterizes reggaeton is referred to as &quot;Dem Bow&quot;. The name &quot;Dem
      Bow&quot; is taken from the dancehall song by Shabba Ranks that first popularized the beat in
      the early 1990s, and appears on his album Just Reality.</skos:definition>
    <skos:exactMatch xml:lang="en">http://dbpedia.org/resource/Reggaeton</skos:exactMatch>
    <skos:inScheme rdf:resource="http://data.europeana.eu/concept/music/genre/Music_Genre_Scheme"/>
    <skos:altLabel xml:lang="en">Reggaeton</skos:altLabel>
  </skos:Concept>

  <skos:Concept rdf:about="http://data.europeana.eu/concept/music/genre/Rhythm_and_blues">
    <skos:prefLabel xml:lang="en">Rhythm and blues</skos:prefLabel>
    <skos:prefLabel xml:lang="ar">ريذم أند بلوز</skos:prefLabel>
    <skos:prefLabel xml:lang="bg">Ритъм енд блус</skos:prefLabel>
    <skos:prefLabel xml:lang="ca">Rhythm and blues</skos:prefLabel>
    <skos:prefLabel xml:lang="hr">Ritam i blues</skos:prefLabel>
    <skos:prefLabel xml:lang="cs">Rhythm and blues</skos:prefLabel>
    <skos:prefLabel xml:lang="da">Rhythm and blues</skos:prefLabel>
    <skos:prefLabel xml:lang="nl">Rhythm-and-blues</skos:prefLabel>
    <skos:prefLabel xml:lang="et">Rütm ja bluus</skos:prefLabel>
    <skos:prefLabel xml:lang="fil">Rhythm and blues</skos:prefLabel>
    <skos:prefLabel xml:lang="fi">Rhythm and blues</skos:prefLabel>
    <skos:prefLabel xml:lang="fr">Rhythm and blues</skos:prefLabel>
    <skos:prefLabel xml:lang="de">Rhythm and Blues</skos:prefLabel>
    <skos:prefLabel xml:lang="el">Rhythm and blues</skos:prefLabel>
    <skos:prefLabel xml:lang="hi">रिद्म एंड ब्लूज़</skos:prefLabel>
    <skos:prefLabel xml:lang="hu">Rhythm and blues</skos:prefLabel>
    <skos:prefLabel xml:lang="id">R&amp;B</skos:prefLabel>
    <skos:prefLabel xml:lang="it">Rhythm and blues</skos:prefLabel>
    <skos:prefLabel xml:lang="ja">リズム・アンド・ブルース</skos:prefLabel>
    <skos:prefLabel xml:lang="ko">리듬 앤 블루스</skos:prefLabel>
    <skos:prefLabel xml:lang="lv">R&amp;B</skos:prefLabel>
    <skos:prefLabel xml:lang="lt">Ritmenbliuzas</skos:prefLabel>
    <skos:prefLabel xml:lang="ms">Rhythm and blues</skos:prefLabel>
    <skos:prefLabel xml:lang="no">Rhythm and blues</skos:prefLabel>
    <skos:prefLabel xml:lang="fa">ریتم اند بلوز</skos:prefLabel>
    <skos:prefLabel xml:lang="pl">Rhythm and blues</skos:prefLabel>
    <skos:prefLabel xml:lang="pt">Rhythm and blues</skos:prefLabel>
    <skos:prefLabel xml:lang="ro">Muzică rhythm and blues</skos:prefLabel>
    <skos:prefLabel xml:lang="ru">Ритм-н-блюз</skos:prefLabel>
    <skos:prefLabel xml:lang="sr">Ritam i bluz</skos:prefLabel>
    <skos:prefLabel xml:lang="sk">Rhythm and blues</skos:prefLabel>
    <skos:prefLabel xml:lang="sl">Ritem in blues</skos:prefLabel>
    <skos:prefLabel xml:lang="es">Rhythm and blues</skos:prefLabel>
    <skos:prefLabel xml:lang="sv">Rhythm and blues</skos:prefLabel>
    <skos:prefLabel xml:lang="th">อาร์แอนด์บี</skos:prefLabel>
    <skos:prefLabel xml:lang="tr">Rhythm and Blues</skos:prefLabel>
    <skos:prefLabel xml:lang="uk">Ритм-енд-блюз</skos:prefLabel>
    <skos:prefLabel xml:lang="vi">Rhythm and blues</skos:prefLabel>
    <skos:closeMatch rdf:resource="http://rdf.freebase.com/ns/m.06j6l"/>
    <skos:broader rdf:resource="http://data.europeana.eu/concept/music/genre/Popular_music"/>
    <skos:definition xml:lang="en">Rhythm and blues, often abbreviated to R&amp;B or RnB, is a genre
      of popular African-American music that originated in the 1940s. The term was originally used
      by record companies to describe recordings marketed predominantly to urban African Americans,
      at a time when &quot;urbane, rocking, jazz based music with a heavy, insistent beat&quot; was
      becoming more popular. &lt;p&gt; The term rhythm and blues has undergone a number of shifts in
      meaning, for example, in the early 1950s it was frequently applied to blues records. Starting
      in the mid-1950s, after this style of music contributed to the development of rock and roll,
      the term &quot;R&amp;B&quot; became used to refer to music styles that developed from and
      incorporated electric blues, as well as gospel and soul music. By the 1970s, rhythm and blues
      was used as a blanket term for soul and funk. In the 1980s, a newer style of R&amp;B
      developed, becoming known as &quot;Contemporary R&amp;B&quot;.</skos:definition>
    <skos:exactMatch xml:lang="en">http://dbpedia.org/resource/Rhythm_and_blues</skos:exactMatch>
    <skos:inScheme rdf:resource="http://data.europeana.eu/concept/music/genre/Music_Genre_Scheme"/>
    <skos:altLabel xml:lang="en">R&amp;B</skos:altLabel>
    <skos:altLabel xml:lang="en">RnB</skos:altLabel>
    <skos:altLabel xml:lang="en">Rhythm and blues</skos:altLabel>
  </skos:Concept>

  <skos:Concept rdf:about="http://data.europeana.eu/concept/music/genre/Rockabilly">
    <skos:prefLabel xml:lang="en">Rockabilly</skos:prefLabel>
    <skos:prefLabel xml:lang="bg">Рокабили</skos:prefLabel>
    <skos:prefLabel xml:lang="ca">Rockabilly</skos:prefLabel>
    <skos:prefLabel xml:lang="hr">Rockabilly</skos:prefLabel>
    <skos:prefLabel xml:lang="cs">Rockabilly</skos:prefLabel>
    <skos:prefLabel xml:lang="da">Rockabilly</skos:prefLabel>
    <skos:prefLabel xml:lang="nl">Rockabilly</skos:prefLabel>
    <skos:prefLabel xml:lang="et">Rockabilly</skos:prefLabel>
    <skos:prefLabel xml:lang="fi">Rockabilly</skos:prefLabel>
    <skos:prefLabel xml:lang="fr">Rockabilly</skos:prefLabel>
    <skos:prefLabel xml:lang="de">Rockabilly</skos:prefLabel>
    <skos:prefLabel xml:lang="el">Rockabilly</skos:prefLabel>
    <skos:prefLabel xml:lang="hu">Rockabilly</skos:prefLabel>
    <skos:prefLabel xml:lang="id">Rockabilly</skos:prefLabel>
    <skos:prefLabel xml:lang="it">Rockabilly</skos:prefLabel>
    <skos:prefLabel xml:lang="ja">ロカビリー</skos:prefLabel>
    <skos:prefLabel xml:lang="ko">로커빌리</skos:prefLabel>
    <skos:prefLabel xml:lang="lv">Rockabilly</skos:prefLabel>
    <skos:prefLabel xml:lang="no">Rockabilly</skos:prefLabel>
    <skos:prefLabel xml:lang="pl">Rockabilly</skos:prefLabel>
    <skos:prefLabel xml:lang="pt">Rockabilly</skos:prefLabel>
    <skos:prefLabel xml:lang="ro">Rockabilly</skos:prefLabel>
    <skos:prefLabel xml:lang="ru">Рокабилли</skos:prefLabel>
    <skos:prefLabel xml:lang="sk">Rockabilly</skos:prefLabel>
    <skos:prefLabel xml:lang="sl">Rockabilly</skos:prefLabel>
    <skos:prefLabel xml:lang="es">Rockabilly</skos:prefLabel>
    <skos:prefLabel xml:lang="sv">Rockabilly</skos:prefLabel>
    <skos:prefLabel xml:lang="th">ร็อกอะบิลลี</skos:prefLabel>
    <skos:prefLabel xml:lang="tr">Rockabilly</skos:prefLabel>
    <skos:prefLabel xml:lang="uk">Рокабілі</skos:prefLabel>
    <skos:closeMatch rdf:resource="http://rdf.freebase.com/ns/m.017371"/>
    <skos:broader rdf:resource="http://data.europeana.eu/concept/music/genre/Country_music_fusions"/>
    <skos:definition xml:lang="en">Rockabilly is one of the earliest styles of rock and roll music,
      dating to the early 1950s in the United States, especially the South. As a genre it blends the
      sound of American folk and Western musical styles, such as country and bluegrass, with that of
      rhythm and blues, leading to what is considered &quot;classic&quot; rock and roll. Some have
      also described it as a blend of the bluegrass style with rock and roll. The term
      &quot;rockabilly&quot; itself is a portmanteau of &quot;rock&quot; and &quot;hillbilly&quot;,
      the latter a reference to the country music that contributed strongly to the style's
      development. Other important influences on rockabilly include western swing and boogie woogie.
      &lt;p&gt; Defining features of the rockabilly sound included strong rhythms, vocal twangs and
      common use of the tape echo, but the progressive addition of different instruments and vocal
      harmonies led to its &quot;dilution&quot;. Initially popularised by artists such as Bill
      Haley, Elvis Presley, Carl Perkins and Jerry Lee Lewis, the influence and success of the style
      waned in the 1960s, nonetheless, during the late 1970s and early 1980s, rockabilly enjoyed a
      major revival through acts such as the Stray Cats.</skos:definition>
    <skos:exactMatch xml:lang="en">http://dbpedia.org/resource/Rockabilly</skos:exactMatch>
    <skos:inScheme rdf:resource="http://data.europeana.eu/concept/music/genre/Music_Genre_Scheme"/>
    <skos:altLabel xml:lang="en">Rockabilly</skos:altLabel>
  </skos:Concept>

  <skos:Concept rdf:about="http://data.europeana.eu/concept/music/genre/Rumba">
    <skos:prefLabel xml:lang="en">Rumba</skos:prefLabel>
    <skos:prefLabel xml:lang="fr">Rumba</skos:prefLabel>
    <skos:prefLabel xml:lang="de">Rumba</skos:prefLabel>
    <skos:prefLabel xml:lang="it">Rumba</skos:prefLabel>
    <skos:prefLabel xml:lang="ja">ルンバ</skos:prefLabel>
    <skos:prefLabel xml:lang="ru">Румба</skos:prefLabel>
    <skos:prefLabel xml:lang="es">Rumba</skos:prefLabel>
    <skos:closeMatch rdf:resource="http://rdf.freebase.com/ns/m.0160wq"/>
    <skos:broader
      rdf:resource="http://data.europeana.eu/concept/music/genre/Latin_American_music_popular"/>
    <skos:definition xml:lang="en">Rumba is a family of percussive rhythms, song and ballroom dance
      that originated in Cuba as a combination of various musical traditions. The name derives from
      the Cuban Spanish word rumbo which means &quot;party&quot; or &quot;spree&quot;. It is
      secular, with no religious connections. People of African descent in Havana and Matanzas
      originally used the word rumba as a synonym for party. Olavo Alén states that over time,
      &quot;rumba ceased to be simply another word for party and took on the meaning both of a
      defined Cuban musical genre and also of a very specific form of dance.&quot; The term spread
      in the 1930s and 1940s to the faster popular music of Cuba, where it was used as a catch-all
      term, rather like salsa today. Also, the term is used in the international Latin-American
      dance syllabus, but in reference to a slower dance based on the bolero-son. Ballroom rumba, or
      rhumba, is essentially son as opposed to the older folkloric rumba. Similarly, the African
      style of pop music called African Rumba or soukous is also son-based. &lt;p&gt; The term is
      also used today for various styles of popular music from Spain, as part of the so-called
      Cantes de ida y vuelta, or music that developed between both sides of the Atlantic. Flamenco
      rumba is a genre that is entirely different from Cuban rumba.</skos:definition>
    <skos:exactMatch xml:lang="en">http://dbpedia.org/resource/Rumba</skos:exactMatch>
    <skos:inScheme rdf:resource="http://data.europeana.eu/concept/music/genre/Music_Genre_Scheme"/>
    <skos:altLabel xml:lang="en">Rumba</skos:altLabel>
  </skos:Concept>

  <skos:Concept rdf:about="http://data.europeana.eu/concept/music/genre/Samba">
    <skos:prefLabel xml:lang="en">Samba</skos:prefLabel>
    <skos:prefLabel xml:lang="ar">سامبا</skos:prefLabel>
    <skos:prefLabel xml:lang="bg">Самба</skos:prefLabel>
    <skos:prefLabel xml:lang="ca">Samba</skos:prefLabel>
    <skos:prefLabel xml:lang="hr">Samba</skos:prefLabel>
    <skos:prefLabel xml:lang="nl">Samba</skos:prefLabel>
    <skos:prefLabel xml:lang="et">Samba</skos:prefLabel>
    <skos:prefLabel xml:lang="fi">Samba</skos:prefLabel>
    <skos:prefLabel xml:lang="fr">Samba</skos:prefLabel>
    <skos:prefLabel xml:lang="de">Samba</skos:prefLabel>
    <skos:prefLabel xml:lang="hu">Szamba</skos:prefLabel>
    <skos:prefLabel xml:lang="id">Samba</skos:prefLabel>
    <skos:prefLabel xml:lang="it">Samba</skos:prefLabel>
    <skos:prefLabel xml:lang="ja">サンバ</skos:prefLabel>
    <skos:prefLabel xml:lang="ko">삼바</skos:prefLabel>
    <skos:prefLabel xml:lang="lv">Samba</skos:prefLabel>
    <skos:prefLabel xml:lang="lt">Samba</skos:prefLabel>
    <skos:prefLabel xml:lang="ms">Samba</skos:prefLabel>
    <skos:prefLabel xml:lang="no">Samba</skos:prefLabel>
    <skos:prefLabel xml:lang="fa">سامبا</skos:prefLabel>
    <skos:prefLabel xml:lang="pl">Samba de Roda</skos:prefLabel>
    <skos:prefLabel xml:lang="pt">Samba</skos:prefLabel>
    <skos:prefLabel xml:lang="ro">Samba</skos:prefLabel>
    <skos:prefLabel xml:lang="ru">Самба</skos:prefLabel>
    <skos:prefLabel xml:lang="sr">Самба</skos:prefLabel>
    <skos:prefLabel xml:lang="sl">Samba</skos:prefLabel>
    <skos:prefLabel xml:lang="es">Samba</skos:prefLabel>
    <skos:prefLabel xml:lang="sv">Samba</skos:prefLabel>
    <skos:prefLabel xml:lang="th">แซมบา</skos:prefLabel>
    <skos:prefLabel xml:lang="tr">Samba</skos:prefLabel>
    <skos:prefLabel xml:lang="uk">Самба</skos:prefLabel>
    <skos:prefLabel xml:lang="vi">Samba</skos:prefLabel>
    <skos:closeMatch rdf:resource="http://rdf.freebase.com/ns/m.06__c"/>
    <skos:broader
      rdf:resource="http://data.europeana.eu/concept/music/genre/Latin_American_music_popular"/>
    <skos:definition xml:lang="en">Samba is a Brazilian dance and musical genre originating in
      Bahia, Brazil, and with its roots Africa via the West African slave trade and African
      religious traditions, particularly Angola and the Congo. &lt;p&gt; It is recognized around the
      world as a symbol of Brazil and the Brazilian Carnival. Considered one of the most popular
      Brazilian cultural expressions, samba has become an icon of Brazilian national identity. The
      Bahian Samba de Roda, which became a UNESCO Heritage of Humanity in 2005, is the main root of
      the samba carioca, the samba that is played and danced in Rio de Janeiro. &lt;p&gt; The modern
      samba that emerged at the beginning of the 20th century is predominantly in a 2/4 tempo varied
      with the conscious use of a sung chorus to a batucada rhythm, with various stanzas of
      declaratory verses. Traditionally, the samba is played by strings and various percussion
      instruments such as tamborim. Influenced by American orchestras in vogue since the Second
      World War and the cultural impact of US music post-war, samba began to use trombones,
      trumpets, choros, flutes, and clarinets.</skos:definition>
    <skos:exactMatch xml:lang="en">http://dbpedia.org/resource/Samba</skos:exactMatch>
    <skos:inScheme rdf:resource="http://data.europeana.eu/concept/music/genre/Music_Genre_Scheme"/>
    <skos:altLabel xml:lang="en">Samba</skos:altLabel>
  </skos:Concept>

  <skos:Concept rdf:about="http://data.europeana.eu/concept/music/genre/Sevdalinka">
    <skos:prefLabel xml:lang="en">Sevdalinka</skos:prefLabel>
    <skos:prefLabel xml:lang="hr">Sevdalinka</skos:prefLabel>
    <skos:prefLabel xml:lang="cs">Sevdalinka</skos:prefLabel>
    <skos:prefLabel xml:lang="nl">Sevdah</skos:prefLabel>
    <skos:prefLabel xml:lang="fi">Sevdalinka</skos:prefLabel>
    <skos:prefLabel xml:lang="fr">Sevdalinka</skos:prefLabel>
    <skos:prefLabel xml:lang="de">Sevdalinka</skos:prefLabel>
    <skos:prefLabel xml:lang="el">Σεβνταλίνκα</skos:prefLabel>
    <skos:prefLabel xml:lang="pl">Sevdalinka</skos:prefLabel>
    <skos:prefLabel xml:lang="sr">Севдалинка</skos:prefLabel>
    <skos:prefLabel xml:lang="sv">Sevdah</skos:prefLabel>
    <skos:prefLabel xml:lang="tr">Sevdalinka</skos:prefLabel>
    <skos:prefLabel xml:lang="uk">Севдалінка</skos:prefLabel>
    <skos:closeMatch rdf:resource="http://rdf.freebase.com/ns/m.03svns"/>
    <skos:broader rdf:resource="http://data.europeana.eu/concept/music/genre/Folk_music_traditional"/>
    <skos:definition xml:lang="en">Sevdalinka is a traditional genre of folk music from Bosnia and
      Herzegovina. Sevdalinka is part of the Bosniak culture, but is also popular across the
      ex-Yugoslavia region, especially in Croatia, Macedonia, Montenegro and Serbia. The actual
      composers of many sevdalinkas are unknown. &lt;p&gt; In musical sense, sevdalinka is
      characterized by a slow or moderate tempo and intense, emotional melodies. Sevdalinka songs
      are very elaborate, emotionally charged and are traditionally sung with passion and fervor.
      The combination of Oriental, European and Sephardic elements make this type of music stand out
      among other types of folk music from the Balkans. Like a lot of Balkan folk music, Sevdalinka
      features very sombre, minor sounding modes, but unlike other types of Balkan folklore it more
      intensely features minor second intervals, thus hinting to oriental Makams and Phrygian mode.
      As a result, the melodies are noted for leaving a strong melancholic feeling with the
      listener. &lt;p&gt; The singer will often impose the rhythm and tempo of the song, both of
      which can vary throughout the song.</skos:definition>
    <skos:exactMatch xml:lang="en">http://dbpedia.org/resource/Sevdalinka</skos:exactMatch>
    <skos:inScheme rdf:resource="http://data.europeana.eu/concept/music/genre/Music_Genre_Scheme"/>
    <skos:altLabel xml:lang="en">Sevdalinka</skos:altLabel>
  </skos:Concept>

  <skos:Concept rdf:about="http://data.europeana.eu/concept/music/genre/Ska">
    <skos:prefLabel xml:lang="en">Ska</skos:prefLabel>
    <skos:prefLabel xml:lang="ar">سكا</skos:prefLabel>
    <skos:prefLabel xml:lang="bg">Ска</skos:prefLabel>
    <skos:prefLabel xml:lang="ca">Ska</skos:prefLabel>
    <skos:prefLabel xml:lang="hr">Ska</skos:prefLabel>
    <skos:prefLabel xml:lang="cs">Ska</skos:prefLabel>
    <skos:prefLabel xml:lang="da">Ska</skos:prefLabel>
    <skos:prefLabel xml:lang="nl">Ska</skos:prefLabel>
    <skos:prefLabel xml:lang="et">Ska</skos:prefLabel>
    <skos:prefLabel xml:lang="fi">Ska</skos:prefLabel>
    <skos:prefLabel xml:lang="fr">Ska</skos:prefLabel>
    <skos:prefLabel xml:lang="de">Ska</skos:prefLabel>
    <skos:prefLabel xml:lang="el">Σκα</skos:prefLabel>
    <skos:prefLabel xml:lang="hu">Ska</skos:prefLabel>
    <skos:prefLabel xml:lang="id">Ska</skos:prefLabel>
    <skos:prefLabel xml:lang="it">Ska</skos:prefLabel>
    <skos:prefLabel xml:lang="ja">スカ</skos:prefLabel>
    <skos:prefLabel xml:lang="ko">스카</skos:prefLabel>
    <skos:prefLabel xml:lang="lv">Ska</skos:prefLabel>
    <skos:prefLabel xml:lang="lt">Ska</skos:prefLabel>
    <skos:prefLabel xml:lang="ms">Ska</skos:prefLabel>
    <skos:prefLabel xml:lang="no">Ska</skos:prefLabel>
    <skos:prefLabel xml:lang="pl">Ska</skos:prefLabel>
    <skos:prefLabel xml:lang="pt">Ska</skos:prefLabel>
    <skos:prefLabel xml:lang="ru">Ска</skos:prefLabel>
    <skos:prefLabel xml:lang="sr">Ска</skos:prefLabel>
    <skos:prefLabel xml:lang="sk">Ska</skos:prefLabel>
    <skos:prefLabel xml:lang="sl">Ska</skos:prefLabel>
    <skos:prefLabel xml:lang="es">Ska</skos:prefLabel>
    <skos:prefLabel xml:lang="sv">Ska</skos:prefLabel>
    <skos:prefLabel xml:lang="th">สกา</skos:prefLabel>
    <skos:prefLabel xml:lang="tr">Ska</skos:prefLabel>
    <skos:prefLabel xml:lang="uk">Ска</skos:prefLabel>
    <skos:closeMatch rdf:resource="http://rdf.freebase.com/ns/m.06rqw"/>
    <skos:broader rdf:resource="http://data.europeana.eu/concept/music/genre/Popular_music"/>
    <skos:definition xml:lang="en">Ska is a music genre that originated in Jamaica in the late
      1950s, and was the precursor to rocksteady and reggae. Ska combined elements of Caribbean
      mento and calypso with American jazz and rhythm and blues. It is characterized by a walking
      bass line accented with rhythms on the upbeat. In the early 1960s, ska was the dominant music
      genre of Jamaica and was popular with British mods. Later it became popular with many
      skinheads. &lt;p&gt; Music historians typically divide the history of ska into three periods:
      the original Jamaican scene of the 1960s, the English 2 Tone ska revival of the late 1970s,
      and the third wave ska movement, which started in the 1980s and rose to popularity in the US
      in the 1990s.</skos:definition>
    <skos:exactMatch xml:lang="en">http://dbpedia.org/resource/Ska</skos:exactMatch>
    <skos:inScheme rdf:resource="http://data.europeana.eu/concept/music/genre/Music_Genre_Scheme"/>
    <skos:altLabel xml:lang="en">Ska</skos:altLabel>
  </skos:Concept>

  <skos:Concept rdf:about="http://data.europeana.eu/concept/music/genre/Son">
    <skos:prefLabel xml:lang="en">Son</skos:prefLabel>
    <skos:prefLabel xml:lang="ca">Son</skos:prefLabel>
    <skos:prefLabel xml:lang="cs">Son</skos:prefLabel>
    <skos:prefLabel xml:lang="nl">Son</skos:prefLabel>
    <skos:prefLabel xml:lang="fi">Son</skos:prefLabel>
    <skos:prefLabel xml:lang="fr">Son cubain</skos:prefLabel>
    <skos:prefLabel xml:lang="de">Son Cubano</skos:prefLabel>
    <skos:prefLabel xml:lang="it">Son cubano</skos:prefLabel>
    <skos:prefLabel xml:lang="ja">ソン</skos:prefLabel>
    <skos:prefLabel xml:lang="pl">Son</skos:prefLabel>
    <skos:prefLabel xml:lang="ru">Сон</skos:prefLabel>
    <skos:prefLabel xml:lang="es">Son cubano</skos:prefLabel>
    <skos:prefLabel xml:lang="sv">Son</skos:prefLabel>
    <skos:prefLabel xml:lang="tr">Son</skos:prefLabel>
    <skos:closeMatch rdf:resource="http://rdf.freebase.com/ns/m.03t8hl"/>
    <skos:broader
      rdf:resource="http://data.europeana.eu/concept/music/genre/Latin_American_music_fusions"/>
    <skos:definition xml:lang="en">Son cubano is a style of music and dance that originated in Cuba
      and gained worldwide popularity in the 1930s. Son combines the structure and elements of
      Spanish canción and the Spanish guitar with African rhythms and percussion instruments of
      Bantu origin. The Cuban son is one of the most influential and widespread forms of Latin
      American music: its derivatives and fusions, especially salsa, have spread across the world.
      &lt;p&gt; The word son has also come to be used for other traditional rural musical styles of
      Spanish-speaking countries. For example, in Mexico the Son Jarocho of Veracruz and the Son
      Huasteco of the Sierra Huasteca constitute distinct popular musical genre. They are not
      derived from the Cuban son.</skos:definition>
    <skos:exactMatch xml:lang="en">http://dbpedia.org/resource/Son</skos:exactMatch>
    <skos:inScheme rdf:resource="http://data.europeana.eu/concept/music/genre/Music_Genre_Scheme"/>
    <skos:altLabel xml:lang="en">Son</skos:altLabel>
  </skos:Concept>

  <skos:Concept rdf:about="http://data.europeana.eu/concept/music/genre/Soul">
    <skos:prefLabel xml:lang="en">Soul</skos:prefLabel>
    <skos:prefLabel xml:lang="ar">السول</skos:prefLabel>
    <skos:prefLabel xml:lang="bg">Соул</skos:prefLabel>
    <skos:prefLabel xml:lang="ca">Soul</skos:prefLabel>
    <skos:prefLabel xml:lang="hr">Soul</skos:prefLabel>
    <skos:prefLabel xml:lang="cs">Soul (hudba)</skos:prefLabel>
    <skos:prefLabel xml:lang="da">Soul</skos:prefLabel>
    <skos:prefLabel xml:lang="nl">Soul</skos:prefLabel>
    <skos:prefLabel xml:lang="fil">Musikang Soul</skos:prefLabel>
    <skos:prefLabel xml:lang="fi">Soul (musiikki)</skos:prefLabel>
    <skos:prefLabel xml:lang="fr">Musique soul</skos:prefLabel>
    <skos:prefLabel xml:lang="de">Soul</skos:prefLabel>
    <skos:prefLabel xml:lang="el">Σόουλ</skos:prefLabel>
    <skos:prefLabel xml:lang="hu">Soul</skos:prefLabel>
    <skos:prefLabel xml:lang="id">Musik soul</skos:prefLabel>
    <skos:prefLabel xml:lang="it">Soul</skos:prefLabel>
    <skos:prefLabel xml:lang="ja">ソウルミュージック</skos:prefLabel>
    <skos:prefLabel xml:lang="ko">솔 음악</skos:prefLabel>
    <skos:prefLabel xml:lang="lv">Soulmūzika</skos:prefLabel>
    <skos:prefLabel xml:lang="lt">Soul muzika</skos:prefLabel>
    <skos:prefLabel xml:lang="no">Soulmusikk</skos:prefLabel>
    <skos:prefLabel xml:lang="fa">موسیقی سول</skos:prefLabel>
    <skos:prefLabel xml:lang="pl">Soul</skos:prefLabel>
    <skos:prefLabel xml:lang="pt">Soul</skos:prefLabel>
    <skos:prefLabel xml:lang="ro">Muzică soul</skos:prefLabel>
    <skos:prefLabel xml:lang="ru">Соул</skos:prefLabel>
    <skos:prefLabel xml:lang="sr">Соул</skos:prefLabel>
    <skos:prefLabel xml:lang="sk">Soul (hudba)</skos:prefLabel>
    <skos:prefLabel xml:lang="sl">Soul</skos:prefLabel>
    <skos:prefLabel xml:lang="es">Soul</skos:prefLabel>
    <skos:prefLabel xml:lang="sv">Soul</skos:prefLabel>
    <skos:prefLabel xml:lang="th">โซล</skos:prefLabel>
    <skos:prefLabel xml:lang="tr">Soul</skos:prefLabel>
    <skos:prefLabel xml:lang="uk">Соул</skos:prefLabel>
    <skos:prefLabel xml:lang="vi">Soul</skos:prefLabel>
    <skos:closeMatch rdf:resource="http://rdf.freebase.com/ns/m.0gywn"/>
    <skos:broader rdf:resource="http://data.europeana.eu/concept/music/genre/Americana_popular"/>
    <skos:definition xml:lang="en">Soul music is a popular music genre that originated in the United
      States in the 1950s and early 1960s. It combined elements of African-American gospel music,
      rhythm and blues, and often jazz. Soul music became popular for dancing and listening in the
      United States – where music such as that of the Motown, Atlantic and Stax labels was
      influential during the period of the civil rights movement – and across the world, directly
      influencing rock music and the music of Africa. &lt;p&gt; According to the Rock and Roll Hall
      of Fame, soul is &quot;music that arose out of the black experience in America through the
      transmutation of gospel and rhythm &amp; blues into a form of funky, secular testifying&quot;.
      Catchy rhythms, stressed by handclaps and extemporaneous body moves, are an important feature
      of soul music. Other characteristics are a call and response between the soloist and the
      chorus, and an especially tense vocal sound. The style also occasionally uses improvisational
      additions, twirls and auxiliary sounds.</skos:definition>
    <skos:exactMatch xml:lang="en">http://dbpedia.org/resource/Soul</skos:exactMatch>
    <skos:inScheme rdf:resource="http://data.europeana.eu/concept/music/genre/Music_Genre_Scheme"/>
    <skos:altLabel xml:lang="en">Soul music</skos:altLabel>
  </skos:Concept>

  <skos:Concept rdf:about="http://data.europeana.eu/concept/music/genre/Swing_music">
    <skos:prefLabel xml:lang="en">Swing</skos:prefLabel>
    <skos:prefLabel xml:lang="ar">سوينغ</skos:prefLabel>
    <skos:prefLabel xml:lang="bg">Суинг</skos:prefLabel>
    <skos:prefLabel xml:lang="ca">Swing</skos:prefLabel>
    <skos:prefLabel xml:lang="hr">Swing</skos:prefLabel>
    <skos:prefLabel xml:lang="cs">Swing</skos:prefLabel>
    <skos:prefLabel xml:lang="da">Swing</skos:prefLabel>
    <skos:prefLabel xml:lang="nl">Swing</skos:prefLabel>
    <skos:prefLabel xml:lang="et">Sving</skos:prefLabel>
    <skos:prefLabel xml:lang="fi">Swing</skos:prefLabel>
    <skos:prefLabel xml:lang="fr">Swing</skos:prefLabel>
    <skos:prefLabel xml:lang="de">Swing</skos:prefLabel>
    <skos:prefLabel xml:lang="el">Σουίνγκ</skos:prefLabel>
    <skos:prefLabel xml:lang="hu">Szving</skos:prefLabel>
    <skos:prefLabel xml:lang="it">Swing</skos:prefLabel>
    <skos:prefLabel xml:lang="ja">スウィング・ジャズ</skos:prefLabel>
    <skos:prefLabel xml:lang="ko">스윙 음악</skos:prefLabel>
    <skos:prefLabel xml:lang="lv">Svings</skos:prefLabel>
    <skos:prefLabel xml:lang="lt">Svingas</skos:prefLabel>
    <skos:prefLabel xml:lang="no">Swing</skos:prefLabel>
    <skos:prefLabel xml:lang="fa">سوینگ</skos:prefLabel>
    <skos:prefLabel xml:lang="pl">Swing</skos:prefLabel>
    <skos:prefLabel xml:lang="pt">Swing</skos:prefLabel>
    <skos:prefLabel xml:lang="ru">Свинг</skos:prefLabel>
    <skos:prefLabel xml:lang="sk">Swing</skos:prefLabel>
    <skos:prefLabel xml:lang="sl">Swing</skos:prefLabel>
    <skos:prefLabel xml:lang="es">Swing</skos:prefLabel>
    <skos:prefLabel xml:lang="sv">Swing</skos:prefLabel>
    <skos:prefLabel xml:lang="th">ดนตรีสวิง</skos:prefLabel>
    <skos:prefLabel xml:lang="tr">Swing</skos:prefLabel>
    <skos:prefLabel xml:lang="uk">Свінг</skos:prefLabel>
    <skos:closeMatch rdf:resource="http://rdf.freebase.com/ns/m.015y_n"/>
    <skos:broader rdf:resource="http://data.europeana.eu/concept/music/genre/Popular_music"/>
    <skos:definition xml:lang="en">Swing music, or simply Swing, is a form of American music that
      developed in the early 1930s and became a distinctive style by 1940. Swing uses a strong
      rhythm section of double bass and drums as the anchor for a lead section of brass instruments
      such as trumpets and trombones, woodwinds including saxophones and clarinets, and sometimes
      stringed instruments such as violin and guitar, medium to fast tempos, and a
      &quot;lilting&quot; swing time rhythm. The name swing came from the phrase ‘swing feel’ where
      the emphasis is on the off–beat or weaker pulse in the music. Swing bands usually featured
      soloists who would improvise on the melody over the arrangement. &lt;p&gt; The danceable swing
      style of big bands and bandleaders such as Benny Goodman was the dominant form of American
      popular music from 1935 to 1946, a period known as the Swing Era. The verb &quot;to
      swing&quot; is also used as a term of praise for playing that has a strong rhythmic
      &quot;groove&quot; or drive.</skos:definition>
    <skos:exactMatch xml:lang="en">http://dbpedia.org/resource/Swing_music</skos:exactMatch>
    <skos:inScheme rdf:resource="http://data.europeana.eu/concept/music/genre/Music_Genre_Scheme"/>
    <skos:altLabel xml:lang="en">Swing music</skos:altLabel>
  </skos:Concept>

  <skos:Concept rdf:about="http://data.europeana.eu/concept/music/genre/Tango">
    <skos:prefLabel xml:lang="en">Tango</skos:prefLabel>
    <skos:prefLabel xml:lang="bg">Танго</skos:prefLabel>
    <skos:prefLabel xml:lang="cs">Argentinské tango</skos:prefLabel>
    <skos:prefLabel xml:lang="da">Tango</skos:prefLabel>
    <skos:prefLabel xml:lang="nl">Tango</skos:prefLabel>
    <skos:prefLabel xml:lang="fi">Tango</skos:prefLabel>
    <skos:prefLabel xml:lang="fr">Tango</skos:prefLabel>
    <skos:prefLabel xml:lang="de">Tango</skos:prefLabel>
    <skos:prefLabel xml:lang="hu">Tangó</skos:prefLabel>
    <skos:prefLabel xml:lang="it">Tango argentino</skos:prefLabel>
    <skos:prefLabel xml:lang="ja">タンゴ</skos:prefLabel>
    <skos:prefLabel xml:lang="ko">탱고</skos:prefLabel>
    <skos:prefLabel xml:lang="lt">Tango muzika</skos:prefLabel>
    <skos:prefLabel xml:lang="no">Tango</skos:prefLabel>
    <skos:prefLabel xml:lang="pl">Tango</skos:prefLabel>
    <skos:prefLabel xml:lang="pt">Tango</skos:prefLabel>
    <skos:prefLabel xml:lang="ru">Танго</skos:prefLabel>
    <skos:prefLabel xml:lang="sr">Танго</skos:prefLabel>
    <skos:prefLabel xml:lang="sl">Tango</skos:prefLabel>
    <skos:prefLabel xml:lang="es">Tango</skos:prefLabel>
    <skos:prefLabel xml:lang="sv">Tangomusik</skos:prefLabel>
    <skos:prefLabel xml:lang="tr">Tango</skos:prefLabel>
    <skos:prefLabel xml:lang="vi">Tango</skos:prefLabel>
    <skos:closeMatch rdf:resource="http://rdf.freebase.com/ns/m.0210vc"/>
    <skos:broader
      rdf:resource="http://data.europeana.eu/concept/music/genre/Latin_American_music_popular"/>
    <skos:definition xml:lang="en">Tango is a style of music in 2/4 or 4/4 time that originated
      among European immigrant populations of Argentina and Uruguay. It is traditionally played on a
      solo guitar, guitar duo, or an ensemble, known as the orquesta típica, which includes at least
      two violins, flute, piano, double bass, and at least two bandoneóns. Sometimes guitars and a
      clarinet join the ensemble. Tango may be purely instrumental or may include a vocalist. Tango
      music and dance have become popular throughout the world.</skos:definition>
    <skos:exactMatch xml:lang="en">http://dbpedia.org/resource/Tango</skos:exactMatch>
    <skos:inScheme rdf:resource="http://data.europeana.eu/concept/music/genre/Music_Genre_Scheme"/>
    <skos:altLabel xml:lang="en">Tango music</skos:altLabel>
  </skos:Concept>

  <skos:Concept rdf:about="http://data.europeana.eu/concept/music/genre/Tarantella">
    <skos:prefLabel xml:lang="en">Tarantella</skos:prefLabel>
    <skos:prefLabel xml:lang="it">Tarantella calabrese</skos:prefLabel>
    <skos:prefLabel xml:lang="es">Tarantella calabresa</skos:prefLabel>
    <skos:closeMatch rdf:resource="http://rdf.freebase.com/ns/m.0nb77pz"/>
    <skos:broader rdf:resource="http://data.europeana.eu/concept/music/genre/Religious_music"/>
    <skos:definition xml:lang="en">Calabrian Tarantella is a generic term to include different
      musical-dancing expressions spread in Calabria peninsula and different from other southern
      Italian dances called simply Tarantella. It is played and danced during religious festivals
      and other social occasions. In recent times the tradition has been revived as new groups are
      taking an interest in instruments which had been falling into obscurity, they played &quot;ad
      usu anticu&quot; or they modernised the sound adding a Bass line or new
      sounds.</skos:definition>
    <skos:exactMatch xml:lang="en">http://dbpedia.org/resource/Tarantella</skos:exactMatch>
    <skos:inScheme rdf:resource="http://data.europeana.eu/concept/music/genre/Music_Genre_Scheme"/>
    <skos:altLabel xml:lang="en">Calabrian Tarantella</skos:altLabel>
  </skos:Concept>

  <skos:Concept rdf:about="http://data.europeana.eu/concept/music/genre/Techno">
    <skos:prefLabel xml:lang="en">Techno</skos:prefLabel>
    <skos:prefLabel xml:lang="bg">Техно</skos:prefLabel>
    <skos:prefLabel xml:lang="ca">Techno</skos:prefLabel>
    <skos:prefLabel xml:lang="hr">Techno</skos:prefLabel>
    <skos:prefLabel xml:lang="cs">Techno</skos:prefLabel>
    <skos:prefLabel xml:lang="da">Techno</skos:prefLabel>
    <skos:prefLabel xml:lang="nl">Techno</skos:prefLabel>
    <skos:prefLabel xml:lang="et">Tekno</skos:prefLabel>
    <skos:prefLabel xml:lang="fi">Tekno</skos:prefLabel>
    <skos:prefLabel xml:lang="fr">Techno</skos:prefLabel>
    <skos:prefLabel xml:lang="de">Techno</skos:prefLabel>
    <skos:prefLabel xml:lang="hu">Techno</skos:prefLabel>
    <skos:prefLabel xml:lang="it">Techno</skos:prefLabel>
    <skos:prefLabel xml:lang="ja">テクノ</skos:prefLabel>
    <skos:prefLabel xml:lang="ko">테크노</skos:prefLabel>
    <skos:prefLabel xml:lang="lv">Tehno</skos:prefLabel>
    <skos:prefLabel xml:lang="lt">Techno</skos:prefLabel>
    <skos:prefLabel xml:lang="no">Techno</skos:prefLabel>
    <skos:prefLabel xml:lang="fa">تکنو</skos:prefLabel>
    <skos:prefLabel xml:lang="pl">Techno</skos:prefLabel>
    <skos:prefLabel xml:lang="pt">Techno</skos:prefLabel>
    <skos:prefLabel xml:lang="ro">Techno</skos:prefLabel>
    <skos:prefLabel xml:lang="ru">Техно</skos:prefLabel>
    <skos:prefLabel xml:lang="sr">Tehno</skos:prefLabel>
    <skos:prefLabel xml:lang="sk">Techno</skos:prefLabel>
    <skos:prefLabel xml:lang="sl">Techno</skos:prefLabel>
    <skos:prefLabel xml:lang="es">Techno</skos:prefLabel>
    <skos:prefLabel xml:lang="sv">Techno</skos:prefLabel>
    <skos:prefLabel xml:lang="th">เทคโน</skos:prefLabel>
    <skos:prefLabel xml:lang="tr">Tekno müzik</skos:prefLabel>
    <skos:prefLabel xml:lang="uk">Техно</skos:prefLabel>
    <skos:prefLabel xml:lang="vi">Techno</skos:prefLabel>
    <skos:closeMatch rdf:resource="http://rdf.freebase.com/ns/m.07gxw"/>
    <skos:broader
      rdf:resource="http://data.europeana.eu/concept/music/genre/Electronic_music_fusions"/>
    <skos:definition xml:lang="en">Techno is a form of electronic dance music that emerged in
      Detroit, Michigan, in the United States during the mid-to-late 1980s. The first recorded use
      of the word techno in reference to a specific genre of music was in 1988. Many styles of
      techno now exist, but Detroit techno is seen as the foundation upon which a number of
      subgenres have been built. &lt;p&gt; The initial take on techno arose from the melding of
      electronic music, in the style of artists such as Kraftwerk, Giorgio Moroder and Yellow Magic
      Orchestra, with African American music styles, including funk, electro, Chicago house and
      electric jazz. Added to this is the influence of futuristic and fictional themes relevant to
      life in American late capitalist society, with Alvin Toffler's book The Third Wave being a
      notable point of reference. Pioneering producer Juan Atkins cites Toffler's phrase
      &quot;techno rebels&quot; as inspiring him to use the word techno to describe the musical
      style he helped to create. This unique blend of influences aligns techno with the aesthetic
      referred to as afrofuturism.</skos:definition>
    <skos:exactMatch xml:lang="en">http://dbpedia.org/resource/Techno</skos:exactMatch>
    <skos:inScheme rdf:resource="http://data.europeana.eu/concept/music/genre/Music_Genre_Scheme"/>
    <skos:altLabel xml:lang="en">Techno music</skos:altLabel>
    <skos:altLabel xml:lang="en">Techno</skos:altLabel>
  </skos:Concept>

  <skos:Concept rdf:about="http://data.europeana.eu/concept/music/genre/Tex-Mex">
    <skos:prefLabel xml:lang="en">Tejano</skos:prefLabel>
    <skos:prefLabel xml:lang="ar">موسيقى تيخانو</skos:prefLabel>
    <skos:prefLabel xml:lang="da">Tex-mex</skos:prefLabel>
    <skos:prefLabel xml:lang="nl">Tex-Mex</skos:prefLabel>
    <skos:prefLabel xml:lang="fi">Texmex</skos:prefLabel>
    <skos:prefLabel xml:lang="fr">Musique Tex-Mex</skos:prefLabel>
    <skos:prefLabel xml:lang="de">Tex-Mex</skos:prefLabel>
    <skos:prefLabel xml:lang="it">Musica Tex-Mex</skos:prefLabel>
    <skos:prefLabel xml:lang="no">Tex-Mex-musikk</skos:prefLabel>
    <skos:prefLabel xml:lang="ru">Музыка техано</skos:prefLabel>
    <skos:prefLabel xml:lang="es">Tex-mex</skos:prefLabel>
    <skos:prefLabel xml:lang="sv">Tejanomusik</skos:prefLabel>
    <skos:closeMatch rdf:resource="http://rdf.freebase.com/ns/m.013rxq"/>
    <skos:broader rdf:resource="http://data.europeana.eu/concept/music/genre/Americana_popular"/>
    <skos:definition xml:lang="en">Tejano music or Tex-Mex music is the name given to various forms
      of folk and popular music originating among the Mexican-American populations of Central and
      Southern Texas. With roots in the late 19th century, it became a music genre with a wider
      audience in the late 20th century thanks to artists such as Selena, often referred to as
      &quot;The Queen of Tejano&quot;, Mazz, Elida Reyna, Los Palominos, Ramón Ayala, Elsa García,
      Laura Canales, La Mafia, Jay Perez, Emilio Navaira, Alicia Villarreal, Gary Hobbs, Shelly
      Lares, Stefani Montiel, David Lee Garza and Jennifer Peña.</skos:definition>
    <skos:exactMatch xml:lang="en">http://dbpedia.org/resource/Tex-Mex</skos:exactMatch>
    <skos:inScheme rdf:resource="http://data.europeana.eu/concept/music/genre/Music_Genre_Scheme"/>
    <skos:altLabel xml:lang="en">Tejano music</skos:altLabel>
  </skos:Concept>

  <skos:Concept rdf:about="http://data.europeana.eu/concept/music/genre/Timba">
    <skos:prefLabel xml:lang="en">Timba</skos:prefLabel>
    <skos:prefLabel xml:lang="nl">Timba</skos:prefLabel>
    <skos:prefLabel xml:lang="fr">Timba</skos:prefLabel>
    <skos:prefLabel xml:lang="de">Timba</skos:prefLabel>
    <skos:prefLabel xml:lang="it">Timba</skos:prefLabel>
    <skos:prefLabel xml:lang="no">Timba</skos:prefLabel>
    <skos:prefLabel xml:lang="es">Timba</skos:prefLabel>
    <skos:prefLabel xml:lang="sv">Timba</skos:prefLabel>
    <skos:closeMatch rdf:resource="http://rdf.freebase.com/ns/m.03vdxm"/>
    <skos:broader
      rdf:resource="http://data.europeana.eu/concept/music/genre/Latin_American_music_popular"/>
    <skos:definition xml:lang="en">Timba is a Cuban genre of music based on popular Cuban music
      along with salsa, American funk/R&amp;B, and the strong influence of Afro-Cuban folkloric
      music.</skos:definition>
    <skos:exactMatch xml:lang="en">http://dbpedia.org/resource/Timba</skos:exactMatch>
    <skos:inScheme rdf:resource="http://data.europeana.eu/concept/music/genre/Music_Genre_Scheme"/>
    <skos:altLabel xml:lang="en">Timba</skos:altLabel>
  </skos:Concept>

  <skos:Concept rdf:about="http://data.europeana.eu/concept/music/genre/Ambient_music">
    <skos:prefLabel xml:lang="en">Ambient</skos:prefLabel>
    <skos:prefLabel xml:lang="bg">Ембиънт</skos:prefLabel>
    <skos:prefLabel xml:lang="ca">Ambient</skos:prefLabel>
    <skos:prefLabel xml:lang="hr">Ambijentalna glazba</skos:prefLabel>
    <skos:prefLabel xml:lang="cs">Ambientní hudba</skos:prefLabel>
    <skos:prefLabel xml:lang="da">Ambient</skos:prefLabel>
    <skos:prefLabel xml:lang="nl">Ambient</skos:prefLabel>
    <skos:prefLabel xml:lang="et">Ambient</skos:prefLabel>
    <skos:prefLabel xml:lang="fi">Ambient</skos:prefLabel>
    <skos:prefLabel xml:lang="fr">Ambient</skos:prefLabel>
    <skos:prefLabel xml:lang="de">Ambient</skos:prefLabel>
    <skos:prefLabel xml:lang="el">Ambient</skos:prefLabel>
    <skos:prefLabel xml:lang="hu">Ambient</skos:prefLabel>
    <skos:prefLabel xml:lang="it">Ambient</skos:prefLabel>
    <skos:prefLabel xml:lang="ja">環境音楽</skos:prefLabel>
    <skos:prefLabel xml:lang="lv">Ambientā mūzika</skos:prefLabel>
    <skos:prefLabel xml:lang="lt">Ambientinė muzika</skos:prefLabel>
    <skos:prefLabel xml:lang="no">Ambient</skos:prefLabel>
    <skos:prefLabel xml:lang="fa">موسیقی امبینت</skos:prefLabel>
    <skos:prefLabel xml:lang="pl">Ambient</skos:prefLabel>
    <skos:prefLabel xml:lang="pt">Música ambiente</skos:prefLabel>
    <skos:prefLabel xml:lang="ro">Ambient</skos:prefLabel>
    <skos:prefLabel xml:lang="ru">Эмбиент</skos:prefLabel>
    <skos:prefLabel xml:lang="sr">Амбијентална музика</skos:prefLabel>
    <skos:prefLabel xml:lang="sk">Ambientná hudba</skos:prefLabel>
    <skos:prefLabel xml:lang="sl">Ambient</skos:prefLabel>
    <skos:prefLabel xml:lang="es">Ambient</skos:prefLabel>
    <skos:prefLabel xml:lang="sv">Ambient</skos:prefLabel>
    <skos:prefLabel xml:lang="th">ดนตรีแอมเบียนต์</skos:prefLabel>
    <skos:prefLabel xml:lang="uk">Ембієнт</skos:prefLabel>
    <skos:closeMatch rdf:resource="http://rdf.freebase.com/ns/m.0fd3y"/>
    <skos:broader rdf:resource="http://data.europeana.eu/concept/music/genre/Electronic_music"/>
    <skos:definition xml:lang="en">Ambient music includes forms of music that put an emphasis on
      tone and atmosphere over traditional musical structure or rhythm. Ambient music is said to
      evoke an &quot;atmospheric&quot;, &quot;visual&quot; or &quot;unobtrusive&quot; quality. To
      quote one pioneer, Brian Eno, &quot;Ambient Music must be able to accommodate many levels of
      listening attention without enforcing one in particular, it must be as ignorable as it is
      interesting.&quot; &lt;p&gt; As a genre it originated in the United Kingdom at a time when new
      sound-making devices such as the synthesizer, were being introduced to a wider market. Robert
      Fripp and Brian Eno popularized ambient music in 1972 while experimenting with tape loop
      techniques. The Orb and Aphex Twin gained commercial success with ambient tracks. Ambient
      compositions are often quite lengthy, much longer than more popular, commercial forms of
      music. Some pieces can reach a half an hour or more in length.</skos:definition>
    <skos:exactMatch xml:lang="en">http://dbpedia.org/resource/Ambient_music</skos:exactMatch>
    <skos:inScheme rdf:resource="http://data.europeana.eu/concept/music/genre/Music_Genre_Scheme"/>
    <skos:altLabel xml:lang="en">Ambient music</skos:altLabel>
  </skos:Concept>

  <skos:Concept rdf:about="http://data.europeana.eu/concept/music/genre/Barbershop_music">
    <skos:prefLabel xml:lang="en">Barbershop</skos:prefLabel>
    <skos:prefLabel xml:lang="ca">Barbershop</skos:prefLabel>
    <skos:prefLabel xml:lang="nl">Barbershop</skos:prefLabel>
    <skos:prefLabel xml:lang="fr">Barbershop</skos:prefLabel>
    <skos:prefLabel xml:lang="de">Barbershop</skos:prefLabel>
    <skos:prefLabel xml:lang="no">Barbershop</skos:prefLabel>
    <skos:prefLabel xml:lang="es">Barbershop</skos:prefLabel>
    <skos:prefLabel xml:lang="sv">Barbershop</skos:prefLabel>
    <skos:closeMatch rdf:resource="http://rdf.freebase.com/ns/m.02268g"/>
    <skos:broader rdf:resource="http://data.europeana.eu/concept/music/genre/Barbershop_music"/>
    <skos:definition xml:lang="en">Barbershop vocal harmony, as codified during the barbershop
      revival era, is a style of a cappella, or unaccompanied vocal music, characterized by
      consonant four-part chords for every melody note in a predominantly homophonic texture. Each
      of the four parts has its own role: generally, the lead sings the melody, the tenor harmonizes
      above the melody, the bass sings the lowest harmonizing notes, and the baritone completes the
      chord, usually below the lead. The melody is not usually sung by the tenor or baritone, except
      for an infrequent note or two to avoid awkward voice leading, in tags or codas, or when some
      appropriate embellishment can be created. Occasional passages may be sung by fewer than four
      voice parts. &lt;p&gt; According to the Barbershop Harmony Society, &quot;Barbershop music
      features songs with understandable lyrics and easily singable melodies, whose tones clearly
      define a tonal center and imply major and minor chords and barbershop seventh chords that
      resolve primarily around the circle of fifths, while making frequent use of other
      resolutions.&quot; Slower barbershop songs, especially ballads, often eschew a continuous
      beat, and notes are often held ad libitum.</skos:definition>
    <skos:exactMatch xml:lang="en">http://dbpedia.org/resource/Barbershop_music</skos:exactMatch>
    <skos:inScheme rdf:resource="http://data.europeana.eu/concept/music/genre/Music_Genre_Scheme"/>
    <skos:altLabel xml:lang="en">Barbershop music</skos:altLabel>
  </skos:Concept>

  <skos:Concept rdf:about="http://data.europeana.eu/concept/music/genre/Bluegrass_music">
    <skos:prefLabel xml:lang="en">Bluegrass</skos:prefLabel>
    <skos:prefLabel xml:lang="ca">Bluegrass</skos:prefLabel>
    <skos:prefLabel xml:lang="hr">Bluegrass</skos:prefLabel>
    <skos:prefLabel xml:lang="cs">Bluegrass</skos:prefLabel>
    <skos:prefLabel xml:lang="da">Bluegrass</skos:prefLabel>
    <skos:prefLabel xml:lang="nl">Bluegrass</skos:prefLabel>
    <skos:prefLabel xml:lang="fi">Bluegrass</skos:prefLabel>
    <skos:prefLabel xml:lang="fr">Bluegrass</skos:prefLabel>
    <skos:prefLabel xml:lang="de">Bluegrass</skos:prefLabel>
    <skos:prefLabel xml:lang="it">Bluegrass</skos:prefLabel>
    <skos:prefLabel xml:lang="ja">ブルーグラス</skos:prefLabel>
    <skos:prefLabel xml:lang="ko">블루그래스</skos:prefLabel>
    <skos:prefLabel xml:lang="no">Bluegrass</skos:prefLabel>
    <skos:prefLabel xml:lang="pl">Muzyka bluegrass</skos:prefLabel>
    <skos:prefLabel xml:lang="pt">Bluegrass</skos:prefLabel>
    <skos:prefLabel xml:lang="ru">Блюграсс</skos:prefLabel>
    <skos:prefLabel xml:lang="sl">Bluegrass</skos:prefLabel>
    <skos:prefLabel xml:lang="es">Bluegrass</skos:prefLabel>
    <skos:prefLabel xml:lang="sv">Bluegrassmusik</skos:prefLabel>
    <skos:prefLabel xml:lang="tr">Bluegrass</skos:prefLabel>
    <skos:prefLabel xml:lang="uk">Блюграс</skos:prefLabel>
    <skos:closeMatch rdf:resource="http://rdf.freebase.com/ns/m.0gg8l"/>
    <skos:broader rdf:resource="http://data.europeana.eu/concept/music/genre/Country"/>
    <skos:definition xml:lang="en">Bluegrass music is a form of American roots music, and a
      sub-genre of country music. Bluegrass was inspired by the music of Appalachia. It has mixed
      roots in Irish, Scottish, Welsh, and English traditional music, and also later influenced by
      the music of African-Americans through incorporation of jazz elements. &lt;p&gt; Settlers from
      the United Kingdom and Ireland arrived in Appalachia during the 18th century, and brought with
      them the musical traditions of their homelands. These traditions consisted primarily of
      English and Scottish ballads—which were essentially unaccompanied narrative—and dance music,
      such as Irish reels, which were accompanied by a fiddle. Many older bluegrass songs come
      directly from the British Isles. Several Appalachian bluegrass ballads, such as &quot;Pretty
      Saro&quot;, &quot;Barbara Allen&quot;, &quot;Cuckoo Bird&quot; and &quot;House
      Carpenter&quot;, come from England and preserve the English ballad tradition both melodically
      and lyrically. Others, such as The Twa Sisters, also come from England, however, the lyrics
      are about Ireland. Some bluegrass fiddle songs popular in Appalachia, such as &quot;Leather
      Britches&quot;, and &quot;Pretty Polly&quot;, have Scottish roots.</skos:definition>
    <skos:exactMatch xml:lang="en">http://dbpedia.org/resource/Bluegrass_music</skos:exactMatch>
    <skos:inScheme rdf:resource="http://data.europeana.eu/concept/music/genre/Music_Genre_Scheme"/>
    <skos:altLabel xml:lang="en">Bluegrass music</skos:altLabel>
    <skos:altLabel xml:lang="en">Bluegrass</skos:altLabel>
  </skos:Concept>

  <skos:Concept rdf:about="http://data.europeana.eu/concept/music/genre/Cajun_music">
    <skos:prefLabel xml:lang="en">Cajun</skos:prefLabel>
    <skos:prefLabel xml:lang="da">Cajun</skos:prefLabel>
    <skos:prefLabel xml:lang="nl">Cajunmuziek</skos:prefLabel>
    <skos:prefLabel xml:lang="fr">Musique cadienne</skos:prefLabel>
    <skos:prefLabel xml:lang="de">Cajun-Musik</skos:prefLabel>
    <skos:prefLabel xml:lang="it">Cajun</skos:prefLabel>
    <skos:prefLabel xml:lang="ja">ケイジャン (音楽)</skos:prefLabel>
    <skos:prefLabel xml:lang="pt">Música cajun</skos:prefLabel>
    <skos:prefLabel xml:lang="sv">Cajunmusik</skos:prefLabel>
    <skos:closeMatch rdf:resource="http://rdf.freebase.com/ns/m.01kp8z"/>
    <skos:broader>
      <skos:Concept
        rdf:about="http://data.europeana.eu/concept/music/genre/American_folk_music_traditional">
        <skos:prefLabel xml:lang="en">Traditional American Folk</skos:prefLabel>
        <skos:prefLabel xml:lang="da">Amerikansk folkemusik</skos:prefLabel>
        <skos:prefLabel xml:lang="fi">Folkmusiikki</skos:prefLabel>
        <skos:prefLabel xml:lang="de">Rootsmusik</skos:prefLabel>
        <skos:prefLabel xml:lang="ja">フォークソング</skos:prefLabel>
        <skos:prefLabel xml:lang="no">Folkemusikk i USA</skos:prefLabel>
        <skos:prefLabel xml:lang="ru">Североамериканский фолк</skos:prefLabel>
        <skos:prefLabel xml:lang="es">Música folclórica de Estados Unidos</skos:prefLabel>
        <skos:closeMatch rdf:resource="http://rdf.freebase.com/ns/m.01kny3"/>
        <skos:broader rdf:resource="http://data.europeana.eu/concept/music/genre/World_music"/>
        <skos:definition xml:lang="en">The traditional part of the American folk music originated
          from North America. This category reffers to genres which are known as traditional music,
          traditional folk music and Native American Music. This category doesn't include the
          contemporary folk music or popular roots music.</skos:definition>
        <skos:broadMatch rdf:resource="http://dbpedia.org/resource//American_folk_music#traditional"/>
        <skos:inScheme
          rdf:resource="http://data.europeana.eu/concept/music/genre/Music_Genre_Scheme"/>
        <skos:altLabel xml:lang="en">American folk music</skos:altLabel>
      </skos:Concept>
    </skos:broader>

    <skos:definition xml:lang="en">Cajun music, an emblematic music of Louisiana, is rooted in the
      ballads of the French-speaking Acadians of Canada. Cajun music is often mentioned in tandem
      with the Creole-based, Cajun-influenced zydeco form. These French Louisiana sounds have
      influenced American popular music for many decades, especially country music, and have
      influenced pop culture through mass media, such as television commercials.</skos:definition>
    <skos:exactMatch xml:lang="en">http://dbpedia.org/resource/Cajun_music</skos:exactMatch>
    <skos:inScheme rdf:resource="http://data.europeana.eu/concept/music/genre/Music_Genre_Scheme"/>
    <skos:altLabel xml:lang="en">Cajun music</skos:altLabel>
  </skos:Concept>

  <skos:Concept rdf:about="http://data.europeana.eu/concept/music/genre/Calypso_music">
    <skos:prefLabel xml:lang="en">Calypso</skos:prefLabel>
    <skos:prefLabel xml:lang="ca">Calipso</skos:prefLabel>
    <skos:prefLabel xml:lang="cs">Kalypso</skos:prefLabel>
    <skos:prefLabel xml:lang="da">Calypso</skos:prefLabel>
    <skos:prefLabel xml:lang="nl">Calypso</skos:prefLabel>
    <skos:prefLabel xml:lang="et">Kalüpso</skos:prefLabel>
    <skos:prefLabel xml:lang="fi">Calypso</skos:prefLabel>
    <skos:prefLabel xml:lang="fr">Calypso</skos:prefLabel>
    <skos:prefLabel xml:lang="de">Calypso</skos:prefLabel>
    <skos:prefLabel xml:lang="el">Καλύψο</skos:prefLabel>
    <skos:prefLabel xml:lang="hu">Calypso</skos:prefLabel>
    <skos:prefLabel xml:lang="it">Calypso</skos:prefLabel>
    <skos:prefLabel xml:lang="ja">カリプソ</skos:prefLabel>
    <skos:prefLabel xml:lang="ko">칼립소</skos:prefLabel>
    <skos:prefLabel xml:lang="no">Calypso</skos:prefLabel>
    <skos:prefLabel xml:lang="fa">کالیپسو</skos:prefLabel>
    <skos:prefLabel xml:lang="pl">Calypso</skos:prefLabel>
    <skos:prefLabel xml:lang="pt">Calipso</skos:prefLabel>
    <skos:prefLabel xml:lang="ru">Калипсо</skos:prefLabel>
    <skos:prefLabel xml:lang="es">Calipso</skos:prefLabel>
    <skos:prefLabel xml:lang="sv">Calypso</skos:prefLabel>
    <skos:closeMatch rdf:resource="http://rdf.freebase.com/ns/m.01446r"/>
    <skos:broader
      rdf:resource="http://data.europeana.eu/concept/music/genre/Latin_American_music_popular"/>
    <skos:definition xml:lang="en">Calypso is a style of Afro-Caribbean music that originated in
      Trinidad and Tobago during the early to mid 20th century. Its rhythms can be traced back to
      West African Kaiso and the arrival of French planters and their slaves from the French
      Antilles in the 1600s. &lt;p&gt; The music, which drew upon African and French influences,
      became the voice of the people, and was characterized by highly rhythmic and harmonic vocals,
      which was most often sung in a French creole and led by a griot. As calypso developed, the
      role of the griot became known as a chantuelle and eventually, calypsonian. As English
      replaced patois as the dominant language, calypso migrated into English, and in so doing it
      attracted more attention from the government. It allowed the masses to challenge the doings of
      the unelected Governor and Legislative Council, and the elected town councils of Port of Spain
      and San Fernando. Calypso continued to play an important role in political expression, and
      also served to document the history of Trinidad and Tobago.</skos:definition>
    <skos:exactMatch xml:lang="en">http://dbpedia.org/resource/Calypso_music</skos:exactMatch>
    <skos:inScheme rdf:resource="http://data.europeana.eu/concept/music/genre/Music_Genre_Scheme"/>
    <skos:altLabel xml:lang="en">Calypso music</skos:altLabel>
  </skos:Concept>

  <skos:Concept rdf:about="http://data.europeana.eu/concept/music/genre/Heavy_metal_music">
    <skos:prefLabel xml:lang="en">Heavy metal</skos:prefLabel>
    <skos:prefLabel xml:lang="ar">موسيقى الميتال</skos:prefLabel>
    <skos:prefLabel xml:lang="bg">Хеви метъл</skos:prefLabel>
    <skos:prefLabel xml:lang="ca">Heavy metal</skos:prefLabel>
    <skos:prefLabel xml:lang="hr">Heavy metal</skos:prefLabel>
    <skos:prefLabel xml:lang="cs">Heavy metal</skos:prefLabel>
    <skos:prefLabel xml:lang="da">Heavy metal</skos:prefLabel>
    <skos:prefLabel xml:lang="nl">Heavy metal</skos:prefLabel>
    <skos:prefLabel xml:lang="et">Heavy metal</skos:prefLabel>
    <skos:prefLabel xml:lang="fi">Metallimusiikki</skos:prefLabel>
    <skos:prefLabel xml:lang="fr">Heavy metal</skos:prefLabel>
    <skos:prefLabel xml:lang="de">Metal</skos:prefLabel>
    <skos:prefLabel xml:lang="el">Χέβι μέταλ μουσική</skos:prefLabel>
    <skos:prefLabel xml:lang="hu">Heavy metal</skos:prefLabel>
    <skos:prefLabel xml:lang="id">Heavy metal</skos:prefLabel>
    <skos:prefLabel xml:lang="it">Heavy metal</skos:prefLabel>
    <skos:prefLabel xml:lang="ja">ヘヴィメタル</skos:prefLabel>
    <skos:prefLabel xml:lang="ko">헤비 메탈</skos:prefLabel>
    <skos:prefLabel xml:lang="lv">Smagais metāls</skos:prefLabel>
    <skos:prefLabel xml:lang="lt">Heavy metal</skos:prefLabel>
    <skos:prefLabel xml:lang="ms">Muzik heavy metal</skos:prefLabel>
    <skos:prefLabel xml:lang="no">Heavy metal</skos:prefLabel>
    <skos:prefLabel xml:lang="fa">موسیقی هوی متال</skos:prefLabel>
    <skos:prefLabel xml:lang="pl">Heavy metal</skos:prefLabel>
    <skos:prefLabel xml:lang="pt">Heavy metal</skos:prefLabel>
    <skos:prefLabel xml:lang="ro">Heavy metal</skos:prefLabel>
    <skos:prefLabel xml:lang="ru">Хеви-метал</skos:prefLabel>
    <skos:prefLabel xml:lang="sr">Хеви метал</skos:prefLabel>
    <skos:prefLabel xml:lang="sk">Heavy metal</skos:prefLabel>
    <skos:prefLabel xml:lang="sl">Metal</skos:prefLabel>
    <skos:prefLabel xml:lang="es">Heavy metal</skos:prefLabel>
    <skos:prefLabel xml:lang="sv">Heavy metal</skos:prefLabel>
    <skos:prefLabel xml:lang="th">เฮฟวีเมทัล</skos:prefLabel>
    <skos:prefLabel xml:lang="tr">Heavy metal</skos:prefLabel>
    <skos:prefLabel xml:lang="uk">Важкий метал</skos:prefLabel>
    <skos:prefLabel xml:lang="vi">Nhạc heavy metal</skos:prefLabel>
    <skos:closeMatch rdf:resource="http://rdf.freebase.com/ns/m.03lty"/>
    <skos:broader rdf:resource="http://data.europeana.eu/concept/music/genre/Rock_music"/>
    <skos:definition xml:lang="en">Heavy metal is a genre of rock music that developed in the late
      1960s and early 1970s, largely in the United Kingdom and the United States. With roots in
      blues rock and psychedelic rock, the bands that created heavy metal developed a thick, massive
      sound, characterized by highly amplified distortion, extended guitar solos, emphatic beats,
      and overall loudness. Heavy metal lyrics and performance styles are often associated with
      masculinity, aggression, and machismo. &lt;p&gt; The first heavy metal bands such as Led
      Zeppelin, Deep Purple and Black Sabbath attracted large audiences, though they were often
      derided by critics, a status common throughout the history of the genre. During the mid-1970s,
      Judas Priest helped spur the genre's evolution by discarding much of its blues influence,
      Motörhead introduced a punk rock sensibility and an increasing emphasis on speed. Bands in the
      New Wave of British Heavy Metal such as Iron Maiden and Saxon followed in a similar vein.
      Before the end of the decade, heavy metal fans became known as &quot;metalheads&quot; or
      &quot;headbangers&quot;. &lt;p&gt; During the 1980s, glam metal became a commercial force with
      groups like Mötley Crüe and Poison.</skos:definition>
    <skos:exactMatch xml:lang="en">http://dbpedia.org/resource/Heavy_metal_music</skos:exactMatch>
    <skos:inScheme rdf:resource="http://data.europeana.eu/concept/music/genre/Music_Genre_Scheme"/>
    <skos:altLabel xml:lang="en">Heavy metal music</skos:altLabel>
    <skos:altLabel xml:lang="en">Heavy metal</skos:altLabel>
  </skos:Concept>

  <skos:Concept rdf:about="http://data.europeana.eu/concept/music/genre/Pop_music">
    <skos:prefLabel xml:lang="en">Pop</skos:prefLabel>
    <skos:prefLabel xml:lang="ar">بوب</skos:prefLabel>
    <skos:prefLabel xml:lang="bg">Поп музика</skos:prefLabel>
    <skos:prefLabel xml:lang="ca">Música pop</skos:prefLabel>
    <skos:prefLabel xml:lang="hr">Pop</skos:prefLabel>
    <skos:prefLabel xml:lang="cs">Pop music</skos:prefLabel>
    <skos:prefLabel xml:lang="da">Popmusik</skos:prefLabel>
    <skos:prefLabel xml:lang="nl">Popmuziek</skos:prefLabel>
    <skos:prefLabel xml:lang="et">Levimuusika</skos:prefLabel>
    <skos:prefLabel xml:lang="fil">Musikang pop</skos:prefLabel>
    <skos:prefLabel xml:lang="fi">Popmusiikki</skos:prefLabel>
    <skos:prefLabel xml:lang="fr">Pop</skos:prefLabel>
    <skos:prefLabel xml:lang="de">Popmusik</skos:prefLabel>
    <skos:prefLabel xml:lang="el">Ποπ μουσική</skos:prefLabel>
    <skos:prefLabel xml:lang="hi">पॉप म्यूज़िक</skos:prefLabel>
    <skos:prefLabel xml:lang="hu">Popzene</skos:prefLabel>
    <skos:prefLabel xml:lang="id">Musik pop</skos:prefLabel>
    <skos:prefLabel xml:lang="it">Musica leggera</skos:prefLabel>
    <skos:prefLabel xml:lang="ja">ポップ・ミュージック</skos:prefLabel>
    <skos:prefLabel xml:lang="ko">팝 음악</skos:prefLabel>
    <skos:prefLabel xml:lang="lv">Popmūzika</skos:prefLabel>
    <skos:prefLabel xml:lang="lt">Popmuzika</skos:prefLabel>
    <skos:prefLabel xml:lang="ms">Muzik pop</skos:prefLabel>
    <skos:prefLabel xml:lang="no">Popmusikk</skos:prefLabel>
    <skos:prefLabel xml:lang="fa">موسیقی پاپ</skos:prefLabel>
    <skos:prefLabel xml:lang="pl">Muzyka pop</skos:prefLabel>
    <skos:prefLabel xml:lang="pt">Música pop</skos:prefLabel>
    <skos:prefLabel xml:lang="ro">Muzică pop</skos:prefLabel>
    <skos:prefLabel xml:lang="ru">Поп-музыка</skos:prefLabel>
    <skos:prefLabel xml:lang="sr">Поп музика</skos:prefLabel>
    <skos:prefLabel xml:lang="sk">Populárna hudba</skos:prefLabel>
    <skos:prefLabel xml:lang="sl">Pop glasba</skos:prefLabel>
    <skos:prefLabel xml:lang="es">Pop</skos:prefLabel>
    <skos:prefLabel xml:lang="sv">Popmusik</skos:prefLabel>
    <skos:prefLabel xml:lang="th">ป็อป</skos:prefLabel>
    <skos:prefLabel xml:lang="tr">Pop Müzik</skos:prefLabel>
    <skos:prefLabel xml:lang="uk">Поп-музика</skos:prefLabel>
    <skos:prefLabel xml:lang="vi">Pop</skos:prefLabel>
    <skos:closeMatch rdf:resource="http://rdf.freebase.com/ns/m.064t9"/>
    <skos:broader rdf:resource="http://data.europeana.eu/concept/music/genre/Pop_music_fusions"/>
    <skos:definition xml:lang="en">Pop music is a genre of popular music which originated in its
      modern form in the 1950s, deriving from rock and roll. The terms &quot;popular music&quot; and
      &quot;pop music&quot; are often used interchangeably, even though the former is a description
      of music which is popular. &lt;p&gt; As a genre, pop music is very eclectic, often borrowing
      elements from other styles including urban, dance, rock, Latin and country, nonetheless, there
      are core elements which define pop. Such include generally short-to-medium length songs,
      written in a basic format, as well as the common employment of repeated choruses, melodic
      tunes, and catchy hooks. &lt;p&gt; So-called &quot;pure pop&quot; music, such as power pop,
      features all these elements, using electric guitars, drums and bass for instrumentation, in
      the case of such music, the main goal is usually that of being pleasurable to listen to,
      rather than having much artistic depth. Pop music is generally thought of as a genre which is
      commercially recorded and desires to have a mass audience appeal.</skos:definition>
    <skos:exactMatch xml:lang="en">http://dbpedia.org/resource/Pop_music</skos:exactMatch>
    <skos:inScheme rdf:resource="http://data.europeana.eu/concept/music/genre/Music_Genre_Scheme"/>
    <skos:altLabel xml:lang="en">Pop music</skos:altLabel>
  </skos:Concept>

  <skos:Concept rdf:about="http://data.europeana.eu/concept/music/genre/Rock_music">
    <skos:prefLabel xml:lang="en">Rock</skos:prefLabel>
    <skos:prefLabel xml:lang="ar">موسيقى الروك</skos:prefLabel>
    <skos:prefLabel xml:lang="bg">Рок музика</skos:prefLabel>
    <skos:prefLabel xml:lang="ca">Música rock</skos:prefLabel>
    <skos:prefLabel xml:lang="hr">Rock</skos:prefLabel>
    <skos:prefLabel xml:lang="cs">Rock and roll</skos:prefLabel>
    <skos:prefLabel xml:lang="da">Rock and roll</skos:prefLabel>
    <skos:prefLabel xml:lang="nl">Rock-'n-roll</skos:prefLabel>
    <skos:prefLabel xml:lang="et">Rokkmuusika</skos:prefLabel>
    <skos:prefLabel xml:lang="fil">Musikang rock</skos:prefLabel>
    <skos:prefLabel xml:lang="fi">Rock</skos:prefLabel>
    <skos:prefLabel xml:lang="fr">Rock</skos:prefLabel>
    <skos:prefLabel xml:lang="de">Rockmusik</skos:prefLabel>
    <skos:prefLabel xml:lang="el">Ροκ μουσική</skos:prefLabel>
    <skos:prefLabel xml:lang="hi">रॉक संगीत</skos:prefLabel>
    <skos:prefLabel xml:lang="hu">Rock</skos:prefLabel>
    <skos:prefLabel xml:lang="id">Musik rock</skos:prefLabel>
    <skos:prefLabel xml:lang="it">Rock and roll</skos:prefLabel>
    <skos:prefLabel xml:lang="ja">ロック</skos:prefLabel>
    <skos:prefLabel xml:lang="ko">로큰롤</skos:prefLabel>
    <skos:prefLabel xml:lang="lv">Rokmūzika</skos:prefLabel>
    <skos:prefLabel xml:lang="lt">Rokenrolas</skos:prefLabel>
    <skos:prefLabel xml:lang="ms">Muzik rock</skos:prefLabel>
    <skos:prefLabel xml:lang="no">Rock and roll</skos:prefLabel>
    <skos:prefLabel xml:lang="fa">راک</skos:prefLabel>
    <skos:prefLabel xml:lang="pl">Rock and roll</skos:prefLabel>
    <skos:prefLabel xml:lang="pt">Rock</skos:prefLabel>
    <skos:prefLabel xml:lang="ro">Muzică rock</skos:prefLabel>
    <skos:prefLabel xml:lang="ru">Рок-музыка</skos:prefLabel>
    <skos:prefLabel xml:lang="sr">Рокенрол</skos:prefLabel>
    <skos:prefLabel xml:lang="sk">Rokenrol</skos:prefLabel>
    <skos:prefLabel xml:lang="sl">Rock</skos:prefLabel>
    <skos:prefLabel xml:lang="es">Rock</skos:prefLabel>
    <skos:prefLabel xml:lang="sv">Rock'n'roll</skos:prefLabel>
    <skos:prefLabel xml:lang="th">ร็อกแอนด์โรล</skos:prefLabel>
    <skos:prefLabel xml:lang="tr">Rock müzik</skos:prefLabel>
    <skos:prefLabel xml:lang="uk">Рок-музика</skos:prefLabel>
    <skos:prefLabel xml:lang="vi">Rock</skos:prefLabel>
    <skos:closeMatch rdf:resource="http://rdf.freebase.com/ns/m.06by7"/>
    <skos:broader rdf:resource="http://data.europeana.eu/concept/music/genre/Popular_music"/>
    <skos:definition xml:lang="en">Rock music is a genre of popular music that originated as
      &quot;rock and roll&quot; in the United States in the 1950s, and developed into a range of
      different styles in the 1960s and later, particularly in the United Kingdom and the United
      States. It has its roots in 1940s' and 1950s' rock and roll, itself heavily influenced by
      rhythm and blues and country music. Rock music also drew strongly on a number of other genres
      such as blues and folk, and incorporated influences from jazz, classical and other musical
      sources. &lt;p&gt; Musically, rock has centered on the electric guitar, usually as part of a
      rock group with electric bass guitar and drums. Typically, rock is song-based music usually
      with a 4/4 time signature using a verse-chorus form, but the genre has become extremely
      diverse. Like pop music, lyrics often stress romantic love but also address a wide variety of
      other themes that are frequently social or political in emphasis. The dominance of rock by
      white, male musicians has been seen as one of the key factors shaping the themes explored in
      rock music. Rock places a higher degree of emphasis on musicianship, live performance, and an
      ideology of authenticity than pop music.</skos:definition>
    <skos:exactMatch xml:lang="en">http://dbpedia.org/resource/Rock_music</skos:exactMatch>
    <skos:inScheme rdf:resource="http://data.europeana.eu/concept/music/genre/Music_Genre_Scheme"/>
    <skos:altLabel xml:lang="en">Rock music</skos:altLabel>
  </skos:Concept>

  <skos:Concept rdf:about="http://data.europeana.eu/concept/music/genre/Salsa_music">
    <skos:prefLabel xml:lang="en">Salsa</skos:prefLabel>
    <skos:prefLabel xml:lang="ar">صلصة</skos:prefLabel>
    <skos:prefLabel xml:lang="ca">Salsa</skos:prefLabel>
    <skos:prefLabel xml:lang="da">Salsa</skos:prefLabel>
    <skos:prefLabel xml:lang="nl">Salsa</skos:prefLabel>
    <skos:prefLabel xml:lang="fi">Salsa</skos:prefLabel>
    <skos:prefLabel xml:lang="fr">Salsa</skos:prefLabel>
    <skos:prefLabel xml:lang="de">Salsa</skos:prefLabel>
    <skos:prefLabel xml:lang="el">Σάλσα</skos:prefLabel>
    <skos:prefLabel xml:lang="it">Salsa</skos:prefLabel>
    <skos:prefLabel xml:lang="ja">サルサ</skos:prefLabel>
    <skos:prefLabel xml:lang="ko">살사</skos:prefLabel>
    <skos:prefLabel xml:lang="lt">Salsa</skos:prefLabel>
    <skos:prefLabel xml:lang="no">Salsa</skos:prefLabel>
    <skos:prefLabel xml:lang="fa">سالسا</skos:prefLabel>
    <skos:prefLabel xml:lang="pl">Salsa</skos:prefLabel>
    <skos:prefLabel xml:lang="pt">Salsa</skos:prefLabel>
    <skos:prefLabel xml:lang="ro">Muzică salsa</skos:prefLabel>
    <skos:prefLabel xml:lang="ru">Сальса</skos:prefLabel>
    <skos:prefLabel xml:lang="es">Salsa</skos:prefLabel>
    <skos:prefLabel xml:lang="sv">Salsa</skos:prefLabel>
    <skos:prefLabel xml:lang="th">ซัลซา</skos:prefLabel>
    <skos:prefLabel xml:lang="tr">Salsa</skos:prefLabel>
    <skos:prefLabel xml:lang="uk">Сальса</skos:prefLabel>
    <skos:closeMatch rdf:resource="http://rdf.freebase.com/ns/m.0ln16"/>
    <skos:broader
      rdf:resource="http://data.europeana.eu/concept/music/genre/Latin_American_music_popular"/>
    <skos:definition xml:lang="en">Salsa music is a general term referring to what is Cuban and
      Puerto Rican popular dance music. The term &quot;Salsa&quot; was initially promoted and
      marketed in New York City during the 1970s. The various musical genres comprising salsa
      include the Cuban son montuno, guaracha, chachachá, mambo, and to a certain extent bolero.
      Salsa is the product of genres such as the Puerto Rican bomba and plena. In some cases, the
      term is also used to describe Dominican merengue, and the Colombian cumbia. Latin jazz, which
      was also developed in New York City, has had a significant influence on salsa arrangers, piano
      guajeos, and instrumental soloists. &lt;p&gt; Salsa is primarily Cuban son, itself a fusion of
      Spanish canción and guitar and Afro-Cuban percussion, merged with North American music styles
      such as jazz. Salsa also occasionally incorporates elements of rock, R&amp;B, and funk. All of
      these non-Cuban elements are grafted onto the basic Cuban son montuno template when performed
      within the context of salsa. &lt;p&gt; The first salsa bands were predominantly
      &quot;Nuyorican&quot; or Puerto Ricans migrated to New York. The music eventually spread
      throughout the Americas. Ultimately, salsa's popularity spread globally.</skos:definition>
    <skos:exactMatch xml:lang="en">http://dbpedia.org/resource/Salsa_music</skos:exactMatch>
    <skos:inScheme rdf:resource="http://data.europeana.eu/concept/music/genre/Music_Genre_Scheme"/>
    <skos:altLabel xml:lang="en">Salsa music</skos:altLabel>
  </skos:Concept>

  <skos:Concept rdf:about="http://data.europeana.eu/concept/music/genre/Schlager_music">
    <skos:prefLabel xml:lang="en">Schlager</skos:prefLabel>
    <skos:prefLabel xml:lang="bg">Шлагер</skos:prefLabel>
    <skos:prefLabel xml:lang="hr">Šlager</skos:prefLabel>
    <skos:prefLabel xml:lang="da">Slager</skos:prefLabel>
    <skos:prefLabel xml:lang="nl">Schlager</skos:prefLabel>
    <skos:prefLabel xml:lang="et">Šlaager</skos:prefLabel>
    <skos:prefLabel xml:lang="fi">Iskelmämusiikki</skos:prefLabel>
    <skos:prefLabel xml:lang="fr">Schlager</skos:prefLabel>
    <skos:prefLabel xml:lang="de">Schlager</skos:prefLabel>
    <skos:prefLabel xml:lang="it">Schlager</skos:prefLabel>
    <skos:prefLabel xml:lang="lv">Šlāgermūzika</skos:prefLabel>
    <skos:prefLabel xml:lang="lt">Šlageris</skos:prefLabel>
    <skos:prefLabel xml:lang="no">Slager</skos:prefLabel>
    <skos:prefLabel xml:lang="pt">Schlager</skos:prefLabel>
    <skos:prefLabel xml:lang="es">Schlager</skos:prefLabel>
    <skos:prefLabel xml:lang="sv">Schlager</skos:prefLabel>
    <skos:closeMatch rdf:resource="http://rdf.freebase.com/ns/m.01rq4x"/>
    <skos:broader rdf:resource="http://data.europeana.eu/concept/music/genre/Pop_music"/>
    <skos:definition xml:lang="en">Schlager music, also known in the United States as entertainer
      music or German hit mix, is a style of popular or electronic music prevalent in Central and
      Northern Europe, and Southeast Europe and also in France and Poland. In Portugal, it was
      adapted and became pimba music. Typical schlager tracks are either sweet, highly sentimental
      ballads with a simple, catchy melody or light pop tunes. Lyrics typically center on love,
      relationships and feelings. The northern variant of schlager has taken elements from Nordic
      and Slavic folk songs, with lyrics tending towards melancholic and elegiac themes. Musically,
      schlager bears similarities to styles such as easy listening music. &lt;p&gt; The word
      schlager is also a loanword in some languages, where it retained its meaning of a &quot;
      hit&quot;. The style has been frequently represented at the Eurovision Song Contest and has
      been popular since it originated in 1956, although it is gradually being replaced by other pop
      music styles.</skos:definition>
    <skos:exactMatch xml:lang="en">http://dbpedia.org/resource/Schlager_music</skos:exactMatch>
    <skos:inScheme rdf:resource="http://data.europeana.eu/concept/music/genre/Music_Genre_Scheme"/>
    <skos:altLabel xml:lang="en">Schlager music</skos:altLabel>
  </skos:Concept>

  <skos:Concept rdf:about="http://data.europeana.eu/concept/music/genre/Soca_music">
    <skos:prefLabel xml:lang="en">Soca</skos:prefLabel>
    <skos:prefLabel xml:lang="da">Soca</skos:prefLabel>
    <skos:prefLabel xml:lang="nl">Soca</skos:prefLabel>
    <skos:prefLabel xml:lang="fr">Soca</skos:prefLabel>
    <skos:prefLabel xml:lang="de">Soca</skos:prefLabel>
    <skos:prefLabel xml:lang="hu">Soca</skos:prefLabel>
    <skos:prefLabel xml:lang="it">Soca</skos:prefLabel>
    <skos:prefLabel xml:lang="ja">ソカ</skos:prefLabel>
    <skos:prefLabel xml:lang="pl">Soca</skos:prefLabel>
    <skos:prefLabel xml:lang="pt">Soca</skos:prefLabel>
    <skos:prefLabel xml:lang="es">Soca</skos:prefLabel>
    <skos:prefLabel xml:lang="sv">Soca</skos:prefLabel>
    <skos:closeMatch rdf:resource="http://rdf.freebase.com/ns/m.0kpck"/>
    <skos:broader
      rdf:resource="http://data.europeana.eu/concept/music/genre/Latin_American_music_fusions"/>
    <skos:definition xml:lang="en">Soca is a style of Caribbean music originating in Trinidad and
      Tobago. &lt;p&gt; Soca developed as an offshoot of Kaiso/calypso, with influences from
      Cadence-lypso, Soul, and Funk. The presence of a large Indian population in Trinidad blended
      traditional Indian musical instruments—particularly the dholak, tabla and dhantal—into a style
      called chutney music. &lt;p&gt; Soca has evolved in the last 20 years primarily by musicians
      from various Anglophone Caribbean countries including Trinidad, Guyana, Saint Vincent and the
      Grenadines, Barbados, Grenada, Saint Lucia, Antigua and Barbuda, United States Virgin Islands,
      British Virgin Islands, The Bahamas, Dominica, Saint Kitts and Nevis, Jamaica, Belize,
      Montserrat and Panama.</skos:definition>
    <skos:exactMatch xml:lang="en">http://dbpedia.org/resource/Soca_music</skos:exactMatch>
    <skos:inScheme rdf:resource="http://data.europeana.eu/concept/music/genre/Music_Genre_Scheme"/>
    <skos:altLabel xml:lang="en">Soca music</skos:altLabel>
  </skos:Concept>

  <skos:Concept rdf:about="http://data.europeana.eu/concept/music/genre/Surf_music">
    <skos:prefLabel xml:lang="en">Surf</skos:prefLabel>
    <skos:prefLabel xml:lang="ca">Música surf</skos:prefLabel>
    <skos:prefLabel xml:lang="hr">Surf glazba</skos:prefLabel>
    <skos:prefLabel xml:lang="cs">Surf rock</skos:prefLabel>
    <skos:prefLabel xml:lang="nl">Surf</skos:prefLabel>
    <skos:prefLabel xml:lang="fi">Surf</skos:prefLabel>
    <skos:prefLabel xml:lang="fr">Surf music</skos:prefLabel>
    <skos:prefLabel xml:lang="de">Surfmusik</skos:prefLabel>
    <skos:prefLabel xml:lang="hu">Surf rock</skos:prefLabel>
    <skos:prefLabel xml:lang="it">Surf pop</skos:prefLabel>
    <skos:prefLabel xml:lang="ko">서프 음악</skos:prefLabel>
    <skos:prefLabel xml:lang="no">Surfemusikk</skos:prefLabel>
    <skos:prefLabel xml:lang="pl">Surf rock</skos:prefLabel>
    <skos:prefLabel xml:lang="pt">Surf music</skos:prefLabel>
    <skos:prefLabel xml:lang="ru">Сёрф-рок</skos:prefLabel>
    <skos:prefLabel xml:lang="sk">Surf rock</skos:prefLabel>
    <skos:prefLabel xml:lang="sl">Surf rock</skos:prefLabel>
    <skos:prefLabel xml:lang="es">Música surf</skos:prefLabel>
    <skos:prefLabel xml:lang="sv">Surf</skos:prefLabel>
    <skos:prefLabel xml:lang="uk">Серф</skos:prefLabel>
    <skos:closeMatch rdf:resource="http://rdf.freebase.com/ns/m.01756d"/>
    <skos:broader rdf:resource="http://data.europeana.eu/concept/music/genre/Rock_music"/>
    <skos:definition xml:lang="en">Surf music is a genre of popular music associated with surf
      culture, particularly as found in Orange County and other areas of Southern California. It was
      especially popular from 1961 to 1966, has subsequently been revived and was highly influential
      on subsequent rock music. It has two major forms: largely instrumental surf rock, with an
      electric guitar or saxophone playing the main melody, largely pioneered by Dick Dale and the
      Del-Tones, and vocal surf pop, including both surf ballads and dance music, often with strong
      harmonies that are most associated with the Beach Boys. Many notable surf bands have been
      equally noted for both surf instrumental and surf pop music, so surf music is generally
      considered as a single genre despite the variety of these styles. During the later stages of
      the surf music craze, many groups started to leave surfing behind and write songs about cars
      and girls, this was later known as hot rod rock. Surf music is often referred to as simply
      surf rock, even though the genre has many forms.</skos:definition>
    <skos:exactMatch xml:lang="en">http://dbpedia.org/resource/Surf_music</skos:exactMatch>
    <skos:inScheme rdf:resource="http://data.europeana.eu/concept/music/genre/Music_Genre_Scheme"/>
    <skos:altLabel xml:lang="en">Surf music</skos:altLabel>
  </skos:Concept>

  <skos:Concept rdf:about="http://data.europeana.eu/concept/music/genre/Afro-Cuban">
    <skos:prefLabel xml:lang="en">Afro-Cuban music</skos:prefLabel>
    <skos:prefLabel xml:lang="fr">Afro-Cubains</skos:prefLabel>
    <skos:prefLabel xml:lang="de">Afrokubaner</skos:prefLabel>
    <skos:prefLabel xml:lang="no">Afro-cubanere</skos:prefLabel>
    <skos:prefLabel xml:lang="pt">Afro-cubanos</skos:prefLabel>
    <skos:prefLabel xml:lang="tr">Afro-Kübalı</skos:prefLabel>
    <skos:closeMatch rdf:resource="http://rdf.freebase.com/ns/m.03yk6g"/>
    <skos:broader
      rdf:resource="http://data.europeana.eu/concept/music/genre/Latin_American_music_popular"/>
    <skos:definition xml:lang="en">The term Afro-Cuban refers to Cubans who mostly have Sub-Saharan
      African ancestry, and to historical or cultural elements in Cuba thought to emanate from this
      community. The term can refer to the combining of African and other cultural elements found in
      Cuban society such as race, religion, music, language, the arts, and class
      culture.</skos:definition>
    <skos:exactMatch xml:lang="en">http://dbpedia.org/resource/Afro-Cuban</skos:exactMatch>
    <skos:inScheme rdf:resource="http://data.europeana.eu/concept/music/genre/Music_Genre_Scheme"/>
    <skos:altLabel xml:lang="en">Afro-Cuban</skos:altLabel>
  </skos:Concept>

  <skos:Concept rdf:about="http://data.europeana.eu/concept/music/genre/Bhangra_(music)">
    <skos:prefLabel xml:lang="en">Bhangra</skos:prefLabel>
    <skos:prefLabel xml:lang="ar">بانغرا</skos:prefLabel>
    <skos:prefLabel xml:lang="nl">Bhangra</skos:prefLabel>
    <skos:prefLabel xml:lang="fi">Bhangra</skos:prefLabel>
    <skos:prefLabel xml:lang="fr">Bhangra</skos:prefLabel>
    <skos:prefLabel xml:lang="de">Bhangra</skos:prefLabel>
    <skos:prefLabel xml:lang="hi">भांगड़ा</skos:prefLabel>
    <skos:prefLabel xml:lang="it">Bhangra</skos:prefLabel>
    <skos:prefLabel xml:lang="ja">バングラ</skos:prefLabel>
    <skos:prefLabel xml:lang="pl">Bhangra</skos:prefLabel>
    <skos:prefLabel xml:lang="pt">Bhangra</skos:prefLabel>
    <skos:prefLabel xml:lang="es">Bhangra</skos:prefLabel>
    <skos:prefLabel xml:lang="sv">Bhangra</skos:prefLabel>
    <skos:prefLabel xml:lang="tr">Bhangra</skos:prefLabel>
    <skos:closeMatch rdf:resource="http://rdf.freebase.com/ns/m.017ht"/>
    <skos:broader rdf:resource="http://data.europeana.eu/concept/music/genre/Pop_music_fusions"/>
    <skos:definition xml:lang="en">Bha?g?? is an upbeat type of popular music associated with
      Punjabi culture. It was developed in Britain in the 1980s by first and second generation
      immigrants from the Punjab region of India and Pakistan forming the Punjabi diaspora, drawing
      from music and song of the Punjab region as well as various Western musical styles. It is seen
      by some in the West as an expression of South Asian culture as a whole. Bhangra music was
      replaced by Punjabi folk music in the mid 1990s. Using the derivative form of Punjabi Folk
      music and Hip hop, known as Folkhop.</skos:definition>
    <skos:exactMatch xml:lang="en">http://dbpedia.org/resource/Bhangra_(music)</skos:exactMatch>
    <skos:inScheme rdf:resource="http://data.europeana.eu/concept/music/genre/Music_Genre_Scheme"/>
    <skos:altLabel xml:lang="en">Bhangra</skos:altLabel>
  </skos:Concept>

  <skos:Concept rdf:about="http://data.europeana.eu/concept/music/genre/Copla_(music)">
    <skos:prefLabel xml:lang="en">Copla</skos:prefLabel>
    <skos:prefLabel xml:lang="ca">Copla andalusa</skos:prefLabel>
    <skos:prefLabel xml:lang="fr">Copla</skos:prefLabel>
    <skos:prefLabel xml:lang="de">Copla andaluza</skos:prefLabel>
    <skos:prefLabel xml:lang="it">Copla andalusa</skos:prefLabel>
    <skos:prefLabel xml:lang="pl">Copla</skos:prefLabel>
    <skos:prefLabel xml:lang="es">Copla andaluza</skos:prefLabel>
    <skos:closeMatch rdf:resource="http://rdf.freebase.com/ns/m.0bwgmrk"/>
    <skos:broader rdf:resource="http://data.europeana.eu/concept/music/genre/Popular_music"/>
    <skos:definition xml:lang="en">The copla or copla andaluza is a form of Spanish popular song,
      deriving from the poetic form of the same name. Although the genre has a long heritage, it
      flourished in the 1940s, and is epitomized by songwriters Antonio Quintero, Rafael de León and
      Manuel Quiroga. It is also associated with the Catalonian folk-dance, the sardana. &lt;p&gt;
      One of the first singers of coplas was Raquel Meller. Initially she sang cuplé, which later
      evolved in Andalusian and Spanish song into the copla as it is known today. Other well-known
      singers of coplas are Imperio Argentina, Manolo Corrales, Estrellita Castro, Concha Piquer,
      Miguel de Molina, Lola Flores, Marifé de Triana, Juanita Reina, Manolo Escobar, Juanito
      Valderrama, Sara Montiel and Antonio Molina. &lt;p&gt; Particularly of note is es: Carlos
      Cano, who was a key figure in reviving the popularity of the copla in the later 20th century.
      More recent singers of coplas include Rocío Jurado, Bambino, María Jiménez, Isabel Pantoja,
      Martirio, and es:Miguel Poveda and, even more recently, Pasión Vega, Clara Montes, Pastora
      Soler, Aurora Guirado, Diana Navarro, Concha Buika, La Shica and Montse Delgado. Some of these
      artists, particularly Pasión Vega and Diana Navarro, have bent and stretched the genre in
      directions that have come to be known as Nueva Copla.</skos:definition>
    <skos:exactMatch xml:lang="en">http://dbpedia.org/resource/Copla_(music)</skos:exactMatch>
    <skos:inScheme rdf:resource="http://data.europeana.eu/concept/music/genre/Music_Genre_Scheme"/>
    <skos:altLabel xml:lang="en">Copla</skos:altLabel>
  </skos:Concept>

  <skos:Concept rdf:about="http://data.europeana.eu/concept/music/genre/Mambo_(music)">
    <skos:prefLabel xml:lang="en">Mambo</skos:prefLabel>
    <skos:prefLabel xml:lang="ar">المامبو</skos:prefLabel>
    <skos:prefLabel xml:lang="ca">Mambo</skos:prefLabel>
    <skos:prefLabel xml:lang="nl">Mambo (dans)</skos:prefLabel>
    <skos:prefLabel xml:lang="fr">Mambo</skos:prefLabel>
    <skos:prefLabel xml:lang="de">Mambo</skos:prefLabel>
    <skos:prefLabel xml:lang="hu">Mambó</skos:prefLabel>
    <skos:prefLabel xml:lang="it">Mambo</skos:prefLabel>
    <skos:prefLabel xml:lang="ja">マンボ</skos:prefLabel>
    <skos:prefLabel xml:lang="pl">Mambo (taniec)</skos:prefLabel>
    <skos:prefLabel xml:lang="sr">Мамбо</skos:prefLabel>
    <skos:prefLabel xml:lang="es">Mambo</skos:prefLabel>
    <skos:prefLabel xml:lang="sv">Mambo (dans)</skos:prefLabel>
    <skos:closeMatch rdf:resource="http://rdf.freebase.com/ns/m.055nc"/>
    <skos:broader
      rdf:resource="http://data.europeana.eu/concept/music/genre/Latin_American_music_popular"/>
    <skos:definition xml:lang="en">Mambo is a musical form and dance style that developed originally
      in Cuba, with further significant developments by Cuban musicians in Mexico and the USA. The
      word &quot;mambo&quot; means &quot;conversation with the gods&quot; in Kikongo, the language
      spoken by Central African slaves taken to Cuba.</skos:definition>
    <skos:exactMatch xml:lang="en">http://dbpedia.org/resource/Mambo_(music)</skos:exactMatch>
    <skos:inScheme rdf:resource="http://data.europeana.eu/concept/music/genre/Music_Genre_Scheme"/>
    <skos:altLabel xml:lang="en">Mambo</skos:altLabel>
  </skos:Concept>

  <skos:Concept rdf:about="http://data.europeana.eu/concept/music/genre/March_(music)">
    <skos:prefLabel xml:lang="en">March</skos:prefLabel>
    <skos:prefLabel xml:lang="ar">مارش</skos:prefLabel>
    <skos:prefLabel xml:lang="ca">Marxa</skos:prefLabel>
    <skos:prefLabel xml:lang="hr">Koračnice</skos:prefLabel>
    <skos:prefLabel xml:lang="cs">Pochod (hudba)</skos:prefLabel>
    <skos:prefLabel xml:lang="da">March</skos:prefLabel>
    <skos:prefLabel xml:lang="nl">Mars</skos:prefLabel>
    <skos:prefLabel xml:lang="et">Marss</skos:prefLabel>
    <skos:prefLabel xml:lang="fi">Marssi</skos:prefLabel>
    <skos:prefLabel xml:lang="fr">Marche</skos:prefLabel>
    <skos:prefLabel xml:lang="de">Marschmusik</skos:prefLabel>
    <skos:prefLabel xml:lang="el">Εμβατήριο</skos:prefLabel>
    <skos:prefLabel xml:lang="id">Musik mars</skos:prefLabel>
    <skos:prefLabel xml:lang="it">Marcia</skos:prefLabel>
    <skos:prefLabel xml:lang="ja">行進曲</skos:prefLabel>
    <skos:prefLabel xml:lang="ko">행진곡</skos:prefLabel>
    <skos:prefLabel xml:lang="no">Marsj</skos:prefLabel>
    <skos:prefLabel xml:lang="pl">Marsz</skos:prefLabel>
    <skos:prefLabel xml:lang="pt">Marcha</skos:prefLabel>
    <skos:prefLabel xml:lang="ru">Марш</skos:prefLabel>
    <skos:prefLabel xml:lang="es">Marcha</skos:prefLabel>
    <skos:prefLabel xml:lang="sv">Marschmusik</skos:prefLabel>
    <skos:prefLabel xml:lang="th">มาร์ช</skos:prefLabel>
    <skos:prefLabel xml:lang="tr">Marş</skos:prefLabel>
    <skos:prefLabel xml:lang="uk">Марш</skos:prefLabel>
    <skos:closeMatch rdf:resource="http://rdf.freebase.com/ns/m.0cdr_y"/>
    <skos:broader rdf:resource="http://data.europeana.eu/concept/music/genre/Martial_music"/>
    <skos:definition xml:lang="en">A march, as a musical genre, is a piece of music with a strong
      regular rhythm which in origin was expressly written for marching to and most frequently
      performed by a military band. In mood, marches range from the moving death march in Wagner's
      Götterdämmerung to the brisk military marches of John Philip Sousa and the martial hymns of
      the late 19th century. Examples of the varied use of the march can be found in Beethoven's
      Eroica Symphony, in the Marches Militaires of Franz Schubert, in the Marche funèbre in
      Chopin's Sonata in B flat minor, and in the Dead March in Handel's Saul.</skos:definition>
    <skos:exactMatch xml:lang="en">http://dbpedia.org/resource/March_(music)</skos:exactMatch>
    <skos:inScheme rdf:resource="http://data.europeana.eu/concept/music/genre/Music_Genre_Scheme"/>
    <skos:altLabel xml:lang="en">March</skos:altLabel>
  </skos:Concept>

  <skos:Concept rdf:about="http://data.europeana.eu/concept/music/genre/Milonga_(music)">
    <skos:prefLabel xml:lang="en">Milonga</skos:prefLabel>
    <skos:prefLabel xml:lang="ca">Milonga</skos:prefLabel>
    <skos:prefLabel xml:lang="cs">Milonga</skos:prefLabel>
    <skos:prefLabel xml:lang="nl">Milonga</skos:prefLabel>
    <skos:prefLabel xml:lang="fi">Milonga</skos:prefLabel>
    <skos:prefLabel xml:lang="fr">Milonga pampeana</skos:prefLabel>
    <skos:prefLabel xml:lang="de">Milonga</skos:prefLabel>
    <skos:prefLabel xml:lang="hu">Milonga</skos:prefLabel>
    <skos:prefLabel xml:lang="it">Milonga</skos:prefLabel>
    <skos:prefLabel xml:lang="ja">ミロンガ</skos:prefLabel>
    <skos:prefLabel xml:lang="no">Milonga</skos:prefLabel>
    <skos:prefLabel xml:lang="pl">Milonga</skos:prefLabel>
    <skos:prefLabel xml:lang="pt">Milonga</skos:prefLabel>
    <skos:prefLabel xml:lang="ru">Милонга</skos:prefLabel>
    <skos:prefLabel xml:lang="sk">Milonga</skos:prefLabel>
    <skos:prefLabel xml:lang="sl">Milonga</skos:prefLabel>
    <skos:prefLabel xml:lang="es">Milonga</skos:prefLabel>
    <skos:prefLabel xml:lang="sv">Milonga</skos:prefLabel>
    <skos:prefLabel xml:lang="tr">Milonga</skos:prefLabel>
    <skos:closeMatch rdf:resource="http://rdf.freebase.com/ns/m.01qq2k"/>
    <skos:broader
      rdf:resource="http://data.europeana.eu/concept/music/genre/Latin_American_music_traditional"/>
    <skos:definition xml:lang="en">Milonga is a musical genre that originated in the Río de la Plata
      areas of Argentina and Uruguay. It was very popular in the 1870s. It was derived from an
      earlier style of singing known as the payada de contrapunto. The song was set to a lively 2/4
      tempo, as are most milongas. &lt;p&gt; &quot;Milonga is an excited habanera.&quot; The
      original habanera divided into four pulses, in a standard two-four where every note was
      stressed. In becoming milonga, though, all four notes turned strong, as tempo was doubled. The
      strength of the first beat weakened the fourth giving an almost waltz-like feel to milonga:
      one-two-three, one-two-three. Habanera is a slower, more explicit sounding one, two,
      three-four. At least one modern tango pianist believes the polka influenced the speeding up of
      the milonga. &lt;p&gt; Milonga has a syncopated beat, consisting of 8 beats with accents on
      the 1st, 4th, 5th, and 7th beats. &lt;p&gt; Regular 2/4 &lt;p&gt; [1] 2 3 4 [5] 6 7 8
      &lt;p&gt; Milonga &lt;p&gt; [1] 2 3 [4] [5] 6 [7] 8, sometimes also [1] [2] 3 [4] [5] 6 [7] 8
      &lt;p&gt; 332 &lt;p&gt; [1] 2 3 [4] 5 6 [7] 8 &lt;p&gt; Over time, dance steps and other
      musical influences were added, eventually giving rise to the tango.</skos:definition>
    <skos:exactMatch xml:lang="en">http://dbpedia.org/resource/Milonga_(music)</skos:exactMatch>
    <skos:inScheme rdf:resource="http://data.europeana.eu/concept/music/genre/Music_Genre_Scheme"/>
    <skos:altLabel xml:lang="en">Milonga</skos:altLabel>
  </skos:Concept>

  <skos:Concept rdf:about="http://data.europeana.eu/concept/music/genre/Romance_(music)">
    <skos:prefLabel xml:lang="en">Romance</skos:prefLabel>
    <skos:prefLabel xml:lang="ar">موسيقى رومانسية</skos:prefLabel>
    <skos:prefLabel xml:lang="da">Romance</skos:prefLabel>
    <skos:prefLabel xml:lang="nl">Romance</skos:prefLabel>
    <skos:prefLabel xml:lang="et">Romanss</skos:prefLabel>
    <skos:prefLabel xml:lang="fr">Romance</skos:prefLabel>
    <skos:prefLabel xml:lang="it">Romanza</skos:prefLabel>
    <skos:prefLabel xml:lang="ja">ロマンス</skos:prefLabel>
    <skos:prefLabel xml:lang="ko">로망스</skos:prefLabel>
    <skos:prefLabel xml:lang="lt">Romansas</skos:prefLabel>
    <skos:prefLabel xml:lang="ro">Romanță</skos:prefLabel>
    <skos:prefLabel xml:lang="ru">Романс</skos:prefLabel>
    <skos:prefLabel xml:lang="es">Romanza</skos:prefLabel>
    <skos:prefLabel xml:lang="uk">Романс</skos:prefLabel>
    <skos:prefLabel xml:lang="vi">Romance</skos:prefLabel>
    <skos:closeMatch rdf:resource="http://rdf.freebase.com/ns/m.02l2pp"/>
    <skos:broader rdf:resource="http://data.europeana.eu/concept/music/genre/Art_music"/>
    <skos:definition xml:lang="en">The term romance has a centuries-long history. Applied to
      narrative ballads in Spain, it came to be used by the 18th century for simple lyrical pieces
      not only for voice, but also for instruments alone. The Oxford Dictionary of Music states that
      &quot;generally it implies a specially personal or tender quality&quot;.</skos:definition>
    <skos:exactMatch xml:lang="en">http://dbpedia.org/resource/Romance_(music)</skos:exactMatch>
    <skos:inScheme rdf:resource="http://data.europeana.eu/concept/music/genre/Music_Genre_Scheme"/>
    <skos:altLabel xml:lang="en">Romance</skos:altLabel>
  </skos:Concept>

  <skos:Concept rdf:about="http://data.europeana.eu/concept/music/genre/Arabesque_(Turkish_music)">
    <skos:prefLabel xml:lang="en">Arabesque</skos:prefLabel>
    <skos:prefLabel xml:lang="ar">أرابيسك</skos:prefLabel>
    <skos:prefLabel xml:lang="nl">Arabeskmuziek</skos:prefLabel>
    <skos:prefLabel xml:lang="fi">Arabeskimusiikki</skos:prefLabel>
    <skos:prefLabel xml:lang="de">Arabeske</skos:prefLabel>
    <skos:prefLabel xml:lang="tr">Arabesk müzik</skos:prefLabel>
    <skos:closeMatch rdf:resource="http://rdf.freebase.com/ns/m.0613ds"/>
    <skos:broader rdf:resource="http://data.europeana.eu/concept/music/genre/Art_music"/>
    <skos:definition xml:lang="en">Arabesque or Arabesk is a term created by Turkish musicologists
      for an Arabic style of music created in Turkey. The genre was particularly popular in Turkey
      in the decades from the 1960s through the 1990s. As with Arabic music itself, its aesthetics
      have evolved over the decades. Although melodies and rhythms are predominantly Byzantine and
      Arabic influenced, it also draws ideas from other aspects of Balkan and Middle Eastern music,
      including ba?lama music and Ottoman forms of oriental music.</skos:definition>
    <skos:exactMatch xml:lang="en"
      >http://dbpedia.org/resource/Arabesque_(Turkish_music)</skos:exactMatch>
    <skos:inScheme rdf:resource="http://data.europeana.eu/concept/music/genre/Music_Genre_Scheme"/>
    <skos:altLabel xml:lang="en">Arabesque</skos:altLabel>
  </skos:Concept>

  <skos:Concept rdf:about="http://data.europeana.eu/concept/music/genre/Ballad">
    <skos:prefLabel xml:lang="en">Ballad</skos:prefLabel>
    <skos:closeMatch rdf:resource="http://rdf.freebase.com/ns/m.01gjw"/>
    <skos:broader rdf:resource="http://data.europeana.eu/concept/music/genre/Popular_music"/>
    <skos:definition xml:lang="en">A ballad is a form of verse, often a narrative set to music.
      Ballads derive from the medieval French chanson balladée or ballade, which were originally
      &quot;dancing songs&quot;. Ballads were particularly characteristic of the popular poetry and
      song of the British Isles from the later medieval period until the 19th century and used
      extensively across Europe and later the Americas, Australia and North Africa. Many ballads
      were written and sold as single sheet broadsides. The form was often used by poets and
      composers from the 18th century onwards to produce lyrical ballads. In the later 19th century
      it took on the meaning of a slow form of popular love song and the term is now often used as
      synonymous with any love song, particularly the pop or rock power ballad.</skos:definition>
    <skos:exactMatch xml:lang="en">http://dbpedia.org/resource/Ballad</skos:exactMatch>
    <skos:inScheme rdf:resource="http://data.europeana.eu/concept/music/genre/Music_Genre_Scheme"/>
  </skos:Concept>

  <skos:Concept rdf:about="http://data.europeana.eu/concept/music/genre/Biguine">
    <skos:prefLabel xml:lang="en">Beguine</skos:prefLabel>
    <skos:prefLabel xml:lang="nl">Beguine</skos:prefLabel>
    <skos:prefLabel xml:lang="fi">Beguine</skos:prefLabel>
    <skos:prefLabel xml:lang="fr">Biguine</skos:prefLabel>
    <skos:prefLabel xml:lang="de">Beguine</skos:prefLabel>
    <skos:prefLabel xml:lang="it">Beguine</skos:prefLabel>
    <skos:prefLabel xml:lang="pl">Beguine</skos:prefLabel>
    <skos:prefLabel xml:lang="ru">Бегин</skos:prefLabel>
    <skos:prefLabel xml:lang="es">Beguine</skos:prefLabel>
    <skos:closeMatch rdf:resource="http://rdf.freebase.com/ns/m.05bffx"/>
    <skos:broader
      rdf:resource="http://data.europeana.eu/concept/music/genre/Latin_American_music_popular"/>
    <skos:definition xml:lang="en">Biguine is a rhythm-centric style of music that originated in
      Martinique in the 19th century. It fuses 19th-century French ballroom dance steps with African
      rhythms.</skos:definition>
    <skos:exactMatch xml:lang="en">http://dbpedia.org/resource/Biguine</skos:exactMatch>
    <skos:inScheme rdf:resource="http://data.europeana.eu/concept/music/genre/Music_Genre_Scheme"/>
    <skos:altLabel xml:lang="en">Biguine</skos:altLabel>
  </skos:Concept>

  <skos:Concept rdf:about="http://data.europeana.eu/concept/music/genre/Bomba_(Puerto_Rico)">
    <skos:prefLabel xml:lang="en">Bomba</skos:prefLabel>
    <skos:prefLabel xml:lang="fr">Bomba</skos:prefLabel>
    <skos:prefLabel xml:lang="it">Bomba</skos:prefLabel>
    <skos:prefLabel xml:lang="es">Bomba</skos:prefLabel>
    <skos:closeMatch rdf:resource="http://rdf.freebase.com/ns/m.036q2d"/>
    <skos:broader
      rdf:resource="http://data.europeana.eu/concept/music/genre/Latin_American_music_traditional"/>
    <skos:definition xml:lang="en">Bomba is one of the traditional musical styles of Puerto Rico. It
      is the mixture of the three different cultures of the Island, the Spanish, African and Taino
      cultures. The base rhythm is played by two or more drums. &lt;p&gt; While bomba can be used as
      the generic name for a number of rhythms, its real meaning is about the encounter and creative
      relationship between dancers, percussionists, and singers. Bomba is a communal activity that
      still thrives in its traditional centers of Loíza, Santurce, Mayagüez, Ponce, and New York
      City.</skos:definition>
    <skos:exactMatch xml:lang="en">http://dbpedia.org/resource/Bomba_(Puerto_Rico)</skos:exactMatch>
    <skos:inScheme rdf:resource="http://data.europeana.eu/concept/music/genre/Music_Genre_Scheme"/>
    <skos:altLabel xml:lang="en">Bomba</skos:altLabel>
  </skos:Concept>

  <skos:Concept rdf:about="http://data.europeana.eu/concept/music/genre/Bomba_(Ecuador)">
    <skos:prefLabel xml:lang="en">Bomba del Chota</skos:prefLabel>
    <skos:prefLabel xml:lang="es">Bomba del Chota</skos:prefLabel>
    <skos:closeMatch rdf:resource="http://rdf.freebase.com/ns/m.06c87y"/>
    <skos:broader
      rdf:resource="http://data.europeana.eu/concept/music/genre/Latin_American_music_traditional"/>
    <skos:definition xml:lang="en">Bomba or Bomba del Chota is an Afro-Ecuadorian music, dance and
      rum al form from the Chota Valley area of Ecuador in the province of Imbabura and Carchi. Its
      origins can be traced back to Africa via the middle passage and the use of African slave labor
      during the country's colonial period. Africans brought to labor as slaves in Ecuador brought
      with them this music form heavily influenced from the Bantu cultures of the Congo. The people
      dance in pairs to the drums and use improvisation to build relationships between the dancer
      and lead drummer. &lt;p&gt; This music and dance tends to have a prominent Spanish, mestizo
      and indigenous influence in the melodies. It could go from a mid tempo to a very fast rhythm.
      It is usually played with guitars along with the main local instrument which is also called
      bomba which is a drum along with a guiro and sometimes bombos and bongos. A variation of it is
      la banda mocha which are groups that play bomba with a bombo, guiro and plant leafs to give
      melody. &lt;p&gt; Recently it is enjoying some national exposure but outside of the Chota
      Valley it is mostly popular in cities such as Quito and Ibarra which have important
      concentrations of afro-chotan people. In these cities sometimes it is played in discothèques
      and has some public performances as well as popularity among mestizo and indigenous
      people.</skos:definition>
    <skos:exactMatch xml:lang="en">http://dbpedia.org/resource/Bomba_(Ecuador)</skos:exactMatch>
    <skos:inScheme rdf:resource="http://data.europeana.eu/concept/music/genre/Music_Genre_Scheme"/>
    <skos:altLabel xml:lang="en">Bomba</skos:altLabel>
  </skos:Concept>

  <skos:Concept rdf:about="http://data.europeana.eu/concept/music/genre/Concerto">
    <skos:prefLabel xml:lang="en">Concerto</skos:prefLabel>
    <skos:prefLabel xml:lang="ar">كونشرتو</skos:prefLabel>
    <skos:prefLabel xml:lang="bg">Концерт</skos:prefLabel>
    <skos:prefLabel xml:lang="ca">Concert</skos:prefLabel>
    <skos:prefLabel xml:lang="cs">Koncert</skos:prefLabel>
    <skos:prefLabel xml:lang="da">Koncert</skos:prefLabel>
    <skos:prefLabel xml:lang="nl">Concerto</skos:prefLabel>
    <skos:prefLabel xml:lang="et">Instrumentaalkontsert</skos:prefLabel>
    <skos:prefLabel xml:lang="fi">Konsertto</skos:prefLabel>
    <skos:prefLabel xml:lang="fr">Concerto</skos:prefLabel>
    <skos:prefLabel xml:lang="de">Instrumentalkonzert</skos:prefLabel>
    <skos:prefLabel xml:lang="el">Κοντσέρτο</skos:prefLabel>
    <skos:prefLabel xml:lang="hu">Versenymű</skos:prefLabel>
    <skos:prefLabel xml:lang="it">Concerto</skos:prefLabel>
    <skos:prefLabel xml:lang="ja">協奏曲</skos:prefLabel>
    <skos:prefLabel xml:lang="ko">협주곡</skos:prefLabel>
    <skos:prefLabel xml:lang="no">Solokonsert</skos:prefLabel>
    <skos:prefLabel xml:lang="fa">کنسرتو</skos:prefLabel>
    <skos:prefLabel xml:lang="pl">Koncert</skos:prefLabel>
    <skos:prefLabel xml:lang="pt">Concerto</skos:prefLabel>
    <skos:prefLabel xml:lang="ro">Concert</skos:prefLabel>
    <skos:prefLabel xml:lang="ru">Концерт</skos:prefLabel>
    <skos:prefLabel xml:lang="sr">Концерт</skos:prefLabel>
    <skos:prefLabel xml:lang="sl">Koncert</skos:prefLabel>
    <skos:prefLabel xml:lang="es">Concierto</skos:prefLabel>
    <skos:prefLabel xml:lang="sv">Konsert</skos:prefLabel>
    <skos:prefLabel xml:lang="th">ดนตรีประชัน</skos:prefLabel>
    <skos:prefLabel xml:lang="tr">Konçerto</skos:prefLabel>
    <skos:prefLabel xml:lang="uk">Концерт</skos:prefLabel>
    <skos:prefLabel xml:lang="vi">Concerto</skos:prefLabel>
    <skos:closeMatch rdf:resource="http://rdf.freebase.com/ns/m.0c0y7"/>
    <skos:broader rdf:resource="http://data.europeana.eu/concept/music/genre/Classical_music"/>
    <skos:definition xml:lang="en">A concerto is a musical composition usually composed in three
      parts or movements, in which one solo instrument is accompanied by an orchestra or concert
      band. &lt;p&gt; The etymology is uncertain, but the word seems to have originated from the
      conjunction of the two Latin words conserere and certamen: the idea is that the two parts in a
      concerto, the soloist and the orchestra or concert band, alternate episodes of opposition,
      cooperation, and independence in the creation of the music flow. &lt;p&gt; The concerto, as
      understood in this modern way, arose in the Baroque period side by side with the concerto
      grosso, which contrasted a small group of instruments with the rest of the orchestra. The
      popularity of the concerto grosso form declined after the Baroque period, and the genre was
      not revived until the 20th century. The solo concerto, however, has remained a vital musical
      force from its inception to this day.</skos:definition>
    <skos:exactMatch xml:lang="en">http://dbpedia.org/page/Concerto</skos:exactMatch>
    <skos:inScheme rdf:resource="http://data.europeana.eu/concept/music/genre/Music_Genre_Scheme"/>
    <skos:altLabel xml:lang="en">Concerto</skos:altLabel>
  </skos:Concept>

  <skos:Concept rdf:about="http://data.europeana.eu/concept/music/genre/Dastgah">
    <skos:prefLabel xml:lang="en">Dastgah</skos:prefLabel>
    <skos:prefLabel xml:lang="fr">Dastgâh</skos:prefLabel>
    <skos:prefLabel xml:lang="de">Dastgah</skos:prefLabel>
    <skos:prefLabel xml:lang="ja">ダストガー</skos:prefLabel>
    <skos:prefLabel xml:lang="fa">دستگاه‌های موسیقی ایرانی</skos:prefLabel>
    <skos:prefLabel xml:lang="ru">Дестгях</skos:prefLabel>
    <skos:prefLabel xml:lang="es">Dastgah</skos:prefLabel>
    <skos:closeMatch rdf:resource="http://rdf.freebase.com/ns/m.07_mdk"/>
    <skos:broader
      rdf:resource="http://data.europeana.eu/concept/music/genre/Music_of_Asia_traditional"/>
    <skos:definition xml:lang="en">Dastg?h is a musical modal system in traditional Persian art
      music. Persian art music consists of twelve principal musical modal systems or dastg?hs, in
      spite of 50 or more extant dastg?hs, theorists generally refer to a set of twelve principal
      ones. A dastg?h is a melody type on the basis of which a performer produces extemporised
      pieces. &lt;p&gt; Each dastg?h consists of seven basic notes, plus several variable notes used
      for ornamentation and modulation. Each dastg?h is a certain modal variety subject to a course
      of development that is determined by the pre-established order of sequences, and revolves
      around 365 central nuclear melodies known as gushehs which the individual musician comes to
      know through experience and absorption. This process of centonization is personal, and it is a
      tradition of great subtlety and depth. The full collection of gushehs in all dastg?hs is
      referred to as the radif. During the meeting of The Inter-governmental Committee for the
      Safeguarding of the Intangible Heritage of the United Nations, held between 28 September – 2
      October 2009 in Abu Dhabi, radifs were officially registered on the UNESCO List of the
      Intangible Cultural Heritage of Humanity.</skos:definition>
    <skos:exactMatch xml:lang="en">http://dbpedia.org/resource/Dastgah</skos:exactMatch>
    <skos:inScheme rdf:resource="http://data.europeana.eu/concept/music/genre/Music_Genre_Scheme"/>
    <skos:altLabel xml:lang="en">Dastgah</skos:altLabel>
  </skos:Concept>

  <skos:Concept rdf:about="http://data.europeana.eu/concept/music/genre/Epic_(genre)">
    <skos:prefLabel xml:lang="en">Epic</skos:prefLabel>
    <skos:prefLabel xml:lang="da">Epik</skos:prefLabel>
    <skos:prefLabel xml:lang="lt">Epopėja</skos:prefLabel>
    <skos:prefLabel xml:lang="pt">Épico</skos:prefLabel>
    <skos:prefLabel xml:lang="ro">Epic</skos:prefLabel>
    <skos:prefLabel xml:lang="ru">Эпопея</skos:prefLabel>
    <skos:prefLabel xml:lang="sr">Еп</skos:prefLabel>
    <skos:prefLabel xml:lang="sv">Epik</skos:prefLabel>
    <skos:prefLabel xml:lang="tr">Epik</skos:prefLabel>
    <skos:prefLabel xml:lang="uk">Епопея</skos:prefLabel>
    <skos:prefLabel xml:lang="vi">Sử thi</skos:prefLabel>
    <skos:broader rdf:resource="http://data.europeana.eu/concept/music/genre/Art_music"/>
    <skos:exactMatch xml:lang="en">http://dbpedia.org/page/Epic_(genre)</skos:exactMatch>
    <skos:inScheme rdf:resource="http://data.europeana.eu/concept/music/genre/Music_Genre_Scheme"/>
    <skos:altLabel xml:lang="en">Epic</skos:altLabel>
  </skos:Concept>

  <skos:Concept rdf:about="http://data.europeana.eu/concept/music/genre/Filin_(music)">
    <skos:prefLabel xml:lang="en">Filin</skos:prefLabel>
    <skos:prefLabel xml:lang="fr">Filin</skos:prefLabel>
    <skos:prefLabel xml:lang="es">Filin</skos:prefLabel>
    <skos:closeMatch rdf:resource="http://rdf.freebase.com/ns/m.05c4kxb"/>
    <skos:broader
      rdf:resource="http://data.europeana.eu/concept/music/genre/Latin_American_music_popular"/>
    <skos:definition xml:lang="en">Filin was a Cuban, but US–influenced, popular song fashion of the
      late 1940s to the early 1960s. The word is derived from feeling, and is sometimes spelled
      feelín or even el feeling. It describes a style of post-microphone jazz-influenced romantic
      song. &lt;p&gt; The Cuban roots of filín were in the bolero and the canción. It was related to
      the trova: in fact, filín was sometimes regarded as a renewal or reinvigoration, of the old
      trova. Some Cuban quartets, such as Cuarteto d'Aida and Los Zafiros, modelled themselves on
      U.S. close-harmony groups. Others were singers who had heard Ella Fitzgerald, Sarah Vaughan
      and Nat King Cole. Filín singers included César Portillo de la Luz, José Antonio Méndez, who
      spent a decade in Mexico from 1949 to 1959, Frank Domínguez, the blind pianist Frank Emilio
      Flynn, and the great singers of boleros Elena Burke and the still-performing Omara Portuondo,
      who both came from the Cuarteto d'Aida. &lt;p&gt; A house in Havana, where the trovador Tirso
      Díaz lived, became a meeting-place for singers and musicians interested in filín. Here
      lyricists and singers could meet arrangers, such as Bebo Valdés, El Niño Rivera, Peruchín, and
      get help to develop their work.</skos:definition>
    <skos:exactMatch xml:lang="en">http://dbpedia.org/resource/Filin_(music)</skos:exactMatch>
    <skos:inScheme rdf:resource="http://data.europeana.eu/concept/music/genre/Music_Genre_Scheme"/>
    <skos:altLabel xml:lang="en">Filin</skos:altLabel>
  </skos:Concept>

  <skos:Concept rdf:about="http://data.europeana.eu/concept/music/genre/Free_improvisation">
    <skos:prefLabel xml:lang="en">Free improvisation</skos:prefLabel>
    <skos:prefLabel xml:lang="nl">Improvisatie (muziek)</skos:prefLabel>
    <skos:prefLabel xml:lang="fr">Musique improvisée</skos:prefLabel>
    <skos:prefLabel xml:lang="de">Neue Improvisationsmusik</skos:prefLabel>
    <skos:prefLabel xml:lang="it">Improvvisazione libera</skos:prefLabel>
    <skos:prefLabel xml:lang="ru">Свободная импровизация</skos:prefLabel>
    <skos:prefLabel xml:lang="es">Improvisación libre</skos:prefLabel>
    <skos:prefLabel xml:lang="sv">Fri improvisationsmusik</skos:prefLabel>
    <skos:closeMatch rdf:resource="http://rdf.freebase.com/ns/m.0f_j1"/>
    <skos:broader rdf:resource="http://data.europeana.eu/concept/music/genre/Jazz_fusions"/>
    <skos:definition xml:lang="en">Free improvisation or free music is improvised music without any
      rules beyond the logic or inclination of the musician involved. The term can refer to both a
      technique and as a recognizable genre in its own right. &lt;p&gt; Free improvisation, as a
      genre of music, developed in the U.S. and Europe in the mid to late 1960s, largely as an
      outgrowth of free jazz and modern classical musics. None of its primary exponents can be said
      to be famous amongst the general public, however, in experimental circles, a number of free
      musicians are well known, including saxophonists Evan Parker, Anthony Braxton, Peter Brötzmann
      and John Zorn, drummer Christian Lillinger, trombonist George Lewis, guitarists Derek Bailey,
      Henry Kaiser and Fred Frith and the improvising groups The Art Ensemble of Chicago and
      AMM.</skos:definition>
    <skos:exactMatch xml:lang="en">http://dbpedia.org/resource/Free_improvisation</skos:exactMatch>
    <skos:inScheme rdf:resource="http://data.europeana.eu/concept/music/genre/Music_Genre_Scheme"/>
    <skos:altLabel xml:lang="en">Free improvisation</skos:altLabel>
  </skos:Concept>

  <skos:Concept rdf:about="http://data.europeana.eu/concept/music/genre/Giddha">
    <skos:prefLabel xml:lang="en">Giddha</skos:prefLabel>
    <skos:prefLabel xml:lang="nl">Gidda</skos:prefLabel>
    <skos:prefLabel xml:lang="de">Giddha</skos:prefLabel>
    <skos:prefLabel xml:lang="hi">गिद्दा</skos:prefLabel>
    <skos:closeMatch rdf:resource="http://rdf.freebase.com/ns/m.03rmvt"/>
    <skos:broader
      rdf:resource="http://data.europeana.eu/concept/music/genre/Music_of_Asia_traditional"/>
    <skos:definition xml:lang="en">Giddha is a popular folk dance of women in Punjab region of India
      and Pakistan. The dance is often considered derived from the ancient dance known as the ring
      dance and is just as energetic as Bhangra, at the same time it manages to creatively display
      feminine grace, elegance and elasticity. It is a very colourful dance form which is now copied
      in all regions of the country. Women perform this dance mainly at festive or social
      occasions.</skos:definition>
    <skos:exactMatch xml:lang="en">http://dbpedia.org/resource/Giddha</skos:exactMatch>
    <skos:inScheme rdf:resource="http://data.europeana.eu/concept/music/genre/Music_Genre_Scheme"/>
    <skos:altLabel xml:lang="en">Giddha</skos:altLabel>
  </skos:Concept>

  <skos:Concept rdf:about="http://data.europeana.eu/concept/music/genre/Romani_music">
    <skos:prefLabel xml:lang="en">Gypsy music</skos:prefLabel>
    <skos:prefLabel xml:lang="hr">Romska glazba</skos:prefLabel>
    <skos:prefLabel xml:lang="nl">Zigeunermuziek</skos:prefLabel>
    <skos:prefLabel xml:lang="fr">Musique tzigane</skos:prefLabel>
    <skos:prefLabel xml:lang="de">Musik der Roma</skos:prefLabel>
    <skos:prefLabel xml:lang="ja">ロマ音楽</skos:prefLabel>
    <skos:prefLabel xml:lang="no">Sigøynermusikk</skos:prefLabel>
    <skos:prefLabel xml:lang="pl">Muzyka cygańska</skos:prefLabel>
    <skos:prefLabel xml:lang="sk">Rómska hudba</skos:prefLabel>
    <skos:prefLabel xml:lang="sv">Romsk musik</skos:prefLabel>
    <skos:closeMatch rdf:resource="http://rdf.freebase.com/ns/m.01cmnj"/>
    <skos:broader rdf:resource="http://data.europeana.eu/concept/music/genre/Folk_music_traditional"/>
    <skos:definition xml:lang="en">Romani music is the music of the Romani people, who have their
      origins in Northern India, but today live mostly in Europe. &lt;p&gt; Historically nomadic,
      though now largely settled, the Romani people have long acted as entertainers and tradesmen.
      In many of the places Romanies live they have become known as musicians. The wide distances
      travelled have introduced a multitude of influences, starting with Indian roots and adding
      elements of Greek, Arabic, Persian, Turkish, Serbian, Czech, Slavic, Romanian, German, Dutch,
      French and Spanish musical forms. &lt;p&gt; It is difficult to define the parameters of a
      unified Romani musical style, as there are many differences in melodic, harmonic, rhythmic,
      and formal structures from region to region. Lyrics to Romani songs are often sung in one or
      more dialects of the Romani language, and dance frequently accompanies Romani music
      performance. &lt;p&gt; There is a strong tradition of Romani music in Central and Eastern
      Europe, notably in countries such as Hungary, Romania and the former Yugoslavia. The
      quintessentially Spanish flamenco is to a very large extent the music of the Romani people of
      Andalusia.</skos:definition>
    <skos:exactMatch xml:lang="en">http://dbpedia.org/resource/Romani_music</skos:exactMatch>
    <skos:inScheme rdf:resource="http://data.europeana.eu/concept/music/genre/Music_Genre_Scheme"/>
    <skos:altLabel xml:lang="en">Romani music</skos:altLabel>
  </skos:Concept>

  <skos:Concept rdf:about="http://data.europeana.eu/concept/music/genre/Hora_(dance)">
    <skos:prefLabel xml:lang="en">Hora</skos:prefLabel>
    <skos:prefLabel xml:lang="bg">Хоро</skos:prefLabel>
    <skos:prefLabel xml:lang="nl">Hora</skos:prefLabel>
    <skos:prefLabel xml:lang="fil">Hora</skos:prefLabel>
    <skos:prefLabel xml:lang="fi">Hora</skos:prefLabel>
    <skos:prefLabel xml:lang="fr">Hora</skos:prefLabel>
    <skos:prefLabel xml:lang="de">Horo</skos:prefLabel>
    <skos:prefLabel xml:lang="el">Τσουρτούγουζους</skos:prefLabel>
    <skos:prefLabel xml:lang="pl">Hora</skos:prefLabel>
    <skos:prefLabel xml:lang="pt">Hora</skos:prefLabel>
    <skos:prefLabel xml:lang="ro">Horă</skos:prefLabel>
    <skos:prefLabel xml:lang="ru">Хора</skos:prefLabel>
    <skos:prefLabel xml:lang="sv">Hora</skos:prefLabel>
    <skos:prefLabel xml:lang="tr">Hora</skos:prefLabel>
    <skos:closeMatch rdf:resource="http://rdf.freebase.com/ns/m.020twq"/>
    <skos:broader rdf:resource="http://data.europeana.eu/concept/music/genre/Folk_music_traditional"/>
    <skos:definition xml:lang="en">Hora, also known as horo and oro, is a type of circle dance
      originating in the Balkans but also found in other countries.</skos:definition>
    <skos:exactMatch xml:lang="en">http://dbpedia.org/resource/Hora_(dance)</skos:exactMatch>
    <skos:inScheme rdf:resource="http://data.europeana.eu/concept/music/genre/Music_Genre_Scheme"/>
    <skos:altLabel xml:lang="en">Hora</skos:altLabel>
  </skos:Concept>

  <skos:Concept rdf:about="http://data.europeana.eu/concept/music/genre/Huayno">
    <skos:prefLabel xml:lang="en">Huayno</skos:prefLabel>
    <skos:prefLabel xml:lang="ca">Huayno</skos:prefLabel>
    <skos:prefLabel xml:lang="fr">Huayno</skos:prefLabel>
    <skos:prefLabel xml:lang="it">Huayno</skos:prefLabel>
    <skos:prefLabel xml:lang="ja">ワイニョ</skos:prefLabel>
    <skos:prefLabel xml:lang="lt">Huayno</skos:prefLabel>
    <skos:prefLabel xml:lang="pl">Huayno</skos:prefLabel>
    <skos:prefLabel xml:lang="pt">Huaino</skos:prefLabel>
    <skos:prefLabel xml:lang="es">Huayno</skos:prefLabel>
    <skos:prefLabel xml:lang="uk">Уайньйо</skos:prefLabel>
    <skos:closeMatch rdf:resource="http://rdf.freebase.com/ns/m.04jm4w"/>
    <skos:broader
      rdf:resource="http://data.europeana.eu/concept/music/genre/Latin_American_music_traditional"/>
    <skos:definition xml:lang="en">Huayno is a genre of popular Andean Music and dance originally
      from Serrania, Peru. It is especially common in Peru, but also present in Chile, Bolivia,
      Argentina and Ecuador, and is practiced by a variety of ethnic groups, including the Quechua
      and Aymara people. The history of huayno dates back to the colonial Peru as a combination of
      traditional rural folk music and popular urban dance music. High-pitched vocals are
      accompanied by a variety of instruments, including quena, harp, siku, accordion, saxophone,
      charango, lute, violin, guitar, and mandolin. Some elements of huayno originate in the music
      of the pre-Columbian Andes, especially on the territory of former Inca Empire. Huayno utilizes
      a distinctive rhythm in which the first beat is stressed and followed by two short
      beats.</skos:definition>
    <skos:exactMatch xml:lang="en">http://dbpedia.org/resource/Huayno</skos:exactMatch>
    <skos:inScheme rdf:resource="http://data.europeana.eu/concept/music/genre/Music_Genre_Scheme"/>
    <skos:altLabel xml:lang="en">Huayno</skos:altLabel>
  </skos:Concept>

  <skos:Concept rdf:about="http://data.europeana.eu/concept/music/genre/Jazz_fusion">
    <skos:prefLabel xml:lang="en">Jazz Rock</skos:prefLabel>
    <skos:closeMatch rdf:resource="http://rdf.freebase.com/ns/m.01fh36"/>
    <skos:broader rdf:resource="http://data.europeana.eu/concept/music/genre/Jazz_fusions"/>
    <skos:definition xml:lang="en">Jazz fusion, fusion, or jazz-rock are variants of a musical
      fusion genre that developed from mixing funk and R&amp;B rhythms and the amplification and
      electronic effects of rock music, complex time signatures derived from non-Western music and
      extended, typically instrumental compositions with a jazz approach to lengthy group
      improvisations, often using wind and brass and displaying a high level of instrumental
      technique. It was created around the late 1960s. The term &quot;jazz rock&quot; is often used
      as a synonym for &quot;jazz fusion&quot; as well as for music performed by late 1960s and
      1970s-era rock bands that added jazz elements to their music. &lt;p&gt; After a decade of
      popularity during the 1970s, fusion expanded its improvisatory and experimental approaches
      through the 1980s and 1990s. Fusion albums, even those that are made by the same group or
      artist, may include a variety of styles. Rather than being a codified musical style, fusion
      can be viewed as a musical tradition or approach.</skos:definition>
    <skos:exactMatch xml:lang="en">http://dbpedia.org/resource/Jazz_fusion</skos:exactMatch>
    <skos:inScheme rdf:resource="http://data.europeana.eu/concept/music/genre/Music_Genre_Scheme"/>
  </skos:Concept>

  <skos:Concept rdf:about="http://data.europeana.eu/concept/music/genre/Lament">
    <skos:prefLabel xml:lang="en">Laments</skos:prefLabel>
    <skos:prefLabel xml:lang="fr">Lamento</skos:prefLabel>
    <skos:prefLabel xml:lang="de">Lamento</skos:prefLabel>
    <skos:prefLabel xml:lang="it">Lamentazione</skos:prefLabel>
    <skos:prefLabel xml:lang="ja">ラメント</skos:prefLabel>
    <skos:prefLabel xml:lang="lt">Rauda</skos:prefLabel>
    <skos:prefLabel xml:lang="no">Lamento</skos:prefLabel>
    <skos:prefLabel xml:lang="pl">Tren</skos:prefLabel>
    <skos:prefLabel xml:lang="ru">Плач</skos:prefLabel>
    <skos:closeMatch rdf:resource="http://rdf.freebase.com/ns/m.02ytbz"/>
    <skos:broader rdf:resource="http://data.europeana.eu/concept/music/genre/Folk_music_traditional"/>
    <skos:definition xml:lang="en">A lament or lamentation is a passionate expression of grief,
      often in music, poetry, or song form. The grief is most often born of regret, or
      mourning.</skos:definition>
    <skos:exactMatch xml:lang="en">http://dbpedia.org/resource/Lament</skos:exactMatch>
    <skos:inScheme rdf:resource="http://data.europeana.eu/concept/music/genre/Music_Genre_Scheme"/>
    <skos:altLabel xml:lang="en">Lament</skos:altLabel>
  </skos:Concept>

  <skos:Concept rdf:about="http://data.europeana.eu/concept/music/genre/Madrigal">
    <skos:prefLabel xml:lang="en">Madrigal</skos:prefLabel>
    <skos:prefLabel xml:lang="ar">مادريجال</skos:prefLabel>
    <skos:prefLabel xml:lang="bg">Мадригал</skos:prefLabel>
    <skos:prefLabel xml:lang="ca">Madrigal</skos:prefLabel>
    <skos:prefLabel xml:lang="cs">Madrigal</skos:prefLabel>
    <skos:prefLabel xml:lang="da">Madrigal</skos:prefLabel>
    <skos:prefLabel xml:lang="nl">Madrigaal</skos:prefLabel>
    <skos:prefLabel xml:lang="et">Madrigal</skos:prefLabel>
    <skos:prefLabel xml:lang="fi">Madrigaali</skos:prefLabel>
    <skos:prefLabel xml:lang="fr">Madrigal</skos:prefLabel>
    <skos:prefLabel xml:lang="de">Madrigal</skos:prefLabel>
    <skos:prefLabel xml:lang="el">Μαδριγάλι</skos:prefLabel>
    <skos:prefLabel xml:lang="hu">Madrigal</skos:prefLabel>
    <skos:prefLabel xml:lang="it">Madrigale</skos:prefLabel>
    <skos:prefLabel xml:lang="ja">マドリガーレ</skos:prefLabel>
    <skos:prefLabel xml:lang="ko">마드리갈</skos:prefLabel>
    <skos:prefLabel xml:lang="lt">Madrigalas</skos:prefLabel>
    <skos:prefLabel xml:lang="no">Madrigal</skos:prefLabel>
    <skos:prefLabel xml:lang="pl">Madrygał</skos:prefLabel>
    <skos:prefLabel xml:lang="pt">Madrigal</skos:prefLabel>
    <skos:prefLabel xml:lang="ro">Madrigal</skos:prefLabel>
    <skos:prefLabel xml:lang="ru">Мадригал</skos:prefLabel>
    <skos:prefLabel xml:lang="sk">Madrigal</skos:prefLabel>
    <skos:prefLabel xml:lang="sl">Madrigal</skos:prefLabel>
    <skos:prefLabel xml:lang="es">Madrigal</skos:prefLabel>
    <skos:prefLabel xml:lang="sv">Madrigal</skos:prefLabel>
    <skos:prefLabel xml:lang="tr">Madrigal</skos:prefLabel>
    <skos:prefLabel xml:lang="uk">Мадригал</skos:prefLabel>
    <skos:prefLabel xml:lang="vi">Madrigal</skos:prefLabel>
    <skos:closeMatch rdf:resource="http://rdf.freebase.com/ns/m.01x2nx"/>
    <skos:broader rdf:resource="http://data.europeana.eu/concept/music/genre/Classical_music"/>
    <skos:definition xml:lang="en">A madrigal is a secular vocal music composition, usually a
      partsong, of the Renaissance and early Baroque eras. Traditionally, polyphonic madrigals are
      unaccompanied, the number of voices varies from two to eight, and most frequently from three
      to six. It is quite distinct from the Italian Trecento madrigal of the late 13th and 14th
      centuries, with which it shares only the name. &lt;p&gt; Madrigals originated in Italy during
      the 1520s. Unlike many strophic forms of the time, most madrigals were through-composed. In
      the madrigal, the composer attempted to express the emotion contained in each line, and
      sometimes individual words, of a celebrated poem. &lt;p&gt; The madrigal originated in part
      from the frottola, in part from the resurgence in interest in vernacular Italian poetry, and
      also from the influence of the French chanson and polyphonic style of the motet as written by
      the Franco-Flemish composers who had naturalized in Italy during the period. A frottola
      generally would consist of music set to stanzas of text, while madrigals were
      through-composed. However, some of the same poems were used for both frottola and
      madrigals.</skos:definition>
    <skos:exactMatch xml:lang="en">http://dbpedia.org/resource/Madrigal</skos:exactMatch>
    <skos:inScheme rdf:resource="http://data.europeana.eu/concept/music/genre/Music_Genre_Scheme"/>
    <skos:altLabel xml:lang="en">Madrigal</skos:altLabel>
  </skos:Concept>

  <skos:Concept rdf:about="http://data.europeana.eu/concept/music/genre/Maluf">
    <skos:prefLabel xml:lang="en">Ma'luf</skos:prefLabel>
    <skos:prefLabel xml:lang="ar">المالوف</skos:prefLabel>
    <skos:prefLabel xml:lang="fr">Malouf</skos:prefLabel>
    <skos:closeMatch rdf:resource="http://rdf.freebase.com/ns/m.0406kty"/>
    <skos:broader rdf:resource="http://data.europeana.eu/concept/music/genre/Art_music"/>
    <skos:definition xml:lang="en">The maluf is a genre of art music in the Andalusian classical
      music tradition of Algeria, Libya and Tunisia. It was revived in the 1920s by the French
      musicologist Baron Rodolphe d'Erlanger. A detailed description of Malouf in Tunisia can be
      found under &quot;Music of Tunisia&quot;.</skos:definition>
    <skos:exactMatch xml:lang="en">http://dbpedia.org/resource/Ma'luf</skos:exactMatch>
    <skos:inScheme rdf:resource="http://data.europeana.eu/concept/music/genre/Music_Genre_Scheme"/>
    <skos:altLabel xml:lang="en">Ma'luf</skos:altLabel>
  </skos:Concept>

  <skos:Concept rdf:about="http://data.europeana.eu/concept/music/genre/Maqam_al-iraqi">
    <skos:prefLabel xml:lang="en">Maqam</skos:prefLabel>
    <skos:prefLabel xml:lang="ar">المقام العراقي</skos:prefLabel>
    <skos:closeMatch rdf:resource="http://rdf.freebase.com/ns/m.053fhg"/>
    <skos:broader rdf:resource="http://data.europeana.eu/concept/music/genre/Art_music"/>
    <skos:definition xml:lang="en">Iraqi Maqam is at least four hundred year old genre found in Iraq
      and often considered the most perfect form of maqam. The instrumentation of the ensemble used
      in the Iraqi Maqam, Al-Chalghi al-Baghdadi, includes a qari', santur, jawza, tabla or
      dunbug/dumbeg, and sometimes riqq and naqqarat. The focus is on the poem sung in classical
      Arabic or Iraqi dialect. A complete maqam concert is known as fasl and is named after the
      first maqam: bayat, hijaz, rast, nawa, or husayni. &lt;p&gt; A typical performance includes
      the following sections: &lt;p&gt; tahrir, sometimes badwah &lt;p&gt; taslum &lt;p&gt; finalis
      &lt;p&gt; Some well known Iraqi maqam performers include: Mulla Hasan al-Babujachi, Rahmat
      Allah Shiltagh, Khalil Rabbaz, Rahmain Niftar, Rubin Rajwan, Ahmed Zaydan, Mulla Uthman
      al-Mawsili, Jamil al-Baghdadi, Salman Moshe, Rashid al-Qundarchi, Yusuf Huresh, Najm
      al-Shaykhli, Abbas Kambir, Mohammed al-Qubbanchi, Yusuf Omar, Hamed al-Sa‘di, Farida, and
      Husayn al-A‘dhami.</skos:definition>
    <skos:exactMatch xml:lang="en">http://dbpedia.org/resource/Maqam_al-iraqi</skos:exactMatch>
    <skos:inScheme rdf:resource="http://data.europeana.eu/concept/music/genre/Music_Genre_Scheme"/>
    <skos:altLabel xml:lang="en">Maqam al-iraqi</skos:altLabel>
  </skos:Concept>

  <skos:Concept rdf:about="http://data.europeana.eu/concept/music/genre/Delta_blues">
    <skos:prefLabel xml:lang="en">Delta blues</skos:prefLabel>
    <skos:prefLabel xml:lang="bg">Делта блус</skos:prefLabel>
    <skos:prefLabel xml:lang="cs">Delta blues</skos:prefLabel>
    <skos:prefLabel xml:lang="nl">Delta blues</skos:prefLabel>
    <skos:prefLabel xml:lang="fi">Delta blues</skos:prefLabel>
    <skos:prefLabel xml:lang="fr">Delta blues</skos:prefLabel>
    <skos:prefLabel xml:lang="de">Delta Blues</skos:prefLabel>
    <skos:prefLabel xml:lang="it">Delta blues</skos:prefLabel>
    <skos:prefLabel xml:lang="ja">デルタ・ブルース</skos:prefLabel>
    <skos:prefLabel xml:lang="ko">델타 블루스</skos:prefLabel>
    <skos:prefLabel xml:lang="ms">Delta Blues</skos:prefLabel>
    <skos:prefLabel xml:lang="no">Deltablues</skos:prefLabel>
    <skos:prefLabel xml:lang="pl">Blues Delty</skos:prefLabel>
    <skos:prefLabel xml:lang="pt">Delta blues</skos:prefLabel>
    <skos:prefLabel xml:lang="ru">Дельта-блюз</skos:prefLabel>
    <skos:prefLabel xml:lang="es">Delta blues</skos:prefLabel>
    <skos:prefLabel xml:lang="sv">Deltablues</skos:prefLabel>
    <skos:prefLabel xml:lang="uk">Дельта-блюз</skos:prefLabel>
    <skos:closeMatch rdf:resource="http://rdf.freebase.com/ns/m.017323"/>
    <skos:broader rdf:resource="http://data.europeana.eu/concept/music/genre/Blues"/>
    <skos:definition xml:lang="en">The Delta blues is one of the earliest styles of blues music. It
      originated in the Mississippi Delta, a region of the United States that stretches from
      Memphis, Tennessee in the north to Vicksburg, Mississippi in the south, Helena, Arkansas in
      the west to the Yazoo River on the east. The Mississippi Delta area is famous both for its
      fertile soil and its poverty. Guitar, harmonica and cigar box guitar are the dominant
      instruments used, with slide guitar being a hallmark of the style. The vocal styles range from
      introspective and soulful to passionate and fiery. Delta blues is also regarded as a regional
      variation of country blues.</skos:definition>
    <skos:exactMatch xml:lang="en">http://dbpedia.org/resource/Delta_blues</skos:exactMatch>
    <skos:inScheme rdf:resource="http://data.europeana.eu/concept/music/genre/Music_Genre_Scheme"/>
    <skos:altLabel xml:lang="en">Delta blues</skos:altLabel>
  </skos:Concept>

  <skos:Concept rdf:about="http://data.europeana.eu/concept/music/genre/Musical_theatre">
    <skos:prefLabel xml:lang="en">Music theatre</skos:prefLabel>
    <skos:prefLabel xml:lang="ar">مسرح موسيقي</skos:prefLabel>
    <skos:prefLabel xml:lang="bg">Музикален театър</skos:prefLabel>
    <skos:prefLabel xml:lang="ca">Teatre musical</skos:prefLabel>
    <skos:prefLabel xml:lang="hr">Mjuzikl</skos:prefLabel>
    <skos:prefLabel xml:lang="cs">Muzikál</skos:prefLabel>
    <skos:prefLabel xml:lang="da">Musical</skos:prefLabel>
    <skos:prefLabel xml:lang="nl">Musical</skos:prefLabel>
    <skos:prefLabel xml:lang="et">Muusikal</skos:prefLabel>
    <skos:prefLabel xml:lang="fi">Musikaali</skos:prefLabel>
    <skos:prefLabel xml:lang="fr">Comédie musicale</skos:prefLabel>
    <skos:prefLabel xml:lang="de">Musical</skos:prefLabel>
    <skos:prefLabel xml:lang="el">Μιούζικαλ</skos:prefLabel>
    <skos:prefLabel xml:lang="hu">Musical</skos:prefLabel>
    <skos:prefLabel xml:lang="id">Teater musikal</skos:prefLabel>
    <skos:prefLabel xml:lang="it">Musical</skos:prefLabel>
    <skos:prefLabel xml:lang="ja">ミュージカル</skos:prefLabel>
    <skos:prefLabel xml:lang="ko">뮤지컬</skos:prefLabel>
    <skos:prefLabel xml:lang="lt">Muzikinis teatras</skos:prefLabel>
    <skos:prefLabel xml:lang="no">Musikal</skos:prefLabel>
    <skos:prefLabel xml:lang="fa">تئاتر موزیکال</skos:prefLabel>
    <skos:prefLabel xml:lang="pl">Musical</skos:prefLabel>
    <skos:prefLabel xml:lang="pt">Teatro musical</skos:prefLabel>
    <skos:prefLabel xml:lang="ro">Teatru muzical</skos:prefLabel>
    <skos:prefLabel xml:lang="ru">Мюзикл</skos:prefLabel>
    <skos:prefLabel xml:lang="sr">Мјузикл</skos:prefLabel>
    <skos:prefLabel xml:lang="sk">Muzikál</skos:prefLabel>
    <skos:prefLabel xml:lang="sl">Muzikal</skos:prefLabel>
    <skos:prefLabel xml:lang="es">Teatro musical</skos:prefLabel>
    <skos:prefLabel xml:lang="sv">Musikal</skos:prefLabel>
    <skos:prefLabel xml:lang="th">ละครเพลง</skos:prefLabel>
    <skos:prefLabel xml:lang="tr">Müzikal tiyatro</skos:prefLabel>
    <skos:prefLabel xml:lang="uk">Мюзикл</skos:prefLabel>
    <skos:prefLabel xml:lang="vi">Nhạc kịch</skos:prefLabel>
    <skos:closeMatch rdf:resource="http://rdf.freebase.com/ns/m.0557q"/>
    <skos:broader rdf:resource="http://data.europeana.eu/concept/music/genre/Art_music"/>
    <skos:definition xml:lang="en">Musical theatre is a form of theatre that combines songs, spoken
      dialogue, acting, and dance. The story and emotional content of the piece – humor, pathos,
      love, anger – are communicated through the words, music, movement and technical aspects of the
      entertainment as an integrated whole. Although musical theatre overlaps with other theatrical
      forms like opera and dance, it may be distinguished by the equal importance given to the music
      as compared with the dialogue, movement and other elements of the works. Since the early 20th
      century, musical theatre stage works have generally been called, simply, musicals. Although
      music has been a part of dramatic presentations since ancient times, modern Western musical
      theatre emerged during the 19th century, culminating with the works of Gilbert and Sullivan in
      Britain and those of Harrigan and Hart in America. These were followed by the numerous
      Edwardian musical comedies and the musical theatre works of American creators like George M.
      Cohan...</skos:definition>
    <skos:exactMatch xml:lang="en">http://dbpedia.org/resource/Musical_theatre</skos:exactMatch>
    <skos:inScheme rdf:resource="http://data.europeana.eu/concept/music/genre/Music_Genre_Scheme"/>
    <skos:altLabel xml:lang="en">Musical theatre</skos:altLabel>
  </skos:Concept>

  <skos:Concept rdf:about="http://data.europeana.eu/concept/music/genre/New_wave_music">
    <skos:prefLabel xml:lang="en">New wave</skos:prefLabel>
    <skos:prefLabel xml:lang="ar">موجة جديدة</skos:prefLabel>
    <skos:prefLabel xml:lang="bg">Ню уейв</skos:prefLabel>
    <skos:prefLabel xml:lang="ca">New wave</skos:prefLabel>
    <skos:prefLabel xml:lang="hr">Novi val</skos:prefLabel>
    <skos:prefLabel xml:lang="cs">Nová vlna</skos:prefLabel>
    <skos:prefLabel xml:lang="da">New wave</skos:prefLabel>
    <skos:prefLabel xml:lang="nl">New wave</skos:prefLabel>
    <skos:prefLabel xml:lang="fi">Uusi aalto</skos:prefLabel>
    <skos:prefLabel xml:lang="fr">New wave</skos:prefLabel>
    <skos:prefLabel xml:lang="de">New Wave</skos:prefLabel>
    <skos:prefLabel xml:lang="hu">Új hullám</skos:prefLabel>
    <skos:prefLabel xml:lang="id">New wave</skos:prefLabel>
    <skos:prefLabel xml:lang="it">New wave</skos:prefLabel>
    <skos:prefLabel xml:lang="ja">ニュー・ウェーヴ</skos:prefLabel>
    <skos:prefLabel xml:lang="ko">뉴 웨이브</skos:prefLabel>
    <skos:prefLabel xml:lang="lv">Jaunais vilnis</skos:prefLabel>
    <skos:prefLabel xml:lang="lt">New Wave</skos:prefLabel>
    <skos:prefLabel xml:lang="no">New Wave</skos:prefLabel>
    <skos:prefLabel xml:lang="fa">موسیقی موج نو</skos:prefLabel>
    <skos:prefLabel xml:lang="pl">Nowa fala</skos:prefLabel>
    <skos:prefLabel xml:lang="pt">New wave</skos:prefLabel>
    <skos:prefLabel xml:lang="ro">New Wave</skos:prefLabel>
    <skos:prefLabel xml:lang="ru">Новая волна</skos:prefLabel>
    <skos:prefLabel xml:lang="sr">Нови талас</skos:prefLabel>
    <skos:prefLabel xml:lang="sk">New Wave</skos:prefLabel>
    <skos:prefLabel xml:lang="es">New wave</skos:prefLabel>
    <skos:prefLabel xml:lang="sv">New wave-musik</skos:prefLabel>
    <skos:prefLabel xml:lang="th">นิวเวฟ</skos:prefLabel>
    <skos:prefLabel xml:lang="tr">New Wave</skos:prefLabel>
    <skos:prefLabel xml:lang="uk">Нова хвиля</skos:prefLabel>
    <skos:closeMatch rdf:resource="http://rdf.freebase.com/ns/m.059kh"/>
    <skos:broader rdf:resource="http://data.europeana.eu/concept/music/genre/Rock_music"/>
    <skos:definition xml:lang="en">New wave music is an umbrella term for several late-1970s to
      mid-1980s pop/rock musical styles with ties to 1970s punk rock. Initially—as with the later
      post-punk—new wave was broadly analogous to punk rock before branching as a distinctly
      identified genre, incorporating electronic/experimental music, mod, disco and pop. It
      subsequently engendered subgenres and fusions, including New Romantic and gothic rock.
      &lt;p&gt; New wave differs from other movements with ties to first-wave punk as it displays
      characteristics common to pop music, rather than the more &quot;arty&quot; post-punk, though
      it incorporates much of the original punk rock sound and ethos while arguably exhibiting
      greater complexity in both music and lyrics. Common characteristics of new wave music, aside
      from its punk influences, include the use of synthesizers and electronic productions, the
      importance of styling and the arts, as well as a great amount of diversity. &lt;p&gt; New wave
      has been called one of the definitive genres of the 1980s, after it grew partially fixated on
      MTV. and the popularity of several new wave artists, attributing the exposure that was given
      to them by the channel.</skos:definition>
    <skos:exactMatch xml:lang="en">http://dbpedia.org/resource/New_wave_music</skos:exactMatch>
    <skos:inScheme rdf:resource="http://data.europeana.eu/concept/music/genre/Music_Genre_Scheme"/>
    <skos:altLabel xml:lang="en">New Wave music</skos:altLabel>
    <skos:altLabel xml:lang="en">New Wave</skos:altLabel>
  </skos:Concept>

  <skos:Concept rdf:about="http://data.europeana.eu/concept/music/genre/Pansori">
    <skos:prefLabel xml:lang="en">Pansori</skos:prefLabel>
    <skos:prefLabel xml:lang="nl">Pansori</skos:prefLabel>
    <skos:prefLabel xml:lang="fi">Pansori</skos:prefLabel>
    <skos:prefLabel xml:lang="fr">Pansori</skos:prefLabel>
    <skos:prefLabel xml:lang="de">Pansori</skos:prefLabel>
    <skos:prefLabel xml:lang="hu">Phanszori</skos:prefLabel>
    <skos:prefLabel xml:lang="id">Pansori</skos:prefLabel>
    <skos:prefLabel xml:lang="it">Pansori</skos:prefLabel>
    <skos:prefLabel xml:lang="ja">パンソリ</skos:prefLabel>
    <skos:prefLabel xml:lang="ko">판소리</skos:prefLabel>
    <skos:prefLabel xml:lang="fa">پانسوری</skos:prefLabel>
    <skos:prefLabel xml:lang="pl">Pansori</skos:prefLabel>
    <skos:prefLabel xml:lang="ru">Пхансори</skos:prefLabel>
    <skos:prefLabel xml:lang="es">Pansori</skos:prefLabel>
    <skos:prefLabel xml:lang="vi">Hát kể Pansori</skos:prefLabel>
    <skos:closeMatch rdf:resource="http://rdf.freebase.com/ns/m.02vwm_"/>
    <skos:broader
      rdf:resource="http://data.europeana.eu/concept/music/genre/Music_of_Asia_traditional"/>
    <skos:definition xml:lang="en">Pansori is a Korean genre of musical storytelling performed by a
      vocalist and a drummer. The music is usually performed by one sorikkun and one gosu. The term
      pansori is derived from pan, and sori.</skos:definition>
    <skos:exactMatch xml:lang="en">http://dbpedia.org/resource/Pansori</skos:exactMatch>
    <skos:inScheme rdf:resource="http://data.europeana.eu/concept/music/genre/Music_Genre_Scheme"/>
    <skos:altLabel xml:lang="en">Pansori</skos:altLabel>
  </skos:Concept>

  <skos:Concept rdf:about="http://data.europeana.eu/concept/music/genre/Rai">
    <skos:prefLabel xml:lang="en">Raï</skos:prefLabel>
    <skos:prefLabel xml:lang="ar">راي</skos:prefLabel>
    <skos:prefLabel xml:lang="nl">Rai</skos:prefLabel>
    <skos:prefLabel xml:lang="fi">Rai</skos:prefLabel>
    <skos:prefLabel xml:lang="fr">Raï</skos:prefLabel>
    <skos:prefLabel xml:lang="de">Raï</skos:prefLabel>
    <skos:prefLabel xml:lang="hu">Rai</skos:prefLabel>
    <skos:prefLabel xml:lang="id">Rai</skos:prefLabel>
    <skos:prefLabel xml:lang="it">Raï</skos:prefLabel>
    <skos:prefLabel xml:lang="ja">ライ</skos:prefLabel>
    <skos:prefLabel xml:lang="ko">라이</skos:prefLabel>
    <skos:prefLabel xml:lang="ms">Raï</skos:prefLabel>
    <skos:prefLabel xml:lang="pl">Raï</skos:prefLabel>
    <skos:prefLabel xml:lang="pt">Raï</skos:prefLabel>
    <skos:prefLabel xml:lang="ro">Raï</skos:prefLabel>
    <skos:prefLabel xml:lang="ru">Раи</skos:prefLabel>
    <skos:prefLabel xml:lang="es">Raï</skos:prefLabel>
    <skos:prefLabel xml:lang="sv">Raï</skos:prefLabel>
    <skos:prefLabel xml:lang="tr">Raï</skos:prefLabel>
    <skos:closeMatch rdf:resource="http://rdf.freebase.com/ns/m.016zdv"/>
    <skos:broader rdf:resource="http://data.europeana.eu/concept/music/genre/African_popular_music"/>
    <skos:definition xml:lang="en">Raï is a form of folk music that originated in Oran, Algeria from
      Bedouin shepherds, mixed with Spanish, French, African and Arabic musical forms, which dates
      back to the 1930s. &lt;p&gt; Singers of raï are called cheb as opposed to sheikh, the name
      given to Chaabi singers. The tradition arose in cities like Oran, Relizane, Mostaganem, Chlef
      and Sidi-Bel-Abbès, primarily among the poor. Traditionally sung by men, by the end of the
      20th century, female singers had become common. The lyrics of raï have concerned social
      issues, such as disease and the policing of European colonies, that affected native
      populations.</skos:definition>
    <skos:exactMatch xml:lang="en">http://dbpedia.org/resource/Ra%C3%AF</skos:exactMatch>
    <skos:inScheme rdf:resource="http://data.europeana.eu/concept/music/genre/Music_Genre_Scheme"/>
    <skos:altLabel xml:lang="en">Rai</skos:altLabel>
    <skos:altLabel xml:lang="en">Raï</skos:altLabel>
  </skos:Concept>

  <skos:Concept rdf:about="http://data.europeana.eu/concept/music/genre/Hip_hop_music">
    <skos:prefLabel xml:lang="en">Rap</skos:prefLabel>
    <skos:prefLabel xml:lang="ar">هيب هوب</skos:prefLabel>
    <skos:prefLabel xml:lang="bg">Хип-хоп музика</skos:prefLabel>
    <skos:prefLabel xml:lang="ca">Hip hop</skos:prefLabel>
    <skos:prefLabel xml:lang="hr">Hip-hop glazba</skos:prefLabel>
    <skos:prefLabel xml:lang="cs">Hip hop</skos:prefLabel>
    <skos:prefLabel xml:lang="da">Hiphop</skos:prefLabel>
    <skos:prefLabel xml:lang="nl">Hiphop</skos:prefLabel>
    <skos:prefLabel xml:lang="et">Hiphop</skos:prefLabel>
    <skos:prefLabel xml:lang="fi">Hip hop</skos:prefLabel>
    <skos:prefLabel xml:lang="fr">Hip-hop</skos:prefLabel>
    <skos:prefLabel xml:lang="de">Hip-Hop</skos:prefLabel>
    <skos:prefLabel xml:lang="el">Χιπ χοπ</skos:prefLabel>
    <skos:prefLabel xml:lang="hi">हिप हॉप संगीत</skos:prefLabel>
    <skos:prefLabel xml:lang="hu">Hiphop</skos:prefLabel>
    <skos:prefLabel xml:lang="id">Hip-hop</skos:prefLabel>
    <skos:prefLabel xml:lang="it">Hip hop</skos:prefLabel>
    <skos:prefLabel xml:lang="ja">ヒップホップ</skos:prefLabel>
    <skos:prefLabel xml:lang="ko">힙합 음악</skos:prefLabel>
    <skos:prefLabel xml:lang="lv">Hiphops</skos:prefLabel>
    <skos:prefLabel xml:lang="lt">Hiphopas</skos:prefLabel>
    <skos:prefLabel xml:lang="ms">Hip hop</skos:prefLabel>
    <skos:prefLabel xml:lang="no">Hiphop</skos:prefLabel>
    <skos:prefLabel xml:lang="fa">موسیقی هیپ هاپ</skos:prefLabel>
    <skos:prefLabel xml:lang="pl">Hip-hop</skos:prefLabel>
    <skos:prefLabel xml:lang="pt">Hip hop</skos:prefLabel>
    <skos:prefLabel xml:lang="ro">Muzică hip hop</skos:prefLabel>
    <skos:prefLabel xml:lang="ru">Хип-хоп</skos:prefLabel>
    <skos:prefLabel xml:lang="sr">Хип хоп</skos:prefLabel>
    <skos:prefLabel xml:lang="sk">Hip-hop</skos:prefLabel>
    <skos:prefLabel xml:lang="sl">Hip-hop</skos:prefLabel>
    <skos:prefLabel xml:lang="es">Hip hop</skos:prefLabel>
    <skos:prefLabel xml:lang="sv">Hiphop</skos:prefLabel>
    <skos:prefLabel xml:lang="th">ฮิปฮอป</skos:prefLabel>
    <skos:prefLabel xml:lang="tr">Hip hop</skos:prefLabel>
    <skos:prefLabel xml:lang="uk">Хіп-хоп</skos:prefLabel>
    <skos:prefLabel xml:lang="vi">Hip hop</skos:prefLabel>
    <skos:closeMatch rdf:resource="http://rdf.freebase.com/ns/m.0glt670"/>
    <skos:broader rdf:resource="http://data.europeana.eu/concept/music/genre/Popular_music"/>
    <skos:definition xml:lang="en">Hip hop music, also called hip-hop, rap music, or hip-hop music,
      is a music genre consisting of a stylized rhythmic music that commonly accompanies rapping, a
      rhythmic and rhyming speech that is chanted. It developed as part of hip hop culture, a
      subculture defined by four key stylistic elements: MCing/rapping, DJing/scratching, break
      dancing, and graffiti writing. Other elements include sampling, and beatboxing. &lt;p&gt;
      While often used to refer to rapping, &quot;hip hop&quot; more properly denotes the practice
      of the entire subculture. The term hip hop music is sometimes used synonymously with the term
      rap music, though rapping is not a required component of hip hop music, the genre may also
      incorporate other elements of hip hop culture, including DJing and scratching, beatboxing, and
      instrumental tracks.</skos:definition>
    <skos:exactMatch xml:lang="en">http://dbpedia.org/resource/Hip_hop_music</skos:exactMatch>
    <skos:inScheme rdf:resource="http://data.europeana.eu/concept/music/genre/Music_Genre_Scheme"/>
    <skos:altLabel xml:lang="en">Hip hop music</skos:altLabel>
  </skos:Concept>

  <skos:Concept rdf:about="http://data.europeana.eu/concept/music/genre/Rautalanka">
    <skos:prefLabel xml:lang="en">Rautalanka</skos:prefLabel>
    <skos:prefLabel xml:lang="fi">Rautalankamusiikki</skos:prefLabel>
    <skos:prefLabel xml:lang="ru">Рауталанка</skos:prefLabel>
    <skos:closeMatch rdf:resource="http://rdf.freebase.com/ns/m.027jy3r"/>
    <skos:broader rdf:resource="http://data.europeana.eu/concept/music/genre/Surf_music"/>
    <skos:definition xml:lang="en">In common usage the Finnish word rautalanka means instrumental
      rock in general. Some enthusiasts use the term more narrowly to refer to the somewhat distinct
      style of playing it that has developed in Finland over the years. This article is written from
      that more narrow point of view. &lt;p&gt; Rautalanka is typically played by a quartet
      consisting of a lead guitar, rhythm guitar, bass guitar and drum kit. Rautalanka music can
      also include other instruments and vocals. The heyday of rautalanka was in the early 1960s,
      but it has enthusiasts even today. Typical features of rautalanka are sharp and clear
      melodies, fast tempos and extensive use of tape echo, but little or no overdrive or fuzz. What
      distinguishes rautalanka most clearly from other twangy guitar genres is that the melodies
      tend to be in minor keys and melancholic, based on folk tunes and schlager
      songs.</skos:definition>
    <skos:exactMatch xml:lang="en">http://dbpedia.org/resource/Rautalanka</skos:exactMatch>
    <skos:inScheme rdf:resource="http://data.europeana.eu/concept/music/genre/Music_Genre_Scheme"/>
    <skos:altLabel xml:lang="en">Rautalanka</skos:altLabel>
  </skos:Concept>

  <skos:Concept rdf:about="http://data.europeana.eu/concept/music/genre/Revue">
    <skos:prefLabel xml:lang="en">Revue</skos:prefLabel>
    <skos:closeMatch
      rdf:resource="http://data.europeana.eu/concept/music/genre/+http%3A%2F%2Frdf.freebase.com%2Fns%2Fm.03bldk"/>
    <skos:broader rdf:resource="http://data.europeana.eu/concept/music/genre/Art_music"/>
    <skos:definition xml:lang="en">A revue is a type of multi-act popular theatrical entertainment
      that combines music, dance and sketches. The revue has its roots in 19th century American
      popular entertainment and melodrama but grew into a substantial cultural presence of its own
      during its golden years from 1916 to 1932. Though most famous for their visual spectacle,
      revues frequently satirized contemporary figures, news or literature. Due to high ticket
      prices, ribald publicity campaigns and the occasional use of prurient material, the revue was
      typically patronized by audience members who earned even more and felt even less restricted by
      middle-class social mores than their contemporaries in vaudeville. Like much of that era's
      popular entertainments, revues often featured material based on sophisticated, irreverent
      dissections of topical matter, public personae and fads, though the primary attraction was
      found in the frank display of the female body.</skos:definition>
    <skos:exactMatch xml:lang="en">http://dbpedia.org/resource/Revue</skos:exactMatch>
    <skos:inScheme rdf:resource="http://data.europeana.eu/concept/music/genre/Music_Genre_Scheme"/>
  </skos:Concept>

  <skos:Concept rdf:about="http://data.europeana.eu/concept/music/genre/Rocksteady">
    <skos:prefLabel xml:lang="en">Rock steady</skos:prefLabel>
    <skos:prefLabel xml:lang="ca">Rocksteady</skos:prefLabel>
    <skos:prefLabel xml:lang="cs">Rocksteady</skos:prefLabel>
    <skos:prefLabel xml:lang="nl">Rocksteady</skos:prefLabel>
    <skos:prefLabel xml:lang="fi">Rocksteady</skos:prefLabel>
    <skos:prefLabel xml:lang="fr">Rocksteady</skos:prefLabel>
    <skos:prefLabel xml:lang="de">Rocksteady</skos:prefLabel>
    <skos:prefLabel xml:lang="id">Rocksteady</skos:prefLabel>
    <skos:prefLabel xml:lang="it">Rocksteady</skos:prefLabel>
    <skos:prefLabel xml:lang="ja">ロックステディ</skos:prefLabel>
    <skos:prefLabel xml:lang="pl">Rocksteady</skos:prefLabel>
    <skos:prefLabel xml:lang="pt">Rocksteady</skos:prefLabel>
    <skos:prefLabel xml:lang="ru">Рокстеди</skos:prefLabel>
    <skos:prefLabel xml:lang="sk">Rocksteady</skos:prefLabel>
    <skos:prefLabel xml:lang="es">Rocksteady</skos:prefLabel>
    <skos:prefLabel xml:lang="sv">Rocksteady</skos:prefLabel>
    <skos:prefLabel xml:lang="uk">Рокстеді</skos:prefLabel>
    <skos:closeMatch rdf:resource="http://rdf.freebase.com/ns/m.019z2l"/>
    <skos:broader rdf:resource="http://data.europeana.eu/concept/music/genre/Ska"/>
    <skos:definition xml:lang="en">Rocksteady is a music genre that originated in Jamaica around
      1966. A successor to ska and a precursor to reggae, rocksteady was performed by Jamaican vocal
      harmony groups such as The Gaylads, The Maytals, The Heptones and The Paragons. The term
      rocksteady comes from a dance style that was mentioned in the Alton Ellis song &quot;Rock
      Steady&quot;. Dances performed to rocksteady were less energetic than the earlier ska dances.
      The first international rocksteady hit was &quot;Hold Me Tight&quot; by the American soul
      singer Johnny Nash, it reached number one in Canada.</skos:definition>
    <skos:exactMatch xml:lang="en">http://dbpedia.org/resource/Rocksteady</skos:exactMatch>
    <skos:inScheme rdf:resource="http://data.europeana.eu/concept/music/genre/Music_Genre_Scheme"/>
    <skos:altLabel xml:lang="en">Rocksteady</skos:altLabel>
  </skos:Concept>

  <skos:Concept rdf:about="http://data.europeana.eu/concept/music/genre/Sevillanas">
    <skos:prefLabel xml:lang="en">Sevillana</skos:prefLabel>
    <skos:prefLabel xml:lang="ca">Sevillana</skos:prefLabel>
    <skos:prefLabel xml:lang="cs">Sevillanas</skos:prefLabel>
    <skos:prefLabel xml:lang="nl">Sevillana</skos:prefLabel>
    <skos:prefLabel xml:lang="fr">Sevillana</skos:prefLabel>
    <skos:prefLabel xml:lang="de">Sevillanas</skos:prefLabel>
    <skos:prefLabel xml:lang="it">Sevillana</skos:prefLabel>
    <skos:prefLabel xml:lang="ja">セビジャーナス</skos:prefLabel>
    <skos:prefLabel xml:lang="no">Sevillanas</skos:prefLabel>
    <skos:prefLabel xml:lang="pt">Sevilhanas</skos:prefLabel>
    <skos:prefLabel xml:lang="es">Sevillanas</skos:prefLabel>
    <skos:prefLabel xml:lang="sv">Sevillana</skos:prefLabel>
    <skos:closeMatch rdf:resource="http://rdf.freebase.com/ns/m.0334f1"/>
    <skos:broader rdf:resource="http://data.europeana.eu/concept/music/genre/Folk_music_traditional"/>
    <skos:definition xml:lang="en">Sevillanas are a type of folk music and dance of Seville and its
      region. They were derived from the Seguidilla, an old Castilian folk music and dance genre. In
      the nineteenth century they were influenced by Flamenco. They have a relatively limited
      musical pattern but are rich in lyrics based on country life, virgins, country towns,
      neighborhoods, pilgrimage, and love themes. They are sung by a plethora of local groups, like
      the Los Romeros de la Puebla, Los Amigos de Gines, Las Corraleras de Lebrija, Cantores de
      Hispalis, and Los del Río. Every year, dozens of new sevillanas on CD are published. &lt;p&gt;
      Sevillanas can be heard mainly in fairs and festivals, including the famous Seville Fair, La
      Feria de Sevilla. There is an associated dance for the music: &quot;Baile por
      sevillanas&quot;, consisting of four different parts. One can find schools teaching
      &quot;baile por sevillanas&quot; in nearly every town in Spain. &lt;p&gt; Generally speaking,
      a sevillana is very lightheated, happy music.</skos:definition>
    <skos:exactMatch xml:lang="en">http://dbpedia.org/resource/Sevillanas</skos:exactMatch>
    <skos:inScheme rdf:resource="http://data.europeana.eu/concept/music/genre/Music_Genre_Scheme"/>
    <skos:altLabel xml:lang="en">Sevillanas</skos:altLabel>
  </skos:Concept>

  <skos:Concept rdf:about="http://data.europeana.eu/concept/music/genre/Shomyo">
    <skos:prefLabel xml:lang="en">Shomyo</skos:prefLabel>
    <skos:prefLabel xml:lang="fr">Shōmyō</skos:prefLabel>
    <skos:prefLabel xml:lang="de">Shōmyō</skos:prefLabel>
    <skos:prefLabel xml:lang="it">Shōmyō</skos:prefLabel>
    <skos:prefLabel xml:lang="ja">声明</skos:prefLabel>
    <skos:prefLabel xml:lang="es">Shōmyō</skos:prefLabel>
    <skos:closeMatch rdf:resource="http://rdf.freebase.com/ns/m.030cx7"/>
    <skos:broader rdf:resource="http://data.europeana.eu/concept/music/genre/Religious_music"/>
    <skos:definition xml:lang="en">Shōmyō is a style of Japanese Buddhist chant, used mainly in the
      Tendai and Shingon sects. There are two styles: ryokyoku and rikkyoku, described as difficult
      and easy to remember, respectively. &lt;p&gt; Sh?my?, like gagaku, employs the Yo scale, a
      pentatonic scale with ascending intervals of two, three, two, two, and three
      semitones.</skos:definition>
    <skos:exactMatch xml:lang="en">http://dbpedia.org/resource/Shomyo</skos:exactMatch>
    <skos:inScheme rdf:resource="http://data.europeana.eu/concept/music/genre/Music_Genre_Scheme"/>
    <skos:altLabel xml:lang="en">Shōmyō</skos:altLabel>
  </skos:Concept>

  <skos:Concept rdf:about="http://data.europeana.eu/concept/music/genre/Sinawi">
    <skos:prefLabel xml:lang="en">Sinawe</skos:prefLabel>
    <skos:prefLabel xml:lang="id">Sinawi</skos:prefLabel>
    <skos:prefLabel xml:lang="ko">시나위</skos:prefLabel>
    <skos:closeMatch rdf:resource="http://rdf.freebase.com/ns/m.06zp5r"/>
    <skos:broader
      rdf:resource="http://data.europeana.eu/concept/music/genre/Music_of_Asia_traditional"/>
    <skos:definition xml:lang="en">Sinawi, sometimes spelled shinawi, is a traditional form of
      Korean music. It is performed improvisationally by a musical ensemble, and traditionally
      accompanies the rites of Korean shamanism. The style first emerged in the Chungcheong and
      Jeolla provinces, but is now widespread. The traditional sinawi ensemble followed the
      principle of sam-hyeon-yuk-gak, with two flutes, a haegeum, a daegeum, a janggu
      hourglass-drum, and a large buk drum. However, today other traditional Korean instruments such
      as the gayageum and geomungo are also often included.</skos:definition>
    <skos:exactMatch xml:lang="en">http://dbpedia.org/resource/Sinawi</skos:exactMatch>
    <skos:inScheme rdf:resource="http://data.europeana.eu/concept/music/genre/Music_Genre_Scheme"/>
    <skos:altLabel xml:lang="en">Sinawi</skos:altLabel>
  </skos:Concept>

  <skos:Concept rdf:about="http://data.europeana.eu/concept/music/genre/Orchestra">
    <skos:prefLabel xml:lang="en">Symphony</skos:prefLabel>
    <skos:prefLabel xml:lang="ar">أوركسترا</skos:prefLabel>
    <skos:prefLabel xml:lang="bg">Оркестър</skos:prefLabel>
    <skos:prefLabel xml:lang="ca">Orquestra</skos:prefLabel>
    <skos:prefLabel xml:lang="hr">Orkestar</skos:prefLabel>
    <skos:prefLabel xml:lang="cs">Orchestr</skos:prefLabel>
    <skos:prefLabel xml:lang="da">Orkester</skos:prefLabel>
    <skos:prefLabel xml:lang="nl">Orkest</skos:prefLabel>
    <skos:prefLabel xml:lang="et">Orkester</skos:prefLabel>
    <skos:prefLabel xml:lang="fil">Orkestra</skos:prefLabel>
    <skos:prefLabel xml:lang="fi">Orkesteri</skos:prefLabel>
    <skos:prefLabel xml:lang="fr">Orchestre</skos:prefLabel>
    <skos:prefLabel xml:lang="de">Orchester</skos:prefLabel>
    <skos:prefLabel xml:lang="el">Ορχήστρα</skos:prefLabel>
    <skos:prefLabel xml:lang="hu">Zenekar</skos:prefLabel>
    <skos:prefLabel xml:lang="id">Orkestra</skos:prefLabel>
    <skos:prefLabel xml:lang="it">Orchestra</skos:prefLabel>
    <skos:prefLabel xml:lang="ja">オーケストラ</skos:prefLabel>
    <skos:prefLabel xml:lang="ko">관현악단</skos:prefLabel>
    <skos:prefLabel xml:lang="lv">Orķestris</skos:prefLabel>
    <skos:prefLabel xml:lang="lt">Orkestras</skos:prefLabel>
    <skos:prefLabel xml:lang="ms">Orkestra</skos:prefLabel>
    <skos:prefLabel xml:lang="no">Orkester</skos:prefLabel>
    <skos:prefLabel xml:lang="fa">ارکستر</skos:prefLabel>
    <skos:prefLabel xml:lang="pl">Orkiestra</skos:prefLabel>
    <skos:prefLabel xml:lang="pt">Orquestra</skos:prefLabel>
    <skos:prefLabel xml:lang="ro">Orchestră</skos:prefLabel>
    <skos:prefLabel xml:lang="ru">Оркестр</skos:prefLabel>
    <skos:prefLabel xml:lang="sr">Оркестар</skos:prefLabel>
    <skos:prefLabel xml:lang="sk">Orchester</skos:prefLabel>
    <skos:prefLabel xml:lang="sl">Orkester</skos:prefLabel>
    <skos:prefLabel xml:lang="es">Orquesta</skos:prefLabel>
    <skos:prefLabel xml:lang="sv">Orkester</skos:prefLabel>
    <skos:prefLabel xml:lang="th">วงออร์เคสตรา</skos:prefLabel>
    <skos:prefLabel xml:lang="tr">Orkestra</skos:prefLabel>
    <skos:prefLabel xml:lang="uk">Оркестр</skos:prefLabel>
    <skos:prefLabel xml:lang="vi">Dàn nhạc giao hưởng</skos:prefLabel>
    <skos:closeMatch rdf:resource="http://rdf.freebase.com/ns/m.05pd6"/>
    <skos:broader rdf:resource="http://data.europeana.eu/concept/music/genre/Classical_music"/>
    <skos:definition xml:lang="en">Of, relating to, or composed for an orchestra. Suggestive of an
      orchestra or its musical qualities.</skos:definition>
    <skos:exactMatch xml:lang="en">http://dbpedia.org/resource/Orchestra</skos:exactMatch>
    <skos:inScheme rdf:resource="http://data.europeana.eu/concept/music/genre/Music_Genre_Scheme"/>
    <skos:altLabel xml:lang="en">Orchestra</skos:altLabel>
    <skos:altLabel xml:lang="en">Orchestral</skos:altLabel>
  </skos:Concept>

  <skos:Concept rdf:about="http://data.europeana.eu/concept/music/genre/Music_of_Ecuador_Albazo">
    <skos:prefLabel xml:lang="en">Albazo</skos:prefLabel>
    <skos:broader
      rdf:resource="http://data.europeana.eu/concept/music/genre/Latin_American_music_traditional"/>
    <skos:definition xml:lang="en">The music of Ecuador has a long history. Pasillo is a genre of
      indigenous Latin music. In Ecuador it is the &quot;national genre of music.&quot; Through the
      years, many cultures have brought their influences together to create new types of music.
      There are also different kinds of traditional music like albazo, pasacalle, fox incaico,
      tonada, diablada pillareña, capishca, Bomba (highly established in afro-Ecuadorian society in
      cities such as Esmeraldas), and so on.</skos:definition>
    <skos:exactMatch xml:lang="en"
      >http://dbpedia.org/resource/Music_of_Ecuador#Albazo</skos:exactMatch>
    <skos:inScheme rdf:resource="http://data.europeana.eu/concept/music/genre/Music_Genre_Scheme"/>
  </skos:Concept>

  <skos:Concept rdf:about="http://data.europeana.eu/concept/music/genre/Ayarachi">
    <skos:prefLabel xml:lang="en">Ayarachi</skos:prefLabel>
    <skos:broader
      rdf:resource="http://data.europeana.eu/concept/music/genre/Latin_American_music_traditional"/>
    <skos:definition xml:lang="en">Indigen dance in Quenchua region, Peru.</skos:definition>
    <skos:broadMatch rdf:resource="http://es.dbpedia.org/page/Ayarachi"/>
    <skos:inScheme rdf:resource="http://data.europeana.eu/concept/music/genre/Music_Genre_Scheme"/>
  </skos:Concept>

  <skos:Concept rdf:about="http://data.europeana.eu/concept/music/genre/Bailecito">
    <skos:prefLabel xml:lang="en">Bailecito</skos:prefLabel>
    <skos:broader
      rdf:resource="http://data.europeana.eu/concept/music/genre/Latin_American_music_traditional"/>
    <skos:definition xml:lang="en">Specific folcloric dance of Blolivia and
      Argentina</skos:definition>
    <skos:broadMatch rdf:resource="http://es.dbpedia.org/page/Bailecito"/>
    <skos:inScheme rdf:resource="http://data.europeana.eu/concept/music/genre/Music_Genre_Scheme"/>
  </skos:Concept>

  <skos:Concept rdf:about="http://data.europeana.eu/concept/music/genre/Ballet">
    <skos:prefLabel xml:lang="en">Ballet</skos:prefLabel>
    <skos:prefLabel xml:lang="ar">باليه</skos:prefLabel>
    <skos:prefLabel xml:lang="bg">Балет</skos:prefLabel>
    <skos:prefLabel xml:lang="ca">Ballet</skos:prefLabel>
    <skos:prefLabel xml:lang="hr">Balet</skos:prefLabel>
    <skos:prefLabel xml:lang="cs">Balet</skos:prefLabel>
    <skos:prefLabel xml:lang="da">Ballet</skos:prefLabel>
    <skos:prefLabel xml:lang="nl">Ballet</skos:prefLabel>
    <skos:prefLabel xml:lang="et">Ballett</skos:prefLabel>
    <skos:prefLabel xml:lang="fil">Ballet</skos:prefLabel>
    <skos:prefLabel xml:lang="fi">Baletti</skos:prefLabel>
    <skos:prefLabel xml:lang="fr">Ballet</skos:prefLabel>
    <skos:prefLabel xml:lang="de">Ballett</skos:prefLabel>
    <skos:prefLabel xml:lang="el">Μπαλέτο</skos:prefLabel>
    <skos:prefLabel xml:lang="hi">बैले</skos:prefLabel>
    <skos:prefLabel xml:lang="hu">Balett</skos:prefLabel>
    <skos:prefLabel xml:lang="id">Balet</skos:prefLabel>
    <skos:prefLabel xml:lang="it">Balletto</skos:prefLabel>
    <skos:prefLabel xml:lang="ja">バレエ</skos:prefLabel>
    <skos:prefLabel xml:lang="ko">발레</skos:prefLabel>
    <skos:prefLabel xml:lang="lv">Balets</skos:prefLabel>
    <skos:prefLabel xml:lang="lt">Baletas</skos:prefLabel>
    <skos:prefLabel xml:lang="ms">Balet</skos:prefLabel>
    <skos:prefLabel xml:lang="no">Ballett</skos:prefLabel>
    <skos:prefLabel xml:lang="fa">رقص باله</skos:prefLabel>
    <skos:prefLabel xml:lang="pl">Balet</skos:prefLabel>
    <skos:prefLabel xml:lang="pt">Balé</skos:prefLabel>
    <skos:prefLabel xml:lang="ro">Balet</skos:prefLabel>
    <skos:prefLabel xml:lang="ru">Балет</skos:prefLabel>
    <skos:prefLabel xml:lang="sr">Балет</skos:prefLabel>
    <skos:prefLabel xml:lang="sk">Balet</skos:prefLabel>
    <skos:prefLabel xml:lang="sl">Balet</skos:prefLabel>
    <skos:prefLabel xml:lang="es">Ballet</skos:prefLabel>
    <skos:prefLabel xml:lang="sv">Balett</skos:prefLabel>
    <skos:prefLabel xml:lang="th">บัลเลต์</skos:prefLabel>
    <skos:prefLabel xml:lang="tr">Bale</skos:prefLabel>
    <skos:prefLabel xml:lang="uk">Балет</skos:prefLabel>
    <skos:prefLabel xml:lang="vi">Múa Ba Lê</skos:prefLabel>
    <skos:closeMatch rdf:resource="http://rdf.freebase.com/ns/m.0d6n1"/>
    <skos:broader rdf:resource="http://data.europeana.eu/concept/music/genre/Classical_music"/>
    <skos:definition xml:lang="en">Ballet is a type of performance dance that originated in the
      Italian Renaissance courts of the 15th century and later developed into a concert dance form
      in France and Russia. It has since become a widespread, highly technical form of dance with
      its own vocabulary based on French terminology. It has been globally influential and has
      defined the foundational techniques used in many other dance genres. Ballet requires years of
      training to learn and master, and much practice to retain proficiency. It has been taught in
      ballet schools around the world, which have historically used their own cultures to evolve the
      art. &lt;p&gt; Ballet may also refer to a ballet dance work, which consists of the
      choreography and music for a ballet production. A well-known example of this is The
      Nutcracker, a two-act ballet that was originally choreographed by Marius Petipa and Lev Ivanov
      with a music score by Pyotr Ilyich Tchaikovsky. Ballet dance works are choreographed and
      performed by trained artists. Many classical ballet works are performed with classical music
      accompaniment and are theatrical and use elaborate costumes and staging, though there are
      exceptions to this, such as works by George Balanchine.</skos:definition>
    <skos:exactMatch xml:lang="en">http://dbpedia.org/resource/Ballet</skos:exactMatch>
    <skos:inScheme rdf:resource="http://data.europeana.eu/concept/music/genre/Music_Genre_Scheme"/>
    <skos:altLabel xml:lang="en">Ballet</skos:altLabel>
  </skos:Concept>

  <skos:Concept rdf:about="http://data.europeana.eu/concept/music/genre/Music_of_Punjab">
    <skos:prefLabel xml:lang="en">Folk music of Punjab</skos:prefLabel>
    <skos:closeMatch rdf:resource="http://rdf.freebase.com/ns/m.0jwz750"/>
    <skos:broader
      rdf:resource="http://data.europeana.eu/concept/music/genre/Music_of_Asia_traditional"/>
    <skos:definition xml:lang="en">Mentioned in wikipedia in the topic Music of
      punjab</skos:definition>
    <skos:broadMatch rdf:resource="http://dbpedia.org/resource/Music_of_Punjab"/>
    <skos:inScheme rdf:resource="http://data.europeana.eu/concept/music/genre/Music_Genre_Scheme"/>
    <skos:altLabel xml:lang="en">Folk music of Punjab</skos:altLabel>
  </skos:Concept>

  <skos:Concept rdf:about="http://data.europeana.eu/concept/music/genre/Cachua">
    <skos:prefLabel xml:lang="en">Cachua</skos:prefLabel>
    <skos:prefLabel xml:lang="es">Cachua</skos:prefLabel>
    <skos:closeMatch rdf:resource="http://rdf.freebase.com/ns/m.0m0gsw8"/>
    <skos:broader
      rdf:resource="http://data.europeana.eu/concept/music/genre/Latin_American_music_traditional"/>
    <skos:definition xml:lang="en">The cachua is a term from Quechua language qhachwa, meaning
      &quot;round dance,&quot; that is the Spanish name for a Latin-American baroque dance form
      found mainly in Peru. It still exists today as a circle dance. The term was also applied to
      some villancicos to Spanish texts with cachua rhythm, such as two examples in a report
      submitted to Charles IV of Spain c.1788-1790. It is in rapid unsyncopated 2/4
      time.</skos:definition>
    <skos:exactMatch xml:lang="en">http://dbpedia.org/resource/Cachua</skos:exactMatch>
    <skos:inScheme rdf:resource="http://data.europeana.eu/concept/music/genre/Music_Genre_Scheme"/>
    <skos:altLabel xml:lang="en">Cachua</skos:altLabel>
  </skos:Concept>

  <skos:Concept rdf:about="http://data.europeana.eu/concept/music/genre/Carnavalito">
    <skos:prefLabel xml:lang="en">Carnavalito</skos:prefLabel>
    <skos:prefLabel xml:lang="fr">Carnavalito</skos:prefLabel>
    <skos:prefLabel xml:lang="it">Carnavalito</skos:prefLabel>
    <skos:prefLabel xml:lang="ja">カルナバリート</skos:prefLabel>
    <skos:prefLabel xml:lang="es">Carnavalito</skos:prefLabel>
    <skos:closeMatch rdf:resource="http://rdf.freebase.com/ns/m.080hjb5"/>
    <skos:broader
      rdf:resource="http://data.europeana.eu/concept/music/genre/Latin_American_music_traditional"/>
    <skos:definition xml:lang="en">The Carnavalito is a traditional South American dance from the
      altiplano and puna regions that is practiced in relation to religious festivities. The current
      form of the dance is an expression of syncretism between indigenous and Spanish colonial
      culture. &lt;p&gt; The Carnavalito was danced in the Americas long before the Spanish arrived.
      Today it is still danced in the Northwestern Argentina and in western Bolivia. The music is
      characterized by the use of instruments such as the quena, siku and the bombo, its origin
      comes from the Huayno, music similar to the Carnavalito.</skos:definition>
    <skos:exactMatch xml:lang="en">http://dbpedia.org/resource/Carnavalito</skos:exactMatch>
    <skos:inScheme rdf:resource="http://data.europeana.eu/concept/music/genre/Music_Genre_Scheme"/>
    <skos:altLabel xml:lang="en">Carnavalito</skos:altLabel>
  </skos:Concept>

  <skos:Concept rdf:about="http://data.europeana.eu/concept/music/genre/Cha-cha-cha_(music)">
    <skos:prefLabel xml:lang="en">Cha-cha-chá</skos:prefLabel>
    <skos:prefLabel xml:lang="pt">Chá-chá-chá</skos:prefLabel>
    <skos:closeMatch rdf:resource="http://rdf.freebase.com/ns/m.027wh_x"/>
    <skos:broader
      rdf:resource="http://data.europeana.eu/concept/music/genre/Latin_American_music_popular"/>
    <skos:definition xml:lang="en">Cha-cha-chá is a genre of Cuban music. It has been a popular
      dance music which developed from the danzón in the early 1950s, and became widely popular
      throughout Cuba and Mexico, New York.</skos:definition>
    <skos:exactMatch xml:lang="en">http://dbpedia.org/resource/Cha-cha-cha_(music)</skos:exactMatch>
    <skos:inScheme rdf:resource="http://data.europeana.eu/concept/music/genre/Music_Genre_Scheme"/>
    <skos:altLabel xml:lang="en">Cha-cha-cha</skos:altLabel>
  </skos:Concept>

  <skos:Concept
    rdf:about="http://data.europeana.eu/concept/music/genre/Music_of_Kashmir,_Jammu_and_Ladakh_Chakri">
    <skos:prefLabel xml:lang="en">Chakri</skos:prefLabel>
    <skos:broader
      rdf:resource="http://data.europeana.eu/concept/music/genre/Music_of_Asia_traditional"/>
    <skos:definition xml:lang="en"> a form of folk music in Kashmir</skos:definition>
    <skos:broadMatch rdf:resource="http://dbpedia.org/resource/Music_of_Kashmir,_Jammu_and_Ladakh"/>
    <skos:inScheme rdf:resource="http://data.europeana.eu/concept/music/genre/Music_Genre_Scheme"/>
  </skos:Concept>

  <skos:Concept rdf:about="http://data.europeana.eu/concept/music/genre/Chamame">
    <skos:prefLabel xml:lang="en">Chamamé</skos:prefLabel>
    <skos:prefLabel xml:lang="fr">Chamamé</skos:prefLabel>
    <skos:prefLabel xml:lang="de">Chamamé</skos:prefLabel>
    <skos:prefLabel xml:lang="ja">チャマメ</skos:prefLabel>
    <skos:prefLabel xml:lang="pt">Chamamé</skos:prefLabel>
    <skos:prefLabel xml:lang="es">Chamamé</skos:prefLabel>
    <skos:closeMatch rdf:resource="http://rdf.freebase.com/ns/m.0c56g5"/>
    <skos:broader
      rdf:resource="http://data.europeana.eu/concept/music/genre/Latin_American_music_traditional"/>
    <skos:definition xml:lang="en">Chámame is a folk music genre from the Argentine Northeast,
      Mesopotamia and the south of Brazil. Paraná, Santa Catarina, Rio Grande do Sul and Mato Grosso
      do Sul. &lt;p&gt; Jesuit Reductions in the area encouraged cultural growth that lasted until
      the Jesuits were expelled by the Spanish Crown in the late 18th century. Within this area,
      Yapeyú Corrientes was a centre of musical culture that many point to as the birthplace of the
      original Chamamé. Further mixing with instruments such as the Spanish guitar, then the violin
      and the accordion, finally resulted in what we currently know as &quot;Chamamé&quot;. There
      are recordings of Chamamé dating back to the early 20th century, and the term 'Chamamé' was
      already used in 1931, this type of music, prior to that, was often referred to as the
      Corrientes' Polka. &lt;p&gt; The Chamamé, originally schottische brought by the Volga German
      immigrants, has considerable Guaraní influence, mixed with the Spanish guitar and the European
      accordion from those immigrants that arrived in the area at the beginning of the 20th century.
      &lt;p&gt; Among chamamé figures of note are Raúl Barboza, Tarragó Ros, Antonio Tarragó Ros,
      Teresa Parodi, Ernesto Montiel, Tránsito Cocomarola, Mario Millán Medina, and modern musicians
      Chango Spasiuk, Zitto Segovia, Mario Bofill, Alejandro Brittes and Los Núñez con Ruiz
      Guiñazú.</skos:definition>
    <skos:exactMatch xml:lang="en">http://dbpedia.org/resource/Chamamé</skos:exactMatch>
    <skos:inScheme rdf:resource="http://data.europeana.eu/concept/music/genre/Music_Genre_Scheme"/>
    <skos:altLabel xml:lang="en">Chamame</skos:altLabel>
    <skos:altLabel xml:lang="en">Chamamé</skos:altLabel>
  </skos:Concept>

  <skos:Concept rdf:about="http://data.europeana.eu/concept/music/genre/Charleston_(dance)">
    <skos:prefLabel xml:lang="en">Charleston</skos:prefLabel>
    <skos:prefLabel xml:lang="bg">Чарлстон</skos:prefLabel>
    <skos:prefLabel xml:lang="ca">Xarleston</skos:prefLabel>
    <skos:prefLabel xml:lang="cs">Charleston</skos:prefLabel>
    <skos:prefLabel xml:lang="da">Charleston</skos:prefLabel>
    <skos:prefLabel xml:lang="nl">Charleston</skos:prefLabel>
    <skos:prefLabel xml:lang="fi">Charleston</skos:prefLabel>
    <skos:prefLabel xml:lang="fr">Charleston</skos:prefLabel>
    <skos:prefLabel xml:lang="de">Charleston</skos:prefLabel>
    <skos:prefLabel xml:lang="it">Charleston</skos:prefLabel>
    <skos:prefLabel xml:lang="ja">チャールストン</skos:prefLabel>
    <skos:prefLabel xml:lang="pl">Charleston</skos:prefLabel>
    <skos:prefLabel xml:lang="pt">Charleston</skos:prefLabel>
    <skos:prefLabel xml:lang="ru">Чарльстон</skos:prefLabel>
    <skos:prefLabel xml:lang="es">Charlestón</skos:prefLabel>
    <skos:prefLabel xml:lang="sv">Charleston</skos:prefLabel>
    <skos:prefLabel xml:lang="tr">Charleston</skos:prefLabel>
    <skos:prefLabel xml:lang="uk">Чарлстон</skos:prefLabel>
    <skos:closeMatch rdf:resource="http://rdf.freebase.com/ns/m.0g965"/>
    <skos:broader rdf:resource="http://data.europeana.eu/concept/music/genre/Americana_popular"/>
    <skos:definition xml:lang="en">The Charleston is a dance named for the harbor city of
      Charleston, South Carolina. The rhythm was popularized in mainstream dance music in the United
      States by a 1923 tune called &quot;The Charleston&quot; by composer/pianist James P. Johnson
      which originated in the Broadway show Runnin' Wild and became one of the most popular hits of
      the decade. Runnin' Wild ran from 29 October 1923 through 28 June 1924. The peak year for the
      Charleston as a dance by the public was mid-1926 to 1927.</skos:definition>
    <skos:exactMatch xml:lang="en">http://dbpedia.org/resource/Charleston_(dance)</skos:exactMatch>
    <skos:inScheme rdf:resource="http://data.europeana.eu/concept/music/genre/Music_Genre_Scheme"/>
    <skos:altLabel xml:lang="en">Charleston</skos:altLabel>
  </skos:Concept>

  <skos:Concept rdf:about="http://data.europeana.eu/concept/music/genre/Choro">
    <skos:prefLabel xml:lang="en">Choro</skos:prefLabel>
    <skos:prefLabel xml:lang="bg">Шору</skos:prefLabel>
    <skos:prefLabel xml:lang="ca">Xoro</skos:prefLabel>
    <skos:prefLabel xml:lang="fi">Choro</skos:prefLabel>
    <skos:prefLabel xml:lang="fr">Choro</skos:prefLabel>
    <skos:prefLabel xml:lang="de">Choro</skos:prefLabel>
    <skos:prefLabel xml:lang="it">Choro</skos:prefLabel>
    <skos:prefLabel xml:lang="ja">ショーロ</skos:prefLabel>
    <skos:prefLabel xml:lang="fa">شورو</skos:prefLabel>
    <skos:prefLabel xml:lang="pl">Choro</skos:prefLabel>
    <skos:prefLabel xml:lang="pt">Choro</skos:prefLabel>
    <skos:prefLabel xml:lang="ru">Шоро</skos:prefLabel>
    <skos:prefLabel xml:lang="es">Choro</skos:prefLabel>
    <skos:closeMatch rdf:resource="http://rdf.freebase.com/ns/m.02w1p3"/>
    <skos:broader
      rdf:resource="http://data.europeana.eu/concept/music/genre/Latin_American_music_popular"/>
    <skos:definition xml:lang="en">Choro, popularly called chorinho, is an instrumental Brazilian
      popular music genre which originated in 19th century Rio de Janeiro. Despite its name, the
      music often has a fast and happy rhythm. It is characterized by virtuosity, improvisation and
      subtle modulations, and is full of syncopation and counterpoint. Choro is considered the first
      characteristically Brazilian genre of urban popular music. The serenaders who play choros are
      known as chorões.</skos:definition>
    <skos:exactMatch xml:lang="en">http://dbpedia.org/resource/Choro</skos:exactMatch>
    <skos:inScheme rdf:resource="http://data.europeana.eu/concept/music/genre/Music_Genre_Scheme"/>
    <skos:altLabel xml:lang="en">chorinho</skos:altLabel>
    <skos:altLabel xml:lang="en">Choro</skos:altLabel>
  </skos:Concept>

  <skos:Concept rdf:about="http://data.europeana.eu/concept/music/genre/Danzon">
    <skos:prefLabel xml:lang="en">Danzón</skos:prefLabel>
    <skos:prefLabel xml:lang="ca">Danzón</skos:prefLabel>
    <skos:prefLabel xml:lang="fr">Danzón</skos:prefLabel>
    <skos:prefLabel xml:lang="de">Danzón</skos:prefLabel>
    <skos:prefLabel xml:lang="it">Danzón</skos:prefLabel>
    <skos:prefLabel xml:lang="ru">Дансон</skos:prefLabel>
    <skos:prefLabel xml:lang="es">Danzón</skos:prefLabel>
    <skos:prefLabel xml:lang="sv">Danzón</skos:prefLabel>
    <skos:closeMatch rdf:resource="http://rdf.freebase.com/ns/m.02p3xk"/>
    <skos:broader
      rdf:resource="http://data.europeana.eu/concept/music/genre/Latin_American_music_traditional"/>
    <skos:definition xml:lang="en">Danzón is the official musical genre and dance of Cuba. It is
      also an active musical form in Mexico and is still beloved in Puerto Rico. The danzón evolved
      from the Cuban contradanza. &lt;p&gt; The contradanza had English roots and was introduced in
      Cuba probably by the Spanish who ruled the island for almost four centuries and contributed
      thousands of immigrants over the centuries. Or, it is possible that it was introduced in 1762
      with the short-lived British invasion of Havana, or even through Haitian refugees. &lt;p&gt;
      In Cuba, these dances were influenced by African rhythmic and dance styles and so became a
      genuine fusion of European and African influences.</skos:definition>
    <skos:exactMatch xml:lang="en">http://dbpedia.org/resource/Danz%C3%B3n</skos:exactMatch>
    <skos:inScheme rdf:resource="http://data.europeana.eu/concept/music/genre/Music_Genre_Scheme"/>
    <skos:altLabel xml:lang="en">Danzon</skos:altLabel>
    <skos:altLabel xml:lang="en">Danzón</skos:altLabel>
  </skos:Concept>

  <skos:Concept rdf:about="http://data.europeana.eu/concept/music/genre/Festejo">
    <skos:prefLabel xml:lang="en">Festejo</skos:prefLabel>
    <skos:prefLabel xml:lang="nl">Festejo</skos:prefLabel>
    <skos:prefLabel xml:lang="es">Festejo</skos:prefLabel>
    <skos:closeMatch rdf:resource="http://rdf.freebase.com/ns/m.027z2gp"/>
    <skos:broader
      rdf:resource="http://data.europeana.eu/concept/music/genre/Latin_American_music_traditional"/>
    <skos:definition xml:lang="en">Festejo is a festive form of Peruvian music. It can be seen as a
      celebration of Perú's independence and the emancipation of slaves, or as an attempt to
      reinvent diaspora African music without reference to slavery. Composers of all races have
      contributed to the development of festejo repertoire. Its origins are in a competitive circle
      dance performed by men playing cajóns. Nowadays, people of all ages and races participate in a
      witty dance accompanying the festejo.</skos:definition>
    <skos:exactMatch xml:lang="en">http://dbpedia.org/resource/Festejo</skos:exactMatch>
    <skos:inScheme rdf:resource="http://data.europeana.eu/concept/music/genre/Music_Genre_Scheme"/>
    <skos:altLabel xml:lang="en">Festejo</skos:altLabel>
  </skos:Concept>

  <skos:Concept rdf:about="http://data.europeana.eu/concept/music/genre/Forro">
    <skos:prefLabel xml:lang="en">Forró</skos:prefLabel>
    <skos:prefLabel xml:lang="bg">Форо</skos:prefLabel>
    <skos:prefLabel xml:lang="ca">Forró</skos:prefLabel>
    <skos:prefLabel xml:lang="nl">Forró</skos:prefLabel>
    <skos:prefLabel xml:lang="fi">Forró</skos:prefLabel>
    <skos:prefLabel xml:lang="fr">Forró</skos:prefLabel>
    <skos:prefLabel xml:lang="de">Forró</skos:prefLabel>
    <skos:prefLabel xml:lang="it">Forró</skos:prefLabel>
    <skos:prefLabel xml:lang="no">Forró</skos:prefLabel>
    <skos:prefLabel xml:lang="pt">Forró</skos:prefLabel>
    <skos:prefLabel xml:lang="ru">Forró</skos:prefLabel>
    <skos:prefLabel xml:lang="es">Forró</skos:prefLabel>
    <skos:prefLabel xml:lang="sv">Forró</skos:prefLabel>
    <skos:prefLabel xml:lang="uk">Форро</skos:prefLabel>
    <skos:closeMatch rdf:resource="http://rdf.freebase.com/ns/m.05fqyx"/>
    <skos:broader
      rdf:resource="http://data.europeana.eu/concept/music/genre/Latin_American_music_traditional"/>
    <skos:definition xml:lang="en">Forró is a genre of Brazilian music that originated in
      Northeastern Brazil. It encompasses various dance styles as well as a number of different
      musical beats. This music genre has gained widespread popularity in all regions of Brazil.
      Forró is closely associated with Brazilian June Festivals, which celebrate a number of
      Christian saints. The most celebrated is Saint John's day.</skos:definition>
    <skos:exactMatch xml:lang="en">http://dbpedia.org/resource/Forr%C3%B3</skos:exactMatch>
    <skos:inScheme rdf:resource="http://data.europeana.eu/concept/music/genre/Music_Genre_Scheme"/>
    <skos:altLabel xml:lang="en">Forro</skos:altLabel>
    <skos:altLabel xml:lang="en">Forró</skos:altLabel>
  </skos:Concept>

  <skos:Concept
    rdf:about="http://data.europeana.eu/concept/music/genre/Music_of_Ecuador_Fox_incaico">
    <skos:prefLabel xml:lang="en">Fox incaico</skos:prefLabel>
    <skos:broader
      rdf:resource="http://data.europeana.eu/concept/music/genre/Latin_American_music_traditional"/>
    <skos:definition xml:lang="en">The music of Ecuador has a long history. Pasillo is a genre of
      indigenous Latin music. In Ecuador it is the &quot;national genre of music.&quot; Through the
      years, many cultures have brought their influences together to create new types of music.
      There are also different kinds of traditional music like albazo, pasacalle, fox incaico,
      tonada, diablada pillareña, capishca, Bomba</skos:definition>
    <skos:exactMatch xml:lang="en"
      >http://dbpedia.org/resource/Music_of_Ecuador#Fox_incaico</skos:exactMatch>
    <skos:inScheme rdf:resource="http://data.europeana.eu/concept/music/genre/Music_Genre_Scheme"/>
  </skos:Concept>

  <skos:Concept rdf:about="http://data.europeana.eu/concept/music/genre/Fugue">
    <skos:prefLabel xml:lang="en">Fugue</skos:prefLabel>
    <skos:prefLabel xml:lang="ar">فوغا</skos:prefLabel>
    <skos:prefLabel xml:lang="bg">Фуга</skos:prefLabel>
    <skos:prefLabel xml:lang="ca">Fuga</skos:prefLabel>
    <skos:prefLabel xml:lang="cs">Fuga</skos:prefLabel>
    <skos:prefLabel xml:lang="da">Fuga</skos:prefLabel>
    <skos:prefLabel xml:lang="nl">Fuga</skos:prefLabel>
    <skos:prefLabel xml:lang="et">Fuuga</skos:prefLabel>
    <skos:prefLabel xml:lang="fi">Fuuga</skos:prefLabel>
    <skos:prefLabel xml:lang="fr">Fugue</skos:prefLabel>
    <skos:prefLabel xml:lang="de">Fuge</skos:prefLabel>
    <skos:prefLabel xml:lang="el">Φούγκα</skos:prefLabel>
    <skos:prefLabel xml:lang="hu">Fúga</skos:prefLabel>
    <skos:prefLabel xml:lang="it">Fuga</skos:prefLabel>
    <skos:prefLabel xml:lang="ja">フーガ</skos:prefLabel>
    <skos:prefLabel xml:lang="ko">푸가</skos:prefLabel>
    <skos:prefLabel xml:lang="lt">Fuga</skos:prefLabel>
    <skos:prefLabel xml:lang="no">Fuge</skos:prefLabel>
    <skos:prefLabel xml:lang="fa">فوگ</skos:prefLabel>
    <skos:prefLabel xml:lang="pl">Fuga</skos:prefLabel>
    <skos:prefLabel xml:lang="pt">Fuga</skos:prefLabel>
    <skos:prefLabel xml:lang="ro">Fugă</skos:prefLabel>
    <skos:prefLabel xml:lang="ru">Фуга</skos:prefLabel>
    <skos:prefLabel xml:lang="sr">Фуга</skos:prefLabel>
    <skos:prefLabel xml:lang="sk">Fúga</skos:prefLabel>
    <skos:prefLabel xml:lang="sl">Fuga</skos:prefLabel>
    <skos:prefLabel xml:lang="es">Fuga</skos:prefLabel>
    <skos:prefLabel xml:lang="sv">Fuga</skos:prefLabel>
    <skos:prefLabel xml:lang="tr">Füg</skos:prefLabel>
    <skos:prefLabel xml:lang="uk">Фуга</skos:prefLabel>
    <skos:prefLabel xml:lang="vi">Tẩu pháp</skos:prefLabel>
    <skos:closeMatch rdf:resource="http://rdf.freebase.com/ns/m.02yb7"/>
    <skos:broader rdf:resource="http://data.europeana.eu/concept/music/genre/Classical_music"/>
    <skos:definition xml:lang="en">In music, a fugue is a contrapuntal compositional technique in
      two or more voices, built on a subject that is introduced at the beginning in imitation and
      recurs frequently in the course of the composition. &lt;p&gt; The English term fugue
      originated in the 16th century and is derived from the French word fugue or the Italian fuga.
      This in turn comes from Latin, also fuga, which is itself related to both fugere and fugare.
      The adjectival form is fugal. Variants include fughetta and fugato. &lt;p&gt; A fugue usually
      has three sections: an exposition, a development, and a recapitulation containing the return
      of the subject in the fugue's tonic key, though not all fugues have a recapitulation. In the
      Middle Ages, the term was widely used to denote any works in canonic style, by the
      Renaissance, it had come to denote specifically imitative works. Since the 17th century, the
      term fugue has described what is commonly regarded as the most fully developed procedure of
      imitative counterpoint. &lt;p&gt; Most fugues open with a short main theme, the subject, which
      then sounds successively in each voice, when each voice has entered, the exposition is
      complete.</skos:definition>
    <skos:exactMatch xml:lang="en">http://dbpedia.org/resource/Fugue</skos:exactMatch>
    <skos:inScheme rdf:resource="http://data.europeana.eu/concept/music/genre/Music_Genre_Scheme"/>
    <skos:altLabel xml:lang="en">Fugue</skos:altLabel>
  </skos:Concept>

  <skos:Concept rdf:about="http://data.europeana.eu/concept/music/genre/Guaguanco">
    <skos:prefLabel xml:lang="en">Guaguancó</skos:prefLabel>
    <skos:prefLabel xml:lang="es">Guaguancó</skos:prefLabel>
    <skos:prefLabel xml:lang="sv">Guaguanco</skos:prefLabel>
    <skos:closeMatch rdf:resource="http://rdf.freebase.com/ns/m.060t48"/>
    <skos:broader rdf:resource="http://data.europeana.eu/concept/music/genre/Rumba"/>
    <skos:definition xml:lang="en">Guaguancó is a sub-genre of Cuban rumba, combining percussion,
      voices, and dance. There are two main styles: Havana and Matanzas.</skos:definition>
    <skos:exactMatch xml:lang="en">http://dbpedia.org/resource/Guaguanc%C3%B3</skos:exactMatch>
    <skos:inScheme rdf:resource="http://data.europeana.eu/concept/music/genre/Music_Genre_Scheme"/>
    <skos:altLabel xml:lang="en">Guaguanco</skos:altLabel>
    <skos:altLabel xml:lang="en">Guaguancó</skos:altLabel>
  </skos:Concept>

  <skos:Concept rdf:about="http://data.europeana.eu/concept/music/genre/Guarania_(music)">
    <skos:prefLabel xml:lang="en">Guaran¡a</skos:prefLabel>
    <skos:prefLabel xml:lang="ja">グアラニア</skos:prefLabel>
    <skos:prefLabel xml:lang="pt">Guarânia</skos:prefLabel>
    <skos:prefLabel xml:lang="es">Guarania</skos:prefLabel>
    <skos:closeMatch rdf:resource="http://rdf.freebase.com/ns/m.0g93f5"/>
    <skos:broader
      rdf:resource="http://data.europeana.eu/concept/music/genre/Latin_American_music_popular"/>
    <skos:definition xml:lang="en">Guarania is a style of music created in Paraguay by musician José
      Asunción Flores in 1925 with the purpose of expressing the character of the Paraguayan people.
      This is accomplished by the slow and melancholic rhythms and melodies used in the songs.
      &lt;p&gt; Since its creation, the Guarania became the biggest musical phenomenon of Paraguay
      in the 20th century thanks to songs such as Jejuí, Kerasy, India and Arribeño Resay, which
      generated an immediate acceptance. The best known Guarania songs are Recuerdos de Ypakaraí, Ne
      rendápe aju, Mis noches sin ti, Panambí Vera, and Paraguaýpe. &lt;p&gt; The Guarania is highly
      regarded in the urban areas, but not in the countryside. This is because the people in the
      countryside prefer faster styles of songs, such as the paraguayan polka, which is danced
      more.</skos:definition>
    <skos:exactMatch xml:lang="en">http://dbpedia.org/resource/Guarania_(music)</skos:exactMatch>
    <skos:inScheme rdf:resource="http://data.europeana.eu/concept/music/genre/Music_Genre_Scheme"/>
    <skos:altLabel xml:lang="en">Guarania</skos:altLabel>
  </skos:Concept>

  <skos:Concept rdf:about="http://data.europeana.eu/concept/music/genre/Jenkka">
    <skos:prefLabel xml:lang="en">Jenkka</skos:prefLabel>
    <skos:prefLabel xml:lang="et">Jenka</skos:prefLabel>
    <skos:prefLabel xml:lang="fi">Jenkka</skos:prefLabel>
    <skos:prefLabel xml:lang="de">Jenkka</skos:prefLabel>
    <skos:prefLabel xml:lang="ja">ジェンカ</skos:prefLabel>
    <skos:prefLabel xml:lang="no">Jenka</skos:prefLabel>
    <skos:prefLabel xml:lang="ru">Енка</skos:prefLabel>
    <skos:prefLabel xml:lang="sv">Jenka</skos:prefLabel>
    <skos:closeMatch rdf:resource="http://rdf.freebase.com/ns/m.03clh74"/>
    <skos:broader rdf:resource="http://data.europeana.eu/concept/music/genre/Folk_music_traditional"/>
    <skos:definition xml:lang="en">Jenkka [/je??k??/] is a fast Finnish partner dance originated in
      Finnish folk dance. It is danced to the music in 2/4 or 4/4 time signature of about 140 beats
      per minute. &lt;p&gt; Men and women do similar steps. The initial dance position is the man is
      to the left of the woman both facing in the direction of the line of dance, with their inner
      arms on each other's waists. The dancers go forward in a run similar to Polka:
      &quot;left-right-left-hop&quot;, &quot;right-left-right-hop&quot;. After than they join the
      free arms assume the face-to-face closed dance position and proceed with the chain of pivot
      turns stepping &quot;left-right-left-right&quot; or &quot;left-hop-right-hop&quot;. The runs
      of similar steps are normally started at the beginnings of musical phrases. &lt;p&gt; Georg
      Malmstén composed many Jenkkas.</skos:definition>
    <skos:exactMatch xml:lang="en">http://dbpedia.org/resource/Jenkka</skos:exactMatch>
    <skos:inScheme rdf:resource="http://data.europeana.eu/concept/music/genre/Music_Genre_Scheme"/>
    <skos:altLabel xml:lang="en">Jenkka</skos:altLabel>
  </skos:Concept>

  <skos:Concept rdf:about="http://data.europeana.eu/concept/music/genre/Jota_(music)">
    <skos:prefLabel xml:lang="en">Jota</skos:prefLabel>
    <skos:prefLabel xml:lang="ar">خوطا</skos:prefLabel>
    <skos:prefLabel xml:lang="ca">Jota</skos:prefLabel>
    <skos:prefLabel xml:lang="fr">Jota</skos:prefLabel>
    <skos:prefLabel xml:lang="de">Jota</skos:prefLabel>
    <skos:prefLabel xml:lang="hu">Jota</skos:prefLabel>
    <skos:prefLabel xml:lang="it">Jota</skos:prefLabel>
    <skos:prefLabel xml:lang="no">Jota</skos:prefLabel>
    <skos:prefLabel xml:lang="pl">Jota</skos:prefLabel>
    <skos:prefLabel xml:lang="pt">Jota</skos:prefLabel>
    <skos:prefLabel xml:lang="ru">Хота</skos:prefLabel>
    <skos:prefLabel xml:lang="es">Jota</skos:prefLabel>
    <skos:prefLabel xml:lang="uk">Хота</skos:prefLabel>
    <skos:closeMatch rdf:resource="http://rdf.freebase.com/ns/m.026bxb6"/>
    <skos:broader rdf:resource="http://data.europeana.eu/concept/music/genre/Folk_music_traditional"/>
    <skos:definition xml:lang="en">The jota is a genre of music and the associated dance known
      throughout Spain, most likely originating in Aragon. It varies by region, having a
      characteristic form in Aragon, Catalonia Castile, Navarra, Cantabria, Asturias, Galicia, La
      Rioja, Murcia and Eastern Andalusia. Being a visual representation, the jota is danced and
      sung accompanied by castanets, and the interpreters tend to wear regional costumes. In
      Valencia, the jota was once danced during interment ceremonies. &lt;p&gt; The jota tends to
      have a 3/4 rhythm, although some authors maintain that the 6/8 is better adapted to the poetic
      and choreographic structure. For their interpretation, guitars, bandurrias, lutes, dulzaina,
      and drums are used in the Castilian style, while the Galicians use bagpipes, drums, and
      bombos. Theatrical versions are sung and danced with regional costumes and castanets, though
      such things are not used when dancing the jota in less formal settings. The content of the
      songs is quite diverse, from patriotism to religion to sexual exploits. In addition to this,
      the songs also have the effect of helping to generate a sense of local identity and
      cohesion.</skos:definition>
    <skos:exactMatch xml:lang="en">http://dbpedia.org/resource/Jota_(music)</skos:exactMatch>
    <skos:inScheme rdf:resource="http://data.europeana.eu/concept/music/genre/Music_Genre_Scheme"/>
    <skos:altLabel xml:lang="en">Jota</skos:altLabel>
  </skos:Concept>

  <skos:Concept rdf:about="http://data.europeana.eu/concept/music/genre/Juju_music">
    <skos:prefLabel xml:lang="en">Jùjú</skos:prefLabel>
    <skos:prefLabel xml:lang="nl">Juju</skos:prefLabel>
    <skos:prefLabel xml:lang="fi">Juju</skos:prefLabel>
    <skos:prefLabel xml:lang="de">Jùjú</skos:prefLabel>
    <skos:prefLabel xml:lang="pt">Juju</skos:prefLabel>
    <skos:prefLabel xml:lang="es">Jùjú</skos:prefLabel>
    <skos:closeMatch rdf:resource="http://rdf.freebase.com/ns/m.04kjj5"/>
    <skos:broader rdf:resource="http://data.europeana.eu/concept/music/genre/African_popular_music"/>
    <skos:definition xml:lang="en">Jùjú is a style of Nigerian popular music, derived from
      traditional Yoruba percussion. The name comes from a Yoruba word &quot;juju&quot; or
      &quot;jiju&quot; meaning &quot;throwing&quot; or &quot;something being thrown.&quot; Juju
      music did not derive its name from juju, which &quot;is a form of magic and the use of magic
      objects or witchcraft common in West Africa, Haiti, Cuba and other South American
      nations.&quot; It evolved in the 1920s in urban clubs across the countries, and was believed
      to have been created by AbdulRafiu Babatunde King, popularly known as Tunde King. The first
      jùjú recordings were by Tunde King and Ojoge Daniel from the same era of the 1920s when Tunde
      King pioneered it. The lead and predominant instrument of Jùjú is the Iya Ilu,&quot;' talking
      drum. Some Jùjú musicians were itinerant, including early pioneers Ojoge Daniel, Irewole Denge
      and the &quot;blind minstrel&quot; Kokoro. &lt;p&gt; Afro-juju is a style of Nigerian popular
      music, a mixture of Jùjú music and Afrobeat. Its most famous exponent was Shina Peters, who
      was so popular that the press called the phenomenon &quot;Shinamania&quot;. Afro-juju's peak
      of popularity came in the early 1990s.</skos:definition>
    <skos:exactMatch xml:lang="en"
      >http://dbpedia.org/resource/J%C3%B9j%C3%BA_music</skos:exactMatch>
    <skos:inScheme rdf:resource="http://data.europeana.eu/concept/music/genre/Music_Genre_Scheme"/>
    <skos:altLabel xml:lang="en">Jùjú music</skos:altLabel>
    <skos:altLabel xml:lang="en">Juju music</skos:altLabel>
  </skos:Concept>

  <skos:Concept rdf:about="http://data.europeana.eu/concept/music/genre/Music_of_Argentina_kaluyo">
    <skos:prefLabel xml:lang="en">Kaluyo</skos:prefLabel>
    <skos:broader
      rdf:resource="http://data.europeana.eu/concept/music/genre/Latin_American_music_traditional"/>
    <skos:definition xml:lang="en">Cosquín National Folklore Festival typically includes
      representatives from all musical genres created or developed in Argentina:_x000d_ _x000d_
      Baguala_x000d_ _x000d_ Bailecito_x000d_ Kaluyo_x000d_ Candombé_x000d_ Carnavalito_x000d_
      Chacarera_x000d_ Chamarrita_x000d_ Chamamé_x000d_ Chaya_x000d_ Cifra_x000d_ Cielito_x000d_
      _x000d_ _x000d_ _x000d_ Cogollo o Cogoyo_x000d_ La Condición_x000d_ Copla (music)_x000d_ El
      Cuando_x000d_ Cumbia villera_x000d_ Décima_x000d_ Escondido_x000d_ La Firmeza_x000d_
      Gato_x000d_ Guaracha santiagueña_x000d_ Huella_x000d_ Huayno_x000d_ _x000d_ _x000d_ _x000d_
      Malambo_x000d_ Media caña_x000d_ Milonga_x000d_ Murga_x000d_ Pala-Pala_x000d_ El Palito_x000d_
      Payada_x000d_ Pericón_x000d_ Polka_x000d_ Rasguido doble_x000d_ Refalosa_x000d_ El
      Sombrerito_x000d_ _x000d_ _x000d_ _x000d_ Tango_x000d_ Nuevo tango_x000d_ Tonada_x000d_
      Tristecito_x000d_ Triunfo_x000d_ Valsecito criollo_x000d_ Vidala_x000d_ Vidalita_x000d_
      Yaraví_x000d_ Cosquín National Folklore Festival typically includes representatives from all
      musical genres created or developed in
      Argentina:Baguala,Bailecito,Kaluyo,Candombé,Carnavalito,Chacarera,Chamarrita,Chamamé,Chaya,Cifra,Cielito,
      Cogollo o Cogoyo,La Condición,Copla (music),El Cuando,Cumbia villera,Décima,Escondido,La
      Firmeza,Gato,Guaracha santiagueña,Huella,Huayno, Malambo,Media caña,Milonga,Murga,Pala-Pala,El
      Palito,Payada,Pericón,Polka,Rasguido doble,Refalosa,El Sombrerito,Tango,Nuevo
      tango,Tonada,Tristecito,Triunfo,Valsecito
      criollo,Vidala,Vidalita,Yaraví,Zamba,</skos:definition>
    <skos:exactMatch xml:lang="en">http://dbpedia.org/resource/Music_of_Argentina</skos:exactMatch>
    <skos:inScheme rdf:resource="http://data.europeana.eu/concept/music/genre/Music_Genre_Scheme"/>
  </skos:Concept>

  <skos:Concept rdf:about="http://data.europeana.eu/concept/music/genre/Music_of_Mongolia_Hoomi">
    <skos:prefLabel xml:lang="en">Khoomi</skos:prefLabel>
    <skos:broader
      rdf:resource="http://data.europeana.eu/concept/music/genre/Music_of_Asia_traditional"/>
    <skos:definition xml:lang="en"> Khöömi is believed the art of overtone singing has originated
      from south western Mongolia in today's Khovd and Govi-Altai region. Nowadays, overtone singing
      is found throughout the country and Mongolia is often considered as the most active place of
      overtone singing in the world</skos:definition>
    <skos:inScheme rdf:resource="http://data.europeana.eu/concept/music/genre/Music_Genre_Scheme"/>
  </skos:Concept>

  <skos:Concept rdf:about="http://data.europeana.eu/concept/music/genre/Kpanlogo">
    <skos:prefLabel xml:lang="en">Kpanlogo</skos:prefLabel>
    <skos:prefLabel xml:lang="de">Kpanlogo</skos:prefLabel>
    <skos:closeMatch rdf:resource="http://rdf.freebase.com/ns/m.06zrks"/>
    <skos:broader>
      <skos:Concept
        rdf:about="http://data.europeana.eu/concept/music/genre/Music_of_Africa_traditional">
        <skos:prefLabel xml:lang="en">Traditional African</skos:prefLabel>
        <skos:prefLabel xml:lang="ca">Música africana</skos:prefLabel>
        <skos:prefLabel xml:lang="cs">Africká hudba</skos:prefLabel>
        <skos:prefLabel xml:lang="nl">Afrikaanse muziek</skos:prefLabel>
        <skos:prefLabel xml:lang="fr">Musique africaine</skos:prefLabel>
        <skos:prefLabel xml:lang="de">Traditionelle afrikanische Musik</skos:prefLabel>
        <skos:prefLabel xml:lang="hu">Afrika zenéje</skos:prefLabel>
        <skos:prefLabel xml:lang="id">Musik Afrika</skos:prefLabel>
        <skos:prefLabel xml:lang="it">Musica africana</skos:prefLabel>
        <skos:prefLabel xml:lang="no">Afrikansk musikk</skos:prefLabel>
        <skos:prefLabel xml:lang="pt">Música da África</skos:prefLabel>
        <skos:prefLabel xml:lang="es">Música africana</skos:prefLabel>
        <skos:prefLabel xml:lang="sv">Afrikansk musik</skos:prefLabel>
        <skos:closeMatch rdf:resource="http://rdf.freebase.com/ns/m.0164x2"/>
        <skos:broader rdf:resource="http://data.europeana.eu/concept/music/genre/World_music"/>
        <skos:definition xml:lang="en">Given the vastness of the continent, the traditional music of
          Africa is historically ancient, rich, and diverse, with the different regions and nations
          of Africa having distinct musical traditions. Traditional music in much of the continent
          is passed down orally and is not written. In Sub-Saharan African music traditions, it also
          frequently relies heavily on percussion instruments of every variety, including
          xylophones, drums, and tone-producing instruments such as the mbira or &quot;thumb
          piano.&quot; The music and dance of the African diaspora, formed to varying degrees on
          African musical traditions, include American music and many Caribbean genres, such as
          soca, calypso and zouk. Latin American music genres such as the samba, rumba, salsa, and
          other clave-based genres, were also founded to varying degrees on the music of enslaved
          Africans, and have in turn influenced African popular music.</skos:definition>
        <skos:broadMatch rdf:resource="http://dbpedia.org/page/Music_of_Africa"/>
        <skos:inScheme
          rdf:resource="http://data.europeana.eu/concept/music/genre/Music_Genre_Scheme"/>
        <skos:altLabel xml:lang="en">Music of Africa</skos:altLabel>
      </skos:Concept>
    </skos:broader>

    <skos:definition xml:lang="en">panlogo is a recreational dance and music form from Ghana, West
      Africa. It was first played by the Ga ethnih group, most of whom live in and around the
      capital city, Accra, but is now performed and enjoyed throughout the country. It began in the
      early 1960s as an innovative dance form, influenced by American rock and roll, and giving the
      younger Ga generations a point of distinction from their elders. Ghanaian master drummer C.K.
      Ladzekpo states that kpanlogo &quot;is essentially an urban youth dance-drumming and a symbol
      of the commitment of a rapidly growing Ghanaian urban neighborhood youth in advocating their
      perspective in shaping the political vision of post colonial Africa&quot;. The kpanlogo dance
      is often performed low to the ground, with bent knees and bent back, and frequently features
      sexually suggestive motions. The music accompanying the kpanlogo dance is drawn from older Ga
      drumming traditions, such as gome, oge and kolomashie. Kpanlogo music uses three types of
      instruments: nono, fao, and kpanlogo drums. Nono plays the key pattern or timeline of the
      music, supported by the fao. It is common to have three kpanlogo drums in an ensemble, in the
      roles of &quot;male voice&quot;, &quot;female voice&quot; and &quot;master
      drum&quot;</skos:definition>
    <skos:exactMatch xml:lang="en">http://dbpedia.org/resource/Kpanlogo</skos:exactMatch>
    <skos:inScheme rdf:resource="http://data.europeana.eu/concept/music/genre/Music_Genre_Scheme"/>
    <skos:altLabel xml:lang="en">Kpanlogo</skos:altLabel>
  </skos:Concept>

  <skos:Concept rdf:about="http://data.europeana.eu/concept/music/genre/Kullawada">
    <skos:prefLabel xml:lang="en">Kullawada</skos:prefLabel>
    <skos:prefLabel xml:lang="es">Kullahuada</skos:prefLabel>
    <skos:closeMatch rdf:resource="http://rdf.freebase.com/ns/m.03gsfyw"/>
    <skos:broader
      rdf:resource="http://data.europeana.eu/concept/music/genre/Latin_American_music_traditional"/>
    <skos:definition xml:lang="en">The Kullawada is an Aymara folklore dance that is part of the
      Bolivia Andean culture. Originating in the region around the Lake Titicaca, it is traditional
      to be danced among alpaca and sheep wool weavers. The dancers wear colorful, elaborately
      decorated costumes for the dance, which is meant to represent the social class of weavers and
      textile workers. For this reason the dancers use a little spinning wheel as a symbol of the
      dance.</skos:definition>
    <skos:exactMatch xml:lang="en">http://dbpedia.org/resource/Kullawada</skos:exactMatch>
    <skos:inScheme rdf:resource="http://data.europeana.eu/concept/music/genre/Music_Genre_Scheme"/>
    <skos:altLabel xml:lang="en">Kullawada</skos:altLabel>
  </skos:Concept>

  <skos:Concept rdf:about="http://data.europeana.eu/concept/music/genre/Lando_(music)">
    <skos:prefLabel xml:lang="en">Landó</skos:prefLabel>
    <skos:prefLabel xml:lang="fr">Lando</skos:prefLabel>
    <skos:closeMatch rdf:resource="http://rdf.freebase.com/ns/m.070k2b"/>
    <skos:broader
      rdf:resource="http://data.europeana.eu/concept/music/genre/Latin_American_music_traditional"/>
    <skos:definition xml:lang="en">Landó is an Afro-Peruvian form of music in the musica criolla
      genre. Its unique sound had been likened to the American blues genre.</skos:definition>
    <skos:exactMatch xml:lang="en">http://dbpedia.org/resource/Landó_(music)</skos:exactMatch>
    <skos:inScheme rdf:resource="http://data.europeana.eu/concept/music/genre/Music_Genre_Scheme"/>
    <skos:altLabel xml:lang="en">Lando</skos:altLabel>
    <skos:altLabel xml:lang="en">Landó</skos:altLabel>
  </skos:Concept>

  <skos:Concept rdf:about="http://data.europeana.eu/concept/music/genre/Lezginka">
    <skos:prefLabel xml:lang="en">Lezginka</skos:prefLabel>
    <skos:prefLabel xml:lang="ar">ليزغينكا</skos:prefLabel>
    <skos:prefLabel xml:lang="bg">Лезгинка</skos:prefLabel>
    <skos:prefLabel xml:lang="nl">Lezginka</skos:prefLabel>
    <skos:prefLabel xml:lang="de">Lesginka</skos:prefLabel>
    <skos:prefLabel xml:lang="lt">Lezginka</skos:prefLabel>
    <skos:prefLabel xml:lang="fa">رقص لزگی</skos:prefLabel>
    <skos:prefLabel xml:lang="pl">Lezginka</skos:prefLabel>
    <skos:prefLabel xml:lang="ru">Лезгинка</skos:prefLabel>
    <skos:prefLabel xml:lang="sr">Лезгинка</skos:prefLabel>
    <skos:prefLabel xml:lang="sk">Lezginka</skos:prefLabel>
    <skos:prefLabel xml:lang="tr">Lezginka</skos:prefLabel>
    <skos:prefLabel xml:lang="uk">Лезгінка</skos:prefLabel>
    <skos:closeMatch rdf:resource="http://rdf.freebase.com/ns/m.0g5kp7"/>
    <skos:broader
      rdf:resource="http://data.europeana.eu/concept/music/genre/Music_of_Asia_traditional"/>
    <skos:definition xml:lang="en">Lezginka or Lezghinka is a national dance of the Lezgian people,
      and of many peoples in the Caucasus Mountains. It derives its names from the Lezgin people.
      Nevertheless, Georgians, Azeris, Chechens, Lezghins, Ossetians, Circassians, Karachays,
      Balkars, Abkhazians, Kabardins, Ingush, Ingilos, Mountain Jews, the Russian Kuban and Terek
      Cossacks and the various ethnicities of Dagestan such as the Avars, Dargwa and Kumyks have
      their own versions. Lezginka can be a solo, couple or group dance. Men and women are dressed
      in traditional costumes; men wear a sword adorned on their side and women in long, flowing
      dresses. The man, imitating an eagle, dances in quick, concise steps; falling to his knees and
      leaping up quickly. The woman dances quietly, taking light, small steps—giving the appearance
      of her floating around the floor. When the dance is performed in pairs, the couples do not
      touch; the woman acknowledges the man, and dances discreetly about him.</skos:definition>
    <skos:exactMatch xml:lang="en">http://dbpedia.org/resource/Lezginka</skos:exactMatch>
    <skos:inScheme rdf:resource="http://data.europeana.eu/concept/music/genre/Music_Genre_Scheme"/>
    <skos:altLabel xml:lang="en">Lezginka</skos:altLabel>
  </skos:Concept>

  <skos:Concept rdf:about="http://data.europeana.eu/concept/music/genre/Lullaby">
    <skos:prefLabel xml:lang="en">Lullaby</skos:prefLabel>
    <skos:prefLabel xml:lang="ar">تهويدة</skos:prefLabel>
    <skos:prefLabel xml:lang="ca">Cançó de bressol</skos:prefLabel>
    <skos:prefLabel xml:lang="cs">Ukolébavka</skos:prefLabel>
    <skos:prefLabel xml:lang="da">Vuggevise</skos:prefLabel>
    <skos:prefLabel xml:lang="nl">Slaaplied</skos:prefLabel>
    <skos:prefLabel xml:lang="et">Hällilaul</skos:prefLabel>
    <skos:prefLabel xml:lang="fil">Oyayi</skos:prefLabel>
    <skos:prefLabel xml:lang="fi">Kehtolaulu</skos:prefLabel>
    <skos:prefLabel xml:lang="fr">Berceuse</skos:prefLabel>
    <skos:prefLabel xml:lang="de">Wiegenlied</skos:prefLabel>
    <skos:prefLabel xml:lang="hi">लोरी</skos:prefLabel>
    <skos:prefLabel xml:lang="it">Ninna nanna</skos:prefLabel>
    <skos:prefLabel xml:lang="ja">子守唄</skos:prefLabel>
    <skos:prefLabel xml:lang="ko">자장가</skos:prefLabel>
    <skos:prefLabel xml:lang="lt">Lopšinė</skos:prefLabel>
    <skos:prefLabel xml:lang="no">Bånsull</skos:prefLabel>
    <skos:prefLabel xml:lang="fa">لالایی</skos:prefLabel>
    <skos:prefLabel xml:lang="pl">Kołysanka</skos:prefLabel>
    <skos:prefLabel xml:lang="pt">Cantiga de ninar</skos:prefLabel>
    <skos:prefLabel xml:lang="ru">Колыбельная песня</skos:prefLabel>
    <skos:prefLabel xml:lang="es">Nana</skos:prefLabel>
    <skos:prefLabel xml:lang="sv">Vaggvisa</skos:prefLabel>
    <skos:prefLabel xml:lang="th">เพลงกล่อมเด็ก</skos:prefLabel>
    <skos:prefLabel xml:lang="tr">Ninni</skos:prefLabel>
    <skos:prefLabel xml:lang="uk">Колискові пісні</skos:prefLabel>
    <skos:prefLabel xml:lang="vi">Hát ru</skos:prefLabel>
    <skos:closeMatch rdf:resource="http://rdf.freebase.com/ns/m.0nk0v"/>
    <skos:broader rdf:resource="http://data.europeana.eu/concept/music/genre/Childrens_music"/>
    <skos:definition xml:lang="en">A lullaby is a soothing piece of music, usually played or sung to
      young children before they go to sleep, with the intention of aiding that process. As a
      result, the music is often simple and repetitive. Lullabies can be found in many countries,
      and have existed since ancient times. Tonally, most lullabies are simple, often merely
      alternating tonic and dominant harmonies.</skos:definition>
    <skos:exactMatch xml:lang="en">http://dbpedia.org/resource/Lullaby</skos:exactMatch>
    <skos:inScheme rdf:resource="http://data.europeana.eu/concept/music/genre/Music_Genre_Scheme"/>
    <skos:altLabel xml:lang="en">Lullaby</skos:altLabel>
  </skos:Concept>

  <skos:Concept rdf:about="http://data.europeana.eu/concept/music/genre/Epic_of_Manas">
    <skos:prefLabel xml:lang="en">Manas-Epos</skos:prefLabel>
    <skos:prefLabel xml:lang="ar">مناص</skos:prefLabel>
    <skos:prefLabel xml:lang="bg">Епопея на Манас</skos:prefLabel>
    <skos:prefLabel xml:lang="ca">Poema èpic de Manas</skos:prefLabel>
    <skos:prefLabel xml:lang="hr">Manas</skos:prefLabel>
    <skos:prefLabel xml:lang="da">Manas</skos:prefLabel>
    <skos:prefLabel xml:lang="nl">Manas</skos:prefLabel>
    <skos:prefLabel xml:lang="et">Manas</skos:prefLabel>
    <skos:prefLabel xml:lang="fr">Épopée de Manas</skos:prefLabel>
    <skos:prefLabel xml:lang="de">Manas</skos:prefLabel>
    <skos:prefLabel xml:lang="hi">मनास की दास्तान</skos:prefLabel>
    <skos:prefLabel xml:lang="hu">Manasz</skos:prefLabel>
    <skos:prefLabel xml:lang="it">Manas</skos:prefLabel>
    <skos:prefLabel xml:lang="ja">マナス</skos:prefLabel>
    <skos:prefLabel xml:lang="fa">مناس</skos:prefLabel>
    <skos:prefLabel xml:lang="pl">Manas</skos:prefLabel>
    <skos:prefLabel xml:lang="pt">Épico de Manas</skos:prefLabel>
    <skos:prefLabel xml:lang="ru">Манас</skos:prefLabel>
    <skos:prefLabel xml:lang="es">Manas</skos:prefLabel>
    <skos:prefLabel xml:lang="sv">Manaseposet</skos:prefLabel>
    <skos:prefLabel xml:lang="tr">Manas Destanı</skos:prefLabel>
    <skos:prefLabel xml:lang="uk">Манаський епос</skos:prefLabel>
    <skos:closeMatch rdf:resource="http://rdf.freebase.com/ns/m.02n15r"/>
    <skos:broader
      rdf:resource="http://data.europeana.eu/concept/music/genre/Music_of_Asia_traditional"/>
    <skos:definition xml:lang="en">The Epic of Manas is a traditional epic poem of the Kyrgyz
      people. The monumental epic Manas is the most treasured expression of the national heritage of
      the Kyrgyz people. Composed and sung entirely in oral form by various singers throughout the
      centuries, Manas is regarded as the epitome of oral creativity. It is considered to be one of
      the greatest examples of epic poetry, whose importance is not inferior to that of the Homeric
      epic. As nomads, the Kyrgyz had no written language. However, they excelled in oral
      composition, which they artistically employed in their traditional poetry and epic songs. As
      the internationally renowned Kyrgyz writer Chingiz Aitmatov notes: &quot;If other
      peoples/nations displayed their past culture and history in written art, the sculpture,
      architecture, theatre and literature, Kyrgyz people expressed their worldview, pride and
      dignity, battles and their hope for the future in epic genre.&quot; &lt;p&gt; Today there are
      about sixty versions of the epic Manas recorded from various epic singers and oral poets. Its
      longest version, consisting of half a million poetic lines, was written down from one of the
      last master-manaschï Saiakbai Karalaev.</skos:definition>
    <skos:exactMatch xml:lang="en">http://dbpedia.org/resource/Epic_of_Manas</skos:exactMatch>
    <skos:inScheme rdf:resource="http://data.europeana.eu/concept/music/genre/Music_Genre_Scheme"/>
    <skos:altLabel xml:lang="en">Epic of Manas</skos:altLabel>
  </skos:Concept>

  <skos:Concept rdf:about="http://data.europeana.eu/concept/music/genre/Mapale">
    <skos:prefLabel xml:lang="en">Mapalé</skos:prefLabel>
    <skos:prefLabel xml:lang="ca">Mapalé</skos:prefLabel>
    <skos:prefLabel xml:lang="de">Mapalé</skos:prefLabel>
    <skos:prefLabel xml:lang="es">Mapalé</skos:prefLabel>
    <skos:closeMatch rdf:resource="http://rdf.freebase.com/ns/m.03cqtsq"/>
    <skos:broader
      rdf:resource="http://data.europeana.eu/concept/music/genre/Latin_American_music_traditional"/>
    <skos:definition xml:lang="en">Mapalé is a Colombian musical genre and dance original of the
      Afro Colombian culture of the Pacific and Caribbean Regions of Colombia.</skos:definition>
    <skos:exactMatch xml:lang="en">http://dbpedia.org/resource/Mapalé</skos:exactMatch>
    <skos:inScheme rdf:resource="http://data.europeana.eu/concept/music/genre/Music_Genre_Scheme"/>
    <skos:altLabel xml:lang="en">Mapalé</skos:altLabel>
  </skos:Concept>

  <skos:Concept rdf:about="http://data.europeana.eu/concept/music/genre/Marinera">
    <skos:prefLabel xml:lang="en">Marinera</skos:prefLabel>
    <skos:prefLabel xml:lang="fi">Marinera</skos:prefLabel>
    <skos:prefLabel xml:lang="fr">Marinera</skos:prefLabel>
    <skos:prefLabel xml:lang="de">Marinera</skos:prefLabel>
    <skos:prefLabel xml:lang="it">Zamacueca</skos:prefLabel>
    <skos:prefLabel xml:lang="pl">Marinera</skos:prefLabel>
    <skos:prefLabel xml:lang="es">Marinera</skos:prefLabel>
    <skos:prefLabel xml:lang="uk">Марінера</skos:prefLabel>
    <skos:closeMatch rdf:resource="http://rdf.freebase.com/ns/m.0710fh"/>
    <skos:broader
      rdf:resource="http://data.europeana.eu/concept/music/genre/Latin_American_music_traditional"/>
    <skos:definition xml:lang="en">Marinera is a coastal dance of Peru. Marinera is a graceful and
      romantic couple's dance that uses handkerchiefs as props. The dance is an elegant and stylized
      reenactment of a courtship, and it shows a blend of the different cultures of Peru. The dance
      itself has gained a lot of recognition and is one of the most popular traditional dances of
      Peru. Ever since the 1960s, during the month of January, in the city of Trujillo, declared
      national capital of this dance by law N° 24.447, January 24, in 1986, and a National Contest
      of Marinera Nortena is held. In year 2012 the congress of Peruvian republic reclared October 7
      as marinera day and in Trujillo city is celebrated with a parade and dance expressions.
      &lt;p&gt; The origin of the Marinera is generally traced back to the Zamacueca. Nevertheless,
      there are various other theories about where it comes from. Traditional accompaniment for the
      dance is provided by cajón, clarinets, guitars, drums, and bugles.</skos:definition>
    <skos:exactMatch xml:lang="en">http://dbpedia.org/resource/Marinera</skos:exactMatch>
    <skos:inScheme rdf:resource="http://data.europeana.eu/concept/music/genre/Music_Genre_Scheme"/>
    <skos:altLabel xml:lang="en">Marinera</skos:altLabel>
  </skos:Concept>

  <skos:Concept rdf:about="http://data.europeana.eu/concept/music/genre/Mass_(music)">
    <skos:prefLabel xml:lang="en">Mass</skos:prefLabel>
    <skos:prefLabel xml:lang="ar">القداس</skos:prefLabel>
    <skos:prefLabel xml:lang="bg">Меса</skos:prefLabel>
    <skos:prefLabel xml:lang="ca">Missa</skos:prefLabel>
    <skos:prefLabel xml:lang="cs">Mše</skos:prefLabel>
    <skos:prefLabel xml:lang="da">Messe</skos:prefLabel>
    <skos:prefLabel xml:lang="et">Missa</skos:prefLabel>
    <skos:prefLabel xml:lang="fr">Messe</skos:prefLabel>
    <skos:prefLabel xml:lang="de">Messe</skos:prefLabel>
    <skos:prefLabel xml:lang="el">Λειτουργία</skos:prefLabel>
    <skos:prefLabel xml:lang="it">Messa</skos:prefLabel>
    <skos:prefLabel xml:lang="ja">ミサ曲</skos:prefLabel>
    <skos:prefLabel xml:lang="ko">미사곡</skos:prefLabel>
    <skos:prefLabel xml:lang="lv">Mesa</skos:prefLabel>
    <skos:prefLabel xml:lang="lt">Mišios</skos:prefLabel>
    <skos:prefLabel xml:lang="no">Messe</skos:prefLabel>
    <skos:prefLabel xml:lang="fa">مس</skos:prefLabel>
    <skos:prefLabel xml:lang="pl">Msza</skos:prefLabel>
    <skos:prefLabel xml:lang="pt">Missa</skos:prefLabel>
    <skos:prefLabel xml:lang="ru">Месса</skos:prefLabel>
    <skos:prefLabel xml:lang="sk">Omša</skos:prefLabel>
    <skos:prefLabel xml:lang="es">Misa</skos:prefLabel>
    <skos:prefLabel xml:lang="uk">Меса</skos:prefLabel>
    <skos:closeMatch rdf:resource="http://rdf.freebase.com/ns/m.0197_n"/>
    <skos:broader rdf:resource="http://data.europeana.eu/concept/music/genre/Religious_music"/>
    <skos:definition xml:lang="en">The Mass, a form of sacred musical composition, is a choral
      composition that sets the invariable portions of the Eucharistic liturgy to music. Most Masses
      are settings of the liturgy in Latin, the liturgical sacred language of the Catholic Church's
      Roman liturgy, but there are a significant number written in the languages of non-Catholic
      countries where vernacular worship has long been the norm. For example, there are many Masses
      written in English for the Church of England. Musical Masses take their name from the Catholic
      liturgy called &quot;the Mass&quot; as well. &lt;p&gt; Masses can be a cappella, that is,
      without an independent accompaniment, or they can be accompanied by instrumental obbligatos up
      to and including a full orchestra. Many Masses, especially later ones, were never intended to
      be performed during the celebration of an actual mass.</skos:definition>
    <skos:exactMatch xml:lang="en">http://dbpedia.org/resource/Mass_(music)</skos:exactMatch>
    <skos:inScheme rdf:resource="http://data.europeana.eu/concept/music/genre/Music_Genre_Scheme"/>
    <skos:altLabel xml:lang="en">Mass</skos:altLabel>
  </skos:Concept>

  <skos:Concept rdf:about="http://data.europeana.eu/concept/music/genre/Motet">
    <skos:prefLabel xml:lang="en">Motet</skos:prefLabel>
    <skos:prefLabel xml:lang="ar">موتيت</skos:prefLabel>
    <skos:prefLabel xml:lang="bg">Мотет</skos:prefLabel>
    <skos:prefLabel xml:lang="ca">Motet</skos:prefLabel>
    <skos:prefLabel xml:lang="cs">Moteto</skos:prefLabel>
    <skos:prefLabel xml:lang="da">Motet</skos:prefLabel>
    <skos:prefLabel xml:lang="nl">Motet</skos:prefLabel>
    <skos:prefLabel xml:lang="et">Motett</skos:prefLabel>
    <skos:prefLabel xml:lang="fi">Motetti</skos:prefLabel>
    <skos:prefLabel xml:lang="fr">Motet</skos:prefLabel>
    <skos:prefLabel xml:lang="de">Motette</skos:prefLabel>
    <skos:prefLabel xml:lang="el">Μοτέτο</skos:prefLabel>
    <skos:prefLabel xml:lang="hu">Motetta</skos:prefLabel>
    <skos:prefLabel xml:lang="it">Mottetto</skos:prefLabel>
    <skos:prefLabel xml:lang="ja">モテット</skos:prefLabel>
    <skos:prefLabel xml:lang="ko">모테트</skos:prefLabel>
    <skos:prefLabel xml:lang="lt">Motetas</skos:prefLabel>
    <skos:prefLabel xml:lang="no">Motett</skos:prefLabel>
    <skos:prefLabel xml:lang="pl">Motet</skos:prefLabel>
    <skos:prefLabel xml:lang="pt">Moteto</skos:prefLabel>
    <skos:prefLabel xml:lang="ro">Motet</skos:prefLabel>
    <skos:prefLabel xml:lang="ru">Мотет</skos:prefLabel>
    <skos:prefLabel xml:lang="sr">Мотет</skos:prefLabel>
    <skos:prefLabel xml:lang="sk">Moteto</skos:prefLabel>
    <skos:prefLabel xml:lang="sl">Motet</skos:prefLabel>
    <skos:prefLabel xml:lang="es">Motete</skos:prefLabel>
    <skos:prefLabel xml:lang="sv">Motett</skos:prefLabel>
    <skos:prefLabel xml:lang="th">โมเต็ต</skos:prefLabel>
    <skos:prefLabel xml:lang="uk">Мотет</skos:prefLabel>
    <skos:prefLabel xml:lang="vi">Bản Motet</skos:prefLabel>
    <skos:closeMatch rdf:resource="http://rdf.freebase.com/ns/m.0577x"/>
    <skos:broader rdf:resource="http://data.europeana.eu/concept/music/genre/Religious_music"/>
    <skos:definition xml:lang="en">In classical music, a motet is a highly varied choral musical
      composition. The motet was one of the pre-eminent forms of Renaissance music. &lt;p&gt;
      According to Margaret Bent, &quot;a piece of music in several parts with words&quot; is as
      precise a definition of the motet as will serve from the 13th to the late 16th century and
      beyond. This is close to one of the earliest descriptions we have, that of the late
      13th-century theorist Johannes de Grocheo, who believed that the motet was &quot;not intended
      for the vulgar who do not understand its finer points and derive no pleasure from hearing it:
      it is meant for educated people and those who look for refinement in
      art&quot;.</skos:definition>
    <skos:exactMatch xml:lang="en">http://dbpedia.org/resource/Motet</skos:exactMatch>
    <skos:inScheme rdf:resource="http://data.europeana.eu/concept/music/genre/Music_Genre_Scheme"/>
    <skos:altLabel xml:lang="en">Motet</skos:altLabel>
  </skos:Concept>

  <skos:Concept rdf:about="http://data.europeana.eu/concept/music/genre/Nursery_rhyme">
    <skos:prefLabel xml:lang="en">Nursery rhyme</skos:prefLabel>
    <skos:prefLabel xml:lang="ca">Cançó infantil</skos:prefLabel>
    <skos:prefLabel xml:lang="nl">Kinderlied</skos:prefLabel>
    <skos:prefLabel xml:lang="fil">Tugmaang pambata</skos:prefLabel>
    <skos:prefLabel xml:lang="fi">Lastenloru</skos:prefLabel>
    <skos:prefLabel xml:lang="fr">Chanson enfantine</skos:prefLabel>
    <skos:prefLabel xml:lang="de">Kinderreim</skos:prefLabel>
    <skos:prefLabel xml:lang="it">Filastrocca</skos:prefLabel>
    <skos:prefLabel xml:lang="ja">童謡</skos:prefLabel>
    <skos:prefLabel xml:lang="pl">Rymowanka</skos:prefLabel>
    <skos:prefLabel xml:lang="pt">Cantiga de roda</skos:prefLabel>
    <skos:prefLabel xml:lang="es">Canción infantil</skos:prefLabel>
    <skos:prefLabel xml:lang="sv">Ramsa</skos:prefLabel>
    <skos:closeMatch rdf:resource="http://rdf.freebase.com/ns/m.05g86"/>
    <skos:broader rdf:resource="http://data.europeana.eu/concept/music/genre/Childrens_music"/>
    <skos:definition xml:lang="en">The term nursery rhyme is used for traditional poems and songs
      for young children in Britain and many other countries, but usage only dates from the late
      18th/early 19th century and in North America the term &quot;Mother Goose Rhymes&quot;,
      introduced in the mid-1700s, is still often used.</skos:definition>
    <skos:exactMatch xml:lang="en">http://dbpedia.org/resource/Nursery_rhyme</skos:exactMatch>
    <skos:inScheme rdf:resource="http://data.europeana.eu/concept/music/genre/Music_Genre_Scheme"/>
    <skos:altLabel xml:lang="en">Nursery rhymes</skos:altLabel>
    <skos:altLabel xml:lang="en">Nursery rhyme</skos:altLabel>
  </skos:Concept>

  <skos:Concept rdf:about="http://data.europeana.eu/concept/music/genre/One-Step">
    <skos:prefLabel xml:lang="en">One-Step</skos:prefLabel>
    <skos:prefLabel xml:lang="ca">One-step</skos:prefLabel>
    <skos:prefLabel xml:lang="fr">One-step</skos:prefLabel>
    <skos:prefLabel xml:lang="pl">One-step</skos:prefLabel>
    <skos:prefLabel xml:lang="ru">Уанстеп</skos:prefLabel>
    <skos:prefLabel xml:lang="es">One-step</skos:prefLabel>
    <skos:prefLabel xml:lang="sv">One-step</skos:prefLabel>
    <skos:closeMatch rdf:resource="http://rdf.freebase.com/ns/m.04y9r2s"/>
    <skos:broader rdf:resource="http://data.europeana.eu/concept/music/genre/Art_music"/>
    <skos:definition xml:lang="en">The One-Step was a ballroom dance popular in social dancing at
      the beginning of the 20th century. &lt;p&gt; Troy Kinney writes that One-Step originated from
      the Turkey Trot dance, with all mannerisms of the latter removed, so that “of the original
      ‘trot’ nothing remains but the basic step”. &lt;p&gt; The One-Step included the following
      basic figures: &lt;p&gt; The Castle Walk. &lt;p&gt; The Turn is a walking step, pivoting on
      one foot to change direction. The right foot comes from the preceding step to the place of
      starting, while it makes two successive long steps the left foot turns “on its place”. The
      turn?s completion brings the right foot into anterior fourth position. The woman?s steps are
      the converse of the man?s, her left foot making the long steps, while her right foot turns on
      its place. The turn gains smoothness by means of allowing the right knees to touch each other
      lightly. &lt;p&gt; The Dip. Starting with the right foot in posterior fourth position: during
      the first beat, sink, on the second beat, rise, transferring the weight to the left foot,
      gliding the right foot up to third position, on arriving at which it instantly receives the
      weight again, if the dip is to be repeated.</skos:definition>
    <skos:exactMatch xml:lang="en">http://dbpedia.org/resource/One-Step</skos:exactMatch>
    <skos:inScheme rdf:resource="http://data.europeana.eu/concept/music/genre/Music_Genre_Scheme"/>
    <skos:altLabel xml:lang="en">One-Step</skos:altLabel>
  </skos:Concept>

  <skos:Concept rdf:about="http://data.europeana.eu/concept/music/genre/Passacaglia">
    <skos:prefLabel xml:lang="en">Passacaglia</skos:prefLabel>
    <skos:prefLabel xml:lang="ca">Passacaglia</skos:prefLabel>
    <skos:prefLabel xml:lang="cs">Passacaglia</skos:prefLabel>
    <skos:prefLabel xml:lang="nl">Passacaglia</skos:prefLabel>
    <skos:prefLabel xml:lang="fi">Passacaglia</skos:prefLabel>
    <skos:prefLabel xml:lang="fr">Passacaille</skos:prefLabel>
    <skos:prefLabel xml:lang="de">Passacaglia</skos:prefLabel>
    <skos:prefLabel xml:lang="el">Πασσακάλια</skos:prefLabel>
    <skos:prefLabel xml:lang="hu">Passacaglia</skos:prefLabel>
    <skos:prefLabel xml:lang="it">Passacaglia</skos:prefLabel>
    <skos:prefLabel xml:lang="ja">パッサカリア</skos:prefLabel>
    <skos:prefLabel xml:lang="no">Passacaglia</skos:prefLabel>
    <skos:prefLabel xml:lang="pl">Passacaglia</skos:prefLabel>
    <skos:prefLabel xml:lang="pt">Passacaglia</skos:prefLabel>
    <skos:prefLabel xml:lang="ru">Пассакалья</skos:prefLabel>
    <skos:prefLabel xml:lang="sr">Пасакаља</skos:prefLabel>
    <skos:prefLabel xml:lang="es">Pasacalle</skos:prefLabel>
    <skos:prefLabel xml:lang="sv">Passacaglia</skos:prefLabel>
    <skos:prefLabel xml:lang="uk">Пассакалья</skos:prefLabel>
    <skos:prefLabel xml:lang="vi">Passacaglia</skos:prefLabel>
    <skos:closeMatch rdf:resource="http://rdf.freebase.com/ns/m.0199v5"/>
    <skos:broader rdf:resource="http://data.europeana.eu/concept/music/genre/Classical_music"/>
    <skos:definition xml:lang="en">The passacaglia is a musical form that originated in early
      seventeenth-century Spain and is still used today by composers. It is usually of a serious
      character and is often, but not always, based on a bass-ostinato and written in triple
      metre.</skos:definition>
    <skos:exactMatch xml:lang="en">http://dbpedia.org/resource/Passacaglia</skos:exactMatch>
    <skos:inScheme rdf:resource="http://data.europeana.eu/concept/music/genre/Music_Genre_Scheme"/>
    <skos:altLabel xml:lang="en">Passacaglia</skos:altLabel>
  </skos:Concept>

  <skos:Concept rdf:about="http://data.europeana.eu/concept/music/genre/Rondo_Veneziano">
    <skos:prefLabel xml:lang="en">Rondo</skos:prefLabel>
    <skos:prefLabel xml:lang="ar">روندو فينيزيانو</skos:prefLabel>
    <skos:prefLabel xml:lang="cs">Rondò Veneziano</skos:prefLabel>
    <skos:prefLabel xml:lang="fr">Rondò Veneziano</skos:prefLabel>
    <skos:prefLabel xml:lang="de">Rondò Veneziano</skos:prefLabel>
    <skos:prefLabel xml:lang="it">Rondò Veneziano</skos:prefLabel>
    <skos:prefLabel xml:lang="pl">Rondò Veneziano</skos:prefLabel>
    <skos:prefLabel xml:lang="pt">Rondò Veneziano</skos:prefLabel>
    <skos:prefLabel xml:lang="ru">Rondo Veneziano</skos:prefLabel>
    <skos:closeMatch rdf:resource="http://rdf.freebase.com/ns/m.08srqn"/>
    <skos:broader rdf:resource="http://data.europeana.eu/concept/music/genre/Classical_music"/>
    <skos:definition xml:lang="en">Rondò Veneziano is an Italian chamber orchestra, specializing in
      Baroque music, playing original instruments, but incorporating a rock-style rhythm section of
      synthesizer, bass guitar and drums, led by Maestro Gian Piero Reverberi, who is also the
      principal composer of all of the original Rondo Veneziano pieces. The unusual addition of
      modern instruments, more suitable for Jazz, combined with Reverberi's arrangements and
      original compositions, have resulted in lavish novel versions of classical works over the
      years. As a rule in their concert tours, the musicians, mostly women, add to the overall
      Baroque effect wearing Baroque-era attires and coiffures.</skos:definition>
    <skos:exactMatch xml:lang="en">http://dbpedia.org/resource/Rondò_Veneziano</skos:exactMatch>
    <skos:inScheme rdf:resource="http://data.europeana.eu/concept/music/genre/Music_Genre_Scheme"/>
    <skos:altLabel xml:lang="en">Rondò Veneziano</skos:altLabel>
    <skos:altLabel xml:lang="en">Rondo Veneziano</skos:altLabel>
    <skos:altLabel xml:lang="en">Rondo Veneziano (by Gian Piero Reverberi)</skos:altLabel>
    <skos:altLabel xml:lang="en">Rondo' Veneziano</skos:altLabel>
    <skos:altLabel xml:lang="en">Rondo4 Veneziano</skos:altLabel>
    <skos:altLabel xml:lang="en">Rondo Venziano</skos:altLabel>
    <skos:altLabel xml:lang="en">Rondo Veneciano</skos:altLabel>
    <skos:altLabel xml:lang="en">Veneciano, Rondo</skos:altLabel>
  </skos:Concept>

  <skos:Concept rdf:about="http://data.europeana.eu/concept/music/genre/Music_of_Ecuador_Sanjuanito">
    <skos:prefLabel xml:lang="en">Sanjuanito</skos:prefLabel>
    <skos:broader
      rdf:resource="http://data.europeana.eu/concept/music/genre/Latin_American_music_traditional"/>
    <skos:definition xml:lang="en">The music of Ecuador has a long history. Pasillo is a genre of
      indigenous Latin music. In Ecuador it is the &quot;national genre of music.&quot; Through the
      years, many cultures have brought their influences together to create new types of music.
      There are also different kinds of traditional music like albazo, pasacalle, fox incaico,
      tonada, diablada pillareña, capishca, Bomba</skos:definition>
    <skos:exactMatch xml:lang="en"
      >http://dbpedia.org/resource/Music_of_Ecuador#Sanjuanito</skos:exactMatch>
    <skos:inScheme rdf:resource="http://data.europeana.eu/concept/music/genre/Music_Genre_Scheme"/>
  </skos:Concept>

  <skos:Concept rdf:about="http://data.europeana.eu/concept/music/genre/Afro-Bolivian_Saya">
    <skos:prefLabel xml:lang="en">Saya</skos:prefLabel>
    <skos:prefLabel xml:lang="de">Saya</skos:prefLabel>
    <skos:prefLabel xml:lang="es">Saya</skos:prefLabel>
    <skos:closeMatch rdf:resource="http://rdf.freebase.com/ns/m.0b6nrkn"/>
    <skos:broader
      rdf:resource="http://data.europeana.eu/concept/music/genre/Latin_American_music_traditional"/>
    <skos:definition xml:lang="en">The Afro-Bolivian Saya is an art form of traditional Andean and
      Afro-Bolivian music and dance which originated in the Department of La Paz, Bolivia. This
      dance originated in the jungles of the Yungas ares of La Paz Department. Enslaved Africans
      were taken to South America to work in a range of industries. Their customs, music, was merged
      with the native cultures gave rise to mixtures. The specific history of many of these
      practices has disappeared, but many authors have worked to identify cultural survivals in
      Afro-descended groups throughout South America. &lt;p&gt; Many dances have been derived from
      the Saya. Caporales was based on these dances, created and presented to the public for the
      first time in 1969 by the Estrada brothers who were inspired in the Afro-Bolivian Saya
      character of the Caporal . This character was, in turn, inspired by the foreman on the
      haciendas of the Yungas. &lt;p&gt; In the present day, Afro-Bolivians have used the Saya in
      their struggle to reclaim their rights within Bolivian society.</skos:definition>
    <skos:exactMatch xml:lang="en">http://dbpedia.org/resource/Afro-Bolivian_Saya</skos:exactMatch>
    <skos:inScheme rdf:resource="http://data.europeana.eu/concept/music/genre/Music_Genre_Scheme"/>
    <skos:altLabel xml:lang="en">Saya</skos:altLabel>
  </skos:Concept>

  <skos:Concept rdf:about="http://data.europeana.eu/concept/music/genre/Shange">
    <skos:prefLabel xml:lang="en">Shan'ge</skos:prefLabel>
    <skos:prefLabel xml:lang="pl">Shange</skos:prefLabel>
    <skos:closeMatch rdf:resource="http://rdf.freebase.com/ns/m.02r5pjq"/>
    <skos:broader
      rdf:resource="http://data.europeana.eu/concept/music/genre/Music_of_Asia_traditional"/>
    <skos:definition xml:lang="en">Shan'ge is a genre of Chinese folk song. They are commonly sung
      in rural provinces, the word &quot;Shan'ge&quot; means &quot;mountain song&quot;. &lt;p&gt; A
      number of different subtypes are: &lt;p&gt; Hua'er, a form popular in the northwestern China
      provinces such as Gansu, Ningxia and Qinghai, named to the Representative List of the
      Intangible Cultural Heritage of Humanity in 2009 &lt;p&gt; Xintianyou and Shan'qu are popular
      in Shaanxi and Shanxi &lt;p&gt; Zhengjinghong, from the Anhui province &lt;p&gt; Xingguo, from
      the Jiangxi province &lt;p&gt; Hengyang from the Hunan Province &lt;p&gt; Hakka hill song from
      the Guangdong Province &lt;p&gt; Lalu, a Tibetan shan'ge &lt;p&gt; Changdiao, a Mongolian
      shan'ge &lt;p&gt; Feige, a Miao shan'ge</skos:definition>
    <skos:exactMatch xml:lang="en">http://dbpedia.org/resource/Shan'ge</skos:exactMatch>
    <skos:inScheme rdf:resource="http://data.europeana.eu/concept/music/genre/Music_Genre_Scheme"/>
    <skos:altLabel xml:lang="en">Shan'ge</skos:altLabel>
  </skos:Concept>

  <skos:Concept rdf:about="http://data.europeana.eu/concept/music/genre/Shimmy">
    <skos:prefLabel xml:lang="en">Shimmy</skos:prefLabel>
    <skos:prefLabel xml:lang="fr">Shimmy</skos:prefLabel>
    <skos:prefLabel xml:lang="de">Shimmy</skos:prefLabel>
    <skos:prefLabel xml:lang="ja">シミー</skos:prefLabel>
    <skos:prefLabel xml:lang="pl">Shimmy</skos:prefLabel>
    <skos:prefLabel xml:lang="es">Shimmy</skos:prefLabel>
    <skos:closeMatch rdf:resource="http://rdf.freebase.com/ns/m.02v1zs"/>
    <skos:broader rdf:resource="http://data.europeana.eu/concept/music/genre/Art_music"/>
    <skos:definition xml:lang="en">A shimmy is a dance move in which the body is held still, except
      for the shoulders, which are alternated back and forth. When the right shoulder goes back, the
      left one comes forward. It may help to hold the arms out slightly bent at the elbow, and when
      the shoulders are moved, keep the hands in the same position. In 1917, a dance-song titled
      &quot;Shim-Me-Sha-Wabble&quot; by Spencer Williams was published, as was &quot;The Jazz
      Dance&quot;, which included the &quot;Shimmy-She&quot;, among others. Flappers often performed
      the dance in the 1920s. The origin of the name is often attributed to Gilda Gray, a Polish
      emigrant to America. An anecdote says that when she was asked about her dancing style, she
      answered, in heavy accent, &quot;I'm shaking my chemise&quot;. However, in an interview Gilda
      denied having said this, and earlier usages of the word are recorded. In the late 1910s others
      were also attributed as being the &quot;inventor&quot; of the shimmy, including Bee Palmer.
      Mae West, in her autobiography Goodness Had Nothing to Do with It, claimed to have retitled
      the &quot;Shimmy-Shawobble&quot; as the Shimmy herself, after seeing the moves in some black
      nightclubs. &lt;p&gt; The move is also known under different names in various folk dances, in
      Gypsy dances. In Russian this move is called &quot;Tsyganochka&quot;, or &quot;gypsy
      girl&quot;, and is done by gypsy female dancers to produce a chime of costume decorations made
      of the sewn-on coins.</skos:definition>
    <skos:exactMatch xml:lang="en">http://dbpedia.org/resource/Shimmy</skos:exactMatch>
    <skos:inScheme rdf:resource="http://data.europeana.eu/concept/music/genre/Music_Genre_Scheme"/>
    <skos:altLabel xml:lang="en">Shimmy</skos:altLabel>
  </skos:Concept>

  <skos:Concept rdf:about="http://data.europeana.eu/concept/music/genre/Sonata">
    <skos:prefLabel xml:lang="en">Sonata</skos:prefLabel>
    <skos:prefLabel xml:lang="ar">سوناتا</skos:prefLabel>
    <skos:prefLabel xml:lang="bg">Соната</skos:prefLabel>
    <skos:prefLabel xml:lang="ca">Sonata</skos:prefLabel>
    <skos:prefLabel xml:lang="hr">Sonata</skos:prefLabel>
    <skos:prefLabel xml:lang="cs">Sonáta</skos:prefLabel>
    <skos:prefLabel xml:lang="da">Sonate</skos:prefLabel>
    <skos:prefLabel xml:lang="nl">Sonate</skos:prefLabel>
    <skos:prefLabel xml:lang="et">Sonaat</skos:prefLabel>
    <skos:prefLabel xml:lang="fi">Sonaatti</skos:prefLabel>
    <skos:prefLabel xml:lang="fr">Sonate</skos:prefLabel>
    <skos:prefLabel xml:lang="de">Sonate</skos:prefLabel>
    <skos:prefLabel xml:lang="el">Σονάτα</skos:prefLabel>
    <skos:prefLabel xml:lang="hu">Szonáta</skos:prefLabel>
    <skos:prefLabel xml:lang="id">Sonata</skos:prefLabel>
    <skos:prefLabel xml:lang="it">Sonata</skos:prefLabel>
    <skos:prefLabel xml:lang="ja">ソナタ</skos:prefLabel>
    <skos:prefLabel xml:lang="ko">소나타</skos:prefLabel>
    <skos:prefLabel xml:lang="lv">Sonāte</skos:prefLabel>
    <skos:prefLabel xml:lang="lt">Sonata</skos:prefLabel>
    <skos:prefLabel xml:lang="no">Sonate</skos:prefLabel>
    <skos:prefLabel xml:lang="fa">سونات</skos:prefLabel>
    <skos:prefLabel xml:lang="pl">Sonata</skos:prefLabel>
    <skos:prefLabel xml:lang="pt">Sonata</skos:prefLabel>
    <skos:prefLabel xml:lang="ro">Sonată</skos:prefLabel>
    <skos:prefLabel xml:lang="ru">Соната</skos:prefLabel>
    <skos:prefLabel xml:lang="sr">Соната</skos:prefLabel>
    <skos:prefLabel xml:lang="sk">Sonáta</skos:prefLabel>
    <skos:prefLabel xml:lang="sl">Sonata</skos:prefLabel>
    <skos:prefLabel xml:lang="es">Sonata</skos:prefLabel>
    <skos:prefLabel xml:lang="sv">Sonat</skos:prefLabel>
    <skos:prefLabel xml:lang="tr">Sonat</skos:prefLabel>
    <skos:prefLabel xml:lang="uk">Соната</skos:prefLabel>
    <skos:prefLabel xml:lang="vi">Sonata</skos:prefLabel>
    <skos:closeMatch rdf:resource="http://rdf.freebase.com/ns/m.0c0yr"/>
    <skos:broader rdf:resource="http://data.europeana.eu/concept/music/genre/Classical_music"/>
    <skos:definition xml:lang="en">Sonata, in music, literally means a piece played as opposed to a
      cantata, a piece sung. The term, being vague, evolved through the history of music,
      designating a variety of forms until the Classical era, when it took on increasing importance,
      and by the early 19th century came to represent a principle of composing large scale works. It
      was applied to most instrumental genres and regarded—alongside the fugue—as one of two
      fundamental methods of organizing, interpreting and analyzing concert music. Though the
      musical style of sonatas has changed since the Classical era, most 20th- and 21st-century
      sonatas still maintain the same structure.</skos:definition>
    <skos:exactMatch xml:lang="en">http://dbpedia.org/resource/Sonata</skos:exactMatch>
    <skos:inScheme rdf:resource="http://data.europeana.eu/concept/music/genre/Music_Genre_Scheme"/>
    <skos:altLabel xml:lang="en">Sonata</skos:altLabel>
  </skos:Concept>

  <skos:Concept rdf:about="http://data.europeana.eu/concept/music/genre/Music_of_Bolivia_Taquirari">
    <skos:prefLabel xml:lang="en">Taquirari</skos:prefLabel>
    <skos:broader
      rdf:resource="http://data.europeana.eu/concept/music/genre/Latin_American_music_traditional"/>
    <skos:inScheme rdf:resource="http://data.europeana.eu/concept/music/genre/Music_Genre_Scheme"/>
  </skos:Concept>

  <skos:Concept rdf:about="http://data.europeana.eu/concept/music/genre/Tonada">
    <skos:prefLabel xml:lang="en">Tonada</skos:prefLabel>
    <skos:prefLabel xml:lang="es">Tonada</skos:prefLabel>
    <skos:closeMatch rdf:resource="http://rdf.freebase.com/ns/m.0m0fmr9"/>
    <skos:broader
      rdf:resource="http://data.europeana.eu/concept/music/genre/Latin_American_music_traditional"/>
    <skos:definition xml:lang="en">The tonada is a folk music style of Latin America, particularly
      Chile, but also documented in Peru and elsewhere. Although tonada is a Spanish word which can
      mean anything sung, played or danced, musicological usage in Spanish and English is more
      specific.</skos:definition>
    <skos:exactMatch xml:lang="en">http://dbpedia.org/resource/Tonada</skos:exactMatch>
    <skos:inScheme rdf:resource="http://data.europeana.eu/concept/music/genre/Music_Genre_Scheme"/>
    <skos:altLabel xml:lang="en">Tonada</skos:altLabel>
  </skos:Concept>

  <skos:Concept rdf:about="http://data.europeana.eu/concept/music/genre/Mariachi">
    <skos:prefLabel xml:lang="en">Mariachi</skos:prefLabel>
    <skos:prefLabel xml:lang="ca">Mariatxi</skos:prefLabel>
    <skos:prefLabel xml:lang="hr">Mariachi</skos:prefLabel>
    <skos:prefLabel xml:lang="da">Mariachi</skos:prefLabel>
    <skos:prefLabel xml:lang="nl">Mariachi</skos:prefLabel>
    <skos:prefLabel xml:lang="fi">Mariachi</skos:prefLabel>
    <skos:prefLabel xml:lang="fr">Mariachi</skos:prefLabel>
    <skos:prefLabel xml:lang="de">Mariachi</skos:prefLabel>
    <skos:prefLabel xml:lang="it">Mariachi</skos:prefLabel>
    <skos:prefLabel xml:lang="ja">マリアッチ</skos:prefLabel>
    <skos:prefLabel xml:lang="ko">마리아치</skos:prefLabel>
    <skos:prefLabel xml:lang="lt">Mariači</skos:prefLabel>
    <skos:prefLabel xml:lang="no">Mariachi</skos:prefLabel>
    <skos:prefLabel xml:lang="fa">ماریاچی</skos:prefLabel>
    <skos:prefLabel xml:lang="pl">Mariachi</skos:prefLabel>
    <skos:prefLabel xml:lang="pt">Mariachi</skos:prefLabel>
    <skos:prefLabel xml:lang="ro">Mariachi</skos:prefLabel>
    <skos:prefLabel xml:lang="ru">Мариачи</skos:prefLabel>
    <skos:prefLabel xml:lang="sr">Маријачи</skos:prefLabel>
    <skos:prefLabel xml:lang="es">Mariachi</skos:prefLabel>
    <skos:prefLabel xml:lang="sv">Mariachi</skos:prefLabel>
    <skos:prefLabel xml:lang="uk">Маріачі</skos:prefLabel>
    <skos:closeMatch rdf:resource="http://rdf.freebase.com/ns/m.01_qs1"/>
    <skos:broader
      rdf:resource="http://data.europeana.eu/concept/music/genre/Latin_American_music_fusions"/>
    <skos:definition xml:lang="en">Mariachi is a form of folk music from Mexico. Mariachi began as a
      regional folk style called “Son Jaliscience” in the center west of Mexico originally played
      only with string instruments and musicians dressed in the white pants and shirts of peasant
      farmers. From the 19th to 20th century, migrations from rural areas into cities such as
      Guadalajara and Mexico City, along with the Mexican government's cultural promotion gradually
      re-labeled it as Son style, with its alternative name of “mariachi” becoming used for the
      “urban” form. Modifications of the music include influences from other music such as polkas
      and waltzes, the addition of trumpets and the use of charro outfits by mariachi musicians. The
      musical style began to take on national prominence in the first half of the 20th century, with
      its promotion at presidential inaugurations and on the radio in the 1920s.</skos:definition>
    <skos:exactMatch xml:lang="en">http://dbpedia.org/resource/Mariachi</skos:exactMatch>
    <skos:inScheme rdf:resource="http://data.europeana.eu/concept/music/genre/Music_Genre_Scheme"/>
    <skos:altLabel xml:lang="en">Mariachi</skos:altLabel>
  </skos:Concept>

  <skos:Concept rdf:about="http://data.europeana.eu/concept/music/genre/Synthpunk">
    <skos:prefLabel xml:lang="en">Synthpunk</skos:prefLabel>
    <skos:prefLabel xml:lang="cs">Synthpunk</skos:prefLabel>
    <skos:prefLabel xml:lang="nl">Electropunk</skos:prefLabel>
    <skos:prefLabel xml:lang="fr">Synthpunk</skos:prefLabel>
    <skos:prefLabel xml:lang="de">Electropunk</skos:prefLabel>
    <skos:prefLabel xml:lang="hu">Elektropunk</skos:prefLabel>
    <skos:prefLabel xml:lang="it">Synthpunk</skos:prefLabel>
    <skos:prefLabel xml:lang="pt">Synthpunk</skos:prefLabel>
    <skos:prefLabel xml:lang="ru">Синтипанк</skos:prefLabel>
    <skos:prefLabel xml:lang="sk">Synthpunk</skos:prefLabel>
    <skos:prefLabel xml:lang="es">Synthpunk</skos:prefLabel>
    <skos:closeMatch rdf:resource="http://rdf.freebase.com/ns/m.01_sz1"/>
    <skos:broader
      rdf:resource="http://data.europeana.eu/concept/music/genre/Electronic_rock_fusions"/>
    <skos:definition xml:lang="en">Synthpunk is a music genre combining elements of electronic music
      and punk rock.</skos:definition>
    <skos:exactMatch xml:lang="en">http://dbpedia.org/resource/Synthpunk</skos:exactMatch>
    <skos:inScheme rdf:resource="http://data.europeana.eu/concept/music/genre/Music_Genre_Scheme"/>
    <skos:altLabel xml:lang="en">Electropunk</skos:altLabel>
    <skos:altLabel xml:lang="en">Synthpunk</skos:altLabel>
  </skos:Concept>

  <skos:Concept rdf:about="http://data.europeana.eu/concept/music/genre/Post-punk">
    <skos:prefLabel xml:lang="en">Post-punk</skos:prefLabel>
    <skos:prefLabel xml:lang="bg">Пост-пънк</skos:prefLabel>
    <skos:prefLabel xml:lang="ca">Post-punk</skos:prefLabel>
    <skos:prefLabel xml:lang="cs">Post-punk</skos:prefLabel>
    <skos:prefLabel xml:lang="da">Post punk</skos:prefLabel>
    <skos:prefLabel xml:lang="nl">Postpunk</skos:prefLabel>
    <skos:prefLabel xml:lang="fi">Post-punk</skos:prefLabel>
    <skos:prefLabel xml:lang="fr">Post-punk</skos:prefLabel>
    <skos:prefLabel xml:lang="de">Post-Punk</skos:prefLabel>
    <skos:prefLabel xml:lang="it">Post-punk</skos:prefLabel>
    <skos:prefLabel xml:lang="ja">ポストパンク</skos:prefLabel>
    <skos:prefLabel xml:lang="ko">포스트 펑크</skos:prefLabel>
    <skos:prefLabel xml:lang="lv">Postpankroks</skos:prefLabel>
    <skos:prefLabel xml:lang="no">Post-punk</skos:prefLabel>
    <skos:prefLabel xml:lang="fa">پست-پانک</skos:prefLabel>
    <skos:prefLabel xml:lang="pl">Post punk</skos:prefLabel>
    <skos:prefLabel xml:lang="pt">Pós-punk</skos:prefLabel>
    <skos:prefLabel xml:lang="ro">Post-punk</skos:prefLabel>
    <skos:prefLabel xml:lang="ru">Пост-панк</skos:prefLabel>
    <skos:prefLabel xml:lang="sr">Post-pank</skos:prefLabel>
    <skos:prefLabel xml:lang="sk">Post-punk</skos:prefLabel>
    <skos:prefLabel xml:lang="es">Post-punk</skos:prefLabel>
    <skos:prefLabel xml:lang="sv">Postpunk</skos:prefLabel>
    <skos:prefLabel xml:lang="th">โพสต์พังค์</skos:prefLabel>
    <skos:prefLabel xml:lang="tr">Post-punk</skos:prefLabel>
    <skos:prefLabel xml:lang="uk">Пост-панк</skos:prefLabel>
    <skos:closeMatch rdf:resource="http://rdf.freebase.com/ns/m.011j5x"/>
    <skos:broader rdf:resource="http://data.europeana.eu/concept/music/genre/Rock_music_fusions"/>
    <skos:definition xml:lang="en">Post-punk is a rock music genre that paralleled and emerged from
      the initial punk rock explosion of the late 1970s. The genre is an artsier and more
      experimental form of punk. Post-punk laid the groundwork for alternative rock by broadening
      the range of punk and underground music, incorporating elements of krautrock, dub music,
      American funk and studio experimentation into the genre. It was the focus of the 1980s
      alternative music/independent scene, and led to the development of genres such as gothic rock
      and industrial music.</skos:definition>
    <skos:exactMatch xml:lang="en">http://dbpedia.org/resource/Post-punk</skos:exactMatch>
    <skos:inScheme rdf:resource="http://data.europeana.eu/concept/music/genre/Music_Genre_Scheme"/>
    <skos:altLabel xml:lang="en">Post-punk</skos:altLabel>
  </skos:Concept>

  <skos:Concept rdf:about="http://data.europeana.eu/concept/music/genre/Indie_rock">
    <skos:prefLabel xml:lang="en">Indie rock</skos:prefLabel>
    <skos:prefLabel xml:lang="ar">إندي روك</skos:prefLabel>
    <skos:prefLabel xml:lang="bg">Инди рок</skos:prefLabel>
    <skos:prefLabel xml:lang="ca">Indie rock</skos:prefLabel>
    <skos:prefLabel xml:lang="cs">Indie rock</skos:prefLabel>
    <skos:prefLabel xml:lang="da">Indie rock</skos:prefLabel>
    <skos:prefLabel xml:lang="nl">Indie</skos:prefLabel>
    <skos:prefLabel xml:lang="et">Indie rock</skos:prefLabel>
    <skos:prefLabel xml:lang="fi">Indie rock</skos:prefLabel>
    <skos:prefLabel xml:lang="fr">Rock indépendant</skos:prefLabel>
    <skos:prefLabel xml:lang="de">Indie-Rock</skos:prefLabel>
    <skos:prefLabel xml:lang="hu">Indie rock</skos:prefLabel>
    <skos:prefLabel xml:lang="it">Indie rock</skos:prefLabel>
    <skos:prefLabel xml:lang="ja">インディー・ロック</skos:prefLabel>
    <skos:prefLabel xml:lang="ko">인디 록</skos:prefLabel>
    <skos:prefLabel xml:lang="lv">Indīroks</skos:prefLabel>
    <skos:prefLabel xml:lang="lt">Indie Rock</skos:prefLabel>
    <skos:prefLabel xml:lang="ms">Rock indie</skos:prefLabel>
    <skos:prefLabel xml:lang="no">Indie-rock</skos:prefLabel>
    <skos:prefLabel xml:lang="fa">ایندی راک</skos:prefLabel>
    <skos:prefLabel xml:lang="pl">Indie rock</skos:prefLabel>
    <skos:prefLabel xml:lang="pt">Indie rock</skos:prefLabel>
    <skos:prefLabel xml:lang="ro">Indie rock</skos:prefLabel>
    <skos:prefLabel xml:lang="ru">Инди-рок</skos:prefLabel>
    <skos:prefLabel xml:lang="sr">Indi rok</skos:prefLabel>
    <skos:prefLabel xml:lang="sk">Indie rock</skos:prefLabel>
    <skos:prefLabel xml:lang="sl">Indie rock</skos:prefLabel>
    <skos:prefLabel xml:lang="es">Indie rock</skos:prefLabel>
    <skos:prefLabel xml:lang="sv">Indierock</skos:prefLabel>
    <skos:prefLabel xml:lang="th">อินดี้ร็อก</skos:prefLabel>
    <skos:prefLabel xml:lang="tr">Bağımsız rock</skos:prefLabel>
    <skos:prefLabel xml:lang="uk">Інді-рок</skos:prefLabel>
    <skos:prefLabel xml:lang="vi">Indie rock</skos:prefLabel>
    <skos:closeMatch rdf:resource="http://rdf.freebase.com/ns/m.01243b"/>
    <skos:broader
      rdf:resource="http://data.europeana.eu/concept/music/genre/Alternative_rock_fusions"/>
    <skos:definition xml:lang="en">Indie rock is a genre of alternative rock that originated in the
      United Kingdom and the United States in the 1980s. Indie rock is extremely diverse, with
      sub-genres that include indie pop, jangle pop, C86, and lo-fi, among others. Originally used
      to describe record labels, the term became associated with the music they produced and was
      initially used interchangeably with alternative rock. As grunge and punk revival bands in the
      US, and then Britpop bands in the UK, broke into the mainstream in the 1990s, it came to be
      used to identify those acts that retained an outsider and underground perspective. In the
      2000s, as a result of changes in the music industry and the growing importance of the
      Internet, a number of indie rock acts began to enjoy commercial success, leading to questions
      about its meaningfulness as a term.</skos:definition>
    <skos:exactMatch xml:lang="en">http://dbpedia.org/resource/Indie_rock</skos:exactMatch>
    <skos:inScheme rdf:resource="http://data.europeana.eu/concept/music/genre/Music_Genre_Scheme"/>
    <skos:altLabel xml:lang="en">Indie rock</skos:altLabel>
  </skos:Concept>

  <skos:Concept rdf:about="http://data.europeana.eu/concept/music/genre/Alternative_hip_hop">
    <skos:prefLabel xml:lang="en">Alternative hip hop</skos:prefLabel>
    <skos:prefLabel xml:lang="ar">هيب هوب بديل</skos:prefLabel>
    <skos:prefLabel xml:lang="nl">Alternatieve hiphop</skos:prefLabel>
    <skos:prefLabel xml:lang="fr">Hip-hop alternatif</skos:prefLabel>
    <skos:prefLabel xml:lang="de">Alternative Hip-Hop</skos:prefLabel>
    <skos:prefLabel xml:lang="it">Alternative rap</skos:prefLabel>
    <skos:prefLabel xml:lang="ja">オルタナティブ・ヒップホップ</skos:prefLabel>
    <skos:prefLabel xml:lang="ko">얼터너티브 힙합</skos:prefLabel>
    <skos:prefLabel xml:lang="lt">Alternatyvus hip hopas</skos:prefLabel>
    <skos:prefLabel xml:lang="no">Alternativ hip hop</skos:prefLabel>
    <skos:prefLabel xml:lang="pl">Alternatywny hip-hop</skos:prefLabel>
    <skos:prefLabel xml:lang="pt">Hip hop alternativo</skos:prefLabel>
    <skos:prefLabel xml:lang="ru">Альтернативный хип-хоп</skos:prefLabel>
    <skos:prefLabel xml:lang="sk">Alternatívny hip-hop</skos:prefLabel>
    <skos:prefLabel xml:lang="es">Rap alternativo</skos:prefLabel>
    <skos:prefLabel xml:lang="sv">Alternativ hiphop</skos:prefLabel>
    <skos:prefLabel xml:lang="th">อัลเทอร์เนทีฟฮิปฮอป</skos:prefLabel>
    <skos:prefLabel xml:lang="uk">Альтернативний хіп-хоп</skos:prefLabel>
    <skos:closeMatch rdf:resource="http://rdf.freebase.com/ns/m.012yc"/>
    <skos:broader rdf:resource="http://data.europeana.eu/concept/music/genre/Hip_hop_music_fusions"/>
    <skos:definition xml:lang="en">Alternative hip hop is a sub-genre of hip hop music that
      encompasses the wide range of styles of hip hop that have not become identified as mainstream.
      Allmusic defines it as follows: &lt;p&gt; Alternative rap refers to hip hop groups that tend
      not to conform to any of the traditional stereotypes of rap, such as gangsta, bass, hardcore,
      pop, and party rap. Instead, they blur genres - drawing equally from funk and rock, as well as
      jazz, soul, reggae, country, electronica, and even folk.</skos:definition>
    <skos:exactMatch xml:lang="en">http://dbpedia.org/resource/Alternative_hip_hop</skos:exactMatch>
    <skos:inScheme rdf:resource="http://data.europeana.eu/concept/music/genre/Music_Genre_Scheme"/>
    <skos:altLabel xml:lang="en">Underground Rap</skos:altLabel>
    <skos:altLabel xml:lang="en">Alternative hip hop</skos:altLabel>
  </skos:Concept>

  <skos:Concept rdf:about="http://data.europeana.eu/concept/music/genre/Electroclash">
    <skos:prefLabel xml:lang="en">Electroclash</skos:prefLabel>
    <skos:prefLabel xml:lang="ca">Electroclash</skos:prefLabel>
    <skos:prefLabel xml:lang="da">Electroclash</skos:prefLabel>
    <skos:prefLabel xml:lang="nl">Electroclash</skos:prefLabel>
    <skos:prefLabel xml:lang="fi">Electroclash</skos:prefLabel>
    <skos:prefLabel xml:lang="fr">Electroclash</skos:prefLabel>
    <skos:prefLabel xml:lang="de">Electroclash</skos:prefLabel>
    <skos:prefLabel xml:lang="it">Electroclash</skos:prefLabel>
    <skos:prefLabel xml:lang="ja">エレクトロクラッシュ</skos:prefLabel>
    <skos:prefLabel xml:lang="ko">일렉트로클래시</skos:prefLabel>
    <skos:prefLabel xml:lang="pl">Electroclash</skos:prefLabel>
    <skos:prefLabel xml:lang="pt">Electroclash</skos:prefLabel>
    <skos:prefLabel xml:lang="ru">Электроклэш</skos:prefLabel>
    <skos:prefLabel xml:lang="sk">Electroclash</skos:prefLabel>
    <skos:prefLabel xml:lang="es">Electroclash</skos:prefLabel>
    <skos:prefLabel xml:lang="sv">Electroclash</skos:prefLabel>
    <skos:prefLabel xml:lang="tr">Electroclash</skos:prefLabel>
    <skos:prefLabel xml:lang="uk">Електроклеш</skos:prefLabel>
    <skos:closeMatch rdf:resource="http://rdf.freebase.com/ns/m.0133k0"/>
    <skos:broader
      rdf:resource="http://data.europeana.eu/concept/music/genre/Electronic_rock_fusions"/>
    <skos:definition xml:lang="en">Electroclash, also known as retro electro, tech pop, nouveau
      disco, the new new wave – and ambiguously both synthcore and electropunk – is a style of music
      that fuses 1980s electro and new wave synthpop with 1990s techno and electronic dance music.
      It emerged in New York and Detroit in the later 1990s, pioneered by acts including Collider,
      I-F and those associated with Gerald Donald, and is associated with acts including Peaches,
      Adult, Legowelt, and Fischerspooner. It was popularised by the Electroclash Festival in 2001
      and 2002 and subsequent European tours, but faded as a distinctive style in the early 2000s,
      when it was fused with tech house to form the electro house genre.</skos:definition>
    <skos:exactMatch xml:lang="en">http://dbpedia.org/resource/Electroclash</skos:exactMatch>
    <skos:inScheme rdf:resource="http://data.europeana.eu/concept/music/genre/Music_Genre_Scheme"/>
    <skos:altLabel xml:lang="en">Electroclash</skos:altLabel>
  </skos:Concept>

  <skos:Concept
    rdf:about="http://data.europeana.eu/concept/music/genre/Contemporary_Christian_music">
    <skos:prefLabel xml:lang="en">Contemporary Christian music</skos:prefLabel>
    <skos:prefLabel xml:lang="hr">Suvremena kršćanska glazba</skos:prefLabel>
    <skos:prefLabel xml:lang="fi">Contemporary Christian Music</skos:prefLabel>
    <skos:prefLabel xml:lang="de">Christliche Popmusik</skos:prefLabel>
    <skos:prefLabel xml:lang="ja">コンテンポラリー・クリスチャン・ミュージック</skos:prefLabel>
    <skos:prefLabel xml:lang="ko">현대 기독교 음악</skos:prefLabel>
    <skos:prefLabel xml:lang="pl">Współczesna muzyka chrześcijańska</skos:prefLabel>
    <skos:prefLabel xml:lang="pt">Música cristã contemporânea</skos:prefLabel>
    <skos:prefLabel xml:lang="ru">Современная христианская музыка</skos:prefLabel>
    <skos:prefLabel xml:lang="sl">Duhovna ritmična glasba</skos:prefLabel>
    <skos:prefLabel xml:lang="es">Ardent Records</skos:prefLabel>
    <skos:prefLabel xml:lang="sv">Samtida kristen musik</skos:prefLabel>
    <skos:closeMatch rdf:resource="http://rdf.freebase.com/ns/m.0145rs"/>
    <skos:broader rdf:resource="http://data.europeana.eu/concept/music/genre/Pop_music_fusions"/>
    <skos:definition xml:lang="en">Contemporary Christian music is a genre of modern popular music
      which is lyrically focused on matters concerned with the Christian faith. It formed as those
      affected by the 1960s Jesus movement revival began to express themselves in a more
      contemporary style of music than the hymns, Gospel and Southern Gospel music that was
      prevalent in the church at the time. Today, the term is typically used to refer to pop, rock,
      or praise &amp; worship styles. &lt;p&gt; It has representation on several music charts
      including Billboard's Christian Albums, Christian Songs, Hot Christian AC, Christian CHR, Soft
      AC/Inspirational, and Christian Digital Songs as well as the UK's Official Christian &amp;
      Gospel Albums Chart. Top-selling CCM artists will also appear on the Billboard 200. In the
      iTunes Store, the genre is represented as part of the Christian and gospel
      genre.</skos:definition>
    <skos:exactMatch xml:lang="en"
      >http://dbpedia.org/resource/Contemporary_Christian_music</skos:exactMatch>
    <skos:inScheme rdf:resource="http://data.europeana.eu/concept/music/genre/Music_Genre_Scheme"/>
    <skos:altLabel xml:lang="en">Contemporary Christian music</skos:altLabel>
  </skos:Concept>

  <skos:Concept rdf:about="http://data.europeana.eu/concept/music/genre/Southern_rock">
    <skos:prefLabel xml:lang="en">Southern rock</skos:prefLabel>
    <skos:prefLabel xml:lang="cs">Jižanský rock</skos:prefLabel>
    <skos:prefLabel xml:lang="da">Southern rock</skos:prefLabel>
    <skos:prefLabel xml:lang="nl">Southern rock</skos:prefLabel>
    <skos:prefLabel xml:lang="fi">Southern rock</skos:prefLabel>
    <skos:prefLabel xml:lang="fr">Rock sudiste</skos:prefLabel>
    <skos:prefLabel xml:lang="de">Southern Rock</skos:prefLabel>
    <skos:prefLabel xml:lang="it">Southern rock</skos:prefLabel>
    <skos:prefLabel xml:lang="ja">サザン・ロック</skos:prefLabel>
    <skos:prefLabel xml:lang="ko">서던 록</skos:prefLabel>
    <skos:prefLabel xml:lang="lt">Pietietiškas rokas</skos:prefLabel>
    <skos:prefLabel xml:lang="no">Southern rock</skos:prefLabel>
    <skos:prefLabel xml:lang="fa">راک جنوبی</skos:prefLabel>
    <skos:prefLabel xml:lang="pl">Southern rock</skos:prefLabel>
    <skos:prefLabel xml:lang="pt">Southern rock</skos:prefLabel>
    <skos:prefLabel xml:lang="ru">Сатерн-рок</skos:prefLabel>
    <skos:prefLabel xml:lang="sk">Južanský rock</skos:prefLabel>
    <skos:prefLabel xml:lang="es">Rock sureño</skos:prefLabel>
    <skos:prefLabel xml:lang="sv">Southern rock</skos:prefLabel>
    <skos:closeMatch rdf:resource="http://rdf.freebase.com/ns/m.015pdg"/>
    <skos:broader rdf:resource="http://data.europeana.eu/concept/music/genre/Rock_music_fusions"/>
    <skos:definition xml:lang="en">Southern rock is a subgenre of rock music and a genre of
      Americana. It developed in the Southern United States from rock and roll, country music, and
      blues, and is focused generally on electric guitar and vocals. Although the origin of the term
      southern rock is unknown, &quot;many people feel that these important contributors to the
      development of rock and roll have been minimized in rock's history.&quot; The most important
      figures of southern rock can be listed as The Allman Brothers Band, Lynyrd Skynyrd, Dixie
      Dregs, Molly Hatchet, the Marshall Tucker Band, The Outlaws, the Charlie Daniels Band and 38
      Special.</skos:definition>
    <skos:exactMatch xml:lang="en">http://dbpedia.org/resource/Southern_rock</skos:exactMatch>
    <skos:inScheme rdf:resource="http://data.europeana.eu/concept/music/genre/Music_Genre_Scheme"/>
    <skos:altLabel xml:lang="en">Southern rock</skos:altLabel>
  </skos:Concept>

  <skos:Concept rdf:about="http://data.europeana.eu/concept/music/genre/West_Coast_hip_hop">
    <skos:prefLabel xml:lang="en">West Coast hip hop</skos:prefLabel>
    <skos:prefLabel xml:lang="cs">West Coast rap</skos:prefLabel>
    <skos:prefLabel xml:lang="da">Vestkystshiphop</skos:prefLabel>
    <skos:prefLabel xml:lang="nl">West Coast hiphop</skos:prefLabel>
    <skos:prefLabel xml:lang="fi">West Coast hip hop</skos:prefLabel>
    <skos:prefLabel xml:lang="fr">Rap West Coast</skos:prefLabel>
    <skos:prefLabel xml:lang="de">Westcoast-Hip-Hop</skos:prefLabel>
    <skos:prefLabel xml:lang="it">West Coast rap</skos:prefLabel>
    <skos:prefLabel xml:lang="ja">ウエスト・コースト・ヒップホップ</skos:prefLabel>
    <skos:prefLabel xml:lang="ko">웨스트 코스트 힙합</skos:prefLabel>
    <skos:prefLabel xml:lang="lv">Rietumkrasta hiphops</skos:prefLabel>
    <skos:prefLabel xml:lang="no">Vestkystrap</skos:prefLabel>
    <skos:prefLabel xml:lang="fa">وست کوست هیپ هاپ</skos:prefLabel>
    <skos:prefLabel xml:lang="pl">West Coast hip-hop</skos:prefLabel>
    <skos:prefLabel xml:lang="pt">West Coast hip hop</skos:prefLabel>
    <skos:prefLabel xml:lang="ru">Хип-хоп Западного побережья</skos:prefLabel>
    <skos:prefLabel xml:lang="sk">West Coast hip-hop</skos:prefLabel>
    <skos:prefLabel xml:lang="es">West Coast rap</skos:prefLabel>
    <skos:prefLabel xml:lang="sv">Västkusthiphop</skos:prefLabel>
    <skos:prefLabel xml:lang="th">เวสต์โคสต์ฮิปฮอป</skos:prefLabel>
    <skos:prefLabel xml:lang="tr">West Coast hip hop</skos:prefLabel>
    <skos:prefLabel xml:lang="uk">Хіп-хоп Західного узбережжя</skos:prefLabel>
    <skos:closeMatch rdf:resource="http://rdf.freebase.com/ns/m.016_rm"/>
    <skos:broader rdf:resource="http://data.europeana.eu/concept/music/genre/Hip_hop_music_fusions"/>
    <skos:definition xml:lang="en">West Coast hip hop is a hip hop music subgenre that encompasses
      any artists or music that originates in the Western United States region of the United States.
      The gangsta rap subgenre of West Coast hip hop began to dominate from a radio play and sales
      standpoint during the early 1990s with the birth of G-funk and the emergence of Suge Knight's
      Death Row Records.</skos:definition>
    <skos:exactMatch xml:lang="en">http://dbpedia.org/resource/West_Coast_hip_hop</skos:exactMatch>
    <skos:inScheme rdf:resource="http://data.europeana.eu/concept/music/genre/Music_Genre_Scheme"/>
    <skos:altLabel xml:lang="en">West Coast hip hop</skos:altLabel>
  </skos:Concept>

  <skos:Concept rdf:about="http://data.europeana.eu/concept/music/genre/Power_pop">
    <skos:prefLabel xml:lang="en">Power pop</skos:prefLabel>
    <skos:prefLabel xml:lang="ca">Power-pop</skos:prefLabel>
    <skos:prefLabel xml:lang="hr">Power pop</skos:prefLabel>
    <skos:prefLabel xml:lang="cs">Power pop</skos:prefLabel>
    <skos:prefLabel xml:lang="nl">Powerpop</skos:prefLabel>
    <skos:prefLabel xml:lang="fi">Voimapop</skos:prefLabel>
    <skos:prefLabel xml:lang="fr">Powerpop</skos:prefLabel>
    <skos:prefLabel xml:lang="de">Power Pop</skos:prefLabel>
    <skos:prefLabel xml:lang="id">Power pop</skos:prefLabel>
    <skos:prefLabel xml:lang="it">Power pop</skos:prefLabel>
    <skos:prefLabel xml:lang="ja">パワー・ポップ</skos:prefLabel>
    <skos:prefLabel xml:lang="ko">파워 팝</skos:prefLabel>
    <skos:prefLabel xml:lang="no">Powerpop</skos:prefLabel>
    <skos:prefLabel xml:lang="pl">Power pop</skos:prefLabel>
    <skos:prefLabel xml:lang="pt">Power pop</skos:prefLabel>
    <skos:prefLabel xml:lang="ru">Пауэр-поп</skos:prefLabel>
    <skos:prefLabel xml:lang="sk">Power pop</skos:prefLabel>
    <skos:prefLabel xml:lang="es">Power pop</skos:prefLabel>
    <skos:prefLabel xml:lang="sv">Powerpop</skos:prefLabel>
    <skos:prefLabel xml:lang="th">พาวเวอร์ป็อป</skos:prefLabel>
    <skos:prefLabel xml:lang="uk">Павер-поп</skos:prefLabel>
    <skos:closeMatch rdf:resource="http://rdf.freebase.com/ns/m.016ybr"/>
    <skos:broader rdf:resource="http://data.europeana.eu/concept/music/genre/Rock_music_fusions"/>
    <skos:definition xml:lang="en">Power pop is a popular musical genre that draws its inspiration
      from 1960s British and American pop and rock music. It typically incorporates a combination of
      musical devices such as strong melodies, clear vocals and crisp vocal harmonies, economical
      arrangements and prominent guitar riffs. Instrumental solos are usually kept to a minimum, and
      blues elements are largely downplayed. &lt;p&gt; Recordings tend to display production values
      that lean toward compression and a forceful drum beat. Instruments usually include one or more
      electric guitars, an electric bass guitar, a drum kit and sometimes electric keyboards or
      synthesizers. &lt;p&gt; While its cultural impact has waxed and waned over the decades, power
      pop is among rock's most enduring subgenres.</skos:definition>
    <skos:exactMatch xml:lang="en">http://dbpedia.org/resource/Power_pop</skos:exactMatch>
    <skos:inScheme rdf:resource="http://data.europeana.eu/concept/music/genre/Music_Genre_Scheme"/>
    <skos:altLabel xml:lang="en">Power pop</skos:altLabel>
  </skos:Concept>

  <skos:Concept rdf:about="http://data.europeana.eu/concept/music/genre/Zydeco">
    <skos:prefLabel xml:lang="en">Zydeco</skos:prefLabel>
    <skos:prefLabel xml:lang="nl">Zydeco</skos:prefLabel>
    <skos:prefLabel xml:lang="fi">Zydeco</skos:prefLabel>
    <skos:prefLabel xml:lang="fr">Zarico</skos:prefLabel>
    <skos:prefLabel xml:lang="de">Zydeco</skos:prefLabel>
    <skos:prefLabel xml:lang="it">Zydeco</skos:prefLabel>
    <skos:prefLabel xml:lang="ja">ザディコ</skos:prefLabel>
    <skos:prefLabel xml:lang="ko">자이데코</skos:prefLabel>
    <skos:prefLabel xml:lang="pt">Zydeco</skos:prefLabel>
    <skos:prefLabel xml:lang="ru">Зайдеко</skos:prefLabel>
    <skos:prefLabel xml:lang="es">Zydeco</skos:prefLabel>
    <skos:prefLabel xml:lang="sv">Zydeco</skos:prefLabel>
    <skos:closeMatch rdf:resource="http://rdf.freebase.com/ns/m.016zcz"/>
    <skos:broader rdf:resource="http://data.europeana.eu/concept/music/genre/Country_music_fusions"/>
    <skos:definition xml:lang="en">Zydeco is a musical genre evolved in southwest Louisiana by
      French Creole speakers which blends blues, rhythm and blues, and music indigenous to the Ivory
      Coast and the Native people of Louisiana.</skos:definition>
    <skos:exactMatch xml:lang="en">http://dbpedia.org/resource/Zydeco</skos:exactMatch>
    <skos:inScheme rdf:resource="http://data.europeana.eu/concept/music/genre/Music_Genre_Scheme"/>
    <skos:altLabel xml:lang="en">Zydeco</skos:altLabel>
  </skos:Concept>

  <skos:Concept rdf:about="http://data.europeana.eu/concept/music/genre/Alternative_country">
    <skos:prefLabel xml:lang="en">Alternative country</skos:prefLabel>
    <skos:prefLabel xml:lang="da">Alternative country</skos:prefLabel>
    <skos:prefLabel xml:lang="nl">Twang</skos:prefLabel>
    <skos:prefLabel xml:lang="fr">Alternative country</skos:prefLabel>
    <skos:prefLabel xml:lang="de">Alternative Country</skos:prefLabel>
    <skos:prefLabel xml:lang="it">Alternative country</skos:prefLabel>
    <skos:prefLabel xml:lang="pl">Country alternatywne</skos:prefLabel>
    <skos:prefLabel xml:lang="pt">Country alternativo</skos:prefLabel>
    <skos:prefLabel xml:lang="ru">Альт-кантри</skos:prefLabel>
    <skos:prefLabel xml:lang="es">Country alternativo</skos:prefLabel>
    <skos:prefLabel xml:lang="sv">Alternativ country</skos:prefLabel>
    <skos:closeMatch rdf:resource="http://rdf.freebase.com/ns/m.016zgj"/>
    <skos:broader rdf:resource="http://data.europeana.eu/concept/music/genre/Country_music_fusions"/>
    <skos:definition xml:lang="en">Alternative country, insurgent country, or Americana is a loosely
      defined sub-genre of country music, which includes acts that differ significantly in style
      from mainstream or pop country music. It has been used to describe country music bands and
      artists that have incorporated influences ranging from roots rock, bluegrass, rockabilly,
      honky-tonk, alternative rock, folk rock, and sometimes punk. &lt;p&gt; Attempts to combine
      punk and country were pioneered by Jason and the Scorchers, and in the 1980s Southern
      Californian cowpunk scene with bands like the Long Ryders. These styles merged fully in Uncle
      Tupelo's 1990 LP No Depression, which is widely credited as being the first
      &quot;alt-country&quot; album, and gave its name to the online notice board and eventually
      magazine that underpinned the movement. Members and figures associated with Uncle Tupelo
      formed three major bands in the genre: Wilco, Son Volt and Bottle Rockets. Other influential
      bands included Blue Mountain, Whiskeytown, Blood Oranges and Drive-By Truckers, until they
      began to move more in the direction of rock music in the 2000s.</skos:definition>
    <skos:exactMatch xml:lang="en">http://dbpedia.org/resource/Alternative_country</skos:exactMatch>
    <skos:inScheme rdf:resource="http://data.europeana.eu/concept/music/genre/Music_Genre_Scheme"/>
    <skos:altLabel xml:lang="en">Alt-Country</skos:altLabel>
    <skos:altLabel xml:lang="en">Alternative country</skos:altLabel>
  </skos:Concept>

  <skos:Concept rdf:about="http://data.europeana.eu/concept/music/genre/Europop">
    <skos:prefLabel xml:lang="en">Europop</skos:prefLabel>
    <skos:prefLabel xml:lang="ar">يوروبوب</skos:prefLabel>
    <skos:prefLabel xml:lang="ca">Europop</skos:prefLabel>
    <skos:prefLabel xml:lang="fr">Europop</skos:prefLabel>
    <skos:prefLabel xml:lang="de">Europop</skos:prefLabel>
    <skos:prefLabel xml:lang="el">Europop</skos:prefLabel>
    <skos:prefLabel xml:lang="it">Europop</skos:prefLabel>
    <skos:prefLabel xml:lang="ja">ユーロポップ</skos:prefLabel>
    <skos:prefLabel xml:lang="ko">유로팝</skos:prefLabel>
    <skos:prefLabel xml:lang="fa">یوروپاپ</skos:prefLabel>
    <skos:prefLabel xml:lang="pt">Europop</skos:prefLabel>
    <skos:prefLabel xml:lang="ro">Europop</skos:prefLabel>
    <skos:prefLabel xml:lang="ru">Европоп</skos:prefLabel>
    <skos:prefLabel xml:lang="es">Europop</skos:prefLabel>
    <skos:prefLabel xml:lang="sv">Europop</skos:prefLabel>
    <skos:prefLabel xml:lang="th">ยูโรป๊อป</skos:prefLabel>
    <skos:prefLabel xml:lang="tr">Europop</skos:prefLabel>
    <skos:prefLabel xml:lang="uk">Європоп</skos:prefLabel>
    <skos:closeMatch rdf:resource="http://rdf.freebase.com/ns/m.016zxr"/>
    <skos:broader rdf:resource="http://data.europeana.eu/concept/music/genre/Pop_music_fusions"/>
    <skos:definition xml:lang="en">Europop refers to a style of pop music that first developed in
      today's form in Europe, throughout the late 1970s. Europop topped the charts throughout the
      1980s and 1990s. Many successful Europop artists came from France, Germany, Italy, Ireland,
      Netherlands and the United Kingdom, but most were Swedish in origin. &lt;p&gt; In the 1970s
      and early 1980s, such groups were primarily popular in continental countries, with the
      exception of ABBA. The Swedish four-piece band achieved great success in the UK, where they
      scored nineteen top 10 singles and nine chart-topping albums, and in North America and
      Australia. &lt;p&gt; In the late 1980s and early 1990s, Roxette and Ace of Base led Europop in
      American and British mainstream audiences. In the 1990s, pop groups like the Spice Girls,
      Aqua, Backstreet Boys and singer DJ BoBo were strongly influenced by Europop. Throughout the
      late 1990s and early 2000s, the Italian dance group Eiffel 65 were highly active in this
      genre. In the 2000s, one of the most popular representatives of Europop music was Swedish pop
      group Alcazar. &lt;p&gt; One of the main differences between American and European pop is that
      Europop is generally more dance and trance oriented.</skos:definition>
    <skos:exactMatch xml:lang="en">http://dbpedia.org/resource/Europop</skos:exactMatch>
    <skos:inScheme rdf:resource="http://data.europeana.eu/concept/music/genre/Music_Genre_Scheme"/>
    <skos:altLabel xml:lang="en">Europop</skos:altLabel>
  </skos:Concept>

  <skos:Concept rdf:about="http://data.europeana.eu/concept/music/genre/Doom_metal">
    <skos:prefLabel xml:lang="en">Doom metal</skos:prefLabel>
    <skos:prefLabel xml:lang="ar">دوم ميتال</skos:prefLabel>
    <skos:prefLabel xml:lang="hr">Doom metal</skos:prefLabel>
    <skos:prefLabel xml:lang="cs">Doom metal</skos:prefLabel>
    <skos:prefLabel xml:lang="da">Doom metal</skos:prefLabel>
    <skos:prefLabel xml:lang="nl">Doommetal</skos:prefLabel>
    <skos:prefLabel xml:lang="fi">Doom metal</skos:prefLabel>
    <skos:prefLabel xml:lang="fr">Doom metal</skos:prefLabel>
    <skos:prefLabel xml:lang="de">Doom Metal</skos:prefLabel>
    <skos:prefLabel xml:lang="el">Doom Metal</skos:prefLabel>
    <skos:prefLabel xml:lang="hu">Doom metal</skos:prefLabel>
    <skos:prefLabel xml:lang="id">Doom metal</skos:prefLabel>
    <skos:prefLabel xml:lang="it">Doom metal</skos:prefLabel>
    <skos:prefLabel xml:lang="ja">ドゥームメタル</skos:prefLabel>
    <skos:prefLabel xml:lang="ko">둠 메탈</skos:prefLabel>
    <skos:prefLabel xml:lang="lv">Dūmmetāls</skos:prefLabel>
    <skos:prefLabel xml:lang="lt">Doom metal</skos:prefLabel>
    <skos:prefLabel xml:lang="no">Doom metal</skos:prefLabel>
    <skos:prefLabel xml:lang="fa">دوم متال</skos:prefLabel>
    <skos:prefLabel xml:lang="pl">Doom metal</skos:prefLabel>
    <skos:prefLabel xml:lang="pt">Doom metal</skos:prefLabel>
    <skos:prefLabel xml:lang="ro">Doom metal</skos:prefLabel>
    <skos:prefLabel xml:lang="ru">Дум-метал</skos:prefLabel>
    <skos:prefLabel xml:lang="sr">Дум метал</skos:prefLabel>
    <skos:prefLabel xml:lang="sk">Doom metal</skos:prefLabel>
    <skos:prefLabel xml:lang="es">Doom metal</skos:prefLabel>
    <skos:prefLabel xml:lang="sv">Doom metal</skos:prefLabel>
    <skos:prefLabel xml:lang="th">ดูมเมทัล</skos:prefLabel>
    <skos:prefLabel xml:lang="tr">Doom metal</skos:prefLabel>
    <skos:prefLabel xml:lang="uk">Дум-метал</skos:prefLabel>
    <skos:closeMatch rdf:resource="http://rdf.freebase.com/ns/m.0172rj"/>
    <skos:broader
      rdf:resource="http://data.europeana.eu/concept/music/genre/Heavy_metal_music_fusions"/>
    <skos:definition xml:lang="en">Doom metal is an extreme form of heavy metal music that typically
      uses slower tempos, low-tuned guitars and a much &quot;thicker&quot; or &quot;heavier&quot;
      sound than other metal genres. Both the music and the lyrics intend to evoke a sense of
      despair, dread, and impending doom. The genre is strongly influenced by the early work of
      Black Sabbath, who formed a prototype for doom metal with songs such as &quot;Black
      Sabbath&quot;, &quot;Electric Funeral&quot; and &quot;Into the Void&quot;. During the first
      half of the 1980s, a number of bands from England, the United States and Sweden defined doom
      metal as a distinct genre.</skos:definition>
    <skos:exactMatch xml:lang="en">http://dbpedia.org/resource/Doom_metal</skos:exactMatch>
    <skos:inScheme rdf:resource="http://data.europeana.eu/concept/music/genre/Music_Genre_Scheme"/>
    <skos:altLabel xml:lang="en">Doom metal</skos:altLabel>
  </skos:Concept>

  <skos:Concept rdf:about="http://data.europeana.eu/concept/music/genre/Funk_metal">
    <skos:prefLabel xml:lang="en">Funk metal</skos:prefLabel>
    <skos:prefLabel xml:lang="cs">Funk metal</skos:prefLabel>
    <skos:prefLabel xml:lang="da">Funk metal</skos:prefLabel>
    <skos:prefLabel xml:lang="nl">Funkmetal</skos:prefLabel>
    <skos:prefLabel xml:lang="fi">Funk metal</skos:prefLabel>
    <skos:prefLabel xml:lang="fr">Funk metal</skos:prefLabel>
    <skos:prefLabel xml:lang="de">Funk Metal</skos:prefLabel>
    <skos:prefLabel xml:lang="it">Funk metal</skos:prefLabel>
    <skos:prefLabel xml:lang="ko">펑크 메탈</skos:prefLabel>
    <skos:prefLabel xml:lang="lt">Funk-metalas</skos:prefLabel>
    <skos:prefLabel xml:lang="no">Funk metal</skos:prefLabel>
    <skos:prefLabel xml:lang="pl">Funk metal</skos:prefLabel>
    <skos:prefLabel xml:lang="pt">Funk metal</skos:prefLabel>
    <skos:prefLabel xml:lang="ro">Funk metal</skos:prefLabel>
    <skos:prefLabel xml:lang="ru">Фанк метал</skos:prefLabel>
    <skos:prefLabel xml:lang="sk">Funk metal</skos:prefLabel>
    <skos:prefLabel xml:lang="es">Funk metal</skos:prefLabel>
    <skos:prefLabel xml:lang="sv">Funk metal</skos:prefLabel>
    <skos:prefLabel xml:lang="tr">Funk metal</skos:prefLabel>
    <skos:prefLabel xml:lang="uk">Фанк-метал</skos:prefLabel>
    <skos:closeMatch rdf:resource="http://rdf.freebase.com/ns/m.01738f"/>
    <skos:broader
      rdf:resource="http://data.europeana.eu/concept/music/genre/Heavy_metal_music_fusions"/>
    <skos:definition xml:lang="en">Funk metal is a subgenre of funk rock and alternative metal that
      fuses elements of heavy metal and funk.</skos:definition>
    <skos:exactMatch xml:lang="en">http://dbpedia.org/resource/Funk_metal</skos:exactMatch>
    <skos:inScheme rdf:resource="http://data.europeana.eu/concept/music/genre/Music_Genre_Scheme"/>
    <skos:altLabel xml:lang="en">Funk metal</skos:altLabel>
  </skos:Concept>

  <skos:Concept rdf:about="http://data.europeana.eu/concept/music/genre/Glam_metal">
    <skos:prefLabel xml:lang="en">Glam metal</skos:prefLabel>
    <skos:prefLabel xml:lang="ar">جلام ميتال</skos:prefLabel>
    <skos:prefLabel xml:lang="bg">Глем метъл</skos:prefLabel>
    <skos:prefLabel xml:lang="ca">Glam metal</skos:prefLabel>
    <skos:prefLabel xml:lang="hr">Glam metal</skos:prefLabel>
    <skos:prefLabel xml:lang="cs">Glam metal</skos:prefLabel>
    <skos:prefLabel xml:lang="da">Glam metal</skos:prefLabel>
    <skos:prefLabel xml:lang="nl">Glam metal</skos:prefLabel>
    <skos:prefLabel xml:lang="et">Glam metal</skos:prefLabel>
    <skos:prefLabel xml:lang="fi">Glam metal</skos:prefLabel>
    <skos:prefLabel xml:lang="fr">Glam metal</skos:prefLabel>
    <skos:prefLabel xml:lang="de">Glam Metal</skos:prefLabel>
    <skos:prefLabel xml:lang="el">Glam Metal</skos:prefLabel>
    <skos:prefLabel xml:lang="hu">Glam metal</skos:prefLabel>
    <skos:prefLabel xml:lang="id">Glam Metal</skos:prefLabel>
    <skos:prefLabel xml:lang="it">Hair metal</skos:prefLabel>
    <skos:prefLabel xml:lang="ja">グラム・メタル</skos:prefLabel>
    <skos:prefLabel xml:lang="ko">글램 메탈</skos:prefLabel>
    <skos:prefLabel xml:lang="lv">Popmetāls</skos:prefLabel>
    <skos:prefLabel xml:lang="lt">Pop metal</skos:prefLabel>
    <skos:prefLabel xml:lang="no">Glam metal</skos:prefLabel>
    <skos:prefLabel xml:lang="fa">گلم متال</skos:prefLabel>
    <skos:prefLabel xml:lang="pl">Glam metal</skos:prefLabel>
    <skos:prefLabel xml:lang="pt">Glam metal</skos:prefLabel>
    <skos:prefLabel xml:lang="ro">Glam metal</skos:prefLabel>
    <skos:prefLabel xml:lang="ru">Глэм-метал</skos:prefLabel>
    <skos:prefLabel xml:lang="sk">Glam metal</skos:prefLabel>
    <skos:prefLabel xml:lang="es">Glam metal</skos:prefLabel>
    <skos:prefLabel xml:lang="sv">Glam metal</skos:prefLabel>
    <skos:prefLabel xml:lang="th">แกลมเมทัล</skos:prefLabel>
    <skos:prefLabel xml:lang="tr">Glam metal</skos:prefLabel>
    <skos:prefLabel xml:lang="uk">Глем-метал</skos:prefLabel>
    <skos:closeMatch rdf:resource="http://rdf.freebase.com/ns/m.0173b0"/>
    <skos:broader
      rdf:resource="http://data.europeana.eu/concept/music/genre/Heavy_metal_music_fusions"/>
    <skos:definition xml:lang="en">Glam metal is a subgenre of hard rock and heavy metal. It
      combines elements of this genre with punk rock and pop music, adding catchy hooks and guitar
      riffs, while borrowing from the aesthetic of 1970s glam rock. &lt;p&gt; It arose in the late
      1970s and early 1980s in the United States, particularly on the Los Angeles Sunset Strip music
      scene, pioneered by bands such as Kix, Hanoi Rocks, Mötley Crüe, Quiet Riot, and Bon Jovi. It
      was popular throughout the 1980s and the beginning of the 1990s, bringing to prominence bands
      including Poison, Cinderella, and Warrant. &lt;p&gt; The genre rapidly lost mainstream
      interest from 1992 to 1994 with the rise of grunge and the release of albums such as Nirvana's
      Nevermind, but it has enjoyed something of a revival since the beginning of the new millennium
      with reunions of many popular acts from the genre`s 1980s heyday, as well as the retro styling
      of new bands including The Darkness and Steel Panther.</skos:definition>
    <skos:exactMatch xml:lang="en">http://dbpedia.org/resource/Glam_metal</skos:exactMatch>
    <skos:inScheme rdf:resource="http://data.europeana.eu/concept/music/genre/Music_Genre_Scheme"/>
    <skos:altLabel xml:lang="en">Glam metal</skos:altLabel>
  </skos:Concept>

  <skos:Concept rdf:about="http://data.europeana.eu/concept/music/genre/Jump_blues">
    <skos:prefLabel xml:lang="en">Jump blues</skos:prefLabel>
    <skos:prefLabel xml:lang="cs">Jump blues</skos:prefLabel>
    <skos:prefLabel xml:lang="fr">Jump blues</skos:prefLabel>
    <skos:prefLabel xml:lang="de">Jump Blues</skos:prefLabel>
    <skos:prefLabel xml:lang="it">Jump blues</skos:prefLabel>
    <skos:prefLabel xml:lang="ja">ジャンプ・ブルース</skos:prefLabel>
    <skos:prefLabel xml:lang="no">Jump-blues</skos:prefLabel>
    <skos:prefLabel xml:lang="pl">Jump blues</skos:prefLabel>
    <skos:prefLabel xml:lang="pt">Jump blues</skos:prefLabel>
    <skos:prefLabel xml:lang="es">Jump blues</skos:prefLabel>
    <skos:closeMatch rdf:resource="http://rdf.freebase.com/ns/m.01750n"/>
    <skos:broader rdf:resource="http://data.europeana.eu/concept/music/genre/Blues_fusions"/>
    <skos:definition xml:lang="en">Jump blues is an up-tempo blues usually played by small groups
      and featuring horns. It was very popular in the 1940s, and the movement was a precursor to the
      arrival of rhythm and blues and rock and roll. More recently, there was renewed interest in
      jump blues in the 1990s as part of the swing revival.</skos:definition>
    <skos:exactMatch xml:lang="en">http://dbpedia.org/resource/Jump_blues</skos:exactMatch>
    <skos:inScheme rdf:resource="http://data.europeana.eu/concept/music/genre/Music_Genre_Scheme"/>
    <skos:altLabel xml:lang="en">Jump blues</skos:altLabel>
  </skos:Concept>

  <skos:Concept rdf:about="http://data.europeana.eu/concept/music/genre/Country_blues">
    <skos:prefLabel xml:lang="en">Country blues</skos:prefLabel>
    <skos:prefLabel xml:lang="ca">Blues tradicional</skos:prefLabel>
    <skos:prefLabel xml:lang="fr">Blues traditionnel</skos:prefLabel>
    <skos:prefLabel xml:lang="de">Country Blues</skos:prefLabel>
    <skos:prefLabel xml:lang="it">Country blues</skos:prefLabel>
    <skos:prefLabel xml:lang="ja">カントリー・ブルース</skos:prefLabel>
    <skos:prefLabel xml:lang="lv">Lauku blūzs</skos:prefLabel>
    <skos:prefLabel xml:lang="no">Country blues</skos:prefLabel>
    <skos:prefLabel xml:lang="pl">Country blues</skos:prefLabel>
    <skos:prefLabel xml:lang="pt">Country blues</skos:prefLabel>
    <skos:prefLabel xml:lang="ru">Кантри-блюз</skos:prefLabel>
    <skos:prefLabel xml:lang="es">Country blues</skos:prefLabel>
    <skos:prefLabel xml:lang="sv">Countryblues</skos:prefLabel>
    <skos:prefLabel xml:lang="uk">Кантрі-блюз</skos:prefLabel>
    <skos:closeMatch rdf:resource="http://rdf.freebase.com/ns/m.017510"/>
    <skos:broader rdf:resource="http://data.europeana.eu/concept/music/genre/Country_music_fusions"/>
    <skos:definition xml:lang="en">Country blues is acoustic, mainly guitar-driven forms of the
      blues. It often incorporated elements of rural gospel, ragtime, hillbilly, and dixieland jazz.
      After blues' birth in the Southern United States, it quickly spread throughout the country,
      giving birth to a host of regional styles. These include Memphis, Detroit, Chicago, Texas,
      Piedmont, Louisiana, West Coast, Atlanta, St. Louis, East Coast, Swamp, New Orleans, Delta,
      Hill country and Kansas City blues. &lt;p&gt; When African-American musical tastes began to
      change in the early 1960s, moving toward soul and rhythm and blues music, country blues found
      renewed popularity as &quot;folk blues&quot; and was sold to a primarily white, college-age
      audience. Traditional artists like Big Bill Broonzy and Sonny Boy Williamson II reinvented
      themselves as folk blues artists, while Piedmont bluesmen like Sonny Terry and Brownie McGhee
      found great success on the folk festival circuit. Contemporary country blues artists such as
      Ramon Goose have fused country blues and African styles of music to create new hybrids.
      &lt;p&gt; Seminal compilations of pre-WWII country blues recordings assembled in the 1950s are
      the Anthology of American Folk Music and The Country Blues.</skos:definition>
    <skos:exactMatch xml:lang="en">http://dbpedia.org/resource/Country_blues</skos:exactMatch>
    <skos:inScheme rdf:resource="http://data.europeana.eu/concept/music/genre/Music_Genre_Scheme"/>
    <skos:altLabel xml:lang="en">Country blues</skos:altLabel>
  </skos:Concept>

  <skos:Concept rdf:about="http://data.europeana.eu/concept/music/genre/Highlife">
    <skos:prefLabel xml:lang="en">Highlife</skos:prefLabel>
    <skos:prefLabel xml:lang="fi">Highlife</skos:prefLabel>
    <skos:prefLabel xml:lang="fr">Highlife</skos:prefLabel>
    <skos:prefLabel xml:lang="de">Highlife</skos:prefLabel>
    <skos:prefLabel xml:lang="ja">ハイライフ</skos:prefLabel>
    <skos:prefLabel xml:lang="no">Highlife</skos:prefLabel>
    <skos:prefLabel xml:lang="pt">Highlife</skos:prefLabel>
    <skos:prefLabel xml:lang="es">Highlife</skos:prefLabel>
    <skos:prefLabel xml:lang="sv">Highlife</skos:prefLabel>
    <skos:closeMatch rdf:resource="http://rdf.freebase.com/ns/m.0175l4"/>
    <skos:broader
      rdf:resource="http://data.europeana.eu/concept/music/genre/African_popular_music_fusions"/>
    <skos:definition xml:lang="en">Highlife is a music genre that originated in Ghana at the turn of
      the 20th century and incorporated the traditional harmonic 9th, as well as melodic and the
      main rhythmic structures in traditional Akan music, and married them with Western instruments
      and ideas. Highlife was associated with the local African aristocracy during the colonial
      period. Highlife spread to Sierra Leone, Liberia, Gambia and Nigeria via Ghanaian workers,
      among other West African countries, by the 1930s. It is very popular in Liberia and all of
      English-speaking West Africa, although little has been produced in other countries due to
      economic challenges brought on by war and instability. &lt;p&gt; Highlife is characterised by
      jazzy horns and multiple guitars which lead the band. Recently it has acquired an uptempo,
      synth-driven sound. Joromi is a sub-genre. &lt;p&gt; This arpeggiated highlife guitar part is
      modeled after an Afro-Cuban guajeo. The pattern of attack-points is nearly identical to the
      3-2 clave motif guajeo shown earlier in this article. The bell pattern known in Cuba as clave
      is indigenous to Ghana and Nigeria, and is used in highlife.</skos:definition>
    <skos:exactMatch xml:lang="en">http://dbpedia.org/resource/Highlife</skos:exactMatch>
    <skos:inScheme rdf:resource="http://data.europeana.eu/concept/music/genre/Music_Genre_Scheme"/>
    <skos:altLabel xml:lang="en">Highlife</skos:altLabel>
  </skos:Concept>

  <skos:Concept rdf:about="http://data.europeana.eu/concept/music/genre/Dream_pop">
    <skos:prefLabel xml:lang="en">Dream pop</skos:prefLabel>
    <skos:prefLabel xml:lang="nl">Dreampop</skos:prefLabel>
    <skos:prefLabel xml:lang="fr">Dream pop</skos:prefLabel>
    <skos:prefLabel xml:lang="de">Dream Pop</skos:prefLabel>
    <skos:prefLabel xml:lang="it">Dream pop</skos:prefLabel>
    <skos:prefLabel xml:lang="ja">ドリーム・ポップ</skos:prefLabel>
    <skos:prefLabel xml:lang="ko">드림 팝</skos:prefLabel>
    <skos:prefLabel xml:lang="lv">Drīmpops</skos:prefLabel>
    <skos:prefLabel xml:lang="pl">Dream pop</skos:prefLabel>
    <skos:prefLabel xml:lang="pt">Dream pop</skos:prefLabel>
    <skos:prefLabel xml:lang="ru">Дрим-поп</skos:prefLabel>
    <skos:prefLabel xml:lang="es">Dream pop</skos:prefLabel>
    <skos:prefLabel xml:lang="sv">Dream pop</skos:prefLabel>
    <skos:prefLabel xml:lang="th">ดรีมป็อป</skos:prefLabel>
    <skos:prefLabel xml:lang="tr">Dream pop</skos:prefLabel>
    <skos:prefLabel xml:lang="vi">Dream pop</skos:prefLabel>
    <skos:closeMatch rdf:resource="http://rdf.freebase.com/ns/m.0175zz"/>
    <skos:broader
      rdf:resource="http://data.europeana.eu/concept/music/genre/Alternative_rock_fusions"/>
    <skos:definition xml:lang="en">Dream pop is a subgenre of alternative rock.</skos:definition>
    <skos:exactMatch xml:lang="en">http://dbpedia.org/resource/Dream_pop</skos:exactMatch>
    <skos:inScheme rdf:resource="http://data.europeana.eu/concept/music/genre/Music_Genre_Scheme"/>
    <skos:altLabel xml:lang="en">Dream pop</skos:altLabel>
  </skos:Concept>

  <skos:Concept rdf:about="http://data.europeana.eu/concept/music/genre/Makossa">
    <skos:prefLabel xml:lang="en">Makossa</skos:prefLabel>
    <skos:prefLabel xml:lang="da">Makossa</skos:prefLabel>
    <skos:prefLabel xml:lang="fr">Makossa</skos:prefLabel>
    <skos:prefLabel xml:lang="de">Makossa</skos:prefLabel>
    <skos:prefLabel xml:lang="id">Makossa</skos:prefLabel>
    <skos:prefLabel xml:lang="it">Makossa</skos:prefLabel>
    <skos:prefLabel xml:lang="ja">マコッサ</skos:prefLabel>
    <skos:prefLabel xml:lang="no">Makossa</skos:prefLabel>
    <skos:prefLabel xml:lang="pt">Makossa</skos:prefLabel>
    <skos:prefLabel xml:lang="es">Makossa</skos:prefLabel>
    <skos:closeMatch rdf:resource="http://rdf.freebase.com/ns/m.0176kg"/>
    <skos:broader
      rdf:resource="http://data.europeana.eu/concept/music/genre/African_popular_music_fusions"/>
    <skos:definition xml:lang="en">Makossa is a noted Cameroonian popular urban musical style. Like
      much other late 20th century music of Sub-Saharan Africa It uses strong electric bass rhythms
      and prominent brass. In the 1980s makossa had a wave of mainstream success across Africa and
      to a lesser extent abroad. &lt;p&gt; Makossa, which means &quot; dance&quot; in the Duala
      language, originated from a Duala dance called the kossa. Emmanuel Nelle Eyoum started using
      the refrain kossa kossa in his songs with his group Los Calvinos. The style began to take
      shape in the 1950s though the first recordings were not seen until a decade later. Artists
      such as Eboa Lotin, Misse Ngoh and especially Manu Dibango, who popularised makossa throughout
      the world with his song &quot;Soul Makossa&quot; in the early 1970s. The chant from the song,
      mamako, mamasa, maka makossa, was later used by Michael Jackson in &quot;Wanna Be Startin'
      Somethin'&quot;. Many other performers followed suit. The 2010 World cup also brought makossa
      to the international stage as Shakira sampled the Golden Sounds popular song &quot;Zamina
      mina&quot;. &lt;p&gt; Makassi is a lighter style of makossa.</skos:definition>
    <skos:exactMatch xml:lang="en">http://dbpedia.org/resource/Makossa</skos:exactMatch>
    <skos:inScheme rdf:resource="http://data.europeana.eu/concept/music/genre/Music_Genre_Scheme"/>
    <skos:altLabel xml:lang="en">Makossa</skos:altLabel>
  </skos:Concept>

  <skos:Concept rdf:about="http://data.europeana.eu/concept/music/genre/Stoner_rock">
    <skos:prefLabel xml:lang="en">Stoner rock</skos:prefLabel>
    <skos:prefLabel xml:lang="cs">Stoner rock</skos:prefLabel>
    <skos:prefLabel xml:lang="da">Psykedelisk metal</skos:prefLabel>
    <skos:prefLabel xml:lang="nl">Stonerrock</skos:prefLabel>
    <skos:prefLabel xml:lang="fi">Stoner rock</skos:prefLabel>
    <skos:prefLabel xml:lang="fr">Stoner rock</skos:prefLabel>
    <skos:prefLabel xml:lang="de">Stoner Rock</skos:prefLabel>
    <skos:prefLabel xml:lang="hu">Stoner rock</skos:prefLabel>
    <skos:prefLabel xml:lang="it">Stoner rock</skos:prefLabel>
    <skos:prefLabel xml:lang="ja">ストーナーロック</skos:prefLabel>
    <skos:prefLabel xml:lang="ko">스토너 록</skos:prefLabel>
    <skos:prefLabel xml:lang="no">Stoner rock</skos:prefLabel>
    <skos:prefLabel xml:lang="pl">Stoner rock</skos:prefLabel>
    <skos:prefLabel xml:lang="pt">Stoner rock</skos:prefLabel>
    <skos:prefLabel xml:lang="ro">Stoner rock</skos:prefLabel>
    <skos:prefLabel xml:lang="ru">Стоунер-рок</skos:prefLabel>
    <skos:prefLabel xml:lang="sk">Stoner rock</skos:prefLabel>
    <skos:prefLabel xml:lang="es">Stoner rock</skos:prefLabel>
    <skos:prefLabel xml:lang="sv">Stonerrock</skos:prefLabel>
    <skos:prefLabel xml:lang="th">สโตเนอร์ร็อก</skos:prefLabel>
    <skos:prefLabel xml:lang="uk">Стоунер-рок</skos:prefLabel>
    <skos:closeMatch rdf:resource="http://rdf.freebase.com/ns/m.018lg0"/>
    <skos:broader
      rdf:resource="http://data.europeana.eu/concept/music/genre/Heavy_metal_music_fusions"/>
    <skos:definition xml:lang="en">Stoner rock or stoner metal is a musical subgenre which combines
      elements of traditional heavy metal, psychedelic rock, blues rock, acid rock, and doom metal.
      Stoner rock is typically slow-to-mid tempo and features a heavily distorted, groove laden
      bass-heavy sound, melodic vocals, and &quot;retro&quot; production. The genre emerged during
      the early 1990s and was pioneered foremost by the Californian bands Kyuss and
      Sleep.</skos:definition>
    <skos:exactMatch xml:lang="en">http://dbpedia.org/resource/Stoner_rock</skos:exactMatch>
    <skos:inScheme rdf:resource="http://data.europeana.eu/concept/music/genre/Music_Genre_Scheme"/>
    <skos:altLabel xml:lang="en">Stoner metal</skos:altLabel>
    <skos:altLabel xml:lang="en">Stoner rock</skos:altLabel>
  </skos:Concept>

  <skos:Concept rdf:about="http://data.europeana.eu/concept/music/genre/Cowpunk">
    <skos:prefLabel xml:lang="en">Cowpunk</skos:prefLabel>
    <skos:prefLabel xml:lang="nl">Cowpunk</skos:prefLabel>
    <skos:prefLabel xml:lang="fr">Cowpunk</skos:prefLabel>
    <skos:prefLabel xml:lang="it">Cowpunk</skos:prefLabel>
    <skos:prefLabel xml:lang="pl">Cowpunk</skos:prefLabel>
    <skos:prefLabel xml:lang="pt">Cowpunk</skos:prefLabel>
    <skos:prefLabel xml:lang="ru">Кантри-панк</skos:prefLabel>
    <skos:prefLabel xml:lang="es">Cowpunk</skos:prefLabel>
    <skos:closeMatch rdf:resource="http://rdf.freebase.com/ns/m.018yv3"/>
    <skos:broader rdf:resource="http://data.europeana.eu/concept/music/genre/Punk_rock_fusions"/>
    <skos:definition xml:lang="en">Cowpunk or Country punk is a subgenre of punk rock that began in
      the UK and California in the late 1970s and early 1980s. It combines punk rock or New Wave
      with country music, folk music, and blues in sound, subject matter, attitude, and style. Many
      of the musicians in this scene have now become associated with alternative country or roots
      rock.</skos:definition>
    <skos:exactMatch xml:lang="en">http://dbpedia.org/resource/Cowpunk</skos:exactMatch>
    <skos:inScheme rdf:resource="http://data.europeana.eu/concept/music/genre/Music_Genre_Scheme"/>
    <skos:altLabel xml:lang="en">Cowpunk</skos:altLabel>
  </skos:Concept>

  <skos:Concept rdf:about="http://data.europeana.eu/concept/music/genre/Space_rock">
    <skos:prefLabel xml:lang="en">Space rock</skos:prefLabel>
    <skos:prefLabel xml:lang="ca">Rock espacial</skos:prefLabel>
    <skos:prefLabel xml:lang="cs">Space rock</skos:prefLabel>
    <skos:prefLabel xml:lang="nl">Spacerock</skos:prefLabel>
    <skos:prefLabel xml:lang="fi">Space rock</skos:prefLabel>
    <skos:prefLabel xml:lang="fr">Space rock</skos:prefLabel>
    <skos:prefLabel xml:lang="de">Space Rock</skos:prefLabel>
    <skos:prefLabel xml:lang="it">Space rock</skos:prefLabel>
    <skos:prefLabel xml:lang="ko">스페이스록</skos:prefLabel>
    <skos:prefLabel xml:lang="no">Space rock</skos:prefLabel>
    <skos:prefLabel xml:lang="fa">اسپیس راک</skos:prefLabel>
    <skos:prefLabel xml:lang="pl">Space rock</skos:prefLabel>
    <skos:prefLabel xml:lang="pt">Space rock</skos:prefLabel>
    <skos:prefLabel xml:lang="ru">Спейс-рок</skos:prefLabel>
    <skos:prefLabel xml:lang="sk">Space rock</skos:prefLabel>
    <skos:prefLabel xml:lang="es">Rock espacial</skos:prefLabel>
    <skos:prefLabel xml:lang="sv">Space rock</skos:prefLabel>
    <skos:prefLabel xml:lang="tr">Space metal</skos:prefLabel>
    <skos:prefLabel xml:lang="uk">Спейс-рок</skos:prefLabel>
    <skos:closeMatch rdf:resource="http://rdf.freebase.com/ns/m.0190_q"/>
    <skos:broader rdf:resource="http://data.europeana.eu/concept/music/genre/Rock_music_fusions"/>
    <skos:definition xml:lang="en">Space rock is a subgenre of rock music, the term originally
      referred to a group of early, mostly British, 1970s progressive and psychedelic rock bands
      such as Hawkwind, Gong and Pink Floyd, characterised by slow, lengthy instrumental passages
      dominated by electronic organs, synthesizers, experimental guitar work and science fiction or
      outer space-related lyrical themes, though it was later repurposed to refer to a series of
      late 1980s British alternative rock bands that drew from earlier influences to create a more
      ambient but still melodic form of pop music. The term was revived in the 21st century to refer
      to a new crop of bands including The Flowers of Hell, Comets on Fire, and Flotation Toy
      Warning who diversely draw upon the ideas and sounds of both waves of the genre's
      founders.</skos:definition>
    <skos:exactMatch xml:lang="en">http://dbpedia.org/resource/Space_rock</skos:exactMatch>
    <skos:inScheme rdf:resource="http://data.europeana.eu/concept/music/genre/Music_Genre_Scheme"/>
    <skos:altLabel xml:lang="en">Space rock</skos:altLabel>
  </skos:Concept>

  <skos:Concept rdf:about="http://data.europeana.eu/concept/music/genre/Power_metal">
    <skos:prefLabel xml:lang="en">Power metal</skos:prefLabel>
    <skos:prefLabel xml:lang="ar">باور ميتال</skos:prefLabel>
    <skos:prefLabel xml:lang="bg">Пауър метъл</skos:prefLabel>
    <skos:prefLabel xml:lang="ca">Power metal</skos:prefLabel>
    <skos:prefLabel xml:lang="hr">Power metal</skos:prefLabel>
    <skos:prefLabel xml:lang="cs">Power metal</skos:prefLabel>
    <skos:prefLabel xml:lang="da">Power metal</skos:prefLabel>
    <skos:prefLabel xml:lang="nl">Powermetal</skos:prefLabel>
    <skos:prefLabel xml:lang="et">Power metal</skos:prefLabel>
    <skos:prefLabel xml:lang="fi">Power metal</skos:prefLabel>
    <skos:prefLabel xml:lang="fr">Power metal</skos:prefLabel>
    <skos:prefLabel xml:lang="de">Power Metal</skos:prefLabel>
    <skos:prefLabel xml:lang="el">Power Metal</skos:prefLabel>
    <skos:prefLabel xml:lang="hu">Power metal</skos:prefLabel>
    <skos:prefLabel xml:lang="id">Musik power metal</skos:prefLabel>
    <skos:prefLabel xml:lang="it">Power metal</skos:prefLabel>
    <skos:prefLabel xml:lang="ja">パワーメタル</skos:prefLabel>
    <skos:prefLabel xml:lang="ko">파워 메탈</skos:prefLabel>
    <skos:prefLabel xml:lang="lv">Power metal</skos:prefLabel>
    <skos:prefLabel xml:lang="lt">Power metal</skos:prefLabel>
    <skos:prefLabel xml:lang="ms">Power metal</skos:prefLabel>
    <skos:prefLabel xml:lang="no">Power metal</skos:prefLabel>
    <skos:prefLabel xml:lang="fa">پاور متال</skos:prefLabel>
    <skos:prefLabel xml:lang="pl">Power metal</skos:prefLabel>
    <skos:prefLabel xml:lang="pt">Power metal</skos:prefLabel>
    <skos:prefLabel xml:lang="ro">Power metal</skos:prefLabel>
    <skos:prefLabel xml:lang="ru">Пауэр-метал</skos:prefLabel>
    <skos:prefLabel xml:lang="sr">Пауер метал</skos:prefLabel>
    <skos:prefLabel xml:lang="sk">Power metal</skos:prefLabel>
    <skos:prefLabel xml:lang="sl">Power metal</skos:prefLabel>
    <skos:prefLabel xml:lang="es">Power metal</skos:prefLabel>
    <skos:prefLabel xml:lang="sv">Power metal</skos:prefLabel>
    <skos:prefLabel xml:lang="th">พาวเวอร์เมทัล</skos:prefLabel>
    <skos:prefLabel xml:lang="tr">Power metal</skos:prefLabel>
    <skos:prefLabel xml:lang="uk">Павер-метал</skos:prefLabel>
    <skos:closeMatch rdf:resource="http://rdf.freebase.com/ns/m.0190xp"/>
    <skos:broader
      rdf:resource="http://data.europeana.eu/concept/music/genre/Heavy_metal_music_fusions"/>
    <skos:definition xml:lang="en">Power metal is a subgenre of heavy metal combining
      characteristics of traditional metal with speed metal, often within symphonic context.
      Generally, power metal is characterized by a more uplifting sound, in contrast to the
      heaviness and dissonance prevalent in styles such as doom metal and death metal. Power metal
      bands usually have anthem-like songs with fantasy-based subject matter and strong choruses,
      thus creating a theatrical, dramatic and emotionally &quot;powerful&quot; sound. The term was
      first used in the middle of the '80s and refers to two different but related styles: the first
      pioneered and largely practiced in North America with a harder sound similar to speed metal,
      and a later more widespread and popular style based in Europe, Latin America and Japan, with a
      lighter, more melodic sound and frequent use of keyboards.</skos:definition>
    <skos:exactMatch xml:lang="en">http://dbpedia.org/resource/Power_metal</skos:exactMatch>
    <skos:inScheme rdf:resource="http://data.europeana.eu/concept/music/genre/Music_Genre_Scheme"/>
    <skos:altLabel xml:lang="en">Power metal</skos:altLabel>
  </skos:Concept>

  <skos:Concept rdf:about="http://data.europeana.eu/concept/music/genre/G-Funk">
    <skos:prefLabel xml:lang="en">G-funk</skos:prefLabel>
    <skos:prefLabel xml:lang="ca">G-Funk</skos:prefLabel>
    <skos:prefLabel xml:lang="hr">G-funk</skos:prefLabel>
    <skos:prefLabel xml:lang="cs">G-Funk</skos:prefLabel>
    <skos:prefLabel xml:lang="nl">G-funk</skos:prefLabel>
    <skos:prefLabel xml:lang="fi">G-funk</skos:prefLabel>
    <skos:prefLabel xml:lang="fr">Gangsta funk</skos:prefLabel>
    <skos:prefLabel xml:lang="de">G-Funk</skos:prefLabel>
    <skos:prefLabel xml:lang="it">G-funk</skos:prefLabel>
    <skos:prefLabel xml:lang="ja">Gファンク</skos:prefLabel>
    <skos:prefLabel xml:lang="ko">지펑크</skos:prefLabel>
    <skos:prefLabel xml:lang="no">G-Funk</skos:prefLabel>
    <skos:prefLabel xml:lang="pl">G-Funk</skos:prefLabel>
    <skos:prefLabel xml:lang="pt">G-funk</skos:prefLabel>
    <skos:prefLabel xml:lang="ru">Джи-фанк</skos:prefLabel>
    <skos:prefLabel xml:lang="sk">G-funk</skos:prefLabel>
    <skos:prefLabel xml:lang="es">G-funk</skos:prefLabel>
    <skos:prefLabel xml:lang="sv">G-funk</skos:prefLabel>
    <skos:prefLabel xml:lang="tr">G-funk</skos:prefLabel>
    <skos:closeMatch rdf:resource="http://rdf.freebase.com/ns/m.0190zg"/>
    <skos:broader rdf:resource="http://data.europeana.eu/concept/music/genre/Hip_hop_music_fusions"/>
    <skos:definition xml:lang="en">G-funk, or gangsta-funk, is a sub-genre of hip hop music that
      emerged from West Coast gangsta rap in the early 1990s.</skos:definition>
    <skos:exactMatch xml:lang="en">http://dbpedia.org/resource/G-Funk</skos:exactMatch>
    <skos:inScheme rdf:resource="http://data.europeana.eu/concept/music/genre/Music_Genre_Scheme"/>
    <skos:altLabel xml:lang="en">G-funk</skos:altLabel>
  </skos:Concept>

  <skos:Concept rdf:about="http://data.europeana.eu/concept/music/genre/Worldbeat">
    <skos:prefLabel xml:lang="en">Worldbeat</skos:prefLabel>
    <skos:prefLabel xml:lang="de">Worldbeat</skos:prefLabel>
    <skos:prefLabel xml:lang="it">Worldbeat</skos:prefLabel>
    <skos:prefLabel xml:lang="pl">Worldbeat</skos:prefLabel>
    <skos:prefLabel xml:lang="pt">Worldbeat</skos:prefLabel>
    <skos:prefLabel xml:lang="ro">Worldbeat</skos:prefLabel>
    <skos:prefLabel xml:lang="es">Worldbeat</skos:prefLabel>
    <skos:closeMatch rdf:resource="http://rdf.freebase.com/ns/m.0190zy"/>
    <skos:broader rdf:resource="http://data.europeana.eu/concept/music/genre/Jazz_fusions"/>
    <skos:definition xml:lang="en">Worldbeat is a music genre that blends Western pop music or rock
      music with traditional, folk or world music influences. Worldbeat is similar to other cross
      pollination labels of contemporary and roots genres, and which suggest a rhythmic, harmonic or
      textural contrast between its modern and ethnic elements.</skos:definition>
    <skos:exactMatch xml:lang="en">http://dbpedia.org/resource/Worldbeat</skos:exactMatch>
    <skos:inScheme rdf:resource="http://data.europeana.eu/concept/music/genre/Music_Genre_Scheme"/>
    <skos:altLabel xml:lang="en">Worldbeat</skos:altLabel>
  </skos:Concept>

  <skos:Concept rdf:about="http://data.europeana.eu/concept/music/genre/Pop_punk">
    <skos:prefLabel xml:lang="en">Pop punk</skos:prefLabel>
    <skos:prefLabel xml:lang="bg">Поп пънк</skos:prefLabel>
    <skos:prefLabel xml:lang="ca">Pop punk</skos:prefLabel>
    <skos:prefLabel xml:lang="hr">Pop punk</skos:prefLabel>
    <skos:prefLabel xml:lang="cs">Pop punk</skos:prefLabel>
    <skos:prefLabel xml:lang="da">Pop-punk</skos:prefLabel>
    <skos:prefLabel xml:lang="nl">Poppunk</skos:prefLabel>
    <skos:prefLabel xml:lang="fi">Pop punk</skos:prefLabel>
    <skos:prefLabel xml:lang="fr">Pop punk</skos:prefLabel>
    <skos:prefLabel xml:lang="de">Pop-Punk</skos:prefLabel>
    <skos:prefLabel xml:lang="hu">Pop-punk</skos:prefLabel>
    <skos:prefLabel xml:lang="it">Pop punk</skos:prefLabel>
    <skos:prefLabel xml:lang="ja">ポップ・パンク</skos:prefLabel>
    <skos:prefLabel xml:lang="ko">팝 펑크</skos:prefLabel>
    <skos:prefLabel xml:lang="lv">Poppanks</skos:prefLabel>
    <skos:prefLabel xml:lang="no">Pop-punk</skos:prefLabel>
    <skos:prefLabel xml:lang="pl">Pop punk</skos:prefLabel>
    <skos:prefLabel xml:lang="pt">Pop punk</skos:prefLabel>
    <skos:prefLabel xml:lang="ru">Поп-панк</skos:prefLabel>
    <skos:prefLabel xml:lang="sk">Pop punk</skos:prefLabel>
    <skos:prefLabel xml:lang="sl">Pop punk</skos:prefLabel>
    <skos:prefLabel xml:lang="es">Pop punk</skos:prefLabel>
    <skos:prefLabel xml:lang="sv">Poppunk</skos:prefLabel>
    <skos:prefLabel xml:lang="th">ป็อปพังก์</skos:prefLabel>
    <skos:prefLabel xml:lang="tr">Pop punk</skos:prefLabel>
    <skos:prefLabel xml:lang="uk">Поп-панк</skos:prefLabel>
    <skos:closeMatch rdf:resource="http://rdf.freebase.com/ns/m.01cbwl"/>
    <skos:broader rdf:resource="http://data.europeana.eu/concept/music/genre/Punk_rock_fusions"/>
    <skos:definition xml:lang="en">Pop punk is a fusion music genre that combines elements of punk
      rock with pop music to varying degrees. The music typically combines fast punk tempos, chord
      changes and loud guitars with pop-influenced melodies and lyrical themes. &lt;p&gt;
      Pop-influenced punk rock emerged in the mid 1970s in multiple countries, and was stylistically
      similar to power pop. By the early 1980s, several bands merged hardcore punk with pop music to
      create a new, faster pop punk sound. Pop punk particularly thrived in California, where
      independent record labels adopted a do it yourself approach to releasing music. In the mid
      1990s, a few pop punk bands sold millions of records and received extensive radio and
      television airplay. A second wave of pop punk in the late 1990s represented the genre's
      mainstream peak, although some pop punk bands scored successful album chartings in the 2000s.
      The genre generally waned in popularity by the late 2000s, although it still retains a smaller
      but dedicated following.</skos:definition>
    <skos:exactMatch xml:lang="en">http://dbpedia.org/resource/Pop_punk</skos:exactMatch>
    <skos:inScheme rdf:resource="http://data.europeana.eu/concept/music/genre/Music_Genre_Scheme"/>
    <skos:altLabel xml:lang="en">Pop punk</skos:altLabel>
  </skos:Concept>

  <skos:Concept rdf:about="http://data.europeana.eu/concept/music/genre/Hip_house">
    <skos:prefLabel xml:lang="en">Hip house</skos:prefLabel>
    <skos:prefLabel xml:lang="ca">Hip house</skos:prefLabel>
    <skos:prefLabel xml:lang="cs">Hip house</skos:prefLabel>
    <skos:prefLabel xml:lang="nl">Hiphouse</skos:prefLabel>
    <skos:prefLabel xml:lang="fi">Hip house</skos:prefLabel>
    <skos:prefLabel xml:lang="fr">Hip-house</skos:prefLabel>
    <skos:prefLabel xml:lang="de">Hip House</skos:prefLabel>
    <skos:prefLabel xml:lang="it">Hip house</skos:prefLabel>
    <skos:prefLabel xml:lang="pl">Hip house</skos:prefLabel>
    <skos:prefLabel xml:lang="pt">Hip house</skos:prefLabel>
    <skos:prefLabel xml:lang="ru">Хип-хаус</skos:prefLabel>
    <skos:prefLabel xml:lang="sk">Hip house</skos:prefLabel>
    <skos:prefLabel xml:lang="es">Hip house</skos:prefLabel>
    <skos:prefLabel xml:lang="sv">Hip house</skos:prefLabel>
    <skos:prefLabel xml:lang="th">ฮิปเฮ้าส์</skos:prefLabel>
    <skos:prefLabel xml:lang="uk">Хіп-хауз</skos:prefLabel>
    <skos:closeMatch rdf:resource="http://rdf.freebase.com/ns/m.01d_s5"/>
    <skos:broader rdf:resource="http://data.europeana.eu/concept/music/genre/Hip_hop_music_fusions"/>
    <skos:definition xml:lang="en">Hip house, also known as rap house or house rap, is a musical
      genre that mixes elements of house music and hip-hop. The style rose to prominence during the
      1980s in Chicago and New York. Hip house originated in Chicago and quickly became popular
      across the U.S. and in the UK, with tracks like &quot;Rok Da House&quot; by UK producers the
      Beatmasters featuring British female emcees the Cookie Crew. &lt;p&gt; Minor controversy
      ensued in 1989 when a U.S. record called &quot;Turn Up the Bass&quot; by Tyree Cooper
      featuring Kool Rock Steady claimed it was the &quot;first hip house record on vinyl&quot;. The
      Beatmasters disputed this, pointing out that &quot;Rok Da House&quot; had originally been
      written and pressed to vinyl in 1986. The outfit then released &quot;Who’s in the House?&quot;
      featuring British emcee Merlin, containing the lines &quot;Beatmasters stand to attention, hip
      house is your invention&quot; and &quot;Watch out Tyree, we come faster&quot;. More claims to
      the hip-house crown were subsequently laid down in tracks by Fast Eddie, Rob Base and DJ E-Z
      Rock, and Toni Scott.</skos:definition>
    <skos:exactMatch xml:lang="en">http://dbpedia.org/resource/Hip_house</skos:exactMatch>
    <skos:inScheme rdf:resource="http://data.europeana.eu/concept/music/genre/Music_Genre_Scheme"/>
    <skos:altLabel xml:lang="en">Hip house</skos:altLabel>
  </skos:Concept>

  <skos:Concept rdf:about="http://data.europeana.eu/concept/music/genre/Go-go">
    <skos:prefLabel xml:lang="en">Go-go</skos:prefLabel>
    <skos:prefLabel xml:lang="cs">Go-go</skos:prefLabel>
    <skos:prefLabel xml:lang="nl">Go-go</skos:prefLabel>
    <skos:prefLabel xml:lang="fr">Go-go</skos:prefLabel>
    <skos:prefLabel xml:lang="de">Gogo</skos:prefLabel>
    <skos:prefLabel xml:lang="ja">ゴーゴー</skos:prefLabel>
    <skos:prefLabel xml:lang="sv">Go-go</skos:prefLabel>
    <skos:closeMatch rdf:resource="http://rdf.freebase.com/ns/m.01dsw2"/>
    <skos:broader
      rdf:resource="http://data.europeana.eu/concept/music/genre/Electronic_music_fusions"/>
    <skos:definition xml:lang="en">Go-go is a subgenre associated with funk that originated in the
      Washington, D.C., area during the mid-1960s to late-'70s. It remains primarily popular in the
      area as a uniquely regional music style. A great number of bands contributed to the early
      evolution of the genre, but the Young Senators, Black Heat, and singer-guitarist Chuck Brown
      and the Soul Searchers are credited with having developed most of the hallmarks of the style.
      &lt;p&gt; Inspired by artists such as the groups formerly mentioned, Go-Go. is a blend of
      funk, rhythm and blues, and early hip-hop, with a focus on lo-fi percussion instruments and
      funk-style jamming in place of dance tracks, although some sampling is used. As such, it is
      primarily a dance hall music with an emphasis on live audience call and response. Go-go
      rhythms are also incorporated into street percussion. &lt;p&gt; In technical terms,
      &quot;Go-go's essential beat is characterized by a syncopated, dotted rhythm that consists of
      a series of quarter and eighth notes … which is underscored most dramatically by the bass drum
      and snare drum, and the hi-hat… [and] is ornamented by the other percussion instruments,
      especially by the conga drums, timbales, and hand-held cowbells.&quot;</skos:definition>
    <skos:exactMatch xml:lang="en">http://dbpedia.org/resource/Go-go</skos:exactMatch>
    <skos:inScheme rdf:resource="http://data.europeana.eu/concept/music/genre/Music_Genre_Scheme"/>
    <skos:altLabel xml:lang="en">Go-go</skos:altLabel>
  </skos:Concept>

  <skos:Concept rdf:about="http://data.europeana.eu/concept/music/genre/Oldschool_jungle">
    <skos:prefLabel xml:lang="en">Oldschool jungle</skos:prefLabel>
    <skos:closeMatch rdf:resource="http://rdf.freebase.com/ns/m.01f9gb"/>
    <skos:broader
      rdf:resource="http://data.europeana.eu/concept/music/genre/Electronic_music_fusions"/>
    <skos:definition xml:lang="en">Oldskool jungle, or simply jungle, is a genre of electronic music
      that incorporates influences from other genres, including breakbeat hardcore and
      reggae/dub/dancehall. It is one of several types of music often simply referred to as
      &quot;jungle music&quot;. The fast tempos, breakbeats and other heavily syncopated percussive
      loops, samples and synthesized effects make up the easily recognizable form of jungle. Long
      pitch-shifted snare rolls are common in oldskool jungle. &lt;p&gt; The terms
      &quot;jungle&quot; and &quot;drum and bass&quot; are often used interchangeably, although
      whether the two genres are actually distinct is an ongoing topic of debate. For those
      individuals who consider the two genres as separate entities, drum and bass is usually
      considered to have departed from jungle in the mid to late-1990s. &lt;p&gt; Producers create
      the drum patterns, which are sometimes completely off-beat, by cutting apart breakbeats.
      Jungle producers incorporated classic Jamaican/Caribbean sound-system culture
      production-methods. The slow, deep basslines and simple melodies accentuated the overall
      production, giving jungle its &quot;rolling&quot; quality.</skos:definition>
    <skos:exactMatch xml:lang="en">http://dbpedia.org/resource/Oldschool_jungle</skos:exactMatch>
    <skos:inScheme rdf:resource="http://data.europeana.eu/concept/music/genre/Music_Genre_Scheme"/>
  </skos:Concept>

  <skos:Concept rdf:about="http://data.europeana.eu/concept/music/genre/Jazz_rap">
    <skos:prefLabel xml:lang="en">Jazz rap</skos:prefLabel>
    <skos:prefLabel xml:lang="nl">Jazz rap</skos:prefLabel>
    <skos:prefLabel xml:lang="fr">Jazz rap</skos:prefLabel>
    <skos:prefLabel xml:lang="de">Jazz-Rap</skos:prefLabel>
    <skos:prefLabel xml:lang="it">Jazz rap</skos:prefLabel>
    <skos:prefLabel xml:lang="ja">ジャズ・ラップ</skos:prefLabel>
    <skos:prefLabel xml:lang="pl">Jazz-hop</skos:prefLabel>
    <skos:prefLabel xml:lang="pt">Jazz rap</skos:prefLabel>
    <skos:prefLabel xml:lang="ru">Джаз-рэп</skos:prefLabel>
    <skos:prefLabel xml:lang="es">Jazz rap</skos:prefLabel>
    <skos:prefLabel xml:lang="sv">Jazzrap</skos:prefLabel>
    <skos:closeMatch rdf:resource="http://rdf.freebase.com/ns/m.01f9y_"/>
    <skos:broader rdf:resource="http://data.europeana.eu/concept/music/genre/Hip_hop_music_fusions"/>
    <skos:definition xml:lang="en">Jazz rap is a sub-genre of hip hop music that incorporates jazz
      influences, developed in the late 1980s and early 1990s. The lyrics are often based on
      political consciousness, Afrocentrism, and general positivism. Allmusic writes that the genre
      &quot;was an attempt to fuse African-American music of the past with a newly dominant form of
      the present, paying tribute to and reinvigorating the former while expanding the horizons of
      the latter&quot;. Musically, the rhythms have been typically those of hip hop rather than
      jazz, over which are placed repetitive phrases of jazz instrumentation: trumpet, double bass,
      etc. The amount of improvisation varies between artists: some groups improvise lyrics and
      solos, while many of them do not. A Tribe Called Quest, De La Soul and Digable Planets are
      pioneers of the jazz rap genre.</skos:definition>
    <skos:exactMatch xml:lang="en">http://dbpedia.org/resource/Jazz_rap</skos:exactMatch>
    <skos:inScheme rdf:resource="http://data.europeana.eu/concept/music/genre/Music_Genre_Scheme"/>
    <skos:altLabel xml:lang="en">Jazz rap</skos:altLabel>
  </skos:Concept>

  <skos:Concept rdf:about="http://data.europeana.eu/concept/music/genre/Neo_soul">
    <skos:prefLabel xml:lang="en">Neo soul</skos:prefLabel>
    <skos:prefLabel xml:lang="hr">Neo soul</skos:prefLabel>
    <skos:prefLabel xml:lang="nl">Neo-soul</skos:prefLabel>
    <skos:prefLabel xml:lang="fi">Neo soul</skos:prefLabel>
    <skos:prefLabel xml:lang="fr">Neo soul</skos:prefLabel>
    <skos:prefLabel xml:lang="de">Neo-Soul</skos:prefLabel>
    <skos:prefLabel xml:lang="it">Neo soul</skos:prefLabel>
    <skos:prefLabel xml:lang="ja">ネオ・ソウル</skos:prefLabel>
    <skos:prefLabel xml:lang="ko">네오 솔</skos:prefLabel>
    <skos:prefLabel xml:lang="pl">Neo soul</skos:prefLabel>
    <skos:prefLabel xml:lang="pt">Neo soul</skos:prefLabel>
    <skos:prefLabel xml:lang="ru">Неосоул</skos:prefLabel>
    <skos:prefLabel xml:lang="es">Neo soul</skos:prefLabel>
    <skos:prefLabel xml:lang="sv">Neosoul</skos:prefLabel>
    <skos:prefLabel xml:lang="th">นีโอโซล</skos:prefLabel>
    <skos:closeMatch rdf:resource="http://rdf.freebase.com/ns/m.01fm07"/>
    <skos:broader rdf:resource="http://data.europeana.eu/concept/music/genre/Hip_hop_music_fusions"/>
    <skos:definition xml:lang="en">Neo soul is a term coined by music industry entrepreneur Kedar
      Massenburg during the late 1990s to market and describe a style of music that emerged from
      soul and contemporary R&amp;B. Heavily based in soul music, neo soul is distinguished by a
      less conventional sound than its contemporary R&amp;B counterpart, with incorporated elements
      ranging from jazz, funk, and hip hop to pop, fusion, and African music. It has been noted by
      music writers for its traditional R&amp;B influences, conscious-driven lyrics, and strong
      female presence. &lt;p&gt; Neo soul developed during the 1980s and early 1990s, in the United
      States and United Kingdom, as a soul &quot;revival&quot; movement. It earned mainstream
      success during the 1990s, with the commercial and critical breakthroughs of several neo soul
      artists that were marketed as an alternative to the producer-driven, digitally approached
      R&amp;B of the time. Since its initial mainstream popularity and impact on the sound of
      contemporary R&amp;B, it has been expanded and diversified musically through the works of both
      African-American and international artists.</skos:definition>
    <skos:exactMatch xml:lang="en">http://dbpedia.org/resource/Neo_soul</skos:exactMatch>
    <skos:inScheme rdf:resource="http://data.europeana.eu/concept/music/genre/Music_Genre_Scheme"/>
    <skos:altLabel xml:lang="en">Neo soul</skos:altLabel>
  </skos:Concept>

  <skos:Concept rdf:about="http://data.europeana.eu/concept/music/genre/Ska_punk">
    <skos:prefLabel xml:lang="en">Ska punk</skos:prefLabel>
    <skos:prefLabel xml:lang="ca">Ska punk</skos:prefLabel>
    <skos:prefLabel xml:lang="cs">Ska punk</skos:prefLabel>
    <skos:prefLabel xml:lang="da">Ska punk</skos:prefLabel>
    <skos:prefLabel xml:lang="nl">Ska-punk</skos:prefLabel>
    <skos:prefLabel xml:lang="et">Ska-punk</skos:prefLabel>
    <skos:prefLabel xml:lang="fi">Ska punk</skos:prefLabel>
    <skos:prefLabel xml:lang="fr">Ska punk</skos:prefLabel>
    <skos:prefLabel xml:lang="de">Ska-Punk</skos:prefLabel>
    <skos:prefLabel xml:lang="hu">Ska punk</skos:prefLabel>
    <skos:prefLabel xml:lang="id">Ska punk</skos:prefLabel>
    <skos:prefLabel xml:lang="it">Ska punk</skos:prefLabel>
    <skos:prefLabel xml:lang="ja">スカコア</skos:prefLabel>
    <skos:prefLabel xml:lang="ko">스카 펑크</skos:prefLabel>
    <skos:prefLabel xml:lang="no">Ska-punk</skos:prefLabel>
    <skos:prefLabel xml:lang="pl">Ska punk</skos:prefLabel>
    <skos:prefLabel xml:lang="pt">Ska punk</skos:prefLabel>
    <skos:prefLabel xml:lang="ro">Ska punk</skos:prefLabel>
    <skos:prefLabel xml:lang="ru">Ска-панк</skos:prefLabel>
    <skos:prefLabel xml:lang="sk">Ska punk</skos:prefLabel>
    <skos:prefLabel xml:lang="sl">Ska punk</skos:prefLabel>
    <skos:prefLabel xml:lang="es">Ska punk</skos:prefLabel>
    <skos:prefLabel xml:lang="sv">Ska-punk</skos:prefLabel>
    <skos:prefLabel xml:lang="th">สกาพังก์</skos:prefLabel>
    <skos:prefLabel xml:lang="tr">Ska punk</skos:prefLabel>
    <skos:prefLabel xml:lang="uk">Ска-панк</skos:prefLabel>
    <skos:closeMatch rdf:resource="http://rdf.freebase.com/ns/m.01g888"/>
    <skos:broader rdf:resource="http://data.europeana.eu/concept/music/genre/Punk_rock_fusions"/>
    <skos:definition xml:lang="en">Ska punk is a fusion music genre that combines ska and punk rock.
      It achieved its highest level of commercial success in the United States in the late 1990s.
      Ska-core is a subgenre of ska punk, blending ska with hardcore punk. &lt;p&gt; The more
      punk-influenced style of ska punk often features faster tempos, guitar distortion, onbeat punk
      rock-style interludes, and punk-style vocals. The more ska-influenced style features a more
      developed instrumentation and a cleaner vocal and musical sound. Common instruments include
      electric guitar, electric bass, drums, brass instruments, reed instruments and
      keyboards.</skos:definition>
    <skos:exactMatch xml:lang="en">http://dbpedia.org/resource/Ska_punk</skos:exactMatch>
    <skos:inScheme rdf:resource="http://data.europeana.eu/concept/music/genre/Music_Genre_Scheme"/>
    <skos:altLabel xml:lang="en">Ska punk</skos:altLabel>
  </skos:Concept>

  <skos:Concept rdf:about="http://data.europeana.eu/concept/music/genre/Madchester">
    <skos:prefLabel xml:lang="en">Madchester</skos:prefLabel>
    <skos:prefLabel xml:lang="fi">Madchester</skos:prefLabel>
    <skos:prefLabel xml:lang="fr">Madchester</skos:prefLabel>
    <skos:prefLabel xml:lang="de">Madchester</skos:prefLabel>
    <skos:prefLabel xml:lang="it">Madchester</skos:prefLabel>
    <skos:prefLabel xml:lang="ja">マッドチェスター</skos:prefLabel>
    <skos:prefLabel xml:lang="ko">매드체스터</skos:prefLabel>
    <skos:prefLabel xml:lang="no">Madchester</skos:prefLabel>
    <skos:prefLabel xml:lang="pl">Madchester</skos:prefLabel>
    <skos:prefLabel xml:lang="pt">Madchester</skos:prefLabel>
    <skos:prefLabel xml:lang="ru">Мэдчестер</skos:prefLabel>
    <skos:prefLabel xml:lang="es">Madchester</skos:prefLabel>
    <skos:prefLabel xml:lang="sv">Madchester</skos:prefLabel>
    <skos:prefLabel xml:lang="th">แมดเชสเตอร์</skos:prefLabel>
    <skos:closeMatch rdf:resource="http://rdf.freebase.com/ns/m.01h0kx"/>
    <skos:broader rdf:resource="http://data.europeana.eu/concept/music/genre/Rock_music_fusions"/>
    <skos:definition xml:lang="en">Madchester is a British music scene that developed in the
      Manchester area, England, towards the late 1980s and into the early 1990s. The music that
      emerged from the scene mixed alternative rock, psychedelic rock and electronic dance music.
      Artists associated with the scene included the Happy Mondays, the Stone Roses, the Inspiral
      Carpets, Northside, Paris Angels, 808 State, James, the Charlatans, and A Guy Called Gerald.
      At that time, the Haçienda nightclub was a major catalyst for the distinctive musical ethos in
      the city that was called the Second Summer of Love. Although the scene spawned several widely
      acclaimed acts, it has also been described by critic Penny Anderson of The Guardian as
      &quot;the breeding ground for aggressively marketed mediocrity&quot;.</skos:definition>
    <skos:exactMatch xml:lang="en">http://dbpedia.org/resource/Madchester</skos:exactMatch>
    <skos:inScheme rdf:resource="http://data.europeana.eu/concept/music/genre/Music_Genre_Scheme"/>
    <skos:altLabel xml:lang="en">Madchester</skos:altLabel>
  </skos:Concept>

  <skos:Concept rdf:about="http://data.europeana.eu/concept/music/genre/Tech_house">
    <skos:prefLabel xml:lang="en">Tech house</skos:prefLabel>
    <skos:prefLabel xml:lang="cs">Tech house</skos:prefLabel>
    <skos:prefLabel xml:lang="da">Techhouse</skos:prefLabel>
    <skos:prefLabel xml:lang="fr">Tech House</skos:prefLabel>
    <skos:prefLabel xml:lang="de">Tech House</skos:prefLabel>
    <skos:prefLabel xml:lang="it">Tech-house</skos:prefLabel>
    <skos:prefLabel xml:lang="ja">テックハウス</skos:prefLabel>
    <skos:prefLabel xml:lang="pl">Tech house</skos:prefLabel>
    <skos:prefLabel xml:lang="ru">Тек-хаус</skos:prefLabel>
    <skos:prefLabel xml:lang="sk">Tech house</skos:prefLabel>
    <skos:prefLabel xml:lang="es">Tech house</skos:prefLabel>
    <skos:prefLabel xml:lang="sv">Tech house</skos:prefLabel>
    <skos:closeMatch rdf:resource="http://rdf.freebase.com/ns/m.01hyfj"/>
    <skos:broader rdf:resource="http://data.europeana.eu/concept/music/genre/House_music_fusions"/>
    <skos:definition xml:lang="en">Tech house is a subgenre of house music that mixes elements of
      techno with house. The term tech house developed as a shorthand record store name for a
      category of electronic dance music that combined musical aspects of techno, such as
      &quot;rugged basslines&quot; and &quot;steely beats,&quot; with the harmonies and grooves of
      progressive house. The music originally had a clean and minimal production style that was
      associated with techno from Detroit and the UK. In the mid to late 1990s a scene developed in
      England around club nights such as The Drop run by Mr.C &amp; Plink Plonk, Heart &amp; Soul,
      and Wiggle run by Terry Francis and Nathan Coles. Other DJs and artists associated with the
      sound at that time included Charles Webster, Bushwacka!, Dave Angel, Herbert, Funk D'Void, Ian
      O'Brien, Derrick Carter, and Stacey Pullen. By the late 90's London nightclub The End, owned
      by the former Shamen rapper Richard West and Layo Paskin, was considered the home of tech
      house in the UK.</skos:definition>
    <skos:exactMatch xml:lang="en">http://dbpedia.org/resource/Tech_house</skos:exactMatch>
    <skos:inScheme rdf:resource="http://data.europeana.eu/concept/music/genre/Music_Genre_Scheme"/>
    <skos:altLabel xml:lang="en">Tech house</skos:altLabel>
  </skos:Concept>

  <skos:Concept rdf:about="http://data.europeana.eu/concept/music/genre/Ghettotech">
    <skos:prefLabel xml:lang="en">Ghettotech</skos:prefLabel>
    <skos:prefLabel xml:lang="ca">Ghettotech</skos:prefLabel>
    <skos:prefLabel xml:lang="cs">Ghetto-Tech</skos:prefLabel>
    <skos:prefLabel xml:lang="nl">Ghettotech</skos:prefLabel>
    <skos:prefLabel xml:lang="fr">Ghettotech</skos:prefLabel>
    <skos:prefLabel xml:lang="de">Ghetto Tech</skos:prefLabel>
    <skos:prefLabel xml:lang="it">Ghettotech</skos:prefLabel>
    <skos:prefLabel xml:lang="pl">Ghettotech</skos:prefLabel>
    <skos:prefLabel xml:lang="sk">Ghettotech</skos:prefLabel>
    <skos:prefLabel xml:lang="es">Ghettotech</skos:prefLabel>
    <skos:closeMatch rdf:resource="http://rdf.freebase.com/ns/m.01n428"/>
    <skos:broader rdf:resource="http://data.europeana.eu/concept/music/genre/Techno_fusions"/>
    <skos:definition xml:lang="en">Ghettotech is a form of electronic music originating from Detroit
      and Chicago. It combines elements of Chicago's ghetto house with electro, techno and UK
      garage. It features four-on-the-floor rhythms and is usually faster than most other dance
      music genres, at roughly 145 to 170 bpm, and sometimes features pornographic lyrics. As DJ
      Godfather puts it, &quot;the beats are really gritty, really raw, nothing polished.&quot;
      &lt;p&gt; Ghettotech was born as a DJing style, inspired by the eclecticism of The
      Electrifying Mojo and the fast-paced mixing and turntablism of The Wizard, with DJs mixing
      genres including jungle, ghetto house, hip hop, R&amp;B, electro and Detroit techno. The
      general BPM of the music's mixing style increases over time. &lt;p&gt; Ghettotech is an
      integral part of the Detroit Electronic Music Festival, an annual event. A Detroit ghettotech
      style of dancing is called the jit. It is an improvisational dance that mainly centers around
      the fast movement of the feet. Chicago's equivalent dance style is Juke, where the focus is on
      the footwork dating back to the late 1980s.</skos:definition>
    <skos:exactMatch xml:lang="en">http://dbpedia.org/resource/Ghettotech</skos:exactMatch>
    <skos:inScheme rdf:resource="http://data.europeana.eu/concept/music/genre/Music_Genre_Scheme"/>
    <skos:altLabel xml:lang="en">Ghettotech</skos:altLabel>
  </skos:Concept>

  <skos:Concept rdf:about="http://data.europeana.eu/concept/music/genre/Ghetto_house">
    <skos:prefLabel xml:lang="en">Ghetto house</skos:prefLabel>
    <skos:prefLabel xml:lang="cs">Booty House</skos:prefLabel>
    <skos:prefLabel xml:lang="fr">Ghetto house</skos:prefLabel>
    <skos:prefLabel xml:lang="es">Ghetto house</skos:prefLabel>
    <skos:closeMatch rdf:resource="http://rdf.freebase.com/ns/m.01n4lj"/>
    <skos:broader rdf:resource="http://data.europeana.eu/concept/music/genre/Hip_hop_music_fusions"/>
    <skos:definition xml:lang="en">Ghetto house, or booty house, is a type of Chicago house which
      started being recognized as a distinct style from around 1992 onwards. It features minimal 808
      and 909 drum machine-driven tracks and sometimes sexually explicit lyrics. &lt;p&gt; The
      template of classic Chicago house music was used with the addition of sexual lyrics. It has
      usually been made on minimal equipment with little or no effects. It usually features a
      &quot;4-to-the-floor&quot; kick drum along with Roland 808 and 909 synthesized tom-tom sounds,
      minimal use of analogue synths, and short, slightly dirty sounding vocals samples, often
      repeated in various ways. Also common are 808 and 909 clap sounds, and full &quot;rapped&quot;
      verses and choruses.</skos:definition>
    <skos:exactMatch xml:lang="en">http://dbpedia.org/resource/Ghetto_house</skos:exactMatch>
    <skos:inScheme rdf:resource="http://data.europeana.eu/concept/music/genre/Music_Genre_Scheme"/>
    <skos:altLabel xml:lang="en">Booty House</skos:altLabel>
    <skos:altLabel xml:lang="en">Ghetto house</skos:altLabel>
  </skos:Concept>

  <skos:Concept rdf:about="http://data.europeana.eu/concept/music/genre/Soul_jazz">
    <skos:prefLabel xml:lang="en">Soul jazz</skos:prefLabel>
    <skos:prefLabel xml:lang="cs">Soul-jazz</skos:prefLabel>
    <skos:prefLabel xml:lang="fi">Soul jazz</skos:prefLabel>
    <skos:prefLabel xml:lang="fr">Soul jazz</skos:prefLabel>
    <skos:prefLabel xml:lang="de">Soul-Jazz</skos:prefLabel>
    <skos:prefLabel xml:lang="it">Soul jazz</skos:prefLabel>
    <skos:prefLabel xml:lang="ja">ファンキー・ジャズ</skos:prefLabel>
    <skos:prefLabel xml:lang="ko">솔 재즈</skos:prefLabel>
    <skos:prefLabel xml:lang="pt">Soul jazz</skos:prefLabel>
    <skos:prefLabel xml:lang="sv">Soul jazz</skos:prefLabel>
    <skos:closeMatch rdf:resource="http://rdf.freebase.com/ns/m.01n5sn"/>
    <skos:broader rdf:resource="http://data.europeana.eu/concept/music/genre/Jazz_fusions"/>
    <skos:definition xml:lang="en">Soul jazz is a development of jazz incorporating strong
      influences from blues, soul, gospel and rhythm and blues in music for small groups, often an
      organ trio featuring a Hammond organ.</skos:definition>
    <skos:exactMatch xml:lang="en">http://dbpedia.org/resource/Soul_jazz</skos:exactMatch>
    <skos:inScheme rdf:resource="http://data.europeana.eu/concept/music/genre/Music_Genre_Scheme"/>
    <skos:altLabel xml:lang="en">Soul jazz</skos:altLabel>
  </skos:Concept>

  <skos:Concept rdf:about="http://data.europeana.eu/concept/music/genre/Riot_grrrl">
    <skos:prefLabel xml:lang="en">Riot grrrl</skos:prefLabel>
    <skos:prefLabel xml:lang="bg">Riot grrrl</skos:prefLabel>
    <skos:prefLabel xml:lang="cs">Riot Grrrl</skos:prefLabel>
    <skos:prefLabel xml:lang="nl">Riot Grrrl</skos:prefLabel>
    <skos:prefLabel xml:lang="fi">Riot grrrl</skos:prefLabel>
    <skos:prefLabel xml:lang="fr">Riot grrrl</skos:prefLabel>
    <skos:prefLabel xml:lang="de">Riot Grrrl</skos:prefLabel>
    <skos:prefLabel xml:lang="it">Riot grrrl</skos:prefLabel>
    <skos:prefLabel xml:lang="ko">라이엇 걸</skos:prefLabel>
    <skos:prefLabel xml:lang="lt">Riot grrrl</skos:prefLabel>
    <skos:prefLabel xml:lang="fa">رایت گرررل</skos:prefLabel>
    <skos:prefLabel xml:lang="pl">Riot Grrrl</skos:prefLabel>
    <skos:prefLabel xml:lang="pt">Riot Grrrl</skos:prefLabel>
    <skos:prefLabel xml:lang="ru">Riot Grrrl</skos:prefLabel>
    <skos:prefLabel xml:lang="es">Riot grrrl</skos:prefLabel>
    <skos:prefLabel xml:lang="sv">Riot grrrl</skos:prefLabel>
    <skos:prefLabel xml:lang="tr">Riot Grrrl</skos:prefLabel>
    <skos:closeMatch rdf:resource="http://rdf.freebase.com/ns/m.01nd9f"/>
    <skos:broader rdf:resource="http://data.europeana.eu/concept/music/genre/Punk_rock_fusions"/>
    <skos:definition xml:lang="en">Riot grrrl is an underground feminist punk rock movement that
      originally started in the early 1990s, in Washington, D.C., and the greater Pacific Northwest,
      especially Olympia, Washington and Portland, Oregon. It is often associated with third-wave
      feminism, which is sometimes seen as its starting point. It has also been described as musical
      genre that came out of indie rock, with the punk scene serving as an inspiration for a musical
      movement in which women could express themselves in the same way men had been doing for the
      past several years. &lt;p&gt; Riot grrrl bands often address issues such as rape, domestic
      abuse, sexuality, racism, patriarchy, and female empowerment. Bands associated with the
      movement include Bikini Kill, Huggy Bear, Bratmobile, Heavens to Betsy, Excuse 17, Skinned
      Teen, Calamity Jane, Emily's Sassy Lime, Sleater-Kinney, and also queercore like Team Dresch
      and The Butchies. In addition to a music scene and genre, riot grrrl is a subculture involving
      a DIY ethic, zines, art, political action, and activism. Riot grrrls are known to hold
      meetings, start chapters, and support and organize women in music.</skos:definition>
    <skos:exactMatch xml:lang="en">http://dbpedia.org/resource/Riot_grrrl</skos:exactMatch>
    <skos:inScheme rdf:resource="http://data.europeana.eu/concept/music/genre/Music_Genre_Scheme"/>
    <skos:altLabel xml:lang="en">Riot grrrl</skos:altLabel>
  </skos:Concept>

  <skos:Concept rdf:about="http://data.europeana.eu/concept/music/genre/Digital_Hardcore">
    <skos:prefLabel xml:lang="en">Digital hardcore</skos:prefLabel>
    <skos:prefLabel xml:lang="cs">Digital Hardcore</skos:prefLabel>
    <skos:prefLabel xml:lang="nl">Digital hardcore</skos:prefLabel>
    <skos:prefLabel xml:lang="fi">Digital hardcore</skos:prefLabel>
    <skos:prefLabel xml:lang="fr">Digital hardcore</skos:prefLabel>
    <skos:prefLabel xml:lang="de">Digital Hardcore</skos:prefLabel>
    <skos:prefLabel xml:lang="hu">Digital hardcore</skos:prefLabel>
    <skos:prefLabel xml:lang="it">Digital hardcore</skos:prefLabel>
    <skos:prefLabel xml:lang="pl">Digital hardcore</skos:prefLabel>
    <skos:prefLabel xml:lang="pt">Hardcore digital</skos:prefLabel>
    <skos:prefLabel xml:lang="sk">Digital hardcore</skos:prefLabel>
    <skos:prefLabel xml:lang="es">Digital hardcore</skos:prefLabel>
    <skos:closeMatch rdf:resource="http://rdf.freebase.com/ns/m.01nv0_"/>
    <skos:broader rdf:resource="http://data.europeana.eu/concept/music/genre/Techno_fusions"/>
    <skos:definition xml:lang="en">Digital hardcore is a music genre that melds hardcore punk with
      electronic music such as hardcore techno, industrial and drum and bass. The style developed in
      Germany during the early 1990s, and often has sociological or left-extremist lyrical
      themes.</skos:definition>
    <skos:exactMatch xml:lang="en">http://dbpedia.org/resource/Digital_Hardcore</skos:exactMatch>
    <skos:inScheme rdf:resource="http://data.europeana.eu/concept/music/genre/Music_Genre_Scheme"/>
    <skos:altLabel xml:lang="en">Digital hardcore</skos:altLabel>
  </skos:Concept>

  <skos:Concept rdf:about="http://data.europeana.eu/concept/music/genre/Latin_jazz">
    <skos:prefLabel xml:lang="en">Latin jazz</skos:prefLabel>
    <skos:prefLabel xml:lang="ca">Jazz llatí</skos:prefLabel>
    <skos:prefLabel xml:lang="cs">Latin jazz</skos:prefLabel>
    <skos:prefLabel xml:lang="da">Latin jazz</skos:prefLabel>
    <skos:prefLabel xml:lang="nl">Latin jazz</skos:prefLabel>
    <skos:prefLabel xml:lang="fr">Latin jazz</skos:prefLabel>
    <skos:prefLabel xml:lang="de">Latin Jazz</skos:prefLabel>
    <skos:prefLabel xml:lang="hu">Latin jazz</skos:prefLabel>
    <skos:prefLabel xml:lang="id">Jazz latin</skos:prefLabel>
    <skos:prefLabel xml:lang="it">Latin jazz</skos:prefLabel>
    <skos:prefLabel xml:lang="ja">ラテンジャズ</skos:prefLabel>
    <skos:prefLabel xml:lang="ko">라틴 재즈</skos:prefLabel>
    <skos:prefLabel xml:lang="pl">Latin jazz</skos:prefLabel>
    <skos:prefLabel xml:lang="pt">Latin jazz</skos:prefLabel>
    <skos:prefLabel xml:lang="ru">Латиноамериканский джаз</skos:prefLabel>
    <skos:prefLabel xml:lang="es">Jazz latino</skos:prefLabel>
    <skos:prefLabel xml:lang="sv">Latin jazz</skos:prefLabel>
    <skos:closeMatch rdf:resource="http://rdf.freebase.com/ns/m.01p_2p"/>
    <skos:broader rdf:resource="http://data.europeana.eu/concept/music/genre/Jazz_fusions"/>
    <skos:definition xml:lang="en">Latin jazz is jazz with Latin American rhythms. Although
      musicians continually expand its parameters, the term Latin jazz is generally understood to
      have a more specific meaning than simply jazz from Latin America. Some Latin Jazz typically
      employs rhythms that either have a direct analog in Africa, or exhibit an African influence.
      The two main categories of Latin jazz are: &lt;p&gt; Afro-Cuban jazz—jazz rhythmically based
      on clave, often with a rhythm section employing ostinato patterns from Cuban popular dance
      music. &lt;p&gt; Afro-Brazilian jazz—includes bossa nova and jazz samba.</skos:definition>
    <skos:exactMatch xml:lang="en">http://dbpedia.org/resource/Latin_jazz</skos:exactMatch>
    <skos:inScheme rdf:resource="http://data.europeana.eu/concept/music/genre/Music_Genre_Scheme"/>
    <skos:altLabel xml:lang="en">Latin jazz</skos:altLabel>
  </skos:Concept>

  <skos:Concept rdf:about="http://data.europeana.eu/concept/music/genre/Happy_hardcore">
    <skos:prefLabel xml:lang="en">Happy hardcore</skos:prefLabel>
    <skos:prefLabel xml:lang="ca">Happy hardcore</skos:prefLabel>
    <skos:prefLabel xml:lang="hr">Happy hardcore</skos:prefLabel>
    <skos:prefLabel xml:lang="cs">Happy Hardcore</skos:prefLabel>
    <skos:prefLabel xml:lang="da">Happy hardcore</skos:prefLabel>
    <skos:prefLabel xml:lang="nl">Happy hardcore</skos:prefLabel>
    <skos:prefLabel xml:lang="fi">Happy hardcore</skos:prefLabel>
    <skos:prefLabel xml:lang="fr">Happy hardcore</skos:prefLabel>
    <skos:prefLabel xml:lang="de">Happy Hardcore</skos:prefLabel>
    <skos:prefLabel xml:lang="hu">Happy Hardcore</skos:prefLabel>
    <skos:prefLabel xml:lang="it">Happy hardcore</skos:prefLabel>
    <skos:prefLabel xml:lang="ja">ハッピーハードコア</skos:prefLabel>
    <skos:prefLabel xml:lang="no">Happy hardcore</skos:prefLabel>
    <skos:prefLabel xml:lang="pl">Happy hardcore</skos:prefLabel>
    <skos:prefLabel xml:lang="pt">Happy hardcore</skos:prefLabel>
    <skos:prefLabel xml:lang="ru">Happy hardcore</skos:prefLabel>
    <skos:prefLabel xml:lang="sk">Happy hardcore</skos:prefLabel>
    <skos:prefLabel xml:lang="es">Happy hardcore</skos:prefLabel>
    <skos:prefLabel xml:lang="sv">Happy hardcore</skos:prefLabel>
    <skos:prefLabel xml:lang="th">แฮปปี้ฮาร์ดคอร์</skos:prefLabel>
    <skos:prefLabel xml:lang="tr">Happy hardcore</skos:prefLabel>
    <skos:closeMatch rdf:resource="http://rdf.freebase.com/ns/m.01p4dg"/>
    <skos:broader rdf:resource="http://data.europeana.eu/concept/music/genre/Techno_fusions"/>
    <skos:definition xml:lang="en">Happy hardcore, also known as happycore, is a genre of music
      typified by a very fast tempo, often coupled with solo vocals and sentimental lyrics. Its
      characteristically 4/4 beat &quot;happy&quot; sound distinguishes it from most other forms of
      hardcore techno, which tend to be &quot;darker&quot;. It is typically in a mode with a major
      third, like Ionian or Lydian. In its original incarnation, it was often characterized by piano
      riffs, synthetic stabs and spacey effects. This genre of music is closely related to the
      typically Dutch genre of gabber. Happy hardcore evolved from breakbeat hardcore around
      1991–1993, as the original house music-based rave became faster and began to include
      breakbeats, evolving into oldschool jungle which evolved into drum and bass. Some of the most
      famous artists of this genre include DJ Brisk, Scott Brown, Darren Styles, Hixxy, DJ Paul
      Elstak, Dune, Scooter, Stu Allan, Dougal, and DJ Gammer.</skos:definition>
    <skos:exactMatch xml:lang="en">http://dbpedia.org/resource/Happy_hardcore</skos:exactMatch>
    <skos:inScheme rdf:resource="http://data.europeana.eu/concept/music/genre/Music_Genre_Scheme"/>
    <skos:altLabel xml:lang="en">Happy hardcore</skos:altLabel>
  </skos:Concept>

  <skos:Concept rdf:about="http://data.europeana.eu/concept/music/genre/Jangle_pop">
    <skos:prefLabel xml:lang="en">Jangle pop</skos:prefLabel>
    <skos:prefLabel xml:lang="ca">Jangle pop</skos:prefLabel>
    <skos:prefLabel xml:lang="cs">Jangle pop</skos:prefLabel>
    <skos:prefLabel xml:lang="fr">Jangle pop</skos:prefLabel>
    <skos:prefLabel xml:lang="it">Jangle pop</skos:prefLabel>
    <skos:prefLabel xml:lang="ko">쟁글 팝</skos:prefLabel>
    <skos:prefLabel xml:lang="pl">Jangle pop</skos:prefLabel>
    <skos:prefLabel xml:lang="pt">Jangle pop</skos:prefLabel>
    <skos:prefLabel xml:lang="ru">Джэнгл-поп</skos:prefLabel>
    <skos:prefLabel xml:lang="sk">Jangle pop</skos:prefLabel>
    <skos:prefLabel xml:lang="es">Jangle pop</skos:prefLabel>
    <skos:prefLabel xml:lang="sv">Jangle pop</skos:prefLabel>
    <skos:prefLabel xml:lang="th">แจงเกิลป็อป</skos:prefLabel>
    <skos:prefLabel xml:lang="uk">Дженгл-поп</skos:prefLabel>
    <skos:closeMatch rdf:resource="http://rdf.freebase.com/ns/m.01skxk"/>
    <skos:broader rdf:resource="http://data.europeana.eu/concept/music/genre/Pop_music_fusions"/>
    <skos:definition xml:lang="en">Jangle pop is a genre of alternative rock from the mid-1980s that
      &quot;marked a return to the chiming or jangly guitars and pop melodies of the '60s&quot;, as
      exemplified by The Byrds, with electric twelve-string guitars and power pop song structures.
      Mid-1980s jangle pop was a non-mainstream &quot;pop-based format&quot; with &quot;some
      folk-rock overtones&quot;. Between 1983 and 1987, the description &quot;jangle pop&quot; was,
      in the US, used to describe bands like R.E.M., Let's Active and Tom Petty, and a subgenre
      called &quot;Paisley Underground&quot;, which incorporated psychedelic influences. In the UK
      the term was applied to the new wave of raw and immediate sounding melodic guitar-bands
      collected on the NME's C86 compilations.</skos:definition>
    <skos:exactMatch xml:lang="en">http://dbpedia.org/resource/Jangle_pop</skos:exactMatch>
    <skos:inScheme rdf:resource="http://data.europeana.eu/concept/music/genre/Music_Genre_Scheme"/>
    <skos:altLabel xml:lang="en">Jangle pop</skos:altLabel>
  </skos:Concept>

  <skos:Concept rdf:about="http://data.europeana.eu/concept/music/genre/Nu_jazz">
    <skos:prefLabel xml:lang="en">Nu jazz</skos:prefLabel>
    <skos:prefLabel xml:lang="ca">Nu Jazz</skos:prefLabel>
    <skos:prefLabel xml:lang="nl">Nu jazz</skos:prefLabel>
    <skos:prefLabel xml:lang="fi">Nu-jazz</skos:prefLabel>
    <skos:prefLabel xml:lang="fr">Nu jazz</skos:prefLabel>
    <skos:prefLabel xml:lang="de">Nu-Jazz</skos:prefLabel>
    <skos:prefLabel xml:lang="it">Nu jazz</skos:prefLabel>
    <skos:prefLabel xml:lang="ja">ニュージャズ</skos:prefLabel>
    <skos:prefLabel xml:lang="no">Nu jazz</skos:prefLabel>
    <skos:prefLabel xml:lang="fa">نیو جاز</skos:prefLabel>
    <skos:prefLabel xml:lang="pl">Nu jazz</skos:prefLabel>
    <skos:prefLabel xml:lang="pt">Nu jazz</skos:prefLabel>
    <skos:prefLabel xml:lang="ru">Ню-джаз</skos:prefLabel>
    <skos:prefLabel xml:lang="sk">Nu jazz</skos:prefLabel>
    <skos:prefLabel xml:lang="es">Nu jazz</skos:prefLabel>
    <skos:prefLabel xml:lang="th">นูแจ๊ส</skos:prefLabel>
    <skos:prefLabel xml:lang="uk">Ню джаз</skos:prefLabel>
    <skos:closeMatch rdf:resource="http://rdf.freebase.com/ns/m.01vw77"/>
    <skos:broader rdf:resource="http://data.europeana.eu/concept/music/genre/Jazz_fusions"/>
    <skos:definition xml:lang="en">Nu jazz is an umbrella term coined in the late 1990s to refer to
      music that blends jazz elements with other musical styles, such as funk, soul, electronic
      dance music, and free improvisation. Also written nü-jazz or NuJazz, it is sometimes called
      electronic jazz, electro-jazz, electric jazz, e-jazz, jazztronica, jazz house, phusion,
      neo-jazz, future jazz or Jazz-hop and electro-lounge. &lt;p&gt; According to critic Tony
      Brewer, &lt;p&gt; “Nu Jazz is to Jazz what punk or grunge was to Rock, of course. [...] The
      songs are the focus, not the individual prowess of the musicians. Nu Jazz instrumentation
      ranges from the traditional to the experimental, the melodies are fresh, and the rhythms new
      and alive. It makes Jazz fun again.”</skos:definition>
    <skos:exactMatch xml:lang="en">http://dbpedia.org/resource/Nu_jazz</skos:exactMatch>
    <skos:inScheme rdf:resource="http://data.europeana.eu/concept/music/genre/Music_Genre_Scheme"/>
    <skos:altLabel xml:lang="en">Electrojazz</skos:altLabel>
    <skos:altLabel xml:lang="en">Nu jazz</skos:altLabel>
  </skos:Concept>

  <skos:Concept rdf:about="http://data.europeana.eu/concept/music/genre/Breakcore">
    <skos:prefLabel xml:lang="en">Breakcore</skos:prefLabel>
    <skos:prefLabel xml:lang="hr">Breakcore</skos:prefLabel>
    <skos:prefLabel xml:lang="cs">Breakcore</skos:prefLabel>
    <skos:prefLabel xml:lang="nl">Breakcore</skos:prefLabel>
    <skos:prefLabel xml:lang="fi">Breakcore</skos:prefLabel>
    <skos:prefLabel xml:lang="fr">Breakcore</skos:prefLabel>
    <skos:prefLabel xml:lang="de">Breakcore</skos:prefLabel>
    <skos:prefLabel xml:lang="it">Breakcore</skos:prefLabel>
    <skos:prefLabel xml:lang="ja">ブレイクコア</skos:prefLabel>
    <skos:prefLabel xml:lang="no">Breakcore</skos:prefLabel>
    <skos:prefLabel xml:lang="pl">Breakcore</skos:prefLabel>
    <skos:prefLabel xml:lang="ru">Брейккор</skos:prefLabel>
    <skos:prefLabel xml:lang="sk">Breakcore</skos:prefLabel>
    <skos:prefLabel xml:lang="es">Breakcore</skos:prefLabel>
    <skos:prefLabel xml:lang="sv">Breakcore</skos:prefLabel>
    <skos:prefLabel xml:lang="th">เบรกคอร์</skos:prefLabel>
    <skos:prefLabel xml:lang="uk">Брейккор</skos:prefLabel>
    <skos:closeMatch rdf:resource="http://rdf.freebase.com/ns/m.01y3_q"/>
    <skos:broader rdf:resource="http://data.europeana.eu/concept/music/genre/Techno_fusions"/>
    <skos:definition xml:lang="en">Breakcore or noisecore is a style of electronic dance music
      largely influenced by hardcore, jungle, digital hardcore and industrial music that is
      characterized by its use of heavy kick drums, breaks and a wide palette of sampling sources,
      played at high tempos.</skos:definition>
    <skos:exactMatch xml:lang="en">http://dbpedia.org/resource/Breakcore</skos:exactMatch>
    <skos:inScheme rdf:resource="http://data.europeana.eu/concept/music/genre/Music_Genre_Scheme"/>
    <skos:altLabel xml:lang="en">Breakcore</skos:altLabel>
  </skos:Concept>

  <skos:Concept rdf:about="http://data.europeana.eu/concept/music/genre/Downtempo">
    <skos:prefLabel xml:lang="en">Downtempo</skos:prefLabel>
    <skos:prefLabel xml:lang="bg">Даунтемпо</skos:prefLabel>
    <skos:prefLabel xml:lang="ca">Downtempo</skos:prefLabel>
    <skos:prefLabel xml:lang="hr">Downbeat</skos:prefLabel>
    <skos:prefLabel xml:lang="cs">Downtempo</skos:prefLabel>
    <skos:prefLabel xml:lang="fi">Downtempo</skos:prefLabel>
    <skos:prefLabel xml:lang="fr">Downtempo</skos:prefLabel>
    <skos:prefLabel xml:lang="de">Downbeat</skos:prefLabel>
    <skos:prefLabel xml:lang="hu">Downtempo</skos:prefLabel>
    <skos:prefLabel xml:lang="it">Downtempo</skos:prefLabel>
    <skos:prefLabel xml:lang="no">Downtempo</skos:prefLabel>
    <skos:prefLabel xml:lang="fa">تمپو پایین</skos:prefLabel>
    <skos:prefLabel xml:lang="pl">Downtempo</skos:prefLabel>
    <skos:prefLabel xml:lang="pt">Downtempo</skos:prefLabel>
    <skos:prefLabel xml:lang="ru">Даунтемпо</skos:prefLabel>
    <skos:prefLabel xml:lang="sr">Даунтемпо</skos:prefLabel>
    <skos:prefLabel xml:lang="sk">Downtempo</skos:prefLabel>
    <skos:prefLabel xml:lang="es">Downtempo</skos:prefLabel>
    <skos:prefLabel xml:lang="th">ดาวน์เทมโป</skos:prefLabel>
    <skos:prefLabel xml:lang="tr">Downtempo</skos:prefLabel>
    <skos:prefLabel xml:lang="uk">Downtempo</skos:prefLabel>
    <skos:closeMatch rdf:resource="http://rdf.freebase.com/ns/m.01ym9b"/>
    <skos:broader
      rdf:resource="http://data.europeana.eu/concept/music/genre/Electronic_music_fusions"/>
    <skos:definition xml:lang="en">Downtempo is a type of electronic music style similar to ambient
      music, but usually with a beat or groove. The tempo, as well as the drum patterns of each
      track can vary. Sometimes the beat can be restrained and/or simple. Sometimes the beats are
      more complicated and more featured instead of being in the background, but even then they are
      usually less intense than other kinds of electronic music like trance and house. The tempo is
      often slower than that of traditional electronic dance music. Often the name chill-out music
      is used to refer to songs demonstrative of the genre, but those names also refer to other
      styles of music, and downtempo encompasses a wider variety of styles than those terms alone
      would indicate. Due to the relaxing and often sensual or romantic feel of most downtempo
      music, it is a popular form of background music in 'chill out rooms' of dance parties, and
      many alternative cafes.</skos:definition>
    <skos:exactMatch xml:lang="en">http://dbpedia.org/resource/Downtempo</skos:exactMatch>
    <skos:inScheme rdf:resource="http://data.europeana.eu/concept/music/genre/Music_Genre_Scheme"/>
    <skos:altLabel xml:lang="en">Lounge</skos:altLabel>
    <skos:altLabel xml:lang="en">Chill</skos:altLabel>
    <skos:altLabel xml:lang="en">Downtempo</skos:altLabel>
  </skos:Concept>

  <skos:Concept rdf:about="http://data.europeana.eu/concept/music/genre/Video_game_music">
    <skos:prefLabel xml:lang="en">Video game music</skos:prefLabel>
    <skos:prefLabel xml:lang="ar">موسيقى لعبة فيديو</skos:prefLabel>
    <skos:prefLabel xml:lang="ca">Música de videojocs</skos:prefLabel>
    <skos:prefLabel xml:lang="cs">Herní hudba</skos:prefLabel>
    <skos:prefLabel xml:lang="fi">Videopelimusiikki</skos:prefLabel>
    <skos:prefLabel xml:lang="fr">Musique de jeu vidéo</skos:prefLabel>
    <skos:prefLabel xml:lang="de">Videospielmusik</skos:prefLabel>
    <skos:prefLabel xml:lang="it">Musica per videogiochi</skos:prefLabel>
    <skos:prefLabel xml:lang="ja">ゲームミュージック</skos:prefLabel>
    <skos:prefLabel xml:lang="ko">게임 음악</skos:prefLabel>
    <skos:prefLabel xml:lang="ms">Muzik permainan video</skos:prefLabel>
    <skos:prefLabel xml:lang="fa">موسیقی بازی ویدئویی</skos:prefLabel>
    <skos:prefLabel xml:lang="pt">Música de jogos eletrônicos</skos:prefLabel>
    <skos:prefLabel xml:lang="ru">Музыка в компьютерных играх</skos:prefLabel>
    <skos:prefLabel xml:lang="es">Música de videojuegos</skos:prefLabel>
    <skos:prefLabel xml:lang="sv">Datorspelsmusik</skos:prefLabel>
    <skos:closeMatch rdf:resource="http://rdf.freebase.com/ns/m.01z7dr"/>
    <skos:broader
      rdf:resource="http://data.europeana.eu/concept/music/genre/Electronic_music_fusions"/>
    <skos:definition xml:lang="en">Video game music refers to the soundtrack or background music
      accompanying video games. Originally limited to simple melodies by early sound synthesizer
      technology, video game music has grown to include the same breadth and complexity associated
      with television and movie soundtracks. While simple synthesizer pieces are still common, game
      music now can include full orchestral pieces and licensed popular music. Video games can now
      also generate or alter their soundtrack based on the player's current actions or situation,
      such as indicating missed actions in rhythm games. With the expansion of the video game
      market, artists going between popular music, classical music, the film industry and video
      games has become more common. Composers and artists famous for other music—such as film
      composers Harry Gregson-Williams, Trent Reznor and Hans Zimmer—have worked on soundtracks for
      recent games, while Michael Giacchino, now normally known for his film scores, began with
      Mickey Mania and continued with the Medal of Honor series.</skos:definition>
    <skos:exactMatch xml:lang="en">http://dbpedia.org/resource/Video_game_music</skos:exactMatch>
    <skos:inScheme rdf:resource="http://data.europeana.eu/concept/music/genre/Music_Genre_Scheme"/>
    <skos:altLabel xml:lang="en">Video game music</skos:altLabel>
  </skos:Concept>

  <skos:Concept rdf:about="http://data.europeana.eu/concept/music/genre/Hardcore_techno">
    <skos:prefLabel xml:lang="en">Hardcore techno</skos:prefLabel>
    <skos:prefLabel xml:lang="en">Hardcore</skos:prefLabel>
    <skos:prefLabel xml:lang="ca">Techno hardcore</skos:prefLabel>
    <skos:prefLabel xml:lang="hr">Hardcore techno</skos:prefLabel>
    <skos:prefLabel xml:lang="cs">Hardcore techno</skos:prefLabel>
    <skos:prefLabel xml:lang="fi">Hardcore</skos:prefLabel>
    <skos:prefLabel xml:lang="fr">Techno hardcore</skos:prefLabel>
    <skos:prefLabel xml:lang="de">Hardcore Techno</skos:prefLabel>
    <skos:prefLabel xml:lang="hu">Hardcore techno</skos:prefLabel>
    <skos:prefLabel xml:lang="it">Techno hardcore</skos:prefLabel>
    <skos:prefLabel xml:lang="ja">ハードコアテクノ</skos:prefLabel>
    <skos:prefLabel xml:lang="ko">하드코어 테크노</skos:prefLabel>
    <skos:prefLabel xml:lang="no">Hardcore techno</skos:prefLabel>
    <skos:prefLabel xml:lang="pl">Hardcore</skos:prefLabel>
    <skos:prefLabel xml:lang="pt">Hardcore techno</skos:prefLabel>
    <skos:prefLabel xml:lang="ro">Hardcore techno</skos:prefLabel>
    <skos:prefLabel xml:lang="ru">Хардкор-техно</skos:prefLabel>
    <skos:prefLabel xml:lang="sr">Хардкор техно</skos:prefLabel>
    <skos:prefLabel xml:lang="sk">Hardcore techno</skos:prefLabel>
    <skos:prefLabel xml:lang="es">Techno hardcore</skos:prefLabel>
    <skos:prefLabel xml:lang="sv">Hardcore techno</skos:prefLabel>
    <skos:prefLabel xml:lang="th">ฮาร์ดคอร์</skos:prefLabel>
    <skos:prefLabel xml:lang="uk">Хардкор-техно</skos:prefLabel>
    <skos:closeMatch rdf:resource="http://rdf.freebase.com/ns/m.01z9l_"/>
    <skos:broader
      rdf:resource="http://data.europeana.eu/concept/music/genre/Electronic_music_fusions"/>
    <skos:definition xml:lang="en">Hardcore is a sub-genre of electronic dance music originally
      European from the emergent raves in the 1990s initially designed at Rotterdam in Netherlands
      derived from techno. Its sub-genres are usually distinct from the other electronic dance
      musics by a higher rapidity, the intensity of the kicks and the basses, the rhythm and the
      atmosphere of their theme, the usage of saturation and experimentation close to the industrial
      music.</skos:definition>
    <skos:exactMatch xml:lang="en">http://dbpedia.org/resource/Hardcore_techno</skos:exactMatch>
    <skos:inScheme rdf:resource="http://data.europeana.eu/concept/music/genre/Music_Genre_Scheme"/>
    <skos:altLabel xml:lang="en">Hardcore</skos:altLabel>
  </skos:Concept>

  <skos:Concept rdf:about="http://data.europeana.eu/concept/music/genre/Deep_house">
    <skos:prefLabel xml:lang="en">Deep house</skos:prefLabel>
    <skos:prefLabel xml:lang="cs">Deep house</skos:prefLabel>
    <skos:prefLabel xml:lang="nl">Deephouse</skos:prefLabel>
    <skos:prefLabel xml:lang="fi">Deep house</skos:prefLabel>
    <skos:prefLabel xml:lang="fr">Deep house</skos:prefLabel>
    <skos:prefLabel xml:lang="de">Deep House</skos:prefLabel>
    <skos:prefLabel xml:lang="hu">Deep house</skos:prefLabel>
    <skos:prefLabel xml:lang="it">Deep house</skos:prefLabel>
    <skos:prefLabel xml:lang="ja">ディープ・ハウス</skos:prefLabel>
    <skos:prefLabel xml:lang="ko">딥 하우스</skos:prefLabel>
    <skos:prefLabel xml:lang="lt">Deep house</skos:prefLabel>
    <skos:prefLabel xml:lang="pl">Deep house</skos:prefLabel>
    <skos:prefLabel xml:lang="pt">Deep house</skos:prefLabel>
    <skos:prefLabel xml:lang="ro">Deep house</skos:prefLabel>
    <skos:prefLabel xml:lang="ru">Дип-хаус</skos:prefLabel>
    <skos:prefLabel xml:lang="sk">Deep house</skos:prefLabel>
    <skos:prefLabel xml:lang="es">Deep house</skos:prefLabel>
    <skos:prefLabel xml:lang="sv">Deep house</skos:prefLabel>
    <skos:prefLabel xml:lang="th">ดีปเฮาส์</skos:prefLabel>
    <skos:prefLabel xml:lang="tr">Deep house</skos:prefLabel>
    <skos:prefLabel xml:lang="uk">Діп-хауз</skos:prefLabel>
    <skos:closeMatch rdf:resource="http://rdf.freebase.com/ns/m.01zh00"/>
    <skos:broader rdf:resource="http://data.europeana.eu/concept/music/genre/House_music_fusions"/>
    <skos:definition xml:lang="en">Deep house is a subgenre of house music that originated in the
      1980s, initially fusing elements of Chicago house with 1980s jazz-funk and touches of soul
      music. The lengths of the tracks are usually around 7 and 10 minutes, with tempos usually in
      the range of 120 to 130 BPM. This style of house music can often have an acoustic
      feeling.</skos:definition>
    <skos:exactMatch xml:lang="en">http://dbpedia.org/resource/Deep_house</skos:exactMatch>
    <skos:inScheme rdf:resource="http://data.europeana.eu/concept/music/genre/Music_Genre_Scheme"/>
    <skos:altLabel xml:lang="en">Deep house</skos:altLabel>
  </skos:Concept>

  <skos:Concept rdf:about="http://data.europeana.eu/concept/music/genre/Horror_punk">
    <skos:prefLabel xml:lang="en">Horror punk</skos:prefLabel>
    <skos:prefLabel xml:lang="cs">Horror punk</skos:prefLabel>
    <skos:prefLabel xml:lang="da">Horror punk</skos:prefLabel>
    <skos:prefLabel xml:lang="nl">Horrorpunk</skos:prefLabel>
    <skos:prefLabel xml:lang="fi">Horror punk</skos:prefLabel>
    <skos:prefLabel xml:lang="fr">Horror punk</skos:prefLabel>
    <skos:prefLabel xml:lang="de">Horrorpunk</skos:prefLabel>
    <skos:prefLabel xml:lang="hu">Horror punk</skos:prefLabel>
    <skos:prefLabel xml:lang="it">Horror punk</skos:prefLabel>
    <skos:prefLabel xml:lang="ja">ホラー・パンク</skos:prefLabel>
    <skos:prefLabel xml:lang="ko">호러 펑크</skos:prefLabel>
    <skos:prefLabel xml:lang="no">Horror-punk</skos:prefLabel>
    <skos:prefLabel xml:lang="pl">Horror punk</skos:prefLabel>
    <skos:prefLabel xml:lang="pt">Horror punk</skos:prefLabel>
    <skos:prefLabel xml:lang="ro">Horror punk</skos:prefLabel>
    <skos:prefLabel xml:lang="ru">Хоррор-панк</skos:prefLabel>
    <skos:prefLabel xml:lang="sk">Horror punk</skos:prefLabel>
    <skos:prefLabel xml:lang="es">Horror punk</skos:prefLabel>
    <skos:prefLabel xml:lang="sv">Horrorpunk</skos:prefLabel>
    <skos:prefLabel xml:lang="tr">Horror punk</skos:prefLabel>
    <skos:closeMatch rdf:resource="http://rdf.freebase.com/ns/m.020ngt"/>
    <skos:broader rdf:resource="http://data.europeana.eu/concept/music/genre/Punk_rock_fusions"/>
    <skos:definition xml:lang="en">Horror punk is a music genre that mixes Gothic and punk rock
      sounds with morbid or violent imagery and lyrics, which are often influenced by horror films
      or science fiction B-movies. The genre is similar to and sometimes overlaps with deathrock,
      although deathrock leans more towards an atmospheric Gothic rock sound while horror punk leans
      towards a 1950s-influenced doo-wop and rockabilly sound. Horrorpunk music is typically more
      aggressive and melodic than deathrock. &lt;p&gt; The Misfits are recognized as the progenitors
      of horror punk, releasing a series of singles and EPs beginning in 1977 before releasing their
      first full-length album Walk Among Us in 1982. &lt;p&gt; Horror punk is generally apolitical
      in comparison to other punk rock subgenres, although some songs do refer to political events,
      and some artists like Jack Grisham and Michale Graves have espoused their own political views.
      &lt;p&gt; Horror hardcore, refers to a hybrid of horror punk and hardcore punk. The Misfits'
      1983 album Earth A.D. inaugurated this style and the bands Septic Death, The Banner, and
      Integrity have also been categorized into this subgenre.</skos:definition>
    <skos:exactMatch xml:lang="en">http://dbpedia.org/resource/Horror_punk</skos:exactMatch>
    <skos:inScheme rdf:resource="http://data.europeana.eu/concept/music/genre/Music_Genre_Scheme"/>
    <skos:altLabel xml:lang="en">Horror punk</skos:altLabel>
  </skos:Concept>

  <skos:Concept rdf:about="http://data.europeana.eu/concept/music/genre/New_jack_swing">
    <skos:prefLabel xml:lang="en">New jack swing</skos:prefLabel>
    <skos:prefLabel xml:lang="cs">New jack swing</skos:prefLabel>
    <skos:prefLabel xml:lang="nl">Swingbeat</skos:prefLabel>
    <skos:prefLabel xml:lang="fi">New jack swing</skos:prefLabel>
    <skos:prefLabel xml:lang="fr">New jack swing</skos:prefLabel>
    <skos:prefLabel xml:lang="de">New Jack Swing</skos:prefLabel>
    <skos:prefLabel xml:lang="hu">New jack swing</skos:prefLabel>
    <skos:prefLabel xml:lang="it">New jack swing</skos:prefLabel>
    <skos:prefLabel xml:lang="ja">ニュージャックスウィング</skos:prefLabel>
    <skos:prefLabel xml:lang="ko">뉴 잭 스윙</skos:prefLabel>
    <skos:prefLabel xml:lang="pt">New jack swing</skos:prefLabel>
    <skos:prefLabel xml:lang="ru">Нью-джек-свинг</skos:prefLabel>
    <skos:prefLabel xml:lang="sr">Њу џек свинг</skos:prefLabel>
    <skos:prefLabel xml:lang="sk">New jack swing</skos:prefLabel>
    <skos:prefLabel xml:lang="es">New jack swing</skos:prefLabel>
    <skos:prefLabel xml:lang="sv">New jack swing</skos:prefLabel>
    <skos:prefLabel xml:lang="th">นิวแจ็กสวิง</skos:prefLabel>
    <skos:prefLabel xml:lang="tr">New jack swing</skos:prefLabel>
    <skos:closeMatch rdf:resource="http://rdf.freebase.com/ns/m.021_z5"/>
    <skos:broader rdf:resource="http://data.europeana.eu/concept/music/genre/Hip_hop_music_fusions"/>
    <skos:definition xml:lang="en">New jack swing or swingbeat is a fusion genre spearheaded by
      Teddy Riley and Bernard Belle that became popular from the late-1980s into the early 1990s.
      Its influence, along with hip-hop, seeped into pop culture and was the definitive sound of the
      inventive black New York club scene. It fuses the rhythms, samples, and production techniques
      of hip-hop and dance-pop with the urban contemporary sound of R&amp;B. The new jack swing
      style developed as many previous music styles did, by combining elements of older styles with
      newer sensibilities. It used R&amp;B style vocals sung over hip hop and dance-pop style
      influenced instrumentation. The sound of new jack swing comes from the hip hop
      &quot;swing&quot; beats created by drum machine, and hardware samplers, which was popular
      during the golden age of hip hop, with contemporary R&amp;B style singing. &lt;p&gt;
      Merriam-Webster's online dictionary defines new jack swing as &quot;pop music usually
      performed by black musicians that combines elements of traditional jazz, electronica, smooth
      jazz, funk, rap, and rhythm and blues.&quot;</skos:definition>
    <skos:exactMatch xml:lang="en">http://dbpedia.org/resource/New_jack_swing</skos:exactMatch>
    <skos:inScheme rdf:resource="http://data.europeana.eu/concept/music/genre/Music_Genre_Scheme"/>
    <skos:altLabel xml:lang="en">New jack swing</skos:altLabel>
  </skos:Concept>

  <skos:Concept rdf:about="http://data.europeana.eu/concept/music/genre/Goregrind">
    <skos:prefLabel xml:lang="en">Goregrind</skos:prefLabel>
    <skos:prefLabel xml:lang="bg">Гор</skos:prefLabel>
    <skos:prefLabel xml:lang="cs">Goregrind</skos:prefLabel>
    <skos:prefLabel xml:lang="da">Goregrind</skos:prefLabel>
    <skos:prefLabel xml:lang="fi">Goregrind</skos:prefLabel>
    <skos:prefLabel xml:lang="fr">Goregrind</skos:prefLabel>
    <skos:prefLabel xml:lang="de">Goregrind</skos:prefLabel>
    <skos:prefLabel xml:lang="id">Goregrind</skos:prefLabel>
    <skos:prefLabel xml:lang="it">Goregrind</skos:prefLabel>
    <skos:prefLabel xml:lang="ja">ゴアグラインド</skos:prefLabel>
    <skos:prefLabel xml:lang="ko">고어그라인드</skos:prefLabel>
    <skos:prefLabel xml:lang="pl">Goregrind</skos:prefLabel>
    <skos:prefLabel xml:lang="pt">Goregrind</skos:prefLabel>
    <skos:prefLabel xml:lang="ro">Goregrind</skos:prefLabel>
    <skos:prefLabel xml:lang="ru">Гор-грайнд</skos:prefLabel>
    <skos:prefLabel xml:lang="es">Goregrind</skos:prefLabel>
    <skos:prefLabel xml:lang="sv">Goregrind</skos:prefLabel>
    <skos:prefLabel xml:lang="vi">Goregrind</skos:prefLabel>
    <skos:closeMatch rdf:resource="http://rdf.freebase.com/ns/m.021vlg"/>
    <skos:broader
      rdf:resource="http://data.europeana.eu/concept/music/genre/Heavy_metal_music_fusions"/>
    <skos:definition xml:lang="en">Goregrind is a musical sub-genre of grindcore and death
      metal.</skos:definition>
    <skos:exactMatch xml:lang="en">http://dbpedia.org/resource/Goregrind</skos:exactMatch>
    <skos:inScheme rdf:resource="http://data.europeana.eu/concept/music/genre/Music_Genre_Scheme"/>
    <skos:altLabel xml:lang="en">Goregrind</skos:altLabel>
  </skos:Concept>

  <skos:Concept rdf:about="http://data.europeana.eu/concept/music/genre/Anti-folk">
    <skos:prefLabel xml:lang="en">Anti-folk</skos:prefLabel>
    <skos:prefLabel xml:lang="da">Anti-folk</skos:prefLabel>
    <skos:prefLabel xml:lang="nl">Anti-folk</skos:prefLabel>
    <skos:prefLabel xml:lang="fi">Anti-folk</skos:prefLabel>
    <skos:prefLabel xml:lang="fr">Anti-folk</skos:prefLabel>
    <skos:prefLabel xml:lang="de">Anti-Folk</skos:prefLabel>
    <skos:prefLabel xml:lang="it">Anti-folk</skos:prefLabel>
    <skos:prefLabel xml:lang="ru">Список исполнителей анти-фолка</skos:prefLabel>
    <skos:prefLabel xml:lang="es">Anti-folk</skos:prefLabel>
    <skos:prefLabel xml:lang="sv">Anti-folk</skos:prefLabel>
    <skos:closeMatch rdf:resource="http://rdf.freebase.com/ns/m.02278y"/>
    <skos:broader rdf:resource="http://data.europeana.eu/concept/music/genre/Folk_music_fusions"/>
    <skos:definition xml:lang="en">Anti-folk is a music genre that takes the earnestness of
      politically charged 1960s folk music and subverts it. The defining characteristics of this
      anti-folk are difficult to identify, as they vary from one artist to the next. Nonetheless,
      the music tends to sound raw or experimental, it also generally mocks seriousness and
      pretension in the established mainstream music scene.</skos:definition>
    <skos:exactMatch xml:lang="en">http://dbpedia.org/resource/Anti-folk</skos:exactMatch>
    <skos:inScheme rdf:resource="http://data.europeana.eu/concept/music/genre/Music_Genre_Scheme"/>
    <skos:altLabel xml:lang="en">Anti-folk</skos:altLabel>
  </skos:Concept>

  <skos:Concept rdf:about="http://data.europeana.eu/concept/music/genre/Bitpop">
    <skos:prefLabel xml:lang="en">Bitpop</skos:prefLabel>
    <skos:prefLabel xml:lang="nl">Bitpop</skos:prefLabel>
    <skos:prefLabel xml:lang="fi">Bitpop</skos:prefLabel>
    <skos:prefLabel xml:lang="fr">Bitpop</skos:prefLabel>
    <skos:prefLabel xml:lang="de">Bitpop</skos:prefLabel>
    <skos:prefLabel xml:lang="it">Bitpop</skos:prefLabel>
    <skos:prefLabel xml:lang="fa">بیت پاپ</skos:prefLabel>
    <skos:prefLabel xml:lang="pl">Bitpop</skos:prefLabel>
    <skos:prefLabel xml:lang="ru">Битпоп</skos:prefLabel>
    <skos:prefLabel xml:lang="sv">Bitpop</skos:prefLabel>
    <skos:prefLabel xml:lang="uk">Бітпоп</skos:prefLabel>
    <skos:closeMatch rdf:resource="http://rdf.freebase.com/ns/m.0233jl"/>
    <skos:broader
      rdf:resource="http://data.europeana.eu/concept/music/genre/Electronic_music_fusions"/>
    <skos:definition xml:lang="en">Bitpop is a type of electronic music and subgenre of chiptune
      music, where at least part of the music is made using the sound chips of old 8-bit computers,
      video game consoles and arcade machines.</skos:definition>
    <skos:exactMatch xml:lang="en">http://dbpedia.org/resource/Bitpop</skos:exactMatch>
    <skos:inScheme rdf:resource="http://data.europeana.eu/concept/music/genre/Music_Genre_Scheme"/>
    <skos:altLabel xml:lang="en">Bitpop</skos:altLabel>
  </skos:Concept>

  <skos:Concept rdf:about="http://data.europeana.eu/concept/music/genre/Techstep">
    <skos:prefLabel xml:lang="en">Techstep</skos:prefLabel>
    <skos:prefLabel xml:lang="cs">Techstep</skos:prefLabel>
    <skos:prefLabel xml:lang="nl">Techstep</skos:prefLabel>
    <skos:prefLabel xml:lang="fr">Techstep</skos:prefLabel>
    <skos:prefLabel xml:lang="de">Techstep</skos:prefLabel>
    <skos:prefLabel xml:lang="it">Techstep</skos:prefLabel>
    <skos:prefLabel xml:lang="fa">تک استپ</skos:prefLabel>
    <skos:prefLabel xml:lang="pl">Techstep</skos:prefLabel>
    <skos:prefLabel xml:lang="pt">Techstep</skos:prefLabel>
    <skos:prefLabel xml:lang="ru">Текстеп</skos:prefLabel>
    <skos:prefLabel xml:lang="sk">Techstep</skos:prefLabel>
    <skos:prefLabel xml:lang="es">Techstep</skos:prefLabel>
    <skos:prefLabel xml:lang="sv">Techstep</skos:prefLabel>
    <skos:prefLabel xml:lang="uk">Текстеп</skos:prefLabel>
    <skos:closeMatch rdf:resource="http://rdf.freebase.com/ns/m.024cyw"/>
    <skos:broader
      rdf:resource="http://data.europeana.eu/concept/music/genre/Electronic_music_fusions"/>
    <skos:definition xml:lang="en">Techstep is a subgenre of drum and bass that was popular in the
      late 1990s.</skos:definition>
    <skos:exactMatch xml:lang="en">http://dbpedia.org/resource/Techstep</skos:exactMatch>
    <skos:inScheme rdf:resource="http://data.europeana.eu/concept/music/genre/Music_Genre_Scheme"/>
    <skos:altLabel xml:lang="en">Techstep</skos:altLabel>
  </skos:Concept>

  <skos:Concept rdf:about="http://data.europeana.eu/concept/music/genre/Rock_in_Opposition">
    <skos:prefLabel xml:lang="en">Rock in Opposition</skos:prefLabel>
    <skos:prefLabel xml:lang="cs">Rock in Opposition</skos:prefLabel>
    <skos:prefLabel xml:lang="nl">Rock In Opposition</skos:prefLabel>
    <skos:prefLabel xml:lang="fr">Rock in Opposition</skos:prefLabel>
    <skos:prefLabel xml:lang="de">Rock in Opposition</skos:prefLabel>
    <skos:prefLabel xml:lang="it">Rock In Opposition</skos:prefLabel>
    <skos:prefLabel xml:lang="no">Rock In Opposition</skos:prefLabel>
    <skos:prefLabel xml:lang="fa">راک در اپوزیسیون</skos:prefLabel>
    <skos:prefLabel xml:lang="pl">Rock in Opposition</skos:prefLabel>
    <skos:prefLabel xml:lang="pt">Rock in Opposition</skos:prefLabel>
    <skos:prefLabel xml:lang="ru">Rock in Opposition</skos:prefLabel>
    <skos:prefLabel xml:lang="es">Rock in Opposition</skos:prefLabel>
    <skos:prefLabel xml:lang="sv">Rock in Opposition</skos:prefLabel>
    <skos:closeMatch rdf:resource="http://rdf.freebase.com/ns/m.024xq2"/>
    <skos:broader rdf:resource="http://data.europeana.eu/concept/music/genre/Rock_music_fusions"/>
    <skos:definition xml:lang="en">Rock in Opposition or RIO was a movement representing a
      collective of progressive bands in the late 1970s united in their opposition to the music
      industry that refused to recognise their music. It was initiated by English avant-rock group
      Henry Cow in March 1978 when they invited four mainland European groups to come to London and
      perform in a festival called &quot;Rock in Opposition&quot;.</skos:definition>
    <skos:exactMatch xml:lang="en">http://dbpedia.org/resource/Rock_in_Opposition</skos:exactMatch>
    <skos:inScheme rdf:resource="http://data.europeana.eu/concept/music/genre/Music_Genre_Scheme"/>
    <skos:altLabel xml:lang="en">Rock in Opposition</skos:altLabel>
  </skos:Concept>

  <skos:Concept rdf:about="http://data.europeana.eu/concept/music/genre/Neo-bop_jazz">
    <skos:prefLabel xml:lang="en">Neo-bop jazz</skos:prefLabel>
    <skos:prefLabel xml:lang="nl">Neo-bop</skos:prefLabel>
    <skos:prefLabel xml:lang="fr">Néo-bop</skos:prefLabel>
    <skos:prefLabel xml:lang="de">Neobop</skos:prefLabel>
    <skos:closeMatch rdf:resource="http://rdf.freebase.com/ns/m.0268p62"/>
    <skos:broader rdf:resource="http://data.europeana.eu/concept/music/genre/Jazz_fusions"/>
    <skos:definition xml:lang="en">Neo-bop is a style of jazz that emerged in the 1980s as a
      reaction against free jazz and jazz fusion. In the United States it is associated with Wynton
      Marsalis and &quot;The Young Lions.&quot; The effort earned praise and also criticism. Miles
      Davis called it &quot;warmed over turkey&quot; and others deemed it to be too dependent on the
      past. The movement, however, received praise from Time magazine and others who welcomed the
      return of more accessible forms of jazz. There were also those who deemed it a valid evolution
      from hard bop.</skos:definition>
    <skos:exactMatch xml:lang="en">http://dbpedia.org/resource/Neo-bop_jazz</skos:exactMatch>
    <skos:inScheme rdf:resource="http://data.europeana.eu/concept/music/genre/Music_Genre_Scheme"/>
    <skos:altLabel xml:lang="en">Neo-bop jazz</skos:altLabel>
  </skos:Concept>

  <skos:Concept rdf:about="http://data.europeana.eu/concept/music/genre/Progressive_folk_music">
    <skos:prefLabel xml:lang="en">Progressive folk</skos:prefLabel>
    <skos:prefLabel xml:lang="it">Progressive folk</skos:prefLabel>
    <skos:prefLabel xml:lang="ru">Прогрессив-фолк</skos:prefLabel>
    <skos:closeMatch rdf:resource="http://rdf.freebase.com/ns/m.0269v4c"/>
    <skos:broader rdf:resource="http://data.europeana.eu/concept/music/genre/Folk_music_fusions"/>
    <skos:definition xml:lang="en">Progressive folk or prog folk was originally a type of American
      folk music that pursued a progressive political agenda, but in the United Kingdom the term
      became attached to a sub-genre that rejects or de-emphasizes the conventions of traditional
      folk music and encourages stylistic or thematic innovation. It gave rise to the genre of
      psychedelic or psych folk and had a major impact on the development of progressive
      rock.</skos:definition>
    <skos:exactMatch xml:lang="en"
      >http://dbpedia.org/resource/Progressive_folk_music</skos:exactMatch>
    <skos:inScheme rdf:resource="http://data.europeana.eu/concept/music/genre/Music_Genre_Scheme"/>
    <skos:altLabel xml:lang="en">Progressive folk</skos:altLabel>
  </skos:Concept>

  <skos:Concept rdf:about="http://data.europeana.eu/concept/music/genre/Kansas_City_blues">
    <skos:prefLabel xml:lang="en">Kansas City blues</skos:prefLabel>
    <skos:prefLabel xml:lang="fr">Kansas City blues</skos:prefLabel>
    <skos:closeMatch rdf:resource="http://rdf.freebase.com/ns/m.026k_pw"/>
    <skos:broader rdf:resource="http://data.europeana.eu/concept/music/genre/Blues_fusions"/>
    <skos:definition xml:lang="en">Kansas City blues is a genre of blues music. It has spawned the
      Kansas City Blues &amp; Jazz festival and the Kansas City Blues Society.</skos:definition>
    <skos:exactMatch xml:lang="en">http://dbpedia.org/resource/Kansas_City_blues</skos:exactMatch>
    <skos:inScheme rdf:resource="http://data.europeana.eu/concept/music/genre/Music_Genre_Scheme"/>
    <skos:altLabel xml:lang="en">Kansas City blues</skos:altLabel>
  </skos:Concept>

  <skos:Concept rdf:about="http://data.europeana.eu/concept/music/genre/Onkyokei">
    <skos:prefLabel xml:lang="en">Onkyokei</skos:prefLabel>
    <skos:prefLabel xml:lang="nl">Onkyo</skos:prefLabel>
    <skos:prefLabel xml:lang="fr">Onkyokei</skos:prefLabel>
    <skos:closeMatch rdf:resource="http://rdf.freebase.com/ns/m.027ks1l"/>
    <skos:broader rdf:resource="http://data.europeana.eu/concept/music/genre/Pop_music_fusions"/>
    <skos:definition xml:lang="en">The Onkyo music movement or Onkyokei is a form of free
      improvisation, emerging from Japan in the late 1990s. Onky? places much more emphasis on sound
      texture than on musical structure, distilling elements of techno, noise, and electronic music
      into a unique hybrid. &lt;p&gt; The Off Site, a venue in Tokyo, is home to the Onkyo music
      movement, which is characterized by improvisation, minimalism, and &quot;quiet noise&quot;.
      Onkyo improvisation, &quot;explores the fine-grained textural details of acoustic and
      electronic sound&quot;. &lt;p&gt; It is typified by small and often quiet musical gestures,
      and liberal use of both electronics and silence. Prominent musicians working in this area
      include Toshimaru Nakamura, Sachiko M, Yoshihide Otomo, Tetuzi Akiyama, and Taku Sugimoto.
      &lt;p&gt; It influenced the development of electroacoustic improvisation or EAI, a genre with
      which it is strongly intertwined. The transnational circulation of onkyo also influenced its
      representation as a form of &quot;Japanese new music,&quot; despite claims by its authors that
      onkyo had little to do with Japanese cultural identity.</skos:definition>
    <skos:exactMatch xml:lang="en">http://dbpedia.org/resource/Onkyokei</skos:exactMatch>
    <skos:inScheme rdf:resource="http://data.europeana.eu/concept/music/genre/Music_Genre_Scheme"/>
    <skos:altLabel xml:lang="en">Onkyokei</skos:altLabel>
  </skos:Concept>

  <skos:Concept rdf:about="http://data.europeana.eu/concept/music/genre/Death_metal">
    <skos:prefLabel xml:lang="en">Death metal</skos:prefLabel>
    <skos:prefLabel xml:lang="ar">ديث ميتال</skos:prefLabel>
    <skos:prefLabel xml:lang="bg">Дет метъл</skos:prefLabel>
    <skos:prefLabel xml:lang="ca">Death metal</skos:prefLabel>
    <skos:prefLabel xml:lang="hr">Death metal</skos:prefLabel>
    <skos:prefLabel xml:lang="cs">Death metal</skos:prefLabel>
    <skos:prefLabel xml:lang="da">Dødsmetal</skos:prefLabel>
    <skos:prefLabel xml:lang="nl">Deathmetal</skos:prefLabel>
    <skos:prefLabel xml:lang="et">Death metal</skos:prefLabel>
    <skos:prefLabel xml:lang="fi">Death metal</skos:prefLabel>
    <skos:prefLabel xml:lang="fr">Death metal</skos:prefLabel>
    <skos:prefLabel xml:lang="de">Death Metal</skos:prefLabel>
    <skos:prefLabel xml:lang="hu">Death metal</skos:prefLabel>
    <skos:prefLabel xml:lang="id">Death metal</skos:prefLabel>
    <skos:prefLabel xml:lang="it">Death metal</skos:prefLabel>
    <skos:prefLabel xml:lang="ja">デスメタル</skos:prefLabel>
    <skos:prefLabel xml:lang="ko">데스 메탈</skos:prefLabel>
    <skos:prefLabel xml:lang="lv">Nāves metāls</skos:prefLabel>
    <skos:prefLabel xml:lang="lt">Death metal</skos:prefLabel>
    <skos:prefLabel xml:lang="ms">Death metal</skos:prefLabel>
    <skos:prefLabel xml:lang="no">Death metal</skos:prefLabel>
    <skos:prefLabel xml:lang="fa">دث متال</skos:prefLabel>
    <skos:prefLabel xml:lang="pl">Death metal</skos:prefLabel>
    <skos:prefLabel xml:lang="pt">Death metal</skos:prefLabel>
    <skos:prefLabel xml:lang="ro">Death metal</skos:prefLabel>
    <skos:prefLabel xml:lang="ru">Дэт-метал</skos:prefLabel>
    <skos:prefLabel xml:lang="sr">Det metal</skos:prefLabel>
    <skos:prefLabel xml:lang="sk">Death metal</skos:prefLabel>
    <skos:prefLabel xml:lang="sl">Death metal</skos:prefLabel>
    <skos:prefLabel xml:lang="es">Death metal</skos:prefLabel>
    <skos:prefLabel xml:lang="sv">Death metal</skos:prefLabel>
    <skos:prefLabel xml:lang="th">เดทเมทัล</skos:prefLabel>
    <skos:prefLabel xml:lang="tr">Death metal</skos:prefLabel>
    <skos:prefLabel xml:lang="uk">Дез-метал</skos:prefLabel>
    <skos:prefLabel xml:lang="vi">Death metal</skos:prefLabel>
    <skos:closeMatch rdf:resource="http://rdf.freebase.com/ns/m.0296y"/>
    <skos:broader
      rdf:resource="http://data.europeana.eu/concept/music/genre/Heavy_metal_music_fusions"/>
    <skos:definition xml:lang="en">Death metal is an extreme subgenre of heavy metal music. It
      typically employs heavily distorted guitars, tremolo picking, deep growling vocals, double
      kick or blast beat drumming, minor keys or atonality, and multiple tempo changes. &lt;p&gt;
      Building from the musical structure of thrash metal and early black metal, death metal emerged
      during the mid-1980s. Bands such as Venom, Slayer, and Kreator, were important influences on
      the genre's creation. Possessed and Death, along with bands such as Obituary, Deicide,
      Cannibal Corpse, and Morbid Angel, are often considered pioneers of the genre. In the late
      1980s and early 1990s, death metal gained more media attention as popular genre niche record
      labels like Combat, Earache, and Roadrunner, began to sign death metal bands at a rapid rate.
      Since then, death metal has diversified, spawning a variety of subgenres.</skos:definition>
    <skos:exactMatch xml:lang="en">http://dbpedia.org/resource/Death_metal</skos:exactMatch>
    <skos:inScheme rdf:resource="http://data.europeana.eu/concept/music/genre/Music_Genre_Scheme"/>
    <skos:altLabel xml:lang="en">Death metal</skos:altLabel>
  </skos:Concept>

  <skos:Concept rdf:about="http://data.europeana.eu/concept/music/genre/Noise_rock">
    <skos:prefLabel xml:lang="en">Noise rock</skos:prefLabel>
    <skos:prefLabel xml:lang="bg">Нойз рок</skos:prefLabel>
    <skos:prefLabel xml:lang="hr">Noise rock</skos:prefLabel>
    <skos:prefLabel xml:lang="cs">Noise rock</skos:prefLabel>
    <skos:prefLabel xml:lang="da">Støjrock</skos:prefLabel>
    <skos:prefLabel xml:lang="nl">Noiserock</skos:prefLabel>
    <skos:prefLabel xml:lang="et">Noise rock</skos:prefLabel>
    <skos:prefLabel xml:lang="fr">Noise rock</skos:prefLabel>
    <skos:prefLabel xml:lang="de">Noise-Rock</skos:prefLabel>
    <skos:prefLabel xml:lang="hu">Noise rock</skos:prefLabel>
    <skos:prefLabel xml:lang="it">Noise rock</skos:prefLabel>
    <skos:prefLabel xml:lang="ja">ノイズロック</skos:prefLabel>
    <skos:prefLabel xml:lang="lv">Trokšņu roks</skos:prefLabel>
    <skos:prefLabel xml:lang="no">Støyrock</skos:prefLabel>
    <skos:prefLabel xml:lang="pl">Noise rock</skos:prefLabel>
    <skos:prefLabel xml:lang="pt">Noise rock</skos:prefLabel>
    <skos:prefLabel xml:lang="ro">Noise rock</skos:prefLabel>
    <skos:prefLabel xml:lang="ru">Нойз-рок</skos:prefLabel>
    <skos:prefLabel xml:lang="es">Noise rock</skos:prefLabel>
    <skos:prefLabel xml:lang="sv">Noiserock</skos:prefLabel>
    <skos:prefLabel xml:lang="th">น็อยส์ร็อก</skos:prefLabel>
    <skos:prefLabel xml:lang="tr">Noise rock</skos:prefLabel>
    <skos:prefLabel xml:lang="uk">Нойз-рок</skos:prefLabel>
    <skos:closeMatch rdf:resource="http://rdf.freebase.com/ns/m.029fbr"/>
    <skos:broader rdf:resource="http://data.europeana.eu/concept/music/genre/Punk_rock_fusions"/>
    <skos:definition xml:lang="en">Noise rock, also called noise punk, describes a style of rock
      music that became prominent in the 1980s. Noise rock makes use of the traditional
      instrumentation and iconography of rock, but incorporates atonality and especially dissonance,
      and also frequently discards usual songwriting conventions.</skos:definition>
    <skos:exactMatch xml:lang="en">http://dbpedia.org/resource/Noise_rock</skos:exactMatch>
    <skos:inScheme rdf:resource="http://data.europeana.eu/concept/music/genre/Music_Genre_Scheme"/>
    <skos:altLabel xml:lang="en">Noise rock</skos:altLabel>
  </skos:Concept>

  <skos:Concept rdf:about="http://data.europeana.eu/concept/music/genre/Electro_music">
    <skos:prefLabel xml:lang="en">Electro</skos:prefLabel>
    <skos:prefLabel xml:lang="ar">إليكترو</skos:prefLabel>
    <skos:prefLabel xml:lang="hr">Electro</skos:prefLabel>
    <skos:prefLabel xml:lang="cs">Electro</skos:prefLabel>
    <skos:prefLabel xml:lang="nl">Electro</skos:prefLabel>
    <skos:prefLabel xml:lang="fi">Elektro</skos:prefLabel>
    <skos:prefLabel xml:lang="fr">Electro</skos:prefLabel>
    <skos:prefLabel xml:lang="de">Electro</skos:prefLabel>
    <skos:prefLabel xml:lang="hu">Elektro</skos:prefLabel>
    <skos:prefLabel xml:lang="it">Electro</skos:prefLabel>
    <skos:prefLabel xml:lang="ja">エレクトロ</skos:prefLabel>
    <skos:prefLabel xml:lang="lt">Electro</skos:prefLabel>
    <skos:prefLabel xml:lang="fa">الکترو</skos:prefLabel>
    <skos:prefLabel xml:lang="pl">Electro</skos:prefLabel>
    <skos:prefLabel xml:lang="pt">Electro</skos:prefLabel>
    <skos:prefLabel xml:lang="ro">Electro</skos:prefLabel>
    <skos:prefLabel xml:lang="ru">Электро</skos:prefLabel>
    <skos:prefLabel xml:lang="sk">Electro</skos:prefLabel>
    <skos:prefLabel xml:lang="es">Electro</skos:prefLabel>
    <skos:prefLabel xml:lang="sv">Electro</skos:prefLabel>
    <skos:prefLabel xml:lang="th">ดนตรีอิเล็กโทร</skos:prefLabel>
    <skos:prefLabel xml:lang="uk">Електро</skos:prefLabel>
    <skos:closeMatch rdf:resource="http://rdf.freebase.com/ns/m.029h7y"/>
    <skos:broader rdf:resource="http://data.europeana.eu/concept/music/genre/Hip_hop_music_fusions"/>
    <skos:definition xml:lang="en">Electro is a genre of electronic dance music directly influenced
      by the use of TR-808 drum machines, and funk sampling. Records in the genre typically feature
      drum machines and heavy electronic sounds, usually without vocals, although if vocals are
      present they are delivered in a deadpan manner, often through electronic distortion such as
      vocoding and talkboxing. This is the main distinction between electro and previously prominent
      genres such as disco, in which the electronic sound was only part of the
      instrumentation.</skos:definition>
    <skos:exactMatch xml:lang="en">http://dbpedia.org/resource/Electro_music</skos:exactMatch>
    <skos:inScheme rdf:resource="http://data.europeana.eu/concept/music/genre/Music_Genre_Scheme"/>
    <skos:altLabel xml:lang="en">Electro</skos:altLabel>
  </skos:Concept>

  <skos:Concept rdf:about="http://data.europeana.eu/concept/music/genre/Zouk">
    <skos:prefLabel xml:lang="en">Zouk</skos:prefLabel>
    <skos:prefLabel xml:lang="nl">Zouk</skos:prefLabel>
    <skos:prefLabel xml:lang="fi">Zouk</skos:prefLabel>
    <skos:prefLabel xml:lang="fr">Zouk</skos:prefLabel>
    <skos:prefLabel xml:lang="de">Zouk</skos:prefLabel>
    <skos:prefLabel xml:lang="it">Zouk</skos:prefLabel>
    <skos:prefLabel xml:lang="ja">ズーク</skos:prefLabel>
    <skos:prefLabel xml:lang="ko">주크</skos:prefLabel>
    <skos:prefLabel xml:lang="lv">Zuks</skos:prefLabel>
    <skos:prefLabel xml:lang="pl">Zouk</skos:prefLabel>
    <skos:prefLabel xml:lang="pt">Zouk</skos:prefLabel>
    <skos:prefLabel xml:lang="ro">Zouk</skos:prefLabel>
    <skos:prefLabel xml:lang="ru">Зук</skos:prefLabel>
    <skos:prefLabel xml:lang="es">Zouk</skos:prefLabel>
    <skos:prefLabel xml:lang="sv">Zouk</skos:prefLabel>
    <skos:closeMatch rdf:resource="http://rdf.freebase.com/ns/m.02c65_"/>
    <skos:broader
      rdf:resource="http://data.europeana.eu/concept/music/genre/Latin_American_music_fusions"/>
    <skos:definition xml:lang="en">Zouk is a fast jump up carnival beat style of rhythmic music
      originating from the Caribbean islands of Guadeloupe and Martinique, popularized by the French
      Antilles Kassav' in the 1980s. &lt;p&gt; Elements of gwo ka, tambour bélé, ti bwa and biguine
      vide, including the full use of the MIDI technology, are prominent in zouk. Its originator
      French Antilles Kassav' is the only band that includes it in its repertoire to a lesser
      extent. Too fast, the style lost ground in the 80's due to the strong presence of kadans or
      compas music, the main music of the French Antilles. &lt;p&gt; Today, zouk is the French
      Antilles compas music, also called zouk-love.</skos:definition>
    <skos:exactMatch xml:lang="en">http://dbpedia.org/resource/Zouk</skos:exactMatch>
    <skos:inScheme rdf:resource="http://data.europeana.eu/concept/music/genre/Music_Genre_Scheme"/>
    <skos:altLabel xml:lang="en">Zouk</skos:altLabel>
  </skos:Concept>

  <skos:Concept rdf:about="http://data.europeana.eu/concept/music/genre/Electroacoustic_music">
    <skos:prefLabel xml:lang="en">Electroacoustic music</skos:prefLabel>
    <skos:prefLabel xml:lang="ar">إليكتروكوستيك</skos:prefLabel>
    <skos:prefLabel xml:lang="ca">Música electroacústica</skos:prefLabel>
    <skos:prefLabel xml:lang="cs">Elektroakustická hudba</skos:prefLabel>
    <skos:prefLabel xml:lang="nl">Elektroakoestische muziek</skos:prefLabel>
    <skos:prefLabel xml:lang="et">Elektroakustiline muusika</skos:prefLabel>
    <skos:prefLabel xml:lang="fr">Musique électroacoustique</skos:prefLabel>
    <skos:prefLabel xml:lang="de">Elektroakustische Musik</skos:prefLabel>
    <skos:prefLabel xml:lang="el">Ηλεκτροακουστική μουσική</skos:prefLabel>
    <skos:prefLabel xml:lang="it">Musica elettroacustica</skos:prefLabel>
    <skos:prefLabel xml:lang="ru">Электроакустическая музыка</skos:prefLabel>
    <skos:prefLabel xml:lang="es">Música electroacústica</skos:prefLabel>
    <skos:prefLabel xml:lang="sv">Elektroakustisk musik</skos:prefLabel>
    <skos:prefLabel xml:lang="uk">Електроакустична музика</skos:prefLabel>
    <skos:closeMatch rdf:resource="http://rdf.freebase.com/ns/m.02cr48"/>
    <skos:broader
      rdf:resource="http://data.europeana.eu/concept/music/genre/Electronic_music_fusions"/>
    <skos:definition xml:lang="en">Electroacoustic music originated in Western art music during the
      modern era following the incorporation of electric sound production into compositional
      practice. The initial developments in electroacoustic music composition during the 20th
      century are associated with the activities of the Groupe de Recherches Musicales at the ORTF
      in Paris, the home of musique concrete, the Nordwestdeutscher Rundfunk studio in Cologne,
      where the focus was on the composition of elektronische Musik, and the Columbia-Princeton
      Electronic Music Center in New York, where tape music, electronic music, and computer music
      were all explored.</skos:definition>
    <skos:exactMatch xml:lang="en"
      >http://dbpedia.org/resource/Electroacoustic_music</skos:exactMatch>
    <skos:inScheme rdf:resource="http://data.europeana.eu/concept/music/genre/Music_Genre_Scheme"/>
    <skos:altLabel xml:lang="en">Electroacoustic music</skos:altLabel>
  </skos:Concept>

  <skos:Concept rdf:about="http://data.europeana.eu/concept/music/genre/Acid_rock">
    <skos:prefLabel xml:lang="en">Acid rock</skos:prefLabel>
    <skos:prefLabel xml:lang="hr">Acid rock</skos:prefLabel>
    <skos:prefLabel xml:lang="cs">Acid rock</skos:prefLabel>
    <skos:prefLabel xml:lang="da">Syrerock</skos:prefLabel>
    <skos:prefLabel xml:lang="nl">Acid rock</skos:prefLabel>
    <skos:prefLabel xml:lang="fi">Acid rock</skos:prefLabel>
    <skos:prefLabel xml:lang="fr">Acid rock</skos:prefLabel>
    <skos:prefLabel xml:lang="it">Acid rock</skos:prefLabel>
    <skos:prefLabel xml:lang="fa">اسید راک</skos:prefLabel>
    <skos:prefLabel xml:lang="pl">Acid rock</skos:prefLabel>
    <skos:prefLabel xml:lang="pt">Acid rock</skos:prefLabel>
    <skos:prefLabel xml:lang="ru">Эйсид-рок</skos:prefLabel>
    <skos:prefLabel xml:lang="sr">Есид рок</skos:prefLabel>
    <skos:prefLabel xml:lang="sk">Acid rock</skos:prefLabel>
    <skos:prefLabel xml:lang="es">Rock ácido</skos:prefLabel>
    <skos:prefLabel xml:lang="sv">Acid rock</skos:prefLabel>
    <skos:closeMatch rdf:resource="http://rdf.freebase.com/ns/m.02l96k"/>
    <skos:broader rdf:resource="http://data.europeana.eu/concept/music/genre/Rock_music_fusions"/>
    <skos:definition xml:lang="en">Acid rock is a form of psychedelic rock, which is characterized
      by long instrumental solos, few lyrics, and musical improvisation. Tom Wolfe describes the
      LSD-influenced music of the Jimi Hendrix Experience, Pink Floyd, the Doors, Iron Butterfly,
      Big Brother &amp; the Holding Company, Cream, Jefferson Airplane, Ultimate Spinach, Blue
      Cheer, Quicksilver Messenger Service, the Great Society, Deep Purple and the Grateful Dead as
      &quot;acid rock&quot; in his book about Ken Kesey and the Acid Tests, The Electric Kool-Aid
      Acid Test. &lt;p&gt; &quot;Acid rock&quot; also refers to the subset of psychedelic rock bands
      that were part of, or were influenced by, the San Francisco Sound, and which played loud,
      &quot;heavy&quot; music featuring long improvised solos.</skos:definition>
    <skos:exactMatch xml:lang="en">http://dbpedia.org/resource/Acid_rock</skos:exactMatch>
    <skos:inScheme rdf:resource="http://data.europeana.eu/concept/music/genre/Music_Genre_Scheme"/>
    <skos:altLabel xml:lang="en">Acid rock</skos:altLabel>
  </skos:Concept>

  <skos:Concept rdf:about="http://data.europeana.eu/concept/music/genre/Teen_pop">
    <skos:prefLabel xml:lang="en">Teen pop</skos:prefLabel>
    <skos:prefLabel xml:lang="ar">بوب الشباب</skos:prefLabel>
    <skos:prefLabel xml:lang="ca">Teen pop</skos:prefLabel>
    <skos:prefLabel xml:lang="cs">Teen pop</skos:prefLabel>
    <skos:prefLabel xml:lang="et">Teismeliste pop</skos:prefLabel>
    <skos:prefLabel xml:lang="fi">Teinipop</skos:prefLabel>
    <skos:prefLabel xml:lang="fr">Teen pop</skos:prefLabel>
    <skos:prefLabel xml:lang="id">Pop remaja</skos:prefLabel>
    <skos:prefLabel xml:lang="it">Teen pop</skos:prefLabel>
    <skos:prefLabel xml:lang="ja">ティーン・ポップ</skos:prefLabel>
    <skos:prefLabel xml:lang="ko">틴 팝</skos:prefLabel>
    <skos:prefLabel xml:lang="lt">Teen pop</skos:prefLabel>
    <skos:prefLabel xml:lang="no">Teenpop</skos:prefLabel>
    <skos:prefLabel xml:lang="fa">تین پاپ</skos:prefLabel>
    <skos:prefLabel xml:lang="pl">Teen pop</skos:prefLabel>
    <skos:prefLabel xml:lang="pt">Teen pop</skos:prefLabel>
    <skos:prefLabel xml:lang="ru">Тин-поп</skos:prefLabel>
    <skos:prefLabel xml:lang="es">Teen pop</skos:prefLabel>
    <skos:prefLabel xml:lang="sv">Tonårspop</skos:prefLabel>
    <skos:prefLabel xml:lang="th">ทีนป็อป</skos:prefLabel>
    <skos:prefLabel xml:lang="tr">Teen pop</skos:prefLabel>
    <skos:prefLabel xml:lang="uk">Тін-поп</skos:prefLabel>
    <skos:prefLabel xml:lang="vi">Teen pop</skos:prefLabel>
    <skos:closeMatch rdf:resource="http://rdf.freebase.com/ns/m.02ny8t"/>
    <skos:broader rdf:resource="http://data.europeana.eu/concept/music/genre/Pop_music_fusions"/>
    <skos:definition xml:lang="en">Teen pop is a subgenre of pop music that is created, marketed and
      oriented towards preteens and teenagers. Teen pop copies genres and styles such as pop, dance,
      electronic, R&amp;B, rap, country and rock. Typical characteristics of teen pop music include
      auto-tuned vocals, choreographed dancing, emphasis on visual appeal, lyrics focused on teenage
      issues such as love/relationships, finding yourself, friendships, coming of age, fitting in,
      and growing up, regardless of the artists' age and repeated chorus lines along with a
      generally happy tune in the background.</skos:definition>
    <skos:exactMatch xml:lang="en">http://dbpedia.org/resource/Teen_pop</skos:exactMatch>
    <skos:inScheme rdf:resource="http://data.europeana.eu/concept/music/genre/Music_Genre_Scheme"/>
    <skos:altLabel xml:lang="en">Teen pop</skos:altLabel>
  </skos:Concept>

  <skos:Concept rdf:about="http://data.europeana.eu/concept/music/genre/Breakstep">
    <skos:prefLabel xml:lang="en">Breakstep</skos:prefLabel>
    <skos:prefLabel xml:lang="ru">Брейкстеп</skos:prefLabel>
    <skos:prefLabel xml:lang="sk">Breakstep</skos:prefLabel>
    <skos:prefLabel xml:lang="es">Breakstep</skos:prefLabel>
    <skos:prefLabel xml:lang="uk">Брейкстеп</skos:prefLabel>
    <skos:closeMatch rdf:resource="http://rdf.freebase.com/ns/m.02p722c"/>
    <skos:broader rdf:resource="http://data.europeana.eu/concept/music/genre/Hip_hop_music_fusions"/>
    <skos:definition xml:lang="en">Breakstep, or breakbeat garage, is a type of music that evolved
      from the UK garage scene and influenced the emergence of dubstep.</skos:definition>
    <skos:exactMatch xml:lang="en">http://dbpedia.org/resource/Breakstep</skos:exactMatch>
    <skos:inScheme rdf:resource="http://data.europeana.eu/concept/music/genre/Music_Genre_Scheme"/>
    <skos:altLabel xml:lang="en">Breakstep</skos:altLabel>
  </skos:Concept>

  <skos:Concept rdf:about="http://data.europeana.eu/concept/music/genre/Reggae_fusion">
    <skos:prefLabel xml:lang="en">Reggae fusion</skos:prefLabel>
    <skos:prefLabel xml:lang="cs">Reggae fusion</skos:prefLabel>
    <skos:prefLabel xml:lang="fr">Reggae fusion</skos:prefLabel>
    <skos:prefLabel xml:lang="it">Reggae fusion</skos:prefLabel>
    <skos:prefLabel xml:lang="pt">Reggae fusion</skos:prefLabel>
    <skos:prefLabel xml:lang="ro">Reggae fusion</skos:prefLabel>
    <skos:prefLabel xml:lang="es">Reggae fusion</skos:prefLabel>
    <skos:prefLabel xml:lang="th">เร้กเก้ฟิวชัน</skos:prefLabel>
    <skos:closeMatch rdf:resource="http://rdf.freebase.com/ns/m.02pl5bx"/>
    <skos:broader rdf:resource="http://data.europeana.eu/concept/music/genre/Hip_hop_music_fusions"/>
    <skos:definition xml:lang="en">Reggae fusion is a fusion genre of reggae that mixes reggae or
      dancehall with other genres, such as pop, rock, R&amp;B, jazz &amp; drum and bass. &lt;p&gt;
      In addition to characterizing fusions of reggae music with other genres, the term is used to
      describe artists who frequently switch between reggae and other genres, mainly hip hop, such
      as Kardinal Offishall, Sean Kingston,and Heavy D. The term is also used to describe artists
      who are known to deejay over instrumentals which are neither reggae nor dancehall, such as
      Sean Paul, Rihanna, Bruno Mars, Elephant Man, Shaggy, Beenie Man, Snow, Natasja Saad, Diana
      King, Bridgit Mendler, Delly Ranx, Dionne Bromfield and Tessanne Chin.</skos:definition>
    <skos:exactMatch xml:lang="en">http://dbpedia.org/resource/Reggae_fusion</skos:exactMatch>
    <skos:inScheme rdf:resource="http://data.europeana.eu/concept/music/genre/Music_Genre_Scheme"/>
    <skos:altLabel xml:lang="en">Reggae fusion</skos:altLabel>
  </skos:Concept>

  <skos:Concept rdf:about="http://data.europeana.eu/concept/music/genre/Ethnic_electronica">
    <skos:prefLabel xml:lang="en">Ethnic electronica</skos:prefLabel>
    <skos:prefLabel xml:lang="it">Etno-elettronica</skos:prefLabel>
    <skos:prefLabel xml:lang="fa">اتنیک الکترونیکا</skos:prefLabel>
    <skos:prefLabel xml:lang="ru">Этно-электроника</skos:prefLabel>
    <skos:prefLabel xml:lang="sk">Ethnic electronica</skos:prefLabel>
    <skos:prefLabel xml:lang="es">Etno electrónica</skos:prefLabel>
    <skos:prefLabel xml:lang="uk">Етно-електроніка</skos:prefLabel>
    <skos:closeMatch rdf:resource="http://rdf.freebase.com/ns/m.02py4h1"/>
    <skos:broader
      rdf:resource="http://data.europeana.eu/concept/music/genre/Electronic_music_fusions"/>
    <skos:definition xml:lang="en">Ethnic electronica combines elements of electronic and world
      music and was developed in the 1990s. The term ethnic electronica appears in music zines, in
      online music-related forums and blogs, and also in a title of a 2003 compilation Another Life:
      A Journey Into Ethnic Electronica. The term &quot;ethno-techno&quot; was first seen with the
      release of Ethno-Techno: Sonic Anthropology Vol 1 Wax Trax! in 1994. &lt;p&gt; Notable acts of
      ethnic electronica include Bryn Jones with his project Muslimgauze, the artists of Asian
      underground movement, Mozani Ramzan, Shpongle, Ott, Zavoloka, Banco de Gaia, AeTopus, Zingaia,
      Afro-Celt Sound System, Métisse, A Tribe Called Red, early work by Yat-Kha. Among the
      commercial acts which work with this subgenre: Praise, Enigma, ephemeral mists, Deep Forest,
      Ivan Kupala, Stelsi, Agricantus. Another notable act commonly associated with the genre is
      Beats Antique, which combines world, electronic and Middle Eastern bellydance music
      elements.</skos:definition>
    <skos:exactMatch xml:lang="en">http://dbpedia.org/resource/Ethnic_electronica</skos:exactMatch>
    <skos:inScheme rdf:resource="http://data.europeana.eu/concept/music/genre/Music_Genre_Scheme"/>
    <skos:altLabel xml:lang="en">Ethnic electronica</skos:altLabel>
  </skos:Concept>

  <skos:Concept rdf:about="http://data.europeana.eu/concept/music/genre/Space_disco">
    <skos:prefLabel xml:lang="en">Space disco</skos:prefLabel>
    <skos:prefLabel xml:lang="cs">Space Disco</skos:prefLabel>
    <skos:prefLabel xml:lang="da">Space disco</skos:prefLabel>
    <skos:prefLabel xml:lang="el">Space Disco</skos:prefLabel>
    <skos:prefLabel xml:lang="it">Space disco</skos:prefLabel>
    <skos:prefLabel xml:lang="fa">اسپیس دیسکو</skos:prefLabel>
    <skos:prefLabel xml:lang="pl">Space disco</skos:prefLabel>
    <skos:prefLabel xml:lang="es">Space disco</skos:prefLabel>
    <skos:closeMatch rdf:resource="http://rdf.freebase.com/ns/m.02qtqwt"/>
    <skos:broader
      rdf:resource="http://data.europeana.eu/concept/music/genre/Electronic_music_fusions"/>
    <skos:definition xml:lang="en">Space disco is the fusion of disco music with futuristic themes,
      sounds and visuals, a genre that became popular in the late 1970s. The main idea behind the
      genre is that of an exploration of the wonders of outer space by humans, and many bands often
      included robotic shapes, laser illumination and computer screens sequence in their live
      performances. The artists themselves often dressed in a manner inspired by glam rock and
      somewhat futuristic fashion. &lt;p&gt; Upon reaching Eastern Europe after 1980, the futuristic
      act was mainly dropped as many socialist state authorities often denied access to the stage
      for &quot;inappropriately&quot; dressed artists. Many bands then began performing at free,
      open-music events, festivals and formations to avoid political suppression, and the genre
      itself was slowly assimilated into purely instrumental, almost orchestral
      form.</skos:definition>
    <skos:exactMatch xml:lang="en">http://dbpedia.org/resource/Space_disco</skos:exactMatch>
    <skos:inScheme rdf:resource="http://data.europeana.eu/concept/music/genre/Music_Genre_Scheme"/>
    <skos:altLabel xml:lang="en">Space disco</skos:altLabel>
  </skos:Concept>

  <skos:Concept rdf:about="http://data.europeana.eu/concept/music/genre/Merenrap">
    <skos:prefLabel xml:lang="en">Merenrap</skos:prefLabel>
    <skos:prefLabel xml:lang="it">Merenrap</skos:prefLabel>
    <skos:prefLabel xml:lang="es">Merenrap</skos:prefLabel>
    <skos:closeMatch rdf:resource="http://rdf.freebase.com/ns/m.02r61b"/>
    <skos:broader rdf:resource="http://data.europeana.eu/concept/music/genre/Hip_hop_music_fusions"/>
    <skos:definition xml:lang="en">Merenhouse/Merenrap, is a hip hop music style formed by blending
      Dominican merengue music with rap, dancehall, reggae and hip hop.</skos:definition>
    <skos:exactMatch xml:lang="en">http://dbpedia.org/resource/Merenrap</skos:exactMatch>
    <skos:inScheme rdf:resource="http://data.europeana.eu/concept/music/genre/Music_Genre_Scheme"/>
    <skos:altLabel xml:lang="en">Merenrap</skos:altLabel>
  </skos:Concept>

  <skos:Concept rdf:about="http://data.europeana.eu/concept/music/genre/Indie_folk">
    <skos:prefLabel xml:lang="en">Indie folk</skos:prefLabel>
    <skos:prefLabel xml:lang="nl">Indiefolk</skos:prefLabel>
    <skos:prefLabel xml:lang="de">Indie-Folk</skos:prefLabel>
    <skos:prefLabel xml:lang="it">Indie folk</skos:prefLabel>
    <skos:prefLabel xml:lang="ja">インディー・フォーク</skos:prefLabel>
    <skos:prefLabel xml:lang="ko">인디 포크</skos:prefLabel>
    <skos:prefLabel xml:lang="no">Indiefolk</skos:prefLabel>
    <skos:prefLabel xml:lang="pt">Indie folk</skos:prefLabel>
    <skos:prefLabel xml:lang="ru">Инди-фолк</skos:prefLabel>
    <skos:prefLabel xml:lang="es">Indie folk</skos:prefLabel>
    <skos:prefLabel xml:lang="sv">Indiefolk</skos:prefLabel>
    <skos:prefLabel xml:lang="th">อินดีโฟล์ก</skos:prefLabel>
    <skos:prefLabel xml:lang="tr">İndie folk</skos:prefLabel>
    <skos:prefLabel xml:lang="uk">Інді фольк</skos:prefLabel>
    <skos:closeMatch rdf:resource="http://rdf.freebase.com/ns/m.02rp117"/>
    <skos:broader rdf:resource="http://data.europeana.eu/concept/music/genre/Folk_music_fusions"/>
    <skos:definition xml:lang="en">Indie folk is a music genre that arose in the 1990s from
      musicians in the indie rock community influenced by folk and classic country music. Indie folk
      combines the catchy melodies of indie rock with the acoustical sounds of contemporary folk
      music. Early artists included Ani DiFranco and Dan Bern. Later artists of note included The
      Decemberists, Fleet Foxes, The Cave Singers, Loch Lomond, Bon Iver, Or, The Whale, Great Lake
      Swimmers, and Blind Pilot. &lt;p&gt; The genre is related to freak folk, psych folk, baroque
      pop, and new weird America.</skos:definition>
    <skos:exactMatch xml:lang="en">http://dbpedia.org/resource/Indie_folk</skos:exactMatch>
    <skos:inScheme rdf:resource="http://data.europeana.eu/concept/music/genre/Music_Genre_Scheme"/>
    <skos:altLabel xml:lang="en">Indie folk</skos:altLabel>
  </skos:Concept>

  <skos:Concept rdf:about="http://data.europeana.eu/concept/music/genre/Italo_dance">
    <skos:prefLabel xml:lang="en">Italo dance</skos:prefLabel>
    <skos:prefLabel xml:lang="ca">Italo dance</skos:prefLabel>
    <skos:prefLabel xml:lang="cs">Italo dance</skos:prefLabel>
    <skos:prefLabel xml:lang="fi">Italodance</skos:prefLabel>
    <skos:prefLabel xml:lang="fr">Italodance</skos:prefLabel>
    <skos:prefLabel xml:lang="hu">Italo dance</skos:prefLabel>
    <skos:prefLabel xml:lang="it">Italo dance</skos:prefLabel>
    <skos:prefLabel xml:lang="ko">이탈로 댄스</skos:prefLabel>
    <skos:prefLabel xml:lang="pl">Nu italo disco</skos:prefLabel>
    <skos:prefLabel xml:lang="pt">Italo dance</skos:prefLabel>
    <skos:prefLabel xml:lang="es">Italo dance</skos:prefLabel>
    <skos:prefLabel xml:lang="sv">Italodance</skos:prefLabel>
    <skos:closeMatch rdf:resource="http://rdf.freebase.com/ns/m.02rxlng"/>
    <skos:broader rdf:resource="http://data.europeana.eu/concept/music/genre/Pop_music_fusions"/>
    <skos:definition xml:lang="en">Italo dance, also known as nu Italo disco, nu-Italo or just
      Italo, is an offshoot of the Eurodance music genre, which was especially popular in Europe in
      the late 1990s to the early 2000s.</skos:definition>
    <skos:exactMatch xml:lang="en">http://dbpedia.org/resource/Italo_dance</skos:exactMatch>
    <skos:inScheme rdf:resource="http://data.europeana.eu/concept/music/genre/Music_Genre_Scheme"/>
    <skos:altLabel xml:lang="en">Italo dance</skos:altLabel>
  </skos:Concept>

  <skos:Concept rdf:about="http://data.europeana.eu/concept/music/genre/Free_funk">
    <skos:prefLabel xml:lang="en">Free funk</skos:prefLabel>
    <skos:prefLabel xml:lang="pl">Free funk</skos:prefLabel>
    <skos:closeMatch rdf:resource="http://rdf.freebase.com/ns/m.02ryxvx"/>
    <skos:broader rdf:resource="http://data.europeana.eu/concept/music/genre/Jazz_fusions"/>
    <skos:definition xml:lang="en">Free funk is a term that Allmusic and writer Scott Yanow use to
      describe a combination of avant-garde jazz with funk music that developed in the 1970s.
      Leaders of the genre include Ornette Coleman and his Prime Time group, Ronald Shannon Jackson
      and his group Decoding Society, Jamaaladeen Tacuma and his group Spectacle and James
      &quot;Blood&quot; Ulmer. The music has been quite influential on the M-Base genre, as
      well.</skos:definition>
    <skos:exactMatch xml:lang="en">http://dbpedia.org/resource/Free_funk</skos:exactMatch>
    <skos:inScheme rdf:resource="http://data.europeana.eu/concept/music/genre/Music_Genre_Scheme"/>
    <skos:altLabel xml:lang="en">Free funk</skos:altLabel>
  </skos:Concept>

  <skos:Concept rdf:about="http://data.europeana.eu/concept/music/genre/Crust_punk">
    <skos:prefLabel xml:lang="en">Crust punk</skos:prefLabel>
    <skos:prefLabel xml:lang="ca">Crust punk</skos:prefLabel>
    <skos:prefLabel xml:lang="cs">Crust</skos:prefLabel>
    <skos:prefLabel xml:lang="da">Crust punk</skos:prefLabel>
    <skos:prefLabel xml:lang="nl">Crust punk</skos:prefLabel>
    <skos:prefLabel xml:lang="fi">Crust punk</skos:prefLabel>
    <skos:prefLabel xml:lang="fr">Crust punk</skos:prefLabel>
    <skos:prefLabel xml:lang="de">Crustcore</skos:prefLabel>
    <skos:prefLabel xml:lang="hu">Crust punk</skos:prefLabel>
    <skos:prefLabel xml:lang="it">Crust punk</skos:prefLabel>
    <skos:prefLabel xml:lang="ja">クラストコア</skos:prefLabel>
    <skos:prefLabel xml:lang="ko">크러스트 펑크</skos:prefLabel>
    <skos:prefLabel xml:lang="no">Crust punk</skos:prefLabel>
    <skos:prefLabel xml:lang="pl">Crust punk</skos:prefLabel>
    <skos:prefLabel xml:lang="pt">Crust punk</skos:prefLabel>
    <skos:prefLabel xml:lang="ro">Crust punk</skos:prefLabel>
    <skos:prefLabel xml:lang="ru">Краст-панк</skos:prefLabel>
    <skos:prefLabel xml:lang="sk">Crustcore</skos:prefLabel>
    <skos:prefLabel xml:lang="es">Crust punk</skos:prefLabel>
    <skos:prefLabel xml:lang="sv">Crust</skos:prefLabel>
    <skos:prefLabel xml:lang="uk">Краст-панк</skos:prefLabel>
    <skos:closeMatch rdf:resource="http://rdf.freebase.com/ns/m.02srgf"/>
    <skos:broader rdf:resource="http://data.europeana.eu/concept/music/genre/Punk_rock_fusions"/>
    <skos:definition xml:lang="en">Crust punk is a form of music influenced by anarcho-punk,
      hardcore punk and extreme metal. The style, which evolved in the mid-1980s in England, often
      has songs with dark and pessimistic lyrics that linger on political and social ills. The term
      &quot;crust&quot; was coined by Hellbastard on their 1986 Ripper Crust demo. &lt;p&gt; Crust
      is partly defined by its &quot;bassy&quot; and &quot;dirty&quot; sound. It is often played at
      a fast tempo with occasional slow sections. Vocals are usually guttural and may be grunted,
      growled or screamed. Crust punk takes cues from heavy metal band Black Sabbath and the
      anarcho-punk of Discharge and the extreme metal of bands like Venom, Celtic Frost and
      Motörhead. While the term was first associated with Amebix have been described as the
      originators of the style.</skos:definition>
    <skos:exactMatch xml:lang="en">http://dbpedia.org/resource/Crust_punk</skos:exactMatch>
    <skos:inScheme rdf:resource="http://data.europeana.eu/concept/music/genre/Music_Genre_Scheme"/>
    <skos:altLabel xml:lang="en">Crust punk</skos:altLabel>
  </skos:Concept>

  <skos:Concept rdf:about="http://data.europeana.eu/concept/music/genre/Ambient_house">
    <skos:prefLabel xml:lang="en">Ambient house</skos:prefLabel>
    <skos:prefLabel xml:lang="nl">Ambient house</skos:prefLabel>
    <skos:prefLabel xml:lang="fr">Ambient house</skos:prefLabel>
    <skos:prefLabel xml:lang="it">Ambient house</skos:prefLabel>
    <skos:prefLabel xml:lang="ja">アンビエント・ハウス</skos:prefLabel>
    <skos:prefLabel xml:lang="fa">امبینت هاوس</skos:prefLabel>
    <skos:prefLabel xml:lang="pl">Ambient house</skos:prefLabel>
    <skos:prefLabel xml:lang="pt">Ambient house</skos:prefLabel>
    <skos:prefLabel xml:lang="ro">Ambient house</skos:prefLabel>
    <skos:prefLabel xml:lang="sk">Ambient house</skos:prefLabel>
    <skos:prefLabel xml:lang="es">Ambient house</skos:prefLabel>
    <skos:prefLabel xml:lang="uk">Ембієнт хауз</skos:prefLabel>
    <skos:closeMatch rdf:resource="http://rdf.freebase.com/ns/m.02t3b_"/>
    <skos:broader
      rdf:resource="http://data.europeana.eu/concept/music/genre/Electronic_music_fusions"/>
    <skos:definition xml:lang="en">Ambient house, a music genre that first emerged in the late
      1980s, is a sub-genre of house music, combining elements of acid house and ambient music.
      Tracks in the ambient house genre typically feature four-on-the-floor beat patterns, synth
      pads, and vocal samples integrated in a style classed as
      &quot;atmospheric&quot;.</skos:definition>
    <skos:exactMatch xml:lang="en">http://dbpedia.org/resource/Ambient_house</skos:exactMatch>
    <skos:inScheme rdf:resource="http://data.europeana.eu/concept/music/genre/Music_Genre_Scheme"/>
    <skos:altLabel xml:lang="en">Ambient house</skos:altLabel>
  </skos:Concept>

  <skos:Concept rdf:about="http://data.europeana.eu/concept/music/genre/Industrial_metal">
    <skos:prefLabel xml:lang="en">Industrial metal</skos:prefLabel>
    <skos:prefLabel xml:lang="ca">Metal industrial</skos:prefLabel>
    <skos:prefLabel xml:lang="hr">Industrial metal</skos:prefLabel>
    <skos:prefLabel xml:lang="cs">Industrial metal</skos:prefLabel>
    <skos:prefLabel xml:lang="da">Industrial metal</skos:prefLabel>
    <skos:prefLabel xml:lang="nl">Industrial metal</skos:prefLabel>
    <skos:prefLabel xml:lang="fi">Industrial metal</skos:prefLabel>
    <skos:prefLabel xml:lang="fr">Metal industriel</skos:prefLabel>
    <skos:prefLabel xml:lang="de">Industrial Metal</skos:prefLabel>
    <skos:prefLabel xml:lang="hu">Indusztriális metal</skos:prefLabel>
    <skos:prefLabel xml:lang="id">Industrial metal</skos:prefLabel>
    <skos:prefLabel xml:lang="it">Industrial metal</skos:prefLabel>
    <skos:prefLabel xml:lang="ja">インダストリアル・メタル</skos:prefLabel>
    <skos:prefLabel xml:lang="ko">인더스트리얼 메탈</skos:prefLabel>
    <skos:prefLabel xml:lang="lv">Industriālais metāls</skos:prefLabel>
    <skos:prefLabel xml:lang="lt">Industrial metal</skos:prefLabel>
    <skos:prefLabel xml:lang="no">Industriell metal</skos:prefLabel>
    <skos:prefLabel xml:lang="fa">اینداستریال متال</skos:prefLabel>
    <skos:prefLabel xml:lang="pl">Industrial metal</skos:prefLabel>
    <skos:prefLabel xml:lang="pt">Metal industrial</skos:prefLabel>
    <skos:prefLabel xml:lang="ro">Industrial metal</skos:prefLabel>
    <skos:prefLabel xml:lang="ru">Индастриал-метал</skos:prefLabel>
    <skos:prefLabel xml:lang="sr">Индастријал метал</skos:prefLabel>
    <skos:prefLabel xml:lang="sk">Industriálny metal</skos:prefLabel>
    <skos:prefLabel xml:lang="es">Metal industrial</skos:prefLabel>
    <skos:prefLabel xml:lang="sv">Industrimetal</skos:prefLabel>
    <skos:prefLabel xml:lang="th">อินดัสเทรียลเมทัล</skos:prefLabel>
    <skos:prefLabel xml:lang="tr">Endüstriyel metal</skos:prefLabel>
    <skos:prefLabel xml:lang="uk">Індастріал-метал</skos:prefLabel>
    <skos:closeMatch rdf:resource="http://rdf.freebase.com/ns/m.02t8gf"/>
    <skos:broader
      rdf:resource="http://data.europeana.eu/concept/music/genre/Electronic_music_fusions"/>
    <skos:definition xml:lang="en">Industrial metal is a musical genre that draws from industrial
      dance music, thrash metal and hardcore punk, using repeating metal guitar riffs, sampling,
      synthesizer or sequencer lines, and distorted vocals. Founding industrial metal acts include
      Ministry, Godflesh, and KMFDM. &lt;p&gt; Industrial metal's popularity led to some criticism
      from other artists associated with the industrial scene. Subsequently, it is most well known
      in various European permutations. Industrial metal groups have produced many acclaimed music
      videos.</skos:definition>
    <skos:exactMatch xml:lang="en">http://dbpedia.org/resource/Industrial_metal</skos:exactMatch>
    <skos:inScheme rdf:resource="http://data.europeana.eu/concept/music/genre/Music_Genre_Scheme"/>
    <skos:altLabel xml:lang="en">Industrial metal</skos:altLabel>
  </skos:Concept>

  <skos:Concept rdf:about="http://data.europeana.eu/concept/music/genre/Western_swing">
    <skos:prefLabel xml:lang="en">Western swing</skos:prefLabel>
    <skos:prefLabel xml:lang="cs">Western swing</skos:prefLabel>
    <skos:prefLabel xml:lang="da">Western swing</skos:prefLabel>
    <skos:prefLabel xml:lang="nl">Western Swing</skos:prefLabel>
    <skos:prefLabel xml:lang="fr">Western Swing</skos:prefLabel>
    <skos:prefLabel xml:lang="de">Western Swing</skos:prefLabel>
    <skos:prefLabel xml:lang="pl">Western swing</skos:prefLabel>
    <skos:prefLabel xml:lang="es">Western swing</skos:prefLabel>
    <skos:closeMatch rdf:resource="http://rdf.freebase.com/ns/m.02wydx"/>
    <skos:broader rdf:resource="http://data.europeana.eu/concept/music/genre/Country_music_fusions"/>
    <skos:definition xml:lang="en">Western swing music is a subgenre of American country music that
      originated in the late 1920s in the West and South among the region's Western string bands. It
      is dance music, often with an up-tempo beat, which attracted huge crowds to dance halls and
      clubs in Texas, Oklahoma and California during the 1930s and 40s until a federal war-time
      nightclub tax in 1944 led to its decline. &lt;p&gt; The movement was an outgrowth of jazz, and
      similarities with Gypsy jazz are often noted. The music is an amalgamation of rural, cowboy,
      polka, folk, Dixieland jazz and blues blended with swing, and played by a hot string band
      often augmented with drums, saxophones, pianos and, notably, the steel guitar. The
      electrically amplified stringed instruments, especially the steel guitar, give the music a
      distinctive sound. Later incarnations have also included overtones of bebop. &lt;p&gt; Western
      swing differs in several ways from the music played by the nationally popular horn-driven big
      swing bands of the same era. In Western bands—even the fully orchestrated bands—vocals and
      other instruments followed the fiddle's lead.</skos:definition>
    <skos:exactMatch xml:lang="en">http://dbpedia.org/resource/Western_swing</skos:exactMatch>
    <skos:inScheme rdf:resource="http://data.europeana.eu/concept/music/genre/Music_Genre_Scheme"/>
    <skos:altLabel xml:lang="en">Western swing</skos:altLabel>
  </skos:Concept>

  <skos:Concept rdf:about="http://data.europeana.eu/concept/music/genre/Freestyle_music">
    <skos:prefLabel xml:lang="en">Freestyle</skos:prefLabel>
    <skos:prefLabel xml:lang="cs">Freestyle</skos:prefLabel>
    <skos:prefLabel xml:lang="fr">Freestyle</skos:prefLabel>
    <skos:prefLabel xml:lang="de">Freestyle</skos:prefLabel>
    <skos:prefLabel xml:lang="hu">Freestyle house</skos:prefLabel>
    <skos:prefLabel xml:lang="pl">Freestyle</skos:prefLabel>
    <skos:prefLabel xml:lang="pt">Freestyle</skos:prefLabel>
    <skos:prefLabel xml:lang="ru">Фристайл (рэп)</skos:prefLabel>
    <skos:prefLabel xml:lang="sk">Freestyle</skos:prefLabel>
    <skos:closeMatch rdf:resource="http://rdf.freebase.com/ns/m.02xjb"/>
    <skos:broader rdf:resource="http://data.europeana.eu/concept/music/genre/Hip_hop_music_fusions"/>
    <skos:definition xml:lang="en">Freestyle or Latin freestyle is a form of dance-pop or electronic
      dance music that emerged in the United States in the mid-1980s. It experienced its greatest
      popularity from the late-1980s until the early 1990s. It continues to be produced today and
      enjoys some degree of popularity, especially in the urban communities where Latinos and
      Italian Americans are found. &lt;p&gt; Notable performers in the freestyle genre include
      Stevie B, Corina, Timmy T, George Lamond, TKA, Noel, Company B, Exposé, The Cover Girls, Lisa
      Lisa and Cult Jam, Information Society, Sa-Fire, Sweet Sensation, Trilogy, Shannon, Nancy
      Martinez, Johnny O, Coro, Lisette Melendez, Judy Torres, Rockell, and many others. The music
      can be heard on some radio stations such as WKTU in New York City.</skos:definition>
    <skos:exactMatch xml:lang="en">http://dbpedia.org/resource/Freestyle_music</skos:exactMatch>
    <skos:inScheme rdf:resource="http://data.europeana.eu/concept/music/genre/Music_Genre_Scheme"/>
    <skos:altLabel xml:lang="en">Freestyle music</skos:altLabel>
  </skos:Concept>

  <skos:Concept rdf:about="http://data.europeana.eu/concept/music/genre/Nerdcore">
    <skos:prefLabel xml:lang="en">Nerdcore</skos:prefLabel>
    <skos:prefLabel xml:lang="nl">Nerdcore</skos:prefLabel>
    <skos:prefLabel xml:lang="de">Nerdcore</skos:prefLabel>
    <skos:prefLabel xml:lang="it">Nerdcore rap</skos:prefLabel>
    <skos:prefLabel xml:lang="pt">Nerdcore hip hop</skos:prefLabel>
    <skos:prefLabel xml:lang="ru">Nerdcore</skos:prefLabel>
    <skos:prefLabel xml:lang="es">Nerdcore Hip Hop</skos:prefLabel>
    <skos:closeMatch rdf:resource="http://rdf.freebase.com/ns/m.02y74y"/>
    <skos:broader rdf:resource="http://data.europeana.eu/concept/music/genre/Hip_hop_music_fusions"/>
    <skos:definition xml:lang="en">Nerdcore is a genre of hip hop music characterized by themes and
      subject matter considered to be of general interest to nerds. Self-described nerdcore musician
      MC Frontalot has the earliest known recorded use of the term in the 2000 song &quot;Nerdcore
      Hiphop&quot;. Frontalot, like most nerdcore artists, self-publishes his work and has released
      much of it for free online. As a niche genre, nerdcore generally holds to the DIY ethic, and
      has a history of self-publishing and self-production. &lt;p&gt; Though nerdcore rappers rhyme
      about anything from politics to science fiction, there are some perennial favorites in
      nerdcore subject matter, including Star Wars, role-playing games, science, fantasy and
      computers. &lt;p&gt; Music with similar themes, but different musical styles can be found in
      the filk genres. There are hip hop artists who have recorded compositions which focus on
      similar topics, but who are not generally considered nerdcore. Conversely, one does not need
      to concentrate on those topics to be nerdcore: most of the songs by Frontalot do not focus
      narrowly on stereotypically nerdy topics.</skos:definition>
    <skos:exactMatch xml:lang="en">http://dbpedia.org/resource/Nerdcore</skos:exactMatch>
    <skos:inScheme rdf:resource="http://data.europeana.eu/concept/music/genre/Music_Genre_Scheme"/>
    <skos:altLabel xml:lang="en">Nerdcore</skos:altLabel>
  </skos:Concept>

  <skos:Concept rdf:about="http://data.europeana.eu/concept/music/genre/Blues_rock">
    <skos:prefLabel xml:lang="en">Blues-rock</skos:prefLabel>
    <skos:prefLabel xml:lang="bg">Блус рок</skos:prefLabel>
    <skos:prefLabel xml:lang="ca">Blues rock</skos:prefLabel>
    <skos:prefLabel xml:lang="hr">Blues rock</skos:prefLabel>
    <skos:prefLabel xml:lang="cs">Blues rock</skos:prefLabel>
    <skos:prefLabel xml:lang="da">Blues rock</skos:prefLabel>
    <skos:prefLabel xml:lang="nl">Bluesrock</skos:prefLabel>
    <skos:prefLabel xml:lang="fi">Blues rock</skos:prefLabel>
    <skos:prefLabel xml:lang="fr">Blues rock</skos:prefLabel>
    <skos:prefLabel xml:lang="de">Bluesrock</skos:prefLabel>
    <skos:prefLabel xml:lang="hu">Blues-rock</skos:prefLabel>
    <skos:prefLabel xml:lang="it">Blues rock</skos:prefLabel>
    <skos:prefLabel xml:lang="ja">ブルースロック</skos:prefLabel>
    <skos:prefLabel xml:lang="ko">블루스 록</skos:prefLabel>
    <skos:prefLabel xml:lang="lv">Blūzroks</skos:prefLabel>
    <skos:prefLabel xml:lang="lt">Bliuzrokas</skos:prefLabel>
    <skos:prefLabel xml:lang="no">Bluesrock</skos:prefLabel>
    <skos:prefLabel xml:lang="pl">Blues rock</skos:prefLabel>
    <skos:prefLabel xml:lang="pt">Blues-rock</skos:prefLabel>
    <skos:prefLabel xml:lang="ru">Блюз-рок</skos:prefLabel>
    <skos:prefLabel xml:lang="sk">Blues rock</skos:prefLabel>
    <skos:prefLabel xml:lang="sl">Blues rock</skos:prefLabel>
    <skos:prefLabel xml:lang="es">Blues rock</skos:prefLabel>
    <skos:prefLabel xml:lang="sv">Bluesrock</skos:prefLabel>
    <skos:prefLabel xml:lang="th">บลูส์ร็อก</skos:prefLabel>
    <skos:prefLabel xml:lang="tr">Blues rock</skos:prefLabel>
    <skos:prefLabel xml:lang="uk">Блюз-рок</skos:prefLabel>
    <skos:closeMatch rdf:resource="http://rdf.freebase.com/ns/m.02yv6b"/>
    <skos:broader rdf:resource="http://data.europeana.eu/concept/music/genre/Blues_fusions"/>
    <skos:definition xml:lang="en">Blues rock is a musical genre combining bluesy improvisations
      over the twelve-bar blues and extended boogie jams with rock and roll styles. The core of the
      blues rock sound is created by the electric guitar, piano, bass guitar and drum kit, with the
      electric guitar usually amplified through a tube guitar amplifier, giving it an overdriven
      character. &lt;p&gt; The style began to develop in the mid-1960s in Britain and the United
      States. British bands, such as the Rolling Stones, the Yardbirds and the Animals and American
      bands such as the Butterfield Blues Band and the Siegel–Schwall Band, experimented with music
      from older African-American bluesmen, like Albert King, Howlin' Wolf, Robert Johnson, Jimmy
      Reed, Muddy Waters and B.B. King. While the early blues rock bands &quot;attempted to play
      long, involved improvisations which were commonplace on jazz records&quot;, by the 1970s,
      blues rock got heavier and more riff-based. By the &quot;early '70s, the lines between blues
      rock and hard rock were barely visible&quot;, as bands began recording rock-style
      albums.</skos:definition>
    <skos:exactMatch xml:lang="en">http://dbpedia.org/resource/Blues_rock</skos:exactMatch>
    <skos:inScheme rdf:resource="http://data.europeana.eu/concept/music/genre/Music_Genre_Scheme"/>
    <skos:altLabel xml:lang="en">Blues rock</skos:altLabel>
    <skos:altLabel xml:lang="en">Rock Blues</skos:altLabel>
    <skos:altLabel xml:lang="en">Blues-rock</skos:altLabel>
  </skos:Concept>

  <skos:Concept rdf:about="http://data.europeana.eu/concept/music/genre/Sludge_metal">
    <skos:prefLabel xml:lang="en">Sludge metal</skos:prefLabel>
    <skos:prefLabel xml:lang="hr">Sludge metal</skos:prefLabel>
    <skos:prefLabel xml:lang="cs">Sludge metal</skos:prefLabel>
    <skos:prefLabel xml:lang="da">Sludge metal</skos:prefLabel>
    <skos:prefLabel xml:lang="nl">Sludgemetal</skos:prefLabel>
    <skos:prefLabel xml:lang="fi">Sludge metal</skos:prefLabel>
    <skos:prefLabel xml:lang="fr">Sludge metal</skos:prefLabel>
    <skos:prefLabel xml:lang="de">Sludge</skos:prefLabel>
    <skos:prefLabel xml:lang="hu">Sludge metal</skos:prefLabel>
    <skos:prefLabel xml:lang="it">Sludge metal</skos:prefLabel>
    <skos:prefLabel xml:lang="no">Sludge metal</skos:prefLabel>
    <skos:prefLabel xml:lang="pl">Sludge metal</skos:prefLabel>
    <skos:prefLabel xml:lang="pt">Sludge metal</skos:prefLabel>
    <skos:prefLabel xml:lang="ro">Sludge metal</skos:prefLabel>
    <skos:prefLabel xml:lang="ru">Сладж-метал</skos:prefLabel>
    <skos:prefLabel xml:lang="sr">Sladž metal</skos:prefLabel>
    <skos:prefLabel xml:lang="sk">Sludge metal</skos:prefLabel>
    <skos:prefLabel xml:lang="es">Sludge metal</skos:prefLabel>
    <skos:prefLabel xml:lang="sv">Sludge metal</skos:prefLabel>
    <skos:prefLabel xml:lang="tr">Sludge metal</skos:prefLabel>
    <skos:prefLabel xml:lang="uk">Сладж-метал</skos:prefLabel>
    <skos:closeMatch rdf:resource="http://rdf.freebase.com/ns/m.02yy88"/>
    <skos:broader
      rdf:resource="http://data.europeana.eu/concept/music/genre/Heavy_metal_music_fusions"/>
    <skos:definition xml:lang="en">Sludge metal is a subgenre of heavy metal that melds elements of
      doom metal and hardcore punk and sometimes incorporates influences from grunge and noise rock.
      Sludge metal is typically harsh and abrasive, often featuring shouted or screamed vocals,
      heavily distorted instruments and sharply contrasting tempos. While the style was anticipated
      by the Melvins from Washington, many of its earliest pioneers were from the city of New
      Orleans.</skos:definition>
    <skos:exactMatch xml:lang="en">http://dbpedia.org/resource/Sludge_metal</skos:exactMatch>
    <skos:inScheme rdf:resource="http://data.europeana.eu/concept/music/genre/Music_Genre_Scheme"/>
    <skos:altLabel xml:lang="en">Sludge metal</skos:altLabel>
  </skos:Concept>

  <skos:Concept rdf:about="http://data.europeana.eu/concept/music/genre/Metalcore">
    <skos:prefLabel xml:lang="en">Metalcore</skos:prefLabel>
    <skos:prefLabel xml:lang="bg">Метълкор</skos:prefLabel>
    <skos:prefLabel xml:lang="ca">Metalcore</skos:prefLabel>
    <skos:prefLabel xml:lang="hr">Metalcore</skos:prefLabel>
    <skos:prefLabel xml:lang="cs">Metalcore</skos:prefLabel>
    <skos:prefLabel xml:lang="da">Metalcore</skos:prefLabel>
    <skos:prefLabel xml:lang="nl">Metalcore</skos:prefLabel>
    <skos:prefLabel xml:lang="et">Metalcore</skos:prefLabel>
    <skos:prefLabel xml:lang="fi">Metalcore</skos:prefLabel>
    <skos:prefLabel xml:lang="fr">Metalcore</skos:prefLabel>
    <skos:prefLabel xml:lang="de">Metalcore</skos:prefLabel>
    <skos:prefLabel xml:lang="hu">Metalcore</skos:prefLabel>
    <skos:prefLabel xml:lang="id">Metalcore</skos:prefLabel>
    <skos:prefLabel xml:lang="it">Metalcore</skos:prefLabel>
    <skos:prefLabel xml:lang="ja">メタルコア</skos:prefLabel>
    <skos:prefLabel xml:lang="ko">메탈코어</skos:prefLabel>
    <skos:prefLabel xml:lang="lv">Metālkors</skos:prefLabel>
    <skos:prefLabel xml:lang="lt">Metalcore</skos:prefLabel>
    <skos:prefLabel xml:lang="ms">Metalcore</skos:prefLabel>
    <skos:prefLabel xml:lang="no">Metalcore</skos:prefLabel>
    <skos:prefLabel xml:lang="fa">متال‌کور</skos:prefLabel>
    <skos:prefLabel xml:lang="pl">Metalcore</skos:prefLabel>
    <skos:prefLabel xml:lang="pt">Metalcore</skos:prefLabel>
    <skos:prefLabel xml:lang="ro">Metalcore</skos:prefLabel>
    <skos:prefLabel xml:lang="ru">Металкор</skos:prefLabel>
    <skos:prefLabel xml:lang="sr">Металкор</skos:prefLabel>
    <skos:prefLabel xml:lang="sk">Metalcore</skos:prefLabel>
    <skos:prefLabel xml:lang="sl">Metalcore</skos:prefLabel>
    <skos:prefLabel xml:lang="es">Metalcore</skos:prefLabel>
    <skos:prefLabel xml:lang="sv">Metalcore</skos:prefLabel>
    <skos:prefLabel xml:lang="th">เมทัลคอร์</skos:prefLabel>
    <skos:prefLabel xml:lang="tr">Metalcore</skos:prefLabel>
    <skos:prefLabel xml:lang="uk">Металкор</skos:prefLabel>
    <skos:prefLabel xml:lang="vi">Metalcore</skos:prefLabel>
    <skos:closeMatch rdf:resource="http://rdf.freebase.com/ns/m.02z7f3"/>
    <skos:broader
      rdf:resource="http://data.europeana.eu/concept/music/genre/Heavy_metal_music_fusions"/>
    <skos:definition xml:lang="en">Metalcore is a broad fusion genre of extreme metal and hardcore
      punk. The name is an amalgam of the names of the two genres, distinguished by its emphasis on
      breakdowns, which are slow, intense passages that are conducive to moshing. Pioneering bands,
      such as— Hogan's Heroes, Earth Crisis, and Integrity, —are described to lean more toward
      hardcore punk, whereas latter bands—Killswitch Engage, Bury Tomorrow, Underoath, All That
      Remains, Trivium, As I Lay Dying, Bullet for My Valentine, and The Devil Wears Prada —are
      described to lean more towards metal. Sepultura, who has been credited as &quot;helped to lay
      the groundwork&quot; in the 2000s, and Pantera, who influenced Trivium, Atreyu, Bleeding
      Through and Unearth, have also been influential in the 2000s, and the further development of
      metalcore.</skos:definition>
    <skos:exactMatch xml:lang="en">http://dbpedia.org/resource/Metalcore</skos:exactMatch>
    <skos:inScheme rdf:resource="http://data.europeana.eu/concept/music/genre/Music_Genre_Scheme"/>
    <skos:altLabel xml:lang="en">Metalcore</skos:altLabel>
  </skos:Concept>

  <skos:Concept rdf:about="http://data.europeana.eu/concept/music/genre/Hardstyle">
    <skos:prefLabel xml:lang="en">Hardstyle</skos:prefLabel>
    <skos:prefLabel xml:lang="ca">Hardstyle</skos:prefLabel>
    <skos:prefLabel xml:lang="hr">Hardstyle</skos:prefLabel>
    <skos:prefLabel xml:lang="cs">Hardstyle</skos:prefLabel>
    <skos:prefLabel xml:lang="da">Hardstyle</skos:prefLabel>
    <skos:prefLabel xml:lang="nl">Hardstyle</skos:prefLabel>
    <skos:prefLabel xml:lang="et">Hardstyle</skos:prefLabel>
    <skos:prefLabel xml:lang="fi">Hardstyle</skos:prefLabel>
    <skos:prefLabel xml:lang="fr">Hardstyle</skos:prefLabel>
    <skos:prefLabel xml:lang="de">Hardstyle</skos:prefLabel>
    <skos:prefLabel xml:lang="hu">Hardstyle</skos:prefLabel>
    <skos:prefLabel xml:lang="it">Hardstyle</skos:prefLabel>
    <skos:prefLabel xml:lang="ms">Hardstyle</skos:prefLabel>
    <skos:prefLabel xml:lang="no">Hardstyle</skos:prefLabel>
    <skos:prefLabel xml:lang="fa">هارداستایل</skos:prefLabel>
    <skos:prefLabel xml:lang="pl">Hardstyle</skos:prefLabel>
    <skos:prefLabel xml:lang="pt">Hardstyle</skos:prefLabel>
    <skos:prefLabel xml:lang="ro">Hardstyle</skos:prefLabel>
    <skos:prefLabel xml:lang="ru">Хардстайл</skos:prefLabel>
    <skos:prefLabel xml:lang="sk">Hardstyle</skos:prefLabel>
    <skos:prefLabel xml:lang="es">Hardstyle</skos:prefLabel>
    <skos:prefLabel xml:lang="sv">Hardstyle</skos:prefLabel>
    <skos:closeMatch rdf:resource="http://rdf.freebase.com/ns/m.02zs97"/>
    <skos:broader rdf:resource="http://data.europeana.eu/concept/music/genre/Techno_fusions"/>
    <skos:definition xml:lang="en">Hardstyle is an electronic dance genre mixing influences from
      hardtechno, hard house, hard trance, and hardcore. Hardstyle typically consists of a deep,
      hard-sounding kick drum, intense faded or reversed basslines accompanying the beat, a synth
      playing a melody, and detuned and distorted sounds. It bears some similarities to hard trance.
      Many hardcore artists produce hardstyle tracks as well, and many newer Hardstyle tracks are
      written in compound time.</skos:definition>
    <skos:exactMatch xml:lang="en">http://dbpedia.org/resource/Hardstyle</skos:exactMatch>
    <skos:inScheme rdf:resource="http://data.europeana.eu/concept/music/genre/Music_Genre_Scheme"/>
    <skos:altLabel xml:lang="en">Hardstyle</skos:altLabel>
  </skos:Concept>

  <skos:Concept rdf:about="http://data.europeana.eu/concept/music/genre/Bouncy_techno">
    <skos:prefLabel xml:lang="en">Bouncy techno</skos:prefLabel>
    <skos:prefLabel xml:lang="cs">Happy Gabber</skos:prefLabel>
    <skos:prefLabel xml:lang="fr">Happy gabber</skos:prefLabel>
    <skos:prefLabel xml:lang="sk">Happy gabber</skos:prefLabel>
    <skos:closeMatch rdf:resource="http://rdf.freebase.com/ns/m.033ln8"/>
    <skos:broader rdf:resource="http://data.europeana.eu/concept/music/genre/Techno_fusions"/>
    <skos:definition xml:lang="en">Bouncy techno is a hardcore dance music rave style that developed
      in the early 1990s from Scotland and North England. Described as an accessible gabber-like
      form, it was popularised by Scott Brown under numerous aliases. The sound became prominent in
      the northern United Kingdom rave scene before it broke into the hardcore homeland of the
      Netherlands through Paul Elstak, where it became known there as happy hardcore and funcore.
      &lt;p&gt; A subsequent mainstream-aimed Eurodance tangent appeared in Germany and itself back
      into the Netherlands. The music of Brown also changed the Southern England happy breakbeat
      style away from its breakbeat foundation and into a bouncy derivative. These different country
      entrails created a single pan European hardcore briefly in the mid-1990s. Bouncy techno
      rapidly declined from this point for a variety of reasons.</skos:definition>
    <skos:exactMatch xml:lang="en">http://dbpedia.org/resource/Bouncy_techno</skos:exactMatch>
    <skos:inScheme rdf:resource="http://data.europeana.eu/concept/music/genre/Music_Genre_Scheme"/>
    <skos:altLabel xml:lang="en">Bouncy techno</skos:altLabel>
  </skos:Concept>

  <skos:Concept rdf:about="http://data.europeana.eu/concept/music/genre/Noise_pop">
    <skos:prefLabel xml:lang="en">Noise pop</skos:prefLabel>
    <skos:prefLabel xml:lang="nl">Noisepop</skos:prefLabel>
    <skos:prefLabel xml:lang="fr">Noise pop</skos:prefLabel>
    <skos:prefLabel xml:lang="it">Noise pop</skos:prefLabel>
    <skos:prefLabel xml:lang="ja">ノイズポップ</skos:prefLabel>
    <skos:prefLabel xml:lang="no">Støypop</skos:prefLabel>
    <skos:prefLabel xml:lang="pl">Noise pop</skos:prefLabel>
    <skos:prefLabel xml:lang="ru">Нойз-поп</skos:prefLabel>
    <skos:prefLabel xml:lang="es">Noise pop</skos:prefLabel>
    <skos:closeMatch rdf:resource="http://rdf.freebase.com/ns/m.034487"/>
    <skos:broader
      rdf:resource="http://data.europeana.eu/concept/music/genre/Alternative_rock_fusions"/>
    <skos:definition xml:lang="en">Noise pop is a subgenre of alternative rock developed in the
      mid-1980s in the UK and US that mixes dissonant noise or feedback, or both, with the melodic
      instrumentation and production elements more often found in pop music, making it more melodic
      than noise rock.</skos:definition>
    <skos:exactMatch xml:lang="en">http://dbpedia.org/resource/Noise_pop</skos:exactMatch>
    <skos:inScheme rdf:resource="http://data.europeana.eu/concept/music/genre/Music_Genre_Scheme"/>
    <skos:altLabel xml:lang="en">Noise pop</skos:altLabel>
  </skos:Concept>

  <skos:Concept rdf:about="http://data.europeana.eu/concept/music/genre/Eurodance">
    <skos:prefLabel xml:lang="en">Eurodance</skos:prefLabel>
    <skos:prefLabel xml:lang="ar">يورودانس</skos:prefLabel>
    <skos:prefLabel xml:lang="bg">Евроденс</skos:prefLabel>
    <skos:prefLabel xml:lang="ca">Eurodance</skos:prefLabel>
    <skos:prefLabel xml:lang="hr">Eurodance</skos:prefLabel>
    <skos:prefLabel xml:lang="cs">Eurodance</skos:prefLabel>
    <skos:prefLabel xml:lang="da">Eurodance</skos:prefLabel>
    <skos:prefLabel xml:lang="nl">Eurodance</skos:prefLabel>
    <skos:prefLabel xml:lang="fi">Eurodance</skos:prefLabel>
    <skos:prefLabel xml:lang="fr">Eurodance</skos:prefLabel>
    <skos:prefLabel xml:lang="de">Eurodance</skos:prefLabel>
    <skos:prefLabel xml:lang="hu">Eurodance</skos:prefLabel>
    <skos:prefLabel xml:lang="id">Eurodance</skos:prefLabel>
    <skos:prefLabel xml:lang="it">Eurodance</skos:prefLabel>
    <skos:prefLabel xml:lang="ja">ユーロダンス</skos:prefLabel>
    <skos:prefLabel xml:lang="ko">유로댄스</skos:prefLabel>
    <skos:prefLabel xml:lang="lv">Eirodeju mūzika</skos:prefLabel>
    <skos:prefLabel xml:lang="lt">Eurodance</skos:prefLabel>
    <skos:prefLabel xml:lang="no">Eurodance</skos:prefLabel>
    <skos:prefLabel xml:lang="fa">یورودنس</skos:prefLabel>
    <skos:prefLabel xml:lang="pl">Eurodance</skos:prefLabel>
    <skos:prefLabel xml:lang="pt">Eurodance</skos:prefLabel>
    <skos:prefLabel xml:lang="ro">Eurodance</skos:prefLabel>
    <skos:prefLabel xml:lang="ru">Евродэнс</skos:prefLabel>
    <skos:prefLabel xml:lang="sk">Eurodance</skos:prefLabel>
    <skos:prefLabel xml:lang="es">Eurodance</skos:prefLabel>
    <skos:prefLabel xml:lang="sv">Eurodance</skos:prefLabel>
    <skos:prefLabel xml:lang="th">ยูโรแดนซ์</skos:prefLabel>
    <skos:prefLabel xml:lang="tr">Eurodans</skos:prefLabel>
    <skos:prefLabel xml:lang="uk">Євроденс</skos:prefLabel>
    <skos:closeMatch rdf:resource="http://rdf.freebase.com/ns/m.035wcs"/>
    <skos:broader
      rdf:resource="http://data.europeana.eu/concept/music/genre/Electronic_music_fusions"/>
    <skos:definition xml:lang="en">Eurodance is a genre of electronic dance music that originated in
      the late 1980s primarily in Europe. It combines many elements of house, techno, hi-NRG and
      Euro disco. Eurodance production continues to evolve with a more modernized style that
      incorporates more elements from trance music. &lt;p&gt; This genre of music is heavily
      influenced by the use of rich melodic vocals, either exclusively by itself or inclusively with
      rapped verses. This, combined with cutting-edge synthesizer, strong bass rhythm and melodic
      hooks, establishes the core foundation of Eurodance music. &lt;p&gt; It peaked at Ibiza's
      summer festivals of 1994 in Spain and its intense popularity then spread around the world,
      which carried on into late 1997.</skos:definition>
    <skos:exactMatch xml:lang="en">http://dbpedia.org/resource/Eurodance</skos:exactMatch>
    <skos:inScheme rdf:resource="http://data.europeana.eu/concept/music/genre/Music_Genre_Scheme"/>
    <skos:altLabel xml:lang="en">Eurodance</skos:altLabel>
  </skos:Concept>

  <skos:Concept rdf:about="http://data.europeana.eu/concept/music/genre/Gangsta_rap">
    <skos:prefLabel xml:lang="en">Gangsta rap</skos:prefLabel>
    <skos:prefLabel xml:lang="ar">غانغستا راب</skos:prefLabel>
    <skos:prefLabel xml:lang="bg">Гангста рап</skos:prefLabel>
    <skos:prefLabel xml:lang="ca">Gangsta rap</skos:prefLabel>
    <skos:prefLabel xml:lang="cs">Gangsta rap</skos:prefLabel>
    <skos:prefLabel xml:lang="nl">Gangstarap</skos:prefLabel>
    <skos:prefLabel xml:lang="fi">Gangsta rap</skos:prefLabel>
    <skos:prefLabel xml:lang="fr">Gangsta rap</skos:prefLabel>
    <skos:prefLabel xml:lang="de">Gangsta-Rap</skos:prefLabel>
    <skos:prefLabel xml:lang="it">Gangsta rap</skos:prefLabel>
    <skos:prefLabel xml:lang="ja">ギャングスタ・ラップ</skos:prefLabel>
    <skos:prefLabel xml:lang="ko">갱스터 랩</skos:prefLabel>
    <skos:prefLabel xml:lang="lv">Gangsta reps</skos:prefLabel>
    <skos:prefLabel xml:lang="no">Gangster rap</skos:prefLabel>
    <skos:prefLabel xml:lang="fa">گنگستا رپ</skos:prefLabel>
    <skos:prefLabel xml:lang="pl">Gangsta rap</skos:prefLabel>
    <skos:prefLabel xml:lang="pt">Gangsta rap</skos:prefLabel>
    <skos:prefLabel xml:lang="ru">Гангста-рэп</skos:prefLabel>
    <skos:prefLabel xml:lang="sk">Gangsta rap</skos:prefLabel>
    <skos:prefLabel xml:lang="es">Gangsta rap</skos:prefLabel>
    <skos:prefLabel xml:lang="sv">Gangstarap</skos:prefLabel>
    <skos:prefLabel xml:lang="tr">Gangsta rap</skos:prefLabel>
    <skos:prefLabel xml:lang="uk">Гангста-реп</skos:prefLabel>
    <skos:closeMatch rdf:resource="http://rdf.freebase.com/ns/m.036jv"/>
    <skos:broader rdf:resource="http://data.europeana.eu/concept/music/genre/Hip_hop_music_fusions"/>
    <skos:definition xml:lang="en">Gangsta rap is a subgenre of hip hop music that evolved from
      hardcore hip hop. The genre was pioneered in the mid-1980s by rappers such as Schoolly D and
      Ice-T, and was popularized in the later part of the 1980s by groups like N.W.A. After the
      national attention that Ice-T and N.W.A attracted in the late 1980s and early 1990s, gangsta
      rap became the most commercially lucrative subgenre of hip hop. Some gangsta rappers have been
      associated, or allegedly have ties with the Bloods or Crips gangs. &lt;p&gt; The subject
      matter inherent in gangsta rap has caused a great deal of controversy. Criticism has come from
      both left wing and right wing commentators, as well as religious leaders, who have accused the
      genre of promoting crime, serial killing, violence, profanity, sex addiction, homophobia,
      racism, promiscuity, misogyny, rape, street gangs, drive-by shootings, vandalism, thievery,
      drug dealing, alcohol abuse, substance abuse, disregarding law enforcement, materialism, and
      narcissism. The White House administrations of both George H. W. Bush and Bill Clinton
      criticized the genre.</skos:definition>
    <skos:exactMatch xml:lang="en">http://dbpedia.org/resource/Gangsta_rap</skos:exactMatch>
    <skos:inScheme rdf:resource="http://data.europeana.eu/concept/music/genre/Music_Genre_Scheme"/>
    <skos:altLabel xml:lang="en">Gangsta rap</skos:altLabel>
  </skos:Concept>

  <skos:Concept rdf:about="http://data.europeana.eu/concept/music/genre/Smooth_jazz">
    <skos:prefLabel xml:lang="en">Smooth jazz</skos:prefLabel>
    <skos:prefLabel xml:lang="da">Smooth jazz</skos:prefLabel>
    <skos:prefLabel xml:lang="nl">Smooth jazz</skos:prefLabel>
    <skos:prefLabel xml:lang="fi">Smooth jazz</skos:prefLabel>
    <skos:prefLabel xml:lang="fr">Smooth jazz</skos:prefLabel>
    <skos:prefLabel xml:lang="de">Smooth Jazz</skos:prefLabel>
    <skos:prefLabel xml:lang="hu">Smooth jazz</skos:prefLabel>
    <skos:prefLabel xml:lang="id">Smooth jazz</skos:prefLabel>
    <skos:prefLabel xml:lang="it">Smooth jazz</skos:prefLabel>
    <skos:prefLabel xml:lang="ja">スムーズジャズ</skos:prefLabel>
    <skos:prefLabel xml:lang="ko">스무스 재즈</skos:prefLabel>
    <skos:prefLabel xml:lang="fa">جاز نرم</skos:prefLabel>
    <skos:prefLabel xml:lang="pl">Smooth jazz</skos:prefLabel>
    <skos:prefLabel xml:lang="pt">Smooth jazz</skos:prefLabel>
    <skos:prefLabel xml:lang="ru">Смут-джаз</skos:prefLabel>
    <skos:prefLabel xml:lang="es">Smooth jazz</skos:prefLabel>
    <skos:prefLabel xml:lang="sv">Smooth jazz</skos:prefLabel>
    <skos:prefLabel xml:lang="th">สมูธแจ๊ส</skos:prefLabel>
    <skos:prefLabel xml:lang="tr">Caz pop</skos:prefLabel>
    <skos:prefLabel xml:lang="uk">Smooth jazz</skos:prefLabel>
    <skos:closeMatch rdf:resource="http://rdf.freebase.com/ns/m.037n97"/>
    <skos:broader rdf:resource="http://data.europeana.eu/concept/music/genre/Jazz_fusions"/>
    <skos:definition xml:lang="en">Smooth jazz is a genre of music that grew out of jazz fusion and
      is influenced by jazz, R&amp;B, funk, rock, and pop music styles. It is also the name of a
      radio format. &lt;p&gt; Modern derivatives of the genre include the more-recent New Adult
      Contemporary format of broadcast radio. &quot;Smooth jazz&quot; was once successful as a radio
      format, however, in 2007, the popularity of the format began to slide. Consequently, it was
      abandoned by several high-profile radio stations across the U.S.A., including WQCD in New
      York, WJJZ in Philadelphia, and KKSF in San Francisco. Many industry insiders have speculated
      that the smooth jazz format may die out, particularly with many of industry giant Clear
      Channel Communications' stations dropping the genre. Critics of the company, however, blame
      Clear Channel for the format's decline, citing too much repetition of a sharply-reduced number
      of tracks on Clear Channel-owned stations that alienated many listeners. Despite the format's
      demise on commercial radio, a growing number of non-commercial stations have taken up the
      music.</skos:definition>
    <skos:exactMatch xml:lang="en">http://dbpedia.org/resource/Smooth_jazz</skos:exactMatch>
    <skos:inScheme rdf:resource="http://data.europeana.eu/concept/music/genre/Music_Genre_Scheme"/>
    <skos:altLabel xml:lang="en">Smooth jazz</skos:altLabel>
  </skos:Concept>

  <skos:Concept rdf:about="http://data.europeana.eu/concept/music/genre/Rap_opera">
    <skos:prefLabel xml:lang="en">Rap opera</skos:prefLabel>
    <skos:closeMatch rdf:resource="http://rdf.freebase.com/ns/m.038dx6"/>
    <skos:broader rdf:resource="http://data.europeana.eu/concept/music/genre/Hip_hop_music_fusions"/>
    <skos:definition xml:lang="en">A rap opera or hip hopera is a series of hip hop songs in the
      form of an opera, inspired by the concept of rock opera. Examples of a hip hopera include
      Trapped in the Closet by R. Kelly, A Prince Among Thieves by Prince Paul, Refletchons by
      Fletch, and Deltron 3030. &lt;p&gt; Like its predecessor, rap opera tells a story through
      consecutive pieces of music involving the same character or characters. Rap opera may be a
      purely auditory experience, or it may be associated with a musical, comic book, or other art
      form. It is a relatively young, spontaneous form, performed more by amateurs and non-profit
      groups than by professional emcees. &lt;p&gt; When R&amp;B singer R. Kelly was asked on IFC
      how he defined his Trapped in the Closet series, Kelly stated that he described it as a hip
      hopera or musical opera, and that it was now too long to be called a song. In 2001, MTV
      debuted a telefilm titled Carmen: A Hip Hopera, directed by Robert Townsend and starring
      Beyoncé Knowles and Mekhi Phifer. Volume 10 also released an album called Hip-Hopera in 1994.
      The former is contemporary R&amp;B, not hip hop music.</skos:definition>
    <skos:exactMatch xml:lang="en">http://dbpedia.org/resource/Rap_opera</skos:exactMatch>
    <skos:inScheme rdf:resource="http://data.europeana.eu/concept/music/genre/Music_Genre_Scheme"/>
    <skos:altLabel xml:lang="en">Rap opera</skos:altLabel>
  </skos:Concept>

  <skos:Concept rdf:about="http://data.europeana.eu/concept/music/genre/Dark_ambient">
    <skos:prefLabel xml:lang="en">Dark ambient</skos:prefLabel>
    <skos:prefLabel xml:lang="cs">Dark ambient</skos:prefLabel>
    <skos:prefLabel xml:lang="da">Dark ambient</skos:prefLabel>
    <skos:prefLabel xml:lang="nl">Dark ambient</skos:prefLabel>
    <skos:prefLabel xml:lang="fi">Dark ambient</skos:prefLabel>
    <skos:prefLabel xml:lang="fr">Dark ambient</skos:prefLabel>
    <skos:prefLabel xml:lang="de">Dark Ambient</skos:prefLabel>
    <skos:prefLabel xml:lang="hu">Dark ambient</skos:prefLabel>
    <skos:prefLabel xml:lang="it">Dark ambient</skos:prefLabel>
    <skos:prefLabel xml:lang="ja">ダーク・アンビエント</skos:prefLabel>
    <skos:prefLabel xml:lang="lv">Tumšais ambients</skos:prefLabel>
    <skos:prefLabel xml:lang="lt">Dark ambient</skos:prefLabel>
    <skos:prefLabel xml:lang="fa">دارک امبینت</skos:prefLabel>
    <skos:prefLabel xml:lang="pl">Dark ambient</skos:prefLabel>
    <skos:prefLabel xml:lang="pt">Dark ambient</skos:prefLabel>
    <skos:prefLabel xml:lang="ro">Dark ambient</skos:prefLabel>
    <skos:prefLabel xml:lang="ru">Дарк-эмбиент</skos:prefLabel>
    <skos:prefLabel xml:lang="sk">Dark ambient</skos:prefLabel>
    <skos:prefLabel xml:lang="es">Dark ambient</skos:prefLabel>
    <skos:prefLabel xml:lang="sv">Dark ambient</skos:prefLabel>
    <skos:prefLabel xml:lang="uk">Дарк-ембієнт</skos:prefLabel>
    <skos:closeMatch rdf:resource="http://rdf.freebase.com/ns/m.03bzc7"/>
    <skos:broader
      rdf:resource="http://data.europeana.eu/concept/music/genre/Electronic_music_fusions"/>
    <skos:definition xml:lang="en">Dark ambient is a subgenre of ambient music that features
      foreboding, ominous, or discordant overtones, some of which were heavily inspired by elements
      of industrial music. Dark ambient has its roots in the 1970s, with the introduction of newer,
      smaller, and more affordable effects units, synthesizer and sampling technology. Dark ambient
      is an unusually diverse genre, related to mainstream ambient music as well as noise, yet
      generally free from derivatives and connections to other genres or styles.</skos:definition>
    <skos:exactMatch xml:lang="en">http://dbpedia.org/resource/Dark_ambient</skos:exactMatch>
    <skos:inScheme rdf:resource="http://data.europeana.eu/concept/music/genre/Music_Genre_Scheme"/>
    <skos:altLabel xml:lang="en">Dark ambient</skos:altLabel>
  </skos:Concept>

  <skos:Concept rdf:about="http://data.europeana.eu/concept/music/genre/Post-disco">
    <skos:prefLabel xml:lang="en">Post-disco</skos:prefLabel>
    <skos:prefLabel xml:lang="de">Post-Disco</skos:prefLabel>
    <skos:prefLabel xml:lang="hu">Posztdiszkó</skos:prefLabel>
    <skos:prefLabel xml:lang="ja">ポスト・ディスコ</skos:prefLabel>
    <skos:prefLabel xml:lang="pl">Post-disco</skos:prefLabel>
    <skos:prefLabel xml:lang="ro">Post-disco</skos:prefLabel>
    <skos:prefLabel xml:lang="sk">Post-disco</skos:prefLabel>
    <skos:prefLabel xml:lang="es">Post-disco</skos:prefLabel>
    <skos:prefLabel xml:lang="th">โพสต์ดิสโก้</skos:prefLabel>
    <skos:closeMatch rdf:resource="http://rdf.freebase.com/ns/m.03c34yl"/>
    <skos:broader
      rdf:resource="http://data.europeana.eu/concept/music/genre/Electronic_music_fusions"/>
    <skos:definition xml:lang="en">Post-disco was an era in popular music history. It began in the
      late 1970s with the backlash against disco music in the United States, starting in Chicago,
      Illinois and spreading elsewhere, and ended with the mainstream appearance of house music in
      the late 1980s. Post-disco can also mean a disco movement initially of urban contemporary
      artists that started in the New York City area partially in response to over-commercialization
      and artistic downfall of disco culture. &lt;p&gt; During the late 1970s and early 1980s
      post-disco styles were developed by a mixed community of DJs and producers. Relative to disco
      much of this music displayed an increasingly electronic character and it featured
      &quot;radically different sounds&quot; to the former. The music tended to be
      technology-centric, keyboard-ladden, melodic, with funk-oriented bass lines, synth riffs, dub
      music aesthetics, and background jazzy or blues-y piano layers. Strings and brass section
      synthesizer sounds were preferred to the lush orchestration heard on many disco tracks,
      although such arrangements would later resurface in some house music. Soulful female vocals,
      however, remained an essence of post-disco.</skos:definition>
    <skos:exactMatch xml:lang="en">http://dbpedia.org/resource/Post-disco</skos:exactMatch>
    <skos:inScheme rdf:resource="http://data.europeana.eu/concept/music/genre/Music_Genre_Scheme"/>
    <skos:altLabel xml:lang="en">Post Disco</skos:altLabel>
    <skos:altLabel xml:lang="en">Post-disco</skos:altLabel>
  </skos:Concept>

  <skos:Concept rdf:about="http://data.europeana.eu/concept/music/genre/Eurobeat">
    <skos:prefLabel xml:lang="en">Eurobeat</skos:prefLabel>
    <skos:prefLabel xml:lang="ca">Eurobeat</skos:prefLabel>
    <skos:prefLabel xml:lang="cs">Eurobeat</skos:prefLabel>
    <skos:prefLabel xml:lang="nl">Eurobeat</skos:prefLabel>
    <skos:prefLabel xml:lang="fi">Eurobeat</skos:prefLabel>
    <skos:prefLabel xml:lang="fr">Eurobeat</skos:prefLabel>
    <skos:prefLabel xml:lang="de">Eurobeat</skos:prefLabel>
    <skos:prefLabel xml:lang="el">Eurobeat</skos:prefLabel>
    <skos:prefLabel xml:lang="id">Eurobeat</skos:prefLabel>
    <skos:prefLabel xml:lang="it">Eurobeat</skos:prefLabel>
    <skos:prefLabel xml:lang="ja">ユーロビート</skos:prefLabel>
    <skos:prefLabel xml:lang="ko">유로비트</skos:prefLabel>
    <skos:prefLabel xml:lang="no">Eurobeat</skos:prefLabel>
    <skos:prefLabel xml:lang="pl">Eurobeat</skos:prefLabel>
    <skos:prefLabel xml:lang="pt">Eurobeat</skos:prefLabel>
    <skos:prefLabel xml:lang="ru">Евробит</skos:prefLabel>
    <skos:prefLabel xml:lang="sk">Eurobeat</skos:prefLabel>
    <skos:prefLabel xml:lang="es">Eurobeat</skos:prefLabel>
    <skos:prefLabel xml:lang="sv">Eurobeat</skos:prefLabel>
    <skos:prefLabel xml:lang="th">ยูโรบีต</skos:prefLabel>
    <skos:closeMatch rdf:resource="http://rdf.freebase.com/ns/m.03cnzj"/>
    <skos:broader rdf:resource="http://data.europeana.eu/concept/music/genre/Pop_music_fusions"/>
    <skos:definition xml:lang="en">Eurobeat is either a form of the British dance-pop variant of
      Italo disco or Hi-NRG-driven Italo disco music that both developed in the late 1980s.
      &lt;p&gt; In the United States, Eurobeat was sometimes marketed as Hi-NRG and for a short
      while shared this term with the very early freestyle music hits. Italo disco was often
      referred to as Eurobeat, probably due to the negative connotations of the word
      &quot;disco&quot; in the United States in the 1980s. &lt;p&gt; &quot;Eurobeat&quot; is also
      directly related to the Japanese Para Para dance culture, but in a completely different way,
      explained later in this article.</skos:definition>
    <skos:exactMatch xml:lang="en">http://dbpedia.org/resource/Eurobeat</skos:exactMatch>
    <skos:inScheme rdf:resource="http://data.europeana.eu/concept/music/genre/Music_Genre_Scheme"/>
    <skos:altLabel xml:lang="en">Eurobeat</skos:altLabel>
  </skos:Concept>

  <skos:Concept rdf:about="http://data.europeana.eu/concept/music/genre/Grindcore">
    <skos:prefLabel xml:lang="en">Grindcore</skos:prefLabel>
    <skos:prefLabel xml:lang="bg">Грайндкор</skos:prefLabel>
    <skos:prefLabel xml:lang="hr">Grindcore</skos:prefLabel>
    <skos:prefLabel xml:lang="cs">Grindcore</skos:prefLabel>
    <skos:prefLabel xml:lang="da">Grindcore</skos:prefLabel>
    <skos:prefLabel xml:lang="nl">Grindcore</skos:prefLabel>
    <skos:prefLabel xml:lang="et">Grindcore</skos:prefLabel>
    <skos:prefLabel xml:lang="fi">Grindcore</skos:prefLabel>
    <skos:prefLabel xml:lang="fr">Grindcore</skos:prefLabel>
    <skos:prefLabel xml:lang="de">Grindcore</skos:prefLabel>
    <skos:prefLabel xml:lang="hu">Grindcore</skos:prefLabel>
    <skos:prefLabel xml:lang="id">Grindcore</skos:prefLabel>
    <skos:prefLabel xml:lang="it">Grindcore</skos:prefLabel>
    <skos:prefLabel xml:lang="ja">グラインドコア</skos:prefLabel>
    <skos:prefLabel xml:lang="ko">그라인드코어</skos:prefLabel>
    <skos:prefLabel xml:lang="lt">Grindcore</skos:prefLabel>
    <skos:prefLabel xml:lang="no">Grindcore</skos:prefLabel>
    <skos:prefLabel xml:lang="fa">گریندکور</skos:prefLabel>
    <skos:prefLabel xml:lang="pl">Grindcore</skos:prefLabel>
    <skos:prefLabel xml:lang="pt">Grindcore</skos:prefLabel>
    <skos:prefLabel xml:lang="ro">Grindcore</skos:prefLabel>
    <skos:prefLabel xml:lang="ru">Грайндкор</skos:prefLabel>
    <skos:prefLabel xml:lang="sr">Грајнд кор</skos:prefLabel>
    <skos:prefLabel xml:lang="sk">Grindcore</skos:prefLabel>
    <skos:prefLabel xml:lang="sl">Grindcore</skos:prefLabel>
    <skos:prefLabel xml:lang="es">Grindcore</skos:prefLabel>
    <skos:prefLabel xml:lang="sv">Grindcore</skos:prefLabel>
    <skos:prefLabel xml:lang="tr">Grindcore</skos:prefLabel>
    <skos:prefLabel xml:lang="uk">Грайндкор</skos:prefLabel>
    <skos:closeMatch rdf:resource="http://rdf.freebase.com/ns/m.03fpx"/>
    <skos:broader rdf:resource="http://data.europeana.eu/concept/music/genre/Punk_rock_fusions"/>
    <skos:definition xml:lang="en">Grindcore is an extreme genre of music that originated in the
      early- to mid-1980s. It draws inspiration from some of the most abrasive-sounding music genres
      – including thrash metal, industrial music, noise music and the more extreme varieties of
      hardcore punk, such as crust punk. Grindcore is characterized by a noise-filled sound that
      uses heavily distorted, down-tuned guitars, grinding overdriven bass, high speed tempo, blast
      beats, and vocals which consist of growls and high-pitched shrieks. Early groups like Napalm
      Death are credited with laying the groundwork for the style. It is most prevalent today in
      North America and Europe, with popular contributors such as Brutal Truth and Nasum. Lyrical
      themes range from a primary focus on social and political concerns, to gory subject matter and
      black humor. &lt;p&gt; A trait of grindcore is the &quot;microsong&quot;. Several bands have
      produced songs that are only seconds in length. British band Napalm Death holds the Guinness
      World Record for shortest song ever recorded with the one-second &quot;You Suffer&quot;. Many
      bands record simple phrases that may be rhythmically sprawled out across an instrumental
      lasting only a couple of bars in length.</skos:definition>
    <skos:exactMatch xml:lang="en">http://dbpedia.org/resource/Grindcore</skos:exactMatch>
    <skos:inScheme rdf:resource="http://data.europeana.eu/concept/music/genre/Music_Genre_Scheme"/>
    <skos:altLabel xml:lang="en">Grind</skos:altLabel>
    <skos:altLabel xml:lang="en">Grindcore</skos:altLabel>
  </skos:Concept>

  <skos:Concept rdf:about="http://data.europeana.eu/concept/music/genre/Street_punk">
    <skos:prefLabel xml:lang="en">Street punk</skos:prefLabel>
    <skos:prefLabel xml:lang="bg">Стрийт пънк</skos:prefLabel>
    <skos:prefLabel xml:lang="hr">Streetpunk</skos:prefLabel>
    <skos:prefLabel xml:lang="cs">Street punk</skos:prefLabel>
    <skos:prefLabel xml:lang="nl">Streetpunk</skos:prefLabel>
    <skos:prefLabel xml:lang="fr">Street punk</skos:prefLabel>
    <skos:prefLabel xml:lang="de">Streetpunk</skos:prefLabel>
    <skos:prefLabel xml:lang="it">Street punk</skos:prefLabel>
    <skos:prefLabel xml:lang="pt">Street punk</skos:prefLabel>
    <skos:prefLabel xml:lang="ru">Стрит-панк</skos:prefLabel>
    <skos:prefLabel xml:lang="es">Street punk</skos:prefLabel>
    <skos:prefLabel xml:lang="sv">Streetpunk</skos:prefLabel>
    <skos:closeMatch rdf:resource="http://rdf.freebase.com/ns/m.03gq340"/>
    <skos:broader rdf:resource="http://data.europeana.eu/concept/music/genre/Punk_rock_fusions"/>
    <skos:definition xml:lang="en">Street punk is a working class-based genre of punk rock which
      took shape in the early 1980s, partly as a rebellion against the perceived artistic
      pretensions of the first wave of British punk. Street punk emerged from the Oi! style,
      performed by bands such as Sham 69, Angelic Upstarts, Cockney Rejects, The Exploited, and Cock
      Sparrer. However, street punk continued beyond the confines of the original Oi! form. Street
      punks generally have a much more outlandish appearance than the working class or skinhead
      image cultivated by many Oi! groups. Street punks often have multi-coloured hair, mohawks,
      spike-encrusted leather vests, and clothing with political slogans or the names of punk
      bands.</skos:definition>
    <skos:exactMatch xml:lang="en">http://dbpedia.org/resource/Street_punk</skos:exactMatch>
    <skos:inScheme rdf:resource="http://data.europeana.eu/concept/music/genre/Music_Genre_Scheme"/>
    <skos:altLabel xml:lang="en">Street punk</skos:altLabel>
  </skos:Concept>

  <skos:Concept rdf:about="http://data.europeana.eu/concept/music/genre/Sambass">
    <skos:prefLabel xml:lang="en">Sambass</skos:prefLabel>
    <skos:prefLabel xml:lang="fr">Sambass</skos:prefLabel>
    <skos:prefLabel xml:lang="fa">سامباس</skos:prefLabel>
    <skos:prefLabel xml:lang="pl">Sambass</skos:prefLabel>
    <skos:prefLabel xml:lang="pt">Drum and bossa</skos:prefLabel>
    <skos:prefLabel xml:lang="sk">Sambass</skos:prefLabel>
    <skos:prefLabel xml:lang="es">Sambass</skos:prefLabel>
    <skos:closeMatch rdf:resource="http://rdf.freebase.com/ns/m.03m8f7_"/>
    <skos:broader
      rdf:resource="http://data.europeana.eu/concept/music/genre/Electronic_music_fusions"/>
    <skos:definition xml:lang="en">Sambass, drum 'n' bossa or drum 'n' sambass is a regional
      sub-genre of drum and bass music mostly native to Brazil, which combines drum and bass rhythms
      with influences from Latin American music. &lt;p&gt; Popular artists in the genre include DJ
      Marky, DJ Patife, XRS Land, Drumagick, Bungle, Marcelinho da Lua, Kaleidoscopio and DJ Roots,
      and four compilation albums titles &quot;Sambass Vol. 1&quot; through &quot;Sambass Vol.
      4&quot; were released to international acclaim by the Italian record label
      Cuadra.</skos:definition>
    <skos:exactMatch xml:lang="en">http://dbpedia.org/resource/Sambass</skos:exactMatch>
    <skos:inScheme rdf:resource="http://data.europeana.eu/concept/music/genre/Music_Genre_Scheme"/>
    <skos:altLabel xml:lang="en">Sambass</skos:altLabel>
  </skos:Concept>

  <skos:Concept rdf:about="http://data.europeana.eu/concept/music/genre/House_music">
    <skos:prefLabel xml:lang="en">House music</skos:prefLabel>
    <skos:prefLabel xml:lang="ar">هاوس</skos:prefLabel>
    <skos:prefLabel xml:lang="bg">Хаус</skos:prefLabel>
    <skos:prefLabel xml:lang="ca">House (música)</skos:prefLabel>
    <skos:prefLabel xml:lang="hr">House glazba</skos:prefLabel>
    <skos:prefLabel xml:lang="cs">House Music</skos:prefLabel>
    <skos:prefLabel xml:lang="da">House</skos:prefLabel>
    <skos:prefLabel xml:lang="nl">House (muziekstijl)</skos:prefLabel>
    <skos:prefLabel xml:lang="et">House</skos:prefLabel>
    <skos:prefLabel xml:lang="fi">House</skos:prefLabel>
    <skos:prefLabel xml:lang="fr">House music</skos:prefLabel>
    <skos:prefLabel xml:lang="de">House</skos:prefLabel>
    <skos:prefLabel xml:lang="hu">House</skos:prefLabel>
    <skos:prefLabel xml:lang="id">Musik house</skos:prefLabel>
    <skos:prefLabel xml:lang="it">Musica house</skos:prefLabel>
    <skos:prefLabel xml:lang="ja">ハウス</skos:prefLabel>
    <skos:prefLabel xml:lang="ko">하우스</skos:prefLabel>
    <skos:prefLabel xml:lang="lv">Hausmūzika</skos:prefLabel>
    <skos:prefLabel xml:lang="lt">House</skos:prefLabel>
    <skos:prefLabel xml:lang="no">House</skos:prefLabel>
    <skos:prefLabel xml:lang="fa">موسیقی هاوس</skos:prefLabel>
    <skos:prefLabel xml:lang="pl">House</skos:prefLabel>
    <skos:prefLabel xml:lang="pt">House</skos:prefLabel>
    <skos:prefLabel xml:lang="ro">Muzică House</skos:prefLabel>
    <skos:prefLabel xml:lang="ru">Хаус</skos:prefLabel>
    <skos:prefLabel xml:lang="sr">Хаус музика</skos:prefLabel>
    <skos:prefLabel xml:lang="sk">House</skos:prefLabel>
    <skos:prefLabel xml:lang="sl">House</skos:prefLabel>
    <skos:prefLabel xml:lang="es">House</skos:prefLabel>
    <skos:prefLabel xml:lang="sv">House</skos:prefLabel>
    <skos:prefLabel xml:lang="th">เฮาส์</skos:prefLabel>
    <skos:prefLabel xml:lang="tr">House müzik</skos:prefLabel>
    <skos:prefLabel xml:lang="uk">Хауз</skos:prefLabel>
    <skos:closeMatch rdf:resource="http://rdf.freebase.com/ns/m.03mb9"/>
    <skos:broader
      rdf:resource="http://data.europeana.eu/concept/music/genre/Electronic_music_fusions"/>
    <skos:definition xml:lang="en">House music is a genre of electronic dance music that originated
      in Chicago in the early 1980s. It was initially popularized circa 1984 in Chicago, but
      beginning in 1985, it fanned out to other major cities across North and South America, as well
      as Europe and later Australia. Early house music commercial success in Europe saw songs such
      as &quot;Pump Up The Volume&quot; by MARRS, &quot;House Nation&quot; by House Master Boyz and
      the Rude Boy of House, &quot;Theme from S'Express&quot; by S'Express and &quot;Doctorin' the
      House&quot; by Coldcut in the pop charts. Since the early to mid-1990s, house music has been
      infused in mainstream pop and dance music worldwide. &lt;p&gt; Early house music was generally
      dance-based music characterized by repetitive 4/4 beats, rhythms mainly provided by drum
      machines, off-beat hi-hat cymbals, and synthesized basslines. While house displayed several
      characteristics similar to disco music, it was more electronic and minimalistic, and the
      repetitive rhythm of house was more important than the song itself.</skos:definition>
    <skos:exactMatch xml:lang="en">http://dbpedia.org/resource/House_music</skos:exactMatch>
    <skos:inScheme rdf:resource="http://data.europeana.eu/concept/music/genre/Music_Genre_Scheme"/>
    <skos:altLabel xml:lang="en">House</skos:altLabel>
    <skos:altLabel xml:lang="en">House music</skos:altLabel>
  </skos:Concept>

  <skos:Concept rdf:about="http://data.europeana.eu/concept/music/genre/Swamp_pop">
    <skos:prefLabel xml:lang="en">Swamp pop</skos:prefLabel>
    <skos:prefLabel xml:lang="fr">Swamp pop</skos:prefLabel>
    <skos:prefLabel xml:lang="de">Swamp Rock</skos:prefLabel>
    <skos:prefLabel xml:lang="it">Swamp rock</skos:prefLabel>
    <skos:prefLabel xml:lang="no">Swamp rock</skos:prefLabel>
    <skos:prefLabel xml:lang="pt">Swamp rock</skos:prefLabel>
    <skos:prefLabel xml:lang="ro">Swamp rock</skos:prefLabel>
    <skos:prefLabel xml:lang="es">Swamp rock</skos:prefLabel>
    <skos:prefLabel xml:lang="sv">Swamp rock</skos:prefLabel>
    <skos:closeMatch rdf:resource="http://rdf.freebase.com/ns/m.03n15_"/>
    <skos:broader rdf:resource="http://data.europeana.eu/concept/music/genre/Pop_music_fusions"/>
    <skos:definition xml:lang="en">Swamp pop is a musical genre indigenous to the Acadiana region of
      south Louisiana and an adjoining section of southeast Texas. Created in the 1950s and early
      1960s by teenaged Cajuns and black Creoles, it combines New Orleans-style rhythm and blues,
      country and western, and traditional French Louisiana musical influences. Although a fairly
      obscure genre, swamp pop maintains a large audience in its south Louisiana and southeast Texas
      homeland, and it has acquired a small but passionate cult following in the United Kingdom,
      northern Europe, and Japan.</skos:definition>
    <skos:exactMatch xml:lang="en">http://dbpedia.org/resource/Swamp_pop</skos:exactMatch>
    <skos:inScheme rdf:resource="http://data.europeana.eu/concept/music/genre/Music_Genre_Scheme"/>
    <skos:altLabel xml:lang="en">Swamp pop</skos:altLabel>
  </skos:Concept>

  <skos:Concept rdf:about="http://data.europeana.eu/concept/music/genre/Chutney_music">
    <skos:prefLabel xml:lang="en">Chutney music</skos:prefLabel>
    <skos:prefLabel xml:lang="ca">Música chutney</skos:prefLabel>
    <skos:prefLabel xml:lang="de">Chutney</skos:prefLabel>
    <skos:prefLabel xml:lang="hi">चटनी संगीत</skos:prefLabel>
    <skos:prefLabel xml:lang="pt">Música chutney</skos:prefLabel>
    <skos:closeMatch rdf:resource="http://rdf.freebase.com/ns/m.03qtv7"/>
    <skos:broader
      rdf:resource="http://data.europeana.eu/concept/music/genre/Latin_American_music_fusions"/>
    <skos:definition xml:lang="en">Chutney music is a form indigenous to the southern Caribbean,
      popular in Guyana, Trinidad and Suriname.</skos:definition>
    <skos:exactMatch xml:lang="en">http://dbpedia.org/resource/Chutney_music</skos:exactMatch>
    <skos:inScheme rdf:resource="http://data.europeana.eu/concept/music/genre/Music_Genre_Scheme"/>
    <skos:altLabel xml:lang="en">Chutney music</skos:altLabel>
  </skos:Concept>

  <skos:Concept rdf:about="http://data.europeana.eu/concept/music/genre/Folktronica">
    <skos:prefLabel xml:lang="en">Folktronica</skos:prefLabel>
    <skos:prefLabel xml:lang="nl">Folktronica</skos:prefLabel>
    <skos:prefLabel xml:lang="de">Folktronica</skos:prefLabel>
    <skos:prefLabel xml:lang="it">Folktronica</skos:prefLabel>
    <skos:prefLabel xml:lang="ja">フォークトロニカ</skos:prefLabel>
    <skos:prefLabel xml:lang="pl">Folktronica</skos:prefLabel>
    <skos:prefLabel xml:lang="pt">Folktronica</skos:prefLabel>
    <skos:prefLabel xml:lang="sk">Folktronica</skos:prefLabel>
    <skos:prefLabel xml:lang="es">Folktrónica</skos:prefLabel>
    <skos:prefLabel xml:lang="sv">Folktronica</skos:prefLabel>
    <skos:closeMatch rdf:resource="http://rdf.freebase.com/ns/m.03rlps"/>
    <skos:broader
      rdf:resource="http://data.europeana.eu/concept/music/genre/Electronic_music_fusions"/>
    <skos:definition xml:lang="en">Folktronica or electrofolk is a genre of music comprising various
      elements of folk music and electronica, often featuring samplings of acoustic
      instruments—especially stringed instruments—and incorporating hip hop or dance rhythms.
      Typically, computers are used during the recording process.</skos:definition>
    <skos:exactMatch xml:lang="en">http://dbpedia.org/resource/Folktronica</skos:exactMatch>
    <skos:inScheme rdf:resource="http://data.europeana.eu/concept/music/genre/Music_Genre_Scheme"/>
    <skos:altLabel xml:lang="en">Folktronica</skos:altLabel>
  </skos:Concept>

  <skos:Concept rdf:about="http://data.europeana.eu/concept/music/genre/Techno-folk">
    <skos:prefLabel xml:lang="en">Folktronica</skos:prefLabel>
    <skos:closeMatch rdf:resource="http://rdf.freebase.com/ns/m.03rlps"/>
    <skos:broader rdf:resource="http://data.europeana.eu/concept/music/genre/Folk_music_fusions"/>
    <skos:definition xml:lang="en">Folktronica or electrofolk is a genre of music comprising various
      elements of folk music and electronica, often featuring samplings of acoustic
      instruments—especially stringed instruments—and incorporating hip hop or dance rhythms.
      Typically, computers are used during the recording process.</skos:definition>
    <skos:exactMatch xml:lang="en">http://dbpedia.org/resource/Techno-folk</skos:exactMatch>
    <skos:inScheme rdf:resource="http://data.europeana.eu/concept/music/genre/Music_Genre_Scheme"/>
  </skos:Concept>

  <skos:Concept rdf:about="http://data.europeana.eu/concept/music/genre/Celtic_metal">
    <skos:prefLabel xml:lang="en">Celtic metal</skos:prefLabel>
    <skos:prefLabel xml:lang="cs">Celtic metal</skos:prefLabel>
    <skos:prefLabel xml:lang="fr">Metal celtique</skos:prefLabel>
    <skos:prefLabel xml:lang="it">Celtic metal</skos:prefLabel>
    <skos:prefLabel xml:lang="ru">Келтик-метал</skos:prefLabel>
    <skos:closeMatch rdf:resource="http://rdf.freebase.com/ns/m.03x_cnr"/>
    <skos:broader
      rdf:resource="http://data.europeana.eu/concept/music/genre/Heavy_metal_music_fusions"/>
    <skos:definition xml:lang="en">Celtic metal is a subgenre of folk metal that developed in the
      1990s in Ireland. As the name suggests, the genre is a fusion of heavy metal and Celtic music.
      The early pioneers of the genre were the Irish bands Cruachan, Primordial and Waylander. The
      genre has since expanded beyond Irish shores and is known to be performed today by bands from
      numerous other countries.</skos:definition>
    <skos:exactMatch xml:lang="en">http://dbpedia.org/resource/Celtic_metal</skos:exactMatch>
    <skos:inScheme rdf:resource="http://data.europeana.eu/concept/music/genre/Music_Genre_Scheme"/>
    <skos:altLabel xml:lang="en">Celtic metal</skos:altLabel>
  </skos:Concept>

  <skos:Concept rdf:about="http://data.europeana.eu/concept/music/genre/Indie_pop">
    <skos:prefLabel xml:lang="en">Indie pop</skos:prefLabel>
    <skos:prefLabel xml:lang="ca">Indie pop</skos:prefLabel>
    <skos:prefLabel xml:lang="hr">Indie pop</skos:prefLabel>
    <skos:prefLabel xml:lang="cs">Indie pop</skos:prefLabel>
    <skos:prefLabel xml:lang="fi">Indie pop</skos:prefLabel>
    <skos:prefLabel xml:lang="fr">Indie pop</skos:prefLabel>
    <skos:prefLabel xml:lang="de">Independent</skos:prefLabel>
    <skos:prefLabel xml:lang="id">Indie pop</skos:prefLabel>
    <skos:prefLabel xml:lang="it">Indie pop</skos:prefLabel>
    <skos:prefLabel xml:lang="ja">ギターポップ</skos:prefLabel>
    <skos:prefLabel xml:lang="ko">인디 팝</skos:prefLabel>
    <skos:prefLabel xml:lang="lt">Indie popsas</skos:prefLabel>
    <skos:prefLabel xml:lang="ms">Pop indie</skos:prefLabel>
    <skos:prefLabel xml:lang="pl">Indie pop</skos:prefLabel>
    <skos:prefLabel xml:lang="pt">Indie pop</skos:prefLabel>
    <skos:prefLabel xml:lang="ru">Инди-поп</skos:prefLabel>
    <skos:prefLabel xml:lang="sr">Инди поп</skos:prefLabel>
    <skos:prefLabel xml:lang="sk">Indie pop</skos:prefLabel>
    <skos:prefLabel xml:lang="es">Indie pop</skos:prefLabel>
    <skos:prefLabel xml:lang="sv">Indiepop</skos:prefLabel>
    <skos:prefLabel xml:lang="th">อินดี้ป็อป</skos:prefLabel>
    <skos:prefLabel xml:lang="uk">Інді-поп</skos:prefLabel>
    <skos:closeMatch rdf:resource="http://rdf.freebase.com/ns/m.03xnwz"/>
    <skos:broader
      rdf:resource="http://data.europeana.eu/concept/music/genre/Alternative_rock_fusions"/>
    <skos:definition xml:lang="en">Indie pop is a genre of alternative rock music that originated in
      the United Kingdom in the mid-1980s, with its roots in Scottish post-punk bands on the
      Postcard Records label in the early 1980s and the dominant UK independent band of the
      mid-1980s, the Smiths. Indie pop was inspired by punk's DIY ethic and related ideologies, and
      it generated a thriving fanzine, label, and club and gig circuit. Indie pop differs from indie
      rock to the extent that it is more melodic, less abrasive, and relatively angst-free.
      &lt;p&gt; The term &quot;indie&quot; had been used for some time to describe artists on
      independent labels, but the key moment in the naming of &quot;indie pop&quot; as a genre was
      the release of NME's C86 tape in 1986. The compilation featured, among other artists, Primal
      Scream, the Pastels, and the Wedding Present, and &quot;indie&quot; quickly became shorthand
      for a genre whose defining conventions were identified as jangling guitars, a love of '60s
      pop, and melodic power pop song structures.</skos:definition>
    <skos:exactMatch xml:lang="en">http://dbpedia.org/resource/Indie_pop</skos:exactMatch>
    <skos:inScheme rdf:resource="http://data.europeana.eu/concept/music/genre/Music_Genre_Scheme"/>
    <skos:altLabel xml:lang="en">Indie pop</skos:altLabel>
  </skos:Concept>

  <skos:Concept rdf:about="http://data.europeana.eu/concept/music/genre/Punk_jazz">
    <skos:prefLabel xml:lang="en">Punk jazz</skos:prefLabel>
    <skos:prefLabel xml:lang="fr">Jazz punk</skos:prefLabel>
    <skos:prefLabel xml:lang="it">Punk jazz</skos:prefLabel>
    <skos:prefLabel xml:lang="pt">Punk jazz</skos:prefLabel>
    <skos:prefLabel xml:lang="ru">Панк-джаз</skos:prefLabel>
    <skos:closeMatch rdf:resource="http://rdf.freebase.com/ns/m.0411nml"/>
    <skos:broader rdf:resource="http://data.europeana.eu/concept/music/genre/Jazz_fusions"/>
    <skos:definition xml:lang="en">Punk jazz describes the amalgamation of elements of the jazz
      tradition with the instrumentation or conceptual heritage of punk rock. John Zorn's band Naked
      City, James Chance and the Contortions, Lounge Lizards, Universal Congress Of, Laughing Clowns
      and Zymosis are notable examples of punk jazz artists.</skos:definition>
    <skos:exactMatch xml:lang="en">http://dbpedia.org/resource/Punk_jazz</skos:exactMatch>
    <skos:inScheme rdf:resource="http://data.europeana.eu/concept/music/genre/Music_Genre_Scheme"/>
    <skos:altLabel xml:lang="en">Punk jazz</skos:altLabel>
  </skos:Concept>

  <skos:Concept rdf:about="http://data.europeana.eu/concept/music/genre/Industrial_hip_hop">
    <skos:prefLabel xml:lang="en">Industrial hip hop</skos:prefLabel>
    <skos:prefLabel xml:lang="nl">Industrial rap</skos:prefLabel>
    <skos:prefLabel xml:lang="it">Industrial hip hop</skos:prefLabel>
    <skos:prefLabel xml:lang="ru">Индустриальный хип-хоп</skos:prefLabel>
    <skos:prefLabel xml:lang="th">อินดัสเทรียลฮิปฮอป</skos:prefLabel>
    <skos:closeMatch rdf:resource="http://rdf.freebase.com/ns/m.0414y1g"/>
    <skos:broader rdf:resource="http://data.europeana.eu/concept/music/genre/Hip_hop_music_fusions"/>
    <skos:definition xml:lang="en">Industrial hip hop is a fusion of industrial music with the
      rhythms or vocals of hip hop music.</skos:definition>
    <skos:exactMatch xml:lang="en">http://dbpedia.org/resource/Industrial_hip_hop</skos:exactMatch>
    <skos:inScheme rdf:resource="http://data.europeana.eu/concept/music/genre/Music_Genre_Scheme"/>
    <skos:altLabel xml:lang="en">Industrial hip hop</skos:altLabel>
  </skos:Concept>

  <skos:Concept rdf:about="http://data.europeana.eu/concept/music/genre/D-beat">
    <skos:prefLabel xml:lang="en">D-beat</skos:prefLabel>
    <skos:prefLabel xml:lang="hr">D-beat</skos:prefLabel>
    <skos:prefLabel xml:lang="cs">D-beat</skos:prefLabel>
    <skos:prefLabel xml:lang="da">D-beat</skos:prefLabel>
    <skos:prefLabel xml:lang="nl">D-beat</skos:prefLabel>
    <skos:prefLabel xml:lang="fi">D-beat</skos:prefLabel>
    <skos:prefLabel xml:lang="de">D-Beat</skos:prefLabel>
    <skos:prefLabel xml:lang="it">D-beat</skos:prefLabel>
    <skos:prefLabel xml:lang="ko">D-beat</skos:prefLabel>
    <skos:prefLabel xml:lang="pl">D-Beat</skos:prefLabel>
    <skos:prefLabel xml:lang="pt">D-beat</skos:prefLabel>
    <skos:prefLabel xml:lang="sk">D-beat</skos:prefLabel>
    <skos:prefLabel xml:lang="es">D-beat</skos:prefLabel>
    <skos:prefLabel xml:lang="sv">Kängpunk</skos:prefLabel>
    <skos:closeMatch rdf:resource="http://rdf.freebase.com/ns/m.041613"/>
    <skos:broader rdf:resource="http://data.europeana.eu/concept/music/genre/Punk_rock_fusions"/>
    <skos:definition xml:lang="en">D-beat is a style of hardcore punk, developed in the early 1980s
      by imitators of Discharge, after whom the genre is named, as well as a drum beat
      characteristic of this subgenre. Discharge may have themselves inherited the beat from
      Motörhead. The first such group was The Varukers. D-beat is closely associated with crust
      punk, which is a heavier, more complex variation. The style was particularly popular in
      Sweden, and developed there by groups such as Crude SS, Anti Cimex, Mob 47, Driller Killer,
      and No Security. Other D-beat groups include Doom, from the UK, Disclose, from Japan, Crucifix
      and Final Conflict, from the U.S., Ratos de Porão, from Brazil, and MG15, from Spain. While
      the style initially developed in the early 1980s, a number of new groups working within the
      subgenre emerged in the mid-1990s. These include the Swedish groups Wolfbrigade, Totalitär,
      Avskum, Skitsystem and Disfear.</skos:definition>
    <skos:exactMatch xml:lang="en">http://dbpedia.org/resource/D-beat</skos:exactMatch>
    <skos:inScheme rdf:resource="http://data.europeana.eu/concept/music/genre/Music_Genre_Scheme"/>
    <skos:altLabel xml:lang="en">D-beat</skos:altLabel>
  </skos:Concept>

  <skos:Concept rdf:about="http://data.europeana.eu/concept/music/genre/Italo_house">
    <skos:prefLabel xml:lang="en">Italo house</skos:prefLabel>
    <skos:prefLabel xml:lang="ca">Italo house</skos:prefLabel>
    <skos:prefLabel xml:lang="da">Italo</skos:prefLabel>
    <skos:prefLabel xml:lang="nl">Italo</skos:prefLabel>
    <skos:prefLabel xml:lang="de">Italo-Disco</skos:prefLabel>
    <skos:prefLabel xml:lang="it">Italo house</skos:prefLabel>
    <skos:prefLabel xml:lang="ja">イタロ・ハウス</skos:prefLabel>
    <skos:prefLabel xml:lang="pl">Italo house</skos:prefLabel>
    <skos:prefLabel xml:lang="pt">Italo House</skos:prefLabel>
    <skos:closeMatch rdf:resource="http://rdf.freebase.com/ns/m.0416x0"/>
    <skos:broader rdf:resource="http://data.europeana.eu/concept/music/genre/House_music_fusions"/>
    <skos:definition xml:lang="en">Italo house is a form of house music originating in Italy.
      Typically popular in Italy, Britain and United States since the late 1980s, it fuses house
      music and Italo disco. The genre's main musical characteristic is its use of predominantly
      electronic piano chords in a more lyrical form than classic Chicago House records. The best
      known example is Black Box's Ride On Time, but the genre became very popular in the late 1980s
      and early 1990s for the uplifting and anthemic tunes against the background of
      indie-dance.</skos:definition>
    <skos:exactMatch xml:lang="en">http://dbpedia.org/resource/Italo_house</skos:exactMatch>
    <skos:inScheme rdf:resource="http://data.europeana.eu/concept/music/genre/Music_Genre_Scheme"/>
    <skos:altLabel xml:lang="en">Italo house</skos:altLabel>
  </skos:Concept>

  <skos:Concept rdf:about="http://data.europeana.eu/concept/music/genre/Alternative_dance">
    <skos:prefLabel xml:lang="en">Alternative dance</skos:prefLabel>
    <skos:prefLabel xml:lang="cs">Alternative dance</skos:prefLabel>
    <skos:prefLabel xml:lang="nl">Alternative dance</skos:prefLabel>
    <skos:prefLabel xml:lang="fr">Indie dance</skos:prefLabel>
    <skos:prefLabel xml:lang="it">Alternative dance</skos:prefLabel>
    <skos:prefLabel xml:lang="pl">Alternative dance</skos:prefLabel>
    <skos:prefLabel xml:lang="pt">Dance alternativo</skos:prefLabel>
    <skos:prefLabel xml:lang="ru">Альтернативная танцевальная музыка</skos:prefLabel>
    <skos:prefLabel xml:lang="sk">Alternative dance</skos:prefLabel>
    <skos:prefLabel xml:lang="sv">Alternativ dance</skos:prefLabel>
    <skos:prefLabel xml:lang="th">อัลเทอร์เนทีฟแดนซ์</skos:prefLabel>
    <skos:prefLabel xml:lang="tr">Alternatif dans</skos:prefLabel>
    <skos:closeMatch rdf:resource="http://rdf.freebase.com/ns/m.041738"/>
    <skos:broader
      rdf:resource="http://data.europeana.eu/concept/music/genre/Electronic_rock_fusions"/>
    <skos:definition xml:lang="en">Alternative dance or indie dance is a musical genre that mixes
      various rock subgenres with electronic dance music. Although largely confined to the British
      Isles, it has gained American and worldwide exposure through acts such as New Order in the
      1980s and The Prodigy in the 1990s.</skos:definition>
    <skos:exactMatch xml:lang="en">http://dbpedia.org/resource/Alternative_dance</skos:exactMatch>
    <skos:inScheme rdf:resource="http://data.europeana.eu/concept/music/genre/Music_Genre_Scheme"/>
    <skos:altLabel xml:lang="en">Alternative dance</skos:altLabel>
  </skos:Concept>

  <skos:Concept rdf:about="http://data.europeana.eu/concept/music/genre/Turbofolk">
    <skos:prefLabel xml:lang="en">Turbo-folk</skos:prefLabel>
    <skos:prefLabel xml:lang="bg">Чалга</skos:prefLabel>
    <skos:prefLabel xml:lang="hr">Turbofolk</skos:prefLabel>
    <skos:prefLabel xml:lang="cs">Turbofolk</skos:prefLabel>
    <skos:prefLabel xml:lang="fi">Turbofolk</skos:prefLabel>
    <skos:prefLabel xml:lang="fr">Turbo folk</skos:prefLabel>
    <skos:prefLabel xml:lang="de">Turbo-Folk</skos:prefLabel>
    <skos:prefLabel xml:lang="el">Τούρμπο - Φόλκ</skos:prefLabel>
    <skos:prefLabel xml:lang="hu">Turbofolk</skos:prefLabel>
    <skos:prefLabel xml:lang="ja">ターボ・フォーク</skos:prefLabel>
    <skos:prefLabel xml:lang="pl">Turbofolk</skos:prefLabel>
    <skos:prefLabel xml:lang="pt">Turbofolk</skos:prefLabel>
    <skos:prefLabel xml:lang="ru">Турбо-фолк</skos:prefLabel>
    <skos:prefLabel xml:lang="sr">Турбо-фолк музика</skos:prefLabel>
    <skos:prefLabel xml:lang="sl">Turbo folk</skos:prefLabel>
    <skos:prefLabel xml:lang="es">Turbo-folk</skos:prefLabel>
    <skos:prefLabel xml:lang="uk">Турбо-фолк</skos:prefLabel>
    <skos:closeMatch rdf:resource="http://rdf.freebase.com/ns/m.047rw_"/>
    <skos:broader rdf:resource="http://data.europeana.eu/concept/music/genre/Pop_music_fusions"/>
    <skos:definition xml:lang="en">Turbo-folk is a musical sub-genre that originated in the Balkans.
      Having mainstream popularity in Serbia, although closely associated with Serbian performers,
      its sound is also popular in Bosnia and Herzegovina, Slovenia, Croatia, Macedonia, Albania,
      Bulgaria, Turkey and Montenegro. Its style is a sub-genre of folk music with dance, Eurodance
      and/or pop elements, with similar styles in Greece, Bulgaria, Romania and
      Albania.</skos:definition>
    <skos:exactMatch xml:lang="en">http://dbpedia.org/resource/Turbofolk</skos:exactMatch>
    <skos:inScheme rdf:resource="http://data.europeana.eu/concept/music/genre/Music_Genre_Scheme"/>
    <skos:altLabel xml:lang="en">Turbo-folk</skos:altLabel>
  </skos:Concept>

  <skos:Concept rdf:about="http://data.europeana.eu/concept/music/genre/Symphonic_metal">
    <skos:prefLabel xml:lang="en">Symphonic metal</skos:prefLabel>
    <skos:prefLabel xml:lang="ar">ميتال سيمفوني</skos:prefLabel>
    <skos:prefLabel xml:lang="bg">Симфоничен метъл</skos:prefLabel>
    <skos:prefLabel xml:lang="ca">Symphonic metal</skos:prefLabel>
    <skos:prefLabel xml:lang="hr">Simfonijski metal</skos:prefLabel>
    <skos:prefLabel xml:lang="cs">Symfonický metal</skos:prefLabel>
    <skos:prefLabel xml:lang="da">Symfonisk metal</skos:prefLabel>
    <skos:prefLabel xml:lang="nl">Symfonische metal</skos:prefLabel>
    <skos:prefLabel xml:lang="et">Sümfooniline metal</skos:prefLabel>
    <skos:prefLabel xml:lang="fi">Sinfoninen metalli</skos:prefLabel>
    <skos:prefLabel xml:lang="fr">Metal symphonique</skos:prefLabel>
    <skos:prefLabel xml:lang="de">Symphonic Metal</skos:prefLabel>
    <skos:prefLabel xml:lang="hu">Szimfonikus metal</skos:prefLabel>
    <skos:prefLabel xml:lang="it">Symphonic metal</skos:prefLabel>
    <skos:prefLabel xml:lang="ja">シンフォニックメタル</skos:prefLabel>
    <skos:prefLabel xml:lang="ko">심포닉 메탈</skos:prefLabel>
    <skos:prefLabel xml:lang="lv">Simfoniskais metāls</skos:prefLabel>
    <skos:prefLabel xml:lang="lt">Simfoninis metalas</skos:prefLabel>
    <skos:prefLabel xml:lang="no">Symfonisk metal</skos:prefLabel>
    <skos:prefLabel xml:lang="fa">سمفونیک متال</skos:prefLabel>
    <skos:prefLabel xml:lang="pl">Metal symfoniczny</skos:prefLabel>
    <skos:prefLabel xml:lang="pt">Metal sinfônico</skos:prefLabel>
    <skos:prefLabel xml:lang="ro">Symphonic metal</skos:prefLabel>
    <skos:prefLabel xml:lang="ru">Симфоник-метал</skos:prefLabel>
    <skos:prefLabel xml:lang="sr">Simfonijski metal</skos:prefLabel>
    <skos:prefLabel xml:lang="sk">Symfonický metal</skos:prefLabel>
    <skos:prefLabel xml:lang="sl">Simfonični metal</skos:prefLabel>
    <skos:prefLabel xml:lang="es">Metal sinfónico</skos:prefLabel>
    <skos:prefLabel xml:lang="sv">Symphonic metal</skos:prefLabel>
    <skos:prefLabel xml:lang="th">ซิมโฟนิกเมทัล</skos:prefLabel>
    <skos:prefLabel xml:lang="tr">Senfonik metal</skos:prefLabel>
    <skos:prefLabel xml:lang="uk">Симфо-метал</skos:prefLabel>
    <skos:prefLabel xml:lang="vi">Symphonic metal</skos:prefLabel>
    <skos:closeMatch rdf:resource="http://rdf.freebase.com/ns/m.04b675"/>
    <skos:broader
      rdf:resource="http://data.europeana.eu/concept/music/genre/Heavy_metal_music_fusions"/>
    <skos:definition xml:lang="en">Symphonic metal is a subgenre of metal music which combines the
      characteristics of this genre, such as heavy drums and guitars, with different elements of
      classical music including symphonic instruments, choirs and on occasion, a full symphony
      orchestra. Keyboards reminiscent of power metal also often find a dominant place in this
      subgenre. Symphonic metal bands often feature classically trained female vocalists, giving
      rise to the nickname Opera Metal or operatic metal, and it is not uncommon for them to feature
      a second vocalist performing growls, a more common characteristic of gothic metal. Perhaps the
      most typical and prominent examples of symphonic metal bands are Finnish Nightwish and Dutch
      Epica, both of which place a large focus on elements prevalent in film scores on top of the
      more basic classical components utilized more widely in the genre.</skos:definition>
    <skos:exactMatch xml:lang="en">http://dbpedia.org/resource/Symphonic_metal</skos:exactMatch>
    <skos:inScheme rdf:resource="http://data.europeana.eu/concept/music/genre/Music_Genre_Scheme"/>
    <skos:altLabel xml:lang="en">Symphonic black metal</skos:altLabel>
    <skos:altLabel xml:lang="en">Symphonic metal</skos:altLabel>
  </skos:Concept>

  <skos:Concept rdf:about="http://data.europeana.eu/concept/music/genre/Crossover_thrash">
    <skos:prefLabel xml:lang="en">Crossover thrash</skos:prefLabel>
    <skos:prefLabel xml:lang="ca">Crossover thrash</skos:prefLabel>
    <skos:prefLabel xml:lang="cs">Crossover thrash</skos:prefLabel>
    <skos:prefLabel xml:lang="da">Crossover thrash</skos:prefLabel>
    <skos:prefLabel xml:lang="nl">Crossover thrash</skos:prefLabel>
    <skos:prefLabel xml:lang="fi">Punk metal</skos:prefLabel>
    <skos:prefLabel xml:lang="fr">Crossover thrash</skos:prefLabel>
    <skos:prefLabel xml:lang="it">Punk metal</skos:prefLabel>
    <skos:prefLabel xml:lang="ja">クロスオーバー・スラッシュ</skos:prefLabel>
    <skos:prefLabel xml:lang="lt">Thrashcore</skos:prefLabel>
    <skos:prefLabel xml:lang="no">Crossover thrash</skos:prefLabel>
    <skos:prefLabel xml:lang="pl">Crossover thrash</skos:prefLabel>
    <skos:prefLabel xml:lang="pt">Crossover thrash</skos:prefLabel>
    <skos:prefLabel xml:lang="ro">Crossover thrash</skos:prefLabel>
    <skos:prefLabel xml:lang="ru">Кроссовер-трэш</skos:prefLabel>
    <skos:prefLabel xml:lang="sk">Crossover thrash</skos:prefLabel>
    <skos:prefLabel xml:lang="es">Crossover thrash</skos:prefLabel>
    <skos:closeMatch rdf:resource="http://rdf.freebase.com/ns/m.04f73rc"/>
    <skos:broader
      rdf:resource="http://data.europeana.eu/concept/music/genre/Heavy_metal_music_fusions"/>
    <skos:definition xml:lang="en">Crossover thrash is a form of thrash metal and hardcore punk
      which had mixed both genres together or had influences from each other. The genre lies on a
      continuum between heavy metal and punk rock. Other genres on the same continuum have
      significant overlap with crossover thrash, and besides tradition hardcore punk and thrash
      metal, include such related genres as thrashcore, grindcore and skate punk.</skos:definition>
    <skos:exactMatch xml:lang="en">http://dbpedia.org/resource/Crossover_thrash</skos:exactMatch>
    <skos:inScheme rdf:resource="http://data.europeana.eu/concept/music/genre/Music_Genre_Scheme"/>
    <skos:altLabel xml:lang="en">Crossover thrash</skos:altLabel>
  </skos:Concept>

  <skos:Concept rdf:about="http://data.europeana.eu/concept/music/genre/Kizomba">
    <skos:prefLabel xml:lang="en">Kizomba</skos:prefLabel>
    <skos:prefLabel xml:lang="fr">Kizomba</skos:prefLabel>
    <skos:prefLabel xml:lang="de">Kizomba</skos:prefLabel>
    <skos:prefLabel xml:lang="ja">キゾンバ</skos:prefLabel>
    <skos:prefLabel xml:lang="pl">Kizomba</skos:prefLabel>
    <skos:prefLabel xml:lang="pt">Kizomba</skos:prefLabel>
    <skos:prefLabel xml:lang="ru">Кизомба</skos:prefLabel>
    <skos:prefLabel xml:lang="sr">Кизомба</skos:prefLabel>
    <skos:prefLabel xml:lang="es">Kizomba</skos:prefLabel>
    <skos:prefLabel xml:lang="sv">Kizomba</skos:prefLabel>
    <skos:closeMatch rdf:resource="http://rdf.freebase.com/ns/m.04g0m3"/>
    <skos:broader
      rdf:resource="http://data.europeana.eu/concept/music/genre/African_popular_music_fusions"/>
    <skos:definition xml:lang="en">Kizomba is one of the most popular genres of dance and music
      originating in Angola. It mixes influences of traditional semba with Angolan merengue and
      Kilapanda. On this basis, Kizomba music emerged as a more modern music genre with a sensual
      touch mixed with African rhythm. Unlike semba, kizomba music is characterised by a slower and
      usually very romantic rhythm, sung generally in Portuguese. &lt;p&gt; It was the Kimbundu name
      for a dance in Angola as early as 1894. The Kizomba dancing style is also known to be very
      sensual and flows with a music of a romantic flow.</skos:definition>
    <skos:exactMatch xml:lang="en">http://dbpedia.org/resource/Kizomba</skos:exactMatch>
    <skos:inScheme rdf:resource="http://data.europeana.eu/concept/music/genre/Music_Genre_Scheme"/>
    <skos:altLabel xml:lang="en">Kizomba</skos:altLabel>
  </skos:Concept>

  <skos:Concept rdf:about="http://data.europeana.eu/concept/music/genre/Grime_(music)">
    <skos:prefLabel xml:lang="en">Grime</skos:prefLabel>
    <skos:prefLabel xml:lang="cs">Grime</skos:prefLabel>
    <skos:prefLabel xml:lang="da">Grime</skos:prefLabel>
    <skos:prefLabel xml:lang="nl">Grime</skos:prefLabel>
    <skos:prefLabel xml:lang="et">Grime</skos:prefLabel>
    <skos:prefLabel xml:lang="fi">Grime</skos:prefLabel>
    <skos:prefLabel xml:lang="fr">Grime</skos:prefLabel>
    <skos:prefLabel xml:lang="de">Grime</skos:prefLabel>
    <skos:prefLabel xml:lang="it">Grime</skos:prefLabel>
    <skos:prefLabel xml:lang="ja">グライム</skos:prefLabel>
    <skos:prefLabel xml:lang="ko">그라임</skos:prefLabel>
    <skos:prefLabel xml:lang="no">Grime</skos:prefLabel>
    <skos:prefLabel xml:lang="pl">Grime</skos:prefLabel>
    <skos:prefLabel xml:lang="pt">Grime</skos:prefLabel>
    <skos:prefLabel xml:lang="ro">Grime</skos:prefLabel>
    <skos:prefLabel xml:lang="ru">Грайм</skos:prefLabel>
    <skos:prefLabel xml:lang="sk">Grime</skos:prefLabel>
    <skos:prefLabel xml:lang="es">Grime</skos:prefLabel>
    <skos:prefLabel xml:lang="sv">Grime</skos:prefLabel>
    <skos:prefLabel xml:lang="th">ไกรม์</skos:prefLabel>
    <skos:prefLabel xml:lang="uk">Грайм</skos:prefLabel>
    <skos:closeMatch rdf:resource="http://rdf.freebase.com/ns/m.04j_h4"/>
    <skos:broader rdf:resource="http://data.europeana.eu/concept/music/genre/Hip_hop_music_fusions"/>
    <skos:definition xml:lang="en">Grime, also known as 8-bar, nu shape, sublow and eskibeat, is a
      style of British music that emerged in Bow, London. It was developed by teens of mostly
      African and Caribbean heritage, in the early 2000s, primarily as a development of UK garage,
      drum and bass, hip hop and dancehall. &lt;p&gt; Pioneers of this stylized music include
      English rappers Dizzee Rascal, Wiley, Kano, Roll Deep, Lethal Bizzle, More Fire Crew, Tinchy
      Stryder, Ruff Sqwad, Skepta, JME, Jammer, Boy Better Know, Crazy Titch, Durrty Goodz, Newham
      Generals, Ghetts, Devlin, Scorcher, Wretch 32 and Chip. &lt;p&gt; Grime crews included Roll
      Deep, Boy Better Know, Ruff Sqwad, More Fire Crew and So Solid Crew.</skos:definition>
    <skos:exactMatch xml:lang="en">http://dbpedia.org/resource/Grime_(music)</skos:exactMatch>
    <skos:inScheme rdf:resource="http://data.europeana.eu/concept/music/genre/Music_Genre_Scheme"/>
    <skos:altLabel xml:lang="en">Grime</skos:altLabel>
  </skos:Concept>

  <skos:Concept rdf:about="http://data.europeana.eu/concept/music/genre/Drone_metal">
    <skos:prefLabel xml:lang="en">Drone metal</skos:prefLabel>
    <skos:prefLabel xml:lang="hr">Drone doom</skos:prefLabel>
    <skos:prefLabel xml:lang="cs">Drone metal</skos:prefLabel>
    <skos:prefLabel xml:lang="de">Drone Doom</skos:prefLabel>
    <skos:prefLabel xml:lang="it">Drone doom metal</skos:prefLabel>
    <skos:prefLabel xml:lang="pl">Drone doom</skos:prefLabel>
    <skos:prefLabel xml:lang="ro">Drone metal</skos:prefLabel>
    <skos:prefLabel xml:lang="ru">Дроун-метал</skos:prefLabel>
    <skos:prefLabel xml:lang="sk">Drone metal</skos:prefLabel>
    <skos:prefLabel xml:lang="es">Drone doom</skos:prefLabel>
    <skos:prefLabel xml:lang="tr">Drone metal</skos:prefLabel>
    <skos:closeMatch rdf:resource="http://rdf.freebase.com/ns/m.04jpg_k"/>
    <skos:broader
      rdf:resource="http://data.europeana.eu/concept/music/genre/Heavy_metal_music_fusions"/>
    <skos:definition xml:lang="en">Drone metal is a style of heavy metal that melds the slow tempos
      and heaviness of doom metal with the long-duration tones of drone music. Drone metal is
      sometimes associated with post-metal or experimental metal.</skos:definition>
    <skos:exactMatch xml:lang="en">http://dbpedia.org/resource/Drone_metal</skos:exactMatch>
    <skos:inScheme rdf:resource="http://data.europeana.eu/concept/music/genre/Music_Genre_Scheme"/>
    <skos:altLabel xml:lang="en">Drone metal</skos:altLabel>
  </skos:Concept>

  <skos:Concept rdf:about="http://data.europeana.eu/concept/music/genre/Fuji_music">
    <skos:prefLabel xml:lang="en">Fuji music</skos:prefLabel>
    <skos:prefLabel xml:lang="pt">Fuji</skos:prefLabel>
    <skos:prefLabel xml:lang="es">Fuji</skos:prefLabel>
    <skos:closeMatch rdf:resource="http://rdf.freebase.com/ns/m.04kjhv"/>
    <skos:broader
      rdf:resource="http://data.europeana.eu/concept/music/genre/African_popular_music_fusions"/>
    <skos:definition xml:lang="en">Fuji is a popular Nigerian musical genre. It arose from the
      improvisation Ajisari/were music tradition, which is a kind of music performed to wake Muslims
      before dawn during the Ramadan fasting season. Were music/Ajisari itself was made popular by
      Alhaji Sikiru Ayinde Barrister.</skos:definition>
    <skos:exactMatch xml:lang="en">http://dbpedia.org/resource/Fuji_music</skos:exactMatch>
    <skos:inScheme rdf:resource="http://data.europeana.eu/concept/music/genre/Music_Genre_Scheme"/>
    <skos:altLabel xml:lang="en">Fuji music</skos:altLabel>
  </skos:Concept>

  <skos:Concept rdf:about="http://data.europeana.eu/concept/music/genre/Rap_metal">
    <skos:prefLabel xml:lang="en">Rap metal</skos:prefLabel>
    <skos:prefLabel xml:lang="cs">Rap metal</skos:prefLabel>
    <skos:prefLabel xml:lang="da">Rap metal</skos:prefLabel>
    <skos:prefLabel xml:lang="fr">Rapcore</skos:prefLabel>
    <skos:prefLabel xml:lang="hu">Rap metal</skos:prefLabel>
    <skos:prefLabel xml:lang="it">Rap metal</skos:prefLabel>
    <skos:prefLabel xml:lang="ja">ラップメタル</skos:prefLabel>
    <skos:prefLabel xml:lang="ko">랩 메탈</skos:prefLabel>
    <skos:prefLabel xml:lang="fa">رپ متال</skos:prefLabel>
    <skos:prefLabel xml:lang="pt">Rap metal</skos:prefLabel>
    <skos:prefLabel xml:lang="ro">Rap metal</skos:prefLabel>
    <skos:prefLabel xml:lang="ru">Рэп-метал</skos:prefLabel>
    <skos:prefLabel xml:lang="sk">Rap metal</skos:prefLabel>
    <skos:prefLabel xml:lang="es">Rap metal</skos:prefLabel>
    <skos:prefLabel xml:lang="sv">Rapmetal</skos:prefLabel>
    <skos:prefLabel xml:lang="uk">Реп-метал</skos:prefLabel>
    <skos:closeMatch rdf:resource="http://rdf.freebase.com/ns/m.04n7jdv"/>
    <skos:broader rdf:resource="http://data.europeana.eu/concept/music/genre/Rock_music_fusions"/>
    <skos:definition xml:lang="en">Rap metal is a sub-genre of rap rock and alternative metal music
      which fuses vocal and instrumental elements of hip hop with heavy metal.</skos:definition>
    <skos:exactMatch xml:lang="en">http://dbpedia.org/resource/Rap_metal</skos:exactMatch>
    <skos:inScheme rdf:resource="http://data.europeana.eu/concept/music/genre/Music_Genre_Scheme"/>
    <skos:altLabel xml:lang="en">Rap metal</skos:altLabel>
  </skos:Concept>

  <skos:Concept rdf:about="http://data.europeana.eu/concept/music/genre/Italo_disco">
    <skos:prefLabel xml:lang="en">Italo disco</skos:prefLabel>
    <skos:prefLabel xml:lang="bg">Итало-диско</skos:prefLabel>
    <skos:prefLabel xml:lang="ca">Italo disco</skos:prefLabel>
    <skos:prefLabel xml:lang="hr">Italo disco</skos:prefLabel>
    <skos:prefLabel xml:lang="cs">Italo disco</skos:prefLabel>
    <skos:prefLabel xml:lang="da">Italo disco</skos:prefLabel>
    <skos:prefLabel xml:lang="nl">Italodisco</skos:prefLabel>
    <skos:prefLabel xml:lang="fi">Italodisko</skos:prefLabel>
    <skos:prefLabel xml:lang="fr">Italo disco</skos:prefLabel>
    <skos:prefLabel xml:lang="de">Italo-Disco</skos:prefLabel>
    <skos:prefLabel xml:lang="it">Italo disco</skos:prefLabel>
    <skos:prefLabel xml:lang="ko">이탈로 디스코</skos:prefLabel>
    <skos:prefLabel xml:lang="fa">ایتالو دیسکو</skos:prefLabel>
    <skos:prefLabel xml:lang="pl">Italo disco</skos:prefLabel>
    <skos:prefLabel xml:lang="pt">Italo Disco</skos:prefLabel>
    <skos:prefLabel xml:lang="ru">Итало-диско</skos:prefLabel>
    <skos:prefLabel xml:lang="sk">Italo-disco</skos:prefLabel>
    <skos:prefLabel xml:lang="es">Italo disco</skos:prefLabel>
    <skos:prefLabel xml:lang="sv">Italodisco</skos:prefLabel>
    <skos:prefLabel xml:lang="uk">Італо-диско</skos:prefLabel>
    <skos:closeMatch rdf:resource="http://rdf.freebase.com/ns/m.04pcmw"/>
    <skos:broader rdf:resource="http://data.europeana.eu/concept/music/genre/Pop_music_fusions"/>
    <skos:definition xml:lang="en">Italo disco is a genre of music which originated in Italy and was
      mainly produced at the end of the 1970s to mid-1980s. The origin of the genre's name is
      strongly tied to marketing efforts of the ZYX record label, which began licensing and
      marketing the music outside of Italy in 1982. An early form of electronic dance music, Italo
      disco faded in the late 1980s when Italo house eclipsed it. &lt;p&gt; Italo disco borrowed
      elements from traditional disco music, yet was more electronic. The genre employed drum
      machines and synthesizers and was usually sung in English.</skos:definition>
    <skos:exactMatch xml:lang="en">http://dbpedia.org/resource/Italo_disco</skos:exactMatch>
    <skos:inScheme rdf:resource="http://data.europeana.eu/concept/music/genre/Music_Genre_Scheme"/>
    <skos:altLabel xml:lang="en">Italo disco</skos:altLabel>
  </skos:Concept>

  <skos:Concept rdf:about="http://data.europeana.eu/concept/music/genre/Benga_music">
    <skos:prefLabel xml:lang="en">Benga music</skos:prefLabel>
    <skos:prefLabel xml:lang="fi">Benga</skos:prefLabel>
    <skos:prefLabel xml:lang="fr">Benga</skos:prefLabel>
    <skos:prefLabel xml:lang="pt">Benga</skos:prefLabel>
    <skos:closeMatch rdf:resource="http://rdf.freebase.com/ns/m.04q06n"/>
    <skos:broader
      rdf:resource="http://data.europeana.eu/concept/music/genre/African_popular_music_fusions"/>
    <skos:definition xml:lang="en">Benga is a genre of Kenyan popular music. It evolved between the
      late 1940s and late 1960s, in Kenya's capital city of Nairobi. In the 1940s, the African
      Broadcasting Service in Nairobi aired a steady stream of soukous, South African kwela, Zairean
      finger-style guitar and various kinds of Cuban dance music. There were also popular folk songs
      of Kenya's Luo peoples.</skos:definition>
    <skos:exactMatch xml:lang="en">http://dbpedia.org/resource/Benga_music</skos:exactMatch>
    <skos:inScheme rdf:resource="http://data.europeana.eu/concept/music/genre/Music_Genre_Scheme"/>
    <skos:altLabel xml:lang="en">Benga music</skos:altLabel>
  </skos:Concept>

  <skos:Concept rdf:about="http://data.europeana.eu/concept/music/genre/Neofolk">
    <skos:prefLabel xml:lang="en">Neofolk</skos:prefLabel>
    <skos:prefLabel xml:lang="cs">Neofolk</skos:prefLabel>
    <skos:prefLabel xml:lang="nl">Neofolk</skos:prefLabel>
    <skos:prefLabel xml:lang="fr">Néofolk</skos:prefLabel>
    <skos:prefLabel xml:lang="de">Neofolk</skos:prefLabel>
    <skos:prefLabel xml:lang="hu">Neofolk</skos:prefLabel>
    <skos:prefLabel xml:lang="it">Neofolk</skos:prefLabel>
    <skos:prefLabel xml:lang="lt">Neofolklorinė muzika</skos:prefLabel>
    <skos:prefLabel xml:lang="pl">Neofolk</skos:prefLabel>
    <skos:prefLabel xml:lang="pt">Neofolk</skos:prefLabel>
    <skos:prefLabel xml:lang="ru">Неофолк</skos:prefLabel>
    <skos:prefLabel xml:lang="es">Neofolk</skos:prefLabel>
    <skos:prefLabel xml:lang="sv">Neofolk</skos:prefLabel>
    <skos:prefLabel xml:lang="uk">Неофолк</skos:prefLabel>
    <skos:closeMatch rdf:resource="http://rdf.freebase.com/ns/m.04qvq0"/>
    <skos:broader rdf:resource="http://data.europeana.eu/concept/music/genre/Folk_music_fusions"/>
    <skos:definition xml:lang="en">Neofolk is a form of folk music-inspired experimental music that
      emerged from post-industrial music circles. Neofolk can either be solely acoustic folk music
      or a blend of acoustic folk instrumentation aided by varieties of accompanying sounds such as
      pianos, strings and elements of industrial music and experimental music. The genre encompasses
      a wide assortment of themes. Neofolk musicians often have ties to other genres such as
      neoclassical and martial industrial.</skos:definition>
    <skos:exactMatch xml:lang="en">http://dbpedia.org/resource/Neofolk</skos:exactMatch>
    <skos:inScheme rdf:resource="http://data.europeana.eu/concept/music/genre/Music_Genre_Scheme"/>
    <skos:altLabel xml:lang="en">Neofolk</skos:altLabel>
  </skos:Concept>

  <skos:Concept rdf:about="http://data.europeana.eu/concept/music/genre/Mathcore">
    <skos:prefLabel xml:lang="en">Mathcore</skos:prefLabel>
    <skos:prefLabel xml:lang="nl">Mathcore</skos:prefLabel>
    <skos:prefLabel xml:lang="fi">Mathcore</skos:prefLabel>
    <skos:prefLabel xml:lang="fr">Mathcore</skos:prefLabel>
    <skos:prefLabel xml:lang="de">Mathcore</skos:prefLabel>
    <skos:prefLabel xml:lang="it">Mathcore</skos:prefLabel>
    <skos:prefLabel xml:lang="ja">カオティック・ハードコア</skos:prefLabel>
    <skos:prefLabel xml:lang="pl">Mathcore</skos:prefLabel>
    <skos:prefLabel xml:lang="pt">Mathcore</skos:prefLabel>
    <skos:prefLabel xml:lang="ro">Mathcore</skos:prefLabel>
    <skos:prefLabel xml:lang="ru">Маткор</skos:prefLabel>
    <skos:prefLabel xml:lang="sk">Mathcore</skos:prefLabel>
    <skos:prefLabel xml:lang="es">Mathcore</skos:prefLabel>
    <skos:prefLabel xml:lang="uk">Маткор</skos:prefLabel>
    <skos:closeMatch rdf:resource="http://rdf.freebase.com/ns/m.04ymln"/>
    <skos:broader
      rdf:resource="http://data.europeana.eu/concept/music/genre/Heavy_metal_music_fusions"/>
    <skos:definition xml:lang="en">Mathcore is a rhythmically complex and dissonant style of
      metalcore. It has its roots in bands such as Converge, Coalesce, Botch, and The Dillinger
      Escape Plan. The term mathcore is suggested by analogy with math rock. Both math rock and
      mathcore make use of unusual time signatures. Math rock groups such as Slint, Don Caballero,
      Shellac, and Drive Like Jehu have some influence on mathcore, though mathcore is more closely
      related to metalcore. Prominent mathcore groups have been associated with
      grindcore.</skos:definition>
    <skos:exactMatch xml:lang="en">http://dbpedia.org/resource/Mathcore</skos:exactMatch>
    <skos:inScheme rdf:resource="http://data.europeana.eu/concept/music/genre/Music_Genre_Scheme"/>
    <skos:altLabel xml:lang="en">Mathcore</skos:altLabel>
  </skos:Concept>

  <skos:Concept rdf:about="http://data.europeana.eu/concept/music/genre/Psychedelic_folk">
    <skos:prefLabel xml:lang="en">Psychedelic folk</skos:prefLabel>
    <skos:prefLabel xml:lang="cs">Psychedelický folk</skos:prefLabel>
    <skos:prefLabel xml:lang="nl">Psychedelische folk</skos:prefLabel>
    <skos:prefLabel xml:lang="fi">Psykedeelinen folk</skos:prefLabel>
    <skos:prefLabel xml:lang="fr">Folk psychédélique</skos:prefLabel>
    <skos:prefLabel xml:lang="de">Psychedelic Folk</skos:prefLabel>
    <skos:prefLabel xml:lang="it">Folk psichedelico</skos:prefLabel>
    <skos:prefLabel xml:lang="pl">Folk psychodeliczny</skos:prefLabel>
    <skos:prefLabel xml:lang="pt">Psych folk</skos:prefLabel>
    <skos:prefLabel xml:lang="ru">Психоделический фолк</skos:prefLabel>
    <skos:prefLabel xml:lang="sk">Psychedelický folk</skos:prefLabel>
    <skos:prefLabel xml:lang="es">Acid folk</skos:prefLabel>
    <skos:prefLabel xml:lang="sv">Acid folk</skos:prefLabel>
    <skos:closeMatch rdf:resource="http://rdf.freebase.com/ns/m.04z1v0"/>
    <skos:broader rdf:resource="http://data.europeana.eu/concept/music/genre/Folk_music_fusions"/>
    <skos:definition xml:lang="en">Psychedelic folk, psych folk or acid folk is a loosely defined
      form of psychedelic music that originated in the 1960s through the fusion of folk music and
      psychedelic rock. It retained the largely acoustic instrumentation of folk, but added musical
      influences common to psychedelic rock and the psychedelic experience.</skos:definition>
    <skos:exactMatch xml:lang="en">http://dbpedia.org/resource/Psychedelic_folk</skos:exactMatch>
    <skos:inScheme rdf:resource="http://data.europeana.eu/concept/music/genre/Music_Genre_Scheme"/>
    <skos:altLabel xml:lang="en">Psychedelic folk</skos:altLabel>
  </skos:Concept>

  <skos:Concept rdf:about="http://data.europeana.eu/concept/music/genre/Musique_concrete">
    <skos:prefLabel xml:lang="en">Musique concrète</skos:prefLabel>
    <skos:prefLabel xml:lang="ca">Música concreta</skos:prefLabel>
    <skos:prefLabel xml:lang="cs">Musique concrète</skos:prefLabel>
    <skos:prefLabel xml:lang="da">Konkret musik</skos:prefLabel>
    <skos:prefLabel xml:lang="nl">Musique Concrète</skos:prefLabel>
    <skos:prefLabel xml:lang="et">Konkreetne muusika</skos:prefLabel>
    <skos:prefLabel xml:lang="fi">Konkreettinen musiikki</skos:prefLabel>
    <skos:prefLabel xml:lang="fr">Musique concrète</skos:prefLabel>
    <skos:prefLabel xml:lang="de">Musique concrète</skos:prefLabel>
    <skos:prefLabel xml:lang="el">Συγκεκριμένη μουσική</skos:prefLabel>
    <skos:prefLabel xml:lang="it">Musica concreta</skos:prefLabel>
    <skos:prefLabel xml:lang="ja">ミュジーク・コンクレート</skos:prefLabel>
    <skos:prefLabel xml:lang="ko">구체 음악</skos:prefLabel>
    <skos:prefLabel xml:lang="no">Konkret musikk</skos:prefLabel>
    <skos:prefLabel xml:lang="pl">Muzyka konkretna</skos:prefLabel>
    <skos:prefLabel xml:lang="pt">Música concreta</skos:prefLabel>
    <skos:prefLabel xml:lang="ru">Конкретная музыка</skos:prefLabel>
    <skos:prefLabel xml:lang="es">Música concreta</skos:prefLabel>
    <skos:prefLabel xml:lang="sv">Konkret musik</skos:prefLabel>
    <skos:prefLabel xml:lang="uk">Конкретна музика</skos:prefLabel>
    <skos:closeMatch rdf:resource="http://rdf.freebase.com/ns/m.050tp"/>
    <skos:broader
      rdf:resource="http://data.europeana.eu/concept/music/genre/Electronic_music_fusions"/>
    <skos:definition xml:lang="en">Musique concrète is a form of electroacoustic music that is made
      in part from acousmatic sound. It can feature sounds derived from recordings of musical
      instruments, voice, and the natural environment as well as those created using synthesizers
      and computer-based digital signal processing. Also, compositions in this idiom are not
      restricted to the normal musical rules of melody, harmony, rhythm, metre, and so on.
      Originally contrasted with &quot;pure&quot; elektronische Musik, the theoretical basis of
      musique concrète as a compositional practice was developed by Pierre Schaeffer, beginning in
      the early 1940s.</skos:definition>
    <skos:exactMatch xml:lang="en">http://dbpedia.org/resource/Musique_concrète</skos:exactMatch>
    <skos:inScheme rdf:resource="http://data.europeana.eu/concept/music/genre/Music_Genre_Scheme"/>
    <skos:altLabel xml:lang="en">Musique concrete</skos:altLabel>
    <skos:altLabel xml:lang="en">Musique concrète</skos:altLabel>
  </skos:Concept>

  <skos:Concept rdf:about="http://data.europeana.eu/concept/music/genre/Soul_blues">
    <skos:prefLabel xml:lang="en">Soul blues</skos:prefLabel>
    <skos:prefLabel xml:lang="fr">Soul blues</skos:prefLabel>
    <skos:prefLabel xml:lang="it">Soul blues</skos:prefLabel>
    <skos:prefLabel xml:lang="pl">Soul blues</skos:prefLabel>
    <skos:prefLabel xml:lang="es">Soul blues</skos:prefLabel>
    <skos:closeMatch rdf:resource="http://rdf.freebase.com/ns/m.0513lz"/>
    <skos:broader rdf:resource="http://data.europeana.eu/concept/music/genre/Blues_fusions"/>
    <skos:definition xml:lang="en">Soul blues is a style of blues music developed in the late 1960s
      and early 1970s that combines elements of soul music and urban contemporary music. Singers and
      musicians who grew up listening to the traditional electric blues of artists such as Muddy
      Waters, Bo Diddley, Jimmy Reed and Elmore James, soul singers such as Sam Cooke, Ray Charles
      and Otis Redding, and gospel music wanted to bridge their favorite music together. Bobby Bland
      was one of the pioneers of this style. This is a sub-genre of blues that is very popular with
      African American audiences but less known by white audiences. The style continues to be
      popular in the new millennium.</skos:definition>
    <skos:exactMatch xml:lang="en">http://dbpedia.org/resource/Soul_blues</skos:exactMatch>
    <skos:inScheme rdf:resource="http://data.europeana.eu/concept/music/genre/Music_Genre_Scheme"/>
    <skos:altLabel xml:lang="en">Soul blues</skos:altLabel>
  </skos:Concept>

  <skos:Concept rdf:about="http://data.europeana.eu/concept/music/genre/Progressive_bluegrass">
    <skos:prefLabel xml:lang="en">Progressive bluegrass</skos:prefLabel>
    <skos:prefLabel xml:lang="it">Progressive bluegrass</skos:prefLabel>
    <skos:prefLabel xml:lang="ja">プログレッシブ・ブルーグラス</skos:prefLabel>
    <skos:closeMatch rdf:resource="http://rdf.freebase.com/ns/m.054nbl"/>
    <skos:broader rdf:resource="http://data.europeana.eu/concept/music/genre/Country_music_fusions"/>
    <skos:definition xml:lang="en">Progressive bluegrass is one of two major subgenres of bluegrass
      music. It is also known as newgrass, a term attributed to New Grass Revival member Ebo Walker.
      Musicians and bands John Hartford, New Grass Revival, J.D. Crowe and the New South, The
      Dillards, Boone Creek, Country Gazette, and the Seldom Scene pioneered innovations in the
      genre. Some groups began using electric instruments and importing songs from other genres,
      particularly rock &amp; roll. Progressive bluegrass became popular in the late 1960s and
      1970s, but it can be traced back to the banjo and contrabass duets that Earl Scruggs played
      even in the earliest days of the Foggy Mountain Boys. The four key distinguishing elements of
      progressive bluegrass are instrumentation, frequently including electric guitars, drums,
      piano, and more, songs imported or styles imitated from other musical genres like jazz, rock
      and others, non-traditional chord progressions, lengthy &quot;jam band&quot;-style
      improvisation. However, not all these elements are always present in progressive bluegrass.
      &lt;p&gt; Progressive bluegrass continues to be performed by bands today.</skos:definition>
    <skos:exactMatch xml:lang="en"
      >http://dbpedia.org/resource/Progressive_bluegrass</skos:exactMatch>
    <skos:inScheme rdf:resource="http://data.europeana.eu/concept/music/genre/Music_Genre_Scheme"/>
    <skos:altLabel xml:lang="en">Newgrass</skos:altLabel>
    <skos:altLabel xml:lang="en">Progressive bluegrass</skos:altLabel>
  </skos:Concept>

  <skos:Concept rdf:about="http://data.europeana.eu/concept/music/genre/Avant-garde_hip_hop">
    <skos:prefLabel xml:lang="en">Experimental hip hop</skos:prefLabel>
    <skos:prefLabel xml:lang="ar">هيب هوب تجريبي</skos:prefLabel>
    <skos:prefLabel xml:lang="lt">Eksperimentinis hip-hopas</skos:prefLabel>
    <skos:closeMatch rdf:resource="http://rdf.freebase.com/ns/m.0575kxq"/>
    <skos:broader rdf:resource="http://data.europeana.eu/concept/music/genre/Hip_hop_music_fusions"/>
    <skos:definition xml:lang="en">Experimental hip hop is a style of hip-hop that refers to the
      experimental use of structural elements outside of hip-hop considered unconventional within
      the larger hip hop music genre. Definitive Jux, Anticon, Big Dada and Ninja Tune are
      experimental hip hop and acid jazz labels. Experimental hip hop is usually electronically
      produced and incorporates turntablism. There are many artists that introduce acoustic elements
      to the genre to enhance the ability of being played live.</skos:definition>
    <skos:exactMatch xml:lang="en">http://dbpedia.org/resource/Avant-garde_hip_hop</skos:exactMatch>
    <skos:inScheme rdf:resource="http://data.europeana.eu/concept/music/genre/Music_Genre_Scheme"/>
    <skos:altLabel xml:lang="en">Experimental Rap/Hip-Hop</skos:altLabel>
    <skos:altLabel xml:lang="en">Experimental hip hop</skos:altLabel>
  </skos:Concept>

  <skos:Concept rdf:about="http://data.europeana.eu/concept/music/genre/Disco_polo">
    <skos:prefLabel xml:lang="en">Disco polo</skos:prefLabel>
    <skos:prefLabel xml:lang="bg">Полско диско</skos:prefLabel>
    <skos:prefLabel xml:lang="de">Disco Polo</skos:prefLabel>
    <skos:prefLabel xml:lang="ko">디스코 폴로</skos:prefLabel>
    <skos:prefLabel xml:lang="no">Disco polo</skos:prefLabel>
    <skos:prefLabel xml:lang="fa">دیسکو پولو</skos:prefLabel>
    <skos:prefLabel xml:lang="pl">Disco polo</skos:prefLabel>
    <skos:prefLabel xml:lang="pt">Disco polo</skos:prefLabel>
    <skos:prefLabel xml:lang="sv">Disco polo</skos:prefLabel>
    <skos:closeMatch rdf:resource="http://rdf.freebase.com/ns/m.057qzp"/>
    <skos:broader rdf:resource="http://data.europeana.eu/concept/music/genre/Pop_music_fusions"/>
    <skos:definition xml:lang="en">Disco polo is a musical genre native to Poland, which exists in
      its present form since the early 1990s, with a peak in 1995-1997. It was derived from the
      Disco, Euro disco contemporary folk tunes influenced by Italo disco and Polish folk songs.
      &lt;p&gt; The name itself was conceived by S?awomir Skr?ta from the group Blue Star as a
      replacement for an older term, piosenka chodnikowa - which originated from the main means of
      distribution of its recordings in early 1990s - sidewalk stalls on streets and at bazaars.
      Disco polo could be heard mostly at country picnics, country depots, weddings or during
      political campaigning for Polish parliament and presidential elections. Former president
      Aleksander Kwa?niewski was one of the most notable example of a politician who used disco polo
      during his presidential campaign. &lt;p&gt; Traditional instrumentation came to be replaced by
      keyboards later in the '90s, which contributed to a slight change in style, making the songs
      more similar to modern dance music. The style was extensively marketed by the Polsat TV
      station, which produced its own disco polo hit list, in a TV show called Disco
      Relax.</skos:definition>
    <skos:exactMatch xml:lang="en">http://dbpedia.org/resource/Disco_polo</skos:exactMatch>
    <skos:inScheme rdf:resource="http://data.europeana.eu/concept/music/genre/Music_Genre_Scheme"/>
    <skos:altLabel xml:lang="en">Disco polo</skos:altLabel>
  </skos:Concept>

  <skos:Concept rdf:about="http://data.europeana.eu/concept/music/genre/UK_funky">
    <skos:prefLabel xml:lang="en">UK funky</skos:prefLabel>
    <skos:prefLabel xml:lang="pl">UK funky</skos:prefLabel>
    <skos:prefLabel xml:lang="es">UK funky</skos:prefLabel>
    <skos:closeMatch rdf:resource="http://rdf.freebase.com/ns/m.05b_xt3"/>
    <skos:broader rdf:resource="http://data.europeana.eu/concept/music/genre/Hip_hop_music_fusions"/>
    <skos:definition xml:lang="en">UK funky is a genre of electronic dance music from the United
      Kingdom that is heavily influenced by deep house, Afrobeat, soca, electro house, broken beat
      and UK garage. It often gets confused with funky house in America which is mainly disco and
      funk orientated. Typically, UK funky blends beats, bass loops and synths with African and
      Latin percussion in the dem bow rhythm and contemporary R&amp;B-style
      vocals.</skos:definition>
    <skos:exactMatch xml:lang="en">http://dbpedia.org/resource/UK_funky</skos:exactMatch>
    <skos:inScheme rdf:resource="http://data.europeana.eu/concept/music/genre/Music_Genre_Scheme"/>
    <skos:altLabel xml:lang="en">UK funky house</skos:altLabel>
    <skos:altLabel xml:lang="en">UK funky</skos:altLabel>
  </skos:Concept>

  <skos:Concept rdf:about="http://data.europeana.eu/concept/music/genre/Wonky_pop">
    <skos:prefLabel xml:lang="en">Wonky pop</skos:prefLabel>
    <skos:closeMatch rdf:resource="http://rdf.freebase.com/ns/m.05b3t5_"/>
    <skos:broader rdf:resource="http://data.europeana.eu/concept/music/genre/Pop_music_fusions"/>
    <skos:definition xml:lang="en">Wonky pop was a loose grouping of musical acts that played what
      the BBC called &quot;quirky, catchy and credible pop&quot;, rooted in the eccentric side of
      1980s pop music, which was briefly popular in the late 2000s. Artists associated with the
      genre include Mika, Alphabeat and Frankmusik.</skos:definition>
    <skos:exactMatch xml:lang="en">http://dbpedia.org/resource/Wonky_pop</skos:exactMatch>
    <skos:inScheme rdf:resource="http://data.europeana.eu/concept/music/genre/Music_Genre_Scheme"/>
    <skos:altLabel xml:lang="en">Wonky pop</skos:altLabel>
  </skos:Concept>

  <skos:Concept rdf:about="http://data.europeana.eu/concept/music/genre/Pop_rock">
    <skos:prefLabel xml:lang="en">Pop rock</skos:prefLabel>
    <skos:prefLabel xml:lang="ar">بوب روك</skos:prefLabel>
    <skos:prefLabel xml:lang="bg">Поп рок</skos:prefLabel>
    <skos:prefLabel xml:lang="ca">Pop rock</skos:prefLabel>
    <skos:prefLabel xml:lang="hr">Pop rock</skos:prefLabel>
    <skos:prefLabel xml:lang="cs">Pop rock</skos:prefLabel>
    <skos:prefLabel xml:lang="da">Poprock</skos:prefLabel>
    <skos:prefLabel xml:lang="nl">Poprock</skos:prefLabel>
    <skos:prefLabel xml:lang="fi">Pop rock</skos:prefLabel>
    <skos:prefLabel xml:lang="fr">Pop rock</skos:prefLabel>
    <skos:prefLabel xml:lang="de">Pop-Rock</skos:prefLabel>
    <skos:prefLabel xml:lang="hi">पॉप रॉक</skos:prefLabel>
    <skos:prefLabel xml:lang="hu">Pop rock</skos:prefLabel>
    <skos:prefLabel xml:lang="id">Pop rock</skos:prefLabel>
    <skos:prefLabel xml:lang="it">Pop rock</skos:prefLabel>
    <skos:prefLabel xml:lang="ja">ポップ・ロック</skos:prefLabel>
    <skos:prefLabel xml:lang="ko">팝 록</skos:prefLabel>
    <skos:prefLabel xml:lang="lv">Poproks</skos:prefLabel>
    <skos:prefLabel xml:lang="lt">Pop rokas</skos:prefLabel>
    <skos:prefLabel xml:lang="no">Poprock</skos:prefLabel>
    <skos:prefLabel xml:lang="fa">پاپ راک</skos:prefLabel>
    <skos:prefLabel xml:lang="pl">Pop-rock</skos:prefLabel>
    <skos:prefLabel xml:lang="pt">Pop rock</skos:prefLabel>
    <skos:prefLabel xml:lang="ro">Muzică pop-rock</skos:prefLabel>
    <skos:prefLabel xml:lang="ru">Поп-рок</skos:prefLabel>
    <skos:prefLabel xml:lang="sk">Pop rock</skos:prefLabel>
    <skos:prefLabel xml:lang="sl">Pop rock</skos:prefLabel>
    <skos:prefLabel xml:lang="es">Pop rock</skos:prefLabel>
    <skos:prefLabel xml:lang="sv">Poprock</skos:prefLabel>
    <skos:prefLabel xml:lang="th">ป็อปร็อก</skos:prefLabel>
    <skos:prefLabel xml:lang="tr">Pop rock</skos:prefLabel>
    <skos:prefLabel xml:lang="uk">Поп-рок</skos:prefLabel>
    <skos:prefLabel xml:lang="vi">Pop rock</skos:prefLabel>
    <skos:closeMatch rdf:resource="http://rdf.freebase.com/ns/m.05bt6j"/>
    <skos:broader rdf:resource="http://data.europeana.eu/concept/music/genre/Rock_music_fusions"/>
    <skos:definition xml:lang="en">Pop rock is a music genre which mixes a catchy pop style and
      light lyrics in its guitar-based rock songs. There are varying definitions of the term,
      ranging from a slower and mellower form of rock music to a subgenre of pop music. The
      detractors of pop rock often deride it as a slick, commercial product, less authentic than
      rock music.</skos:definition>
    <skos:exactMatch xml:lang="en">http://dbpedia.org/resource/Pop_rock</skos:exactMatch>
    <skos:inScheme rdf:resource="http://data.europeana.eu/concept/music/genre/Music_Genre_Scheme"/>
    <skos:altLabel xml:lang="en">Pop rock</skos:altLabel>
  </skos:Concept>

  <skos:Concept rdf:about="http://data.europeana.eu/concept/music/genre/Electronic_rock">
    <skos:prefLabel xml:lang="en">Electronic rock</skos:prefLabel>
    <skos:prefLabel xml:lang="bg">Електронен рок</skos:prefLabel>
    <skos:prefLabel xml:lang="cs">Synth rock</skos:prefLabel>
    <skos:prefLabel xml:lang="et">Elektrooniline rock</skos:prefLabel>
    <skos:prefLabel xml:lang="fi">Electronic rock</skos:prefLabel>
    <skos:prefLabel xml:lang="fr">Électro-rock</skos:prefLabel>
    <skos:prefLabel xml:lang="de">Synth Rock</skos:prefLabel>
    <skos:prefLabel xml:lang="it">Rock elettronico</skos:prefLabel>
    <skos:prefLabel xml:lang="ja">エレクトロ・ロック</skos:prefLabel>
    <skos:prefLabel xml:lang="ko">전자 록</skos:prefLabel>
    <skos:prefLabel xml:lang="no">Synth rock</skos:prefLabel>
    <skos:prefLabel xml:lang="pl">Rock elektroniczny</skos:prefLabel>
    <skos:prefLabel xml:lang="pt">Rock eletrônico</skos:prefLabel>
    <skos:prefLabel xml:lang="ro">Rock electronic</skos:prefLabel>
    <skos:prefLabel xml:lang="ru">Электронный рок</skos:prefLabel>
    <skos:prefLabel xml:lang="sk">Elektronický rock</skos:prefLabel>
    <skos:prefLabel xml:lang="es">Rock electrónico</skos:prefLabel>
    <skos:prefLabel xml:lang="sv">Elektronisk rock</skos:prefLabel>
    <skos:prefLabel xml:lang="th">อิเล็กทรอนิกส์ร็อก</skos:prefLabel>
    <skos:prefLabel xml:lang="uk">Електро-рок</skos:prefLabel>
    <skos:closeMatch rdf:resource="http://rdf.freebase.com/ns/m.05c6073"/>
    <skos:broader rdf:resource="http://data.europeana.eu/concept/music/genre/Rock_music_fusions"/>
    <skos:definition xml:lang="en">Electronic rock, also commonly referred to as synthrock,
      electrorock, techno-rock, or digital rock is rock music generated with electronic instruments.
      It has been highly dependent on technological developments, particularly the invention and
      refinement of the synthesizer, the development of the MIDI digital format and computer
      technology. &lt;p&gt; In the late 1960s rock musicians began to use electronic instruments,
      like the theremin and Mellotron, to supplement and define their sound, by the end of the
      decade the Moog synthesizer took a leading place in the sound of emerging progressive rock
      bands who would dominate rock in the early 1970s. After the arrival of punk rock a form of
      basic synth rock emerged, increasingly using new digital technology to replace other
      instruments. In the 1980s more commercially oriented synth pop dominated electronic rock. In
      the 1990s big beat and industrial rock were among the most important new trends and in the new
      millennium the spread of recording software led to the development of new distinct genres
      including indietronica, electroclash, dance-punk and new rave.</skos:definition>
    <skos:exactMatch xml:lang="en">http://dbpedia.org/resource/Electronic_rock</skos:exactMatch>
    <skos:inScheme rdf:resource="http://data.europeana.eu/concept/music/genre/Music_Genre_Scheme"/>
    <skos:altLabel xml:lang="en">Electro rock</skos:altLabel>
    <skos:altLabel xml:lang="en">Digital rock</skos:altLabel>
    <skos:altLabel xml:lang="en">Electronic rock</skos:altLabel>
  </skos:Concept>

  <skos:Concept rdf:about="http://data.europeana.eu/concept/music/genre/Nu_metal">
    <skos:prefLabel xml:lang="en">Nu metal</skos:prefLabel>
    <skos:prefLabel xml:lang="ar">نيو ميتال</skos:prefLabel>
    <skos:prefLabel xml:lang="bg">Ню метъл</skos:prefLabel>
    <skos:prefLabel xml:lang="ca">Nu metal</skos:prefLabel>
    <skos:prefLabel xml:lang="hr">Nu metal</skos:prefLabel>
    <skos:prefLabel xml:lang="cs">Nu metal</skos:prefLabel>
    <skos:prefLabel xml:lang="da">Nu-metal</skos:prefLabel>
    <skos:prefLabel xml:lang="nl">Nu metal</skos:prefLabel>
    <skos:prefLabel xml:lang="et">Nu metal</skos:prefLabel>
    <skos:prefLabel xml:lang="fi">Nu metal</skos:prefLabel>
    <skos:prefLabel xml:lang="fr">Nu metal</skos:prefLabel>
    <skos:prefLabel xml:lang="de">Nu Metal</skos:prefLabel>
    <skos:prefLabel xml:lang="el">Nu Metal</skos:prefLabel>
    <skos:prefLabel xml:lang="hu">Nu metal</skos:prefLabel>
    <skos:prefLabel xml:lang="id">Nu metal</skos:prefLabel>
    <skos:prefLabel xml:lang="it">Nu metal</skos:prefLabel>
    <skos:prefLabel xml:lang="ja">ニュー・メタル</skos:prefLabel>
    <skos:prefLabel xml:lang="ko">누 메탈</skos:prefLabel>
    <skos:prefLabel xml:lang="lv">Ņūmetāls</skos:prefLabel>
    <skos:prefLabel xml:lang="lt">Nu metal</skos:prefLabel>
    <skos:prefLabel xml:lang="ms">Nu metal</skos:prefLabel>
    <skos:prefLabel xml:lang="no">Nu metal</skos:prefLabel>
    <skos:prefLabel xml:lang="fa">نیو متال</skos:prefLabel>
    <skos:prefLabel xml:lang="pl">Nu metal</skos:prefLabel>
    <skos:prefLabel xml:lang="pt">Nu metal</skos:prefLabel>
    <skos:prefLabel xml:lang="ro">Nu metal</skos:prefLabel>
    <skos:prefLabel xml:lang="ru">Ню-метал</skos:prefLabel>
    <skos:prefLabel xml:lang="sr">Ну метал</skos:prefLabel>
    <skos:prefLabel xml:lang="sk">Nu metal</skos:prefLabel>
    <skos:prefLabel xml:lang="sl">Nu metal</skos:prefLabel>
    <skos:prefLabel xml:lang="es">Nu metal</skos:prefLabel>
    <skos:prefLabel xml:lang="sv">Nu-metal</skos:prefLabel>
    <skos:prefLabel xml:lang="th">นูเมทัล</skos:prefLabel>
    <skos:prefLabel xml:lang="tr">Nu metal</skos:prefLabel>
    <skos:prefLabel xml:lang="uk">Ню-метал</skos:prefLabel>
    <skos:prefLabel xml:lang="vi">Nu metal</skos:prefLabel>
    <skos:closeMatch rdf:resource="http://rdf.freebase.com/ns/m.05jt_"/>
    <skos:broader
      rdf:resource="http://data.europeana.eu/concept/music/genre/Alternative_rock_fusions"/>
    <skos:definition xml:lang="en">Nu metal is a fusion genre of heavy metal that combines metal
      music with hip hop, hardcore punk and grunge. It is classified as part of alternative
      metal.</skos:definition>
    <skos:exactMatch xml:lang="en">http://dbpedia.org/resource/Nu_metal</skos:exactMatch>
    <skos:inScheme rdf:resource="http://data.europeana.eu/concept/music/genre/Music_Genre_Scheme"/>
    <skos:altLabel xml:lang="en">Nu metal</skos:altLabel>
  </skos:Concept>

  <skos:Concept rdf:about="http://data.europeana.eu/concept/music/genre/Hip_hop_soul">
    <skos:prefLabel xml:lang="en">Hip hop soul</skos:prefLabel>
    <skos:prefLabel xml:lang="ca">Hip-hop soul</skos:prefLabel>
    <skos:prefLabel xml:lang="hr">Hip hop soul</skos:prefLabel>
    <skos:prefLabel xml:lang="cs">Hip-hop soul</skos:prefLabel>
    <skos:prefLabel xml:lang="nl">Urban pop</skos:prefLabel>
    <skos:prefLabel xml:lang="fr">R'n'B</skos:prefLabel>
    <skos:prefLabel xml:lang="de">Contemporary R&amp;B</skos:prefLabel>
    <skos:prefLabel xml:lang="it">Hip hop soul</skos:prefLabel>
    <skos:prefLabel xml:lang="ja">ヒップホップ・ソウル</skos:prefLabel>
    <skos:prefLabel xml:lang="lt">Soul Hiphopas</skos:prefLabel>
    <skos:prefLabel xml:lang="pt">Hip hop soul</skos:prefLabel>
    <skos:prefLabel xml:lang="ru">Хип-хоп соул</skos:prefLabel>
    <skos:prefLabel xml:lang="sk">Hip-hop soul</skos:prefLabel>
    <skos:prefLabel xml:lang="es">Hip hop soul</skos:prefLabel>
    <skos:prefLabel xml:lang="sv">Hiphop soul</skos:prefLabel>
    <skos:prefLabel xml:lang="th">ฮิปฮอป โซล</skos:prefLabel>
    <skos:closeMatch rdf:resource="http://rdf.freebase.com/ns/m.05lwjc"/>
    <skos:broader rdf:resource="http://data.europeana.eu/concept/music/genre/Hip_hop_music_fusions"/>
    <skos:definition xml:lang="en">Hip hop soul is a subgenre of contemporary R&amp;B music, most
      popular during the early to mid 1990s, which fuses rhythm and blues/gospel singing with hip
      hop musical production. The sub genre was the evolution of new jack swing, which had
      incorporated hip-hop influences into R&amp;B music. By contrast, hip hop soul is, as described
      in The Encyclopedia of African American Music, &quot;quite literally soul singing over hip hop
      grooves.&quot; &lt;p&gt; The genre was most popular during the mid 1990s with artists such as
      Mary J. Blige, Jodeci, TLC, R. Kelly, Aaliyah, and Montell Jordan. By the late 1990s, hip hop
      soul would lead to the creation of neo soul, which retained the hip-hop and R&amp;B/gospel
      influences while also adding elements of classic 1970s soul music.</skos:definition>
    <skos:exactMatch xml:lang="en">http://dbpedia.org/resource/Hip_hop_soul</skos:exactMatch>
    <skos:inScheme rdf:resource="http://data.europeana.eu/concept/music/genre/Music_Genre_Scheme"/>
    <skos:altLabel xml:lang="en">Hip hop soul</skos:altLabel>
  </skos:Concept>

  <skos:Concept rdf:about="http://data.europeana.eu/concept/music/genre/Power_electronics_(music)">
    <skos:prefLabel xml:lang="en">Power electronics</skos:prefLabel>
    <skos:prefLabel xml:lang="cs">Power electronics</skos:prefLabel>
    <skos:prefLabel xml:lang="nl">Power electronics</skos:prefLabel>
    <skos:prefLabel xml:lang="fi">Power electronics</skos:prefLabel>
    <skos:prefLabel xml:lang="fr">Death industriel</skos:prefLabel>
    <skos:prefLabel xml:lang="it">Power electronics</skos:prefLabel>
    <skos:prefLabel xml:lang="ru">Пауэр-электроникс</skos:prefLabel>
    <skos:prefLabel xml:lang="sk">Power electronics</skos:prefLabel>
    <skos:prefLabel xml:lang="sv">Power electronics</skos:prefLabel>
    <skos:closeMatch rdf:resource="http://rdf.freebase.com/ns/m.05mr420"/>
    <skos:broader
      rdf:resource="http://data.europeana.eu/concept/music/genre/Electronic_music_fusions"/>
    <skos:definition xml:lang="en">Power electronics was originally coined by William Bennett as
      part of the sleevenotes to the Whitehouse album Psychopathia Sexualis, and is related to the
      early Industrial Records scene but later became more identified with noise music. It consists
      of screeching waves of feedback, analogue synthesizers making sub-bass pulses or high
      frequency squealing sounds, and screamed, distorted, often hateful and offensive lyrics.
      Deeply atonal, there are no conventional melodies or rhythms. Artists include Philip Best,
      Ramleh, Sutcliffe Jügend, and Genocide Organ. &lt;p&gt; Tellus Audio Cassette Magazine
      produced a compilation compact cassette tape called Power Electronics in 1986 that was curated
      by Joseph Nechvatal.</skos:definition>
    <skos:exactMatch xml:lang="en"
      >http://dbpedia.org/resource/Power_electronics_(music)</skos:exactMatch>
    <skos:inScheme rdf:resource="http://data.europeana.eu/concept/music/genre/Music_Genre_Scheme"/>
    <skos:altLabel xml:lang="en">Power electronics</skos:altLabel>
  </skos:Concept>

  <skos:Concept rdf:about="http://data.europeana.eu/concept/music/genre/Powerviolence">
    <skos:prefLabel xml:lang="en">Powerviolence</skos:prefLabel>
    <skos:prefLabel xml:lang="cs">Powerviolence</skos:prefLabel>
    <skos:prefLabel xml:lang="fi">Powerviolence</skos:prefLabel>
    <skos:prefLabel xml:lang="de">Powerviolence</skos:prefLabel>
    <skos:prefLabel xml:lang="it">Power violence</skos:prefLabel>
    <skos:prefLabel xml:lang="pt">Powerviolence</skos:prefLabel>
    <skos:prefLabel xml:lang="ru">Пауэрвайоленс</skos:prefLabel>
    <skos:prefLabel xml:lang="sk">Powerviolence</skos:prefLabel>
    <skos:prefLabel xml:lang="es">Powerviolence</skos:prefLabel>
    <skos:closeMatch rdf:resource="http://rdf.freebase.com/ns/m.05p50f"/>
    <skos:broader rdf:resource="http://data.europeana.eu/concept/music/genre/Punk_rock_fusions"/>
    <skos:definition xml:lang="en">Powerviolence, is a raw and dissonant subgenre of hardcore punk.
      The style is closely related to thrashcore and grindcore. In contrast with grindcore, which is
      a &quot;crossover&quot; idiom containing musical aspects of heavy metal, powerviolence is just
      an augmentation of the most challenging qualities of hardcore punk, like its predecessor, it
      is usually socio-politically charged and iconoclastic.</skos:definition>
    <skos:exactMatch xml:lang="en">http://dbpedia.org/resource/Powerviolence</skos:exactMatch>
    <skos:inScheme rdf:resource="http://data.europeana.eu/concept/music/genre/Music_Genre_Scheme"/>
    <skos:altLabel xml:lang="en">Powerviolence</skos:altLabel>
  </skos:Concept>

  <skos:Concept rdf:about="http://data.europeana.eu/concept/music/genre/Raga_rock">
    <skos:prefLabel xml:lang="en">Raga rock</skos:prefLabel>
    <skos:prefLabel xml:lang="fi">Raga rock</skos:prefLabel>
    <skos:prefLabel xml:lang="de">Raga Rock</skos:prefLabel>
    <skos:prefLabel xml:lang="it">Raga rock</skos:prefLabel>
    <skos:prefLabel xml:lang="ja">ラーガ・ロック</skos:prefLabel>
    <skos:prefLabel xml:lang="pl">Raga rock</skos:prefLabel>
    <skos:prefLabel xml:lang="ru">Рага-рок</skos:prefLabel>
    <skos:prefLabel xml:lang="sk">Raga rock</skos:prefLabel>
    <skos:prefLabel xml:lang="es">Raga rock</skos:prefLabel>
    <skos:closeMatch rdf:resource="http://rdf.freebase.com/ns/m.05r008"/>
    <skos:broader rdf:resource="http://data.europeana.eu/concept/music/genre/Rock_music_fusions"/>
    <skos:definition xml:lang="en">Raga rock is rock or pop music with a heavy Indian influence,
      either in its construction, its timbre, or its use of instrumentation, such as the sitar and
      tabla. More recently, scholars have included British rock music from the 1960s and 1970s that
      utilizes South Asian musical materials and instruments and Western ideas of South Asia.
      &lt;p&gt; Raga rock is not normally considered a specific genre of music, but rather a general
      aspect of any rock significantly influenced by Indian classical music. Since Indian influences
      are primarily limited to 1960s rock, most raga rock is limited to that decade, although
      heavily Indian-derived sounds are found in some post-1960s rock.</skos:definition>
    <skos:exactMatch xml:lang="en">http://dbpedia.org/resource/Raga_rock</skos:exactMatch>
    <skos:inScheme rdf:resource="http://data.europeana.eu/concept/music/genre/Music_Genre_Scheme"/>
    <skos:altLabel xml:lang="en">Raga rock</skos:altLabel>
  </skos:Concept>

  <skos:Concept rdf:about="http://data.europeana.eu/concept/music/genre/Hiplife">
    <skos:prefLabel xml:lang="en">Hiplife</skos:prefLabel>
    <skos:prefLabel xml:lang="fi">Hiplife</skos:prefLabel>
    <skos:prefLabel xml:lang="fr">Hiplife</skos:prefLabel>
    <skos:prefLabel xml:lang="de">Hiplife</skos:prefLabel>
    <skos:prefLabel xml:lang="it">Hip life</skos:prefLabel>
    <skos:prefLabel xml:lang="pt">Hiplife</skos:prefLabel>
    <skos:prefLabel xml:lang="es">Hiplife</skos:prefLabel>
    <skos:closeMatch rdf:resource="http://rdf.freebase.com/ns/m.05r99v"/>
    <skos:broader rdf:resource="http://data.europeana.eu/concept/music/genre/Hip_hop_music_fusions"/>
    <skos:definition xml:lang="en">Hiplife is a Ghanaian musical style which fuses highlife and hip
      hop. It is also influenced by dancehall and reggae. Recorded predominantly in the Ghanaian
      language Akan, hiplife is rapidly gaining popularity throughout West Africa and abroad,
      especially in the United Kingdom, United States, Canada and Germany.</skos:definition>
    <skos:exactMatch xml:lang="en">http://dbpedia.org/resource/Hiplife</skos:exactMatch>
    <skos:inScheme rdf:resource="http://data.europeana.eu/concept/music/genre/Music_Genre_Scheme"/>
    <skos:altLabel xml:lang="en">Hiplife</skos:altLabel>
  </skos:Concept>

  <skos:Concept rdf:about="http://data.europeana.eu/concept/music/genre/Power_noise">
    <skos:prefLabel xml:lang="en">Power noise</skos:prefLabel>
    <skos:prefLabel xml:lang="cs">Rhythmic Noise</skos:prefLabel>
    <skos:prefLabel xml:lang="nl">Power noise</skos:prefLabel>
    <skos:prefLabel xml:lang="fi">Power noise</skos:prefLabel>
    <skos:prefLabel xml:lang="fr">Power noise</skos:prefLabel>
    <skos:prefLabel xml:lang="de">Rhythm ’n’ Noise</skos:prefLabel>
    <skos:prefLabel xml:lang="it">Power noise</skos:prefLabel>
    <skos:prefLabel xml:lang="lv">Industriālais tehno</skos:prefLabel>
    <skos:prefLabel xml:lang="pt">Harsh</skos:prefLabel>
    <skos:prefLabel xml:lang="ru">Пауэр-нойз</skos:prefLabel>
    <skos:prefLabel xml:lang="es">Harsh</skos:prefLabel>
    <skos:prefLabel xml:lang="uk">Пауер-нойз</skos:prefLabel>
    <skos:closeMatch rdf:resource="http://rdf.freebase.com/ns/m.05st7y"/>
    <skos:broader
      rdf:resource="http://data.europeana.eu/concept/music/genre/Electronic_music_fusions"/>
    <skos:definition xml:lang="en">Power noise is a fusion genre among noise music and various
      styles of electronic dance music. It should not be confused with &quot;power
      electronics&quot;, which is not influenced by electronic dance music and is closer to harsh
      noise. Its origins are predominantly European.</skos:definition>
    <skos:exactMatch xml:lang="en">http://dbpedia.org/resource/Power_noise</skos:exactMatch>
    <skos:inScheme rdf:resource="http://data.europeana.eu/concept/music/genre/Music_Genre_Scheme"/>
    <skos:altLabel xml:lang="en">Power noise</skos:altLabel>
  </skos:Concept>

  <skos:Concept rdf:about="http://data.europeana.eu/concept/music/genre/Folk_punk">
    <skos:prefLabel xml:lang="en">Folk punk</skos:prefLabel>
    <skos:prefLabel xml:lang="ca">Folk punk</skos:prefLabel>
    <skos:prefLabel xml:lang="hr">Folk punk</skos:prefLabel>
    <skos:prefLabel xml:lang="fi">Folkpunk</skos:prefLabel>
    <skos:prefLabel xml:lang="fr">Punk folk</skos:prefLabel>
    <skos:prefLabel xml:lang="de">Folk-Punk</skos:prefLabel>
    <skos:prefLabel xml:lang="it">Folk punk</skos:prefLabel>
    <skos:prefLabel xml:lang="pt">Folk-punk</skos:prefLabel>
    <skos:prefLabel xml:lang="ru">Фолк-панк</skos:prefLabel>
    <skos:prefLabel xml:lang="es">Folk punk</skos:prefLabel>
    <skos:prefLabel xml:lang="sv">Folkpunk</skos:prefLabel>
    <skos:prefLabel xml:lang="uk">Фолк-панк</skos:prefLabel>
    <skos:closeMatch rdf:resource="http://rdf.freebase.com/ns/m.05tcx0"/>
    <skos:broader rdf:resource="http://data.europeana.eu/concept/music/genre/Punk_rock_fusions"/>
    <skos:definition xml:lang="en">Folk punk is a fusion of folk music and punk rock. It was
      popularized in the early 1980s by The Pogues in Britain, and by Violent Femmes in the United
      States. Folk punk achieved some mainstream success in that decade. In more recent years, its
      subgenres Celtic punk and Gypsy punk have experienced some commercial
      success.</skos:definition>
    <skos:exactMatch xml:lang="en">http://dbpedia.org/resource/Folk_punk</skos:exactMatch>
    <skos:inScheme rdf:resource="http://data.europeana.eu/concept/music/genre/Music_Genre_Scheme"/>
    <skos:altLabel xml:lang="en">Folk punk</skos:altLabel>
  </skos:Concept>

  <skos:Concept rdf:about="http://data.europeana.eu/concept/music/genre/Samba_rock">
    <skos:prefLabel xml:lang="en">Samba rock</skos:prefLabel>
    <skos:prefLabel xml:lang="fi">Sambarock</skos:prefLabel>
    <skos:prefLabel xml:lang="hu">Szamba-rock</skos:prefLabel>
    <skos:prefLabel xml:lang="it">Samba rock</skos:prefLabel>
    <skos:prefLabel xml:lang="pt">Samba-rock</skos:prefLabel>
    <skos:closeMatch rdf:resource="http://rdf.freebase.com/ns/m.05x2qh"/>
    <skos:broader rdf:resource="http://data.europeana.eu/concept/music/genre/Pop_music_fusions"/>
    <skos:definition xml:lang="en">Samba-rock is a genre of samba and subgenre of rock. Created in
      the 1960s, the genre combines the sounds of Brazilian samba, bebop, jazz and soul. Jorge Ben
      Jor created the style with his album &quot;Bidu/Silêncio no Brooklin&quot;. After this a great
      number of artists followed Ben's beat, including Banda Black Rio and Trio
      Mocoto.</skos:definition>
    <skos:exactMatch xml:lang="en">http://dbpedia.org/resource/Samba_rock</skos:exactMatch>
    <skos:inScheme rdf:resource="http://data.europeana.eu/concept/music/genre/Music_Genre_Scheme"/>
    <skos:altLabel xml:lang="en">Samba rock</skos:altLabel>
  </skos:Concept>

  <skos:Concept rdf:about="http://data.europeana.eu/concept/music/genre/Sufi_rock">
    <skos:prefLabel xml:lang="en">Sufi rock</skos:prefLabel>
    <skos:closeMatch rdf:resource="http://rdf.freebase.com/ns/m.05xjt6"/>
    <skos:broader rdf:resource="http://data.europeana.eu/concept/music/genre/Rock_music_fusions"/>
    <skos:definition xml:lang="en">Sufi rock is a subgenre of rock music that combines rock with
      classical sufi music traditions. It emerged in the early 1990s and became widely popular in
      the late 1990s in Pakistan. The term &quot;sufi rock&quot; was coined in 1993 by writer Nadeem
      F. Paracha to define the Pakistani band, Junoon who pioneered the process of fusing
      conventional rock music with sufi music and imagery. &lt;p&gt; It is mostly based on the
      poetry of famous sufi poets like Rumi, Hafez, Faiz Ahmed Faiz, Shah Abdul Latif Bhittai,
      Bulleh Shah, Waris Shah and even Kabir and is mostly sung in languages like Urdu, Punjabi,
      Sindhi, Persian and Turkish. &lt;p&gt; A few artists like Junoon, Mekaal Hasan Band, and Laal
      have achieved commercial success and mainstream critical recognition while some veteran sufi
      folk singers such as Arif Lohar and Saeen Zahoor have also dabbled in this
      genre.</skos:definition>
    <skos:exactMatch xml:lang="en">http://dbpedia.org/resource/Sufi_rock</skos:exactMatch>
    <skos:inScheme rdf:resource="http://data.europeana.eu/concept/music/genre/Music_Genre_Scheme"/>
    <skos:altLabel xml:lang="en">Sufi rock</skos:altLabel>
  </skos:Concept>

  <skos:Concept rdf:about="http://data.europeana.eu/concept/music/genre/Dance-punk">
    <skos:prefLabel xml:lang="en">Dance-punk</skos:prefLabel>
    <skos:prefLabel xml:lang="cs">Dance-punk</skos:prefLabel>
    <skos:prefLabel xml:lang="nl">Dance-punk</skos:prefLabel>
    <skos:prefLabel xml:lang="fi">Dance-punk</skos:prefLabel>
    <skos:prefLabel xml:lang="fr">Dance-punk</skos:prefLabel>
    <skos:prefLabel xml:lang="it">Dance punk</skos:prefLabel>
    <skos:prefLabel xml:lang="ja">ダンス・パンク</skos:prefLabel>
    <skos:prefLabel xml:lang="pl">Dance-punk</skos:prefLabel>
    <skos:prefLabel xml:lang="pt">Dance-punk</skos:prefLabel>
    <skos:prefLabel xml:lang="ru">Дэнс-панк</skos:prefLabel>
    <skos:prefLabel xml:lang="sk">Dance-punk</skos:prefLabel>
    <skos:prefLabel xml:lang="es">Dance punk</skos:prefLabel>
    <skos:prefLabel xml:lang="sv">Dance-punk</skos:prefLabel>
    <skos:prefLabel xml:lang="th">แดนซ์พังก์</skos:prefLabel>
    <skos:prefLabel xml:lang="uk">Денс-панк</skos:prefLabel>
    <skos:closeMatch rdf:resource="http://rdf.freebase.com/ns/m.05y8n7"/>
    <skos:broader
      rdf:resource="http://data.europeana.eu/concept/music/genre/Electronic_rock_fusions"/>
    <skos:definition xml:lang="en">Dance-punk is a music genre that emerged in the late 1970s, and
      is closely associated with the post-punk and new wave movements.</skos:definition>
    <skos:exactMatch xml:lang="en">http://dbpedia.org/resource/Dance-punk</skos:exactMatch>
    <skos:inScheme rdf:resource="http://data.europeana.eu/concept/music/genre/Music_Genre_Scheme"/>
    <skos:altLabel xml:lang="en">Dance-punk</skos:altLabel>
  </skos:Concept>

  <skos:Concept rdf:about="http://data.europeana.eu/concept/music/genre/Comedy_rock">
    <skos:prefLabel xml:lang="en">Comedy rock</skos:prefLabel>
    <skos:prefLabel xml:lang="cs">Comedy rock</skos:prefLabel>
    <skos:prefLabel xml:lang="da">Comedy rock</skos:prefLabel>
    <skos:prefLabel xml:lang="nl">Comedyrock</skos:prefLabel>
    <skos:prefLabel xml:lang="fi">Huumorirock</skos:prefLabel>
    <skos:prefLabel xml:lang="fr">Comedy rock</skos:prefLabel>
    <skos:prefLabel xml:lang="it">Rock demenziale</skos:prefLabel>
    <skos:prefLabel xml:lang="pl">Comedy rock</skos:prefLabel>
    <skos:prefLabel xml:lang="pt">Rock cômico</skos:prefLabel>
    <skos:prefLabel xml:lang="ru">Камеди-рок</skos:prefLabel>
    <skos:prefLabel xml:lang="sk">Comedy rock</skos:prefLabel>
    <skos:prefLabel xml:lang="es">Rock cómico</skos:prefLabel>
    <skos:prefLabel xml:lang="th">คอเมดี้ร็อก</skos:prefLabel>
    <skos:closeMatch rdf:resource="http://rdf.freebase.com/ns/m.061fhg"/>
    <skos:broader rdf:resource="http://data.europeana.eu/concept/music/genre/Rock_music_fusions"/>
    <skos:definition xml:lang="en">Comedy rock is rock music mixed with comedy, often satire and
      parody.</skos:definition>
    <skos:exactMatch xml:lang="en">http://dbpedia.org/resource/Comedy_rock</skos:exactMatch>
    <skos:inScheme rdf:resource="http://data.europeana.eu/concept/music/genre/Music_Genre_Scheme"/>
    <skos:altLabel xml:lang="en">Comedy rock</skos:altLabel>
  </skos:Concept>

  <skos:Concept rdf:about="http://data.europeana.eu/concept/music/genre/Seggae">
    <skos:prefLabel xml:lang="en">Seggae</skos:prefLabel>
    <skos:prefLabel xml:lang="fr">Seggae</skos:prefLabel>
    <skos:closeMatch rdf:resource="http://rdf.freebase.com/ns/m.063ctq"/>
    <skos:broader
      rdf:resource="http://data.europeana.eu/concept/music/genre/African_popular_music_fusions"/>
    <skos:definition xml:lang="en">Seggae is a fusion genre of sega, the traditional music of the
      Mascarene Islands, and reggae. Seggae is one of the most popular music genres in
      Mauritius.</skos:definition>
    <skos:exactMatch xml:lang="en">http://dbpedia.org/resource/Seggae</skos:exactMatch>
    <skos:inScheme rdf:resource="http://data.europeana.eu/concept/music/genre/Music_Genre_Scheme"/>
    <skos:altLabel xml:lang="en">Seggae</skos:altLabel>
  </skos:Concept>

  <skos:Concept rdf:about="http://data.europeana.eu/concept/music/genre/Christian_country_music">
    <skos:prefLabel xml:lang="en">Christian country music</skos:prefLabel>
    <skos:prefLabel xml:lang="et">Kristlik kantrimuusika</skos:prefLabel>
    <skos:prefLabel xml:lang="de">Country-Gospel</skos:prefLabel>
    <skos:closeMatch rdf:resource="http://rdf.freebase.com/ns/m.064c6f"/>
    <skos:broader rdf:resource="http://data.europeana.eu/concept/music/genre/Country_music_fusions"/>
    <skos:definition xml:lang="en">Christian country music is music that is written to express
      either personal or a communal belief regarding Christian life, as well as to give a Christian
      alternative to mainstream secular music. Christian country music is a form of Christian music
      and a subgenre of both Gospel music and Country music. &lt;p&gt; Like other forms of music the
      creation, performance, significance, and even the definition of Christian country music varies
      according to culture and social context. It is composed and performed for many purposes,
      ranging from aesthetic pleasure, religious or ceremonial purposes, or as an entertainment
      product for the marketplace. However, a common theme as with most Christian music is praise,
      worship or thanks to God and/or Christ.</skos:definition>
    <skos:exactMatch xml:lang="en"
      >http://dbpedia.org/resource/Christian_country_music</skos:exactMatch>
    <skos:inScheme rdf:resource="http://data.europeana.eu/concept/music/genre/Music_Genre_Scheme"/>
    <skos:altLabel xml:lang="en">Country Gospel</skos:altLabel>
    <skos:altLabel xml:lang="en">Inspirational Country</skos:altLabel>
    <skos:altLabel xml:lang="en">Christian country music</skos:altLabel>
  </skos:Concept>

  <skos:Concept rdf:about="http://data.europeana.eu/concept/music/genre/Deathcore">
    <skos:prefLabel xml:lang="en">Deathcore</skos:prefLabel>
    <skos:prefLabel xml:lang="hr">Deathcore</skos:prefLabel>
    <skos:prefLabel xml:lang="cs">Deathcore</skos:prefLabel>
    <skos:prefLabel xml:lang="da">Deathcore</skos:prefLabel>
    <skos:prefLabel xml:lang="nl">Deathcore</skos:prefLabel>
    <skos:prefLabel xml:lang="fi">Deathcore</skos:prefLabel>
    <skos:prefLabel xml:lang="fr">Deathcore</skos:prefLabel>
    <skos:prefLabel xml:lang="de">Deathcore</skos:prefLabel>
    <skos:prefLabel xml:lang="id">Deathcore</skos:prefLabel>
    <skos:prefLabel xml:lang="it">Deathcore</skos:prefLabel>
    <skos:prefLabel xml:lang="ja">デスコア</skos:prefLabel>
    <skos:prefLabel xml:lang="ko">데스코어</skos:prefLabel>
    <skos:prefLabel xml:lang="ms">Deathcore</skos:prefLabel>
    <skos:prefLabel xml:lang="no">Deathcore</skos:prefLabel>
    <skos:prefLabel xml:lang="pl">Deathcore</skos:prefLabel>
    <skos:prefLabel xml:lang="pt">Deathcore</skos:prefLabel>
    <skos:prefLabel xml:lang="ro">Deathcore</skos:prefLabel>
    <skos:prefLabel xml:lang="ru">Дэткор</skos:prefLabel>
    <skos:prefLabel xml:lang="sk">Deathcore</skos:prefLabel>
    <skos:prefLabel xml:lang="es">Deathcore</skos:prefLabel>
    <skos:prefLabel xml:lang="sv">Deathcore</skos:prefLabel>
    <skos:prefLabel xml:lang="th">เดทคอร์</skos:prefLabel>
    <skos:prefLabel xml:lang="tr">Deathcore</skos:prefLabel>
    <skos:prefLabel xml:lang="uk">Дезкор</skos:prefLabel>
    <skos:prefLabel xml:lang="vi">Deathcore</skos:prefLabel>
    <skos:closeMatch rdf:resource="http://rdf.freebase.com/ns/m.066d03"/>
    <skos:broader
      rdf:resource="http://data.europeana.eu/concept/music/genre/Heavy_metal_music_fusions"/>
    <skos:definition xml:lang="en">Deathcore is a genre of extreme metal that combines sounds and
      characteristics of death metal with sounds and characteristics of metalcore. It is defined by
      death metal riffs, blast beats and use of metalcore breakdowns. Deathcore seems to have most
      prominence within the southwestern United States, especially Arizona and inland southern
      California, which are home to many notable bands and various festivals.</skos:definition>
    <skos:exactMatch xml:lang="en">http://dbpedia.org/resource/Deathcore</skos:exactMatch>
    <skos:inScheme rdf:resource="http://data.europeana.eu/concept/music/genre/Music_Genre_Scheme"/>
    <skos:altLabel xml:lang="en">Deathcore</skos:altLabel>
  </skos:Concept>

  <skos:Concept rdf:about="http://data.europeana.eu/concept/music/genre/Country_rap">
    <skos:prefLabel xml:lang="en">Country rap</skos:prefLabel>
    <skos:prefLabel xml:lang="fr">Country rap</skos:prefLabel>
    <skos:prefLabel xml:lang="it">Country rap</skos:prefLabel>
    <skos:prefLabel xml:lang="pt">Country rap</skos:prefLabel>
    <skos:prefLabel xml:lang="ru">Кантри-рэп</skos:prefLabel>
    <skos:prefLabel xml:lang="sk">Country rap</skos:prefLabel>
    <skos:prefLabel xml:lang="es">Country rap</skos:prefLabel>
    <skos:closeMatch rdf:resource="http://rdf.freebase.com/ns/m.067kzv"/>
    <skos:broader rdf:resource="http://data.europeana.eu/concept/music/genre/Country_music_fusions"/>
    <skos:definition xml:lang="en">Country rap is a subgenre of popular music blending country music
      with hip hop music-style rapping, also known as hick-hop or rural rap. &lt;p&gt; Country rap
      began to form as a genre when Bubba Sparxxx and producer Shannon &quot;Fat Shan&quot; Houchins
      created Sparxxx's 2001 debut album Dark Days, Bright Nights as an independent release which
      was later re-released on Interscope Records. The trend continued in 2005 when country artists
      Big &amp; Rich introduced Cowboy Troy to the country world via 2005's &quot;Loco Motive&quot;
      released on Warner Brothers, which reached #2 on Billboard's Top Country Albums chart. Coming
      off the success of Bubba Sparxxx's platinum album debut, Houchins soon after created Average
      Joes Entertainment with country rapper Colt Ford. This was the beginning of country rap taking
      its place as a real and separate genre while at the same time influencing mainstream country.
      Colt Ford has sold over 1.5 million albums including 3 that have landed in the top 10 of
      Billboard's Country Music chart. Ford's 2012 &quot;Declaration Of Independence&quot; debuted
      at #1 proving that country rap is a true genre and spawning a slew of new artists. The Lacs
      and Lenny Cooper have both sold well.</skos:definition>
    <skos:exactMatch xml:lang="en">http://dbpedia.org/resource/Country_rap</skos:exactMatch>
    <skos:inScheme rdf:resource="http://data.europeana.eu/concept/music/genre/Music_Genre_Scheme"/>
    <skos:altLabel xml:lang="en">Country rap</skos:altLabel>
  </skos:Concept>

  <skos:Concept rdf:about="http://data.europeana.eu/concept/music/genre/Country_pop">
    <skos:prefLabel xml:lang="en">Country pop</skos:prefLabel>
    <skos:prefLabel xml:lang="ca">Country-pop</skos:prefLabel>
    <skos:prefLabel xml:lang="hr">Country pop</skos:prefLabel>
    <skos:prefLabel xml:lang="et">Popkantri</skos:prefLabel>
    <skos:prefLabel xml:lang="fr">Country pop</skos:prefLabel>
    <skos:prefLabel xml:lang="it">Country pop</skos:prefLabel>
    <skos:prefLabel xml:lang="ko">컨트리 팝</skos:prefLabel>
    <skos:prefLabel xml:lang="pt">Country pop</skos:prefLabel>
    <skos:prefLabel xml:lang="ru">Кантри-поп</skos:prefLabel>
    <skos:prefLabel xml:lang="es">Country pop</skos:prefLabel>
    <skos:prefLabel xml:lang="sv">Countrypop</skos:prefLabel>
    <skos:prefLabel xml:lang="th">คันทรี ป็อป</skos:prefLabel>
    <skos:prefLabel xml:lang="tr">Country pop</skos:prefLabel>
    <skos:prefLabel xml:lang="uk">Кантрі-поп</skos:prefLabel>
    <skos:closeMatch rdf:resource="http://rdf.freebase.com/ns/m.06924p"/>
    <skos:broader rdf:resource="http://data.europeana.eu/concept/music/genre/Country_music_fusions"/>
    <skos:definition xml:lang="en">Country pop, with roots in both the countrypolitan sound and in
      soft rock, is a subgenre of country music and pop music that first emerged in the 1970s.
      Although the term first referred to country music songs and artists that crossed over to Top
      40 radio, country pop acts are now more likely to cross over to adult
      contemporary.</skos:definition>
    <skos:exactMatch xml:lang="en">http://dbpedia.org/resource/Country_pop</skos:exactMatch>
    <skos:inScheme rdf:resource="http://data.europeana.eu/concept/music/genre/Music_Genre_Scheme"/>
    <skos:altLabel xml:lang="en">Country pop</skos:altLabel>
  </skos:Concept>

  <skos:Concept rdf:about="http://data.europeana.eu/concept/music/genre/Minimal_techno">
    <skos:prefLabel xml:lang="en">Minimal techno</skos:prefLabel>
    <skos:prefLabel xml:lang="cs">Minimal Techno</skos:prefLabel>
    <skos:prefLabel xml:lang="nl">Minimal techno</skos:prefLabel>
    <skos:prefLabel xml:lang="fi">Minimal techno</skos:prefLabel>
    <skos:prefLabel xml:lang="fr">Techno minimale</skos:prefLabel>
    <skos:prefLabel xml:lang="de">Minimal Techno</skos:prefLabel>
    <skos:prefLabel xml:lang="it">Minimal techno</skos:prefLabel>
    <skos:prefLabel xml:lang="pl">Minimal techno</skos:prefLabel>
    <skos:prefLabel xml:lang="pt">Minimal techno</skos:prefLabel>
    <skos:prefLabel xml:lang="ro">Minimal</skos:prefLabel>
    <skos:prefLabel xml:lang="ru">Минимал-техно</skos:prefLabel>
    <skos:prefLabel xml:lang="sk">Minimal techno</skos:prefLabel>
    <skos:prefLabel xml:lang="es">Minimal techno</skos:prefLabel>
    <skos:prefLabel xml:lang="sv">Minimal</skos:prefLabel>
    <skos:prefLabel xml:lang="uk">Мінімал-техно</skos:prefLabel>
    <skos:closeMatch rdf:resource="http://rdf.freebase.com/ns/m.06953q"/>
    <skos:broader rdf:resource="http://data.europeana.eu/concept/music/genre/Techno_fusions"/>
    <skos:definition xml:lang="en">Minimal techno is a minimalist sub-genre of techno. It is
      characterized by a stripped-down aesthetic that exploits the use of repetition, and
      understated development. Minimal techno is thought to have been originally developed in the
      early 1990s by Detroit-based producers Robert Hood and Daniel Bell. By the early 2000s the
      term 'minimal' generally described a style of techno that was popularised in Germany by labels
      such as Kompakt, Perlon, and Richie Hawtin's M-nus, amongst others.</skos:definition>
    <skos:exactMatch xml:lang="en">http://dbpedia.org/resource/Minimal_techno</skos:exactMatch>
    <skos:inScheme rdf:resource="http://data.europeana.eu/concept/music/genre/Music_Genre_Scheme"/>
    <skos:altLabel xml:lang="en">Minimal techno</skos:altLabel>
  </skos:Concept>

  <skos:Concept rdf:about="http://data.europeana.eu/concept/music/genre/Groove_metal">
    <skos:prefLabel xml:lang="en">Groove metal</skos:prefLabel>
    <skos:prefLabel xml:lang="bg">Груув метъл</skos:prefLabel>
    <skos:prefLabel xml:lang="ca">Groove metal</skos:prefLabel>
    <skos:prefLabel xml:lang="hr">Groove metal</skos:prefLabel>
    <skos:prefLabel xml:lang="cs">Groove metal</skos:prefLabel>
    <skos:prefLabel xml:lang="da">Groove metal</skos:prefLabel>
    <skos:prefLabel xml:lang="nl">Groovemetal</skos:prefLabel>
    <skos:prefLabel xml:lang="fr">Groove metal</skos:prefLabel>
    <skos:prefLabel xml:lang="de">Groove Metal</skos:prefLabel>
    <skos:prefLabel xml:lang="el">Groove Metal</skos:prefLabel>
    <skos:prefLabel xml:lang="hu">Groove metal</skos:prefLabel>
    <skos:prefLabel xml:lang="id">Groove Metal</skos:prefLabel>
    <skos:prefLabel xml:lang="it">Groove metal</skos:prefLabel>
    <skos:prefLabel xml:lang="ko">그루브 메탈</skos:prefLabel>
    <skos:prefLabel xml:lang="no">Groove metal</skos:prefLabel>
    <skos:prefLabel xml:lang="fa">گروو متال</skos:prefLabel>
    <skos:prefLabel xml:lang="pl">Groove metal</skos:prefLabel>
    <skos:prefLabel xml:lang="pt">Groove metal</skos:prefLabel>
    <skos:prefLabel xml:lang="ro">Groove metal</skos:prefLabel>
    <skos:prefLabel xml:lang="ru">Грув-метал</skos:prefLabel>
    <skos:prefLabel xml:lang="sk">Groove metal</skos:prefLabel>
    <skos:prefLabel xml:lang="es">Groove metal</skos:prefLabel>
    <skos:prefLabel xml:lang="sv">Groove metal</skos:prefLabel>
    <skos:prefLabel xml:lang="tr">Groove metal</skos:prefLabel>
    <skos:prefLabel xml:lang="uk">Грув-метал</skos:prefLabel>
    <skos:prefLabel xml:lang="vi">Groove metal</skos:prefLabel>
    <skos:closeMatch rdf:resource="http://rdf.freebase.com/ns/m.06bpt_"/>
    <skos:broader
      rdf:resource="http://data.europeana.eu/concept/music/genre/Heavy_metal_music_fusions"/>
    <skos:definition xml:lang="en">Groove metal is a subgenre of heavy metal. It is often used to
      describe Pantera and Exhorder. At its core, groove metal takes the intensity and sonic
      qualities of thrash metal and plays it at a mid-tempo, with most bands making only occasional
      forays into fast tempo.</skos:definition>
    <skos:exactMatch xml:lang="en">http://dbpedia.org/resource/Groove_metal</skos:exactMatch>
    <skos:inScheme rdf:resource="http://data.europeana.eu/concept/music/genre/Music_Genre_Scheme"/>
    <skos:altLabel xml:lang="en">Groove metal</skos:altLabel>
  </skos:Concept>

  <skos:Concept rdf:about="http://data.europeana.eu/concept/music/genre/Rapcore">
    <skos:prefLabel xml:lang="en">Rapcore</skos:prefLabel>
    <skos:prefLabel xml:lang="ar">راب كور</skos:prefLabel>
    <skos:prefLabel xml:lang="bg">Рап кор</skos:prefLabel>
    <skos:prefLabel xml:lang="ca">Rapcore</skos:prefLabel>
    <skos:prefLabel xml:lang="cs">Rapcore</skos:prefLabel>
    <skos:prefLabel xml:lang="da">Rap metal</skos:prefLabel>
    <skos:prefLabel xml:lang="nl">Rapcore</skos:prefLabel>
    <skos:prefLabel xml:lang="fi">Rapcore</skos:prefLabel>
    <skos:prefLabel xml:lang="fr">Rapcore</skos:prefLabel>
    <skos:prefLabel xml:lang="it">Rapcore</skos:prefLabel>
    <skos:prefLabel xml:lang="ja">ラップメタル</skos:prefLabel>
    <skos:prefLabel xml:lang="ko">랩코어</skos:prefLabel>
    <skos:prefLabel xml:lang="lv">Repkors</skos:prefLabel>
    <skos:prefLabel xml:lang="lt">Rapcore</skos:prefLabel>
    <skos:prefLabel xml:lang="pl">Rapcore</skos:prefLabel>
    <skos:prefLabel xml:lang="pt">Rapcore</skos:prefLabel>
    <skos:prefLabel xml:lang="ro">Rapcore</skos:prefLabel>
    <skos:prefLabel xml:lang="ru">Рэпкор</skos:prefLabel>
    <skos:prefLabel xml:lang="sr">Repkor</skos:prefLabel>
    <skos:prefLabel xml:lang="sk">Rapcore</skos:prefLabel>
    <skos:prefLabel xml:lang="es">Rapcore</skos:prefLabel>
    <skos:prefLabel xml:lang="sv">Rapcore</skos:prefLabel>
    <skos:prefLabel xml:lang="tr">Rapcore</skos:prefLabel>
    <skos:prefLabel xml:lang="uk">Репкор</skos:prefLabel>
    <skos:prefLabel xml:lang="vi">Rapcore</skos:prefLabel>
    <skos:closeMatch rdf:resource="http://rdf.freebase.com/ns/m.06cp5"/>
    <skos:broader rdf:resource="http://data.europeana.eu/concept/music/genre/Rock_music_fusions"/>
    <skos:definition xml:lang="en">Rapcore is a subgenre of rap rock fusing vocal and sometimes
      instrumental elements of hip hop with punk rock.</skos:definition>
    <skos:exactMatch xml:lang="en">http://dbpedia.org/resource/Rapcore</skos:exactMatch>
    <skos:inScheme rdf:resource="http://data.europeana.eu/concept/music/genre/Music_Genre_Scheme"/>
    <skos:altLabel xml:lang="en">Rapcore</skos:altLabel>
  </skos:Concept>

  <skos:Concept rdf:about="http://data.europeana.eu/concept/music/genre/Ragga">
    <skos:prefLabel xml:lang="en">Ragga</skos:prefLabel>
    <skos:prefLabel xml:lang="bg">Рага</skos:prefLabel>
    <skos:prefLabel xml:lang="ca">Ragga</skos:prefLabel>
    <skos:prefLabel xml:lang="cs">Raggamuffin</skos:prefLabel>
    <skos:prefLabel xml:lang="fi">Raggamuffin</skos:prefLabel>
    <skos:prefLabel xml:lang="fr">Ragga</skos:prefLabel>
    <skos:prefLabel xml:lang="de">Ragga</skos:prefLabel>
    <skos:prefLabel xml:lang="hu">Ragga</skos:prefLabel>
    <skos:prefLabel xml:lang="id">Ragga</skos:prefLabel>
    <skos:prefLabel xml:lang="it">Raggamuffin</skos:prefLabel>
    <skos:prefLabel xml:lang="ja">ラガマフィン</skos:prefLabel>
    <skos:prefLabel xml:lang="pl">Ragga</skos:prefLabel>
    <skos:prefLabel xml:lang="pt">Ragga</skos:prefLabel>
    <skos:prefLabel xml:lang="ro">Ragga</skos:prefLabel>
    <skos:prefLabel xml:lang="ru">Рагга</skos:prefLabel>
    <skos:prefLabel xml:lang="sk">Raggamuffin</skos:prefLabel>
    <skos:prefLabel xml:lang="es">Raggamuffin</skos:prefLabel>
    <skos:prefLabel xml:lang="sv">Ragga</skos:prefLabel>
    <skos:prefLabel xml:lang="th">รักก้า</skos:prefLabel>
    <skos:closeMatch rdf:resource="http://rdf.freebase.com/ns/m.06czq"/>
    <skos:broader rdf:resource="http://data.europeana.eu/concept/music/genre/Hip_hop_music_fusions"/>
    <skos:definition xml:lang="en">Raggamuffin music, usually abbreviated as ragga, is a sub-genre
      of dancehall music or reggae, in which the instrumentation primarily consists of electronic
      music. Similar to hip hop, sampling often serves a prominent role in raggamuffin music.
      &lt;p&gt; In the mid-1980s, French Antilles Kassav, the first in the Caribbean to use MIDI
      technology, took Caribbean music to another level by recording in a digital format. Wayne
      Smith's &quot;Under Me Sleng Teng&quot; was produced by King Jammy in 1985 on a Casio MT-40
      synthesizer and is generally recognized as the seminal ragga song. &quot;Sleng Teng&quot;
      boosted Jammy's popularity immensely, and other producers quickly released their own versions
      of the riddim, accompanied by dozens of different vocalists. &lt;p&gt; Ragga is now mainly
      used as a synonym for dancehall reggae or for describing dancehall with a deejay chatting
      rather than singjaying or singing on top of the riddim.</skos:definition>
    <skos:exactMatch xml:lang="en">http://dbpedia.org/resource/Ragga</skos:exactMatch>
    <skos:inScheme rdf:resource="http://data.europeana.eu/concept/music/genre/Music_Genre_Scheme"/>
    <skos:altLabel xml:lang="en">Ragga</skos:altLabel>
  </skos:Concept>

  <skos:Concept rdf:about="http://data.europeana.eu/concept/music/genre/Low_Bap">
    <skos:prefLabel xml:lang="en">Low Bap</skos:prefLabel>
    <skos:prefLabel xml:lang="fr">Low bap</skos:prefLabel>
    <skos:prefLabel xml:lang="el">Low Bap</skos:prefLabel>
    <skos:prefLabel xml:lang="es">Low Bap</skos:prefLabel>
    <skos:closeMatch rdf:resource="http://rdf.freebase.com/ns/m.06d4nn"/>
    <skos:broader rdf:resource="http://data.europeana.eu/concept/music/genre/Hip_hop_music_fusions"/>
    <skos:definition xml:lang="en">Low Bap is a sub-genre of the Greek hip hop music scene, that
      emerged in the mid-1990s as the sound of the prominent Greek hip hop group Active Member. It's
      characterized by slower tempo and rapping than usual, often combined with lyrics of political
      content. The words &quot;Low Bap&quot; don't have a specific meaning, they merely represent a
      perspective on life, society and politics that people in the movement have. The Low Bap
      movement has been expanded, so that today it includes bookstores, youth centers and
      specialized magazines. Cinematic attempts, concerts, and festivals have also taken place in an
      effort to broaden the scope of the movement, and introduce new bands to the genre's range of
      followers.</skos:definition>
    <skos:exactMatch xml:lang="en">http://dbpedia.org/resource/Low_Bap</skos:exactMatch>
    <skos:inScheme rdf:resource="http://data.europeana.eu/concept/music/genre/Music_Genre_Scheme"/>
    <skos:altLabel xml:lang="en">Low Bap</skos:altLabel>
  </skos:Concept>

  <skos:Concept rdf:about="http://data.europeana.eu/concept/music/genre/Chopped_and_screwed">
    <skos:prefLabel xml:lang="en">Chopped and screwed</skos:prefLabel>
    <skos:prefLabel xml:lang="nl">Screwed &amp; chopped</skos:prefLabel>
    <skos:prefLabel xml:lang="fi">Chopped and Screwed</skos:prefLabel>
    <skos:prefLabel xml:lang="fr">Chopped and screwed</skos:prefLabel>
    <skos:prefLabel xml:lang="de">Screw</skos:prefLabel>
    <skos:prefLabel xml:lang="it">Chopped and screwed</skos:prefLabel>
    <skos:prefLabel xml:lang="es">Chopped and screwed</skos:prefLabel>
    <skos:prefLabel xml:lang="sv">Screw</skos:prefLabel>
    <skos:closeMatch rdf:resource="http://rdf.freebase.com/ns/m.06h87z"/>
    <skos:broader rdf:resource="http://data.europeana.eu/concept/music/genre/Hip_hop_music_fusions"/>
    <skos:definition xml:lang="en">Chopped and screwed refers to a technique of remixing hip hop
      music which developed in the Houston hip hop scene in the 1990s. This is accomplished by
      slowing the tempo down to between 60 and 70 quarter-note beats per minute and applying
      techniques such as skipping beats, record scratching, stop-time, and affecting portions of the
      music to make a &quot;chopped-up&quot; version of the original. DJ Screw is largely recognized
      as the innovator behind the chopped and screwed genre. DJ Screw's key technique involved
      playing the same record on both turntables with a delay between them of one beat, and quickly
      moving the crossfader side to side. This created an effect where words or sounds would be
      repeated in the music but would still keep the tempo going. A subgenre called ChopNotSlop
      created by OG Ron C has gotten major attention via Drake's Take Care album and the Houston
      music scene started by SUC</skos:definition>
    <skos:exactMatch xml:lang="en">http://dbpedia.org/resource/Chopped_and_screwed</skos:exactMatch>
    <skos:inScheme rdf:resource="http://data.europeana.eu/concept/music/genre/Music_Genre_Scheme"/>
    <skos:altLabel xml:lang="en">screwed and chopped</skos:altLabel>
    <skos:altLabel xml:lang="en">slowed and throwed</skos:altLabel>
    <skos:altLabel xml:lang="en">Chopped and screwed</skos:altLabel>
  </skos:Concept>

  <skos:Concept rdf:about="http://data.europeana.eu/concept/music/genre/Hardstep">
    <skos:prefLabel xml:lang="en">Hardstep</skos:prefLabel>
    <skos:prefLabel xml:lang="cs">Hardstep</skos:prefLabel>
    <skos:prefLabel xml:lang="fa">هارد استپ</skos:prefLabel>
    <skos:prefLabel xml:lang="pl">Hardstep</skos:prefLabel>
    <skos:prefLabel xml:lang="pt">Hardstep</skos:prefLabel>
    <skos:prefLabel xml:lang="ru">Хардстеп</skos:prefLabel>
    <skos:prefLabel xml:lang="sk">Hardstep</skos:prefLabel>
    <skos:prefLabel xml:lang="es">Hardstep</skos:prefLabel>
    <skos:closeMatch rdf:resource="http://rdf.freebase.com/ns/m.06hljn"/>
    <skos:broader
      rdf:resource="http://data.europeana.eu/concept/music/genre/Electronic_music_fusions"/>
    <skos:definition xml:lang="en">Hardstep is a subgenre of drum and bass which emerged in 1994. It
      is characterised by a gritty production style, that has an inner-city feel to it. The breaks
      are less cut-up sounding rather than oldschool jungle, and have faster and harder simple
      electronic melodies. One characteristic is an accentuated, yet sparse percussive beat.
      &lt;p&gt; The genre found favour with junglists, despite being overtaken in popularity by
      techstep, the fans of the style still remain. Nowadays, hardstep is particularly popular in
      the North American drum and bass scene, with artist like Evol Intent, Ewun and Dieselboy.
      Earlier Hardstep artists include DJ Hype and DJ Zinc.</skos:definition>
    <skos:exactMatch xml:lang="en">http://dbpedia.org/resource/Hardstep</skos:exactMatch>
    <skos:inScheme rdf:resource="http://data.europeana.eu/concept/music/genre/Music_Genre_Scheme"/>
    <skos:altLabel xml:lang="en">Hardstep</skos:altLabel>
  </skos:Concept>

  <skos:Concept rdf:about="http://data.europeana.eu/concept/music/genre/Punk_blues">
    <skos:prefLabel xml:lang="en">Punk blues</skos:prefLabel>
    <skos:prefLabel xml:lang="fr">Punk blues</skos:prefLabel>
    <skos:prefLabel xml:lang="it">Punk blues</skos:prefLabel>
    <skos:prefLabel xml:lang="pl">Punk blues</skos:prefLabel>
    <skos:prefLabel xml:lang="pt">Punk blues</skos:prefLabel>
    <skos:prefLabel xml:lang="es">Punk blues</skos:prefLabel>
    <skos:closeMatch rdf:resource="http://rdf.freebase.com/ns/m.06hzq3"/>
    <skos:broader rdf:resource="http://data.europeana.eu/concept/music/genre/Blues_fusions"/>
    <skos:definition xml:lang="en">Punk blues denotes a fusion genre of punk rock and blues. Punk
      blues musicians and bands usually incorporate elements of related styles, such as protopunk
      and blues rock. Its origins lie strongly within the garage rock sound of the 1960s and 1970s.
      &lt;p&gt; Punk blues can be said to favor the common rawness, simplicity and emotion shared
      between the punk and blues genres. Chet Weise, singer/guitarist of The Immortal Lee County
      Killers stated, &quot;Punk and blues are both honest reactions to life. It's blues, it's our
      blues. It's just a bit turned up and a bit faster.&quot;</skos:definition>
    <skos:exactMatch xml:lang="en">http://dbpedia.org/resource/Punk_blues</skos:exactMatch>
    <skos:inScheme rdf:resource="http://data.europeana.eu/concept/music/genre/Music_Genre_Scheme"/>
    <skos:altLabel xml:lang="en">Punk blues</skos:altLabel>
  </skos:Concept>

  <skos:Concept rdf:about="http://data.europeana.eu/concept/music/genre/Euro_disco">
    <skos:prefLabel xml:lang="en">Euro disco</skos:prefLabel>
    <skos:prefLabel xml:lang="bg">Евро-диско</skos:prefLabel>
    <skos:prefLabel xml:lang="ca">Eurodisco</skos:prefLabel>
    <skos:prefLabel xml:lang="cs">Euro disco</skos:prefLabel>
    <skos:prefLabel xml:lang="de">Euro Disco</skos:prefLabel>
    <skos:prefLabel xml:lang="el">Eurodisco</skos:prefLabel>
    <skos:prefLabel xml:lang="fa">یورو دیسکو</skos:prefLabel>
    <skos:prefLabel xml:lang="pl">Euro disco</skos:prefLabel>
    <skos:prefLabel xml:lang="pt">Euro Disco</skos:prefLabel>
    <skos:prefLabel xml:lang="ru">Евродиско</skos:prefLabel>
    <skos:prefLabel xml:lang="sk">Euro disco</skos:prefLabel>
    <skos:prefLabel xml:lang="es">Eurodisco</skos:prefLabel>
    <skos:prefLabel xml:lang="sv">Eurodisco</skos:prefLabel>
    <skos:prefLabel xml:lang="tr">Euro disco</skos:prefLabel>
    <skos:prefLabel xml:lang="uk">Євродиско</skos:prefLabel>
    <skos:closeMatch rdf:resource="http://rdf.freebase.com/ns/m.06jjbp"/>
    <skos:broader rdf:resource="http://data.europeana.eu/concept/music/genre/Pop_music_fusions"/>
    <skos:definition xml:lang="en">Euro disco is the variety of European forms of electronic dance
      music that first originated from disco in the 1970s, incorporating elements of pop, new wave
      and rock into a disco-like continuous dance atmosphere. Many Euro disco compositions feature
      lyrics sung in English, although the singers often share a different mother tongue. &lt;p&gt;
      Euro disco derivatives generally include Europop and Eurodance, with the most prominent
      subgenres being space disco of the late 1970s and Italo disco of the early 1980s. The genre
      has declined in popularity after 1985 in preference to synth rock and Hi-NRG, with a small
      revival of Italo disco in the late 1990s.</skos:definition>
    <skos:exactMatch xml:lang="en">http://dbpedia.org/resource/Euro_disco</skos:exactMatch>
    <skos:inScheme rdf:resource="http://data.europeana.eu/concept/music/genre/Music_Genre_Scheme"/>
    <skos:altLabel xml:lang="en">Euro disco</skos:altLabel>
  </skos:Concept>

  <skos:Concept rdf:about="http://data.europeana.eu/concept/music/genre/Hyphy">
    <skos:prefLabel xml:lang="en">Hyphy</skos:prefLabel>
    <skos:prefLabel xml:lang="fr">Hyphy</skos:prefLabel>
    <skos:prefLabel xml:lang="pt">Hyphy</skos:prefLabel>
    <skos:prefLabel xml:lang="ru">Хайфи</skos:prefLabel>
    <skos:prefLabel xml:lang="uk">Гайфі</skos:prefLabel>
    <skos:closeMatch rdf:resource="http://rdf.freebase.com/ns/m.06kcjr"/>
    <skos:broader rdf:resource="http://data.europeana.eu/concept/music/genre/Hip_hop_music_fusions"/>
    <skos:definition xml:lang="en">The word hyphy is San Francisco Bay Area slang meaning
      &quot;hyperactive.&quot; More specifically it is an adjective that describes the music and the
      urban culture associated with that area. It was created by Oakland-based rapper Keak da Sneak
      when he used the term on an album he recorded in 1994. The hyphy culture began to emerge in
      the late 1990s and early 2000s as a response from Bay Area rappers against commercial hip hop
      for not acknowledging their region for setting trends in the hip hop industry. It is
      distinguished by gritty, pounding rhythms, and in this sense can be associated with San
      Francisco Bay as crunk music is to the Southern United States. An individual is said to
      &quot;get hyphy&quot; when they dance in an overstated, fast paced and ridiculous manner, or
      if they get overly loud with other people. The phrase &quot;to get hyphy&quot; is similar to
      the southern phrase &quot;to get crunk&quot;. Those who consider themselves part of the hyphy
      movement strive for this behavior. &lt;p&gt; Although the &quot;hyphy movement&quot; has just
      recently seen light in mainstream America, it has been a long standing and ever evolving
      culture in the Bay Area since the early 1990s.</skos:definition>
    <skos:exactMatch xml:lang="en">http://dbpedia.org/resource/Hyphy</skos:exactMatch>
    <skos:inScheme rdf:resource="http://data.europeana.eu/concept/music/genre/Music_Genre_Scheme"/>
    <skos:altLabel xml:lang="en">Hyphy</skos:altLabel>
  </skos:Concept>

  <skos:Concept rdf:about="http://data.europeana.eu/concept/music/genre/Progressive_country">
    <skos:prefLabel xml:lang="en">Progressive country</skos:prefLabel>
    <skos:prefLabel xml:lang="it">Progressive country</skos:prefLabel>
    <skos:closeMatch rdf:resource="http://rdf.freebase.com/ns/m.06rlrn"/>
    <skos:broader rdf:resource="http://data.europeana.eu/concept/music/genre/Country_music_fusions"/>
    <skos:definition xml:lang="en">Progressive country is a subgenre of country music developed in
      the early 1970s. In the late 1960s and early 1970s, mainstream country music was dominated by
      the slick Nashville sound and the rock-influenced Bakersfield sound of artists like Merle
      Haggard. A new generation of country artists emerged, influenced by contemporary rock music,
      singer-songwriters such as Bob Dylan, and the liberal politics of the 1960s counterculture.
      &lt;p&gt; Progressive country was a songwriter-based movement and many key artists had
      previously seen success writing for other artists in Nashville, writing for themselves, they
      were more concerned with expanding country music than creating hits. Foremost among these
      artists was Willie Nelson, who returned to Texas after deciding to focus on performing his own
      songs. Nelson soon attained a wide following and inspired other artists in Texas and
      Nashville. &lt;p&gt; By the mid-1970s, progressive country artists entered the mainstream,
      usually in the form of cover versions by other artists. Progressive country also provided the
      basis for outlaw country, a harder-edged, more rock-oriented variant that achieved wide
      success in the late 1970s, as well as cowpunk and alternative country artists in the 1980s
      through today.</skos:definition>
    <skos:exactMatch xml:lang="en">http://dbpedia.org/resource/Progressive_country</skos:exactMatch>
    <skos:inScheme rdf:resource="http://data.europeana.eu/concept/music/genre/Music_Genre_Scheme"/>
    <skos:altLabel xml:lang="en">Progressive country</skos:altLabel>
  </skos:Concept>

  <skos:Concept rdf:about="http://data.europeana.eu/concept/music/genre/Trip_hop">
    <skos:prefLabel xml:lang="en">Trip hop</skos:prefLabel>
    <skos:prefLabel xml:lang="bg">Трип-хоп</skos:prefLabel>
    <skos:prefLabel xml:lang="ca">Trip hop</skos:prefLabel>
    <skos:prefLabel xml:lang="hr">Trip hop</skos:prefLabel>
    <skos:prefLabel xml:lang="cs">Trip hop</skos:prefLabel>
    <skos:prefLabel xml:lang="da">Trip hop</skos:prefLabel>
    <skos:prefLabel xml:lang="nl">Triphop</skos:prefLabel>
    <skos:prefLabel xml:lang="fi">Trip hop</skos:prefLabel>
    <skos:prefLabel xml:lang="fr">Trip hop</skos:prefLabel>
    <skos:prefLabel xml:lang="de">Trip-Hop</skos:prefLabel>
    <skos:prefLabel xml:lang="el">Τριπ χοπ</skos:prefLabel>
    <skos:prefLabel xml:lang="it">Trip hop</skos:prefLabel>
    <skos:prefLabel xml:lang="ja">トリップ・ホップ</skos:prefLabel>
    <skos:prefLabel xml:lang="lv">Triphops</skos:prefLabel>
    <skos:prefLabel xml:lang="lt">Trip-hop</skos:prefLabel>
    <skos:prefLabel xml:lang="no">Trip hop</skos:prefLabel>
    <skos:prefLabel xml:lang="fa">تریپ هاپ</skos:prefLabel>
    <skos:prefLabel xml:lang="pl">Trip hop</skos:prefLabel>
    <skos:prefLabel xml:lang="pt">Trip hop</skos:prefLabel>
    <skos:prefLabel xml:lang="ro">Muzică trip hop</skos:prefLabel>
    <skos:prefLabel xml:lang="ru">Трип-хоп</skos:prefLabel>
    <skos:prefLabel xml:lang="sr">Трип хоп</skos:prefLabel>
    <skos:prefLabel xml:lang="sk">Trip-hop</skos:prefLabel>
    <skos:prefLabel xml:lang="sl">Trip hop</skos:prefLabel>
    <skos:prefLabel xml:lang="es">Trip hop</skos:prefLabel>
    <skos:prefLabel xml:lang="sv">Triphop</skos:prefLabel>
    <skos:prefLabel xml:lang="th">ทริปฮอป</skos:prefLabel>
    <skos:prefLabel xml:lang="tr">Trip hop</skos:prefLabel>
    <skos:prefLabel xml:lang="uk">Тріп-хоп</skos:prefLabel>
    <skos:closeMatch rdf:resource="http://rdf.freebase.com/ns/m.07d2d"/>
    <skos:broader
      rdf:resource="http://data.europeana.eu/concept/music/genre/Electronic_music_fusions"/>
    <skos:definition xml:lang="en">Trip hop is a genre of electronic music that originated in the
      early 1990s in the United Kingdom, especially Bristol. Deriving from &quot;post&quot;-acid
      house, the term was first used by the British music media and press as a way to describe the
      more experimental variant of breakbeat which contained influences of soul, funk and jazz. It
      has been described as &quot;Europe's alternative choice in the second half of the '90s&quot;,
      and &quot;a fusion of hip hop and electronica until neither genre is recognisable.&quot; Trip
      hop music fuses several styles and has much in common with other genres, it has several
      qualities similar to ambient music and its drum-based breakdowns share characteristics with
      hip hop. It also contains elements of R&amp;B, dub and house, as well as other electronic
      music. Trip hop can be highly experimental in nature.</skos:definition>
    <skos:exactMatch xml:lang="en">http://dbpedia.org/resource/Trip_hop</skos:exactMatch>
    <skos:inScheme rdf:resource="http://data.europeana.eu/concept/music/genre/Music_Genre_Scheme"/>
    <skos:altLabel xml:lang="en">Trip hop</skos:altLabel>
  </skos:Concept>

  <skos:Concept rdf:about="http://data.europeana.eu/concept/music/genre/Jazz_blues">
    <skos:prefLabel xml:lang="en">Twelve-bar blues</skos:prefLabel>
    <skos:prefLabel xml:lang="nl">Bluesschema</skos:prefLabel>
    <skos:prefLabel xml:lang="fi">Blueskaava</skos:prefLabel>
    <skos:prefLabel xml:lang="de">Blues#Das Blues-Schema</skos:prefLabel>
    <skos:prefLabel xml:lang="it">Blues in 12 misure</skos:prefLabel>
    <skos:prefLabel xml:lang="ja">ブルース形式</skos:prefLabel>
    <skos:prefLabel xml:lang="no">Tolvtakters blues</skos:prefLabel>
    <skos:prefLabel xml:lang="es">Blues de doce compases</skos:prefLabel>
    <skos:prefLabel xml:lang="sv">Bluestolva</skos:prefLabel>
    <skos:prefLabel xml:lang="uk">Блюзовий період</skos:prefLabel>
    <skos:closeMatch rdf:resource="http://rdf.freebase.com/ns/m.07jgr"/>
    <skos:broader rdf:resource="http://data.europeana.eu/concept/music/genre/Blues_fusions"/>
    <skos:definition xml:lang="en">The 12-bar blues or blues changes is one of the most prominent
      chord progressions in popular music. The blues progression has a distinctive form in lyrics,
      phrase, chord structure, and duration. In its basic form, it is predominantly based on the
      I-IV-V chords of a key. &lt;p&gt; The blues can be played in any key. Mastery of the blues and
      rhythm changes are &quot;critical elements for building a jazz
      repertoire&quot;.</skos:definition>
    <skos:exactMatch xml:lang="en">http://dbpedia.org/resource/Jazz_blues</skos:exactMatch>
    <skos:inScheme rdf:resource="http://data.europeana.eu/concept/music/genre/Music_Genre_Scheme"/>
    <skos:altLabel xml:lang="en">Twelve bar blues</skos:altLabel>
    <skos:altLabel xml:lang="en">Twelve-bar blues</skos:altLabel>
  </skos:Concept>

  <skos:Concept rdf:about="http://data.europeana.eu/concept/music/genre/Trance_music">
    <skos:prefLabel xml:lang="en">Trance music</skos:prefLabel>
    <skos:prefLabel xml:lang="ar">ترانس</skos:prefLabel>
    <skos:prefLabel xml:lang="bg">Транс музика</skos:prefLabel>
    <skos:prefLabel xml:lang="ca">Trance</skos:prefLabel>
    <skos:prefLabel xml:lang="hr">Trance</skos:prefLabel>
    <skos:prefLabel xml:lang="cs">Trance</skos:prefLabel>
    <skos:prefLabel xml:lang="da">Trance</skos:prefLabel>
    <skos:prefLabel xml:lang="nl">Trance</skos:prefLabel>
    <skos:prefLabel xml:lang="et">Trance</skos:prefLabel>
    <skos:prefLabel xml:lang="fi">Trance</skos:prefLabel>
    <skos:prefLabel xml:lang="fr">Trance</skos:prefLabel>
    <skos:prefLabel xml:lang="de">Trance</skos:prefLabel>
    <skos:prefLabel xml:lang="el">Trance</skos:prefLabel>
    <skos:prefLabel xml:lang="hi">ट्रान्स संगीत</skos:prefLabel>
    <skos:prefLabel xml:lang="hu">Trance</skos:prefLabel>
    <skos:prefLabel xml:lang="id">Musik Trance</skos:prefLabel>
    <skos:prefLabel xml:lang="it">Trance</skos:prefLabel>
    <skos:prefLabel xml:lang="ja">トランス</skos:prefLabel>
    <skos:prefLabel xml:lang="ko">트랜스 음악</skos:prefLabel>
    <skos:prefLabel xml:lang="lv">Transs</skos:prefLabel>
    <skos:prefLabel xml:lang="lt">Trance muzika</skos:prefLabel>
    <skos:prefLabel xml:lang="no">Trance</skos:prefLabel>
    <skos:prefLabel xml:lang="fa">موسیقی ترنس</skos:prefLabel>
    <skos:prefLabel xml:lang="pl">Trance</skos:prefLabel>
    <skos:prefLabel xml:lang="pt">Trance</skos:prefLabel>
    <skos:prefLabel xml:lang="ro">Trance</skos:prefLabel>
    <skos:prefLabel xml:lang="ru">Транс</skos:prefLabel>
    <skos:prefLabel xml:lang="sr">Тренс</skos:prefLabel>
    <skos:prefLabel xml:lang="sk">Trance</skos:prefLabel>
    <skos:prefLabel xml:lang="sl">Trance</skos:prefLabel>
    <skos:prefLabel xml:lang="es">Trance</skos:prefLabel>
    <skos:prefLabel xml:lang="sv">Trance</skos:prefLabel>
    <skos:prefLabel xml:lang="th">แทรนซ์</skos:prefLabel>
    <skos:prefLabel xml:lang="tr">Trance müzik</skos:prefLabel>
    <skos:prefLabel xml:lang="uk">Транс</skos:prefLabel>
    <skos:closeMatch rdf:resource="http://rdf.freebase.com/ns/m.07lnk"/>
    <skos:broader
      rdf:resource="http://data.europeana.eu/concept/music/genre/Electronic_music_fusions"/>
    <skos:definition xml:lang="en">Trance is a genre of electronic dance music that developed in the
      1990s in Germany. It is characterized by a tempo of between 125 and mid 160 beats per minute,
      repeating melodic phrases, and a musical form that builds up and down throughout a track.
      Trance is a genre on its own, but also will include other styles of electronic music such as
      techno, house, pop, chill-out, classical music, and film music. &lt;p&gt; A trance refers to a
      state of hypnotism and lessened consciousness. This drifting sensation is portrayed in the
      genre by mixing many layers and rhythms to create build and release. For example, a
      characteristic of virtually all trance songs is the soft mid-song breakdown, beginning with
      and occurring after the orchestration is broken down and the rhythm tracks fade out rapidly,
      leaving the melody, atmospherics, or both to stand alone for anywhere from a few seconds to a
      few minutes. Although the genre can be devoid of vocals, with mixes done by semi-amateurs
      posted online at informal locations, mixers who have gained recognition of major labels put
      out mixes for the radio market with mostly but not limited to female vocals, notably
      photogenic.</skos:definition>
    <skos:exactMatch xml:lang="en">http://dbpedia.org/resource/Trance_music</skos:exactMatch>
    <skos:inScheme rdf:resource="http://data.europeana.eu/concept/music/genre/Music_Genre_Scheme"/>
    <skos:altLabel xml:lang="en">Trance music</skos:altLabel>
  </skos:Concept>

  <skos:Concept rdf:about="http://data.europeana.eu/concept/music/genre/Funky_house">
    <skos:prefLabel xml:lang="en">Funky house</skos:prefLabel>
    <skos:prefLabel xml:lang="nl">Funky house</skos:prefLabel>
    <skos:prefLabel xml:lang="fr">Funky house</skos:prefLabel>
    <skos:prefLabel xml:lang="de">Funky House</skos:prefLabel>
    <skos:prefLabel xml:lang="it">Funky house</skos:prefLabel>
    <skos:prefLabel xml:lang="pl">Funky House</skos:prefLabel>
    <skos:prefLabel xml:lang="es">Funky house</skos:prefLabel>
    <skos:prefLabel xml:lang="sv">Funky house</skos:prefLabel>
    <skos:closeMatch rdf:resource="http://rdf.freebase.com/ns/m.07s383g"/>
    <skos:broader rdf:resource="http://data.europeana.eu/concept/music/genre/House_music_fusions"/>
    <skos:definition xml:lang="en">Funky house is a sub-genre of house music that uses funk samples,
      a funk-inspired bass line or a strong soul influence, combined with drum breaks that draw
      inspiration from 1970s and 1980s funk records. &lt;p&gt; Like most variants of house, the
      genre follows a traditional four to the floor house beat, and makes heavy use of synthesizers,
      samples and soulful vocals, although unlike in more electronically bent Chicago and deep
      house, presence of acoustic instrumentation is much more common. Notable producers that have
      worked in this genre include the Freemasons, Soul Central, Armand van Helden, StoneBridge,
      Seamus Haji, Moto Blanco and Mikey High Jinks. &lt;p&gt; The genre is commercially popular,
      with record labels such as Defected Records, Ministry of Sound, Hed Kandi, and Fierce Angel
      all releasing compilation albums dedicated to the genre. It was particularly successful in the
      early 2000s. &lt;p&gt; Notable artists include Armand Van Helden, Olav Basoski, Les Rythmes
      Digitales, Cassius.</skos:definition>
    <skos:exactMatch xml:lang="en">http://dbpedia.org/resource/Funky_house</skos:exactMatch>
    <skos:inScheme rdf:resource="http://data.europeana.eu/concept/music/genre/Music_Genre_Scheme"/>
    <skos:altLabel xml:lang="en">Funky house</skos:altLabel>
  </skos:Concept>

  <skos:Concept rdf:about="http://data.europeana.eu/concept/music/genre/Dubstep">
    <skos:prefLabel xml:lang="en">Dubstep</skos:prefLabel>
    <skos:prefLabel xml:lang="bg">Дъбстеп</skos:prefLabel>
    <skos:prefLabel xml:lang="ca">Dubstep</skos:prefLabel>
    <skos:prefLabel xml:lang="cs">Dubstep</skos:prefLabel>
    <skos:prefLabel xml:lang="da">Dubstep</skos:prefLabel>
    <skos:prefLabel xml:lang="nl">Dubstep</skos:prefLabel>
    <skos:prefLabel xml:lang="et">Dubstep</skos:prefLabel>
    <skos:prefLabel xml:lang="fi">Dubstep</skos:prefLabel>
    <skos:prefLabel xml:lang="fr">Dubstep</skos:prefLabel>
    <skos:prefLabel xml:lang="de">Dubstep</skos:prefLabel>
    <skos:prefLabel xml:lang="el">Dubstep</skos:prefLabel>
    <skos:prefLabel xml:lang="hu">Dubstep</skos:prefLabel>
    <skos:prefLabel xml:lang="it">Dubstep</skos:prefLabel>
    <skos:prefLabel xml:lang="ja">ダブステップ</skos:prefLabel>
    <skos:prefLabel xml:lang="ko">더브스텝</skos:prefLabel>
    <skos:prefLabel xml:lang="lv">Dabsteps</skos:prefLabel>
    <skos:prefLabel xml:lang="lt">Dubstep</skos:prefLabel>
    <skos:prefLabel xml:lang="ms">Dubstep</skos:prefLabel>
    <skos:prefLabel xml:lang="no">Dubstep</skos:prefLabel>
    <skos:prefLabel xml:lang="fa">داب‌استپ</skos:prefLabel>
    <skos:prefLabel xml:lang="pl">Dubstep</skos:prefLabel>
    <skos:prefLabel xml:lang="pt">Dubstep</skos:prefLabel>
    <skos:prefLabel xml:lang="ro">Dubstep</skos:prefLabel>
    <skos:prefLabel xml:lang="ru">Дабстеп</skos:prefLabel>
    <skos:prefLabel xml:lang="sr">Dabstep</skos:prefLabel>
    <skos:prefLabel xml:lang="sk">Dubstep</skos:prefLabel>
    <skos:prefLabel xml:lang="es">Dubstep</skos:prefLabel>
    <skos:prefLabel xml:lang="sv">Dubstep</skos:prefLabel>
    <skos:prefLabel xml:lang="th">ดั๊บสเตป</skos:prefLabel>
    <skos:prefLabel xml:lang="tr">Dubstep</skos:prefLabel>
    <skos:prefLabel xml:lang="uk">Дабстеп</skos:prefLabel>
    <skos:closeMatch rdf:resource="http://rdf.freebase.com/ns/m.07s72n"/>
    <skos:broader rdf:resource="http://data.europeana.eu/concept/music/genre/Hip_hop_music_fusions"/>
    <skos:definition xml:lang="en">Dubstep is a genre of electronic dance music that originated in
      South London, England. It emerged in the late 1990s as a development within a lineage of
      related styles such as 2-step garage, broken beat, drum and bass, jungle, dub and reggae. In
      the UK the origins of the genre can be traced back to the growth of the Jamaican sound system
      party scene in the early 1980s. The music generally features syncopated drum and percussion
      patterns with bass lines that contain prominent sub bass frequencies. &lt;p&gt; The earliest
      dubstep releases date back to 1998, and were usually featured as B-sides of 2-step garage
      single releases. These tracks were darker, more experimental remixes with less emphasis on
      vocals, and attempted to incorporate elements of breakbeat and drum and bass into 2-step. In
      2001, this and other strains of dark garage music began to be showcased and promoted at
      London's night club Plastic People, at the &quot;Forward&quot; night, which went on to be
      considerably influential to the development of dubstep.</skos:definition>
    <skos:exactMatch xml:lang="en">http://dbpedia.org/resource/Dubstep</skos:exactMatch>
    <skos:inScheme rdf:resource="http://data.europeana.eu/concept/music/genre/Music_Genre_Scheme"/>
    <skos:altLabel xml:lang="en">Dubstep</skos:altLabel>
  </skos:Concept>

  <skos:Concept rdf:about="http://data.europeana.eu/concept/music/genre/Rap_rock">
    <skos:prefLabel xml:lang="en">Rap rock</skos:prefLabel>
    <skos:prefLabel xml:lang="cs">Rap rock</skos:prefLabel>
    <skos:prefLabel xml:lang="da">Rap rock</skos:prefLabel>
    <skos:prefLabel xml:lang="nl">Rap-rock</skos:prefLabel>
    <skos:prefLabel xml:lang="it">Rap rock</skos:prefLabel>
    <skos:prefLabel xml:lang="ja">ラップロック</skos:prefLabel>
    <skos:prefLabel xml:lang="ko">랩 록</skos:prefLabel>
    <skos:prefLabel xml:lang="lt">Rep rokas</skos:prefLabel>
    <skos:prefLabel xml:lang="fa">رپ راک</skos:prefLabel>
    <skos:prefLabel xml:lang="pl">Rap rock</skos:prefLabel>
    <skos:prefLabel xml:lang="pt">Rap rock</skos:prefLabel>
    <skos:prefLabel xml:lang="ro">Rap rock</skos:prefLabel>
    <skos:prefLabel xml:lang="ru">Рэп-рок</skos:prefLabel>
    <skos:prefLabel xml:lang="sr">Rep rok</skos:prefLabel>
    <skos:prefLabel xml:lang="sk">Rap rock</skos:prefLabel>
    <skos:prefLabel xml:lang="es">Rap rock</skos:prefLabel>
    <skos:prefLabel xml:lang="sv">Raprock</skos:prefLabel>
    <skos:prefLabel xml:lang="th">แร็ปร็อก</skos:prefLabel>
    <skos:prefLabel xml:lang="uk">Реп-рок</skos:prefLabel>
    <skos:prefLabel xml:lang="vi">Rap rock</skos:prefLabel>
    <skos:closeMatch rdf:resource="http://rdf.freebase.com/ns/m.07s7gk6"/>
    <skos:broader rdf:resource="http://data.europeana.eu/concept/music/genre/Rock_music_fusions"/>
    <skos:definition xml:lang="en">Rap rock is a cross-genre fusing vocal and instrumental elements
      of hip hop with various forms of rock. Rap rock's most popular subgenres include rap metal and
      rapcore, which include heavy metal-oriented and hardcore punk-oriented influences,
      respectively. One of the earliest examples would be The Clash's song &quot;The Magnificent
      Seven&quot; which fused new wave, hip hop and funk.</skos:definition>
    <skos:exactMatch xml:lang="en">http://dbpedia.org/resource/Rap_rock</skos:exactMatch>
    <skos:inScheme rdf:resource="http://data.europeana.eu/concept/music/genre/Music_Genre_Scheme"/>
    <skos:altLabel xml:lang="en">Rap rock</skos:altLabel>
  </skos:Concept>

  <skos:Concept rdf:about="http://data.europeana.eu/concept/music/genre/Crunkcore">
    <skos:prefLabel xml:lang="en">Crunkcore</skos:prefLabel>
    <skos:prefLabel xml:lang="nl">Crunkcore</skos:prefLabel>
    <skos:prefLabel xml:lang="fr">Crunkcore</skos:prefLabel>
    <skos:prefLabel xml:lang="it">Crunkcore</skos:prefLabel>
    <skos:prefLabel xml:lang="ja">クランク・コア</skos:prefLabel>
    <skos:prefLabel xml:lang="pl">Crunkcore</skos:prefLabel>
    <skos:prefLabel xml:lang="ru">Кранккор</skos:prefLabel>
    <skos:prefLabel xml:lang="sk">Crunkcore</skos:prefLabel>
    <skos:prefLabel xml:lang="es">Crunkcore</skos:prefLabel>
    <skos:prefLabel xml:lang="sv">Crunkcore</skos:prefLabel>
    <skos:closeMatch rdf:resource="http://rdf.freebase.com/ns/m.07s7hjz"/>
    <skos:broader rdf:resource="http://data.europeana.eu/concept/music/genre/Hip_hop_music_fusions"/>
    <skos:definition xml:lang="en">Crunkcore is a musical genre that combines crunk with the vocal
      style of screamo</skos:definition>
    <skos:exactMatch xml:lang="en">http://dbpedia.org/resource/Crunkcore</skos:exactMatch>
    <skos:inScheme rdf:resource="http://data.europeana.eu/concept/music/genre/Music_Genre_Scheme"/>
    <skos:altLabel xml:lang="en">Crunkcore</skos:altLabel>
  </skos:Concept>

  <skos:Concept rdf:about="http://data.europeana.eu/concept/music/genre/Rock_and_roll">
    <skos:prefLabel xml:lang="en">Rock and roll</skos:prefLabel>
    <skos:prefLabel xml:lang="ar">روك أند رول</skos:prefLabel>
    <skos:prefLabel xml:lang="bg">Рокендрол</skos:prefLabel>
    <skos:prefLabel xml:lang="ca">Rock and roll</skos:prefLabel>
    <skos:prefLabel xml:lang="hr">Rock and roll</skos:prefLabel>
    <skos:prefLabel xml:lang="cs">Rock and roll</skos:prefLabel>
    <skos:prefLabel xml:lang="da">Rock and roll</skos:prefLabel>
    <skos:prefLabel xml:lang="nl">Rock-'n-roll</skos:prefLabel>
    <skos:prefLabel xml:lang="et">Rock'n'roll</skos:prefLabel>
    <skos:prefLabel xml:lang="fil">Rock and roll</skos:prefLabel>
    <skos:prefLabel xml:lang="fi">Rock and roll</skos:prefLabel>
    <skos:prefLabel xml:lang="fr">Rock 'n' roll</skos:prefLabel>
    <skos:prefLabel xml:lang="de">Rock ’n’ Roll</skos:prefLabel>
    <skos:prefLabel xml:lang="el">Ροκ εντ ρολ</skos:prefLabel>
    <skos:prefLabel xml:lang="hi">रॉक ऐन्ड रोल​</skos:prefLabel>
    <skos:prefLabel xml:lang="hu">Rock and roll</skos:prefLabel>
    <skos:prefLabel xml:lang="id">Rock and roll</skos:prefLabel>
    <skos:prefLabel xml:lang="it">Rock and roll</skos:prefLabel>
    <skos:prefLabel xml:lang="ja">ロックンロール</skos:prefLabel>
    <skos:prefLabel xml:lang="ko">로큰롤</skos:prefLabel>
    <skos:prefLabel xml:lang="lv">Rokenrols</skos:prefLabel>
    <skos:prefLabel xml:lang="lt">Rokenrolas</skos:prefLabel>
    <skos:prefLabel xml:lang="ms">Rock and roll</skos:prefLabel>
    <skos:prefLabel xml:lang="no">Rock and roll</skos:prefLabel>
    <skos:prefLabel xml:lang="fa">راک اند رول</skos:prefLabel>
    <skos:prefLabel xml:lang="pl">Rock and roll</skos:prefLabel>
    <skos:prefLabel xml:lang="pt">Rock and roll</skos:prefLabel>
    <skos:prefLabel xml:lang="ro">Muzică rock and roll</skos:prefLabel>
    <skos:prefLabel xml:lang="ru">Рок-н-ролл</skos:prefLabel>
    <skos:prefLabel xml:lang="sr">Рокенрол</skos:prefLabel>
    <skos:prefLabel xml:lang="sk">Rokenrol</skos:prefLabel>
    <skos:prefLabel xml:lang="es">Rock and roll</skos:prefLabel>
    <skos:prefLabel xml:lang="sv">Rock'n'roll</skos:prefLabel>
    <skos:prefLabel xml:lang="th">ร็อกแอนด์โรล</skos:prefLabel>
    <skos:prefLabel xml:lang="tr">Rock and roll</skos:prefLabel>
    <skos:prefLabel xml:lang="uk">Рок-н-рол</skos:prefLabel>
    <skos:prefLabel xml:lang="vi">Rock and roll</skos:prefLabel>
    <skos:closeMatch rdf:resource="http://rdf.freebase.com/ns/m.07sbbz2"/>
    <skos:broader rdf:resource="http://data.europeana.eu/concept/music/genre/Rock_music"/>
    <skos:definition xml:lang="en">Rock and roll is a genre of popular music that originated and
      evolved in the United States during the late 1940s and early 1950s, primarily from a
      combination of African-American genres such as blues, jump blues, jazz, and gospel music,
      together with Western swing and country music. Though elements of rock and roll can be heard
      in blues records from the 1920s and in country records of the 1930s, the genre did not acquire
      its name until the 1950s. &lt;p&gt; The term &quot;rock and roll&quot; now has at least two
      different meanings, both in common usage: referring to the first wave of music that originated
      in the US in the 1950s and would later develop into the more encompassing international style
      known as &quot;rock music&quot;, and as a term simply synonymous with the rock music and
      culture in the broad sense. For the purpose of differentiation, this article deals with the
      first definition. &lt;p&gt; In the earliest rock and roll styles of the late 1940s and early
      1950s, either the piano or saxophone was often the lead instrument, but these were generally
      replaced or supplemented by guitar in the middle to late 1950s.</skos:definition>
    <skos:exactMatch xml:lang="en">http://dbpedia.org/resource/Rock_and_roll</skos:exactMatch>
    <skos:inScheme rdf:resource="http://data.europeana.eu/concept/music/genre/Music_Genre_Scheme"/>
    <skos:altLabel xml:lang="en">rock &amp; roll</skos:altLabel>
    <skos:altLabel xml:lang="en">rock 'n' roll</skos:altLabel>
    <skos:altLabel xml:lang="en">Rock and roll</skos:altLabel>
  </skos:Concept>

  <skos:Concept rdf:about="http://data.europeana.eu/concept/music/genre/Post-punk_revival">
    <skos:prefLabel xml:lang="en">Post-punk revival</skos:prefLabel>
    <skos:prefLabel xml:lang="cs">Post-punk revival</skos:prefLabel>
    <skos:prefLabel xml:lang="nl">Postpunkrevival</skos:prefLabel>
    <skos:prefLabel xml:lang="de">Post-Punk Revival</skos:prefLabel>
    <skos:prefLabel xml:lang="lt">Post-punk revival</skos:prefLabel>
    <skos:prefLabel xml:lang="pl">Post-punk revival</skos:prefLabel>
    <skos:prefLabel xml:lang="pt">Post-punk revival</skos:prefLabel>
    <skos:prefLabel xml:lang="ru">Постпанк-ривайвл</skos:prefLabel>
    <skos:prefLabel xml:lang="sk">Post-punk revival</skos:prefLabel>
    <skos:prefLabel xml:lang="es">Post punk revival</skos:prefLabel>
    <skos:prefLabel xml:lang="th">โพสต์พังก์รีไววอล</skos:prefLabel>
    <skos:closeMatch rdf:resource="http://rdf.freebase.com/ns/m.07yklv"/>
    <skos:broader
      rdf:resource="http://data.europeana.eu/concept/music/genre/Alternative_rock_fusions"/>
    <skos:definition xml:lang="en">The post-punk revival was a development in alternative rock of
      the late 20th and early 21st centuries in which bands took inspiration from the original
      sounds and aesthetics of garage rock of the 1960s and post-punk and new wave of the 1980s.
      Bands that broke through to the mainstream from local scenes across the world in the early
      2000s included The Strokes, Interpol, The White Stripes, The Hives and The Vines, who were
      followed to commercial success by many established and new acts. By the end of the decade,
      most of the bands had broken up, moved on to other projects or were on hiatus, although some
      bands returned to recording and touring in the 2010s.</skos:definition>
    <skos:exactMatch xml:lang="en">http://dbpedia.org/resource/Post-punk_revival</skos:exactMatch>
    <skos:inScheme rdf:resource="http://data.europeana.eu/concept/music/genre/Music_Genre_Scheme"/>
    <skos:altLabel xml:lang="en">Post-punk revival</skos:altLabel>
  </skos:Concept>

  <skos:Concept rdf:about="http://data.europeana.eu/concept/music/genre/Jazz-funk">
    <skos:prefLabel xml:lang="en">Jazz-funk</skos:prefLabel>
    <skos:prefLabel xml:lang="ca">Jazz-funk</skos:prefLabel>
    <skos:prefLabel xml:lang="cs">Jazz-funk</skos:prefLabel>
    <skos:prefLabel xml:lang="fr">Jazz-funk</skos:prefLabel>
    <skos:prefLabel xml:lang="de">Jazzfunk</skos:prefLabel>
    <skos:prefLabel xml:lang="it">Jazz-funk</skos:prefLabel>
    <skos:prefLabel xml:lang="ja">ジャズ・ファンク</skos:prefLabel>
    <skos:prefLabel xml:lang="lt">Jazz-funk</skos:prefLabel>
    <skos:prefLabel xml:lang="pl">Jazz-funk</skos:prefLabel>
    <skos:prefLabel xml:lang="pt">Jazz-funk</skos:prefLabel>
    <skos:prefLabel xml:lang="ru">Джаз-фанк</skos:prefLabel>
    <skos:prefLabel xml:lang="sk">Jazz-funk</skos:prefLabel>
    <skos:prefLabel xml:lang="es">Jazz-funk</skos:prefLabel>
    <skos:prefLabel xml:lang="uk">Джаз-фанк</skos:prefLabel>
    <skos:closeMatch rdf:resource="http://rdf.freebase.com/ns/m.07ym47"/>
    <skos:broader rdf:resource="http://data.europeana.eu/concept/music/genre/Jazz_fusions"/>
    <skos:definition xml:lang="en">Jazz-funk is a sub genre of jazz music characterized by a strong
      back beat, electrified sounds and an early prevalence of analog synthesizers. The integration
      of funk, soul, and R&amp;B music and styles into jazz resulted in the creation of a genre
      whose spectrum is quite wide and ranges from strong jazz improvisation to soul, funk or disco
      with jazz arrangements, jazz riffs, and jazz solos, and sometimes soul vocals. &lt;p&gt;
      Jazz-funk is primarily an American genre, where it was popular throughout the 1970s and the
      early 1980s, but it also achieved noted appeal on the club-circuit in England during the
      mid-1970s. Similar genres include soul jazz and jazz fusion, but neither entirely overlap with
      jazz-funk. Notably jazz-funk is less vocal, more arranged and featured more improvisation than
      soul jazz, and retains a strong feel of groove and R&amp;B versus some of the jazz fusion
      production.</skos:definition>
    <skos:exactMatch xml:lang="en">http://dbpedia.org/resource/Jazz-funk</skos:exactMatch>
    <skos:inScheme rdf:resource="http://data.europeana.eu/concept/music/genre/Music_Genre_Scheme"/>
    <skos:altLabel xml:lang="en">Jazz-funk</skos:altLabel>
  </skos:Concept>

  <skos:Concept rdf:about="http://data.europeana.eu/concept/music/genre/Ethno_jazz">
    <skos:prefLabel xml:lang="en">Ethno jazz</skos:prefLabel>
    <skos:prefLabel xml:lang="et">Etnodžäss</skos:prefLabel>
    <skos:prefLabel xml:lang="fr">Ethno-jazz</skos:prefLabel>
    <skos:prefLabel xml:lang="de">Ethno-Jazz</skos:prefLabel>
    <skos:closeMatch rdf:resource="http://rdf.freebase.com/ns/m.08042r"/>
    <skos:broader rdf:resource="http://data.europeana.eu/concept/music/genre/Jazz_fusions"/>
    <skos:definition xml:lang="en">Ethno Jazz, a form of Ethno Music, is sometimes equaled to World
      Music or is regarded as its successor, particularly before the 1990s. An independent meaning
      of &quot;Ethno Jazz&quot; emerged around 1990 with globalisation and later the Internet as
      well as the commercial success of Ethno groups and musicians. From the American and European
      view, interpretations from developing countries, particularly the developing southeast Asia
      and the People's Republic of China, became important. &lt;p&gt; Whereas global regions like
      India, Latin America and Africa had been reached already before 1990, they regained importance
      in the form of Ethno Music, and Ethno Jazz in particular. Notable examples are the emergence
      of jazz through the interaction between New Orleans and Cuba, the Afro-Cuban jazz in the 1940s
      and 50s, Arab influence in Jazz in the 1950s and 60s and Indian influence through The Beatles
      and Rock Jazz of the 1960s and 70s. &lt;p&gt; Ethno Jazz, particularly from the 1990s, meant
      Jazz was in accordance with the more American and European view, but realised with the typical
      musical differences of non-American and -European regions, particularly the expanding centres
      of Southeast Asia and China. Superficially, and out of an American and European view, Ethno
      Jazz is sometimes not as Jazz, but probably something similar missing a more suitable
      classification.</skos:definition>
    <skos:exactMatch xml:lang="en">http://dbpedia.org/resource/Ethno_jazz</skos:exactMatch>
    <skos:inScheme rdf:resource="http://data.europeana.eu/concept/music/genre/Music_Genre_Scheme"/>
    <skos:altLabel xml:lang="en">Ethno jazz</skos:altLabel>
  </skos:Concept>

  <skos:Concept rdf:about="http://data.europeana.eu/concept/music/genre/Kuduro">
    <skos:prefLabel xml:lang="en">Kuduro</skos:prefLabel>
    <skos:prefLabel xml:lang="ar">كودورو</skos:prefLabel>
    <skos:prefLabel xml:lang="nl">Kuduro</skos:prefLabel>
    <skos:prefLabel xml:lang="fr">Kuduro</skos:prefLabel>
    <skos:prefLabel xml:lang="de">Kuduro</skos:prefLabel>
    <skos:prefLabel xml:lang="it">Kuduro</skos:prefLabel>
    <skos:prefLabel xml:lang="ja">クドゥーロ</skos:prefLabel>
    <skos:prefLabel xml:lang="ko">쿠두루</skos:prefLabel>
    <skos:prefLabel xml:lang="pt">Kuduro</skos:prefLabel>
    <skos:prefLabel xml:lang="ru">Кудуро</skos:prefLabel>
    <skos:prefLabel xml:lang="es">Kuduro</skos:prefLabel>
    <skos:prefLabel xml:lang="sv">Kuduro</skos:prefLabel>
    <skos:closeMatch rdf:resource="http://rdf.freebase.com/ns/m.080nby"/>
    <skos:broader
      rdf:resource="http://data.europeana.eu/concept/music/genre/African_popular_music_fusions"/>
    <skos:definition xml:lang="en">Kuduro is a type of music and dance originally developed in
      Angola in the 1980s. It is characterized as uptempo, energetic, and danceable. Kuduro began in
      Luanda, Angola in the late 1980s. Initially, producers sampled traditional carnival music like
      soca and zouk from the Caribbean, and also semba from Angola and laid this around a fast 4/4
      beat. &lt;p&gt; The kuduro is similar to the Kizomba rhythm. The lyrics tend to be very basic
      and overwhelmingly are sung in Portuguese. &lt;p&gt; Buraka Som Sistema is a group with a
      certain relevance in the music genre and defines their musical style into what they call
      progressive kuduro.</skos:definition>
    <skos:exactMatch xml:lang="en">http://dbpedia.org/resource/Kuduro</skos:exactMatch>
    <skos:inScheme rdf:resource="http://data.europeana.eu/concept/music/genre/Music_Genre_Scheme"/>
    <skos:altLabel xml:lang="en">Kuduro</skos:altLabel>
  </skos:Concept>

  <skos:Concept rdf:about="http://data.europeana.eu/concept/music/genre/Dark_cabaret">
    <skos:prefLabel xml:lang="en">Dark cabaret</skos:prefLabel>
    <skos:prefLabel xml:lang="fr">Dark cabaret</skos:prefLabel>
    <skos:prefLabel xml:lang="de">Dark Cabaret</skos:prefLabel>
    <skos:prefLabel xml:lang="it">Dark cabaret</skos:prefLabel>
    <skos:prefLabel xml:lang="pt">Dark cabaret</skos:prefLabel>
    <skos:prefLabel xml:lang="ru">Дарк кабаре</skos:prefLabel>
    <skos:prefLabel xml:lang="es">Dark cabaret</skos:prefLabel>
    <skos:prefLabel xml:lang="sv">Dark cabaret</skos:prefLabel>
    <skos:closeMatch rdf:resource="http://rdf.freebase.com/ns/m.088vmr"/>
    <skos:broader rdf:resource="http://data.europeana.eu/concept/music/genre/Rock_music_fusions"/>
    <skos:definition xml:lang="en">Dark cabaret may be a simple description of the theme and mood of
      a cabaret performance, but more recently has come to define a particular musical genre which
      draws on the aesthetics of the decadent, risqué German Weimar-era cabarets, burlesque and
      vaudeville shows with the stylings of post-1970s goth and punk music.</skos:definition>
    <skos:exactMatch xml:lang="en">http://dbpedia.org/resource/Dark_cabaret</skos:exactMatch>
    <skos:inScheme rdf:resource="http://data.europeana.eu/concept/music/genre/Music_Genre_Scheme"/>
    <skos:altLabel xml:lang="en">Dark cabaret</skos:altLabel>
  </skos:Concept>

  <skos:Concept rdf:about="http://data.europeana.eu/concept/music/genre/Jumpstyle">
    <skos:prefLabel xml:lang="en">Jumpstyle</skos:prefLabel>
    <skos:prefLabel xml:lang="ca">Jumpstyle</skos:prefLabel>
    <skos:prefLabel xml:lang="hr">Jumpstyle</skos:prefLabel>
    <skos:prefLabel xml:lang="cs">Jumpstyle</skos:prefLabel>
    <skos:prefLabel xml:lang="nl">Jump</skos:prefLabel>
    <skos:prefLabel xml:lang="et">Jumpstyle</skos:prefLabel>
    <skos:prefLabel xml:lang="fi">Jumpstyle</skos:prefLabel>
    <skos:prefLabel xml:lang="fr">Jumpstyle</skos:prefLabel>
    <skos:prefLabel xml:lang="de">Jumpstyle</skos:prefLabel>
    <skos:prefLabel xml:lang="hu">Jumpstyle</skos:prefLabel>
    <skos:prefLabel xml:lang="it">Jumpstyle</skos:prefLabel>
    <skos:prefLabel xml:lang="lt">Jumpstyle</skos:prefLabel>
    <skos:prefLabel xml:lang="no">Jumpstyle</skos:prefLabel>
    <skos:prefLabel xml:lang="pl">Jumpstyle</skos:prefLabel>
    <skos:prefLabel xml:lang="pt">Jumpstyle</skos:prefLabel>
    <skos:prefLabel xml:lang="ru">Джампстайл</skos:prefLabel>
    <skos:prefLabel xml:lang="sk">Jumpstyle</skos:prefLabel>
    <skos:prefLabel xml:lang="sl">Jumpstyle</skos:prefLabel>
    <skos:prefLabel xml:lang="es">Jumpstyle</skos:prefLabel>
    <skos:prefLabel xml:lang="sv">Jumpstyle</skos:prefLabel>
    <skos:prefLabel xml:lang="uk">Джампстайл</skos:prefLabel>
    <skos:closeMatch rdf:resource="http://rdf.freebase.com/ns/m.08lv66"/>
    <skos:broader rdf:resource="http://data.europeana.eu/concept/music/genre/Techno_fusions"/>
    <skos:definition xml:lang="en">Jumpstyle is an EDM dance style and hard dance music genre
      popular in Northwestern Europe, United Kingdom, as well as certain parts of Australia and the
      United States. The word originates from a movement of hard dance music followers, and
      especially those devoted to its post-2007. &lt;p&gt; Jumpstyling is often referred to as
      &quot;Jumpen&quot;: a combination of the English word 'Jump' and the Dutch &amp; German suffix
      '-en' . &lt;p&gt; It originated in 1997 in Belgium but gathered bigger popularity in their
      neighboring country the Netherlands in the 2000s.</skos:definition>
    <skos:exactMatch xml:lang="en">http://dbpedia.org/resource/Jumpstyle</skos:exactMatch>
    <skos:inScheme rdf:resource="http://data.europeana.eu/concept/music/genre/Music_Genre_Scheme"/>
    <skos:altLabel xml:lang="en">Jumpstyle</skos:altLabel>
  </skos:Concept>

  <skos:Concept rdf:about="http://data.europeana.eu/concept/music/genre/Celtic_punk">
    <skos:prefLabel xml:lang="en">Celtic punk</skos:prefLabel>
    <skos:prefLabel xml:lang="hr">keltski punk</skos:prefLabel>
    <skos:prefLabel xml:lang="da">Keltisk punk</skos:prefLabel>
    <skos:prefLabel xml:lang="nl">Celtic punk</skos:prefLabel>
    <skos:prefLabel xml:lang="fr">Punk celtique</skos:prefLabel>
    <skos:prefLabel xml:lang="it">Celtic punk</skos:prefLabel>
    <skos:prefLabel xml:lang="ja">アイリッシュ・パンク</skos:prefLabel>
    <skos:prefLabel xml:lang="lv">Ķeltu pankroks</skos:prefLabel>
    <skos:prefLabel xml:lang="pl">Celtic punk rock</skos:prefLabel>
    <skos:prefLabel xml:lang="ro">Celtic punk</skos:prefLabel>
    <skos:prefLabel xml:lang="ru">Кельтик-панк</skos:prefLabel>
    <skos:prefLabel xml:lang="sr">keltski punk</skos:prefLabel>
    <skos:prefLabel xml:lang="es">Celtic punk</skos:prefLabel>
    <skos:prefLabel xml:lang="sv">Celtic punk</skos:prefLabel>
    <skos:closeMatch rdf:resource="http://rdf.freebase.com/ns/m.08vf3v"/>
    <skos:broader rdf:resource="http://data.europeana.eu/concept/music/genre/Punk_rock_fusions"/>
    <skos:definition xml:lang="en">Celtic punk is punk rock mixed with traditional Celtic music. The
      genre was founded in the 1980s by The Pogues, a band of punk musicians in London who
      celebrated their Irish heritage. Celtic punk bands often play covers of traditional Irish or
      Scottish folk and political songs, as well as original compositions. Common themes in Celtic
      punk music include politics, culture, religion, drinking and working class
      pride.</skos:definition>
    <skos:exactMatch xml:lang="en">http://dbpedia.org/resource/Celtic_punk</skos:exactMatch>
    <skos:inScheme rdf:resource="http://data.europeana.eu/concept/music/genre/Music_Genre_Scheme"/>
    <skos:altLabel xml:lang="en">Celtic punk</skos:altLabel>
  </skos:Concept>

  <skos:Concept rdf:about="http://data.europeana.eu/concept/music/genre/Gothic_metal">
    <skos:prefLabel xml:lang="en">Gothic metal</skos:prefLabel>
    <skos:prefLabel xml:lang="ar">غوثيك ميتال</skos:prefLabel>
    <skos:prefLabel xml:lang="bg">Готик метъл</skos:prefLabel>
    <skos:prefLabel xml:lang="hr">Gothic metal</skos:prefLabel>
    <skos:prefLabel xml:lang="cs">Gotický metal</skos:prefLabel>
    <skos:prefLabel xml:lang="da">Gothic metal</skos:prefLabel>
    <skos:prefLabel xml:lang="nl">Gothic metal</skos:prefLabel>
    <skos:prefLabel xml:lang="et">Gothic metal</skos:prefLabel>
    <skos:prefLabel xml:lang="fi">Goottimetalli</skos:prefLabel>
    <skos:prefLabel xml:lang="fr">Gothic metal</skos:prefLabel>
    <skos:prefLabel xml:lang="de">Gothic Metal</skos:prefLabel>
    <skos:prefLabel xml:lang="hu">Gothic metal</skos:prefLabel>
    <skos:prefLabel xml:lang="id">Musik gothic</skos:prefLabel>
    <skos:prefLabel xml:lang="it">Gothic metal</skos:prefLabel>
    <skos:prefLabel xml:lang="ja">ゴシックメタル</skos:prefLabel>
    <skos:prefLabel xml:lang="ko">고딕 메탈</skos:prefLabel>
    <skos:prefLabel xml:lang="lv">Gotiskais metāls</skos:prefLabel>
    <skos:prefLabel xml:lang="lt">Gotikinis metalas</skos:prefLabel>
    <skos:prefLabel xml:lang="no">Gothic metal</skos:prefLabel>
    <skos:prefLabel xml:lang="fa">گوتیک متال</skos:prefLabel>
    <skos:prefLabel xml:lang="pl">Gothic metal</skos:prefLabel>
    <skos:prefLabel xml:lang="pt">Gothic metal</skos:prefLabel>
    <skos:prefLabel xml:lang="ro">Gothic metal</skos:prefLabel>
    <skos:prefLabel xml:lang="ru">Готик-метал</skos:prefLabel>
    <skos:prefLabel xml:lang="sr">Готик метал</skos:prefLabel>
    <skos:prefLabel xml:lang="sk">Gotický metal</skos:prefLabel>
    <skos:prefLabel xml:lang="sl">Gothic metal</skos:prefLabel>
    <skos:prefLabel xml:lang="es">Metal gótico</skos:prefLabel>
    <skos:prefLabel xml:lang="sv">Gothic metal</skos:prefLabel>
    <skos:prefLabel xml:lang="tr">Gotik metal</skos:prefLabel>
    <skos:prefLabel xml:lang="uk">Готичний метал</skos:prefLabel>
    <skos:closeMatch rdf:resource="http://rdf.freebase.com/ns/m.08z0wx"/>
    <skos:broader
      rdf:resource="http://data.europeana.eu/concept/music/genre/Heavy_metal_music_fusions"/>
    <skos:definition xml:lang="en">Gothic metal is a subgenre of heavy metal that combines the
      heaviness of doom metal with the dark atmospheres of gothic rock. The music of gothic metal is
      diverse with bands known to adopt the gothic approach to different styles of heavy metal
      music. The genre originated during the early 1990s in Europe originally as an outgrowth of
      death-doom, a fusion of death metal and doom metal. Lyrics are generally dark and
      introspective with inspiration from gothic fiction as well as personal experiences. &lt;p&gt;
      Pioneers of gothic metal include Paradise Lost, My Dying Bride and Anathema, all from the
      north of England. Other pioneers from the first half of the 1990s include Pyogenesis from
      Germany, Type O Negative, Saviour Machine from the United States, Tiamat from Sweden, and The
      Gathering from the Netherlands. Norwegian band Theatre of Tragedy developed the &quot;beauty
      and the beast&quot; aesthetic of combining aggressive male vocals with clean female vocals, a
      contrast that has since been adopted by many gothic metal groups. During the mid-1990s,
      Moonspell, Theatres des Vampires and Cradle of Filth brought the gothic approach to black
      metal.</skos:definition>
    <skos:exactMatch xml:lang="en">http://dbpedia.org/resource/Gothic_metal</skos:exactMatch>
    <skos:inScheme rdf:resource="http://data.europeana.eu/concept/music/genre/Music_Genre_Scheme"/>
    <skos:altLabel xml:lang="en">Gothic metal</skos:altLabel>
  </skos:Concept>

  <skos:Concept rdf:about="http://data.europeana.eu/concept/music/genre/New_Beat">
    <skos:prefLabel xml:lang="en">New Beat</skos:prefLabel>
    <skos:prefLabel xml:lang="nl">New Beat</skos:prefLabel>
    <skos:prefLabel xml:lang="fi">New beat</skos:prefLabel>
    <skos:prefLabel xml:lang="fr">New beat</skos:prefLabel>
    <skos:prefLabel xml:lang="de">New Beat</skos:prefLabel>
    <skos:prefLabel xml:lang="el">New Beat</skos:prefLabel>
    <skos:prefLabel xml:lang="it">New beat</skos:prefLabel>
    <skos:prefLabel xml:lang="lt">New Beat</skos:prefLabel>
    <skos:prefLabel xml:lang="ru">New Beat</skos:prefLabel>
    <skos:prefLabel xml:lang="sk">New beat</skos:prefLabel>
    <skos:prefLabel xml:lang="es">New beat</skos:prefLabel>
    <skos:prefLabel xml:lang="sv">New beat</skos:prefLabel>
    <skos:closeMatch rdf:resource="http://rdf.freebase.com/ns/m.0911bq"/>
    <skos:broader rdf:resource="http://data.europeana.eu/concept/music/genre/House_music_fusions"/>
    <skos:definition xml:lang="en">New beat is an electronic dance music term that was used in the
      1980s with two different meanings, one a collective term used in the U.S. for various
      electronic music styles, and the other a reference to the new beat sound: a particular
      electronic music genre that flourished in Western Europe during the mid-1980s. New beat is
      also used as a reference to the wider Belgian underground music scene and subculture during
      the 1980s.</skos:definition>
    <skos:exactMatch xml:lang="en">http://dbpedia.org/resource/New_Beat</skos:exactMatch>
    <skos:inScheme rdf:resource="http://data.europeana.eu/concept/music/genre/Music_Genre_Scheme"/>
    <skos:altLabel xml:lang="en">New Beat</skos:altLabel>
  </skos:Concept>

  <skos:Concept rdf:about="http://data.europeana.eu/concept/music/genre/Chillwave">
    <skos:prefLabel xml:lang="en">Chillwave</skos:prefLabel>
    <skos:prefLabel xml:lang="nl">Chillwave</skos:prefLabel>
    <skos:prefLabel xml:lang="fr">Chillwave</skos:prefLabel>
    <skos:prefLabel xml:lang="el">Chillwave</skos:prefLabel>
    <skos:prefLabel xml:lang="it">Chillwave</skos:prefLabel>
    <skos:prefLabel xml:lang="fa">چیل‌ویو</skos:prefLabel>
    <skos:prefLabel xml:lang="pl">Chillwave</skos:prefLabel>
    <skos:prefLabel xml:lang="pt">Chillwave</skos:prefLabel>
    <skos:prefLabel xml:lang="ru">Чиллвейв</skos:prefLabel>
    <skos:prefLabel xml:lang="sv">Chillwave</skos:prefLabel>
    <skos:closeMatch rdf:resource="http://rdf.freebase.com/ns/m.09k5dbs"/>
    <skos:broader
      rdf:resource="http://data.europeana.eu/concept/music/genre/Electronic_music_fusions"/>
    <skos:definition xml:lang="en">Chillwave, sometimes also referred to as glo-fi, is a genre of
      music whose artists are often characterized by their heavy use of effects processing,
      synthesizers, looping, sampling, and heavily filtered vocals with simple melodic lines.
      &lt;p&gt; The genre combines the larger 2000s trends towards 80s retro music and use of
      ambient sound, with modern pop, as in electropop, post-punk revival, psych-folk, nu gaze, and
      witch house. It is often described as &quot;summer music.&quot;</skos:definition>
    <skos:exactMatch xml:lang="en">http://dbpedia.org/resource/Chillwave</skos:exactMatch>
    <skos:inScheme rdf:resource="http://data.europeana.eu/concept/music/genre/Music_Genre_Scheme"/>
    <skos:altLabel xml:lang="en">Chillwave</skos:altLabel>
  </skos:Concept>

  <skos:Concept rdf:about="http://data.europeana.eu/concept/music/genre/Boogie_(genre)">
    <skos:prefLabel xml:lang="en">Boogie</skos:prefLabel>
    <skos:prefLabel xml:lang="ro">Boogie</skos:prefLabel>
    <skos:closeMatch rdf:resource="http://rdf.freebase.com/ns/m.09k7176"/>
    <skos:broader
      rdf:resource="http://data.europeana.eu/concept/music/genre/Electronic_music_fusions"/>
    <skos:definition xml:lang="en">Boogie is a rhythm and blues genre of electronic dance music with
      close ties to the post-disco style, that first emerged in the United States during the late
      1970s to mid-1980s. The sound of boogie defined by bridging acoustic and electronic musical
      instruments with emphasis on vocals and miscellaneous effects later evolved into electro and
      house music.</skos:definition>
    <skos:exactMatch xml:lang="en">http://dbpedia.org/resource/Boogie_(genre)</skos:exactMatch>
    <skos:inScheme rdf:resource="http://data.europeana.eu/concept/music/genre/Music_Genre_Scheme"/>
    <skos:altLabel xml:lang="en">Boogie</skos:altLabel>
  </skos:Concept>

  <skos:Concept rdf:about="http://data.europeana.eu/concept/music/genre/Indietronica">
    <skos:prefLabel xml:lang="en">Indietronica</skos:prefLabel>
    <skos:prefLabel xml:lang="nl">Indietronica</skos:prefLabel>
    <skos:prefLabel xml:lang="de">Indietronic</skos:prefLabel>
    <skos:prefLabel xml:lang="it">Indietronica</skos:prefLabel>
    <skos:prefLabel xml:lang="no">Indietronica</skos:prefLabel>
    <skos:prefLabel xml:lang="pl">Indietronica</skos:prefLabel>
    <skos:prefLabel xml:lang="pt">Indietronica</skos:prefLabel>
    <skos:prefLabel xml:lang="ru">Инди-электроника</skos:prefLabel>
    <skos:prefLabel xml:lang="sk">Indietronica</skos:prefLabel>
    <skos:prefLabel xml:lang="es">Indietrónica</skos:prefLabel>
    <skos:prefLabel xml:lang="sv">Indietronica</skos:prefLabel>
    <skos:prefLabel xml:lang="th">อินดีโทรนิกา</skos:prefLabel>
    <skos:closeMatch rdf:resource="http://rdf.freebase.com/ns/m.09v14qs"/>
    <skos:broader
      rdf:resource="http://data.europeana.eu/concept/music/genre/Electronic_rock_fusions"/>
    <skos:definition xml:lang="en">Indietronica is a music genre that combines indie, electronica,
      rock and pop music. Typical instruments used in indietronica music are the electronic
      keyboard, synthesizer, sampler, software synthesizer, MIDI controller, and drum machine. It is
      also closely related to the relatively less electronic and more acoustic chillwave
      movement.</skos:definition>
    <skos:exactMatch xml:lang="en">http://dbpedia.org/resource/Indietronica</skos:exactMatch>
    <skos:inScheme rdf:resource="http://data.europeana.eu/concept/music/genre/Music_Genre_Scheme"/>
    <skos:altLabel xml:lang="en">Indietronica</skos:altLabel>
  </skos:Concept>

  <skos:Concept rdf:about="http://data.europeana.eu/concept/music/genre/Neo-psychedelia">
    <skos:prefLabel xml:lang="en">Neo-psychedelia</skos:prefLabel>
    <skos:prefLabel xml:lang="it">Neopsichedelia</skos:prefLabel>
    <skos:prefLabel xml:lang="no">Neo-psykedelia</skos:prefLabel>
    <skos:prefLabel xml:lang="pl">Neo-psychodelia</skos:prefLabel>
    <skos:prefLabel xml:lang="pt">Neopsicodelia</skos:prefLabel>
    <skos:prefLabel xml:lang="ru">Неопсиходелия</skos:prefLabel>
    <skos:prefLabel xml:lang="sk">Neo-psychedelia</skos:prefLabel>
    <skos:prefLabel xml:lang="es">Neopsicodelia</skos:prefLabel>
    <skos:closeMatch rdf:resource="http://rdf.freebase.com/ns/m.0b_6yv"/>
    <skos:broader rdf:resource="http://data.europeana.eu/concept/music/genre/Rock_music_fusions"/>
    <skos:definition xml:lang="en">Neo-psychedelia is music that emulates or is heavily influenced
      by the psychedelic music of the 1960s. It began to be revived among British post-punk bands of
      the later 1970s and early 1980s and was taken up by groups including bands of the Paisley
      Underground and Madchester scenes, as well as occasional interest from mainstream artists and
      bands into the new millennium.</skos:definition>
    <skos:exactMatch xml:lang="en">http://dbpedia.org/resource/Neo-psychedelia</skos:exactMatch>
    <skos:inScheme rdf:resource="http://data.europeana.eu/concept/music/genre/Music_Genre_Scheme"/>
    <skos:altLabel xml:lang="en">Neo-psychedelia</skos:altLabel>
  </skos:Concept>

  <skos:Concept rdf:about="http://data.europeana.eu/concept/music/genre/Ragga_jungle">
    <skos:prefLabel xml:lang="en">Ragga jungle</skos:prefLabel>
    <skos:prefLabel xml:lang="nl">Ragga jungle</skos:prefLabel>
    <skos:prefLabel xml:lang="fr">Ragga jungle</skos:prefLabel>
    <skos:prefLabel xml:lang="it">Ragga jungle</skos:prefLabel>
    <skos:prefLabel xml:lang="ru">Рагга-джангл</skos:prefLabel>
    <skos:prefLabel xml:lang="sk">Ragga jungle</skos:prefLabel>
    <skos:prefLabel xml:lang="es">Ragga jungle</skos:prefLabel>
    <skos:closeMatch rdf:resource="http://rdf.freebase.com/ns/m.0bd34m"/>
    <skos:broader rdf:resource="http://data.europeana.eu/concept/music/genre/Hip_hop_music_fusions"/>
    <skos:definition xml:lang="en">Ragga jungle is a genre of music that emerged circa 1989-1990 and
      was initially heavily based on production of Michael West. Early pioneers of the genre also
      include Lennie De Ice, DJ Dextrous, Remarc, MBeat and Ragga Twins.</skos:definition>
    <skos:exactMatch xml:lang="en">http://dbpedia.org/resource/Ragga_jungle</skos:exactMatch>
    <skos:inScheme rdf:resource="http://data.europeana.eu/concept/music/genre/Music_Genre_Scheme"/>
    <skos:altLabel xml:lang="en">Ragga jungle</skos:altLabel>
  </skos:Concept>

  <skos:Concept rdf:about="http://data.europeana.eu/concept/music/genre/Breakbeat_hardcore">
    <skos:prefLabel xml:lang="en">Breakbeat hardcore</skos:prefLabel>
    <skos:prefLabel xml:lang="cs">Breakbeat hardcore</skos:prefLabel>
    <skos:prefLabel xml:lang="fr">Breakbeat hardcore</skos:prefLabel>
    <skos:prefLabel xml:lang="de">Hardcore</skos:prefLabel>
    <skos:prefLabel xml:lang="pl">Breakbeat hardcore</skos:prefLabel>
    <skos:prefLabel xml:lang="ru">Олдскул хардкор</skos:prefLabel>
    <skos:prefLabel xml:lang="sk">Breakbeat hardcore</skos:prefLabel>
    <skos:prefLabel xml:lang="es">Breakbeat hardcore</skos:prefLabel>
    <skos:prefLabel xml:lang="th">เบรกบีตฮาร์ดคอร์</skos:prefLabel>
    <skos:closeMatch rdf:resource="http://rdf.freebase.com/ns/m.0btzx"/>
    <skos:broader
      rdf:resource="http://data.europeana.eu/concept/music/genre/Electronic_music_fusions"/>
    <skos:definition xml:lang="en">Breakbeat hardcore is a derivative of acid house and techno
      music, of the late 1980s and early 1990s, that combines four-on-the-floor rhythms with
      breakbeats, and is associated with the UK rave scene. It was mainly the electronic group The
      Prodigy that brought the genre to prominence in the early 90s. In addition to the including of
      breakbeats the genre also features shuffled drum machine patterns, upbeat piano rolls and
      old-school hoover sounds.</skos:definition>
    <skos:exactMatch xml:lang="en">http://dbpedia.org/resource/Breakbeat_hardcore</skos:exactMatch>
    <skos:inScheme rdf:resource="http://data.europeana.eu/concept/music/genre/Music_Genre_Scheme"/>
    <skos:altLabel xml:lang="en">Breakbeat hardcore</skos:altLabel>
  </skos:Concept>

  <skos:Concept rdf:about="http://data.europeana.eu/concept/music/genre/Moombahton">
    <skos:prefLabel xml:lang="en">Moombahton</skos:prefLabel>
    <skos:prefLabel xml:lang="nl">Moombahton</skos:prefLabel>
    <skos:prefLabel xml:lang="fi">Moombahton</skos:prefLabel>
    <skos:prefLabel xml:lang="fr">Moombahton</skos:prefLabel>
    <skos:prefLabel xml:lang="de">Moombahton</skos:prefLabel>
    <skos:prefLabel xml:lang="it">Moombahton</skos:prefLabel>
    <skos:prefLabel xml:lang="ja">ムーンバートン</skos:prefLabel>
    <skos:prefLabel xml:lang="fa">مومباهتون</skos:prefLabel>
    <skos:prefLabel xml:lang="pl">Moombahton</skos:prefLabel>
    <skos:prefLabel xml:lang="ru">Мумбатон</skos:prefLabel>
    <skos:prefLabel xml:lang="sk">Moombahton</skos:prefLabel>
    <skos:closeMatch rdf:resource="http://rdf.freebase.com/ns/m.0bwfw5g"/>
    <skos:broader
      rdf:resource="http://data.europeana.eu/concept/music/genre/Electronic_music_fusions"/>
    <skos:definition xml:lang="en">Moombahton is a fusion genre of house music and reggaeton that
      was created by American DJ and producer Dave Nada in Washington, D.C., in 2009. Musically, it
      shares rhythmic origins with Dutch house or electro house slowed down to the tempo of
      reggaeton, usually 108 to 115 beats per minute, with reggaeton-influenced drum and percussion
      elements. Other features include &quot;thick basslines, dramatic buildups, a two-step pulse,
      and quick drum fills.&quot; Nada coined the name as a portmanteau of &quot;Moombah&quot; and
      reggaeton.</skos:definition>
    <skos:exactMatch xml:lang="en">http://dbpedia.org/resource/Moombahton</skos:exactMatch>
    <skos:inScheme rdf:resource="http://data.europeana.eu/concept/music/genre/Music_Genre_Scheme"/>
    <skos:altLabel xml:lang="en">Moombahton</skos:altLabel>
  </skos:Concept>

  <skos:Concept rdf:about="http://data.europeana.eu/concept/music/genre/Nintendocore">
    <skos:prefLabel xml:lang="en">Nintendocore</skos:prefLabel>
    <skos:prefLabel xml:lang="hr">Nintendocore</skos:prefLabel>
    <skos:prefLabel xml:lang="cs">Nintendocore</skos:prefLabel>
    <skos:prefLabel xml:lang="nl">Nintendocore</skos:prefLabel>
    <skos:prefLabel xml:lang="fi">Nintendocore</skos:prefLabel>
    <skos:prefLabel xml:lang="fr">Nintendocore</skos:prefLabel>
    <skos:prefLabel xml:lang="de">Nintendocore</skos:prefLabel>
    <skos:prefLabel xml:lang="it">Nintendocore</skos:prefLabel>
    <skos:prefLabel xml:lang="no">Nintendocore</skos:prefLabel>
    <skos:prefLabel xml:lang="fa">نینتندوکور</skos:prefLabel>
    <skos:prefLabel xml:lang="pl">Nintendocore</skos:prefLabel>
    <skos:prefLabel xml:lang="pt">Nintendocore</skos:prefLabel>
    <skos:prefLabel xml:lang="ru">Nintendocore</skos:prefLabel>
    <skos:prefLabel xml:lang="sk">Nintendocore</skos:prefLabel>
    <skos:prefLabel xml:lang="es">Nintendocore</skos:prefLabel>
    <skos:prefLabel xml:lang="sv">Nintendocore</skos:prefLabel>
    <skos:prefLabel xml:lang="uk">Нінтендокор</skos:prefLabel>
    <skos:closeMatch rdf:resource="http://rdf.freebase.com/ns/m.090l0_"/>
    <skos:broader
      rdf:resource="http://data.europeana.eu/concept/music/genre/Electronic_music_fusions"/>
    <skos:definition xml:lang="en">Nintendocore is a music genre that fuses aggressive styles of
      modern rock with chiptune and video game music. Nintendocore emerged from various styles of
      hardcore punk and heavy metal, and has been influenced by many other musical
      genres.</skos:definition>
    <skos:exactMatch xml:lang="en">http://dbpedia.org/resource/Nintendocore</skos:exactMatch>
    <skos:inScheme rdf:resource="http://data.europeana.eu/concept/music/genre/Music_Genre_Scheme"/>
    <skos:altLabel xml:lang="en">Nintendocore</skos:altLabel>
  </skos:Concept>

  <skos:Concept rdf:about="http://data.europeana.eu/concept/music/genre/Gypsy_punk">
    <skos:prefLabel xml:lang="en">Gypsy punk</skos:prefLabel>
    <skos:prefLabel xml:lang="cs">Gypsy punk</skos:prefLabel>
    <skos:prefLabel xml:lang="fr">Gypsy punk</skos:prefLabel>
    <skos:prefLabel xml:lang="it">Gypsy punk</skos:prefLabel>
    <skos:prefLabel xml:lang="pt">Gypsy punk</skos:prefLabel>
    <skos:prefLabel xml:lang="ro">Punk țigănesc</skos:prefLabel>
    <skos:closeMatch rdf:resource="http://rdf.freebase.com/ns/m.0c0_zz"/>
    <skos:broader rdf:resource="http://data.europeana.eu/concept/music/genre/Punk_rock_fusions"/>
    <skos:definition xml:lang="en">Gypsy punk is a hybrid musical genre that crosses traditional
      Romani music with punk rock. One of the first rock groups to incorporate elements of punk and
      Gypsy music was Motherhead Bug, which was active mostly in the early 1990s. A broader audience
      became aware of the genre after the band Gogol Bordello released the album Gypsy Punks:
      Underdog World Strike, with front man Eugene Hütz describing their performance as a
      &quot;Gypsy Punk Cabaret&quot;. The term &quot;Gypsy punk&quot; then came to describe the
      genre and then came under criticism as it was considered exploitative of Roma culture. Gogol
      Bordello have since insisted it was just the name of their album, which was then taken and
      used by the music press as a term to define the genre of their music and similar artists — not
      an offshoot term for authentic Gypsy music. &lt;p&gt; Gypsy punk bands usually combine rock
      beats and instrumentation with more traditional Gypsy instrumentation such as drums,
      tambourine, accordion, fiddle, trumpet and saxophone. In addition, due to the varied ethnic
      makeup of the Gypsy culture, many bands sing in several different languages, often switching
      language many times within a single song.</skos:definition>
    <skos:exactMatch xml:lang="en">http://dbpedia.org/resource/Gypsy_punk</skos:exactMatch>
    <skos:inScheme rdf:resource="http://data.europeana.eu/concept/music/genre/Music_Genre_Scheme"/>
    <skos:altLabel xml:lang="en">Gypsy punk</skos:altLabel>
  </skos:Concept>

  <skos:Concept rdf:about="http://data.europeana.eu/concept/music/genre/Ska_jazz">
    <skos:prefLabel xml:lang="en">Ska jazz</skos:prefLabel>
    <skos:prefLabel xml:lang="fr">Ska-jazz</skos:prefLabel>
    <skos:prefLabel xml:lang="de">Ska-Jazz</skos:prefLabel>
    <skos:prefLabel xml:lang="pl">Ska jazz</skos:prefLabel>
    <skos:prefLabel xml:lang="pt">Ska jazz</skos:prefLabel>
    <skos:prefLabel xml:lang="ru">Ска-джаз</skos:prefLabel>
    <skos:prefLabel xml:lang="es">Ska jazz</skos:prefLabel>
    <skos:prefLabel xml:lang="uk">Ска-джаз</skos:prefLabel>
    <skos:closeMatch rdf:resource="http://rdf.freebase.com/ns/m.0c90g_"/>
    <skos:broader rdf:resource="http://data.europeana.eu/concept/music/genre/Jazz_fusions"/>
    <skos:definition xml:lang="en">Ska jazz is a music genre derived by fusing the melodic content
      of jazz with the rhythmic and harmonic content of early Jamaican Music introduced by the
      &quot;Fathers of Ska&quot; in the late 1950s. The ska-jazz movement that began in New York
      during the 1990s by pioneering avant-garde jazz musicians that pushed the boundaries of reggae
      music, combining traditions with modern tendencies, using the reggae beat along with high
      improvisation and jazz harmonies, primarily by horns and percussion. &lt;p&gt; The ancient
      origin of jazz is West African music, although the instruments used, guitar, bass, saxophone,
      trombone, drums, clarinet and piano, all come from the European world. It predates rocksteady
      and was the harbinger of Jamaican reggae and English Two-tone movement. Ska is characterized
      by the staccato rhythm played on the guitar and its history can be classified into three
      periods— Jamaican reggae, also known as First Wave, the English Two-Tone era, commonly called
      Second Wave, the punk-infused Third Wave.</skos:definition>
    <skos:exactMatch xml:lang="en">http://dbpedia.org/resource/Ska_jazz</skos:exactMatch>
    <skos:inScheme rdf:resource="http://data.europeana.eu/concept/music/genre/Music_Genre_Scheme"/>
    <skos:altLabel xml:lang="en">Ska jazz</skos:altLabel>
  </skos:Concept>

  <skos:Concept rdf:about="http://data.europeana.eu/concept/music/genre/Post-metal">
    <skos:prefLabel xml:lang="en">Post-metal</skos:prefLabel>
    <skos:prefLabel xml:lang="hr">Post-metal</skos:prefLabel>
    <skos:prefLabel xml:lang="cs">Post-metal</skos:prefLabel>
    <skos:prefLabel xml:lang="da">Post-metal</skos:prefLabel>
    <skos:prefLabel xml:lang="fi">Post-metal</skos:prefLabel>
    <skos:prefLabel xml:lang="fr">Post-metal</skos:prefLabel>
    <skos:prefLabel xml:lang="de">Post-Metal</skos:prefLabel>
    <skos:prefLabel xml:lang="it">Post-metal</skos:prefLabel>
    <skos:prefLabel xml:lang="ja">ポストメタル</skos:prefLabel>
    <skos:prefLabel xml:lang="fa">پست-متال</skos:prefLabel>
    <skos:prefLabel xml:lang="pl">Post-metal</skos:prefLabel>
    <skos:prefLabel xml:lang="pt">Post-metal</skos:prefLabel>
    <skos:prefLabel xml:lang="ro">Post-metal</skos:prefLabel>
    <skos:prefLabel xml:lang="ru">Пост-метал</skos:prefLabel>
    <skos:prefLabel xml:lang="sr">Post metal</skos:prefLabel>
    <skos:prefLabel xml:lang="sk">Post-metal</skos:prefLabel>
    <skos:prefLabel xml:lang="es">Post-metal</skos:prefLabel>
    <skos:prefLabel xml:lang="sv">Post-metal</skos:prefLabel>
    <skos:prefLabel xml:lang="uk">Пост-метал</skos:prefLabel>
    <skos:closeMatch rdf:resource="http://rdf.freebase.com/ns/m.0ccxx6"/>
    <skos:broader
      rdf:resource="http://data.europeana.eu/concept/music/genre/Alternative_rock_fusions"/>
    <skos:definition xml:lang="en">Post-metal is a fusion music genre, a mixture between the genres
      of post-rock, heavy metal, and shoegazing. &lt;p&gt; Hydra Head Records owner and Isis
      frontman Aaron Turner originally termed the genre &quot;thinking man's metal&quot;,
      demonstrating that his band was trying to move away from common metal conventions.
      &quot;Post-metal&quot; is the favored name for the growing genre, but it is also referred to
      as &quot;metalgaze&quot; or &quot;shoegaze metal&quot; as a play on shoegazing, as well as
      &quot;atmospheric metal&quot;, &quot;atmospheric sludge metal&quot; or &quot;experimental
      metal&quot;, though this last term is also used to describe avant-garde
      metal.</skos:definition>
    <skos:exactMatch xml:lang="en">http://dbpedia.org/resource/Post-metal</skos:exactMatch>
    <skos:inScheme rdf:resource="http://data.europeana.eu/concept/music/genre/Music_Genre_Scheme"/>
    <skos:altLabel xml:lang="en">Post-metal</skos:altLabel>
  </skos:Concept>

  <skos:Concept rdf:about="http://data.europeana.eu/concept/music/genre/Hokum">
    <skos:prefLabel xml:lang="en">Hokum</skos:prefLabel>
    <skos:prefLabel xml:lang="de">Hokum</skos:prefLabel>
    <skos:closeMatch rdf:resource="http://rdf.freebase.com/ns/m.0dc80p"/>
    <skos:broader rdf:resource="http://data.europeana.eu/concept/music/genre/Blues_fusions"/>
    <skos:definition xml:lang="en">Hokum is a particular song type of American blues music—a
      humorous song which uses extended analogies or euphemistic terms to make sexual innuendos.
      This trope goes back to early blues recordings, and is seen from time to time in modern
      American blues and blues-rock. &lt;p&gt; An example of hokum lyrics is this sample from
      &quot;Meat Balls&quot;, by Lil Johnson, recorded about 1937, &lt;p&gt; &quot;Got out late last
      night, in the rain and sleet &lt;p&gt; Tryin' to find a butcher that grind my meat &lt;p&gt;
      Yes I'm lookin' for a butcher &lt;p&gt; He must be long and tall &lt;p&gt; If he want to grind
      my meat &lt;p&gt; 'Cause I'm wild about my meat balls.&quot;</skos:definition>
    <skos:exactMatch xml:lang="en">http://dbpedia.org/resource/Hokum</skos:exactMatch>
    <skos:inScheme rdf:resource="http://data.europeana.eu/concept/music/genre/Music_Genre_Scheme"/>
    <skos:altLabel xml:lang="en">Hokum</skos:altLabel>
  </skos:Concept>

  <skos:Concept rdf:about="http://data.europeana.eu/concept/music/genre/Bubblegum_pop">
    <skos:prefLabel xml:lang="en">Bubblegum pop</skos:prefLabel>
    <skos:prefLabel xml:lang="hr">Bubblegum pop</skos:prefLabel>
    <skos:prefLabel xml:lang="nl">Bubblegum</skos:prefLabel>
    <skos:prefLabel xml:lang="fi">Purukumipop</skos:prefLabel>
    <skos:prefLabel xml:lang="fr">Bubblegum pop</skos:prefLabel>
    <skos:prefLabel xml:lang="de">Bubblegum</skos:prefLabel>
    <skos:prefLabel xml:lang="it">Bubblegum pop</skos:prefLabel>
    <skos:prefLabel xml:lang="ja">バブルガム・ポップ</skos:prefLabel>
    <skos:prefLabel xml:lang="ko">버블검 팝</skos:prefLabel>
    <skos:prefLabel xml:lang="no">Tyggegummipop</skos:prefLabel>
    <skos:prefLabel xml:lang="pl">Bubblegum rock</skos:prefLabel>
    <skos:prefLabel xml:lang="pt">Bubblegum</skos:prefLabel>
    <skos:prefLabel xml:lang="ru">Бабблгам-поп</skos:prefLabel>
    <skos:prefLabel xml:lang="es">Bubblegum pop</skos:prefLabel>
    <skos:prefLabel xml:lang="sv">Tuggummipop</skos:prefLabel>
    <skos:prefLabel xml:lang="th">บับเบิ้ลกัม ป็อป</skos:prefLabel>
    <skos:prefLabel xml:lang="uk">Баблгам-поп</skos:prefLabel>
    <skos:prefLabel xml:lang="vi">Bubblegum pop</skos:prefLabel>
    <skos:closeMatch rdf:resource="http://rdf.freebase.com/ns/m.0dn16"/>
    <skos:broader rdf:resource="http://data.europeana.eu/concept/music/genre/Pop_music_fusions"/>
    <skos:definition xml:lang="en">Bubblegum pop is a genre of pop music with an upbeat sound
      contrived and marketed to appeal to pre-teens and teenagers, that may be produced in an
      assembly-line process, driven by producers and often using unknown singers. Bubblegum's
      classic period ran from 1967 to 1972. A second wave of bubblegum started two years later and
      ran until 1977 when disco took over and punk rock emerged. &lt;p&gt; The genre was
      predominantly a singles phenomenon rather than an album-oriented one. Also, because many acts
      were manufactured in the studio using session musicians, a large number of bubblegum songs
      were by one-hit wonders. Among the best-known acts of bubblegum's golden era are 1910 Fruitgum
      Company, The Ohio Express and The Archies, an animated group which had the most successful
      bubblegum song with &quot;Sugar, Sugar&quot;, Billboard Magazine's No. 1 single for 1969.
      Singer Tommy Roe, arguably, had the most bubblegum hits of any artist during this period,
      notably 1969's &quot;Dizzy&quot;.</skos:definition>
    <skos:exactMatch xml:lang="en">http://dbpedia.org/resource/Bubblegum_pop</skos:exactMatch>
    <skos:inScheme rdf:resource="http://data.europeana.eu/concept/music/genre/Music_Genre_Scheme"/>
    <skos:altLabel xml:lang="en">Bubblegum pop</skos:altLabel>
  </skos:Concept>

  <skos:Concept rdf:about="http://data.europeana.eu/concept/music/genre/Tech_trance">
    <skos:prefLabel xml:lang="en">Tech trance</skos:prefLabel>
    <skos:prefLabel xml:lang="nl">Techtrance</skos:prefLabel>
    <skos:prefLabel xml:lang="fi">Tech-trance</skos:prefLabel>
    <skos:prefLabel xml:lang="fr">Tech trance</skos:prefLabel>
    <skos:prefLabel xml:lang="de">Tech Trance</skos:prefLabel>
    <skos:prefLabel xml:lang="it">Tech trance</skos:prefLabel>
    <skos:prefLabel xml:lang="pl">Tech trance</skos:prefLabel>
    <skos:prefLabel xml:lang="pt">Tech trance</skos:prefLabel>
    <skos:prefLabel xml:lang="ru">Техно-транс</skos:prefLabel>
    <skos:prefLabel xml:lang="sk">Tech trance</skos:prefLabel>
    <skos:prefLabel xml:lang="uk">Тех-транс</skos:prefLabel>
    <skos:closeMatch rdf:resource="http://rdf.freebase.com/ns/m.0dwqcx"/>
    <skos:broader rdf:resource="http://data.europeana.eu/concept/music/genre/Techno_fusions"/>
    <skos:definition xml:lang="en">Tech trance, also known as techno-trance or techno/trance, is a
      sub-genre within EDM that draws upon the techno and trance genres as the name
      suggests.</skos:definition>
    <skos:exactMatch xml:lang="en">http://dbpedia.org/resource/Tech_trance</skos:exactMatch>
    <skos:inScheme rdf:resource="http://data.europeana.eu/concept/music/genre/Music_Genre_Scheme"/>
    <skos:altLabel xml:lang="en">Tech trance</skos:altLabel>
  </skos:Concept>

  <skos:Concept rdf:about="http://data.europeana.eu/concept/music/genre/Manila_Sound">
    <skos:prefLabel xml:lang="en">Manila Sound</skos:prefLabel>
    <skos:closeMatch rdf:resource="http://rdf.freebase.com/ns/m.0f850t"/>
    <skos:broader rdf:resource="http://data.europeana.eu/concept/music/genre/Pop_music_fusions"/>
    <skos:definition xml:lang="en">Manila Sound is a musical genre in the Philippines that began in
      the early 1970s in Manila, flourished and peaked in the mid to late 1970s, and waned in
      popularity by the early 1980s. It is often considered the &quot;bright side&quot; of the
      Martial Law era and has influenced all modern genres in the country by being the forerunner to
      OPM.</skos:definition>
    <skos:exactMatch xml:lang="en">http://dbpedia.org/resource/Manila_Sound</skos:exactMatch>
    <skos:inScheme rdf:resource="http://data.europeana.eu/concept/music/genre/Music_Genre_Scheme"/>
    <skos:altLabel xml:lang="en">Manila Sound</skos:altLabel>
  </skos:Concept>

  <skos:Concept rdf:about="http://data.europeana.eu/concept/music/genre/Elevator_music">
    <skos:prefLabel xml:lang="en">Elevator music</skos:prefLabel>
    <skos:prefLabel xml:lang="nl">Muzak</skos:prefLabel>
    <skos:prefLabel xml:lang="fi">Hissimusiikki</skos:prefLabel>
    <skos:prefLabel xml:lang="fr">Muzak</skos:prefLabel>
    <skos:prefLabel xml:lang="de">Muzak</skos:prefLabel>
    <skos:prefLabel xml:lang="it">Muzak</skos:prefLabel>
    <skos:prefLabel xml:lang="ja">バックグラウンドミュージック</skos:prefLabel>
    <skos:prefLabel xml:lang="no">Muzak</skos:prefLabel>
    <skos:prefLabel xml:lang="pl">Muzak</skos:prefLabel>
    <skos:prefLabel xml:lang="pt">Música de elevador</skos:prefLabel>
    <skos:prefLabel xml:lang="ru">Музыка для лифтов</skos:prefLabel>
    <skos:prefLabel xml:lang="sv">Muzak</skos:prefLabel>
    <skos:prefLabel xml:lang="tr">Asansör müziği</skos:prefLabel>
    <skos:closeMatch rdf:resource="http://rdf.freebase.com/ns/m.0fd99"/>
    <skos:broader
      rdf:resource="http://data.europeana.eu/concept/music/genre/Electronic_music_fusions"/>
    <skos:definition xml:lang="en">Elevator music refers to a type of popular music, often
      instrumental, that is commonly played through speakers at shopping malls, grocery stores,
      department stores, telephone systems, cruise ships, airliners, hotels, airports, business
      offices, and elevators. The term is also frequently applied as a generic term for any form of
      easy listening, smooth jazz, or middle of the road music, or to the type of recordings
      commonly heard on &quot;beautiful music&quot; radio stations. &lt;p&gt; Elevator music is
      typically set to a very simple melody so that it can be unobtrusively looped back to the
      beginning. The dynamic range is also normally reduced, so that the highs and lows do not
      distract listeners. In a mall or shopping center, elevator music of a specific type has been
      found to have a psychological effect: slower, more relaxed music tends to make people slow
      down and browse longer. Elevator music may also be preferred over broadcast radio stations due
      to the lack of lyrics and commercial interruptions.</skos:definition>
    <skos:exactMatch xml:lang="en">http://dbpedia.org/resource/Elevator_music</skos:exactMatch>
    <skos:inScheme rdf:resource="http://data.europeana.eu/concept/music/genre/Music_Genre_Scheme"/>
    <skos:altLabel xml:lang="en">Elevator music</skos:altLabel>
  </skos:Concept>

  <skos:Concept rdf:about="http://data.europeana.eu/concept/music/genre/Dubtronica">
    <skos:prefLabel xml:lang="en">Dubtronica</skos:prefLabel>
    <skos:prefLabel xml:lang="ru">Дабтроника</skos:prefLabel>
    <skos:prefLabel xml:lang="sk">Dubtronica</skos:prefLabel>
    <skos:prefLabel xml:lang="es">Dubtronica</skos:prefLabel>
    <skos:prefLabel xml:lang="uk">Дабтроніка</skos:prefLabel>
    <skos:closeMatch rdf:resource="http://rdf.freebase.com/ns/m.0fm3c8"/>
    <skos:broader
      rdf:resource="http://data.europeana.eu/concept/music/genre/Electronic_music_fusions"/>
    <skos:definition xml:lang="en">Dubtronica is electronic dance music influenced by dub music.
      Early examples from the 1980s are the experimental English dub of On-U Sound Records and Mad
      Professor. It is also called simply &quot;dub&quot; or &quot;techdub&quot;. &lt;p&gt;
      Dubtronica consists of electronic beats played in a downbeat manner. It is much lower in speed
      than techno and generally warmer than dance-oriented electronica. Some tracks use reggae
      toasters or singers to produce a more accessible form of the music.</skos:definition>
    <skos:exactMatch xml:lang="en">http://dbpedia.org/resource/Dubtronica</skos:exactMatch>
    <skos:inScheme rdf:resource="http://data.europeana.eu/concept/music/genre/Music_Genre_Scheme"/>
    <skos:altLabel xml:lang="en">Dubtronica</skos:altLabel>
  </skos:Concept>

  <skos:Concept rdf:about="http://data.europeana.eu/concept/music/genre/Dance-rock">
    <skos:prefLabel xml:lang="en">Dance-rock</skos:prefLabel>
    <skos:prefLabel xml:lang="cs">Dance-rock</skos:prefLabel>
    <skos:prefLabel xml:lang="it">Dance rock</skos:prefLabel>
    <skos:prefLabel xml:lang="ru">Дэнс-рок</skos:prefLabel>
    <skos:prefLabel xml:lang="sk">Dance-rock</skos:prefLabel>
    <skos:prefLabel xml:lang="th">แดนซ์ร็อก</skos:prefLabel>
    <skos:prefLabel xml:lang="uk">Денс-рок</skos:prefLabel>
    <skos:closeMatch rdf:resource="http://rdf.freebase.com/ns/m.0fp_gqk"/>
    <skos:broader
      rdf:resource="http://data.europeana.eu/concept/music/genre/Electronic_rock_fusions"/>
    <skos:definition xml:lang="en">Dance-rock is a post-disco movement connected with post-punk
      genres with fewer R&amp;B/funk influences, originated in the early 1980s, following the
      mainstream death of punk rock and disco. &lt;p&gt; Examples of early dance-rock include Gina
      X's &quot;No G.D.M.&quot;, artists such as Dinosaur L, Liquid Liquid and Polyrock, and the
      compilation album Disco Not Disco.</skos:definition>
    <skos:exactMatch xml:lang="en">http://dbpedia.org/resource/Dance-rock</skos:exactMatch>
    <skos:inScheme rdf:resource="http://data.europeana.eu/concept/music/genre/Music_Genre_Scheme"/>
    <skos:altLabel xml:lang="en">Dance-rock</skos:altLabel>
  </skos:Concept>

  <skos:Concept rdf:about="http://data.europeana.eu/concept/music/genre/Post-rock">
    <skos:prefLabel xml:lang="en">Post-rock</skos:prefLabel>
    <skos:prefLabel xml:lang="ca">Post-rock</skos:prefLabel>
    <skos:prefLabel xml:lang="cs">Post-rock</skos:prefLabel>
    <skos:prefLabel xml:lang="nl">Post-rock</skos:prefLabel>
    <skos:prefLabel xml:lang="et">Post-rock</skos:prefLabel>
    <skos:prefLabel xml:lang="fi">Post-rock</skos:prefLabel>
    <skos:prefLabel xml:lang="fr">Post-rock</skos:prefLabel>
    <skos:prefLabel xml:lang="de">Post-Rock</skos:prefLabel>
    <skos:prefLabel xml:lang="el">Post-rock</skos:prefLabel>
    <skos:prefLabel xml:lang="hu">Posztrock</skos:prefLabel>
    <skos:prefLabel xml:lang="it">Post-rock</skos:prefLabel>
    <skos:prefLabel xml:lang="ja">ポストロック</skos:prefLabel>
    <skos:prefLabel xml:lang="ko">포스트 록</skos:prefLabel>
    <skos:prefLabel xml:lang="lv">Postroks</skos:prefLabel>
    <skos:prefLabel xml:lang="no">Post-rock</skos:prefLabel>
    <skos:prefLabel xml:lang="fa">پست-راک</skos:prefLabel>
    <skos:prefLabel xml:lang="pl">Post-rock</skos:prefLabel>
    <skos:prefLabel xml:lang="pt">Post-rock</skos:prefLabel>
    <skos:prefLabel xml:lang="ro">Post-rock</skos:prefLabel>
    <skos:prefLabel xml:lang="ru">Пост-рок</skos:prefLabel>
    <skos:prefLabel xml:lang="sr">Post-rok</skos:prefLabel>
    <skos:prefLabel xml:lang="sk">Post-rock</skos:prefLabel>
    <skos:prefLabel xml:lang="es">Post-rock</skos:prefLabel>
    <skos:prefLabel xml:lang="sv">Postrock</skos:prefLabel>
    <skos:prefLabel xml:lang="th">โพสต์ร็อก</skos:prefLabel>
    <skos:prefLabel xml:lang="tr">Post rock</skos:prefLabel>
    <skos:prefLabel xml:lang="uk">Пост-рок</skos:prefLabel>
    <skos:closeMatch rdf:resource="http://rdf.freebase.com/ns/m.0g_bh"/>
    <skos:broader
      rdf:resource="http://data.europeana.eu/concept/music/genre/Alternative_rock_fusions"/>
    <skos:definition xml:lang="en">Post-rock is a subgenre of rock music characterized by the
      influence and use of instruments commonly associated with rock, but using rhythms and
      &quot;guitars as facilitators of timbre and textures&quot; not traditionally found in rock.
      Post-rock bands are often without vocals. &lt;p&gt; Don Caballero and Tortoise were among the
      more prominent bands described as post-rock in the 1990s, but their styles are very different,
      despite being instrumental bands centered on guitars and drums. As such, the term has been the
      subject of backlash from listeners and artists alike. &lt;p&gt; Although firmly rooted in the
      indie or underground scene of the 1980s and early '90s, post-rock's style often bears little
      resemblance musically to that of contemporary indie rock.</skos:definition>
    <skos:exactMatch xml:lang="en">http://dbpedia.org/resource/Post-rock</skos:exactMatch>
    <skos:inScheme rdf:resource="http://data.europeana.eu/concept/music/genre/Music_Genre_Scheme"/>
    <skos:altLabel xml:lang="en">Post-rock</skos:altLabel>
  </skos:Concept>

  <skos:Concept rdf:about="http://data.europeana.eu/concept/music/genre/Space_age_pop">
    <skos:prefLabel xml:lang="en">Space age pop</skos:prefLabel>
    <skos:prefLabel xml:lang="it">Space age pop</skos:prefLabel>
    <skos:prefLabel xml:lang="no">Space age pop</skos:prefLabel>
    <skos:prefLabel xml:lang="pt">Space age pop</skos:prefLabel>
    <skos:prefLabel xml:lang="es">Space age pop</skos:prefLabel>
    <skos:closeMatch rdf:resource="http://rdf.freebase.com/ns/m.0g0zyc"/>
    <skos:broader rdf:resource="http://data.europeana.eu/concept/music/genre/Pop_music_fusions"/>
    <skos:definition xml:lang="en">Space age pop is a music genre associated with Mexican and
      American composers and songwriters in the Space Age of the 1950s and 1960s. It is also called
      bachelor pad music or lounge music. Space age pop was inspired by the spirit of those times,
      an optimism based on the strong post-war economy and technology boom, and excitement about
      humanity's early forays into space. Although there is no specific album, date, or year when
      the genre was born, producer Irwin Chusid identifies its heyday as &quot;roughly 1954 to
      1963—from the dawn of high-fidelity to the arrival of the Beatles.&quot; &lt;p&gt; The music
      is not limited to a single style, and it is not always easily categorized. There are several
      styles that can be recognized as an influence: classical composers like Ravel and Debussy, the
      big bands of the 1940s, and different exotic styles, such as samba, latin, and calypso jazz.
      Space Age pop is related to the genres of lounge music, exotica, or beautiful music, and may
      be regarded as a precursor to the musical genre of space music.</skos:definition>
    <skos:exactMatch xml:lang="en">http://dbpedia.org/resource/Space_age_pop</skos:exactMatch>
    <skos:inScheme rdf:resource="http://data.europeana.eu/concept/music/genre/Music_Genre_Scheme"/>
    <skos:altLabel xml:lang="en">Space age pop</skos:altLabel>
  </skos:Concept>

  <skos:Concept rdf:about="http://data.europeana.eu/concept/music/genre/Skweee">
    <skos:prefLabel xml:lang="en">Skweee</skos:prefLabel>
    <skos:prefLabel xml:lang="cs">Skweee</skos:prefLabel>
    <skos:prefLabel xml:lang="fi">Skweee</skos:prefLabel>
    <skos:prefLabel xml:lang="fr">Skweee</skos:prefLabel>
    <skos:prefLabel xml:lang="de">Skweee</skos:prefLabel>
    <skos:prefLabel xml:lang="fa">اسکویی</skos:prefLabel>
    <skos:prefLabel xml:lang="pl">Skweee</skos:prefLabel>
    <skos:prefLabel xml:lang="ru">Скви</skos:prefLabel>
    <skos:prefLabel xml:lang="sv">Skweee</skos:prefLabel>
    <skos:closeMatch rdf:resource="http://rdf.freebase.com/ns/m.0gcj2x"/>
    <skos:broader
      rdf:resource="http://data.europeana.eu/concept/music/genre/Electronic_music_fusions"/>
    <skos:definition xml:lang="en">Skweee is a musical style, with origin in Sweden and Finland.
      Skweee combines simple synth/chiptune leads and basslines with funk, R&amp;B or soul-like
      rhythms, overall rendering a stripped-down funky sound. The tracks are mostly entirely
      instrumental, though there are exceptions. The name Skweee was coined by Daniel Savio, one of
      the originators of the emerging sound. The name refers to the use of vintage synthesizers in
      the production process, where the aim is to &quot;squeeze out&quot; the most interesting
      sounds possible. &lt;p&gt; The current producers are both newcomers and old, experienced
      producers from the Scandinavian electro and electronica environment. &lt;p&gt; Skweeelicious,
      a blog dedicated to skweee, and community sites such as MySpace and Nation of Skweee have
      played a major role in the distribution of skweee music and public exposure of the genre.
      &lt;p&gt; The major outlets of skweee music are the Swedish record label Flogsta Danshall and
      Finnish record label Harmönia. Norwegian Dødpop, Canadian Ancient Robot, US Losonofono, US
      Titched, US Poisonous Gases, Spanish Lo Fi Funk, Finnish Mässy, and French Mazout have since
      been added to this family.</skos:definition>
    <skos:exactMatch xml:lang="en">http://dbpedia.org/resource/Skweee</skos:exactMatch>
    <skos:inScheme rdf:resource="http://data.europeana.eu/concept/music/genre/Music_Genre_Scheme"/>
    <skos:altLabel xml:lang="en">Skweee</skos:altLabel>
  </skos:Concept>

  <skos:Concept rdf:about="http://data.europeana.eu/concept/music/genre/Psychedelic_pop">
    <skos:prefLabel xml:lang="en">Psychedelic pop</skos:prefLabel>
    <skos:prefLabel xml:lang="cs">Psychedelický pop</skos:prefLabel>
    <skos:prefLabel xml:lang="nl">Psychedelic pop</skos:prefLabel>
    <skos:prefLabel xml:lang="fi">Psykedeelinen pop</skos:prefLabel>
    <skos:prefLabel xml:lang="fr">Pop psychédélique</skos:prefLabel>
    <skos:prefLabel xml:lang="id">Psychedelic pop</skos:prefLabel>
    <skos:prefLabel xml:lang="it">Pop psichedelico</skos:prefLabel>
    <skos:prefLabel xml:lang="pl">Peaking Lights</skos:prefLabel>
    <skos:prefLabel xml:lang="pt">Pop psicodélico</skos:prefLabel>
    <skos:prefLabel xml:lang="ru">Психоделический поп</skos:prefLabel>
    <skos:closeMatch rdf:resource="http://rdf.freebase.com/ns/m.0grjmv"/>
    <skos:broader rdf:resource="http://data.europeana.eu/concept/music/genre/Pop_music_fusions"/>
    <skos:definition xml:lang="en">Psychedelic pop is a psychedelic musical style inspired by the
      sounds of psychedelic folk and psychedelic rock, but applied to a pop music setting. It
      reached its peak during the late 1960s, declining rapidly in the early
      1970s.</skos:definition>
    <skos:exactMatch xml:lang="en">http://dbpedia.org/resource/Psychedelic_pop</skos:exactMatch>
    <skos:inScheme rdf:resource="http://data.europeana.eu/concept/music/genre/Music_Genre_Scheme"/>
    <skos:altLabel xml:lang="en">Psychedelic pop</skos:altLabel>
  </skos:Concept>

  <skos:Concept rdf:about="http://data.europeana.eu/concept/music/genre/Gypsy_jazz">
    <skos:prefLabel xml:lang="en">Gypsy jazz</skos:prefLabel>
    <skos:prefLabel xml:lang="hr">Gypsy jazz</skos:prefLabel>
    <skos:prefLabel xml:lang="da">Sigøjnerjazz</skos:prefLabel>
    <skos:prefLabel xml:lang="nl">Gipsy jazz</skos:prefLabel>
    <skos:prefLabel xml:lang="fr">Jazz manouche</skos:prefLabel>
    <skos:prefLabel xml:lang="de">Gypsy-Jazz</skos:prefLabel>
    <skos:prefLabel xml:lang="hu">Szinti szving</skos:prefLabel>
    <skos:prefLabel xml:lang="id">Gypsy jazz</skos:prefLabel>
    <skos:prefLabel xml:lang="it">Jazz manouche</skos:prefLabel>
    <skos:prefLabel xml:lang="ja">ジプシー・スウィング</skos:prefLabel>
    <skos:prefLabel xml:lang="ko">집시 재즈</skos:prefLabel>
    <skos:prefLabel xml:lang="pt">Gypsy jazz</skos:prefLabel>
    <skos:prefLabel xml:lang="ru">Джаз-мануш</skos:prefLabel>
    <skos:prefLabel xml:lang="es">Gypsy jazz</skos:prefLabel>
    <skos:prefLabel xml:lang="sv">Gypsy jazz</skos:prefLabel>
    <skos:prefLabel xml:lang="uk">Циганський джаз</skos:prefLabel>
    <skos:closeMatch rdf:resource="http://rdf.freebase.com/ns/m.0gz8z_"/>
    <skos:broader rdf:resource="http://data.europeana.eu/concept/music/genre/Jazz_fusions"/>
    <skos:definition xml:lang="en">Gypsy jazz is a style of jazz music often said to have been
      started by guitarist Jean &quot;Django&quot; Reinhardt in the 1930s. Because its origins are
      largely in France it is often called by the French name, &quot;jazz manouche&quot;, or
      alternatively, &quot;manouche jazz&quot;, even in English language sources. Some modern
      dictionaries recommend avoiding using the word &quot;gypsy&quot; because it is felt to have
      been tainted by its frequent use as a pejorative, dictionaries do not, however, caution
      against use of the term &quot;gypsy jazz.&quot; &lt;p&gt; Django was foremost among a group of
      Romani guitarists working in and around Paris in the 1930s through the 1950s, a group which
      also included the brothers Baro, Sarane, and Matelo Ferret and Reinhardt's brother Joseph
      &quot;Nin-Nin&quot; Reinhardt. &lt;p&gt; Many of the musicians in this style worked in Paris
      in various popular Musette ensembles. The Musette style waltz remains an important component
      in the Gypsy jazz repertoire. Reinhardt was noted for combining a dark, chromatic Gypsy flavor
      with the swing articulation of the period. This combination is critical to this style of jazz.
      In addition to this, his approach continues to form the basis for contemporary Gypsy jazz
      guitar.</skos:definition>
    <skos:exactMatch xml:lang="en">http://dbpedia.org/resource/Gypsy_jazz</skos:exactMatch>
    <skos:inScheme rdf:resource="http://data.europeana.eu/concept/music/genre/Music_Genre_Scheme"/>
    <skos:altLabel xml:lang="en">Jazz manouche</skos:altLabel>
    <skos:altLabel xml:lang="en">Gypsy jazz</skos:altLabel>
  </skos:Concept>

  <skos:Concept rdf:about="http://data.europeana.eu/concept/music/genre/New_rave">
    <skos:prefLabel xml:lang="en">New rave</skos:prefLabel>
    <skos:prefLabel xml:lang="cs">New Rave</skos:prefLabel>
    <skos:prefLabel xml:lang="da">Garagepop</skos:prefLabel>
    <skos:prefLabel xml:lang="fr">New rave</skos:prefLabel>
    <skos:prefLabel xml:lang="el">New rave</skos:prefLabel>
    <skos:prefLabel xml:lang="it">New rave</skos:prefLabel>
    <skos:prefLabel xml:lang="ja">ニューレイヴ</skos:prefLabel>
    <skos:prefLabel xml:lang="fa">نیو ریو</skos:prefLabel>
    <skos:prefLabel xml:lang="pl">New rave</skos:prefLabel>
    <skos:prefLabel xml:lang="pt">New rave</skos:prefLabel>
    <skos:prefLabel xml:lang="ru">Нью-рейв</skos:prefLabel>
    <skos:prefLabel xml:lang="sk">New rave</skos:prefLabel>
    <skos:prefLabel xml:lang="es">New rave</skos:prefLabel>
    <skos:prefLabel xml:lang="uk">Нью-рейв</skos:prefLabel>
    <skos:closeMatch rdf:resource="http://rdf.freebase.com/ns/m.0h00cv"/>
    <skos:broader
      rdf:resource="http://data.europeana.eu/concept/music/genre/Electronic_rock_fusions"/>
    <skos:definition xml:lang="en">New rave is several types of music that fuse elements of
      electronic music, new wave, rock, indie, techno, mashup, breakbeat hardcore and electro house.
      It is most commonly applied to a British-based music scene between 2005 and late 2008 of
      fast-paced electronica-influenced indie music that celebrated the late 1980s Madchester and
      rave scenes through the use of neon colours and using the term 'raving' to refer to going
      nightclubbing. &lt;p&gt; The British music magazine NME is largely responsible for
      popularising the term throughout 2006 and 2007, until claiming in mid-2008 reviews that
      &quot;New Rave is over&quot;. The genre has connotations of being a &quot;new&quot; version of
      rave as well as being a play on the term &quot;new wave&quot;. &lt;p&gt; Klaxons, Trash
      Fashion, New Young Pony Club, Hadouken!, Late of the Pier and Shitdisco are generally accepted
      as the main exponents of the genre. &lt;p&gt; The aesthetics of the new rave scene are similar
      to those of the original rave scene, being mostly centred around psychedelic visual effects.
      Glowsticks, neon and other lights are common, and followers of the scene often dress in
      extremely bright and fluorescent colored clothing. New Rave has been defined more by the image
      and aesthetic of its bands and supporters, than by its music. Trash Fashion lead singer, Jet
      Storm, and Electro heroine Uffie, have been described as the scene's very own pin ups.
      Nevertheless, the use of electronic instruments, a musical fusion of rock and dance styles,
      and a particular anarchic, trashy energy are certainly key elements.</skos:definition>
    <skos:exactMatch xml:lang="en">http://dbpedia.org/resource/New_rave</skos:exactMatch>
    <skos:inScheme rdf:resource="http://data.europeana.eu/concept/music/genre/Music_Genre_Scheme"/>
    <skos:altLabel xml:lang="en">Nu Rave</skos:altLabel>
    <skos:altLabel xml:lang="en">New rave</skos:altLabel>
  </skos:Concept>

  <skos:Concept rdf:about="http://data.europeana.eu/concept/music/genre/Hard_NRG">
    <skos:prefLabel xml:lang="en">Hard NRG</skos:prefLabel>
    <skos:prefLabel xml:lang="fi">Hard NRG</skos:prefLabel>
    <skos:closeMatch rdf:resource="http://rdf.freebase.com/ns/m.0h7gl8"/>
    <skos:broader rdf:resource="http://data.europeana.eu/concept/music/genre/House_music_fusions"/>
    <skos:definition xml:lang="en">Hard NRG is an electronic music genre similar in structure to UK
      hard house. The main difference is in the musical/thematic content of each style. &lt;p&gt;
      Where UK hard house has uplifting, playfully fun and tough elements, NRG is ominous, dark,
      aggressive and relentless with its distressed, menacing and gritty sounds on a slightly faster
      BPM than UK hard house. &lt;p&gt; In regard to the mechanics of the scene, many of the labels
      have made a shift from purely vinyl releases to CD single releases and digital downloads.
      &lt;p&gt; Record labels which produce the genre include Vicious Circle, Flashpoint, Tidy Trax,
      Kaktai, Tonka Trax, Tinrib Digital, Noir Records and Noir Digital.</skos:definition>
    <skos:exactMatch xml:lang="en">http://dbpedia.org/resource/Hard_NRG</skos:exactMatch>
    <skos:inScheme rdf:resource="http://data.europeana.eu/concept/music/genre/Music_Genre_Scheme"/>
    <skos:altLabel xml:lang="en">Hard NRG</skos:altLabel>
  </skos:Concept>

  <skos:Concept rdf:about="http://data.europeana.eu/concept/music/genre/Folk_metal">
    <skos:prefLabel xml:lang="en">Folk metal</skos:prefLabel>
    <skos:prefLabel xml:lang="bg">Фолк метъл</skos:prefLabel>
    <skos:prefLabel xml:lang="ca">Folk metal</skos:prefLabel>
    <skos:prefLabel xml:lang="hr">Folk metal</skos:prefLabel>
    <skos:prefLabel xml:lang="cs">Folk metal</skos:prefLabel>
    <skos:prefLabel xml:lang="da">Folk metal</skos:prefLabel>
    <skos:prefLabel xml:lang="nl">Folkmetal</skos:prefLabel>
    <skos:prefLabel xml:lang="et">Folk metal</skos:prefLabel>
    <skos:prefLabel xml:lang="fi">Folk metal</skos:prefLabel>
    <skos:prefLabel xml:lang="fr">Folk metal</skos:prefLabel>
    <skos:prefLabel xml:lang="de">Folk Metal</skos:prefLabel>
    <skos:prefLabel xml:lang="el">Folk metal</skos:prefLabel>
    <skos:prefLabel xml:lang="hu">Folk metal</skos:prefLabel>
    <skos:prefLabel xml:lang="it">Folk metal</skos:prefLabel>
    <skos:prefLabel xml:lang="ja">フォーク・メタル</skos:prefLabel>
    <skos:prefLabel xml:lang="ko">포크 메탈</skos:prefLabel>
    <skos:prefLabel xml:lang="lv">Folkmetāls</skos:prefLabel>
    <skos:prefLabel xml:lang="lt">Folklorinis metalas</skos:prefLabel>
    <skos:prefLabel xml:lang="no">Folk metal</skos:prefLabel>
    <skos:prefLabel xml:lang="fa">فولک متال</skos:prefLabel>
    <skos:prefLabel xml:lang="pl">Folk metal</skos:prefLabel>
    <skos:prefLabel xml:lang="pt">Folk metal</skos:prefLabel>
    <skos:prefLabel xml:lang="ro">Folk metal</skos:prefLabel>
    <skos:prefLabel xml:lang="ru">Фолк-метал</skos:prefLabel>
    <skos:prefLabel xml:lang="sk">Folk metal</skos:prefLabel>
    <skos:prefLabel xml:lang="sl">Folk metal</skos:prefLabel>
    <skos:prefLabel xml:lang="es">Folk metal</skos:prefLabel>
    <skos:prefLabel xml:lang="sv">Folk metal</skos:prefLabel>
    <skos:prefLabel xml:lang="tr">Folk metal</skos:prefLabel>
    <skos:prefLabel xml:lang="uk">Фолк-метал</skos:prefLabel>
    <skos:closeMatch rdf:resource="http://rdf.freebase.com/ns/m.0jrgr"/>
    <skos:broader
      rdf:resource="http://data.europeana.eu/concept/music/genre/Heavy_metal_music_fusions"/>
    <skos:definition xml:lang="en">Folk metal is a sub-genre of heavy metal music that developed in
      Europe during the 1990s, a fusion of heavy metal and traditional folk music. This includes the
      widespread use of folk instruments and, to a lesser extent, traditional singing styles.
      &lt;p&gt; The earliest folk metal band was Skyclad from England. Their debut album The Wayward
      Sons of Mother Earth was released in 1990. It was not until 1994 and 1995 that other early
      contributors in the genre began to emerge from different regions of Europe as well as in
      Israel. Among these early groups, the Irish band Cruachan and the German band Subway to Sally
      each spearheaded a different regional variation that over time became known as Celtic metal
      and medieval metal respectively. Despite their contributions, folk metal remained little known
      with few representatives during the 1990s. It was not until the early 2000s when the genre
      exploded into prominence, particularly in Finland with the efforts of such groups as
      Finntroll, Ensiferum, Korpiklaani, Turisas, and Moonsorrow. &lt;p&gt; The music of folk metal
      is characterised by its diversity with bands known to perform different styles of both heavy
      metal music and folk music.</skos:definition>
    <skos:exactMatch xml:lang="en">http://dbpedia.org/resource/Folk_metal</skos:exactMatch>
    <skos:inScheme rdf:resource="http://data.europeana.eu/concept/music/genre/Music_Genre_Scheme"/>
    <skos:altLabel xml:lang="en">Folk metal</skos:altLabel>
  </skos:Concept>

  <skos:Concept rdf:about="http://data.europeana.eu/concept/music/genre/Electro_house">
    <skos:prefLabel xml:lang="en">Electro house</skos:prefLabel>
    <skos:prefLabel xml:lang="cs">Electro house</skos:prefLabel>
    <skos:prefLabel xml:lang="nl">Electrohouse</skos:prefLabel>
    <skos:prefLabel xml:lang="fi">Electro house</skos:prefLabel>
    <skos:prefLabel xml:lang="fr">Complextro</skos:prefLabel>
    <skos:prefLabel xml:lang="de">Complextro</skos:prefLabel>
    <skos:prefLabel xml:lang="it">Electro house</skos:prefLabel>
    <skos:prefLabel xml:lang="ja">エレクトロ・ハウス</skos:prefLabel>
    <skos:prefLabel xml:lang="ko">일렉트로 하우스</skos:prefLabel>
    <skos:prefLabel xml:lang="no">Electro house</skos:prefLabel>
    <skos:prefLabel xml:lang="fa">الکترو هاوس</skos:prefLabel>
    <skos:prefLabel xml:lang="pl">Electro house</skos:prefLabel>
    <skos:prefLabel xml:lang="pt">Complextro</skos:prefLabel>
    <skos:prefLabel xml:lang="ro">Electro House</skos:prefLabel>
    <skos:prefLabel xml:lang="ru">Электро-хаус</skos:prefLabel>
    <skos:prefLabel xml:lang="sk">Electro house</skos:prefLabel>
    <skos:prefLabel xml:lang="es">Electro house</skos:prefLabel>
    <skos:prefLabel xml:lang="sv">Electrohouse</skos:prefLabel>
    <skos:prefLabel xml:lang="th">อิเล็กทรอเฮาส์</skos:prefLabel>
    <skos:prefLabel xml:lang="uk">Електро-хауз</skos:prefLabel>
    <skos:closeMatch rdf:resource="http://rdf.freebase.com/ns/m.0k0r0n7"/>
    <skos:broader rdf:resource="http://data.europeana.eu/concept/music/genre/House_music_fusions"/>
    <skos:definition xml:lang="en">Electro house is a form of house music. Electro house's
      influences include electro, electroclash, pop, synthpop, and tech house. The term has been
      used to describe the music of many DJ Mag Top 100 DJs, including Deadmau5, Kaskade, Knife
      Party, Madeon, Porter Robinson, and Zedd.</skos:definition>
    <skos:exactMatch xml:lang="en">http://dbpedia.org/resource/Electro_house</skos:exactMatch>
    <skos:inScheme rdf:resource="http://data.europeana.eu/concept/music/genre/Music_Genre_Scheme"/>
    <skos:altLabel xml:lang="en">Synth house</skos:altLabel>
    <skos:altLabel xml:lang="en">Complextro</skos:altLabel>
    <skos:altLabel xml:lang="en">Electro house</skos:altLabel>
  </skos:Concept>

  <skos:Concept rdf:about="http://data.europeana.eu/concept/music/genre/Intelligent_dance_music">
    <skos:prefLabel xml:lang="en">Intelligent dance music</skos:prefLabel>
    <skos:prefLabel xml:lang="cs">IDM</skos:prefLabel>
    <skos:prefLabel xml:lang="nl">Intelligent Dance Music</skos:prefLabel>
    <skos:prefLabel xml:lang="et">IDM</skos:prefLabel>
    <skos:prefLabel xml:lang="fi">IDM</skos:prefLabel>
    <skos:prefLabel xml:lang="fr">Intelligent dance music</skos:prefLabel>
    <skos:prefLabel xml:lang="de">Intelligent Dance Music</skos:prefLabel>
    <skos:prefLabel xml:lang="hu">IDM</skos:prefLabel>
    <skos:prefLabel xml:lang="it">Intelligent dance music</skos:prefLabel>
    <skos:prefLabel xml:lang="ja">インテリジェント・ダンス・ミュージック</skos:prefLabel>
    <skos:prefLabel xml:lang="ko">인텔리전트 댄스 뮤직</skos:prefLabel>
    <skos:prefLabel xml:lang="lt">IDM</skos:prefLabel>
    <skos:prefLabel xml:lang="no">Intelligent dance music</skos:prefLabel>
    <skos:prefLabel xml:lang="fa">موسیقی رقص هوشمند</skos:prefLabel>
    <skos:prefLabel xml:lang="pl">IDM</skos:prefLabel>
    <skos:prefLabel xml:lang="pt">IDM</skos:prefLabel>
    <skos:prefLabel xml:lang="ro">IDM</skos:prefLabel>
    <skos:prefLabel xml:lang="ru">IDM</skos:prefLabel>
    <skos:prefLabel xml:lang="es">Intelligent dance music</skos:prefLabel>
    <skos:prefLabel xml:lang="sv">Intelligent dance music</skos:prefLabel>
    <skos:prefLabel xml:lang="th">ดนตรีอินเทลลิเจนต์แดนซ์</skos:prefLabel>
    <skos:prefLabel xml:lang="uk">IDM</skos:prefLabel>
    <skos:closeMatch rdf:resource="http://rdf.freebase.com/ns/m.0kz10"/>
    <skos:broader
      rdf:resource="http://data.europeana.eu/concept/music/genre/Electronic_music_fusions"/>
    <skos:definition xml:lang="en">Intelligent dance music is a form of electronic music that
      emerged in the early 1990s. It was originally influenced by developments in underground dance
      music such as Detroit techno and various breakbeat styles that were emerging in the UK at that
      time. Stylistically, IDM tended to rely upon individualistic experimentation rather than
      adhering to musical characteristics associated with specific genres of dance music. The range
      of post-techno styles to emerge in the early 1990s were described variously as &quot;art
      techno&quot;, &quot;ambient techno&quot;, &quot;intelligent techno&quot;, and
      &quot;electronica&quot;. In the United States, the latter is often used as a catchall term to
      describe not only downtempo or downbeat/non-dance electronic music but also EDM. &lt;p&gt; The
      term &quot;IDM&quot; is said to have originated in the United States in 1993 with the
      formation of the &quot;IDM list&quot;, an electronic mailing list originally chartered for the
      discussion of music by a number of prominent English artists, especially those appearing on a
      1992 Warp Records compilation called Artificial Intelligence.</skos:definition>
    <skos:exactMatch xml:lang="en"
      >http://dbpedia.org/resource/Intelligent_dance_music</skos:exactMatch>
    <skos:inScheme rdf:resource="http://data.europeana.eu/concept/music/genre/Music_Genre_Scheme"/>
    <skos:altLabel xml:lang="en">IDM</skos:altLabel>
    <skos:altLabel xml:lang="en">Intelligent dance music</skos:altLabel>
  </skos:Concept>

  <skos:Concept rdf:about="http://data.europeana.eu/concept/music/genre/Chiptune">
    <skos:prefLabel xml:lang="en">Chiptune</skos:prefLabel>
    <skos:prefLabel xml:lang="ca">8 bit</skos:prefLabel>
    <skos:prefLabel xml:lang="hr">Chiptune</skos:prefLabel>
    <skos:prefLabel xml:lang="cs">Chiptune</skos:prefLabel>
    <skos:prefLabel xml:lang="nl">Chiptune</skos:prefLabel>
    <skos:prefLabel xml:lang="fi">Chiptune</skos:prefLabel>
    <skos:prefLabel xml:lang="fr">Chiptune</skos:prefLabel>
    <skos:prefLabel xml:lang="de">Chiptune</skos:prefLabel>
    <skos:prefLabel xml:lang="it">Chiptune</skos:prefLabel>
    <skos:prefLabel xml:lang="ja">チップチューン</skos:prefLabel>
    <skos:prefLabel xml:lang="ko">칩튠</skos:prefLabel>
    <skos:prefLabel xml:lang="lt">Chiptune</skos:prefLabel>
    <skos:prefLabel xml:lang="fa">چیپ تیون</skos:prefLabel>
    <skos:prefLabel xml:lang="pl">Chiptune</skos:prefLabel>
    <skos:prefLabel xml:lang="pt">Chiptune</skos:prefLabel>
    <skos:prefLabel xml:lang="ru">Чиптюн</skos:prefLabel>
    <skos:prefLabel xml:lang="sr">Чиптјун</skos:prefLabel>
    <skos:prefLabel xml:lang="es">Chiptunes</skos:prefLabel>
    <skos:prefLabel xml:lang="sv">Chipmusik</skos:prefLabel>
    <skos:prefLabel xml:lang="uk">Чіптюн</skos:prefLabel>
    <skos:closeMatch rdf:resource="http://rdf.freebase.com/ns/m.0lc1r"/>
    <skos:broader
      rdf:resource="http://data.europeana.eu/concept/music/genre/Electronic_music_fusions"/>
    <skos:definition xml:lang="en">A chiptune, also known as chip music or 8-bit music, is
      synthesized electronic music produced by the sound chips of vintage computers, video game
      consoles, and arcade machines, as well as with other methods such as emulation. In the early
      1980s, personal computers became less expensive and more accessible than they had previously
      been. This led to a proliferation of outdated personal computers and game consoles that had
      been abandoned by consumers as they upgraded to newer machines. They were in low demand by
      consumers as a whole, and not difficult to find, making them a highly accessible and
      affordable method of creating sound or art. While it has been a mostly underground genre,
      chiptune has had periods of moderate popularity in the 1980s and 21st century, and has
      influenced the development of electronic dance music.</skos:definition>
    <skos:exactMatch xml:lang="en">http://dbpedia.org/resource/Chiptune</skos:exactMatch>
    <skos:inScheme rdf:resource="http://data.europeana.eu/concept/music/genre/Music_Genre_Scheme"/>
    <skos:altLabel xml:lang="en">chiptunes</skos:altLabel>
    <skos:altLabel xml:lang="en">Chiptune</skos:altLabel>
  </skos:Concept>

  <skos:Concept rdf:about="http://data.europeana.eu/concept/music/genre/Industrial_music">
    <skos:prefLabel xml:lang="en">Industrial music</skos:prefLabel>
    <skos:prefLabel xml:lang="bg">Индъстриъл</skos:prefLabel>
    <skos:prefLabel xml:lang="ca">Música industrial</skos:prefLabel>
    <skos:prefLabel xml:lang="cs">Industriál</skos:prefLabel>
    <skos:prefLabel xml:lang="da">Industrial</skos:prefLabel>
    <skos:prefLabel xml:lang="nl">Industrial</skos:prefLabel>
    <skos:prefLabel xml:lang="fi">Industrial</skos:prefLabel>
    <skos:prefLabel xml:lang="fr">Musique industrielle</skos:prefLabel>
    <skos:prefLabel xml:lang="de">Industrial</skos:prefLabel>
    <skos:prefLabel xml:lang="hu">Indusztriális zene</skos:prefLabel>
    <skos:prefLabel xml:lang="id">Industrial</skos:prefLabel>
    <skos:prefLabel xml:lang="it">Musica industriale</skos:prefLabel>
    <skos:prefLabel xml:lang="ja">インダストリアル</skos:prefLabel>
    <skos:prefLabel xml:lang="ko">인더스트리얼 음악</skos:prefLabel>
    <skos:prefLabel xml:lang="lv">Industriālā mūzika</skos:prefLabel>
    <skos:prefLabel xml:lang="lt">Industrial</skos:prefLabel>
    <skos:prefLabel xml:lang="no">Industrimusikk</skos:prefLabel>
    <skos:prefLabel xml:lang="fa">موسیقی اینداستریال</skos:prefLabel>
    <skos:prefLabel xml:lang="pl">Industrial</skos:prefLabel>
    <skos:prefLabel xml:lang="pt">Música industrial</skos:prefLabel>
    <skos:prefLabel xml:lang="ro">Industrial</skos:prefLabel>
    <skos:prefLabel xml:lang="ru">Индастриал</skos:prefLabel>
    <skos:prefLabel xml:lang="sk">Industriálna hudba</skos:prefLabel>
    <skos:prefLabel xml:lang="sl">Industrialna glasba</skos:prefLabel>
    <skos:prefLabel xml:lang="es">Música industrial</skos:prefLabel>
    <skos:prefLabel xml:lang="sv">Industrial</skos:prefLabel>
    <skos:prefLabel xml:lang="th">ดนตรีอินดัสเทรียล</skos:prefLabel>
    <skos:prefLabel xml:lang="tr">Endüstriyel müzik</skos:prefLabel>
    <skos:prefLabel xml:lang="uk">Індастріал</skos:prefLabel>
    <skos:closeMatch rdf:resource="http://rdf.freebase.com/ns/m.0mmp3"/>
    <skos:broader
      rdf:resource="http://data.europeana.eu/concept/music/genre/Electronic_music_fusions"/>
    <skos:definition xml:lang="en">Industrial music is a style of experimental music that draws on
      transgressive and provocative themes. The term was coined in the mid-1970s with the founding
      of Industrial Records by the band Throbbing Gristle, and the creation of the slogan
      &quot;industrial music for industrial people&quot;. In general, the style is harsh and
      challenging. Allmusic defines industrial as the &quot;most abrasive and aggressive fusion of
      rock and electronic music&quot;, &quot;initially a blend of avant-garde electronics
      experiments and punk provocation&quot;. &lt;p&gt; The first industrial artists experimented
      with noise and aesthetically controversial topics, musically and visually, such as fascism,
      serial killers and the occult. Their production was not limited to music, but included mail
      art, performance art, installation pieces and other art forms. Prominent industrial musicians
      include Throbbing Gristle, SPK, Boyd Rice, Cabaret Voltaire, and Z'EV. The precursors that
      influenced the development of the genre included acts such as electronic group Kraftwerk,
      experimental rock acts such as The Velvet Underground and Frank Zappa, psychedelic rock
      artists such as Jimi Hendrix, and composers such as John Cage.</skos:definition>
    <skos:exactMatch xml:lang="en">http://dbpedia.org/resource/Industrial_music</skos:exactMatch>
    <skos:inScheme rdf:resource="http://data.europeana.eu/concept/music/genre/Music_Genre_Scheme"/>
    <skos:altLabel xml:lang="en">Industrial music</skos:altLabel>
  </skos:Concept>

  <skos:Concept rdf:about="http://data.europeana.eu/concept/music/genre/Electronicore">
    <skos:prefLabel xml:lang="en">Electronicore</skos:prefLabel>
    <skos:prefLabel xml:lang="fr">Electronicore</skos:prefLabel>
    <skos:prefLabel xml:lang="de">Trancecore</skos:prefLabel>
    <skos:prefLabel xml:lang="it">Electronicore</skos:prefLabel>
    <skos:prefLabel xml:lang="ja">エレクトロニコア</skos:prefLabel>
    <skos:prefLabel xml:lang="pt">Electronicore</skos:prefLabel>
    <skos:prefLabel xml:lang="ru">Электроникор</skos:prefLabel>
    <skos:prefLabel xml:lang="sk">Electronicore</skos:prefLabel>
    <skos:prefLabel xml:lang="uk">Електронікор</skos:prefLabel>
    <skos:closeMatch rdf:resource="http://rdf.freebase.com/ns/m.0n4b8qj"/>
    <skos:broader rdf:resource="http://data.europeana.eu/concept/music/genre/Rock_music_fusions"/>
    <skos:definition xml:lang="en">Electronicore describes a stylistic fusion of post-hardcore and
      metalcore with electronic music, specifically electronica. Notable artists of this genre have
      originated from England, the United States, Australia, Canada, France, and Hong
      Kong.</skos:definition>
    <skos:exactMatch xml:lang="en">http://dbpedia.org/resource/Electronicore</skos:exactMatch>
    <skos:inScheme rdf:resource="http://data.europeana.eu/concept/music/genre/Music_Genre_Scheme"/>
    <skos:altLabel xml:lang="en">Electronicore</skos:altLabel>
  </skos:Concept>

  <skos:Concept rdf:about="http://data.europeana.eu/concept/music/genre/Industrial_rock">
    <skos:prefLabel xml:lang="en">Industrial rock</skos:prefLabel>
    <skos:prefLabel xml:lang="cs">Industrial rock</skos:prefLabel>
    <skos:prefLabel xml:lang="nl">Industrial rock</skos:prefLabel>
    <skos:prefLabel xml:lang="fr">Rock industriel</skos:prefLabel>
    <skos:prefLabel xml:lang="de">Industrial Rock</skos:prefLabel>
    <skos:prefLabel xml:lang="it">Industrial rock</skos:prefLabel>
    <skos:prefLabel xml:lang="ja">インダストリアル・ロック</skos:prefLabel>
    <skos:prefLabel xml:lang="ko">인더스트리얼 록</skos:prefLabel>
    <skos:prefLabel xml:lang="lv">Industriālais roks</skos:prefLabel>
    <skos:prefLabel xml:lang="fa">اینداستریال راک</skos:prefLabel>
    <skos:prefLabel xml:lang="pl">Rock industrialny</skos:prefLabel>
    <skos:prefLabel xml:lang="pt">Rock industrial</skos:prefLabel>
    <skos:prefLabel xml:lang="ru">Индастриал-рок</skos:prefLabel>
    <skos:prefLabel xml:lang="sk">Industriálny rock</skos:prefLabel>
    <skos:prefLabel xml:lang="es">Rock industrial</skos:prefLabel>
    <skos:prefLabel xml:lang="sv">Industrirock</skos:prefLabel>
    <skos:prefLabel xml:lang="th">อินดัสเทรียลร็อก</skos:prefLabel>
    <skos:prefLabel xml:lang="tr">Endüstriyel rock</skos:prefLabel>
    <skos:prefLabel xml:lang="uk">Індастріал-рок</skos:prefLabel>
    <skos:closeMatch rdf:resource="http://rdf.freebase.com/ns/m.0xv2x"/>
    <skos:broader
      rdf:resource="http://data.europeana.eu/concept/music/genre/Electronic_music_fusions"/>
    <skos:definition xml:lang="en">Industrial rock is a musical genre that fuses industrial music
      and specific rock subgenres. Industrial rock spawned and is often confused with industrial
      metal. The early fusions of industrial music and rock were practiced by a handful of post-punk
      groups, including Nine Inch Nails, Chrome, Killing Joke, Swans, Foetus and Big Black. Artists
      such as Nine Inch Nails and Marilyn Manson propelled the genre to mainstream
      status.</skos:definition>
    <skos:exactMatch xml:lang="en">http://dbpedia.org/resource/Industrial_rock</skos:exactMatch>
    <skos:inScheme rdf:resource="http://data.europeana.eu/concept/music/genre/Music_Genre_Scheme"/>
    <skos:altLabel xml:lang="en">Industrial rock</skos:altLabel>
  </skos:Concept>

  <skos:Concept rdf:about="http://data.europeana.eu/concept/music/genre/Deathrock">
    <skos:prefLabel xml:lang="en">Deathrock</skos:prefLabel>
    <skos:prefLabel xml:lang="bg">Дет рок</skos:prefLabel>
    <skos:prefLabel xml:lang="da">Death rock</skos:prefLabel>
    <skos:prefLabel xml:lang="nl">Deathrock</skos:prefLabel>
    <skos:prefLabel xml:lang="fi">Deathrock</skos:prefLabel>
    <skos:prefLabel xml:lang="fr">Death rock</skos:prefLabel>
    <skos:prefLabel xml:lang="de">Death-Rock</skos:prefLabel>
    <skos:prefLabel xml:lang="it">Death rock</skos:prefLabel>
    <skos:prefLabel xml:lang="lt">Death Rock</skos:prefLabel>
    <skos:prefLabel xml:lang="no">Deathpunk</skos:prefLabel>
    <skos:prefLabel xml:lang="pl">Death rock</skos:prefLabel>
    <skos:prefLabel xml:lang="pt">Death rock</skos:prefLabel>
    <skos:prefLabel xml:lang="ru">Дэт-рок</skos:prefLabel>
    <skos:prefLabel xml:lang="sk">Deathrock</skos:prefLabel>
    <skos:prefLabel xml:lang="es">Deathrock</skos:prefLabel>
    <skos:prefLabel xml:lang="sv">Deathrock</skos:prefLabel>
    <skos:closeMatch rdf:resource="http://rdf.freebase.com/ns/m.0y2tr"/>
    <skos:broader rdf:resource="http://data.europeana.eu/concept/music/genre/Punk_rock_fusions"/>
    <skos:definition xml:lang="en">Deathrock is a sub-genre of punk rock incorporating horror
      elements and spooky atmospherics, that emerged on the West Coast of the United States in the
      early 1980s.</skos:definition>
    <skos:exactMatch xml:lang="en">http://dbpedia.org/resource/Deathrock</skos:exactMatch>
    <skos:inScheme rdf:resource="http://data.europeana.eu/concept/music/genre/Music_Genre_Scheme"/>
    <skos:altLabel xml:lang="en">Deathrock</skos:altLabel>
  </skos:Concept>

  <skos:Concept rdf:about="http://data.europeana.eu/concept/music/genre/Synthpop">
    <skos:prefLabel xml:lang="en">Synthpop</skos:prefLabel>
    <skos:prefLabel xml:lang="ar">سينثبوب</skos:prefLabel>
    <skos:prefLabel xml:lang="ca">Synthpop</skos:prefLabel>
    <skos:prefLabel xml:lang="hr">Synthpop</skos:prefLabel>
    <skos:prefLabel xml:lang="cs">Synthpop</skos:prefLabel>
    <skos:prefLabel xml:lang="da">Synthpop</skos:prefLabel>
    <skos:prefLabel xml:lang="nl">Synthipop</skos:prefLabel>
    <skos:prefLabel xml:lang="fi">Synthpop</skos:prefLabel>
    <skos:prefLabel xml:lang="fr">Synthpop</skos:prefLabel>
    <skos:prefLabel xml:lang="de">Synthie Pop</skos:prefLabel>
    <skos:prefLabel xml:lang="hu">Szintipop</skos:prefLabel>
    <skos:prefLabel xml:lang="it">Synth pop</skos:prefLabel>
    <skos:prefLabel xml:lang="ja">シンセポップ</skos:prefLabel>
    <skos:prefLabel xml:lang="ko">신스팝</skos:prefLabel>
    <skos:prefLabel xml:lang="lv">Sintpops</skos:prefLabel>
    <skos:prefLabel xml:lang="lt">Synthpop</skos:prefLabel>
    <skos:prefLabel xml:lang="no">Synthpop</skos:prefLabel>
    <skos:prefLabel xml:lang="fa">سینث‌پاپ</skos:prefLabel>
    <skos:prefLabel xml:lang="pl">Synth pop</skos:prefLabel>
    <skos:prefLabel xml:lang="pt">Synthpop</skos:prefLabel>
    <skos:prefLabel xml:lang="ro">Synthpop</skos:prefLabel>
    <skos:prefLabel xml:lang="ru">Синти-поп</skos:prefLabel>
    <skos:prefLabel xml:lang="sk">Synthpop</skos:prefLabel>
    <skos:prefLabel xml:lang="sl">Synthpop</skos:prefLabel>
    <skos:prefLabel xml:lang="es">Synth pop</skos:prefLabel>
    <skos:prefLabel xml:lang="sv">Syntpop</skos:prefLabel>
    <skos:prefLabel xml:lang="th">ซินธ์ป็อป</skos:prefLabel>
    <skos:prefLabel xml:lang="tr">Elektropop</skos:prefLabel>
    <skos:prefLabel xml:lang="uk">Синті-поп</skos:prefLabel>
    <skos:closeMatch rdf:resource="http://rdf.freebase.com/ns/m.0y3_8"/>
    <skos:broader rdf:resource="http://data.europeana.eu/concept/music/genre/Pop_music_fusions"/>
    <skos:definition xml:lang="en">Synthpop, a genre of popular music that first became prominent in
      the 1980s, features the synthesizer as the dominant musical instrument. It was prefigured in
      the 1960s and early 1970s by the use of synthesizers in progressive rock, electronic art rock,
      disco and particularly the &quot;Krautrock&quot; of bands like Kraftwerk. It arose as a
      distinct genre in Japan and the United Kingdom in the post-punk era as part of the new wave
      movement of the late-1970s to the mid-1980s. &lt;p&gt; Early synthpop pioneers included
      Japanese group Yellow Magic Orchestra and British bands Ultravox and The Human League, the
      latter largely used monophonic synthesizers to produce music with a simple and austere sound.
      After the breakthrough of Tubeway Army and Gary Numan in the British Singles Chart, large
      numbers of artists began to enjoy success with a synthesizer-based sound in the early 1980s,
      including Soft Cell, Orchestral Manoeuvres in the Dark and Depeche Mode in the United Kingdom,
      while in Japan, Yellow Magic Orchestra's success opened the way for synthpop bands such as
      P-Model, Plastics, and Hikashu.</skos:definition>
    <skos:exactMatch xml:lang="en">http://dbpedia.org/resource/Synthpop</skos:exactMatch>
    <skos:inScheme rdf:resource="http://data.europeana.eu/concept/music/genre/Music_Genre_Scheme"/>
    <skos:altLabel xml:lang="en">Electropop</skos:altLabel>
    <skos:altLabel xml:lang="en">Electro pop</skos:altLabel>
    <skos:altLabel xml:lang="en">Synthpop</skos:altLabel>
  </skos:Concept>

  <skos:Concept rdf:about="http://data.europeana.eu/concept/music/genre/Skate_punk">
    <skos:prefLabel xml:lang="en">Skate punk</skos:prefLabel>
    <skos:prefLabel xml:lang="ca">Skate punk</skos:prefLabel>
    <skos:prefLabel xml:lang="cs">Skate punk</skos:prefLabel>
    <skos:prefLabel xml:lang="nl">Skatepunk</skos:prefLabel>
    <skos:prefLabel xml:lang="fi">Skate punk</skos:prefLabel>
    <skos:prefLabel xml:lang="fr">Skate punk</skos:prefLabel>
    <skos:prefLabel xml:lang="de">Skatepunk</skos:prefLabel>
    <skos:prefLabel xml:lang="hu">Skate punk</skos:prefLabel>
    <skos:prefLabel xml:lang="it">Skate punk</skos:prefLabel>
    <skos:prefLabel xml:lang="no">Skate punk</skos:prefLabel>
    <skos:prefLabel xml:lang="pl">Skate punk</skos:prefLabel>
    <skos:prefLabel xml:lang="pt">Skate punk</skos:prefLabel>
    <skos:prefLabel xml:lang="ru">Скейт-панк</skos:prefLabel>
    <skos:prefLabel xml:lang="sk">Skate punk</skos:prefLabel>
    <skos:prefLabel xml:lang="es">Skate punk</skos:prefLabel>
    <skos:prefLabel xml:lang="sv">Skatepunk</skos:prefLabel>
    <skos:prefLabel xml:lang="uk">Скейт-панк</skos:prefLabel>
    <skos:closeMatch rdf:resource="http://rdf.freebase.com/ns/m.01hcvm"/>
    <skos:broader rdf:resource="http://data.europeana.eu/concept/music/genre/Punk_rock_fusions"/>
    <skos:definition xml:lang="en">Skate punk is a sub genre of punk rock, originally a derivative
      of the West Coast hardcore punk scene, that is named after its popularity among skateboarders
      and association with skateboarding culture. Skate punk most often describes the sound of
      melodic hardcore bands from the 1990s with an aggressive sound, and similar sounding modern
      bands. Skate videos have traditionally featured this aggressive style of punk rock. This
      played a big part in the coining of the term &quot;skate punk&quot;. Skate punk has gained
      popularity all around the world, including the Nardcore punk scene out of Oxnard,
      California.</skos:definition>
    <skos:exactMatch xml:lang="en">http://dbpedia.org/resource/Skate_punk</skos:exactMatch>
    <skos:inScheme rdf:resource="http://data.europeana.eu/concept/music/genre/Music_Genre_Scheme"/>
    <skos:altLabel xml:lang="en">Skate punk</skos:altLabel>
  </skos:Concept>

  <skos:Concept rdf:about="http://data.europeana.eu/concept/music/genre/Classical_music">
    <skos:prefLabel xml:lang="en">Classical music</skos:prefLabel>
    <skos:prefLabel xml:lang="ar">موسيقى كلاسيكية</skos:prefLabel>
    <skos:prefLabel xml:lang="bg">Класическа музика</skos:prefLabel>
    <skos:prefLabel xml:lang="ca">Música clàssica</skos:prefLabel>
    <skos:prefLabel xml:lang="hr">Klasična glazba</skos:prefLabel>
    <skos:prefLabel xml:lang="cs">Klasická hudba</skos:prefLabel>
    <skos:prefLabel xml:lang="da">Klassisk musik</skos:prefLabel>
    <skos:prefLabel xml:lang="nl">Klassieke muziek</skos:prefLabel>
    <skos:prefLabel xml:lang="et">Klassikaline muusika</skos:prefLabel>
    <skos:prefLabel xml:lang="fil">Musikang klasiko</skos:prefLabel>
    <skos:prefLabel xml:lang="fi">Taidemusiikki</skos:prefLabel>
    <skos:prefLabel xml:lang="fr">Musique classique</skos:prefLabel>
    <skos:prefLabel xml:lang="de">Klassische Musik</skos:prefLabel>
    <skos:prefLabel xml:lang="el">Κλασική μουσική</skos:prefLabel>
    <skos:prefLabel xml:lang="hi">शास्त्रीय संगीत</skos:prefLabel>
    <skos:prefLabel xml:lang="hu">Klasszikus zene</skos:prefLabel>
    <skos:prefLabel xml:lang="id">Musik klasik</skos:prefLabel>
    <skos:prefLabel xml:lang="it">Musica classica</skos:prefLabel>
    <skos:prefLabel xml:lang="ja">クラシック音楽</skos:prefLabel>
    <skos:prefLabel xml:lang="ko">고전 시대 음악</skos:prefLabel>
    <skos:prefLabel xml:lang="es-419">Música clásica</skos:prefLabel>
    <skos:prefLabel xml:lang="lv">Klasiskā mūzika</skos:prefLabel>
    <skos:prefLabel xml:lang="lt">Klasikinė muzika</skos:prefLabel>
    <skos:prefLabel xml:lang="ms">Muzik klasikal</skos:prefLabel>
    <skos:prefLabel xml:lang="no">Klassisk musikk</skos:prefLabel>
    <skos:prefLabel xml:lang="fa">موسیقی کلاسیک</skos:prefLabel>
    <skos:prefLabel xml:lang="pl">Muzyka poważna</skos:prefLabel>
    <skos:prefLabel xml:lang="pt">Música clássica</skos:prefLabel>
    <skos:prefLabel xml:lang="ro">Muzică clasică</skos:prefLabel>
    <skos:prefLabel xml:lang="ru">Классическая музыка</skos:prefLabel>
    <skos:prefLabel xml:lang="sr">Класична музика</skos:prefLabel>
    <skos:prefLabel xml:lang="sk">Klasická hudba</skos:prefLabel>
    <skos:prefLabel xml:lang="sl">Klasična glasba</skos:prefLabel>
    <skos:prefLabel xml:lang="es">Música clásica</skos:prefLabel>
    <skos:prefLabel xml:lang="sv">Klassisk musik</skos:prefLabel>
    <skos:prefLabel xml:lang="th">ดนตรีคลาสสิก</skos:prefLabel>
    <skos:prefLabel xml:lang="tr">Klasik müzik</skos:prefLabel>
    <skos:prefLabel xml:lang="uk">Класична музика</skos:prefLabel>
    <skos:prefLabel xml:lang="vi">Nhạc cổ điển</skos:prefLabel>
    <skos:closeMatch rdf:resource="http://rdf.freebase.com/ns/m.0ggq0m"/>
    <skos:broader rdf:resource="http://data.europeana.eu/concept/music/genre/Art_music"/>
    <skos:definition xml:lang="en">Classical music is art music produced or rooted in the traditions
      of Western music. It encompasses a broad period from roughly the 11th century to the present
      day. The central norms of this tradition became codified between 1550 and 1900, which is known
      as the common practice period. European music is largely distinguished from many other
      non-European and popular musical forms by its system of staff notation, in use since about the
      16th century. Western staff notation is used by composers to prescribe to the performer the
      pitch, speed, meter, individual rhythms and exact execution of a piece of music. This leaves
      less room for practices such as improvisation and ad libitum ornamentation, which are
      frequently heard in non-European art music and in popular music. The term &quot;classical
      music&quot; did not appear until the early 19th century, in an attempt to distinctly
      &quot;canonize&quot; the period from Johann Sebastian Bach to Beethoven as a golden age. The
      earliest reference to &quot;classical music&quot; recorded by the Oxford English Dictionary is
      from about 1836.</skos:definition>
    <skos:exactMatch xml:lang="en">http://dbpedia.org/resource/Classical_music</skos:exactMatch>
    <skos:inScheme rdf:resource="http://data.europeana.eu/concept/music/genre/Music_Genre_Scheme"/>
    <skos:altLabel xml:lang="en">Western art music</skos:altLabel>
    <skos:altLabel xml:lang="en">Classical music</skos:altLabel>
  </skos:Concept>

  <skos:Concept rdf:about="http://data.europeana.eu/concept/music/genre/Doina">
    <skos:prefLabel xml:lang="en">Doina</skos:prefLabel>
    <skos:prefLabel xml:lang="bg">Дойна</skos:prefLabel>
    <skos:prefLabel xml:lang="hr">Doina</skos:prefLabel>
    <skos:prefLabel xml:lang="nl">Doina</skos:prefLabel>
    <skos:prefLabel xml:lang="ko">도이나</skos:prefLabel>
    <skos:prefLabel xml:lang="lt">Doina</skos:prefLabel>
    <skos:prefLabel xml:lang="pt">Doina</skos:prefLabel>
    <skos:prefLabel xml:lang="ro">Doină</skos:prefLabel>
    <skos:prefLabel xml:lang="ru">Дойна</skos:prefLabel>
    <skos:prefLabel xml:lang="es">Doină</skos:prefLabel>
    <skos:closeMatch rdf:resource="http://rdf.freebase.com/ns/m.04qv9g"/>
    <skos:broader rdf:resource="http://data.europeana.eu/concept/music/genre/Folk_music_traditional"/>
    <skos:definition xml:lang="en">The Doina is a Romanian musical tune style, possibly with Middle
      Eastern roots, customary in Romanian peasant music, as well as in Lăutărească. It was also
      adopted into Klezmer music. Similar tunes are found throughout Eastern Europe and the Balkans.
      In some parts of the Balkans this kind of music is referred to as scaros or
      scaru.</skos:definition>
    <skos:exactMatch xml:lang="en">http://dbpedia.org/resource/Doina</skos:exactMatch>
    <skos:inScheme rdf:resource="http://data.europeana.eu/concept/music/genre/Music_Genre_Scheme"/>
    <skos:altLabel xml:lang="en">Doina</skos:altLabel>
  </skos:Concept>

  <skos:Concept
    rdf:about="http://data.europeana.eu/concept/music/genre/Latin_American_music_traditional">
    <skos:prefLabel xml:lang="en">Traditional Latin American music</skos:prefLabel>
    <skos:prefLabel xml:lang="ar">الموسيقى اللاتينية</skos:prefLabel>
    <skos:prefLabel xml:lang="ca">Música llatinoamericana</skos:prefLabel>
    <skos:prefLabel xml:lang="cs">Latinskoamerická hudba</skos:prefLabel>
    <skos:prefLabel xml:lang="nl">Latijns-Amerikaanse muziek</skos:prefLabel>
    <skos:prefLabel xml:lang="fi">Latinalaisamerikkalainen musiikki</skos:prefLabel>
    <skos:prefLabel xml:lang="fr">Musique latine</skos:prefLabel>
    <skos:prefLabel xml:lang="de">Lateinamerikanische Musik</skos:prefLabel>
    <skos:prefLabel xml:lang="hu">Latin zene</skos:prefLabel>
    <skos:prefLabel xml:lang="it">Musica latina</skos:prefLabel>
    <skos:prefLabel xml:lang="ja">ラテン音楽</skos:prefLabel>
    <skos:prefLabel xml:lang="ko">라틴 아메리카의 음악</skos:prefLabel>
    <skos:prefLabel xml:lang="pl">Muzyka latynoamerykańska</skos:prefLabel>
    <skos:prefLabel xml:lang="pt">Música da América Latina</skos:prefLabel>
    <skos:prefLabel xml:lang="ro">Muzică latino</skos:prefLabel>
    <skos:prefLabel xml:lang="ru">Латиноамериканская музыка</skos:prefLabel>
    <skos:prefLabel xml:lang="es">Música de América Latina</skos:prefLabel>
    <skos:prefLabel xml:lang="sv">Latinamerikansk musik</skos:prefLabel>
    <skos:prefLabel xml:lang="uk">Латиноамериканська музика</skos:prefLabel>
    <skos:prefLabel xml:lang="vi">Nhạc Mỹ Latinh</skos:prefLabel>
    <skos:prefLabel xml:lang="en">Popular Latin American</skos:prefLabel>
    <skos:closeMatch rdf:resource="http://rdf.freebase.com/ns/m.0g293"/>
    <skos:broader rdf:resource="http://data.europeana.eu/concept/music/genre/World_music"/>
    <skos:definition xml:lang="en">Traditional music from Latin America</skos:definition>
    <skos:exactMatch xml:lang="en"
      >http://dbpedia.org/resource/Latin_American_music</skos:exactMatch>
    <skos:inScheme rdf:resource="http://data.europeana.eu/concept/music/genre/Music_Genre_Scheme"/>
    <skos:altLabel xml:lang="en">Latin American music</skos:altLabel>
    <skos:altLabel xml:lang="en">Latin music</skos:altLabel>
  </skos:Concept>

  <skos:Concept
    rdf:about="http://data.europeana.eu/concept/music/genre/Latin_American_music_popular">
    <skos:prefLabel xml:lang="en">Popular Latin American</skos:prefLabel>
    <skos:closeMatch rdf:resource="http://rdf.freebase.com/ns/m.0g293"/>
    <skos:broader rdf:resource="http://data.europeana.eu/concept/music/genre/Popular_music"/>
    <skos:definition xml:lang="en">Popular music from Latin America</skos:definition>
    <skos:exactMatch xml:lang="en"
      >http://dbpedia.org/resource/Latin_American_music</skos:exactMatch>
    <skos:inScheme rdf:resource="http://data.europeana.eu/concept/music/genre/Music_Genre_Scheme"/>
  </skos:Concept>

  <skos:Concept rdf:about="http://data.europeana.eu/concept/music/genre/Americana_popular">
    <skos:prefLabel xml:lang="en">Americana</skos:prefLabel>
    <skos:closeMatch rdf:resource="https://www.freebase.com/m/09n5t_"/>
    <skos:broader rdf:resource="http://data.europeana.eu/concept/music/genre/Popular_music"/>
    <skos:definition xml:lang="en">Popular music originated from north America</skos:definition>
    <skos:exactMatch xml:lang="en">http://dbpedia.org/resource/Americana#popular</skos:exactMatch>
    <skos:inScheme rdf:resource="http://data.europeana.eu/concept/music/genre/Music_Genre_Scheme"/>
  </skos:Concept>

  <skos:Concept rdf:about="http://data.europeana.eu/concept/music/genre/Folk_music_traditional">
    <skos:prefLabel xml:lang="en">Traditional European Folk</skos:prefLabel>
    <skos:closeMatch rdf:resource="http://rdf.freebase.com/ns/m.02w4v"/>
    <skos:broader rdf:resource="http://data.europeana.eu/concept/music/genre/World_music"/>
    <skos:definition xml:lang="en">Traditional folk music has been defined in several ways: as music
      transmitted by mouth, as music of the lower classes, and as music with unknown composers. It
      has been contrasted with commercial and classical styles. One meaning often given is that of
      old songs, with no known composers; another is music that has been transmitted and evolved by
      a process of oral transmission or performed by custom over a long period of
      time.</skos:definition>
    <skos:broadMatch rdf:resource="http://dbpedia.org/resource/Folk_music"/>
    <skos:exactMatch xml:lang="en">http://dbpedia.org/resource/Folk_music</skos:exactMatch>
    <skos:inScheme rdf:resource="http://data.europeana.eu/concept/music/genre/Music_Genre_Scheme"/>
  </skos:Concept>

  <skos:Concept rdf:about="http://data.europeana.eu/concept/music/genre/Music_of_Asia_traditional">
    <skos:prefLabel xml:lang="en">Traditional Asian</skos:prefLabel>
    <skos:prefLabel xml:lang="ar">موسيقى آسيا</skos:prefLabel>
    <skos:prefLabel xml:lang="fr">Musique asiatique</skos:prefLabel>
    <skos:prefLabel xml:lang="ko">아시아의 음악</skos:prefLabel>
    <skos:closeMatch rdf:resource="http://rdf.freebase.com/ns/m.028sqc"/>
    <skos:broader rdf:resource="http://data.europeana.eu/concept/music/genre/World_music"/>
    <skos:definition xml:lang="en">Traditional Asian music encompasses numerous different musical
      styles originating from a large number of Asian countries. Musical traditions in Asia Music of
      Central Asia Music of Afghanistan Music of Azerbaijan Music of Kazakhstan Music of Mongolia
      Music of Uzbekistan Music of East Asia Music of China Music of Hong Kong Music of Japan Music
      of Korea Music of Taiwan Music of South Asia Asian Music of Bangladesh Music of Bhutan Music
      of India Ravanahatha Music of Nepal Music of Iran Music of Pakistan Music of Sri Lanka Music
      of Southeast Asia Music of Indonesia Music of Malaysia Music of Vietnam Music of Thailand
      Music of the Philippines Music of West Asia Arabic music Music of Bahrain Music of Jordan
      Music of Lebanon Music of Saudi Arabia Music of the United Arab Emirates Music of Yemen
      Assyrian/Syriac folk music Kurdish music Music of Cyprus Music of Iran Music of Iraq Music of
      Israel Jewish music Music of Palestine Music of Syria Music of Turkey</skos:definition>
    <skos:broadMatch rdf:resource="http://dbpedia.org/resource/Music_of_Asia"/>
    <skos:inScheme rdf:resource="http://data.europeana.eu/concept/music/genre/Music_Genre_Scheme"/>
    <skos:altLabel xml:lang="en">Music of Asia</skos:altLabel>
  </skos:Concept>

  <skos:Concept rdf:about="http://data.europeana.eu/concept/music/genre/Music_of_Ecuador_Pasacalle">
    <skos:prefLabel xml:lang="en">Pasacalle</skos:prefLabel>
    <skos:broader
      rdf:resource="http://data.europeana.eu/concept/music/genre/Latin_American_music_traditional"/>
    <skos:definition xml:lang="en">The music of Ecuador has a long history. Pasillo is a genre of
      indigenous Latin music. In Ecuador it is the &quot;national genre of music.&quot; Through the
      years, many cultures have brought their influences together to create new types of music.
      There are also different kinds of traditional music like albazo, pasacalle, fox incaico,
      tonada, diablada pillareña, capishca, Bomba</skos:definition>
    <skos:broadMatch rdf:resource="http://dbpedia.org/resource/Music_of_Ecuador#Pasacalle"/>
    <skos:inScheme rdf:resource="http://data.europeana.eu/concept/music/genre/Music_Genre_Scheme"/>
  </skos:Concept>

  <skos:Concept
    rdf:about="http://data.europeana.eu/concept/music/genre/Latin_American_music_fusions">
    <skos:prefLabel xml:lang="en">Latin American fusions</skos:prefLabel>
    <skos:closeMatch rdf:resource="http://rdf.freebase.com/ns/m.0g293"/>
    <skos:broader rdf:resource="http://data.europeana.eu/concept/music/genre/Fusion_(music)_fusions"/>
    <skos:definition xml:lang="en">Fusion genres based on Latin American music</skos:definition>
    <skos:broadMatch rdf:resource="http://dbpedia.org/resource/Latin_American_music"/>
    <skos:inScheme rdf:resource="http://data.europeana.eu/concept/music/genre/Music_Genre_Scheme"/>
  </skos:Concept>

  <skos:Concept rdf:about="http://data.europeana.eu/concept/music/genre/Concert">
    <skos:prefLabel xml:lang="en">Concert</skos:prefLabel>
    <skos:prefLabel xml:lang="ar">حفلة موسيقية</skos:prefLabel>
    <skos:prefLabel xml:lang="bg">Концерт</skos:prefLabel>
    <skos:prefLabel xml:lang="ca">Concert</skos:prefLabel>
    <skos:prefLabel xml:lang="hr">Koncert</skos:prefLabel>
    <skos:prefLabel xml:lang="cs">Koncert</skos:prefLabel>
    <skos:prefLabel xml:lang="da">Koncert</skos:prefLabel>
    <skos:prefLabel xml:lang="nl">Concert</skos:prefLabel>
    <skos:prefLabel xml:lang="et">Kontsert</skos:prefLabel>
    <skos:prefLabel xml:lang="fi">Konsertti</skos:prefLabel>
    <skos:prefLabel xml:lang="fr">Concert</skos:prefLabel>
    <skos:prefLabel xml:lang="de">Konzert</skos:prefLabel>
    <skos:prefLabel xml:lang="el">Συναυλία</skos:prefLabel>
    <skos:prefLabel xml:lang="hu">Hangverseny</skos:prefLabel>
    <skos:prefLabel xml:lang="id">Konser</skos:prefLabel>
    <skos:prefLabel xml:lang="it">Concerto</skos:prefLabel>
    <skos:prefLabel xml:lang="ja">演奏会</skos:prefLabel>
    <skos:prefLabel xml:lang="ko">연주회</skos:prefLabel>
    <skos:prefLabel xml:lang="lv">Koncerts</skos:prefLabel>
    <skos:prefLabel xml:lang="lt">Koncertas</skos:prefLabel>
    <skos:prefLabel xml:lang="no">Konsert</skos:prefLabel>
    <skos:prefLabel xml:lang="fa">کنسرت موسیقی</skos:prefLabel>
    <skos:prefLabel xml:lang="pl">Koncert</skos:prefLabel>
    <skos:prefLabel xml:lang="pt">concerto</skos:prefLabel>
    <skos:prefLabel xml:lang="ro">Concert</skos:prefLabel>
    <skos:prefLabel xml:lang="ru">Концерт</skos:prefLabel>
    <skos:prefLabel xml:lang="sr">Концерт</skos:prefLabel>
    <skos:prefLabel xml:lang="sk">Koncert</skos:prefLabel>
    <skos:prefLabel xml:lang="sl">Koncert</skos:prefLabel>
    <skos:prefLabel xml:lang="es">Concierto</skos:prefLabel>
    <skos:prefLabel xml:lang="sv">Konsert</skos:prefLabel>
    <skos:prefLabel xml:lang="th">คอนเสิร์ต</skos:prefLabel>
    <skos:prefLabel xml:lang="tr">Konser</skos:prefLabel>
    <skos:prefLabel xml:lang="uk">Концерт</skos:prefLabel>
    <skos:prefLabel xml:lang="vi">Buổi hoà nhạc</skos:prefLabel>
    <skos:closeMatch rdf:resource="http://rdf.freebase.com/ns/m.01jddz"/>
    <skos:broader rdf:resource="http://data.europeana.eu/concept/music/genre/Fusion_(music)_fusions"/>
    <skos:definition xml:lang="en">A concert is a live performance of music before an audience. The
      performance may be by a single musician, sometimes then called a recital, or by a musical
      ensemble, such as an orchestra, a choir, or a musical band. Concerts are held in a wide
      variety and size of settings, from private houses and small nightclubs, dedicated concert
      halls, entertainment centres and parks to large multipurpose buildings, and even sports
      stadiums. Indoor concerts held in the largest venues are sometimes called &quot;arena
      concerts&quot; or &quot;amphitheatre concerts&quot;. Regardless of the venue, musicians
      usually perform on a stage. Concerts often require live event support with professional audio
      equipment. Before recorded music, concerts would provide the only opportunity one would
      generally have to hear musicians play. Informal names for a concert include &quot;show&quot;
      and &quot;gig&quot;</skos:definition>
    <skos:inScheme rdf:resource="http://data.europeana.eu/concept/music/genre/Music_Genre_Scheme"/>
    <skos:altLabel xml:lang="en">Concert tour</skos:altLabel>
    <skos:altLabel xml:lang="en">Concert</skos:altLabel>
  </skos:Concept>

  <skos:Concept rdf:about="http://data.europeana.eu/concept/music/genre/African_popular_music">
    <skos:prefLabel xml:lang="en">Afropop</skos:prefLabel>
    <skos:closeMatch rdf:resource="http://rdf.freebase.com/ns/m.02p4l6s"/>
    <skos:broader rdf:resource="http://data.europeana.eu/concept/music/genre/Popular_music"/>
    <skos:definition xml:lang="en">African popular music, like African traditional music, is vast
      and varied. Most contemporary genres of African popular music build on cross-pollination with
      western popular music. Many genres of popular music like blues, jazz, salsa, zouk, and rumba
      derive to varying degrees on musical traditions from Africa, taken to the Americas by African
      slaves. These rhythms and sounds have subsequently been adapted by newer genres like rock, and
      rhythm and blues. Likewise, African popular music has adopted elements, particularly the
      musical instruments and recording studio techniques of western music</skos:definition>
    <skos:exactMatch xml:lang="en"
      >http://dbpedia.org/resource/African_popular_music</skos:exactMatch>
    <skos:inScheme rdf:resource="http://data.europeana.eu/concept/music/genre/Music_Genre_Scheme"/>
  </skos:Concept>

  <rdf:Description rdf:about="http://data.europeana.eu/concept/music/genre/dup_Jazz_fusion">
    <skos:altLabel xml:lang="en">Fusion</skos:altLabel>
    <skos:altLabel xml:lang="en">Jazz fusion</skos:altLabel>
    <skos:prefLabel xml:lang="en">Jazz fusion</skos:prefLabel>
    <skos:prefLabel xml:lang="bg">Джаз рок</skos:prefLabel>
    <skos:prefLabel xml:lang="ca">Jazz fusió</skos:prefLabel>
    <skos:prefLabel xml:lang="hr">Jazz fuzija</skos:prefLabel>
    <skos:prefLabel xml:lang="cs">Jazz fusion</skos:prefLabel>
    <skos:prefLabel xml:lang="da">Jazz fusion</skos:prefLabel>
    <skos:prefLabel xml:lang="nl">Fusion</skos:prefLabel>
    <skos:prefLabel xml:lang="et">Jazz fusion</skos:prefLabel>
    <skos:prefLabel xml:lang="fi">Fuusiojazz</skos:prefLabel>
    <skos:prefLabel xml:lang="fr">Jazz-rock fusion</skos:prefLabel>
    <skos:prefLabel xml:lang="de">Fusion</skos:prefLabel>
    <skos:prefLabel xml:lang="hu">Fúziós jazz</skos:prefLabel>
    <skos:prefLabel xml:lang="id">Fusion jazz</skos:prefLabel>
    <skos:prefLabel xml:lang="it">Fusion</skos:prefLabel>
    <skos:prefLabel xml:lang="ja">フュージョン</skos:prefLabel>
    <skos:prefLabel xml:lang="ko">재즈 록</skos:prefLabel>
    <skos:prefLabel xml:lang="lv">Džezroks</skos:prefLabel>
    <skos:prefLabel xml:lang="lt">Jazz fusion</skos:prefLabel>
    <skos:prefLabel xml:lang="no">Jazz-Fusion</skos:prefLabel>
    <skos:prefLabel xml:lang="fa">جز فیوژن</skos:prefLabel>
    <skos:prefLabel xml:lang="pl">Jazz-rock</skos:prefLabel>
    <skos:prefLabel xml:lang="pt">Jazz fusion</skos:prefLabel>
    <skos:prefLabel xml:lang="ro">Jazz fusion</skos:prefLabel>
    <skos:prefLabel xml:lang="ru">Джаз-фьюжн</skos:prefLabel>
    <skos:prefLabel xml:lang="sr">Џез фузија</skos:prefLabel>
    <skos:prefLabel xml:lang="sl">Jazz fusion</skos:prefLabel>
    <skos:prefLabel xml:lang="es">Jazz fusión</skos:prefLabel>
    <skos:prefLabel xml:lang="th">แจ๊สฟิวชัน</skos:prefLabel>
    <skos:prefLabel xml:lang="uk">Джаз-рок</skos:prefLabel>
    <skos:prefLabel xml:lang="en">Jazz Rock</skos:prefLabel>
  </rdf:Description>

  <rdf:Description rdf:about="http://data.europeana.eu/concept/music/genre/dup_Ballad">
    <skos:altLabel xml:lang="en">Ballad</skos:altLabel>
    <skos:prefLabel xml:lang="en">Balada</skos:prefLabel>
    <skos:prefLabel xml:lang="ar">بالاد</skos:prefLabel>
    <skos:prefLabel xml:lang="bg">Балада</skos:prefLabel>
    <skos:prefLabel xml:lang="ca">Balada</skos:prefLabel>
    <skos:prefLabel xml:lang="hr">Balada</skos:prefLabel>
    <skos:prefLabel xml:lang="cs">Balada</skos:prefLabel>
    <skos:prefLabel xml:lang="da">Ballade</skos:prefLabel>
    <skos:prefLabel xml:lang="nl">Ballade</skos:prefLabel>
    <skos:prefLabel xml:lang="et">Ballaad</skos:prefLabel>
    <skos:prefLabel xml:lang="fil">Balada</skos:prefLabel>
    <skos:prefLabel xml:lang="fi">Balladi</skos:prefLabel>
    <skos:prefLabel xml:lang="fr">Ballade</skos:prefLabel>
    <skos:prefLabel xml:lang="de">Ballade</skos:prefLabel>
    <skos:prefLabel xml:lang="hu">Ballada</skos:prefLabel>
    <skos:prefLabel xml:lang="id">Musik balada</skos:prefLabel>
    <skos:prefLabel xml:lang="it">Ballata popolare</skos:prefLabel>
    <skos:prefLabel xml:lang="ja">バラッド</skos:prefLabel>
    <skos:prefLabel xml:lang="ko">발라드</skos:prefLabel>
    <skos:prefLabel xml:lang="lv">Balāde</skos:prefLabel>
    <skos:prefLabel xml:lang="lt">Baladė</skos:prefLabel>
    <skos:prefLabel xml:lang="no">Ballade</skos:prefLabel>
    <skos:prefLabel xml:lang="fa">تصنیف</skos:prefLabel>
    <skos:prefLabel xml:lang="pl">Ballada</skos:prefLabel>
    <skos:prefLabel xml:lang="pt">Balada</skos:prefLabel>
    <skos:prefLabel xml:lang="ro">Baladă</skos:prefLabel>
    <skos:prefLabel xml:lang="ru">Баллада</skos:prefLabel>
    <skos:prefLabel xml:lang="sk">Balada</skos:prefLabel>
    <skos:prefLabel xml:lang="sl">Balada</skos:prefLabel>
    <skos:prefLabel xml:lang="es">Balada</skos:prefLabel>
    <skos:prefLabel xml:lang="sv">Ballad</skos:prefLabel>
    <skos:prefLabel xml:lang="th">บัลลาด</skos:prefLabel>
    <skos:prefLabel xml:lang="tr">Balad</skos:prefLabel>
    <skos:prefLabel xml:lang="uk">Балада</skos:prefLabel>
    <skos:prefLabel xml:lang="vi">Ballad</skos:prefLabel>
    <skos:prefLabel xml:lang="en">Ballad</skos:prefLabel>
  </rdf:Description>

</rdf:RDF>
